@prefix : <http://purl.allotrope.org/voc/afo/domain/WD/2025/06/capillary-electrophoresis#> .
@prefix bfo: <http://purl.obolibrary.org/obo/BFO> .
@prefix dct: <http://purl.org/dc/terms/> .
@prefix owl: <http://www.w3.org/2002/07/owl#> .
@prefix rdf: <http://www.w3.org/1999/02/22-rdf-syntax-ns#> .
@prefix xml: <http://www.w3.org/XML/1998/namespace> .
@prefix xsd: <http://www.w3.org/2001/XMLSchema#> .
@prefix af-c: <http://purl.allotrope.org/ontologies/common#> .
@prefix af-e: <http://purl.allotrope.org/ontologies/equipment#> .
@prefix af-m: <http://purl.allotrope.org/ontologies/material#> .
@prefix af-p: <http://purl.allotrope.org/ontologies/process#> .
@prefix af-q: <http://purl.allotrope.org/ontologies/quality#> .
@prefix af-r: <http://purl.allotrope.org/ontologies/result#> .
@prefix af-x: <http://purl.allotrope.org/ontologies/property#> .
@prefix rdfs: <http://www.w3.org/2000/01/rdf-schema#> .
@prefix skos: <http://www.w3.org/2004/02/skos/core#> .
@prefix af-cur: <http://purl.allotrope.org/ontologies/curation#> .
@base <http://purl.allotrope.org/voc/afo/domain/WD/2025/06/capillary-electrophoresis#> .

<http://purl.allotrope.org/voc/afo/domain/WD/2025/06/capillary-electrophoresis> rdf:type owl:Ontology ;
                                                                                           owl:versionIRI <http://purl.allotrope.org/voc/afo/domain/WD/2025/06/capillary-electrophoresis> ;
                                                                                           owl:imports <http://purl.allotrope.org/voc/afo/WD/2025/06/afo> ,
                                                                                                       <http://purl.allotrope.org/voc/afo/domain/WD/2025/06/electrophoresis> ;
                                                                                           dct:issued "2025-06-25T12:00:00Z"^^xsd:dateTime ;
                                                                                           dct:license <http://purl.allotrope.org/voc/creative-commons-attribution-license> ;
                                                                                           dct:modified "2025-04-04T12:00:00Z"^^xsd:dateTime ;
                                                                                           dct:rights <http://purl.allotrope.org/voc/attribution> ,
                                                                                                      <http://purl.allotrope.org/voc/copyright> ;
                                                                                           dct:title "AFO Capillary Electrophoresis Domain Ontology (WD/2025/06)" ;
                                                                                           owl:priorVersion <http://purl.allotrope.org/voc/afo/domain/WD/2018/11/capillary-electrophoresis> ;
                                                                                           owl:versionInfo "WD/2025/06" .

#################################################################
#    Annotation properties
#################################################################

###  http://purl.allotrope.org/ontologies/property#AFX_0002796
af-x:AFX_0002796 rdf:type owl:AnnotationProperty .


###  http://purl.allotrope.org/ontologies/property#AFX_0002798
af-x:AFX_0002798 rdf:type owl:AnnotationProperty .


###  http://purl.allotrope.org/ontologies/property#AFX_0002809
af-x:AFX_0002809 rdf:type owl:AnnotationProperty .


###  http://purl.org/dc/terms/source
dct:source rdf:type owl:AnnotationProperty .


###  http://www.w3.org/2004/02/skos/core#altLabel
skos:altLabel rdf:type owl:AnnotationProperty .


###  http://www.w3.org/2004/02/skos/core#changeNote
skos:changeNote rdf:type owl:AnnotationProperty .


###  http://www.w3.org/2004/02/skos/core#definition
skos:definition rdf:type owl:AnnotationProperty .


###  http://www.w3.org/2004/02/skos/core#example
skos:example rdf:type owl:AnnotationProperty .


###  http://www.w3.org/2004/02/skos/core#note
skos:note rdf:type owl:AnnotationProperty .


###  http://www.w3.org/2004/02/skos/core#prefLabel
skos:prefLabel rdf:type owl:AnnotationProperty .


###  http://www.w3.org/2004/02/skos/core#scopeNote
skos:scopeNote rdf:type owl:AnnotationProperty .


#################################################################
#    Object Properties
#################################################################

###  http://purl.allotrope.org/ontologies/property#AFX_0000072
af-x:AFX_0000072 rdf:type owl:ObjectProperty .


###  http://purl.allotrope.org/ontologies/property#AFX_0000107
af-x:AFX_0000107 rdf:type owl:ObjectProperty ;
                 rdfs:subPropertyOf af-x:AFX_0000072 ;
                 skos:definition "The period of time for the ramp of rinsing voltage. [Allotrope]" ;
                 skos:prefLabel "capillary rinsing voltage ramp duration" .


###  http://purl.allotrope.org/ontologies/property#AFX_0000108
af-x:AFX_0000108 rdf:type owl:ObjectProperty ;
                 rdfs:subPropertyOf af-x:AFX_0000072 ;
                 skos:altLabel "separation time" ;
                 skos:definition "The period of time used for the separation. The separation time must be longer than the migration time in order to effectively separate the migrating compounds. [Allotrope]" ;
                 skos:prefLabel "capillary electrophoresis separation time" .


###  http://purl.allotrope.org/ontologies/property#AFX_0000109
af-x:AFX_0000109 rdf:type owl:ObjectProperty ;
                 rdfs:subPropertyOf af-x:AFX_0000072 ;
                 skos:altLabel "migration time" ;
                 skos:definition "The capillary electrophoresis migration time is the time taken by a solute to travel from the inlet of the capillary to the detection region, calculated from dividing the effective capillary length by the velocity. [Allotrope]" ;
                 skos:prefLabel "capillary electrophoresis migration time" .


#################################################################
#    Classes
#################################################################

###  http://purl.allotrope.org/ontologies/equipment#AFE_0000063
af-e:AFE_0000063 rdf:type owl:Class ;
                 rdfs:subClassOf af-e:AFE_0000549 ;
                 af-x:AFX_0002798 "true"^^xsd:boolean ;
                 skos:definition "A teflon capillary is a neutral capillary with a teflon coating on its inner surface. [Allotrope]" ;
                 skos:prefLabel "teflon capillary" .


###  http://purl.allotrope.org/ontologies/equipment#AFE_0000232
af-e:AFE_0000232 rdf:type owl:Class ;
                 rdfs:subClassOf af-e:AFE_0000659 ;
                 af-x:AFX_0002798 "true"^^xsd:boolean ;
                 skos:altLabel "bare silica capillary" ,
                               "uncoated silica capillary" ;
                 skos:definition "A bare fused silica capillary has no coatings on its inner or outer surface. [Allotrope]" ;
                 skos:prefLabel "bare fused silica capillary" .


###  http://purl.allotrope.org/ontologies/equipment#AFE_0000549
af-e:AFE_0000549 rdf:type owl:Class ;
                 rdfs:subClassOf af-e:AFE_0000340 ;
                 af-x:AFX_0002798 "true"^^xsd:boolean ;
                 skos:definition "A neutral capillary is one that contains no anchor groups to neither anions nor cations. [Allotrope]" ;
                 skos:prefLabel "neutral capillary" .


###  http://purl.allotrope.org/ontologies/equipment#AFE_0000600
af-e:AFE_0000600 rdf:type owl:Class ;
                 rdfs:subClassOf af-e:AFE_0000659 ;
                 af-x:AFX_0002798 "true"^^xsd:boolean ;
                 skos:altLabel "capillary gel column" ;
                 skos:definition "A gel filled capillary is a separation capillary that contains a gel as stationary phase. [Allotrope]" ;
                 skos:prefLabel "gel filled capillary" .


###  http://purl.allotrope.org/ontologies/equipment#AFE_0000659
af-e:AFE_0000659 rdf:type owl:Class ;
                 rdfs:subClassOf af-e:AFE_0000340 ;
                 af-x:AFX_0002798 "true"^^xsd:boolean ;
                 skos:definition "A fused silica capillary is a separation capillary that consists of silica in amophous form. [Allotrope]" ;
                 skos:prefLabel "fused silica capillary" .


###  http://purl.allotrope.org/ontologies/equipment#AFE_0000868
af-e:AFE_0000868 rdf:type owl:Class ;
                 rdfs:subClassOf af-e:AFE_0000340 ;
                 af-x:AFX_0002798 "true"^^xsd:boolean ;
                 skos:altLabel "functionalized capillary" ;
                 skos:definition "A functionalized capillary is a separation capillary that has a functionalized coating on its inner surface. [Allotrope]" ;
                 skos:prefLabel "coated capillary" .


###  http://purl.allotrope.org/ontologies/material#AFM_0000083
af-m:AFM_0000083 rdf:type owl:Class ;
                 rdfs:subClassOf af-m:AFM_0000053 ;
                 skos:altLabel "BGE" ;
                 skos:definition "The background electrolyte is the running material used in capillary electrophoresis. [Allotrope]" ;
                 skos:prefLabel "background electrolyte" .


###  http://purl.allotrope.org/ontologies/material#AFM_0000144
af-m:AFM_0000144 rdf:type owl:Class ;
                 rdfs:subClassOf af-m:AFM_0000012 ;
                 skos:altLabel "conditioner solution" ;
                 skos:definition "A capillary conditioner is a solution that is used for rinsing a capillary in order to generate a fresh state. [Allotrope]" ;
                 skos:prefLabel "capillary conditioner" .


###  http://purl.allotrope.org/ontologies/material#AFM_0000204
af-m:AFM_0000204 rdf:type owl:Class ;
                 rdfs:subClassOf af-m:AFM_0000921 ;
                 af-x:AFX_0002798 "true"^^xsd:boolean ;
                 skos:definition "Carrier ampholytes are zwitterionic compounds that are used for the creation of pH gradients within the capillary of capillary electrophoresis. [Allotrope]" ;
                 skos:prefLabel "carrier ampholyte" .


###  http://purl.allotrope.org/ontologies/material#AFM_0000274
af-m:AFM_0000274 rdf:type owl:Class ;
                 rdfs:subClassOf af-m:AFM_0000348 ;
                 af-x:AFX_0002796 af-r:AFR_0001223 ;
                 skos:definition "Chemical gel is a material which changes physical state by forming covalent attachments when mixed in an aqueous solution. [Allotrope]" ;
                 skos:prefLabel "chemical gel" .


###  http://purl.allotrope.org/ontologies/material#AFM_0000307
af-m:AFM_0000307 rdf:type owl:Class ;
                 rdfs:subClassOf af-m:AFM_0000053 ;
                 af-x:AFX_0002798 "true"^^xsd:boolean ;
                 skos:definition "A leading electrolyte refers to an ionic analyte which is travelling at a faster rate than other analytes in a separation technique. [Allotrope]" ;
                 skos:prefLabel "leading electrolyte" .


###  http://purl.allotrope.org/ontologies/material#AFM_0000348
af-m:AFM_0000348 rdf:type owl:Class ;
                 rdfs:subClassOf af-m:AFM_0001033 ;
                 af-x:AFX_0002796 af-r:AFR_0001223 ;
                 skos:definition "A capillary electrophoresis gel is a polymer network used in an electrophoresis process. [Allotrope]" ;
                 skos:example "uncrosslinked polyacrylamide, methylcellulose" ;
                 skos:prefLabel "capillary electrophoresis gel" .


###  http://purl.allotrope.org/ontologies/material#AFM_0000349
af-m:AFM_0000349 rdf:type owl:Class ;
                 rdfs:subClassOf af-m:AFM_0000348 ;
                 af-x:AFX_0002796 af-r:AFR_0001223 ;
                 skos:definition "Physical gels are materials which obtain their crosslinking through a form of polymer entanglement, this usually requires  heat input, and the gel settles into place as it cools. [Allotrope]" ;
                 skos:prefLabel "physical gel" .


###  http://purl.allotrope.org/ontologies/material#AFM_0000921
af-m:AFM_0000921 rdf:type owl:Class .


###  http://purl.allotrope.org/ontologies/process#AFP_0000092
af-p:AFP_0000092 rdf:type owl:Class ;
                 rdfs:subClassOf af-p:AFP_0000474 ,
                                 af-p:AFP_0002364 ;
                 skos:altLabel "ACE" ,
                               "CAE" ;
                 skos:definition "An electrophoresis method which takes place in a capillary where the separation medium has specific interactions with the analytes. [CHMO]" ;
                 skos:prefLabel "capillary affinity electrophoresis" .


###  http://purl.allotrope.org/ontologies/process#AFP_0000918
af-p:AFP_0000918 rdf:type owl:Class ;
                 rdfs:subClassOf af-p:AFP_0000669 ;
                 skos:definition "A capillary array electrophoresis uses many capillaries at the same time allowing many analyses at the same time. [Allotrope]" ;
                 skos:prefLabel "capillary array electrophoresis" .


###  http://purl.allotrope.org/ontologies/process#AFP_0001155
af-p:AFP_0001155 rdf:type owl:Class ;
                 rdfs:subClassOf bfo:_0000015 ;
                 skos:altLabel "capillary regeneration" ;
                 skos:definition "Process by which the material of the capillary is treated to result in a uniform charge throughout the surface. [Allotrope]" ;
                 skos:example "Pretreat the capillary for 10 min with 0.1 M sodium hydroxide, 5 min with water, and 10 min with run buffer." ;
                 skos:prefLabel "capillary conditioning" .


###  http://purl.allotrope.org/ontologies/process#AFP_0001165
af-p:AFP_0001165 rdf:type owl:Class ;
                 rdfs:subClassOf af-p:AFP_0000268 ,
                                 af-p:AFP_0000474 ;
                 skos:altLabel "CSE" ;
                 skos:definition "An electrophoresis method that takes place in a capillary and where the separation medium contains a reticulated system, for example an entangled polymer network, that further separates the analytes according to their size and shape. [CHMO]" ;
                 skos:prefLabel "capillary sieving electrophoresis" .


###  http://purl.allotrope.org/ontologies/process#AFP_0001342
af-p:AFP_0001342 rdf:type owl:Class ;
                 rdfs:subClassOf af-p:AFP_0000365 ;
                 skos:altLabel "immobilised pH gradient-IEF"@en-gb ,
                               "IPG based-IEF" ,
                               "IPG-IEF" ,
                               "immobilized pH gradient-IEF" ;
                 skos:changeNote "2016-02-03 Switched labels [OSTHUS]" ,
                                 "2016-02-25 fix translation [OSTHUS]" ;
                 skos:definition "An electrophoresis method for the separation of amphoteric analytes according to their isoelectric points by the application of an electric field along a pH gradient. The pH gradient is formed during casting of the gels therefore cannot be altered during the experiment. [CHMO]" ;
                 skos:prefLabel "immobilised pH gradient-based isoelectric focusing"@en-gb ,
                                "immobilized pH gradient-based isoelectric focusing" .


###  http://purl.allotrope.org/ontologies/process#AFP_0001922
af-p:AFP_0001922 rdf:type owl:Class ;
                 rdfs:subClassOf af-p:AFP_0000365 ,
                                 af-p:AFP_0000474 ;
                 skos:altLabel "CIEF" ,
                               "capillary isoelectric focussing" ;
                 skos:definition "An electrophoresis method for the separation of amphoteric analytes according to their isolectric points by the application of an electric field along a pH gradient in a capillary. [CHMO]" ;
                 skos:prefLabel "capillary isoelectric focusing" .


###  http://purl.allotrope.org/ontologies/process#AFP_0002035
af-p:AFP_0002035 rdf:type owl:Class ;
                 rdfs:subClassOf af-p:AFP_0000474 ,
                                 af-p:AFP_0001644 ;
                 skos:altLabel "CITP" ;
                 skos:definition "An electrophoresis method in a capillary containing a discontinuous buffer system where the analytes migrate according to their electrophoretic mobilities, forming a chain of adjacent zones moving with equal velocity between two solutions, the leading and terminating electrolytes, bracketing the mobility range of the analytes. [CHMO]" ;
                 skos:prefLabel "capillary isotachophoresis" .


###  http://purl.allotrope.org/ontologies/process#AFP_0002317
af-p:AFP_0002317 rdf:type owl:Class ;
                 rdfs:subClassOf af-p:AFP_0001969 ;
                 skos:altLabel "2D CE" ,
                               "2D-CE" ,
                               "CE-CE" ,
                               "CE/CE" ;
                 skos:definition "A two-dimensional separation method where the separation processes are both capillary electrophoresis. [CHMO]" ;
                 skos:prefLabel "two-dimensional capillary electrophoresis" .


#################################################################
#    Individuals
#################################################################

###  http://purl.allotrope.org/voc/attribution
<http://purl.allotrope.org/voc/attribution> rdf:type owl:NamedIndividual ,
                                                     dct:RightsStatement ;
                                            dct:description """
These taxonomies contain material or may constitute derivative works of material which may be subject to copyright by one of the following organizations.  By using these taxonomies, you agree to the following terms and conditions applicable to its contents:
******************************************************************************
Copyright Notice and Terms for IUPAC Gold Book
______________________________________________________________________________
Copyright © 1998, Regents of the University of California
All rights reserved.
Redistribution and use in source and binary forms, with or without modification, are permitted provided that the following conditions are met:
1. Redistributions of source code must retain the above copyright notice, this list of conditions and the following disclaimer.
2. Redistributions in binary form must reproduce the above copyright notice, this list of conditions and the following disclaimer in the documentation and/or other materials provided with the distribution.
THIS SOFTWARE IS PROVIDED BY THE COPYRIGHT HOLDERS AND CONTRIBUTORS \"AS IS\" AND ANY EXPRESS OR IMPLIED WARRANTIES, INCLUDING, BUT NOT LIMITED TO, THE IMPLIED WARRANTIES OF MERCHANTABILITY AND FITNESS FOR A PARTICULAR PURPOSE ARE DISCLAIMED. IN NO EVENT SHALL THE COPYRIGHT HOLDER OR CONTRIBUTORS BE LIABLE FOR ANY DIRECT, INDIRECT, INCIDENTAL, SPECIAL, EXEMPLARY, OR CONSEQUENTIAL DAMAGES (INCLUDING, BUT NOT LIMITED TO, PROCUREMENT OF SUBSTITUTE GOODS OR SERVICES; LOSS OF USE, DATA, OR PROFITS; OR BUSINESS INTERRUPTION) HOWEVER CAUSED AND ON ANY THEORY OF LIABILITY, WHETHER IN CONTRACT, STRICT LIABILITY, OR TORT (INCLUDING NEGLIGENCE OR OTHERWISE) ARISING IN ANY WAY OUT OF THE USE OF THIS SOFTWARE, EVEN IF ADVISED OF THE POSSIBILITY OF SUCH DAMAGE.
******************************************************************************
Copyright Notice and Terms for PSI-MS (Proteomics Standards Initiative - Mass Spectrometry) Mass spectrometer output files and spectra interpretation
_____________________________________________________________________________
Created by Matt Chambers, Andreas Bertsch, Marius Kallhardt, Eric Deutsch Fredrik Levander, Pierre-Alain Binz, and Gerhard Mayer. Publisher: HUPO Proteomics Standards Initiative Mass Spectrometry Standards Working Group and HUPO Proteomics Standards Initiative Proteomics Informatics Working Group. This work is used pursuant to a Creative Commons license available here: http://creativecommons.org/licenses/by/3.0/legalcode

******************************************************************************
Attribution Notice for National Center for Biomedical Ontology materials.

This work contains material from the Cell Ontology and Clinical Measurement Ontology, available here: http://bioportal.bioontology.org/.
******************************************************************************
Attribution Notice for ChEBI
This work contains material from the European Bioinformatics Institute’s ChEBI database.
******************************************************************************
Attribution Notice for Quantities Units Dimensions Data Types (http://www.qudt.org/)
This work contains content from www.qudt.org and is used pursuant to a Creative Commons License available here: http://creativecommons.org/licenses/by-sa/3.0/us/legalcode. The original work may have been modified.
******************************************************************************
Copyright and Attribution Notice for Dublin Core Metadata Initiative Document
This work contains material from the following DCMI document used pursuant to a creative commons license available here: https://creativecommons.org/licenses/by/4.0/legalcode. This material may have been modified or changed.
Timestamped URL:          http://dublincore.org/documents/2012/06/14/dcmi-terms/
Date Issued:                       2012-06-14
Document Status:            This is a DCMI Recommendation.
Copyright © 1995-2015 DCMI. All Rights Reserved. DCMI liability, trademark/service mark, document use and software licensing rules apply.
******************************************************************************

""" ;
                                            dct:title "Derivative works attribution" .


###  http://purl.allotrope.org/voc/copyright
<http://purl.allotrope.org/voc/copyright> rdf:type owl:NamedIndividual ,
                                                   dct:RightsStatement ;
                                          dct:description "(c) 2018 Allotrope Foundation" ;
                                          dct:rightsHolder <http://www.allotrope.org> ;
                                          dct:title "(c) 2018 Allotrope Foundation" .


###  http://purl.allotrope.org/voc/creative-commons-attribution-license
<http://purl.allotrope.org/voc/creative-commons-attribution-license> rdf:type owl:NamedIndividual ,
                                                                              dct:LicenseDocument ;
                                                                     dct:description """This work is licensed under a Creative Commons Attribution 4.0 International License http://creativecommons.org/licenses/by/4.0/.

THESE MATERIALS ARE PROVIDED \"AS IS\" AND ALLOTROPE EXPRESSLY DISCLAIMS ALL WARRANTIES, EXPRESS, IMPLIED OR STATUTORY, INCLUDING, WITHOUT LIMITATION, THE WARRANTIES OF NON-INFRINGEMENT, TITLE, MERCHANTABILITY AND FITNESS FOR A PARTICULAR PURPOSE.

Copyright © 2015-2025 Allotrope Foundation
""" ;
                                                                     dct:title "Creative Commons Attribution 4.0 International Public License" .


###  Generated by the OWL API (version 5.1.19) https://github.com/owlcs/owlapi/
