@prefix : <http://purl.allotrope.org/voc/afo/domain/WD/2025/06/centrifugation#> .
@prefix dct: <http://purl.org/dc/terms/> .
@prefix owl: <http://www.w3.org/2002/07/owl#> .
@prefix rdf: <http://www.w3.org/1999/02/22-rdf-syntax-ns#> .
@prefix xml: <http://www.w3.org/XML/1998/namespace> .
@prefix xsd: <http://www.w3.org/2001/XMLSchema#> .
@prefix af-c: <http://purl.allotrope.org/ontologies/common#> .
@prefix af-e: <http://purl.allotrope.org/ontologies/equipment#> .
@prefix af-m: <http://purl.allotrope.org/ontologies/material#> .
@prefix af-p: <http://purl.allotrope.org/ontologies/process#> .
@prefix af-q: <http://purl.allotrope.org/ontologies/quality#> .
@prefix af-r: <http://purl.allotrope.org/ontologies/result#> .
@prefix af-x: <http://purl.allotrope.org/ontologies/property#> .
@prefix rdfs: <http://www.w3.org/2000/01/rdf-schema#> .
@prefix skos: <http://www.w3.org/2004/02/skos/core#> .
@prefix af-cur: <http://purl.allotrope.org/ontologies/curation#> .
@base <http://purl.allotrope.org/voc/afo/domain/WD/2025/06/centrifugation#> .

<http://purl.allotrope.org/voc/afo/domain/WD/2025/06/centrifugation> rdf:type owl:Ontology ;
                                                                                owl:versionIRI <http://purl.allotrope.org/voc/afo/domain/WD/2025/06/centrifugation> ;
                                                                                owl:imports <http://purl.allotrope.org/voc/afo/WD/2025/06/afo> ;
                                                                                dct:issued "2025-06-25T12:00:00Z"^^xsd:dateTime ;
                                                                                dct:license <http://purl.allotrope.org/voc/creative-commons-attribution-license> ;
                                                                                dct:modified "2025-04-04T12:00:00Z"^^xsd:dateTime ;
                                                                                dct:rights <http://purl.allotrope.org/voc/attribution> ,
                                                                                           <http://purl.allotrope.org/voc/copyright> ;
                                                                                dct:title "AFO Centrifugation Domain Ontology (WD/2025/06)" ;
                                                                                owl:priorVersion <http://purl.allotrope.org/voc/afo/domain/WD/2018/04/centrifugation> ;
                                                                                owl:versionInfo "WD/2025/06" .

#################################################################
#    Annotation properties
#################################################################

###  http://purl.allotrope.org/ontologies/property#AFX_0002796
af-x:AFX_0002796 rdf:type owl:AnnotationProperty .


###  http://purl.allotrope.org/ontologies/property#AFX_0002798
af-x:AFX_0002798 rdf:type owl:AnnotationProperty .


###  http://purl.allotrope.org/ontologies/property#AFX_0002809
af-x:AFX_0002809 rdf:type owl:AnnotationProperty .


###  http://purl.org/dc/terms/source
dct:source rdf:type owl:AnnotationProperty .


###  http://www.w3.org/2004/02/skos/core#altLabel
skos:altLabel rdf:type owl:AnnotationProperty .


###  http://www.w3.org/2004/02/skos/core#changeNote
skos:changeNote rdf:type owl:AnnotationProperty .


###  http://www.w3.org/2004/02/skos/core#definition
skos:definition rdf:type owl:AnnotationProperty .


###  http://www.w3.org/2004/02/skos/core#example
skos:example rdf:type owl:AnnotationProperty .


###  http://www.w3.org/2004/02/skos/core#note
skos:note rdf:type owl:AnnotationProperty .


###  http://www.w3.org/2004/02/skos/core#prefLabel
skos:prefLabel rdf:type owl:AnnotationProperty .


###  http://www.w3.org/2004/02/skos/core#scopeNote
skos:scopeNote rdf:type owl:AnnotationProperty .


#################################################################
#    Object Properties
#################################################################

###  http://purl.allotrope.org/ontologies/property#AFX_0000394
af-x:AFX_0000394 rdf:type owl:ObjectProperty .


#################################################################
#    Classes
#################################################################

###  http://purl.allotrope.org/ontologies/equipment#AFE_0001152
af-e:AFE_0001152 rdf:type owl:Class ;
                 rdfs:subClassOf af-e:AFE_0001151 ,
                                 [ rdf:type owl:Restriction ;
                                   owl:onProperty af-x:AFX_0000394 ;
                                   owl:someValuesFrom af-e:AFE_0001153
                                 ] ;
                 dct:source "https://en.wikipedia.org/wiki/Laboratory_centrifuge" ;
                 skos:altLabel "benchtop centrifuge" ,
                               "lab centrifuge" ;
                 skos:changeNote "2015-11-03 add concept [Amgen]" ,
                                 "2016-02-02 add harmonized property restrictions [OSTHUS]" ;
                 skos:definition "A laboratory centrifuge is a piece of laboratory equipment, driven by a motor, which spins liquid samples at high speed. There are various types of centrifuges, depending on the size and the sample capacity. [Wikipedia]" ;
                 skos:prefLabel "laboratory centrifuge" .


###  http://purl.allotrope.org/ontologies/equipment#AFE_0001153
af-e:AFE_0001153 rdf:type owl:Class ;
                 rdfs:subClassOf af-e:AFE_0000354 ;
                 skos:changeNote "2015-11-03 add concept [Amgen]" ;
                 skos:definition "The rotating part of a centrifuge that holds the samples. [Allotrope]" ;
                 skos:prefLabel "centrifuge rotor" .


###  http://purl.allotrope.org/ontologies/equipment#AFE_0001154
af-e:AFE_0001154 rdf:type owl:Class ;
                 rdfs:subClassOf af-e:AFE_0001152 ;
                 skos:altLabel "Eppendorf" ,
                               "microfuge" ;
                 skos:changeNote "2015-11-03 add concept [Amgen]" ;
                 skos:definition "A laboratory centrifuge for small tubes from 0.2 ml to 2.0 ml (micro tubes), up to 96 well-plates, compact design and small footprint. Can generate forces up to 15000 g. [Wikipedia]" ;
                 skos:prefLabel "microcentrifuge" .


###  http://purl.allotrope.org/ontologies/equipment#AFE_0001155
af-e:AFE_0001155 rdf:type owl:Class ;
                 rdfs:subClassOf af-e:AFE_0001152 ;
                 skos:changeNote "2015-11-03 add concept [Amgen]" ;
                 skos:definition "Moderate-speed centrifuges used for clinical applications like blood collection tubes. [Wikipedia]" ;
                 skos:prefLabel "clinical centrifuge" .


###  http://purl.allotrope.org/ontologies/equipment#AFE_0001156
af-e:AFE_0001156 rdf:type owl:Class ;
                 rdfs:subClassOf af-e:AFE_0001152 ;
                 af-x:AFX_0002795 """[ 
  rdf:type owl:Restriction ;
  owl:onProperty af-x:AFX_0000952 ;
  owl:someValuesFrom af-p:AFP_0000825
]""" ;
                 dct:source "https://en.wikipedia.org/wiki/Ultracentrifuge" ;
                 skos:changeNote "2015-11-03 add concept [Amgen]" ,
                                 "2016-02-02 add harmonized property restrictions [OSTHUS]" ;
                 skos:definition "The ultracentrifuge is a centrifuge optimized for spinning a rotor at very high speeds, capable of generating acceleration as high as 2 000 000 g. [Wikipedia]" ;
                 skos:prefLabel "ultracentrifuge" .


###  http://purl.allotrope.org/ontologies/equipment#AFE_0001157
af-e:AFE_0001157 rdf:type owl:Class ;
                 rdfs:subClassOf af-e:AFE_0001156 ,
                                 af-e:AFE_0001158 ;
                 dct:source "https://en.wikipedia.org/wiki/Ultracentrifuge" ;
                 skos:changeNote "2015-11-03 add concept [Amgen]" ;
                 skos:definition "In an analytical ultracentrifuge, a sample being spun can be monitored in real time through an optical detection system, using ultraviolet light absorption and/or interference optical refractive index sensitive system. [Wikipedia]" ;
                 skos:prefLabel "analytical ultracentrifuge" .


###  http://purl.allotrope.org/ontologies/equipment#AFE_0001158
af-e:AFE_0001158 rdf:type owl:Class ;
                 rdfs:subClassOf af-e:AFE_0001152 ;
                 af-x:AFX_0002795 """[ 
    rdf:type owl:Restriction ;
    owl:onProperty af-x:AFX_0000952 ;
    owl:someValuesFrom af-p:AFP_0001278
]""" ;
                 skos:changeNote "2015-11-03 add concept [Amgen]" ,
                                 "2016-02-02 add harmonized property restrictions [OSTHUS]" ;
                 skos:definition "A centrifuge used for analytical centrifugation. During the centrifugation the sample can be monitored in real time through an optical detection system. [Allotrope]" ;
                 skos:prefLabel "analytical centrifuge" .


###  http://purl.allotrope.org/ontologies/equipment#AFE_0001159
af-e:AFE_0001159 rdf:type owl:Class ;
                 rdfs:subClassOf af-e:AFE_0001156 ,
                                 af-e:AFE_0001160 ;
                 dct:source "https://en.wikipedia.org/wiki/Ultracentrifuge" ;
                 skos:changeNote "2015-11-03 add concept [Amgen]" ;
                 skos:definition "Preparative ultracentrifuges are available with a wide variety of rotors suitable for a great range of experiments. Most rotors are designed to hold tubes that contain the samples. [Wikipedia]" ;
                 skos:prefLabel "preparative ultracentrifuge" .


###  http://purl.allotrope.org/ontologies/equipment#AFE_0001160
af-e:AFE_0001160 rdf:type owl:Class ;
                 rdfs:subClassOf af-e:AFE_0001152 ;
                 af-x:AFX_0002795 """[
   rdf:type owl:Restriction ;
   owl:onProperty af-x:AFX_0000952 ;
   owl:someValuesFrom af-p:AFP_0002068
]""" ;
                 skos:changeNote "2015-11-03 add concept [Amgen]" ,
                                 "2016-02-02 add harmonized property restrictions [OSTHUS]" ;
                 skos:definition "A centrifuge that is used for preparative centrifugation. [Allotrope]" ;
                 skos:prefLabel "preparative centrifuge" .


###  http://purl.allotrope.org/ontologies/equipment#AFE_0001161
af-e:AFE_0001161 rdf:type owl:Class ;
                 rdfs:subClassOf af-e:AFE_0001153 ;
                 dct:source "https://en.wikipedia.org/wiki/Ultracentrifuge" ;
                 skos:changeNote "2015-11-03 add concept [Amgen]" ;
                 skos:definition "Fixed angle rotors are made of a single block of material and hold the tubes in cavities bored at a predetermined angle. [Wikipedia]" ;
                 skos:prefLabel "fixed angle rotor" .


###  http://purl.allotrope.org/ontologies/equipment#AFE_0001162
af-e:AFE_0001162 rdf:type owl:Class ;
                 rdfs:subClassOf af-e:AFE_0001153 ;
                 dct:source "https://en.wikipedia.org/wiki/Ultracentrifuge" ;
                 skos:altLabel "swing head rotor" ;
                 skos:changeNote "2015-11-03 add concept [Amgen]" ;
                 skos:definition "Swinging bucket rotors allow the tubes to hang on hinges so the tubes reorient to the horizontal as the rotor initially accelerates. [Wikipedia]" ;
                 skos:prefLabel "swinging bucket rotor" .


###  http://purl.allotrope.org/ontologies/equipment#AFE_0001163
af-e:AFE_0001163 rdf:type owl:Class ;
                 rdfs:subClassOf af-e:AFE_0001153 ;
                 dct:source "https://en.wikipedia.org/wiki/Ultracentrifuge" ;
                 skos:changeNote "2015-11-03 add concept [Amgen]" ;
                 skos:definition "Zonal rotors are designed to contain a large volume of sample in a single central cavity rather than in tubes. Some zonal rotors are capable of dynamic loading and unloading of samples while the rotor is spinning at high speed. [Wikipedia]" ;
                 skos:prefLabel "zonal rotor" .


###  http://purl.allotrope.org/ontologies/equipment#AFE_0001164
af-e:AFE_0001164 rdf:type owl:Class ;
                 rdfs:subClassOf af-e:AFE_0001152 ;
                 skos:changeNote "2015-11-03 add concept [Amgen]" ;
                 skos:definition "Centrifuge with a rotational speed of 15000-20000 RPM and a centrifugal field of 100000 g with large sample capacity. [Allotrope]" ;
                 skos:prefLabel "high-speed centrifuge" .


###  http://purl.allotrope.org/ontologies/equipment#AFE_0001165
af-e:AFE_0001165 rdf:type owl:Class ;
                 rdfs:subClassOf af-e:AFE_0000354 ;
                 skos:changeNote "2015-11-03 add concept [Amgen]" ;
                 skos:definition "A bowl that is part of a centrifuge that contains the samples. [Allotrope]" ;
                 skos:prefLabel "centrifuge bowl" .


###  http://purl.allotrope.org/ontologies/equipment#AFE_0001166
af-e:AFE_0001166 rdf:type owl:Class ;
                 rdfs:subClassOf af-e:AFE_0000354 ;
                 skos:changeNote "2015-11-03 add concept [Amgen]" ;
                 skos:definition "An safety indicator that indicates a running centrifuge. [Allotrope]" ;
                 skos:prefLabel "centrifuge indicator" .


###  http://purl.allotrope.org/ontologies/equipment#AFE_0001454
af-e:AFE_0001454 rdf:type owl:Class ;
                 rdfs:subClassOf af-e:AFE_0000718 ;
                 af-x:AFX_0002798 "true"^^xsd:boolean ;
                 dct:source "https://en.wikipedia.org/wiki/Laboratory_centrifuge#Centrifuge_tubes" ;
                 skos:changeNote "2015-11-04 add concept [Amgen]" ;
                 skos:definition "Centrifuge tubes are precision-made, high-strength tubes of glass or plastic made to fit exactly in rotor cavities. They may vary in capacity from 50 mL down to much smaller capacities used in microcentrifuges used extensively in molecular biology laboratories. Microcentrifuges typically accommodate disposable plastic microcentrifuge tubes with capacities from 250 μL to 2.0 mL. [Wikipedia]" ;
                 skos:prefLabel "centrifuge tube" .


###  http://purl.allotrope.org/ontologies/process#AFP_0000361
af-p:AFP_0000361 rdf:type owl:Class ;
                 rdfs:subClassOf af-p:AFP_0000825 ;
                 skos:definition "A method where the components of a sample (e.g. plasma lipoproteins) are separated on the basis of their density in a centrifuge according to the centrifugal force they experience. A density gradient is established via equilibrium sedimentation (e.g. using caesium ions), and then analyte molecules concentrate as bands where the molecule density matches that of the surrounding solution. Samples are spun at speeds of up to 150,000 rpm. [CHMO]" ;
                 skos:prefLabel "isopycnic gradient ultracentrifugation" .


###  http://purl.allotrope.org/ontologies/process#AFP_0000647
af-p:AFP_0000647 rdf:type owl:Class ;
                 rdfs:subClassOf af-p:AFP_0000820 ;
                 skos:altLabel "low speed centrifugation" ;
                 skos:definition "A separation method where the components of a sample  are separated on the basis of their density in a centrifuge according to the centrifugal force they experience. Samples are spun at <5000 rpm. [CHMO]" ;
                 skos:prefLabel "low-speed centrifugation" .


###  http://purl.allotrope.org/ontologies/process#AFP_0000684
af-p:AFP_0000684 rdf:type owl:Class ;
                 rdfs:subClassOf af-p:AFP_0000820 ;
                 skos:altLabel "density gradient centrifugation" ;
                 skos:definition "A method where the components of a sample are separated on the basis of their density, in a dense medium or density gradient, in a centrifuge, according to the centrifugal force they experience. [CHMO]" ;
                 skos:prefLabel "density-gradient centrifugation" .


###  http://purl.allotrope.org/ontologies/process#AFP_0000825
af-p:AFP_0000825 rdf:type owl:Class ;
                 rdfs:subClassOf af-p:AFP_0002143 ;
                 skos:altLabel "ultra-centrifugation" ;
                 skos:definition "A method where components of a sample are separated on the basis of their density in an ultracentrifuge according to the centrifugal force they experience. Samples are spun at speeds of up to 150,000 rpm. [CHMO]" ;
                 skos:prefLabel "ultracentrifugation" .


###  http://purl.allotrope.org/ontologies/process#AFP_0001242
af-p:AFP_0001242 rdf:type owl:Class ;
                 rdfs:subClassOf af-p:AFP_0000684 ;
                 skos:altLabel "rate zonal centrifugation" ;
                 skos:definition "A method where the components of a sample are separated on the basis of their density, in a density gradient of e.g. CsCl in a centrifuge, according to mass. The species in the sample move through the gradient until they reach a point where their density and that of the gradient are identical. [CHMO]" ;
                 skos:prefLabel "rate-zonal centrifugation" .


###  http://purl.allotrope.org/ontologies/process#AFP_0001247
af-p:AFP_0001247 rdf:type owl:Class ;
                 rdfs:subClassOf af-p:AFP_0000684 ,
                                 af-p:AFP_0000825 ;
                 skos:altLabel "density gradient ultracentrifugation" ;
                 skos:definition "A method where the components of a sample are separated on the basis of their density, in a dense medium or density gradient, in a centrifuge, according to the centrifugal force they experience. Samples are spun at speeds of up to 150,000 rpm. [CHMO]" ;
                 skos:prefLabel "density-gradient ultracentrifugation" .


###  http://purl.allotrope.org/ontologies/process#AFP_0001278
af-p:AFP_0001278 rdf:type owl:Class ;
                 rdfs:subClassOf af-p:AFP_0000820 ;
                 skos:definition "A separation method where components of a sample are separated on the basis of their density in a centrifuge according to the centrifugal force they experience. During centrifugation the sample can be monitored in real time through an optical detection system or using ultraviolet light absorption. [CHMO]" ;
                 skos:prefLabel "analytical centrifugation" .


###  http://purl.allotrope.org/ontologies/process#AFP_0001678
af-p:AFP_0001678 rdf:type owl:Class ;
                 rdfs:subClassOf af-p:AFP_0000820 ;
                 skos:definition "A separation method where the components of a sample are separated on the basis of their density in a centrifuge according to the centrifugal force they experience. The sample is centrifuged in a number of separate, sequential steps. [CHMO]" ;
                 skos:prefLabel "sequential centrifugation" .


###  http://purl.allotrope.org/ontologies/process#AFP_0001822
af-p:AFP_0001822 rdf:type owl:Class ;
                 rdfs:subClassOf af-p:AFP_0000684 ;
                 skos:altLabel "equilibrium centrifugation" ,
                               "sedimentation equilibrium centrifugation" ;
                 skos:definition "A method where the components of a sample are separated on the basis of their density, in a density gradient of e.g. CsCl in a centrifuge, according to buoyant density. The species in the sample move through the gradient until they reach a point where their density and that of the gradient are identical. [CHMO]" ;
                 skos:prefLabel "isopycnic centrifugation" .


###  http://purl.allotrope.org/ontologies/process#AFP_0002068
af-p:AFP_0002068 rdf:type owl:Class ;
                 rdfs:subClassOf af-p:AFP_0000820 ;
                 skos:definition "A method where a sample is purified by removing impurities on the basis of their density in a centrifuge. [CHMO]" ;
                 skos:prefLabel "preparative centrifugation" .


###  http://purl.allotrope.org/ontologies/process#AFP_0002143
af-p:AFP_0002143 rdf:type owl:Class ;
                 rdfs:subClassOf af-p:AFP_0000820 ;
                 skos:altLabel "high speed centrifugation" ;
                 skos:definition "A separation method where components of a sample are separated on the basis of their density in a centrifuge according to the centrifugal force they experience. Samples are spun at >5000 rpm. [CHMO]" ;
                 skos:prefLabel "high-speed centrifugation" .


###  http://purl.allotrope.org/ontologies/process#AFP_0002240
af-p:AFP_0002240 rdf:type owl:Class ;
                 rdfs:subClassOf af-p:AFP_0001678 ;
                 skos:definition "A separation method where the components of a cell are separated on the basis of their density in a centrifuge according to the centrifugal force they experience. The sample is centrifuged in a number of separate, sequential steps; each time the pellet is removed and the speed increased. [CHMO]" ;
                 skos:prefLabel "differential centrifugation" .


#################################################################
#    Individuals
#################################################################

###  http://purl.allotrope.org/voc/attribution
<http://purl.allotrope.org/voc/attribution> rdf:type owl:NamedIndividual ,
                                                     dct:RightsStatement ;
                                            dct:description """
These taxonomies contain material or may constitute derivative works of material which may be subject to copyright by one of the following organizations.  By using these taxonomies, you agree to the following terms and conditions applicable to its contents:
******************************************************************************
Copyright Notice and Terms for IUPAC Gold Book
______________________________________________________________________________
Copyright © 1998, Regents of the University of California
All rights reserved.
Redistribution and use in source and binary forms, with or without modification, are permitted provided that the following conditions are met:
1. Redistributions of source code must retain the above copyright notice, this list of conditions and the following disclaimer.
2. Redistributions in binary form must reproduce the above copyright notice, this list of conditions and the following disclaimer in the documentation and/or other materials provided with the distribution.
THIS SOFTWARE IS PROVIDED BY THE COPYRIGHT HOLDERS AND CONTRIBUTORS \"AS IS\" AND ANY EXPRESS OR IMPLIED WARRANTIES, INCLUDING, BUT NOT LIMITED TO, THE IMPLIED WARRANTIES OF MERCHANTABILITY AND FITNESS FOR A PARTICULAR PURPOSE ARE DISCLAIMED. IN NO EVENT SHALL THE COPYRIGHT HOLDER OR CONTRIBUTORS BE LIABLE FOR ANY DIRECT, INDIRECT, INCIDENTAL, SPECIAL, EXEMPLARY, OR CONSEQUENTIAL DAMAGES (INCLUDING, BUT NOT LIMITED TO, PROCUREMENT OF SUBSTITUTE GOODS OR SERVICES; LOSS OF USE, DATA, OR PROFITS; OR BUSINESS INTERRUPTION) HOWEVER CAUSED AND ON ANY THEORY OF LIABILITY, WHETHER IN CONTRACT, STRICT LIABILITY, OR TORT (INCLUDING NEGLIGENCE OR OTHERWISE) ARISING IN ANY WAY OUT OF THE USE OF THIS SOFTWARE, EVEN IF ADVISED OF THE POSSIBILITY OF SUCH DAMAGE.
******************************************************************************
Copyright Notice and Terms for PSI-MS (Proteomics Standards Initiative - Mass Spectrometry) Mass spectrometer output files and spectra interpretation
_____________________________________________________________________________
Created by Matt Chambers, Andreas Bertsch, Marius Kallhardt, Eric Deutsch Fredrik Levander, Pierre-Alain Binz, and Gerhard Mayer. Publisher: HUPO Proteomics Standards Initiative Mass Spectrometry Standards Working Group and HUPO Proteomics Standards Initiative Proteomics Informatics Working Group. This work is used pursuant to a Creative Commons license available here: http://creativecommons.org/licenses/by/3.0/legalcode

******************************************************************************
Attribution Notice for National Center for Biomedical Ontology materials.

This work contains material from the Cell Ontology and Clinical Measurement Ontology, available here: http://bioportal.bioontology.org/.
******************************************************************************
Attribution Notice for ChEBI
This work contains material from the European Bioinformatics Institute’s ChEBI database.
******************************************************************************
Attribution Notice for Quantities Units Dimensions Data Types (http://www.qudt.org/)
This work contains content from www.qudt.org and is used pursuant to a Creative Commons License available here: http://creativecommons.org/licenses/by-sa/3.0/us/legalcode. The original work may have been modified.
******************************************************************************
Copyright and Attribution Notice for Dublin Core Metadata Initiative Document
This work contains material from the following DCMI document used pursuant to a creative commons license available here: https://creativecommons.org/licenses/by/4.0/legalcode. This material may have been modified or changed.
Timestamped URL:          http://dublincore.org/documents/2012/06/14/dcmi-terms/
Date Issued:                       2012-06-14
Document Status:            This is a DCMI Recommendation.
Copyright © 1995-2015 DCMI. All Rights Reserved. DCMI liability, trademark/service mark, document use and software licensing rules apply.
******************************************************************************

""" ;
                                            dct:title "Derivative works attribution" .


###  http://purl.allotrope.org/voc/copyright
<http://purl.allotrope.org/voc/copyright> rdf:type owl:NamedIndividual ,
                                                   dct:RightsStatement ;
                                          dct:description "Copyright © 2019 Allotrope Foundation" ;
                                          dct:rightsHolder <http://www.allotrope.org> ;
                                          dct:title "Copyright © 2019 Allotrope Foundation" .


###  http://purl.allotrope.org/voc/creative-commons-attribution-license
<http://purl.allotrope.org/voc/creative-commons-attribution-license> rdf:type owl:NamedIndividual ,
                                                                              dct:LicenseDocument ;
                                                                     dct:description """This work is licensed under a Creative Commons Attribution 4.0 International License http://creativecommons.org/licenses/by/4.0/.

THESE MATERIALS ARE PROVIDED \"AS IS\" AND ALLOTROPE EXPRESSLY DISCLAIMS ALL WARRANTIES, EXPRESS, IMPLIED OR STATUTORY, INCLUDING, WITHOUT LIMITATION, THE WARRANTIES OF NON-INFRINGEMENT, TITLE, MERCHANTABILITY AND FITNESS FOR A PARTICULAR PURPOSE.

Copyright © 2015-2025 Allotrope Foundation
""" ;
                                                                     dct:title "Creative Commons Attribution 4.0 International Public License" .


###  Generated by the OWL API (version 5.1.19) https://github.com/owlcs/owlapi/
