@prefix : <http://purl.allotrope.org/voc/afo/domain/WD/2025/06/gc#> .
@prefix cl: <http://purl.obolibrary.org/obo/CL> .
@prefix go: <http://purl.obolibrary.org/obo/GO> .
@prefix ro: <http://purl.obolibrary.org/obo/RO> .
@prefix bfo: <http://purl.obolibrary.org/obo/BFO> .
@prefix dct: <http://purl.org/dc/terms/> .
@prefix iao: <http://purl.obolibrary.org/obo/IAO> .
@prefix obi: <http://purl.obolibrary.org/obo/OBI> .
@prefix owl: <http://www.w3.org/2002/07/owl#> .
@prefix rdf: <http://www.w3.org/1999/02/22-rdf-syntax-ns#> .
@prefix xml: <http://www.w3.org/XML/1998/namespace> .
@prefix xsd: <http://www.w3.org/2001/XMLSchema#> .
@prefix af-c: <http://purl.allotrope.org/ontologies/common#> .
@prefix af-e: <http://purl.allotrope.org/ontologies/equipment#> .
@prefix af-m: <http://purl.allotrope.org/ontologies/material#> .
@prefix af-p: <http://purl.allotrope.org/ontologies/process#> .
@prefix af-q: <http://purl.allotrope.org/ontologies/quality#> .
@prefix af-r: <http://purl.allotrope.org/ontologies/result#> .
@prefix af-x: <http://purl.allotrope.org/ontologies/property#> .
@prefix rdfs: <http://www.w3.org/2000/01/rdf-schema#> .
@prefix skos: <http://www.w3.org/2004/02/skos/core#> .
@prefix af-fn: <http://purl.allotrope.org/ontologies/function#> .
@prefix af-rl: <http://purl.allotrope.org/ontologies/role#> .
@prefix af-cur: <http://purl.allotrope.org/ontologies/curation#> .
@base <http://purl.allotrope.org/voc/afo/domain/WD/2025/06/gc#> .

<http://purl.allotrope.org/voc/afo/domain/WD/2025/06/gc> rdf:type owl:Ontology ;
                                                                    owl:versionIRI <http://purl.allotrope.org/voc/afo/domain/WD/2025/06/gc> ;
                                                                    owl:imports <http://purl.allotrope.org/voc/afo/WD/2025/06/afo> ,
                                                                                <http://purl.allotrope.org/voc/afo/domain/WD/2025/06/chromatography> ;
                                                                    dct:issued "2025-06-25T12:00:00Z"^^xsd:dateTime ;
                                                                    dct:license <http://purl.allotrope.org/voc/creative-commons-attribution-license> ;
                                                                    dct:modified "2025-04-04T12:00:00Z"^^xsd:dateTime ;
                                                                    dct:rights <http://purl.allotrope.org/voc/attribution> ,
                                                                               <http://purl.allotrope.org/voc/copyright> ;
                                                                    dct:title "AFO Gas Chromatography Domain Ontology (WD/2025/06)" ;
                                                                    owl:priorVersion <http://purl.allotrope.org/voc/afo/domain/WD/2025/03/gc> ;
                                                                    owl:versionInfo "WD/2025/06" .

#################################################################
#    Annotation properties
#################################################################

###  http://purl.allotrope.org/ontologies/property#AFX_0002796
af-x:AFX_0002796 rdf:type owl:AnnotationProperty .


###  http://purl.allotrope.org/ontologies/property#AFX_0002798
af-x:AFX_0002798 rdf:type owl:AnnotationProperty .


###  http://purl.allotrope.org/ontologies/property#AFX_0002809
af-x:AFX_0002809 rdf:type owl:AnnotationProperty .


###  http://purl.org/dc/terms/source
dct:source rdf:type owl:AnnotationProperty .


###  http://www.w3.org/2004/02/skos/core#altLabel
skos:altLabel rdf:type owl:AnnotationProperty .


###  http://www.w3.org/2004/02/skos/core#changeNote
skos:changeNote rdf:type owl:AnnotationProperty .


###  http://www.w3.org/2004/02/skos/core#definition
skos:definition rdf:type owl:AnnotationProperty .


###  http://www.w3.org/2004/02/skos/core#example
skos:example rdf:type owl:AnnotationProperty .


###  http://www.w3.org/2004/02/skos/core#note
skos:note rdf:type owl:AnnotationProperty .


###  http://www.w3.org/2004/02/skos/core#prefLabel
skos:prefLabel rdf:type owl:AnnotationProperty .


###  http://www.w3.org/2004/02/skos/core#scopeNote
skos:scopeNote rdf:type owl:AnnotationProperty .


#################################################################
#    Object Properties
#################################################################

###  http://purl.obolibrary.org/obo/RO_0000056
ro:_0000056 rdf:type owl:ObjectProperty .


#################################################################
#    Classes
#################################################################

###  http://purl.allotrope.org/ontologies/equipment#AFE_0000161
af-e:AFE_0000161 rdf:type owl:Class .


###  http://purl.allotrope.org/ontologies/equipment#AFE_0000526
af-e:AFE_0000526 rdf:type owl:Class ;
                 rdfs:subClassOf af-e:AFE_0000718 ;
                 af-x:AFX_0002798 "true"^^xsd:boolean ;
                 skos:definition "The inlet liner is a tube that allows a sample which is injected in the liquid phase to pass into the gaseous phase and onto the column. [Allotrope]" ;
                 skos:prefLabel "inlet liner" .


###  http://purl.allotrope.org/ontologies/equipment#AFE_0000591
af-e:AFE_0000591 rdf:type owl:Class ;
                 rdfs:subClassOf af-e:AFE_0000024 ;
                 af-x:AFX_0002798 "true"^^xsd:boolean ;
                 skos:altLabel "2D GC" ,
                               "2D gas chromatograph" ,
                               "GCxGC" ,
                               "two-dimensional gas chromatograph" ;
                 skos:changeNote "2016-02-02 add harmonized property restrictions [Allotrope]" ;
                 skos:definition "In GC × GC two columns are connected sequentially, typically the first dimension is a conventional column and the second dimension is a short fast GC type, with a modulator positioned between them. [Wikipedia]" ;
                 skos:prefLabel "two-dimensional gas chromatography system" .


###  http://purl.allotrope.org/ontologies/equipment#AFE_0000671
af-e:AFE_0000671 rdf:type owl:Class ;
                 rdfs:subClassOf af-e:AFE_0000161 ;
                 skos:altLabel "PTV injector" ;
                 skos:definition "Temperature controlled sample introduction inlet. [Allotrope]" ;
                 skos:prefLabel "PTV inlet" .


###  http://purl.allotrope.org/ontologies/equipment#AFE_0000772
af-e:AFE_0000772 rdf:type owl:Class ;
                 owl:equivalentClass [ owl:intersectionOf ( af-e:AFE_0000217
                                                            [ rdf:type owl:Restriction ;
                                                              owl:onProperty ro:_0000056 ;
                                                              owl:someValuesFrom af-p:AFP_0000310
                                                            ]
                                                          ) ;
                                       rdf:type owl:Class
                                     ] ;
                 af-x:AFX_0002798 "true"^^xsd:boolean ;
                 skos:definition "A chromatography column used for gas chromatography. [Allotrope]" ;
                 skos:prefLabel "gas chromatography column" .


###  http://purl.allotrope.org/ontologies/equipment#AFE_0000787
af-e:AFE_0000787 rdf:type owl:Class ;
                 rdfs:subClassOf af-e:AFE_0000161 ;
                 skos:altLabel "cool on column" ,
                               "on-column injector" ;
                 skos:definition "The sample is introduced directly into the column without prior heating in the inlet. [Allotrope]" ;
                 skos:prefLabel "on-column inlet" .


###  http://purl.allotrope.org/ontologies/equipment#AFE_0000835
af-e:AFE_0000835 rdf:type owl:Class ;
                 rdfs:subClassOf af-e:AFE_0000161 ;
                 skos:altLabel "P/T system" ;
                 skos:definition "An inlet whereby the volatiles are first purged from the sample via. a carrier gas, trapped in the inlet headspace, condensed and adsorbed at lower temperatures prior to being introduced onto the GC column. [Allotrope]" ;
                 skos:prefLabel "purge and trap system" .


###  http://purl.allotrope.org/ontologies/equipment#AFE_0000885
af-e:AFE_0000885 rdf:type owl:Class ;
                 rdfs:subClassOf af-e:AFE_0000161 ;
                 skos:definition "An open split inlet splits the gas flow to two different outlets with one being an open system at atmospheric pressure. [Allotrope]" ;
                 skos:prefLabel "open split inlet" .


###  http://purl.allotrope.org/ontologies/process#AFP_0000534
af-p:AFP_0000534 rdf:type owl:Class ;
                 rdfs:subClassOf af-p:AFP_0000422 ;
                 skos:altLabel "MESI-GC" ,
                               "membrane extraction with sorbent interface gas chromatography" ,
                               "membrane extraction with sorbent interface-gas chromatography" ;
                 skos:definition "A separation method where the sample is first transferred from one phase (the 'donor' or 'feed' phase) to another (the 'acceptor' or 'strip' phase) across a non-porous non-polar polymer membrane. The membrane extracts the analytes from their matrix, and these are subsequently trapped on a polymeric trap with a porous sorbent using a carrier gas stream. In the second step, the mixture in the carrier gas stream is further separated by gas chromatography. [CHMO]" ;
                 skos:prefLabel "membrane extraction with a sorbent interface-gas chromatography" .


###  http://purl.allotrope.org/ontologies/process#AFP_0000652
af-p:AFP_0000652 rdf:type owl:Class ;
                 rdfs:subClassOf af-p:AFP_0000310 ;
                 skos:altLabel "GLC" ,
                               "gas-liquid chromatography" ;
                 skos:definition "Gas chromatography where the stationary phase is a liquid. [CHMO]" ;
                 skos:prefLabel "gas-liquid chromatography" .


###  http://purl.allotrope.org/ontologies/process#AFP_0000716
af-p:AFP_0000716 rdf:type owl:Class ;
                 rdfs:subClassOf af-p:AFP_0000310 ;
                 skos:altLabel "Py-GC" ,
                               "py-GC" ,
                               "pyrolysis GC" ,
                               "pyrolysis-GC" ,
                               "pyrolysis-gas chromatography" ;
                 skos:definition "The chemical degradation of a sample by thermal energy where the volatile pyrolysates are then separated by column chromatography where the mobile phase is a gas. [CHMO]" ;
                 skos:prefLabel "pyrolysis gas chromatography" .


###  http://purl.allotrope.org/ontologies/process#AFP_0001541
af-p:AFP_0001541 rdf:type owl:Class ;
                 rdfs:subClassOf af-p:AFP_0000310 ;
                 skos:altLabel "2D GC" ,
                               "2D gas chromatography" ,
                               "GCxGC" ;
                 skos:definition "In GC × GC two columns are connected sequentially, typically the first dimension is a conventional column and the second dimension is a short fast GC type, with a modulator positioned between them. [Wikipedia]" ;
                 skos:prefLabel "two-dimensional gas chromatography" .


###  http://purl.allotrope.org/ontologies/process#AFP_0001847
af-p:AFP_0001847 rdf:type owl:Class ;
                 rdfs:subClassOf af-p:AFP_0000310 ;
                 skos:altLabel "CSP GC" ,
                               "CSP-GC" ,
                               "GC on a chiral stationary phase" ,
                               "chiral GC" ;
                 skos:definition "Column chromatography where the mobile phase is a gas and the stationary phase is a chiral, high-boiling-point, thermally-stable liquid such as a chiral polysiloxane. [CHMO]" ;
                 skos:prefLabel "chiral stationary phase gas chromatography" .


###  http://purl.allotrope.org/ontologies/process#AFP_0001923
af-p:AFP_0001923 rdf:type owl:Class ;
                 rdfs:subClassOf af-p:AFP_0000310 ;
                 skos:altLabel "GSC" ;
                 skos:definition "Gas chromatography where the stationary phase is a solid. [CHMO]" ;
                 skos:prefLabel "gas-solid chromatography" .


###  http://purl.allotrope.org/ontologies/process#AFP_0002147
af-p:AFP_0002147 rdf:type owl:Class ;
                 rdfs:subClassOf af-p:AFP_0001159 ;
                 skos:altLabel "programmed-temperature vaporisation"@en-gb ,
                               "PTV" ,
                               "programmed-temperature vaporization" ;
                 skos:definition "A sample preparation method for gas chromatography in which the sample is deposited into the inlet of the chromatograph at a low temperature, then the inlet temperature is rapidly raised to vaporise the desired components and cause their transfer onto the column. [CHMO]" ;
                 skos:prefLabel "programmed temperature vaporisation"@en-gb ,
                                "programmed temperature vaporization" .


###  http://purl.allotrope.org/ontologies/process#AFP_0002444
af-p:AFP_0002444 rdf:type owl:Class ;
                 rdfs:subClassOf af-p:AFP_0000310 ;
                 skos:altLabel "IGC" ;
                 skos:definition "A surface characterization technique in which a pulse or constant concentration of a known gas or vapour (probe molecule) is injected into a column packed with the solid sample at a fixed carrier gas flow rate. The retention time of the probe molecule is then measured using a  traditional gas chromatography detector. [CHMO]" ;
                 skos:prefLabel "inverse gas chromatography" .


###  http://purl.allotrope.org/ontologies/result#AFR_0000314
af-r:AFR_0000314 rdf:type owl:Class ;
                 rdfs:subClassOf af-r:AFR_0000523 ;
                 skos:definition "Result of a gas chromatography run. [Allotrope]" ;
                 skos:prefLabel "gas chromatography result" .


###  http://purl.allotrope.org/ontologies/result#AFR_0000523
af-r:AFR_0000523 rdf:type owl:Class .


###  http://purl.allotrope.org/ontologies/role#AFRL_0000431
af-rl:AFRL_0000431 rdf:type owl:Class ;
                   rdfs:subClassOf af-rl:AFRL_0000432 ;
                   af-x:AFX_0002796 af-r:AFR_0001223 ;
                   dct:license <http://purl.allotrope.org/voc/iupac-license> ;
                   dct:rights <http://purl.allotrope.org/voc/iupac-copyright> ;
                   skos:altLabel "volumetric internal standard" ;
                   skos:changeNote "2024-09-12 Added license and rights fields." ;
                   skos:definition "Compound added in a fixed reproducible amount to a solution to be analyzed by gas chromatography to permit corrections for uncontrolled variations in injected volumes. [IUPAC]" ;
                   skos:prefLabel "volumetric internal standard role" .


#################################################################
#    Individuals
#################################################################

###  http://purl.allotrope.org/voc/attribution
<http://purl.allotrope.org/voc/attribution> rdf:type owl:NamedIndividual ,
                                                     dct:RightsStatement ;
                                            dct:description """
These taxonomies contain material or may constitute derivative works of material which may be subject to copyright by one of the following organizations.  By using these taxonomies, you agree to the following terms and conditions applicable to its contents:
******************************************************************************
Copyright Notice and Terms for IUPAC Gold Book
______________________________________________________________________________
Copyright © 1998, Regents of the University of California
All rights reserved.
Redistribution and use in source and binary forms, with or without modification, are permitted provided that the following conditions are met:
1. Redistributions of source code must retain the above copyright notice, this list of conditions and the following disclaimer.
2. Redistributions in binary form must reproduce the above copyright notice, this list of conditions and the following disclaimer in the documentation and/or other materials provided with the distribution.
THIS SOFTWARE IS PROVIDED BY THE COPYRIGHT HOLDERS AND CONTRIBUTORS \"AS IS\" AND ANY EXPRESS OR IMPLIED WARRANTIES, INCLUDING, BUT NOT LIMITED TO, THE IMPLIED WARRANTIES OF MERCHANTABILITY AND FITNESS FOR A PARTICULAR PURPOSE ARE DISCLAIMED. IN NO EVENT SHALL THE COPYRIGHT HOLDER OR CONTRIBUTORS BE LIABLE FOR ANY DIRECT, INDIRECT, INCIDENTAL, SPECIAL, EXEMPLARY, OR CONSEQUENTIAL DAMAGES (INCLUDING, BUT NOT LIMITED TO, PROCUREMENT OF SUBSTITUTE GOODS OR SERVICES; LOSS OF USE, DATA, OR PROFITS; OR BUSINESS INTERRUPTION) HOWEVER CAUSED AND ON ANY THEORY OF LIABILITY, WHETHER IN CONTRACT, STRICT LIABILITY, OR TORT (INCLUDING NEGLIGENCE OR OTHERWISE) ARISING IN ANY WAY OUT OF THE USE OF THIS SOFTWARE, EVEN IF ADVISED OF THE POSSIBILITY OF SUCH DAMAGE.
******************************************************************************
Copyright Notice and Terms for PSI-MS (Proteomics Standards Initiative - Mass Spectrometry) Mass spectrometer output files and spectra interpretation
_____________________________________________________________________________
Created by Matt Chambers, Andreas Bertsch, Marius Kallhardt, Eric Deutsch Fredrik Levander, Pierre-Alain Binz, and Gerhard Mayer. Publisher: HUPO Proteomics Standards Initiative Mass Spectrometry Standards Working Group and HUPO Proteomics Standards Initiative Proteomics Informatics Working Group. This work is used pursuant to a Creative Commons license available here: http://creativecommons.org/licenses/by/3.0/legalcode

******************************************************************************
Attribution Notice for National Center for Biomedical Ontology materials.

This work contains material from the Cell Ontology and Clinical Measurement Ontology, available here: http://bioportal.bioontology.org/.
******************************************************************************
Attribution Notice for ChEBI
This work contains material from the European Bioinformatics Institute’s ChEBI database.
******************************************************************************
Attribution Notice for Quantities Units Dimensions Data Types (http://www.qudt.org/)
This work contains content from www.qudt.org and is used pursuant to a Creative Commons License available here: http://creativecommons.org/licenses/by-sa/3.0/us/legalcode. The original work may have been modified.
******************************************************************************
Copyright and Attribution Notice for Dublin Core Metadata Initiative Document
This work contains material from the following DCMI document used pursuant to a creative commons license available here: https://creativecommons.org/licenses/by/4.0/legalcode. This material may have been modified or changed.
Timestamped URL:          http://dublincore.org/documents/2012/06/14/dcmi-terms/
Date Issued:                       2012-06-14
Document Status:            This is a DCMI Recommendation.
Copyright © 1995-2015 DCMI. All Rights Reserved. DCMI liability, trademark/service mark, document use and software licensing rules apply.
******************************************************************************

""" ;
                                            dct:title "Derivative works attribution" .


###  http://purl.allotrope.org/voc/copyright
<http://purl.allotrope.org/voc/copyright> rdf:type owl:NamedIndividual ,
                                                   dct:RightsStatement ;
                                          dct:description "Copyright © 2015-2025 Allotrope Foundation" ;
                                          dct:rightsHolder <http://www.allotrope.org> ;
                                          dct:title "Copyright © 2015-2025 Allotrope Foundation" .


###  http://purl.allotrope.org/voc/creative-commons-attribution-license
<http://purl.allotrope.org/voc/creative-commons-attribution-license> rdf:type owl:NamedIndividual ;
                                                                     dct:description """This work is licensed under a Creative Commons Attribution 4.0 International License http://creativecommons.org/licenses/by/4.0/.

THESE MATERIALS ARE PROVIDED \"AS IS\" AND ALLOTROPE EXPRESSLY DISCLAIMS ALL WARRANTIES, EXPRESS, IMPLIED OR STATUTORY, INCLUDING, WITHOUT LIMITATION, THE WARRANTIES OF NON-INFRINGEMENT, TITLE, MERCHANTABILITY AND FITNESS FOR A PARTICULAR PURPOSE.

Copyright © 2015-2025 Allotrope Foundation
""" ;
                                                                     dct:rightsHolder <http://www.allotrope.org> ;
                                                                     dct:title "Creative Commons Attribution 4.0 International Public License" .


###  http://purl.allotrope.org/voc/iupac-copyright
<http://purl.allotrope.org/voc/iupac-copyright> rdf:type owl:NamedIndividual ,
                                                         dct:RightsStatement ;
                                                dct:description "Copyright © 2019 International Union of Pure Applied Chemistry" .


###  http://purl.allotrope.org/voc/iupac-license
<http://purl.allotrope.org/voc/iupac-license> rdf:type owl:NamedIndividual ,
                                                       dct:LicenseDocument ;
                                              dct:description "Reproduced by permission of International Union of Pure and Applied Chemistry" .


###  Generated by the OWL API (version 5.1.19) https://github.com/owlcs/owlapi/
