@prefix : <http://purl.allotrope.org/voc/afo/domain/WD/2025/06/moessbauer#> .
@prefix cl: <http://purl.obolibrary.org/obo/CL> .
@prefix go: <http://purl.obolibrary.org/obo/GO> .
@prefix ro: <http://purl.obolibrary.org/obo/RO> .
@prefix bfo: <http://purl.obolibrary.org/obo/BFO> .
@prefix dct: <http://purl.org/dc/terms/> .
@prefix iao: <http://purl.obolibrary.org/obo/IAO> .
@prefix obi: <http://purl.obolibrary.org/obo/OBI> .
@prefix owl: <http://www.w3.org/2002/07/owl#> .
@prefix rdf: <http://www.w3.org/1999/02/22-rdf-syntax-ns#> .
@prefix xml: <http://www.w3.org/XML/1998/namespace> .
@prefix xsd: <http://www.w3.org/2001/XMLSchema#> .
@prefix af-c: <http://purl.allotrope.org/ontologies/common#> .
@prefix af-e: <http://purl.allotrope.org/ontologies/equipment#> .
@prefix af-m: <http://purl.allotrope.org/ontologies/material#> .
@prefix af-p: <http://purl.allotrope.org/ontologies/process#> .
@prefix af-q: <http://purl.allotrope.org/ontologies/quality#> .
@prefix af-r: <http://purl.allotrope.org/ontologies/result#> .
@prefix af-x: <http://purl.allotrope.org/ontologies/property#> .
@prefix rdfs: <http://www.w3.org/2000/01/rdf-schema#> .
@prefix skos: <http://www.w3.org/2004/02/skos/core#> .
@prefix af-cur: <http://purl.allotrope.org/ontologies/curation#> .
@base <http://purl.allotrope.org/voc/afo/domain/WD/2025/06/moessbauer#> .

<http://purl.allotrope.org/voc/afo/domain/WD/2025/06/moessbauer> rdf:type owl:Ontology ;
                                                                            owl:versionIRI <http://purl.allotrope.org/voc/afo/domain/WD/2025/06/moessbauer> ;
                                                                            owl:imports <http://purl.allotrope.org/voc/afo/WD/2025/06/afo> ;
                                                                            dct:issued "2025-06-25T12:00:00Z"^^xsd:dateTime ;
                                                                            dct:license <http://purl.allotrope.org/voc/creative-commons-attribution-license> ;
                                                                            dct:modified "2025-04-04T12:00:00Z"^^xsd:dateTime ;
                                                                            dct:rights <http://purl.allotrope.org/voc/attribution> ,
                                                                                       <http://purl.allotrope.org/voc/copyright> ;
                                                                            dct:title "AFO Moessbauer Domain Ontology (WD/2025/06)" ;
                                                                            owl:priorVersion <http://purl.allotrope.org/voc/afo/domain/WD/2018/04/moessbauer> ;
                                                                            owl:versionInfo "WD/2025/06" .

#################################################################
#    Annotation properties
#################################################################

###  http://purl.allotrope.org/ontologies/property#AFX_0002796
af-x:AFX_0002796 rdf:type owl:AnnotationProperty .


###  http://purl.allotrope.org/ontologies/property#AFX_0002798
af-x:AFX_0002798 rdf:type owl:AnnotationProperty .


###  http://purl.allotrope.org/ontologies/property#AFX_0002809
af-x:AFX_0002809 rdf:type owl:AnnotationProperty .


###  http://purl.org/dc/terms/source
dct:source rdf:type owl:AnnotationProperty .


###  http://www.w3.org/2004/02/skos/core#altLabel
skos:altLabel rdf:type owl:AnnotationProperty .


###  http://www.w3.org/2004/02/skos/core#changeNote
skos:changeNote rdf:type owl:AnnotationProperty .


###  http://www.w3.org/2004/02/skos/core#definition
skos:definition rdf:type owl:AnnotationProperty .


###  http://www.w3.org/2004/02/skos/core#example
skos:example rdf:type owl:AnnotationProperty .


###  http://www.w3.org/2004/02/skos/core#note
skos:note rdf:type owl:AnnotationProperty .


###  http://www.w3.org/2004/02/skos/core#prefLabel
skos:prefLabel rdf:type owl:AnnotationProperty .


###  http://www.w3.org/2004/02/skos/core#scopeNote
skos:scopeNote rdf:type owl:AnnotationProperty .


#################################################################
#    Classes
#################################################################

###  http://purl.allotrope.org/ontologies/process#AFP_0000151
af-p:AFP_0000151 rdf:type owl:Class ;
                 rdfs:subClassOf af-p:AFP_0000317 ;
                 skos:altLabel "125Te Moessbauer spectroscopy" ,
                               "125Te Mossbauer spectroscopy" ,
                               "125Te recoil-free gamma-ray resonance absorption spectroscopy" ,
                               "tellurium-125 Moessbauer spectroscopy" ;
                 skos:definition "A type of spectroscopy where the intensity of a gamma-rays beam transmitted through a solid sample containing 125Te nuclei is detected. [CHMO]" ;
                 skos:prefLabel "125Te Mossbauer spectroscopy" .


###  http://purl.allotrope.org/ontologies/process#AFP_0000968
af-p:AFP_0000968 rdf:type owl:Class ;
                 rdfs:subClassOf af-p:AFP_0000317 ;
                 skos:altLabel "DC EMS" ,
                               "DCEMS" ,
                               "DS EMS" ,
                               "DS MS" ,
                               "DSEMS" ,
                               "DSMS" ,
                               "depth-selective Mossbauer spectrometry" ,
                               "depth-selective Moßbauer spectrometry" ,
                               "depth-selective Moßbauer spectroscopy" ,
                               "depth-selective Mössbauer spectrometry" ,
                               "depth-selective Mößbauer spectrometry" ,
                               "depth-selective Mößbauer spectroscopy" ,
                               "depth-selective conversion electron Mossbauer spectrometry" ,
                               "depth-selective conversion electron Moßbauer spectrometry" ,
                               "depth-selective conversion electron Moßbauer spectroscopy" ,
                               "depth-selective conversion electron Mösbauer spectrometry" ,
                               "depth-selective conversion electron Mössbauer spectroscopy" ,
                               "depth-selective conversion electron Mößbauer spectrometry" ,
                               "depth-selective conversion electron Mößbauer spectroscopy" ,
                               "depth-selective electron Mossbauer spectrometry" ,
                               "depth-selective electron Mossbauer spectroscopy" ,
                               "depth-selective electron Moßbauer spectrometry" ,
                               "depth-selective electron Moßbauer spectroscopy" ,
                               "depth-selective electron Mössbauer spectrometry" ,
                               "depth-selective electron Mössbauer spectroscopy" ,
                               "depth-selective electron Mößbauer spectrometry" ,
                               "depth-selective electron Mößbauer spectroscopy" ;
                 skos:changeNote "2016-02-03 Fixed spelling [OSTHUS]" ;
                 skos:definition "A type of spectroscopy where gamma-rays are absorbed by a sample resulting in the ejection of conversion electrons, the energy distribution of which is measured. [CHMO]" ;
                 skos:prefLabel "depth-selective Mossbauer spectroscopy" .


###  http://purl.allotrope.org/ontologies/process#AFP_0001021
af-p:AFP_0001021 rdf:type owl:Class ;
                 rdfs:subClassOf af-p:AFP_0000317 ;
                 skos:altLabel "129Xe Moessbauer spectrometry" ,
                               "129Xe Moessbauer spectroscopy" ,
                               "129Xe Mossbauer spectrometry" ,
                               "129Xe Mossbauer spectroscopy" ,
                               "129Xe Mössbauer spectrometry" ,
                               "129Xe Mössbauer spectroscopy" ,
                               "129Xe Mößbauer spectrometry" ,
                               "129Xe Mößbauer spectroscopy" ,
                               "129Xe recoil-free gamma-ray resonance absorption spectroscopy" ,
                               "xenon-129 Moessbauer spectroscopy" ,
                               "xenon-129 Mößbauer spectroscopy" ;
                 skos:definition "A type of spectroscopy where the intensity of a gamma-rays beam transmitted through a solid sample containing 129Xe nuclei is detected. [CHMO]" ;
                 skos:prefLabel "129Xe Mossbauer spectroscopy" .


###  http://purl.allotrope.org/ontologies/process#AFP_0001191
af-p:AFP_0001191 rdf:type owl:Class ;
                 rdfs:subClassOf af-p:AFP_0000317 ;
                 skos:altLabel "121Sb Moessbauer spectroscopy" ,
                               "121Sb Mossbauer spectroscopy" ,
                               "121Sb recoil-free gamma-ray resonance absorption spectroscopy" ,
                               "antimony-121 Moessbauer spectroscopy" ;
                 skos:definition "A type of spectroscopy where the intensity of a gamma-rays beam transmitted through a solid sample containing 121Sb nuclei is detected. [CHMO]" ;
                 skos:prefLabel "121Sb Mossbauer spectroscopy" .


###  http://purl.allotrope.org/ontologies/process#AFP_0001263
af-p:AFP_0001263 rdf:type owl:Class ;
                 rdfs:subClassOf af-p:AFP_0000317 ;
                 skos:altLabel "119Sn Moessbauer spectroscopy" ,
                               "119Sn Mossbauer spectroscopy" ,
                               "119Sn Mössbauer spectroscopy" ,
                               "119Sn Mößbauer spectroscopy" ,
                               "119Sn recoil-free gamma-ray resonance absorption spectroscopy" ,
                               "tin-119 Moessbauer spectroscopy" ,
                               "tin-119 Mößbauer spectroscopy" ;
                 skos:definition "A type of spectroscopy where the intensity of a gamma-rays beam transmitted through a solid sample containing 119Sn nuclei is detected. [CHMO]" ;
                 skos:prefLabel "119Sn Mossbauer spectroscopy" .


###  http://purl.allotrope.org/ontologies/process#AFP_0001724
af-p:AFP_0001724 rdf:type owl:Class ;
                 rdfs:subClassOf af-p:AFP_0000317 ;
                 skos:altLabel "127I Moessbauer spectroscopy" ,
                               "127I Mossbauer spectroscopy" ,
                               "127I Mössbauer spectroscopy" ,
                               "127I Mößbauer spectroscopy" ,
                               "127I recoil-free gamma-ray resonance absorption spectroscopy" ,
                               "iodine-127 Moessbauer spectroscopy" ,
                               "iodine-127 Mößbauer spectroscopy" ;
                 skos:definition "A type of spectroscopy where the intensity of a gamma-rays beam transmitted through a solid sample containing 127I nuclei is detected. [CHMO]" ;
                 skos:prefLabel "127I Mossbauer spectroscopy" .


###  http://purl.allotrope.org/ontologies/process#AFP_0001808
af-p:AFP_0001808 rdf:type owl:Class ;
                 rdfs:subClassOf af-p:AFP_0000317 ;
                 skos:altLabel "57Fe Moessbauer spectroscopy" ,
                               "57Fe Mossbauer spectroscopy" ,
                               "57Fe Mössbauer spectroscopy" ,
                               "57Fe Mößbauer spectroscopy" ,
                               "57Fe recoil-free gamma-ray resonance absorption spectroscopy" ,
                               "iron-57 Moessbauer spectroscopy" ,
                               "iron-57 Mößbauer spectroscopy" ;
                 skos:definition "A type of spectroscopy where the intensity of a gamma-rays beam transmitted through a solid sample containing 57Fe nuclei is detected. [CHMO]" ;
                 skos:prefLabel "57Fe Mossbauer spectroscopy" .


###  http://purl.allotrope.org/ontologies/process#AFP_0001829
af-p:AFP_0001829 rdf:type owl:Class ;
                 rdfs:subClassOf af-p:AFP_0000317 ;
                 skos:altLabel "151Eu Moessbauer spectroscopy" ,
                               "151Eu Mossbauer spectroscopy" ,
                               "151Eu recoil-free gamma-ray resonance absorption spectroscopy" ,
                               "europium-151 Moessbauer spectroscopy" ;
                 skos:definition "A type of spectroscopy where the intensity of a gamma-rays beam transmitted through a solid sample containing 151Eu nuclei is detected. [CHMO]" ;
                 skos:prefLabel "151Eu Mossbauer spectroscopy" .


###  http://purl.allotrope.org/ontologies/process#AFP_0001862
af-p:AFP_0001862 rdf:type owl:Class ;
                 rdfs:subClassOf af-p:AFP_0000317 ;
                 skos:altLabel "197Au Moessbauer spectroscopy" ,
                               "197Au Mossbauer spectroscopy" ,
                               "197Au recoil-free gamma-ray resonance absorption spectroscopy" ,
                               "gold-197 Moessbauer spectroscopy" ;
                 skos:definition "A type of spectroscopy where the intensity of a gamma-rays beam transmitted through a solid sample containing 197Au nuclei is detected. [CHMO]" ;
                 skos:prefLabel "197Au Mossbauer spectroscopy" .


###  http://purl.allotrope.org/ontologies/process#AFP_0002173
af-p:AFP_0002173 rdf:type owl:Class ;
                 rdfs:subClassOf af-p:AFP_0000317 ;
                 skos:altLabel "129I Moessbauer spectroscopy" ,
                               "129I Mossbauer spectroscopy" ,
                               "129I recoil-free gamma-ray resonance absorption spectroscopy" ,
                               "iodine-129 Moessbauer spectroscopy" ;
                 skos:definition "A type of spectroscopy where the intensity of a gamma-rays beam transmitted through a solid sample containing 129I nuclei is detected. [CHMO]" ;
                 skos:prefLabel "129I Mossbauer spectroscopy" .


#################################################################
#    Individuals
#################################################################

###  http://purl.allotrope.org/voc/attribution
<http://purl.allotrope.org/voc/attribution> rdf:type owl:NamedIndividual ,
                                                     dct:RightsStatement ;
                                            dct:description """
These taxonomies contain material or may constitute derivative works of material which may be subject to copyright by one of the following organizations.  By using these taxonomies, you agree to the following terms and conditions applicable to its contents:
******************************************************************************
Copyright Notice and Terms for IUPAC Gold Book
______________________________________________________________________________
Copyright © 1998, Regents of the University of California
All rights reserved.
Redistribution and use in source and binary forms, with or without modification, are permitted provided that the following conditions are met:
1. Redistributions of source code must retain the above copyright notice, this list of conditions and the following disclaimer.
2. Redistributions in binary form must reproduce the above copyright notice, this list of conditions and the following disclaimer in the documentation and/or other materials provided with the distribution.
THIS SOFTWARE IS PROVIDED BY THE COPYRIGHT HOLDERS AND CONTRIBUTORS \"AS IS\" AND ANY EXPRESS OR IMPLIED WARRANTIES, INCLUDING, BUT NOT LIMITED TO, THE IMPLIED WARRANTIES OF MERCHANTABILITY AND FITNESS FOR A PARTICULAR PURPOSE ARE DISCLAIMED. IN NO EVENT SHALL THE COPYRIGHT HOLDER OR CONTRIBUTORS BE LIABLE FOR ANY DIRECT, INDIRECT, INCIDENTAL, SPECIAL, EXEMPLARY, OR CONSEQUENTIAL DAMAGES (INCLUDING, BUT NOT LIMITED TO, PROCUREMENT OF SUBSTITUTE GOODS OR SERVICES; LOSS OF USE, DATA, OR PROFITS; OR BUSINESS INTERRUPTION) HOWEVER CAUSED AND ON ANY THEORY OF LIABILITY, WHETHER IN CONTRACT, STRICT LIABILITY, OR TORT (INCLUDING NEGLIGENCE OR OTHERWISE) ARISING IN ANY WAY OUT OF THE USE OF THIS SOFTWARE, EVEN IF ADVISED OF THE POSSIBILITY OF SUCH DAMAGE.
******************************************************************************
Copyright Notice and Terms for PSI-MS (Proteomics Standards Initiative - Mass Spectrometry) Mass spectrometer output files and spectra interpretation
_____________________________________________________________________________
Created by Matt Chambers, Andreas Bertsch, Marius Kallhardt, Eric Deutsch Fredrik Levander, Pierre-Alain Binz, and Gerhard Mayer. Publisher: HUPO Proteomics Standards Initiative Mass Spectrometry Standards Working Group and HUPO Proteomics Standards Initiative Proteomics Informatics Working Group. This work is used pursuant to a Creative Commons license available here: http://creativecommons.org/licenses/by/3.0/legalcode

******************************************************************************
Attribution Notice for National Center for Biomedical Ontology materials.

This work contains material from the Cell Ontology and Clinical Measurement Ontology, available here: http://bioportal.bioontology.org/.
******************************************************************************
Attribution Notice for ChEBI
This work contains material from the European Bioinformatics Institute’s ChEBI database.
******************************************************************************
Attribution Notice for Quantities Units Dimensions Data Types (http://www.qudt.org/)
This work contains content from www.qudt.org and is used pursuant to a Creative Commons License available here: http://creativecommons.org/licenses/by-sa/3.0/us/legalcode. The original work may have been modified.
******************************************************************************
Copyright and Attribution Notice for Dublin Core Metadata Initiative Document
This work contains material from the following DCMI document used pursuant to a creative commons license available here: https://creativecommons.org/licenses/by/4.0/legalcode. This material may have been modified or changed.
Timestamped URL:          http://dublincore.org/documents/2012/06/14/dcmi-terms/
Date Issued:                       2012-06-14
Document Status:            This is a DCMI Recommendation.
Copyright © 1995-2015 DCMI. All Rights Reserved. DCMI liability, trademark/service mark, document use and software licensing rules apply.
******************************************************************************

""" ;
                                            dct:title "Derivative works attribution" .


###  http://purl.allotrope.org/voc/copyright
<http://purl.allotrope.org/voc/copyright> rdf:type owl:NamedIndividual ,
                                                   dct:RightsStatement ;
                                          dct:description "Copyright © 2019 Allotrope Foundation" ;
                                          dct:rightsHolder <http://www.allotrope.org> ;
                                          dct:title "Copyright © 2019 Allotrope Foundation" .


###  http://purl.allotrope.org/voc/creative-commons-attribution-license
<http://purl.allotrope.org/voc/creative-commons-attribution-license> rdf:type owl:NamedIndividual ,
                                                                              dct:LicenseDocument ;
                                                                     dct:description """This work is licensed under a Creative Commons Attribution 4.0 International License http://creativecommons.org/licenses/by/4.0/.

THESE MATERIALS ARE PROVIDED \"AS IS\" AND ALLOTROPE EXPRESSLY DISCLAIMS ALL WARRANTIES, EXPRESS, IMPLIED OR STATUTORY, INCLUDING, WITHOUT LIMITATION, THE WARRANTIES OF NON-INFRINGEMENT, TITLE, MERCHANTABILITY AND FITNESS FOR A PARTICULAR PURPOSE.

Copyright © 2015-2025 Allotrope Foundation
""" ;
                                                                     dct:title "Creative Commons Attribution 4.0 International Public License" .


###  Generated by the OWL API (version 5.1.19) https://github.com/owlcs/owlapi/
