@prefix : <http://purl.allotrope.org/voc/afo/domain/WD/2025/06/titration#> .
@prefix cl: <http://purl.obolibrary.org/obo/CL> .
@prefix go: <http://purl.obolibrary.org/obo/GO> .
@prefix ro: <http://purl.obolibrary.org/obo/RO> .
@prefix bfo: <http://purl.obolibrary.org/obo/BFO> .
@prefix dct: <http://purl.org/dc/terms/> .
@prefix iao: <http://purl.obolibrary.org/obo/IAO> .
@prefix obi: <http://purl.obolibrary.org/obo/OBI> .
@prefix owl: <http://www.w3.org/2002/07/owl#> .
@prefix pav: <http://purl.org/pav/> .
@prefix rdf: <http://www.w3.org/1999/02/22-rdf-syntax-ns#> .
@prefix xml: <http://www.w3.org/XML/1998/namespace> .
@prefix xsd: <http://www.w3.org/2001/XMLSchema#> .
@prefix af-c: <http://purl.allotrope.org/ontologies/common#> .
@prefix af-e: <http://purl.allotrope.org/ontologies/equipment#> .
@prefix af-m: <http://purl.allotrope.org/ontologies/material#> .
@prefix af-p: <http://purl.allotrope.org/ontologies/process#> .
@prefix af-q: <http://purl.allotrope.org/ontologies/quality#> .
@prefix af-r: <http://purl.allotrope.org/ontologies/result#> .
@prefix af-x: <http://purl.allotrope.org/ontologies/property#> .
@prefix rdfs: <http://www.w3.org/2000/01/rdf-schema#> .
@prefix skos: <http://www.w3.org/2004/02/skos/core#> .
@prefix af-fn: <http://purl.allotrope.org/ontologies/function#> .
@prefix af-re: <http://purl.allotrope.org/ontologies/realizable#> .
@prefix af-rl: <http://purl.allotrope.org/ontologies/role#> .
@prefix af-cur: <http://purl.allotrope.org/ontologies/curation#> .
@base <http://purl.allotrope.org/voc/afo/domain/WD/2025/06/titration#> .

<http://purl.allotrope.org/voc/afo/domain/WD/2025/06/titration> rdf:type owl:Ontology ;
                                                                           owl:versionIRI <http://purl.allotrope.org/voc/afo/domain/WD/2025/06/titration> ;
                                                                           owl:imports <http://purl.allotrope.org/voc/afo/WD/2025/06/afo> ,
                                                                                       <http://purl.allotrope.org/voc/afo/domain/REC/2025/06/titration> ,
                                                                                       <http://purl.allotrope.org/voc/afo/domain/WD/2025/06/electrochemistry> ,
                                                                                       <http://purl.allotrope.org/voc/afo/domain/WD/2025/06/weighing> ;
                                                                           dct:issued "2025-06-25T12:00:00Z"^^xsd:dateTime ;
                                                                           dct:license <http://purl.allotrope.org/voc/creative-commons-attribution-license> ;
                                                                           dct:modified "2025-04-04T12:00:00Z"^^xsd:dateTime ;
                                                                           dct:rights <http://purl.allotrope.org/voc/attribution> ,
                                                                                      <http://purl.allotrope.org/voc/copyright> ;
                                                                           dct:title "AFO Titration Domain Ontology (WD/2025/06)" ;
                                                                           owl:priorVersion <http://purl.allotrope.org/voc/afo/domain/WD/2025/03/titration> ;
                                                                           owl:versionInfo "WD/2025/06" .

#################################################################
#    Annotation properties
#################################################################

###  http://purl.allotrope.org/ontologies/property#AFX_0002796
af-x:AFX_0002796 rdf:type owl:AnnotationProperty .


###  http://purl.allotrope.org/ontologies/property#AFX_0002798
af-x:AFX_0002798 rdf:type owl:AnnotationProperty .


###  http://purl.allotrope.org/ontologies/property#AFX_0002809
af-x:AFX_0002809 rdf:type owl:AnnotationProperty .


###  http://purl.org/dc/terms/source
dct:source rdf:type owl:AnnotationProperty .


###  http://www.w3.org/2004/02/skos/core#altLabel
skos:altLabel rdf:type owl:AnnotationProperty .


###  http://www.w3.org/2004/02/skos/core#changeNote
skos:changeNote rdf:type owl:AnnotationProperty .


###  http://www.w3.org/2004/02/skos/core#definition
skos:definition rdf:type owl:AnnotationProperty .


###  http://www.w3.org/2004/02/skos/core#example
skos:example rdf:type owl:AnnotationProperty .


###  http://www.w3.org/2004/02/skos/core#note
skos:note rdf:type owl:AnnotationProperty .


###  http://www.w3.org/2004/02/skos/core#prefLabel
skos:prefLabel rdf:type owl:AnnotationProperty .


###  http://www.w3.org/2004/02/skos/core#scopeNote
skos:scopeNote rdf:type owl:AnnotationProperty .


#################################################################
#    Classes
#################################################################

###  http://purl.allotrope.org/ontologies/equipment#AFE_0000049
af-e:AFE_0000049 rdf:type owl:Class .


###  http://purl.allotrope.org/ontologies/equipment#AFE_0000053
af-e:AFE_0000053 rdf:type owl:Class ;
                 rdfs:subClassOf af-e:AFE_0000531 ;
                 skos:definition "A generator electrode with a diaphragm. [Allotrope]" ;
                 skos:prefLabel "generator electrode with diaphragm" .


###  http://purl.allotrope.org/ontologies/equipment#AFE_0000304
af-e:AFE_0000304 rdf:type owl:Class ;
                 rdfs:subClassOf af-e:AFE_0000299 ;
                 skos:altLabel "Karl Fischer homogeniser"@en-gb ,
                               "Karl Fischer homogenizer" ;
                 skos:definition "A homogenizer that is used in the case of Karl Fischer analysis to aid in sample dissolution. [Allotrope]" ;
                 skos:prefLabel "Karl-Fischer homogeniser"@en-gb ,
                                "Karl-Fischer homogenizer" .


###  http://purl.allotrope.org/ontologies/equipment#AFE_0000324
af-e:AFE_0000324 rdf:type owl:Class ;
                 rdfs:subClassOf af-e:AFE_0000115 ;
                 skos:altLabel "Karl Fischer coulometry cell" ;
                 skos:definition "A titration cell used for Karl Fischer analysis. [Allotrope]" ;
                 skos:prefLabel "Karl-Fischer coulometry cell" .


###  http://purl.allotrope.org/ontologies/equipment#AFE_0000502
af-e:AFE_0000502 rdf:type owl:Class ;
                 rdfs:subClassOf af-e:AFE_0000531 ;
                 skos:definition "A generator electrode without a diaphragm. [Allotrope]" ;
                 skos:prefLabel "generator electrode without diaphragm" .


###  http://purl.allotrope.org/ontologies/equipment#AFE_0000531
af-e:AFE_0000531 rdf:type owl:Class ;
                 rdfs:subClassOf af-e:AFE_0000049 ;
                 skos:definition "A generator anodic Karl Fischer electrode (there is no separate cathode compartment with reduction taking place on the platinum surface). [Allotrope]" ;
                 skos:prefLabel "generator electrode" .


###  http://purl.allotrope.org/ontologies/process#AFP_0000293
af-p:AFP_0000293 rdf:type owl:Class ;
                 rdfs:subClassOf af-p:AFP_0000505 ;
                 skos:altLabel "high frequency conductometric titration" ;
                 skos:definition "The process of determining the quantity of a sample by adding measured increments of a titrant until the end-point is reached. The titration is monitored by measuring the conductance of the solution, the current is provided by a high-frequency source. [CHMO]" ;
                 skos:prefLabel "high-frequency conductometric titration" .


###  http://purl.allotrope.org/ontologies/process#AFP_0000448
af-p:AFP_0000448 rdf:type owl:Class ;
                 rdfs:subClassOf af-p:AFP_0001775 ;
                 skos:definition "The process of determining the quantity of a sample by adding measured increments of a titrant until the end-point is reached. The titration is followed by measuring the intensity/wavelength of fluorescence emitted by the sample. [CHMO]" ;
                 skos:prefLabel "fluorescence titration" .


###  http://purl.allotrope.org/ontologies/process#AFP_0000505
af-p:AFP_0000505 rdf:type owl:Class ;
                 rdfs:subClassOf af-p:AFP_0001916 ;
                 skos:definition "The process of determining the quantity of a sample by adding measured increments of a titrant until the end-point is reached. The titration is monitored by measuring the conductance of the solution. [CHMO]" ;
                 skos:prefLabel "conductometric titration" .


###  http://purl.allotrope.org/ontologies/process#AFP_0000555
af-p:AFP_0000555 rdf:type owl:Class ;
                 rdfs:subClassOf af-p:AFP_0000154 ;
                 skos:altLabel "ITC" ,
                               "isothermal titration microcalorimetry" ,
                               "titration calorimetry" ;
                 skos:definition "The measurement of thermodynamic parameters (e.g. enthalpy) at constant temperature during a titration. [CHMO]" ;
                 skos:prefLabel "isothermal titration calorimetry" .


###  http://purl.allotrope.org/ontologies/process#AFP_0000700
af-p:AFP_0000700 rdf:type owl:Class ;
                 rdfs:subClassOf af-p:AFP_0001916 ;
                 skos:definition "The process of determining the quantity of a sample by adding measured increments of a titrant until the end-point is reached. The titration performed in a calorimeter which produces a plot of heat change vs. volume of titrant. [CHMO]" ;
                 skos:prefLabel "calorimetric titration" .


###  http://purl.allotrope.org/ontologies/process#AFP_0000759
af-p:AFP_0000759 rdf:type owl:Class ;
                 af-x:AFX_0002865 <http://purl.allotrope.org/voc/afo/domain/WD/2025/06/nmr> ;
                 skos:definition "A technique or procedure applied in nuclear magnetic resonance experiments. [CHMO]" ;
                 skos:prefLabel "nuclear magnetic resonance method" .


###  http://purl.allotrope.org/ontologies/process#AFP_0000897
af-p:AFP_0000897 rdf:type owl:Class ;
                 rdfs:subClassOf af-p:AFP_0001501 ;
                 skos:altLabel "UV titration" ,
                               "ultra-violet titration" ;
                 skos:definition "The process of determining the quantity of a sample by adding measured increments of a titrant until the end-point, at which essentially all of the sample has reacted, is reached. The titration is followed by measuring the absorbance of radiation in the ultraviolet range (190-400 nm) by the sample. [CHMO]" ;
                 skos:prefLabel "ultraviolet titration" .


###  http://purl.allotrope.org/ontologies/process#AFP_0000912
af-p:AFP_0000912 rdf:type owl:Class ;
                 rdfs:subClassOf af-p:AFP_0001916 ;
                 skos:definition "The process of determining the quantity of a sample by adding measured increments of a titrant until the end-point, at which essentially all of the sample has reacted, is reached. The titration is followed by measuring the relative permittivity of the solution as a function of the solution volume. [CHMO]" ;
                 skos:prefLabel "dielectrometric titration" .


###  http://purl.allotrope.org/ontologies/process#AFP_0001052
af-p:AFP_0001052 rdf:type owl:Class ;
                 rdfs:subClassOf af-p:AFP_0001510 ;
                 skos:altLabel "acidimetry" ;
                 skos:definition "The process of determining the quantity of a sample (a base) by adding measured increments of a titrant (an acid) until the endpoint, at which essentially all of the sample has reacted, is reached. [CHMO]" ;
                 skos:prefLabel "acidimetric titration" .


###  http://purl.allotrope.org/ontologies/process#AFP_0001067
af-p:AFP_0001067 rdf:type owl:Class ;
                 rdfs:subClassOf af-p:AFP_0001292 ;
                 skos:altLabel "EPR-monitored oxidation-reduction titration" ,
                               "EPR-monitored redox titration" ,
                               "ESR-monitored oxidation-reduction titration" ,
                               "ESR-monitored redox titration" ,
                               "electron paramagnetic resonance monitored redox titration" ,
                               "electron spin resonance monitored oxidation-reduction titration" ,
                               "electron spin resonance monitored redox titration" ;
                 skos:definition "The process of determining the quantity of a sample by monitoring a redox process until the endpoint, at which essentially all of the sample has reacted, is reached. The titration is followed by monitoring the amplitude of an EPR signal (the response of an atom with an unpaired electron to a perturbing magnetic field) from one of the reactants. [CHMO]" ;
                 skos:prefLabel "electron paramagnetic resonance monitored oxidation-reduction titration" .


###  http://purl.allotrope.org/ontologies/process#AFP_0001292
af-p:AFP_0001292 rdf:type owl:Class .


###  http://purl.allotrope.org/ontologies/process#AFP_0001501
af-p:AFP_0001501 rdf:type owl:Class ;
                 rdfs:subClassOf af-p:AFP_0001916 ;
                 skos:altLabel "absorbance titration" ,
                               "absorption spectral titration" ;
                 skos:definition "The process of determining the quantity of a sample by adding measured increments of a titrant until the end-point, at which essentially all of the sample has reacted, is reached. The titration is followed by measuring the absorbance of radiation by the sample. [CHMO]" ;
                 skos:prefLabel "absorption titration" .


###  http://purl.allotrope.org/ontologies/process#AFP_0001510
af-p:AFP_0001510 rdf:type owl:Class .


###  http://purl.allotrope.org/ontologies/process#AFP_0001604
af-p:AFP_0001604 rdf:type owl:Class ;
                 rdfs:subClassOf af-p:AFP_0001501 ;
                 skos:definition "The process of determining the quantity of a sample by adding measured increments of a titrant until the end-point, at which essentially all of the sample has reacted, is reached. The titration is followed by measuring the absorbance of radiation in the range ultraviolet to near-infrared (0.1-2.5 µm) by the sample. [CHMO]" ;
                 skos:prefLabel "spectrophotometric titration" .


###  http://purl.allotrope.org/ontologies/process#AFP_0001663
af-p:AFP_0001663 rdf:type owl:Class ;
                 rdfs:subClassOf af-p:AFP_0001501 ;
                 skos:altLabel "CD titration" ,
                               "CD titration experiment" ,
                               "CD titration experiments" ;
                 skos:definition "The process of determining the quantity of a sample by adding measured increments of a titrant until the end-point, at which essentially all of the sample has reacted, is reached. The titration is followed by measuring the differential absorption of left- and right-handed circularly polarised light by the sample. [CHMO]" ;
                 skos:prefLabel "circular dichroism titration" .


###  http://purl.allotrope.org/ontologies/process#AFP_0001775
af-p:AFP_0001775 rdf:type owl:Class ;
                 rdfs:subClassOf af-p:AFP_0001916 ;
                 skos:definition "The process of determining the quantity of a sample by adding measured increments of a titrant until the end-point is reached. The titration is followed by measuring the intensity/wavelength of radiation emitted by the sample. [CHMO]" ;
                 skos:prefLabel "emission titration" .


###  http://purl.allotrope.org/ontologies/process#AFP_0002377
af-p:AFP_0002377 rdf:type owl:Class ;
                 rdfs:subClassOf af-p:AFP_0000759 ,
                                 af-p:AFP_0001916 ;
                 skos:altLabel "NMR titration" ;
                 skos:definition "The process of determining the quantity of a sample by adding measured increments of a titrant until the end-point is reached. The titration is monitored by observing the changes in sucessive NMR spectra, taken after each addition of titrant. [CHMO]" ;
                 skos:prefLabel "nuclear magnetic resonance titration" .


###  http://purl.allotrope.org/ontologies/process#AFP_0002378
af-p:AFP_0002378 rdf:type owl:Class ;
                 rdfs:subClassOf af-p:AFP_0001510 ;
                 skos:altLabel "alkalimetry" ;
                 skos:definition "The process of determining the quantity of a sample (an acid) by adding measured increments of a titrant (a base) until the endpoint, at which essentially all of the sample has reacted, is reached. [CHMO]" ;
                 skos:prefLabel "alkalimetric titration" .


###  http://purl.allotrope.org/ontologies/process#AFP_0002390
af-p:AFP_0002390 rdf:type owl:Class ;
                 rdfs:subClassOf af-p:AFP_0001916 ;
                 skos:definition "The process of determining the quantity of a sample by adding measured increments of a titrant until the end-point, at which essentially all of the sample has reacted, is reached. The titration is followed by measuring the potential difference between indicator and reference electrodes under conditions where the current passed is sufficiently small to maintain thermodynamic equilibrium. [CHMO]" ;
                 skos:prefLabel "potentiometric titration" .


###  http://purl.allotrope.org/ontologies/result#AFR_0000043
af-r:AFR_0000043 rdf:type owl:Class ;
                 rdfs:subClassOf af-r:AFR_0000490 ;
                 skos:altLabel "fluorescence spectral titration data" ,
                               "fluorescence titration data" ,
                               "fluorescence titration plot" ;
                 skos:definition "A plot of volume of titrant vs. fluorescence intensity obtained from a fluorescence titration experiment. [CHMO]" ;
                 skos:prefLabel "fluorescence titration curve" .


###  http://purl.allotrope.org/ontologies/result#AFR_0000117
af-r:AFR_0000117 rdf:type owl:Class ;
                 rdfs:subClassOf af-r:AFR_0000490 ;
                 skos:altLabel "absorbance titration data" ,
                               "absorbance titration plot" ,
                               "absorption spectral titration data" ,
                               "absorption titration data" ,
                               "absorption titration plot" ;
                 skos:definition "A plot of volume of titrant vs. absorbance obtained from an absorbance titration experiment. [CHMO]" ;
                 skos:prefLabel "absorbance titration curve" .


#################################################################
#    Individuals
#################################################################

###  http://purl.allotrope.org/voc/attribution
<http://purl.allotrope.org/voc/attribution> rdf:type owl:NamedIndividual ,
                                                     dct:RightsStatement ;
                                            dct:description """
These taxonomies contain material or may constitute derivative works of material which may be subject to copyright by one of the following organizations.  By using these taxonomies, you agree to the following terms and conditions applicable to its contents:
******************************************************************************
Copyright Notice and Terms for IUPAC Gold Book
______________________________________________________________________________
Copyright © 1998, Regents of the University of California
All rights reserved.
Redistribution and use in source and binary forms, with or without modification, are permitted provided that the following conditions are met:
1. Redistributions of source code must retain the above copyright notice, this list of conditions and the following disclaimer.
2. Redistributions in binary form must reproduce the above copyright notice, this list of conditions and the following disclaimer in the documentation and/or other materials provided with the distribution.
THIS SOFTWARE IS PROVIDED BY THE COPYRIGHT HOLDERS AND CONTRIBUTORS \"AS IS\" AND ANY EXPRESS OR IMPLIED WARRANTIES, INCLUDING, BUT NOT LIMITED TO, THE IMPLIED WARRANTIES OF MERCHANTABILITY AND FITNESS FOR A PARTICULAR PURPOSE ARE DISCLAIMED. IN NO EVENT SHALL THE COPYRIGHT HOLDER OR CONTRIBUTORS BE LIABLE FOR ANY DIRECT, INDIRECT, INCIDENTAL, SPECIAL, EXEMPLARY, OR CONSEQUENTIAL DAMAGES (INCLUDING, BUT NOT LIMITED TO, PROCUREMENT OF SUBSTITUTE GOODS OR SERVICES; LOSS OF USE, DATA, OR PROFITS; OR BUSINESS INTERRUPTION) HOWEVER CAUSED AND ON ANY THEORY OF LIABILITY, WHETHER IN CONTRACT, STRICT LIABILITY, OR TORT (INCLUDING NEGLIGENCE OR OTHERWISE) ARISING IN ANY WAY OUT OF THE USE OF THIS SOFTWARE, EVEN IF ADVISED OF THE POSSIBILITY OF SUCH DAMAGE.
******************************************************************************
Copyright Notice and Terms for PSI-MS (Proteomics Standards Initiative - Mass Spectrometry) Mass spectrometer output files and spectra interpretation
_____________________________________________________________________________
Created by Matt Chambers, Andreas Bertsch, Marius Kallhardt, Eric Deutsch Fredrik Levander, Pierre-Alain Binz, and Gerhard Mayer. Publisher: HUPO Proteomics Standards Initiative Mass Spectrometry Standards Working Group and HUPO Proteomics Standards Initiative Proteomics Informatics Working Group. This work is used pursuant to a Creative Commons license available here: http://creativecommons.org/licenses/by/3.0/legalcode

******************************************************************************
Attribution Notice for National Center for Biomedical Ontology materials.

This work contains material from the Cell Ontology and Clinical Measurement Ontology, available here: http://bioportal.bioontology.org/.
******************************************************************************
Attribution Notice for ChEBI
This work contains material from the European Bioinformatics Institute’s ChEBI database.
******************************************************************************
Attribution Notice for Quantities Units Dimensions Data Types (http://www.qudt.org/)
This work contains content from www.qudt.org and is used pursuant to a Creative Commons License available here: http://creativecommons.org/licenses/by-sa/3.0/us/legalcode. The original work may have been modified.
******************************************************************************
Copyright and Attribution Notice for Dublin Core Metadata Initiative Document
This work contains material from the following DCMI document used pursuant to a creative commons license available here: https://creativecommons.org/licenses/by/4.0/legalcode. This material may have been modified or changed.
Timestamped URL:          http://dublincore.org/documents/2012/06/14/dcmi-terms/
Date Issued:                       2012-06-14
Document Status:            This is a DCMI Recommendation.
Copyright © 1995-2015 DCMI. All Rights Reserved. DCMI liability, trademark/service mark, document use and software licensing rules apply.
******************************************************************************

""" ;
                                            dct:title "Derivative works attribution" .


###  http://purl.allotrope.org/voc/copyright
<http://purl.allotrope.org/voc/copyright> rdf:type owl:NamedIndividual ,
                                                   dct:RightsStatement ;
                                          dct:description "(c) 2017 Allotrope Foundation" ;
                                          dct:title "(c) 2017 Allotrope Foundation" .


###  http://purl.allotrope.org/voc/creative-commons-attribution-license
<http://purl.allotrope.org/voc/creative-commons-attribution-license> rdf:type owl:NamedIndividual ,
                                                                              dct:LicenseDocument ;
                                                                     dct:description """This work is licensed under a Creative Commons Attribution 4.0 International License http://creativecommons.org/licenses/by/4.0/.

THESE MATERIALS ARE PROVIDED \"AS IS\" AND ALLOTROPE EXPRESSLY DISCLAIMS ALL WARRANTIES, EXPRESS, IMPLIED OR STATUTORY, INCLUDING, WITHOUT LIMITATION, THE WARRANTIES OF NON-INFRINGEMENT, TITLE, MERCHANTABILITY AND FITNESS FOR A PARTICULAR PURPOSE.

Copyright © 2015-2025 Allotrope Foundation
""" ;
                                                                     dct:title "Creative Commons Attribution 4.0 International Public License" .


###  http://purl.allotrope.org/voc/afo/domain/WD/2018/04/titration
<http://purl.allotrope.org/voc/afo/domain/WD/2018/04/titration> rdf:type owl:NamedIndividual ;
                                                                dct:rightsHolder <http://www.allotrope.org> .


###  Generated by the OWL API (version 5.1.19) https://github.com/owlcs/owlapi/
