@prefix : <http://purl.allotrope.org/voc/afo/domain/WD/2025/06/velocimetry#> .
@prefix cl: <http://purl.obolibrary.org/obo/CL> .
@prefix go: <http://purl.obolibrary.org/obo/GO> .
@prefix ro: <http://purl.obolibrary.org/obo/RO> .
@prefix bfo: <http://purl.obolibrary.org/obo/BFO> .
@prefix dct: <http://purl.org/dc/terms/> .
@prefix iao: <http://purl.obolibrary.org/obo/IAO> .
@prefix obi: <http://purl.obolibrary.org/obo/OBI> .
@prefix owl: <http://www.w3.org/2002/07/owl#> .
@prefix rdf: <http://www.w3.org/1999/02/22-rdf-syntax-ns#> .
@prefix xml: <http://www.w3.org/XML/1998/namespace> .
@prefix xsd: <http://www.w3.org/2001/XMLSchema#> .
@prefix af-c: <http://purl.allotrope.org/ontologies/common#> .
@prefix af-e: <http://purl.allotrope.org/ontologies/equipment#> .
@prefix af-m: <http://purl.allotrope.org/ontologies/material#> .
@prefix af-p: <http://purl.allotrope.org/ontologies/process#> .
@prefix af-q: <http://purl.allotrope.org/ontologies/quality#> .
@prefix af-r: <http://purl.allotrope.org/ontologies/result#> .
@prefix af-x: <http://purl.allotrope.org/ontologies/property#> .
@prefix rdfs: <http://www.w3.org/2000/01/rdf-schema#> .
@prefix skos: <http://www.w3.org/2004/02/skos/core#> .
@prefix af-cur: <http://purl.allotrope.org/ontologies/curation#> .
@base <http://purl.allotrope.org/voc/afo/domain/WD/2025/06/velocimetry#> .

<http://purl.allotrope.org/voc/afo/domain/WD/2025/06/velocimetry> rdf:type owl:Ontology ;
                                                                             owl:versionIRI <http://purl.allotrope.org/voc/afo/domain/WD/2025/06/velocimetry> ;
                                                                             owl:imports <http://purl.allotrope.org/voc/afo/WD/2025/06/afo> ;
                                                                             dct:issued "2025-06-25T12:00:00Z"^^xsd:dateTime ;
                                                                             dct:license <http://purl.allotrope.org/voc/creative-commons-attribution-license> ;
                                                                             dct:modified "2025-04-04T12:00:00Z"^^xsd:dateTime ;
                                                                             dct:rights <http://purl.allotrope.org/voc/attribution> ,
                                                                                        <http://purl.allotrope.org/voc/copyright> ;
                                                                             dct:title "AFO Velocimetry Domain Ontology (WD/2025/06)" ;
                                                                             owl:priorVersion <http://purl.allotrope.org/voc/afo/domain/WD/2018/04/velocimetry> ;
                                                                             owl:versionInfo "WD/2025/06" .

#################################################################
#    Annotation properties
#################################################################

###  http://purl.allotrope.org/ontologies/property#AFX_0002796
af-x:AFX_0002796 rdf:type owl:AnnotationProperty .


###  http://purl.allotrope.org/ontologies/property#AFX_0002798
af-x:AFX_0002798 rdf:type owl:AnnotationProperty .


###  http://purl.allotrope.org/ontologies/property#AFX_0002809
af-x:AFX_0002809 rdf:type owl:AnnotationProperty .


###  http://purl.org/dc/terms/source
dct:source rdf:type owl:AnnotationProperty .


###  http://www.w3.org/2004/02/skos/core#altLabel
skos:altLabel rdf:type owl:AnnotationProperty .


###  http://www.w3.org/2004/02/skos/core#changeNote
skos:changeNote rdf:type owl:AnnotationProperty .


###  http://www.w3.org/2004/02/skos/core#definition
skos:definition rdf:type owl:AnnotationProperty .


###  http://www.w3.org/2004/02/skos/core#example
skos:example rdf:type owl:AnnotationProperty .


###  http://www.w3.org/2004/02/skos/core#note
skos:note rdf:type owl:AnnotationProperty .


###  http://www.w3.org/2004/02/skos/core#prefLabel
skos:prefLabel rdf:type owl:AnnotationProperty .


###  http://www.w3.org/2004/02/skos/core#scopeNote
skos:scopeNote rdf:type owl:AnnotationProperty .


#################################################################
#    Classes
#################################################################

###  http://purl.allotrope.org/ontologies/process#AFP_0000075
af-p:AFP_0000075 rdf:type owl:Class ;
                 rdfs:subClassOf af-p:AFP_0000705 ;
                 skos:altLabel "PIV" ,
                               "particle image velocimetry" ,
                               "particle imaging velocimetry" ,
                               "particle-imaging velocimetry" ;
                 skos:definition "A method for determining the velocity of fluids by pulsing a planar laser light sheet twice, and recording images of fine particles lying in the light sheet using a video camera or a photograph. [CHMO]" ;
                 skos:prefLabel "particle-image velocimetry" .


###  http://purl.allotrope.org/ontologies/process#AFP_0000104
af-p:AFP_0000104 rdf:type owl:Class ;
                 rdfs:subClassOf af-p:AFP_0000759 ,
                                 af-p:AFP_0002434 ;
                 skos:altLabel "NMR velocimetry" ,
                               "nuclear magnetic resonance (NMR) velocimetry" ;
                 skos:definition "The measurement of the velocity of a moving object or medium using an NMR signal. [CHMO]" ;
                 skos:prefLabel "nuclear magnetic resonance velocimetry" .


###  http://purl.allotrope.org/ontologies/process#AFP_0000123
af-p:AFP_0000123 rdf:type owl:Class ;
                 rdfs:subClassOf af-p:AFP_0000104 ;
                 skos:altLabel "ST" ,
                               "spin tagging" ,
                               "spin tagging NMR velocimetry" ,
                               "spin tagging nuclear magnetic resonance velocimetry" ;
                 skos:definition "A method for determining the velocity of a fluid by tagging (presaturating the magnetization in) a particular group of spins and tracking them in a fluid flow using NMR spectroscopy. [CHMO]" ;
                 skos:prefLabel "spin tagging velocimetry" .


###  http://purl.allotrope.org/ontologies/process#AFP_0000140
af-p:AFP_0000140 rdf:type owl:Class ;
                 rdfs:subClassOf af-p:AFP_0000104 ;
                 skos:altLabel "pulsed gradient spin echo NMR velocimetry" ,
                               "pulsed gradient spin echo nuclear magnetic resonance velocimetry" ,
                               "pulsed gradient spin echo velocimetry" ;
                 skos:definition "A method for determining the velocity of fluids by using a pulsed-field gradient spin echo sequence to encode the velocity into an NMR signal. Both flow and Brownian motion components of the velocity are measured. [CHMO]" ;
                 skos:prefLabel "pulsed-field gradient velocimetry" .


###  http://purl.allotrope.org/ontologies/process#AFP_0000160
af-p:AFP_0000160 rdf:type owl:Class ;
                 rdfs:subClassOf af-p:AFP_0000340 ;
                 skos:altLabel "LITA velocimetry" ,
                               "laser-induced thermal acoustic (LITA) velocimetry" ,
                               "laser-induced thermal acoustic velocimetry" ;
                 skos:definition "A method for determining the velocity of a sample flow using two coherent intersecting pulsed laser beams to create a density grating in the sample and a third, continuous, laser beam to detect the Doppler shift in the signal. [CHMO]" ;
                 skos:prefLabel "laser-induced thermal-acoustic velocimetry" .


###  http://purl.allotrope.org/ontologies/process#AFP_0000182
af-p:AFP_0000182 rdf:type owl:Class ;
                 rdfs:subClassOf af-p:AFP_0000705 ;
                 skos:altLabel "LDA" ,
                               "laser Doppler anemometry" ,
                               "laser anemometry" ,
                               "optical anemometry" ;
                 skos:definition "A method for determining the velocity or zeta-potential of a sample by measuring the Doppler shift experienced by light. A laser beam is directed at a series of fine particles in the medium of interest, and the reflected (or Doppler-shifted) beam then produces an interference pattern with a reference beam. [CHMO]" ;
                 skos:prefLabel "laser Doppler velocimetry" .


###  http://purl.allotrope.org/ontologies/process#AFP_0000340
af-p:AFP_0000340 rdf:type owl:Class ;
                 rdfs:subClassOf af-p:AFP_0002434 ;
                 skos:altLabel "ADV" ,
                               "UDV" ,
                               "acoustic Doppler velocimetry" ,
                               "acoustic velocimetry" ,
                               "sonic velocimetry" ,
                               "ultrasound Doppler velocimetry " ,
                               "ultrasound-Doppler velocimetry " ,
                               "velocity measurement using ultrasound" ;
                 skos:definition "A method for determining the velocity of a sample by measuring the Doppler shift experienced by ultrasound radiation. [CHMO]" ;
                 skos:prefLabel "ultrasonic velocimetry" .


###  http://purl.allotrope.org/ontologies/process#AFP_0000592
af-p:AFP_0000592 rdf:type owl:Class ;
                 rdfs:subClassOf af-p:AFP_0002434 ;
                 skos:altLabel "microwave Doppler velocimetry" ;
                 skos:definition "A method for determining the velocity of a sample by measuring the Doppler shift experienced by microwave radiation. This is the method used by police to measure the speed of a vehicle using a radar gun. [CHMO]" ;
                 skos:prefLabel "microwave velocimetry" .


###  http://purl.allotrope.org/ontologies/process#AFP_0000650
af-p:AFP_0000650 rdf:type owl:Class ;
                 rdfs:subClassOf af-p:AFP_0000160 ;
                 skos:altLabel "heterodyne LITA velocimetry" ,
                               "heterodyne laser-induced thermal acoustic velocimetry" ;
                 skos:definition "A method for determining the velocity of a sample flow using two coherent intersecting pulsed laser beams to create a density grating in the sample and a third, continuous, laser beam to detect the Doppler shift in the signal. Heterodyne signal detection (non-linear mixing with radiation of a reference frequency) is employed to recover the Doppler shift. [CHMO]" ;
                 skos:prefLabel "laser-induced thermal-acoustic velocimetry with heterodyne detection" .


###  http://purl.allotrope.org/ontologies/process#AFP_0000705
af-p:AFP_0000705 rdf:type owl:Class ;
                 rdfs:subClassOf af-p:AFP_0002434 ;
                 skos:definition "The measurement of the velocity of a moving object or medium using light. [CHMO]" ;
                 skos:prefLabel "optical velocimetry" .


###  http://purl.allotrope.org/ontologies/process#AFP_0000759
af-p:AFP_0000759 rdf:type owl:Class .


###  http://purl.allotrope.org/ontologies/process#AFP_0000852
af-p:AFP_0000852 rdf:type owl:Class ;
                 rdfs:subClassOf af-p:AFP_0002019 ;
                 skos:altLabel "flow-compensated phase contrast NMR velocimetry" ,
                               "flow-compensated phase contrast nuclear magnetic resonance velocimetry" ;
                 skos:definition "A method for determining the velocity of fluids by using magnetic field gradients to encode velocity information into the phase of the NMR signal. All other contributions to the magnetic gradient phase are set to zero; the only velocity contribution to the phase is due to the flow of the sample ('flow compensation'). [CHMO]" ;
                 skos:prefLabel "flow-compensated phase-contrast velocimetry" .


###  http://purl.allotrope.org/ontologies/process#AFP_0001030
af-p:AFP_0001030 rdf:type owl:Class ;
                 rdfs:subClassOf af-p:AFP_0000340 ;
                 skos:altLabel "USV" ,
                               "ultrasonic speckle velocity measurement " ;
                 skos:definition "A method for measuring the velocity of a sample by detecting and analysing successive ultrasonic speckle signals that result from the interference of backscattered echoes of successive incident pulses of ultrasonic radiation (36 MHz). [CHMO]" ;
                 skos:prefLabel "ultrasonic speckle velocimetry" .


###  http://purl.allotrope.org/ontologies/process#AFP_0001201
af-p:AFP_0001201 rdf:type owl:Class ;
                 rdfs:subClassOf af-p:AFP_0000340 ;
                 skos:altLabel "HITUV" ,
                               "high temperature ultrasonic velocimetry" ;
                 skos:changeNote "2016-02-03 Fixed typo [OSTHUS]" ;
                 skos:definition "A method for detemining the velocity of metallic or semiconductor melts (at ~1000 deg. C) by measuring the Doppler shift experienced by ultrasound radiation. [CHMO]" ;
                 skos:prefLabel "high-temperature ultrasonic velocimetry" .


###  http://purl.allotrope.org/ontologies/process#AFP_0001959
af-p:AFP_0001959 rdf:type owl:Class ;
                 rdfs:subClassOf af-p:AFP_0001030 ;
                 skos:altLabel "USV" ,
                               "ultrasonic speckle velocity measurement " ;
                 skos:definition "A method for measuring the velocity of a sample by detecting and analysing successive ultrasonic speckle signals that result from the interference of backscattered echoes of successive incident pulses of ultrasonic radiation (36 MHz) as a function of time. [CHMO]" ;
                 skos:prefLabel "time-resolved ultrasonic speckle velocimetry" .


###  http://purl.allotrope.org/ontologies/process#AFP_0002019
af-p:AFP_0002019 rdf:type owl:Class ;
                 rdfs:subClassOf af-p:AFP_0000104 ;
                 skos:altLabel "PC velocimetry" ,
                               "phase contrast velocimetry" ,
                               "phase-contrast NMR velocimetry" ,
                               "phase-contrast nuclear magnetic resonance velocimetry" ;
                 skos:definition "A method for determining the velocity of fluids by using magnetic field gradients to encode velocity information into the phase of an NMR signal. [CHMO]" ;
                 skos:prefLabel "phase-contrast velocimetry" .


###  http://purl.allotrope.org/ontologies/process#AFP_0002079
af-p:AFP_0002079 rdf:type owl:Class ;
                 rdfs:subClassOf af-p:AFP_0000075 ;
                 skos:altLabel "microPIV" ,
                               "microscopic particle image velocimetry " ,
                               "microscopic particle imaging velocimetry " ,
                               "microscopic particle-imaging velocimetry " ,
                               "µPIV" ;
                 skos:definition "A method for determining the velocity of fluids by pulsing a planar laser light sheet twice, and recording images of microscopic particles lying in the light sheet using a video camera or a photograph. [CHMO]" ;
                 skos:prefLabel "microscopic particle-image velocimetry" .


###  http://purl.allotrope.org/ontologies/process#AFP_0002112
af-p:AFP_0002112 rdf:type owl:Class ;
                 rdfs:subClassOf af-p:AFP_0000104 ;
                 skos:altLabel "MMMEV" ,
                               "multiple modulation multiple echo velocimetry" ;
                 skos:definition "A method for determining the velocity of fluids by encoding it into an NMR signal. The NMR signal is produced using multiple spin echoes from several radio frequency pulses in the presence of a constant magnetic field gradient. [CHMO]" ;
                 skos:prefLabel "multiple-modulation multiple-echo velocimetry" .


###  http://purl.allotrope.org/ontologies/process#AFP_0002406
af-p:AFP_0002406 rdf:type owl:Class ;
                 rdfs:subClassOf af-p:AFP_0000705 ;
                 skos:altLabel "PTV" ,
                               "particle tracking velocimetry" ;
                 skos:definition "A method for determining the velocity of fluids by tracking the diffracted or fluorescent light emitted from individual particles in successive digital camera images. [CHMO]" ;
                 skos:prefLabel "particle-tracking velocimetry" .


#################################################################
#    Individuals
#################################################################

###  http://purl.allotrope.org/voc/attribution
<http://purl.allotrope.org/voc/attribution> rdf:type owl:NamedIndividual ,
                                                     dct:RightsStatement ;
                                            dct:description """
These taxonomies contain material or may constitute derivative works of material which may be subject to copyright by one of the following organizations.  By using these taxonomies, you agree to the following terms and conditions applicable to its contents:
******************************************************************************
Copyright Notice and Terms for IUPAC Gold Book
______________________________________________________________________________
Copyright © 1998, Regents of the University of California
All rights reserved.
Redistribution and use in source and binary forms, with or without modification, are permitted provided that the following conditions are met:
1. Redistributions of source code must retain the above copyright notice, this list of conditions and the following disclaimer.
2. Redistributions in binary form must reproduce the above copyright notice, this list of conditions and the following disclaimer in the documentation and/or other materials provided with the distribution.
THIS SOFTWARE IS PROVIDED BY THE COPYRIGHT HOLDERS AND CONTRIBUTORS \"AS IS\" AND ANY EXPRESS OR IMPLIED WARRANTIES, INCLUDING, BUT NOT LIMITED TO, THE IMPLIED WARRANTIES OF MERCHANTABILITY AND FITNESS FOR A PARTICULAR PURPOSE ARE DISCLAIMED. IN NO EVENT SHALL THE COPYRIGHT HOLDER OR CONTRIBUTORS BE LIABLE FOR ANY DIRECT, INDIRECT, INCIDENTAL, SPECIAL, EXEMPLARY, OR CONSEQUENTIAL DAMAGES (INCLUDING, BUT NOT LIMITED TO, PROCUREMENT OF SUBSTITUTE GOODS OR SERVICES; LOSS OF USE, DATA, OR PROFITS; OR BUSINESS INTERRUPTION) HOWEVER CAUSED AND ON ANY THEORY OF LIABILITY, WHETHER IN CONTRACT, STRICT LIABILITY, OR TORT (INCLUDING NEGLIGENCE OR OTHERWISE) ARISING IN ANY WAY OUT OF THE USE OF THIS SOFTWARE, EVEN IF ADVISED OF THE POSSIBILITY OF SUCH DAMAGE.
******************************************************************************
Copyright Notice and Terms for PSI-MS (Proteomics Standards Initiative - Mass Spectrometry) Mass spectrometer output files and spectra interpretation
_____________________________________________________________________________
Created by Matt Chambers, Andreas Bertsch, Marius Kallhardt, Eric Deutsch Fredrik Levander, Pierre-Alain Binz, and Gerhard Mayer. Publisher: HUPO Proteomics Standards Initiative Mass Spectrometry Standards Working Group and HUPO Proteomics Standards Initiative Proteomics Informatics Working Group. This work is used pursuant to a Creative Commons license available here: http://creativecommons.org/licenses/by/3.0/legalcode

******************************************************************************
Attribution Notice for National Center for Biomedical Ontology materials.

This work contains material from the Cell Ontology and Clinical Measurement Ontology, available here: http://bioportal.bioontology.org/.
******************************************************************************
Attribution Notice for ChEBI
This work contains material from the European Bioinformatics Institute’s ChEBI database.
******************************************************************************
Attribution Notice for Quantities Units Dimensions Data Types (http://www.qudt.org/)
This work contains content from www.qudt.org and is used pursuant to a Creative Commons License available here: http://creativecommons.org/licenses/by-sa/3.0/us/legalcode. The original work may have been modified.
******************************************************************************
Copyright and Attribution Notice for Dublin Core Metadata Initiative Document
This work contains material from the following DCMI document used pursuant to a creative commons license available here: https://creativecommons.org/licenses/by/4.0/legalcode. This material may have been modified or changed.
Timestamped URL:          http://dublincore.org/documents/2012/06/14/dcmi-terms/
Date Issued:                       2012-06-14
Document Status:            This is a DCMI Recommendation.
Copyright © 1995-2015 DCMI. All Rights Reserved. DCMI liability, trademark/service mark, document use and software licensing rules apply.
******************************************************************************

""" ;
                                            dct:title "Derivative works attribution" .


###  http://purl.allotrope.org/voc/copyright
<http://purl.allotrope.org/voc/copyright> rdf:type owl:NamedIndividual ,
                                                   dct:RightsStatement ;
                                          dct:description "Copyright © 2019 Allotrope Foundation" ;
                                          dct:rightsHolder <http://www.allotrope.org> ;
                                          dct:title "Copyright © 2019 Allotrope Foundation" .


###  http://purl.allotrope.org/voc/creative-commons-attribution-license
<http://purl.allotrope.org/voc/creative-commons-attribution-license> rdf:type owl:NamedIndividual ,
                                                                              dct:LicenseDocument ;
                                                                     dct:description """This work is licensed under a Creative Commons Attribution 4.0 International License http://creativecommons.org/licenses/by/4.0/.

THESE MATERIALS ARE PROVIDED \"AS IS\" AND ALLOTROPE EXPRESSLY DISCLAIMS ALL WARRANTIES, EXPRESS, IMPLIED OR STATUTORY, INCLUDING, WITHOUT LIMITATION, THE WARRANTIES OF NON-INFRINGEMENT, TITLE, MERCHANTABILITY AND FITNESS FOR A PARTICULAR PURPOSE.

Copyright © 2015-2025 Allotrope Foundation
""" ;
                                                                     dct:title "Creative Commons Attribution 4.0 International Public License" .


###  Generated by the OWL API (version 5.1.19) https://github.com/owlcs/owlapi/
