@prefix : <http://purl.allotrope.org/voc/afo/domain/REC/2025/06/bet-analysis#> .
@prefix go: <http://purl.obolibrary.org/obo/GO> .
@prefix ms: <http://purl.obolibrary.org/obo/MS> .
@prefix ro: <http://purl.obolibrary.org/obo/RO> .
@prefix bfo: <http://purl.obolibrary.org/obo/BFO> .
@prefix dct: <http://purl.org/dc/terms/> .
@prefix iao: <http://purl.obolibrary.org/obo/IAO> .
@prefix obi: <http://purl.obolibrary.org/obo/OBI> .
@prefix owl: <http://www.w3.org/2002/07/owl#> .
@prefix rdf: <http://www.w3.org/1999/02/22-rdf-syntax-ns#> .
@prefix xml: <http://www.w3.org/XML/1998/namespace> .
@prefix xsd: <http://www.w3.org/2001/XMLSchema#> .
@prefix af-c: <http://purl.allotrope.org/ontologies/common#> .
@prefix af-e: <http://purl.allotrope.org/ontologies/equipment#> .
@prefix af-m: <http://purl.allotrope.org/ontologies/material#> .
@prefix af-p: <http://purl.allotrope.org/ontologies/process#> .
@prefix af-q: <http://purl.allotrope.org/ontologies/quality#> .
@prefix af-r: <http://purl.allotrope.org/ontologies/result#> .
@prefix af-x: <http://purl.allotrope.org/ontologies/property#> .
@prefix chmo: <http://purl.obolibrary.org/obo/CHMO> .
@prefix envo: <http://purl.obolibrary.org/obo/ENVO> .
@prefix foaf: <http://xmlns.com/foaf/0.1/> .
@prefix mamo: <http://purl.obolibrary.org/obo/MAMO> .
@prefix ncit: <http://purl.obolibrary.org/obo/NCIT> .
@prefix omit: <http://purl.obolibrary.org/obo/OMIT> .
@prefix pato: <http://purl.obolibrary.org/obo/PATO> .
@prefix rdfs: <http://www.w3.org/2000/01/rdf-schema#> .
@prefix skos: <http://www.w3.org/2004/02/skos/core#> .
@prefix af-rl: <http://purl.allotrope.org/ontologies/role#> .
@prefix af-cur: <http://purl.allotrope.org/ontologies/curation#> .
@base <http://purl.allotrope.org/voc/afo/domain/REC/2025/06/bet-analysis#> .

<http://purl.allotrope.org/voc/afo/domain/REC/2025/06/bet-analysis> rdf:type owl:Ontology ;
                                                                               owl:versionIRI <http://purl.allotrope.org/voc/afo/domain/REC/2025/06/bet-analysis> ;
                                                                               owl:imports <http://purl.allotrope.org/voc/afo/REC/2025/06/afo> ;
                                                                               dct:contributor <http://www.allotrope.org> ;
                                                                               dct:issued "2025-06-25T12:00:00Z"^^xsd:dateTime ;
                                                                               dct:license <http://purl.allotrope.org/voc/creative-commons-attribution-license> ;
                                                                               dct:modified "2025-04-04T12:00:00Z"^^xsd:dateTime ;
                                                                               dct:publisher <http://www.allotrope.org> ;
                                                                               dct:rights <http://purl.allotrope.org/voc/attribution> ,
                                                                                          <http://purl.allotrope.org/voc/copyright> ;
                                                                               dct:rightsHolder <http://www.allotrope.org> ;
                                                                               dct:title "AFO BET Analysis Domain Ontology (REC/2025/06)" ;
                                                                               owl:priorVersion <http://purl.allotrope.org/voc/afo/domain/REC/2025/03/bet-analysis> ;
                                                                               owl:versionInfo "REC/2025/06" .

#################################################################
#    Classes
#################################################################

###  http://purl.allotrope.org/ontologies/process#AFP_0003761
af-p:AFP_0003761 rdf:type owl:Class ;
                 rdfs:subClassOf af-p:AFP_0002294 ;
                 skos:definition "A BET analysis is a measuring process for calculating surface area based on the Brunauer–Emmett–Teller (BET) theory of multiple adsorption layers. [Allotrope]" ;
                 skos:prefLabel "BET analysis" .


###  http://purl.allotrope.org/ontologies/result#AFR_0002116
af-r:AFR_0002116 rdf:type owl:Class ;
                 rdfs:subClassOf iao:_0000310 ;
                 skos:definition "A BET point document is a document that encompasses the information associated with a single BET measurement point. [Allotrope]" ;
                 skos:prefLabel "BET point document" .


###  http://purl.allotrope.org/ontologies/result#AFR_0002117
af-r:AFR_0002117 rdf:type owl:Class ;
                 rdfs:subClassOf af-r:AFR_0001583 ;
                 skos:altLabel "relative pressure" ;
                 skos:definition "A relative pressure is a quality quantification facet that quantifies the pressure of a pure substance in a chamber relative to its saturation pressure. [Allotrope]" ;
                 skos:prefLabel "relative pressure (BET)" .


###  http://purl.allotrope.org/ontologies/result#AFR_0002118
af-r:AFR_0002118 rdf:type owl:Class ;
                 rdfs:subClassOf af-r:AFR_0001843 ;
                 skos:definition "An adsorbed volume is a quality quantification facet that denotes the quantity of absorbant calculated to be adsorbed at STP. [Allotrope]" ;
                 skos:prefLabel "adsorbed volume at STP" .


###  http://purl.allotrope.org/ontologies/result#AFR_0002122
af-r:AFR_0002122 rdf:type owl:Class ;
                 rdfs:subClassOf af-r:AFR_0001583 ;
                 skos:definition "A BET C constant is a calculated constant from a BET analysis equal to Exp(E1−EL) where E1 is  heat of adsorption for the first layer and EL is the heat of vaporization for layers beyond the first layer. [Allotrope]" ;
                 skos:prefLabel "BET C constant" .


###  http://purl.allotrope.org/ontologies/result#AFR_0002123
af-r:AFR_0002123 rdf:type owl:Class ;
                 rdfs:subClassOf af-r:AFR_0001583 ;
                 skos:definition "A monolayer quantity is a volume of a monolayer based on the cross-sectional area of the adsorbent gas. [Allotrope]" ;
                 skos:prefLabel "monolayer quantity" .


###  http://purl.allotrope.org/ontologies/result#AFR_0002286
af-r:AFR_0002286 rdf:type owl:Class ;
                 rdfs:subClassOf af-r:AFR_0001060 ;
                 dct:source <https://en.wikipedia.org/wiki/BET_theory> ;
                 skos:altLabel "Brunauer–Emmett–Teller plot" ;
                 skos:definition "A BET plot is a data distribution function of an adsorption isotherm with 1/v[(p0/p)-1] on the y-axis and p/p0 on the x-axis, where p is equilibrium pressure and p0 saturation pressure of adsorbates at the temperature of adsorption, and v is the adsorbed gas quantity. [Wikipedia]" ;
                 skos:prefLabel "BET plot" .


###  http://purl.allotrope.org/ontologies/result#AFR_0002287
af-r:AFR_0002287 rdf:type owl:Class ;
                 rdfs:subClassOf <http://purl.org/linked-data/cube#DataSet> ,
                                 [ rdf:type owl:Restriction ;
                                   owl:onProperty [ owl:inverseOf af-x:AFX_0002737
                                                  ] ;
                                   owl:someValuesFrom af-r:AFR_0002286
                                 ] ;
                 skos:altLabel "Brunauer–Emmett–Teller plot data cube" ;
                 skos:definition "A BET plot data cube is a data cube that represents a BET plot. [Allotrope]" ;
                 skos:prefLabel "BET plot data cube" .


###  http://purl.org/dc/terms/LicenseDocument
dct:LicenseDocument rdf:type owl:Class .


###  http://purl.org/dc/terms/RightsStatement
dct:RightsStatement rdf:type owl:Class .


#################################################################
#    Individuals
#################################################################

###  http://www.allotrope.org
<http://www.allotrope.org> rdf:type owl:NamedIndividual ,
                                    foaf:Organization ;
                           foaf:name "Allotrope Foundation" .


###  http://purl.allotrope.org/voc/attribution
<http://purl.allotrope.org/voc/attribution> rdf:type owl:NamedIndividual ,
                                                     dct:RightsStatement ;
                                            dct:description """
These taxonomies contain material or may constitute derivative works of material which may be subject to copyright by one of the following organizations.  By using these taxonomies, you agree to the following terms and conditions applicable to its contents:
******************************************************************************
Copyright Notice and Terms for IUPAC Gold Book
______________________________________________________________________________
Copyright © 1998, Regents of the University of California
All rights reserved.
Redistribution and use in source and binary forms, with or without modification, are permitted provided that the following conditions are met:
1. Redistributions of source code must retain the above copyright notice, this list of conditions and the following disclaimer.
2. Redistributions in binary form must reproduce the above copyright notice, this list of conditions and the following disclaimer in the documentation and/or other materials provided with the distribution.
THIS SOFTWARE IS PROVIDED BY THE COPYRIGHT HOLDERS AND CONTRIBUTORS \"AS IS\" AND ANY EXPRESS OR IMPLIED WARRANTIES, INCLUDING, BUT NOT LIMITED TO, THE IMPLIED WARRANTIES OF MERCHANTABILITY AND FITNESS FOR A PARTICULAR PURPOSE ARE DISCLAIMED. IN NO EVENT SHALL THE COPYRIGHT HOLDER OR CONTRIBUTORS BE LIABLE FOR ANY DIRECT, INDIRECT, INCIDENTAL, SPECIAL, EXEMPLARY, OR CONSEQUENTIAL DAMAGES (INCLUDING, BUT NOT LIMITED TO, PROCUREMENT OF SUBSTITUTE GOODS OR SERVICES; LOSS OF USE, DATA, OR PROFITS; OR BUSINESS INTERRUPTION) HOWEVER CAUSED AND ON ANY THEORY OF LIABILITY, WHETHER IN CONTRACT, STRICT LIABILITY, OR TORT (INCLUDING NEGLIGENCE OR OTHERWISE) ARISING IN ANY WAY OUT OF THE USE OF THIS SOFTWARE, EVEN IF ADVISED OF THE POSSIBILITY OF SUCH DAMAGE.
******************************************************************************
Copyright Notice and Terms for PSI-MS (Proteomics Standards Initiative - Mass Spectrometry) Mass spectrometer output files and spectra interpretation
_____________________________________________________________________________
Created by Matt Chambers, Andreas Bertsch, Marius Kallhardt, Eric Deutsch Fredrik Levander, Pierre-Alain Binz, and Gerhard Mayer. Publisher: HUPO Proteomics Standards Initiative Mass Spectrometry Standards Working Group and HUPO Proteomics Standards Initiative Proteomics Informatics Working Group. This work is used pursuant to a Creative Commons license available here: http://creativecommons.org/licenses/by/3.0/legalcode

******************************************************************************
Attribution Notice for National Center for Biomedical Ontology materials.

This work contains material from the Cell Ontology and Clinical Measurement Ontology, available here: http://bioportal.bioontology.org/.
******************************************************************************
Attribution Notice for ChEBI
This work contains material from the European Bioinformatics Institute’s ChEBI database.
******************************************************************************
Attribution Notice for Quantities Units Dimensions Data Types (http://www.qudt.org/)
This work contains content from www.qudt.org and is used pursuant to a Creative Commons License available here: http://creativecommons.org/licenses/by-sa/3.0/us/legalcode. The original work may have been modified.
******************************************************************************
Copyright and Attribution Notice for Dublin Core Metadata Initiative Document
This work contains material from the following DCMI document used pursuant to a creative commons license available here: https://creativecommons.org/licenses/by/4.0/legalcode. This material may have been modified or changed.
Timestamped URL:          http://dublincore.org/documents/2012/06/14/dcmi-terms/
Date Issued:                       2012-06-14
Document Status:            This is a DCMI Recommendation.
Copyright © 1995-2015 DCMI. All Rights Reserved. DCMI liability, trademark/service mark, document use and software licensing rules apply.
******************************************************************************

""" ;
                                            dct:title "Derivative works attribution" .


###  http://purl.allotrope.org/voc/copyright
<http://purl.allotrope.org/voc/copyright> rdf:type owl:NamedIndividual ,
                                                   dct:RightsStatement ;
                                          dct:description "Copyright © 2015-2025 Allotrope Foundation" ;
                                          dct:rightsHolder <http://www.allotrope.org> ;
                                          dct:title "Copyright © 2015-2025 Allotrope Foundation" .


###  http://purl.allotrope.org/voc/creative-commons-attribution-license
<http://purl.allotrope.org/voc/creative-commons-attribution-license> rdf:type owl:NamedIndividual ,
                                                                              dct:LicenseDocument ;
                                                                     dct:description """This work is licensed under a Creative Commons Attribution 4.0 International License http://creativecommons.org/licenses/by/4.0/.

THESE MATERIALS ARE PROVIDED \"AS IS\" AND ALLOTROPE EXPRESSLY DISCLAIMS ALL WARRANTIES, EXPRESS, IMPLIED OR STATUTORY, INCLUDING, WITHOUT LIMITATION, THE WARRANTIES OF NON-INFRINGEMENT, TITLE, MERCHANTABILITY AND FITNESS FOR A PARTICULAR PURPOSE.

Copyright © 2015-2025 Allotrope Foundation
""" ;
                                                                     dct:title "Creative Commons Attribution 4.0 International Public License" .


###  Generated by the OWL API (version 5.1.19) https://github.com/owlcs/owlapi/
