@prefix : <http://purl.allotrope.org/voc/afo/domain/REC/2025/06/eln#> .
@prefix cl: <http://purl.obolibrary.org/obo/CL> .
@prefix go: <http://purl.obolibrary.org/obo/GO> .
@prefix ro: <http://purl.obolibrary.org/obo/RO> .
@prefix bfo: <http://purl.obolibrary.org/obo/BFO> .
@prefix dct: <http://purl.org/dc/terms/> .
@prefix iao: <http://purl.obolibrary.org/obo/IAO> .
@prefix obi: <http://purl.obolibrary.org/obo/OBI> .
@prefix owl: <http://www.w3.org/2002/07/owl#> .
@prefix rdf: <http://www.w3.org/1999/02/22-rdf-syntax-ns#> .
@prefix xml: <http://www.w3.org/XML/1998/namespace> .
@prefix xsd: <http://www.w3.org/2001/XMLSchema#> .
@prefix af-c: <http://purl.allotrope.org/ontologies/common#> .
@prefix af-e: <http://purl.allotrope.org/ontologies/equipment#> .
@prefix af-m: <http://purl.allotrope.org/ontologies/material#> .
@prefix af-p: <http://purl.allotrope.org/ontologies/process#> .
@prefix af-q: <http://purl.allotrope.org/ontologies/quality#> .
@prefix af-r: <http://purl.allotrope.org/ontologies/result#> .
@prefix af-x: <http://purl.allotrope.org/ontologies/property#> .
@prefix chmo: <http://purl.obolibrary.org/obo/CHMO> .
@prefix foaf: <http://xmlns.com/foaf/0.1/> .
@prefix pato: <http://purl.obolibrary.org/obo/PATO> .
@prefix rdfs: <http://www.w3.org/2000/01/rdf-schema#> .
@prefix skos: <http://www.w3.org/2004/02/skos/core#> .
@prefix af-cur: <http://purl.allotrope.org/ontologies/curation#> .
@base <http://purl.allotrope.org/voc/afo/domain/REC/2025/06/eln#> .

<http://purl.allotrope.org/voc/afo/domain/REC/2025/06/eln> rdf:type owl:Ontology ;
                                                                      owl:versionIRI <http://purl.allotrope.org/voc/afo/domain/REC/2025/06/eln> ;
                                                                      owl:imports <http://purl.allotrope.org/voc/afo/REC/2025/06/afo> ;
                                                                      dct:contributor <http://www.allotrope.org> ;
                                                                      dct:issued "2025-06-25T12:00:00Z"^^xsd:dateTime ;
                                                                      dct:license <http://purl.allotrope.org/voc/creative-commons-attribution-license> ;
                                                                      dct:modified "2025-04-04T12:00:00Z"^^xsd:dateTime ;
                                                                      dct:publisher <http://www.allotrope.org> ;
                                                                      dct:rights <http://purl.allotrope.org/voc/attribution> ,
                                                                                 <http://purl.allotrope.org/voc/copyright> ;
                                                                      dct:rightsHolder <http://www.allotrope.org> ;
                                                                      dct:title "AFO Electronic Lab Notebook Domain Ontology (REC/2025/06)" ;
                                                                      owl:versionInfo "REC/2025/06" .

#################################################################
#    Annotation properties
#################################################################

###  http://purl.allotrope.org/ontologies/property#AFX_0002796
af-x:AFX_0002796 rdf:type owl:AnnotationProperty .


###  http://purl.allotrope.org/ontologies/property#AFX_0002798
af-x:AFX_0002798 rdf:type owl:AnnotationProperty .


###  http://purl.allotrope.org/ontologies/property#AFX_0002809
af-x:AFX_0002809 rdf:type owl:AnnotationProperty .


###  http://purl.org/dc/terms/source
dct:source rdf:type owl:AnnotationProperty .


###  http://purl.org/pav/importedFrom
<http://purl.org/pav/importedFrom> rdf:type owl:AnnotationProperty .


###  http://www.w3.org/2004/02/skos/core#altLabel
skos:altLabel rdf:type owl:AnnotationProperty .


###  http://www.w3.org/2004/02/skos/core#changeNote
skos:changeNote rdf:type owl:AnnotationProperty .


###  http://www.w3.org/2004/02/skos/core#definition
skos:definition rdf:type owl:AnnotationProperty .


###  http://www.w3.org/2004/02/skos/core#example
skos:example rdf:type owl:AnnotationProperty .


###  http://www.w3.org/2004/02/skos/core#note
skos:note rdf:type owl:AnnotationProperty .


###  http://www.w3.org/2004/02/skos/core#prefLabel
skos:prefLabel rdf:type owl:AnnotationProperty .


###  http://www.w3.org/2004/02/skos/core#scopeNote
skos:scopeNote rdf:type owl:AnnotationProperty .


#################################################################
#    Classes
#################################################################

###  http://purl.allotrope.org/ontologies/equipment#AFE_0002286
af-e:AFE_0002286 rdf:type owl:Class ;
                 rdfs:subClassOf af-e:AFE_0002232 ;
                 skos:altLabel "ELN" ,
                               "electronic lab notebook" ;
                 skos:definition "An electronic lab notebook system is a data system used in laboratories to record the execution and results of experiments. [Allotrope]" ;
                 skos:prefLabel "electronic lab notebook system" .


###  http://purl.allotrope.org/ontologies/result#AFR_0003087
af-r:AFR_0003087 rdf:type owl:Class ;
                 rdfs:subClassOf af-c:AFC_0000160 ,
                                 iao:_0000310 ,
                                 [ rdf:type owl:Restriction ;
                                   owl:onProperty ro:_0002351 ;
                                   owl:someValuesFrom af-r:AFR_0003088
                                 ] ;
                 skos:definition "An electronic lab notebook entry aggregate document is a document that aggregates electronic lab notebook entry documents. [Allotrope]" ;
                 skos:prefLabel "electronic lab notebook entry aggregate document" .


###  http://purl.allotrope.org/ontologies/result#AFR_0003088
af-r:AFR_0003088 rdf:type owl:Class ;
                 rdfs:subClassOf iao:_0000310 ,
                                 [ rdf:type owl:Restriction ;
                                   owl:onProperty iao:_0000136 ;
                                   owl:someValuesFrom af-r:AFR_0003141
                                 ] ;
                 skos:definition "A electronic lab notebook entry document is a document that encompasses the information associated with some electronic lab notebook entry. [Allotrope]" ;
                 skos:prefLabel "electronic lab notebook entry document" .


###  http://purl.allotrope.org/ontologies/result#AFR_0003089
af-r:AFR_0003089 rdf:type owl:Class ;
                 rdfs:subClassOf af-r:AFR_0000917 ,
                                 [ rdf:type owl:Restriction ;
                                   owl:onProperty af-x:AFX_0002717 ;
                                   owl:someValuesFrom af-r:AFR_0003141
                                 ] ;
                 skos:definition "An electronic lab notebook entry identifier is an identifier that identifies some electronic lab notebook entry. [Allotrope]" ;
                 skos:prefLabel "electronic lab notebook entry identifier" .


###  http://purl.allotrope.org/ontologies/result#AFR_0003090
af-r:AFR_0003090 rdf:type owl:Class ;
                 rdfs:subClassOf iao:_0000590 ,
                                 [ rdf:type owl:Restriction ;
                                   owl:onProperty iao:_0000219 ;
                                   owl:someValuesFrom af-r:AFR_0003141
                                 ] ;
                 skos:definition "An electronic lab notebook entry name is a written name that denotes some electronic lab notebook entry. [Allotrope]" ;
                 skos:prefLabel "electronic lab notebook entry name" .


###  http://purl.allotrope.org/ontologies/result#AFR_0003091
af-r:AFR_0003091 rdf:type owl:Class ;
                 owl:equivalentClass [ owl:intersectionOf ( af-r:AFR_0001277
                                                            [ rdf:type owl:Restriction ;
                                                              owl:onProperty af-x:AFX_0002806 ;
                                                              owl:someValuesFrom af-r:AFR_0003141
                                                            ]
                                                          ) ;
                                       rdf:type owl:Class
                                     ] ;
                 skos:definition "An electronic lab notebook entry type is a classification datum that classifies some electronic lab notebook entry. [Allotrope]" ;
                 skos:prefLabel "electronic lab notebook entry type" .


###  http://purl.allotrope.org/ontologies/result#AFR_0003092
af-r:AFR_0003092 rdf:type owl:Class ;
                 owl:equivalentClass [ owl:intersectionOf ( af-r:AFR_0001277
                                                            [ rdf:type owl:Restriction ;
                                                              owl:onProperty af-x:AFX_0002806 ;
                                                              owl:someValuesFrom [ owl:intersectionOf ( af-p:AFP_0003374
                                                                                                        [ rdf:type owl:Restriction ;
                                                                                                          owl:onProperty af-x:AFX_0002876 ;
                                                                                                          owl:someValuesFrom af-r:AFR_0003141
                                                                                                        ]
                                                                                                      ) ;
                                                                                   rdf:type owl:Class
                                                                                 ]
                                                            ]
                                                          ) ;
                                       rdf:type owl:Class
                                     ] ;
                 skos:definition "An electronic lab notebook entry state type is a classification datum that classifies the state of some electronic lab notebook entry. [Allotrope]" ;
                 skos:prefLabel "electronic lab notebook entry state type" .


###  http://purl.allotrope.org/ontologies/result#AFR_0003101
af-r:AFR_0003101 rdf:type owl:Class ;
                 rdfs:subClassOf af-c:AFC_0000160 ,
                                 iao:_0000310 ,
                                 [ rdf:type owl:Restriction ;
                                   owl:onProperty ro:_0002351 ;
                                   owl:someValuesFrom af-r:AFR_0003102
                                 ] ;
                 skos:definition "A section aggregate document is a document that aggregates section documents. [Allotrope]" ;
                 skos:prefLabel "section aggregate document" .


###  http://purl.allotrope.org/ontologies/result#AFR_0003102
af-r:AFR_0003102 rdf:type owl:Class ;
                 rdfs:subClassOf iao:_0000310 ,
                                 [ rdf:type owl:Restriction ;
                                   owl:onProperty iao:_0000136 ;
                                   owl:someValuesFrom af-r:AFR_0003137
                                 ] ;
                 skos:definition "A section document is a document that encompasses the information associated with some section. [Allotrope]" ;
                 skos:prefLabel "section document" .


###  http://purl.allotrope.org/ontologies/result#AFR_0003103
af-r:AFR_0003103 rdf:type owl:Class ;
                 rdfs:subClassOf af-r:AFR_0000917 ,
                                 [ rdf:type owl:Restriction ;
                                   owl:onProperty af-x:AFX_0002717 ;
                                   owl:someValuesFrom af-r:AFR_0003137
                                 ] ;
                 skos:definition "A section identifier is an identifier that identifies some section. [Allotrope]" ;
                 skos:prefLabel "section identifier" .


###  http://purl.allotrope.org/ontologies/result#AFR_0003104
af-r:AFR_0003104 rdf:type owl:Class ;
                 rdfs:subClassOf iao:_0000590 ,
                                 [ rdf:type owl:Restriction ;
                                   owl:onProperty iao:_0000219 ;
                                   owl:someValuesFrom af-r:AFR_0003137
                                 ] ;
                 skos:definition "A section name is a written name that denotes some section. [Allotrope]" ;
                 skos:prefLabel "section name" .


###  http://purl.allotrope.org/ontologies/result#AFR_0003105
af-r:AFR_0003105 rdf:type owl:Class ;
                 rdfs:subClassOf af-c:AFC_0000160 ,
                                 iao:_0000310 ,
                                 [ rdf:type owl:Restriction ;
                                   owl:onProperty ro:_0002351 ;
                                   owl:someValuesFrom af-r:AFR_0003106
                                 ] ;
                 skos:definition "A field aggregate document is a document that aggregates field documents. [Allotrope]" ;
                 skos:prefLabel "field aggregate document" .


###  http://purl.allotrope.org/ontologies/result#AFR_0003106
af-r:AFR_0003106 rdf:type owl:Class ;
                 rdfs:subClassOf iao:_0000310 ,
                                 [ rdf:type owl:Restriction ;
                                   owl:onProperty iao:_0000136 ;
                                   owl:someValuesFrom af-r:AFR_0003138
                                 ] ;
                 skos:definition "A field document is a document that encompasses the information associated with some field. [Allotrope]" ;
                 skos:prefLabel "field document" .


###  http://purl.allotrope.org/ontologies/result#AFR_0003107
af-r:AFR_0003107 rdf:type owl:Class ;
                 rdfs:subClassOf af-r:AFR_0000917 ,
                                 [ rdf:type owl:Restriction ;
                                   owl:onProperty af-x:AFX_0002717 ;
                                   owl:someValuesFrom af-r:AFR_0003138
                                 ] ;
                 skos:definition "A field identifier is an identifier that identifies some field. [Allotrope]" ;
                 skos:prefLabel "field identifier" .


###  http://purl.allotrope.org/ontologies/result#AFR_0003108
af-r:AFR_0003108 rdf:type owl:Class ;
                 rdfs:subClassOf iao:_0000590 ,
                                 [ rdf:type owl:Restriction ;
                                   owl:onProperty iao:_0000219 ;
                                   owl:someValuesFrom af-r:AFR_0003138
                                 ] ;
                 skos:definition "A field name is a written name that denotes some field. [Allotrope]" ;
                 skos:prefLabel "field name" .


###  http://purl.allotrope.org/ontologies/result#AFR_0003109
af-r:AFR_0003109 rdf:type owl:Class ;
                 owl:equivalentClass [ owl:intersectionOf ( af-r:AFR_0001277
                                                            [ rdf:type owl:Restriction ;
                                                              owl:onProperty af-x:AFX_0002806 ;
                                                              owl:someValuesFrom af-r:AFR_0003138
                                                            ]
                                                          ) ;
                                       rdf:type owl:Class
                                     ] ;
                 skos:definition "A field type is a classification datum that classifies the content and intended usage of some field. [Allotrope]" ;
                 skos:prefLabel "field type" .


###  http://purl.allotrope.org/ontologies/result#AFR_0003110
af-r:AFR_0003110 rdf:type owl:Class ;
                 rdfs:subClassOf af-c:AFC_0000160 ,
                                 iao:_0000310 ,
                                 [ rdf:type owl:Restriction ;
                                   owl:onProperty ro:_0002351 ;
                                   owl:someValuesFrom af-r:AFR_0003111
                                 ] ;
                 skos:definition "A table aggregate document is a document that aggregates table documents. [Allotrope]" ;
                 skos:prefLabel "table aggregate document" .


###  http://purl.allotrope.org/ontologies/result#AFR_0003111
af-r:AFR_0003111 rdf:type owl:Class ;
                 rdfs:subClassOf iao:_0000310 ,
                                 [ rdf:type owl:Restriction ;
                                   owl:onProperty iao:_0000136 ;
                                   owl:someValuesFrom iao:_0000306
                                 ] ;
                 skos:definition "A table document is a document that encompasses the information associated with some table. [Allotrope]" ;
                 skos:prefLabel "table document" .


###  http://purl.allotrope.org/ontologies/result#AFR_0003112
af-r:AFR_0003112 rdf:type owl:Class ;
                 rdfs:subClassOf af-r:AFR_0000917 ,
                                 [ rdf:type owl:Restriction ;
                                   owl:onProperty af-x:AFX_0002717 ;
                                   owl:someValuesFrom iao:_0000306
                                 ] ;
                 skos:definition "A table identifier is an identifier that identifies some table. [Allotrope]" ;
                 skos:prefLabel "table identifier" .


###  http://purl.allotrope.org/ontologies/result#AFR_0003113
af-r:AFR_0003113 rdf:type owl:Class ;
                 rdfs:subClassOf iao:_0000590 ,
                                 [ rdf:type owl:Restriction ;
                                   owl:onProperty iao:_0000219 ;
                                   owl:someValuesFrom iao:_0000306
                                 ] ;
                 skos:definition "A table name is a written name that denotes some table. [Allotrope]" ;
                 skos:prefLabel "table name" .


###  http://purl.allotrope.org/ontologies/result#AFR_0003114
af-r:AFR_0003114 rdf:type owl:Class ;
                 rdfs:subClassOf af-c:AFC_0000160 ,
                                 iao:_0000310 ,
                                 [ rdf:type owl:Restriction ;
                                   owl:onProperty ro:_0002351 ;
                                   owl:someValuesFrom af-r:AFR_0003115
                                 ] ;
                 skos:definition "A table cell aggregate document is a document that aggregates table cell documents. [Allotrope]" ;
                 skos:prefLabel "table cell aggregate document" .


###  http://purl.allotrope.org/ontologies/result#AFR_0003115
af-r:AFR_0003115 rdf:type owl:Class ;
                 rdfs:subClassOf iao:_0000310 ,
                                 [ rdf:type owl:Restriction ;
                                   owl:onProperty iao:_0000136 ;
                                   owl:someValuesFrom af-r:AFR_0003140
                                 ] ;
                 skos:definition "A table cell document is a document that encompasses the information associated with some table cell. [Allotrope]" ;
                 skos:prefLabel "table cell document" .


###  http://purl.allotrope.org/ontologies/result#AFR_0003116
af-r:AFR_0003116 rdf:type owl:Class ;
                 rdfs:subClassOf af-r:AFR_0000917 ,
                                 [ rdf:type owl:Restriction ;
                                   owl:onProperty af-x:AFX_0002717 ;
                                   owl:someValuesFrom af-r:AFR_0003140
                                 ] ;
                 skos:definition "A table cell identifier is an identifier that identifies some table cell. [Allotrope]" ;
                 skos:prefLabel "table cell identifier" .


###  http://purl.allotrope.org/ontologies/result#AFR_0003117
af-r:AFR_0003117 rdf:type owl:Class ;
                 rdfs:subClassOf iao:_0000590 ,
                                 [ rdf:type owl:Restriction ;
                                   owl:onProperty iao:_0000219 ;
                                   owl:someValuesFrom af-r:AFR_0003140
                                 ] ;
                 skos:definition "A table cell name is a written name that denotes some table cell. [Allotrope]" ;
                 skos:prefLabel "table cell name" .


###  http://purl.allotrope.org/ontologies/result#AFR_0003118
af-r:AFR_0003118 rdf:type owl:Class ;
                 rdfs:subClassOf af-c:AFC_0000160 ,
                                 iao:_0000310 ,
                                 [ rdf:type owl:Restriction ;
                                   owl:onProperty ro:_0002351 ;
                                   owl:someValuesFrom af-r:AFR_0003119
                                 ] ;
                 skos:definition "A property aggregate document is a document that aggregates property documents. [Allotrope]" ;
                 skos:prefLabel "property aggregate document" .


###  http://purl.allotrope.org/ontologies/result#AFR_0003119
af-r:AFR_0003119 rdf:type owl:Class ;
                 rdfs:subClassOf iao:_0000310 ,
                                 [ rdf:type owl:Restriction ;
                                   owl:onProperty iao:_0000136 ;
                                   owl:someValuesFrom af-r:AFR_0003139
                                 ] ;
                 skos:definition "A property document is a document that encompasses the information associated with some property. [Allotrope]" ;
                 skos:prefLabel "property document" .


###  http://purl.allotrope.org/ontologies/result#AFR_0003120
af-r:AFR_0003120 rdf:type owl:Class ;
                 rdfs:subClassOf iao:_0000590 ,
                                 [ rdf:type owl:Restriction ;
                                   owl:onProperty iao:_0000219 ;
                                   owl:someValuesFrom af-r:AFR_0003139
                                 ] ;
                 skos:definition "A property name is a written name that denotes some property. [Allotrope]" ;
                 skos:prefLabel "property name" .


###  http://purl.allotrope.org/ontologies/result#AFR_0003121
af-r:AFR_0003121 rdf:type owl:Class ;
                 owl:equivalentClass [ owl:intersectionOf ( af-r:AFR_0001277
                                                            [ rdf:type owl:Restriction ;
                                                              owl:onProperty af-x:AFX_0002806 ;
                                                              owl:someValuesFrom af-r:AFR_0003139
                                                            ]
                                                          ) ;
                                       rdf:type owl:Class
                                     ] ;
                 skos:definition "A property type is a classification datum that classifies some property. [Allotrope]" ;
                 skos:prefLabel "property type" .


###  http://purl.allotrope.org/ontologies/result#AFR_0003137
af-r:AFR_0003137 rdf:type owl:Class ;
                 rdfs:subClassOf af-c:AFC_0000166 ,
                                 [ rdf:type owl:Restriction ;
                                   owl:onProperty af-x:AFX_0002800 ;
                                   owl:someValuesFrom af-r:AFR_0003141
                                 ] ,
                                 [ rdf:type owl:Restriction ;
                                   owl:onProperty ro:_0002351 ;
                                   owl:someValuesFrom iao:_0000030
                                 ] ;
                 skos:definition "A section is a collection of information content entities in an electronic lab notebook entry with a shared descriptive purpose. [Allotrope]" ;
                 skos:prefLabel "section (ELN)" .


###  http://purl.allotrope.org/ontologies/result#AFR_0003138
af-r:AFR_0003138 rdf:type owl:Class ;
                 rdfs:subClassOf af-c:AFC_0000166 ,
                                 [ rdf:type owl:Restriction ;
                                   owl:onProperty ro:_0002351 ;
                                   owl:someValuesFrom iao:_0000030
                                 ] ;
                 skos:definition "A field is a collection of information content entities in an electronic lab notebook entry with a common representation form. [Allotrope]" ;
                 skos:prefLabel "field (ELN)" .


###  http://purl.allotrope.org/ontologies/result#AFR_0003139
af-r:AFR_0003139 rdf:type owl:Class ;
                 rdfs:subClassOf af-r:AFR_0000923 ;
                 skos:definition "A property is a facet in an electronic lab notebook entry capturing the information about some value and its representation form. [Allotrope]" ;
                 skos:prefLabel "property (ELN)" .


###  http://purl.allotrope.org/ontologies/result#AFR_0003141
af-r:AFR_0003141 rdf:type owl:Class ;
                 rdfs:subClassOf af-r:AFR_0002038 ;
                 skos:definition "An electronic lab notebook entry is an electronic record that is stored in an electronic lab notebook. [Allotrope]" ;
                 skos:prefLabel "electronic lab notebook entry" .


#################################################################
#    Individuals
#################################################################

###  http://www.allotrope.org
<http://www.allotrope.org> rdf:type owl:NamedIndividual ,
                                    foaf:Organization ;
                           foaf:name "Allotrope Foundation" .


###  http://purl.allotrope.org/voc/attribution
<http://purl.allotrope.org/voc/attribution> rdf:type owl:NamedIndividual ,
                                                     dct:RightsStatement ;
                                            dct:description """
These taxonomies contain material or may constitute derivative works of material which may be subject to copyright by one of the following organizations.  By using these taxonomies, you agree to the following terms and conditions applicable to its contents:
******************************************************************************
Copyright Notice and Terms for IUPAC Gold Book
______________________________________________________________________________
Copyright © 1998, Regents of the University of California
All rights reserved.
Redistribution and use in source and binary forms, with or without modification, are permitted provided that the following conditions are met:
1. Redistributions of source code must retain the above copyright notice, this list of conditions and the following disclaimer.
2. Redistributions in binary form must reproduce the above copyright notice, this list of conditions and the following disclaimer in the documentation and/or other materials provided with the distribution.
THIS SOFTWARE IS PROVIDED BY THE COPYRIGHT HOLDERS AND CONTRIBUTORS \"AS IS\" AND ANY EXPRESS OR IMPLIED WARRANTIES, INCLUDING, BUT NOT LIMITED TO, THE IMPLIED WARRANTIES OF MERCHANTABILITY AND FITNESS FOR A PARTICULAR PURPOSE ARE DISCLAIMED. IN NO EVENT SHALL THE COPYRIGHT HOLDER OR CONTRIBUTORS BE LIABLE FOR ANY DIRECT, INDIRECT, INCIDENTAL, SPECIAL, EXEMPLARY, OR CONSEQUENTIAL DAMAGES (INCLUDING, BUT NOT LIMITED TO, PROCUREMENT OF SUBSTITUTE GOODS OR SERVICES; LOSS OF USE, DATA, OR PROFITS; OR BUSINESS INTERRUPTION) HOWEVER CAUSED AND ON ANY THEORY OF LIABILITY, WHETHER IN CONTRACT, STRICT LIABILITY, OR TORT (INCLUDING NEGLIGENCE OR OTHERWISE) ARISING IN ANY WAY OUT OF THE USE OF THIS SOFTWARE, EVEN IF ADVISED OF THE POSSIBILITY OF SUCH DAMAGE.
******************************************************************************
Copyright Notice and Terms for PSI-MS (Proteomics Standards Initiative - Mass Spectrometry) Mass spectrometer output files and spectra interpretation
_____________________________________________________________________________
Created by Matt Chambers, Andreas Bertsch, Marius Kallhardt, Eric Deutsch Fredrik Levander, Pierre-Alain Binz, and Gerhard Mayer. Publisher: HUPO Proteomics Standards Initiative Mass Spectrometry Standards Working Group and HUPO Proteomics Standards Initiative Proteomics Informatics Working Group. This work is used pursuant to a Creative Commons license available here: http://creativecommons.org/licenses/by/3.0/legalcode

******************************************************************************
Attribution Notice for National Center for Biomedical Ontology materials.

This work contains material from the Cell Ontology and Clinical Measurement Ontology, available here: http://bioportal.bioontology.org/.
******************************************************************************
Attribution Notice for ChEBI
This work contains material from the European Bioinformatics Institute’s ChEBI database.
******************************************************************************
Attribution Notice for Quantities Units Dimensions Data Types (http://www.qudt.org/)
This work contains content from www.qudt.org and is used pursuant to a Creative Commons License available here: http://creativecommons.org/licenses/by-sa/3.0/us/legalcode. The original work may have been modified.
******************************************************************************
Copyright and Attribution Notice for Dublin Core Metadata Initiative Document
This work contains material from the following DCMI document used pursuant to a creative commons license available here: https://creativecommons.org/licenses/by/4.0/legalcode. This material may have been modified or changed.
Timestamped URL:          http://dublincore.org/documents/2012/06/14/dcmi-terms/
Date Issued:                       2012-06-14
Document Status:            This is a DCMI Recommendation.
Copyright © 1995-2015 DCMI. All Rights Reserved. DCMI liability, trademark/service mark, document use and software licensing rules apply.
******************************************************************************

""" ;
                                            dct:title "Derivative works attribution" .


###  http://purl.allotrope.org/voc/copyright
<http://purl.allotrope.org/voc/copyright> rdf:type owl:NamedIndividual ,
                                                   dct:RightsStatement ;
                                          dct:description "Copyright © 2015-2025 Allotrope Foundation" ;
                                          dct:rightsHolder <http://www.allotrope.org> ;
                                          dct:title "Copyright © 2015-2025 Allotrope Foundation" .


###  http://purl.allotrope.org/voc/creative-commons-attribution-license
<http://purl.allotrope.org/voc/creative-commons-attribution-license> rdf:type owl:NamedIndividual ,
                                                                              dct:LicenseDocument ;
                                                                     dct:description """This work is licensed under a Creative Commons Attribution 4.0 International License http://creativecommons.org/licenses/by/4.0/.

THESE MATERIALS ARE PROVIDED \"AS IS\" AND ALLOTROPE EXPRESSLY DISCLAIMS ALL WARRANTIES, EXPRESS, IMPLIED OR STATUTORY, INCLUDING, WITHOUT LIMITATION, THE WARRANTIES OF NON-INFRINGEMENT, TITLE, MERCHANTABILITY AND FITNESS FOR A PARTICULAR PURPOSE.

Copyright © 2015-2025 Allotrope Foundation
""" ;
                                                                     dct:title "Creative Commons Attribution 4.0 International Public License" .


###  Generated by the OWL API (version 5.1.19) https://github.com/owlcs/owlapi/
