@prefix : <http://purl.allotrope.org/voc/afo/domain/REC/2025/06/fingerprinting#> .
@prefix cl: <http://purl.obolibrary.org/obo/CL> .
@prefix go: <http://purl.obolibrary.org/obo/GO> .
@prefix ro: <http://purl.obolibrary.org/obo/RO> .
@prefix bfo: <http://purl.obolibrary.org/obo/BFO> .
@prefix dct: <http://purl.org/dc/terms/> .
@prefix iao: <http://purl.obolibrary.org/obo/IAO> .
@prefix obi: <http://purl.obolibrary.org/obo/OBI> .
@prefix owl: <http://www.w3.org/2002/07/owl#> .
@prefix rdf: <http://www.w3.org/1999/02/22-rdf-syntax-ns#> .
@prefix xml: <http://www.w3.org/XML/1998/namespace> .
@prefix xsd: <http://www.w3.org/2001/XMLSchema#> .
@prefix af-c: <http://purl.allotrope.org/ontologies/common#> .
@prefix af-e: <http://purl.allotrope.org/ontologies/equipment#> .
@prefix af-m: <http://purl.allotrope.org/ontologies/material#> .
@prefix af-p: <http://purl.allotrope.org/ontologies/process#> .
@prefix af-q: <http://purl.allotrope.org/ontologies/quality#> .
@prefix af-r: <http://purl.allotrope.org/ontologies/result#> .
@prefix af-x: <http://purl.allotrope.org/ontologies/property#> .
@prefix chmo: <http://purl.obolibrary.org/obo/CHMO> .
@prefix foaf: <http://xmlns.com/foaf/0.1/> .
@prefix rdfs: <http://www.w3.org/2000/01/rdf-schema#> .
@prefix skos: <http://www.w3.org/2004/02/skos/core#> .
@prefix af-cq: <http://purl.allotrope.org/ontologies/common/qualifier#> .
@prefix af-fn: <http://purl.allotrope.org/ontologies/function#> .
@prefix af-re: <http://purl.allotrope.org/ontologies/realizable#> .
@prefix af-rl: <http://purl.allotrope.org/ontologies/role#> .
@prefix af-cur: <http://purl.allotrope.org/ontologies/curation#> .
@base <http://purl.allotrope.org/voc/afo/domain/REC/2025/06/fingerprinting#> .

<http://purl.allotrope.org/voc/afo/domain/REC/2025/06/fingerprinting> rdf:type owl:Ontology ;
                                                                                 owl:versionIRI <http://purl.allotrope.org/voc/afo/domain/REC/2025/06/fingerprinting> ;
                                                                                 owl:imports <http://purl.allotrope.org/voc/afo/REC/2025/06/afo> ;
                                                                                 dct:contributor <http://www.allotrope.org> ;
                                                                                 dct:issued "2025-06-25T12:00:00Z"^^xsd:dateTime ;
                                                                                 dct:license <http://purl.allotrope.org/voc/creative-commons-attribution-license> ;
                                                                                 dct:modified "2025-04-04T12:00:00Z"^^xsd:dateTime ;
                                                                                 dct:publisher <http://www.allotrope.org> ;
                                                                                 dct:rights <http://purl.allotrope.org/voc/attribution> ,
                                                                                            <http://purl.allotrope.org/voc/copyright> ;
                                                                                 dct:rightsHolder <http://www.allotrope.org> ;
                                                                                 dct:title "AFO Fingerprinting Domain Ontology (REC/2025/06)" ;
                                                                                 owl:priorVersion <http://purl.allotrope.org/voc/afo/domain/REC/@PRIOR_VERSION/fingerprinting> ;
                                                                                 owl:versionInfo "REC/2025/06" .

#################################################################
#    Annotation properties
#################################################################

###  http://purl.allotrope.org/ontologies/property#AFX_0002796
af-x:AFX_0002796 rdf:type owl:AnnotationProperty .


###  http://purl.allotrope.org/ontologies/property#AFX_0002798
af-x:AFX_0002798 rdf:type owl:AnnotationProperty .


###  http://purl.allotrope.org/ontologies/property#AFX_0002809
af-x:AFX_0002809 rdf:type owl:AnnotationProperty .


###  http://purl.org/dc/terms/source
dct:source rdf:type owl:AnnotationProperty .


###  http://www.w3.org/2004/02/skos/core#altLabel
skos:altLabel rdf:type owl:AnnotationProperty .


###  http://www.w3.org/2004/02/skos/core#changeNote
skos:changeNote rdf:type owl:AnnotationProperty .


###  http://www.w3.org/2004/02/skos/core#definition
skos:definition rdf:type owl:AnnotationProperty .


###  http://www.w3.org/2004/02/skos/core#example
skos:example rdf:type owl:AnnotationProperty .


###  http://www.w3.org/2004/02/skos/core#note
skos:note rdf:type owl:AnnotationProperty .


###  http://www.w3.org/2004/02/skos/core#prefLabel
skos:prefLabel rdf:type owl:AnnotationProperty .


###  http://www.w3.org/2004/02/skos/core#scopeNote
skos:scopeNote rdf:type owl:AnnotationProperty .


#################################################################
#    Classes
#################################################################

###  http://purl.allotrope.org/ontologies/result#AFR_0001607
af-r:AFR_0001607 rdf:type owl:Class ;
                 rdfs:subClassOf af-r:AFR_0001609 ;
                 skos:definition "The top identified substance is an analysis assay result facet that denotes the substance (class of materials) that has been identified by the analysis and ranked top in some measure of hit quality. [Allotrope]" ;
                 skos:prefLabel "top identified substance" .


###  http://purl.allotrope.org/ontologies/result#AFR_0001608
af-r:AFR_0001608 rdf:type owl:Class ;
                 rdfs:subClassOf af-r:AFR_0001609 ;
                 skos:altLabel "HQI" ;
                 skos:definition "The hit quality index is a measure how well the spectrum measured compares against a reference spectra of a search database. [Allotrope]" ;
                 skos:prefLabel "hit quality index" .


###  http://purl.allotrope.org/ontologies/result#AFR_0001609
af-r:AFR_0001609 rdf:type owl:Class ;
                 rdfs:subClassOf af-r:AFR_0000923 ,
                                 [ rdf:type owl:Restriction ;
                                   owl:onProperty af-x:AFX_0002734 ;
                                   owl:someValuesFrom af-p:AFP_0002691
                                 ] ;
                 skos:definition "A fingerprinting result facet is a facet that is the result of a fingerprinting process. [Allotrope]" ;
                 skos:prefLabel "fingerprinting result facet" .


###  http://purl.allotrope.org/ontologies/result#AFR_0001610
af-r:AFR_0001610 rdf:type owl:Class ;
                 rdfs:subClassOf af-r:AFR_0001505 ,
                                 [ rdf:type owl:Restriction ;
                                   owl:onProperty af-x:AFX_0000553 ;
                                   owl:someValuesFrom af-p:AFP_0002691
                                 ] ,
                                 [ rdf:type owl:Restriction ;
                                   owl:onProperty af-x:AFX_0002730 ;
                                   owl:someValuesFrom [ owl:intersectionOf ( af-rl:AFRL_0000019
                                                                             [ rdf:type owl:Restriction ;
                                                                               owl:onProperty bfo:_0000054 ;
                                                                               owl:someValuesFrom af-p:AFP_0002691
                                                                             ]
                                                                           ) ;
                                                        rdf:type owl:Class
                                                      ]
                                 ] ;
                 skos:definition "A fingerprinting parameter is a datum that is has a parameter role in some fingerprinting process. [Allotrope]" ;
                 skos:prefLabel "fingerprinting parameter" .


###  http://purl.allotrope.org/ontologies/result#AFR_0001611
af-r:AFR_0001611 rdf:type owl:Class ;
                 rdfs:subClassOf af-r:AFR_0001610 ;
                 skos:altLabel "HQI margin" ;
                 skos:definition "The hit quality index margin is a permitted hit quality index margin in either way (+/-) to account for noise and error. [Allotrope]" ;
                 skos:prefLabel "hit quality index margin" .


###  http://purl.allotrope.org/ontologies/result#AFR_0001612
af-r:AFR_0001612 rdf:type owl:Class ;
                 rdfs:subClassOf af-r:AFR_0001610 ;
                 skos:altLabel "HQI threshold" ;
                 skos:definition "The hit quality index threshold is a specification of a minimal hit quality index value for accepting positive match of the matched spectrum against the library spectrum. [Allotrope]" ;
                 skos:prefLabel "hit quality index threshold" .


###  http://purl.allotrope.org/ontologies/result#AFR_0001613
af-r:AFR_0001613 rdf:type owl:Class ;
                 rdfs:subClassOf af-r:AFR_0001608 ,
                                 [ rdf:type owl:Restriction ;
                                   owl:onProperty af-x:AFX_0002699 ;
                                   owl:someValuesFrom [ owl:intersectionOf ( af-m:AFM_0000275
                                                                             [ rdf:type owl:Restriction ;
                                                                               owl:onProperty ro:_0000087 ;
                                                                               owl:someValuesFrom af-rl:AFRL_0000127
                                                                             ]
                                                                           ) ;
                                                        rdf:type owl:Class
                                                      ]
                                 ] ;
                 skos:altLabel "analyte HQI" ,
                               "substance HQI" ,
                               "substance hit quality index" ;
                 skos:definition "The analyte hit quality index is hit quality index of the measured spectrum of the analyte against a spectrum library. [Allotrope]" ;
                 skos:prefLabel "analyte hit quality index" .


###  http://purl.allotrope.org/ontologies/result#AFR_0001614
af-r:AFR_0001614 rdf:type owl:Class ;
                 rdfs:subClassOf af-r:AFR_0001610 ,
                                 iao:_0000590 ;
                 skos:definition "A spectrum library name is a name that denotes a library of spectra used for substance identification by fingerprinting. [Allotrope]" ;
                 skos:prefLabel "spectrum library name" .


###  http://purl.allotrope.org/ontologies/result#AFR_0001615
af-r:AFR_0001615 rdf:type owl:Class ;
                 rdfs:subClassOf af-r:AFR_0001610 ;
                 skos:definition "The library search upper limit is an upper limit on the abscissa values of spectra to be searched. [Allotrope]" ;
                 skos:prefLabel "library search upper limit" .


###  http://purl.allotrope.org/ontologies/result#AFR_0001616
af-r:AFR_0001616 rdf:type owl:Class ;
                 rdfs:subClassOf af-r:AFR_0001610 ;
                 skos:definition "The library search lower limit is a lower limit on the abscissa values of spectra to be searched. [Allotrope]" ;
                 skos:prefLabel "library search lower limit" .


###  http://purl.allotrope.org/ontologies/result#AFR_0001617
af-r:AFR_0001617 rdf:type owl:Class ;
                 rdfs:subClassOf af-r:AFR_0001616 ;
                 skos:altLabel "library search lower wavenumber limit" ;
                 skos:definition "The library search start wavenumber is a lower limit on the wavenumber values of spectra to be searched. [Allotrope]" ;
                 skos:prefLabel "library search start wavenumber" .


###  http://purl.allotrope.org/ontologies/result#AFR_0001618
af-r:AFR_0001618 rdf:type owl:Class ;
                 rdfs:subClassOf af-r:AFR_0001615 ;
                 skos:altLabel "library search upper wavenumber limit" ;
                 skos:definition "The library search stop wavenumber is an upper limit on the wavenumber values of spectra to be searched. [Allotrope]" ;
                 skos:prefLabel "library search stop wavenumber" .


###  http://purl.allotrope.org/ontologies/result#AFR_0001953
af-r:AFR_0001953 rdf:type owl:Class ;
                 rdfs:subClassOf af-r:AFR_0000922 ;
                 skos:altLabel "library search report" ,
                               "library search result" ;
                 skos:definition "A spectral library search result is a report that lists the hits on search in a spectral library database. [Allotrope]" ;
                 skos:prefLabel "spectral library search result" .


###  http://purl.allotrope.org/ontologies/result#AFR_0001954
af-r:AFR_0001954 rdf:type owl:Class ;
                 rdfs:subClassOf af-r:AFR_0000922 ;
                 skos:altLabel "hit" ,
                               "library search hit" ,
                               "search hit" ;
                 skos:definition "A spectral library search hit is a result of a library search where a record matches some search criteria. [Allotrope]" ;
                 skos:prefLabel "spectral library search hit" .


###  http://purl.org/dc/terms/LicenseDocument
dct:LicenseDocument rdf:type owl:Class .


###  http://purl.org/dc/terms/RightsStatement
dct:RightsStatement rdf:type owl:Class .


#################################################################
#    Individuals
#################################################################

###  http://www.allotrope.org
<http://www.allotrope.org> rdf:type owl:NamedIndividual ,
                                    foaf:Organization ;
                           foaf:name "Allotrope Foundation" .


###  http://purl.allotrope.org/voc/attribution
<http://purl.allotrope.org/voc/attribution> rdf:type owl:NamedIndividual ,
                                                     dct:RightsStatement ;
                                            dct:description """
These taxonomies contain material or may constitute derivative works of material which may be subject to copyright by one of the following organizations.  By using these taxonomies, you agree to the following terms and conditions applicable to its contents:
******************************************************************************
Copyright Notice and Terms for IUPAC Gold Book
______________________________________________________________________________
Copyright © 1998, Regents of the University of California
All rights reserved.
Redistribution and use in source and binary forms, with or without modification, are permitted provided that the following conditions are met:
1. Redistributions of source code must retain the above copyright notice, this list of conditions and the following disclaimer.
2. Redistributions in binary form must reproduce the above copyright notice, this list of conditions and the following disclaimer in the documentation and/or other materials provided with the distribution.
THIS SOFTWARE IS PROVIDED BY THE COPYRIGHT HOLDERS AND CONTRIBUTORS \"AS IS\" AND ANY EXPRESS OR IMPLIED WARRANTIES, INCLUDING, BUT NOT LIMITED TO, THE IMPLIED WARRANTIES OF MERCHANTABILITY AND FITNESS FOR A PARTICULAR PURPOSE ARE DISCLAIMED. IN NO EVENT SHALL THE COPYRIGHT HOLDER OR CONTRIBUTORS BE LIABLE FOR ANY DIRECT, INDIRECT, INCIDENTAL, SPECIAL, EXEMPLARY, OR CONSEQUENTIAL DAMAGES (INCLUDING, BUT NOT LIMITED TO, PROCUREMENT OF SUBSTITUTE GOODS OR SERVICES; LOSS OF USE, DATA, OR PROFITS; OR BUSINESS INTERRUPTION) HOWEVER CAUSED AND ON ANY THEORY OF LIABILITY, WHETHER IN CONTRACT, STRICT LIABILITY, OR TORT (INCLUDING NEGLIGENCE OR OTHERWISE) ARISING IN ANY WAY OUT OF THE USE OF THIS SOFTWARE, EVEN IF ADVISED OF THE POSSIBILITY OF SUCH DAMAGE.
******************************************************************************
Copyright Notice and Terms for PSI-MS (Proteomics Standards Initiative - Mass Spectrometry) Mass spectrometer output files and spectra interpretation
_____________________________________________________________________________
Created by Matt Chambers, Andreas Bertsch, Marius Kallhardt, Eric Deutsch Fredrik Levander, Pierre-Alain Binz, and Gerhard Mayer. Publisher: HUPO Proteomics Standards Initiative Mass Spectrometry Standards Working Group and HUPO Proteomics Standards Initiative Proteomics Informatics Working Group. This work is used pursuant to a Creative Commons license available here: http://creativecommons.org/licenses/by/3.0/legalcode

******************************************************************************
Attribution Notice for National Center for Biomedical Ontology materials. 

This work contains material from the Cell Ontology and Clinical Measurement Ontology, available here: http://bioportal.bioontology.org/.
******************************************************************************
Attribution Notice for ChEBI
This work contains material from the European Bioinformatics Institute’s ChEBI database. 
******************************************************************************
Attribution Notice for Quantities Units Dimensions Data Types (http://www.qudt.org/)
This work contains content from www.qudt.org and is used pursuant to a Creative Commons License available here: http://creativecommons.org/licenses/by-sa/3.0/us/legalcode. The original work may have been modified. 
******************************************************************************
Copyright and Attribution Notice for Dublin Core Metadata Initiative Document
This work contains material from the following DCMI document used pursuant to a creative commons license available here: https://creativecommons.org/licenses/by/4.0/legalcode. This material may have been modified or changed.
Timestamped URL:          http://dublincore.org/documents/2012/06/14/dcmi-terms/ 
Date Issued:                       2012-06-14 
Document Status:            This is a DCMI Recommendation.
Copyright © 1995-2015 DCMI. All Rights Reserved. DCMI liability, trademark/service mark, document use and software licensing rules apply. 
******************************************************************************

""" ;
                                            dct:title "Derivative works attribution" .


###  http://purl.allotrope.org/voc/copyright
<http://purl.allotrope.org/voc/copyright> rdf:type owl:NamedIndividual ,
                                                   dct:RightsStatement ;
                                          dct:description "Copyright © 2015-2025 Allotrope Foundation" ;
                                          dct:rightsHolder <http://www.allotrope.org> ;
                                          dct:title "Copyright © 2015-2025 Allotrope Foundation" .


###  http://purl.allotrope.org/voc/creative-commons-attribution-license
<http://purl.allotrope.org/voc/creative-commons-attribution-license> rdf:type owl:NamedIndividual ,
                                                                              dct:LicenseDocument ;
                                                                     dct:description """This work is licensed under a Creative Commons Attribution 4.0 International License http://creativecommons.org/licenses/by/4.0/.

THESE MATERIALS ARE PROVIDED \"AS IS\" AND ALLOTROPE EXPRESSLY DISCLAIMS ALL WARRANTIES, EXPRESS, IMPLIED OR STATUTORY, INCLUDING, WITHOUT LIMITATION, THE WARRANTIES OF NON-INFRINGEMENT, TITLE, MERCHANTABILITY AND FITNESS FOR A PARTICULAR PURPOSE.

Copyright © 2015-2025 Allotrope Foundation
""" ;
                                                                     dct:title "Creative Commons Attribution 4.0 International Public License" .


###  Generated by the OWL API (version 5.1.19) https://github.com/owlcs/owlapi/
