@prefix : <http://purl.allotrope.org/voc/afo/domain/REC/2025/06/fluorescence#> .
@prefix cl: <http://purl.obolibrary.org/obo/CL> .
@prefix go: <http://purl.obolibrary.org/obo/GO> .
@prefix ro: <http://purl.obolibrary.org/obo/RO> .
@prefix bfo: <http://purl.obolibrary.org/obo/BFO> .
@prefix dct: <http://purl.org/dc/terms/> .
@prefix iao: <http://purl.obolibrary.org/obo/IAO> .
@prefix obi: <http://purl.obolibrary.org/obo/OBI> .
@prefix owl: <http://www.w3.org/2002/07/owl#> .
@prefix rdf: <http://www.w3.org/1999/02/22-rdf-syntax-ns#> .
@prefix xml: <http://www.w3.org/XML/1998/namespace> .
@prefix xsd: <http://www.w3.org/2001/XMLSchema#> .
@prefix af-c: <http://purl.allotrope.org/ontologies/common#> .
@prefix af-e: <http://purl.allotrope.org/ontologies/equipment#> .
@prefix af-m: <http://purl.allotrope.org/ontologies/material#> .
@prefix af-p: <http://purl.allotrope.org/ontologies/process#> .
@prefix af-q: <http://purl.allotrope.org/ontologies/quality#> .
@prefix af-r: <http://purl.allotrope.org/ontologies/result#> .
@prefix af-x: <http://purl.allotrope.org/ontologies/property#> .
@prefix chmo: <http://purl.obolibrary.org/obo/CHMO> .
@prefix foaf: <http://xmlns.com/foaf/0.1/> .
@prefix pato: <http://purl.obolibrary.org/obo/PATO> .
@prefix rdfs: <http://www.w3.org/2000/01/rdf-schema#> .
@prefix skos: <http://www.w3.org/2004/02/skos/core#> .
@prefix af-rl: <http://purl.allotrope.org/ontologies/role#> .
@prefix chebi: <http://purl.obolibrary.org/obo/CHEBI> .
@prefix af-cur: <http://purl.allotrope.org/ontologies/curation#> .
@base <http://purl.allotrope.org/voc/afo/domain/REC/2025/06/fluorescence#> .

<http://purl.allotrope.org/voc/afo/domain/REC/2025/06/fluorescence> rdf:type owl:Ontology ;
                                                                               owl:versionIRI <http://purl.allotrope.org/voc/afo/domain/REC/2025/06/fluorescence> ;
                                                                               owl:imports <http://purl.allotrope.org/voc/afo/REC/2025/06/afo> ;
                                                                               dct:contributor <http://www.allotrope.org> ;
                                                                               dct:issued "2025-06-25T12:00:00Z"^^xsd:dateTime ;
                                                                               dct:license <http://purl.allotrope.org/voc/creative-commons-attribution-license> ;
                                                                               dct:modified "2025-06-11T12:00:00Z"^^xsd:dateTime ;
                                                                               dct:publisher <http://www.allotrope.org> ;
                                                                               dct:rights <http://purl.allotrope.org/voc/attribution> ,
                                                                                          <http://purl.allotrope.org/voc/copyright> ;
                                                                               dct:rightsHolder <http://www.allotrope.org> ;
                                                                               dct:title "AFO Fluorescence Domain Ontology (REC/2025/06)" ;
                                                                               owl:versionInfo "REC/2025/06" .

#################################################################
#    Annotation properties
#################################################################

###  http://purl.allotrope.org/ontologies/property#AFX_0002796
af-x:AFX_0002796 rdf:type owl:AnnotationProperty .


###  http://purl.allotrope.org/ontologies/property#AFX_0002798
af-x:AFX_0002798 rdf:type owl:AnnotationProperty .


###  http://purl.allotrope.org/ontologies/property#AFX_0002809
af-x:AFX_0002809 rdf:type owl:AnnotationProperty .


###  http://purl.org/dc/terms/source
dct:source rdf:type owl:AnnotationProperty .


###  http://www.w3.org/2004/02/skos/core#altLabel
skos:altLabel rdf:type owl:AnnotationProperty .


###  http://www.w3.org/2004/02/skos/core#changeNote
skos:changeNote rdf:type owl:AnnotationProperty .


###  http://www.w3.org/2004/02/skos/core#definition
skos:definition rdf:type owl:AnnotationProperty .


###  http://www.w3.org/2004/02/skos/core#example
skos:example rdf:type owl:AnnotationProperty .


###  http://www.w3.org/2004/02/skos/core#note
skos:note rdf:type owl:AnnotationProperty .


###  http://www.w3.org/2004/02/skos/core#prefLabel
skos:prefLabel rdf:type owl:AnnotationProperty .


###  http://www.w3.org/2004/02/skos/core#scopeNote
skos:scopeNote rdf:type owl:AnnotationProperty .


#################################################################
#    Classes
#################################################################

###  http://purl.allotrope.org/ontologies/result#AFR_0002481
af-r:AFR_0002481 rdf:type owl:Class ;
                 rdfs:subClassOf af-r:AFR_0000992 ,
                                 <http://purl.org/linked-data/cube#DataSet> ,
                                 [ rdf:type owl:Restriction ;
                                   owl:onProperty [ owl:inverseOf af-x:AFX_0002737
                                                  ] ;
                                   owl:someValuesFrom af-r:AFR_0002483
                                 ] ;
                 skos:definition "A fluorescence excitation spectrum data cube is a data cube that represents a fluorescence excitation spectrum. [Allotrope]" ;
                 skos:prefLabel "fluorescence excitation spectrum data cube" .


###  http://purl.allotrope.org/ontologies/result#AFR_0002482
af-r:AFR_0002482 rdf:type owl:Class ;
                 rdfs:subClassOf af-r:AFR_0000992 ,
                                 <http://purl.org/linked-data/cube#DataSet> ,
                                 [ rdf:type owl:Restriction ;
                                   owl:onProperty [ owl:inverseOf af-x:AFX_0002737
                                                  ] ;
                                   owl:someValuesFrom af-r:AFR_0000136
                                 ] ;
                 skos:definition "A fluorescence emission spectrum data cube is a data cube that represents a fluorescence emission spectrum. [Allotrope]" ;
                 skos:prefLabel "fluorescence emission spectrum data cube" .


###  http://purl.allotrope.org/ontologies/result#AFR_0002483
af-r:AFR_0002483 rdf:type owl:Class ;
                 rdfs:subClassOf af-r:AFR_0000068 ;
                 skos:definition "A fluorescence excitation spectrum is a spectrum that plots the intensity of fluorescence of a material entity vs the excitation wavelength at a defined emission wavelength. [Allotrope]" ;
                 skos:prefLabel "fluorescence excitation spectrum" .


###  http://purl.allotrope.org/ontologies/result#AFR_0002870
af-r:AFR_0002870 rdf:type owl:Class ;
                 rdfs:subClassOf af-r:AFR_0001243 ;
                 skos:definition "A fluorescent tag setting is a setting that specifies the fluorescent tag being targeted. [Allotrope]" ;
                 skos:prefLabel "fluorescent tag setting" .


###  http://purl.allotrope.org/ontologies/result#AFR_0002875
af-r:AFR_0002875 rdf:type owl:Class ;
                 rdfs:subClassOf af-r:AFR_0001277 ,
                                 [ rdf:type owl:Restriction ;
                                   owl:onProperty af-x:AFX_0002806 ;
                                   owl:someValuesFrom [ owl:intersectionOf ( chebi:_23367
                                                                             [ rdf:type owl:Restriction ;
                                                                               owl:onProperty ro:_0000087 ;
                                                                               owl:someValuesFrom af-rl:AFRL_0000573
                                                                             ]
                                                                           ) ;
                                                        rdf:type owl:Class
                                                      ]
                                 ] ;
                 af-x:AFX_0002798 "true"^^xsd:boolean ;
                 skos:definition "A fluorescent tag identifier is an identifier for the type of molecules having the role of fluorescent tag. [Allotrope]" ;
                 skos:prefLabel "fluorescent tag identifier" .


###  http://purl.allotrope.org/ontologies/result#AFR_0002964
af-r:AFR_0002964 rdf:type owl:Class ;
                 rdfs:subClassOf af-r:AFR_0000576 ,
                                 [ rdf:type owl:Restriction ;
                                   owl:onProperty af-x:AFX_0002816 ;
                                   owl:someValuesFrom af-p:AFP_0003846
                                 ] ;
                 af-x:AFX_0002798 "true"^^xsd:boolean ;
                 skos:definition "A fluorescence emission profile is a profile that quantifies the fluorescence emission of a material entity over time. [Allotrope]" ;
                 skos:prefLabel "fluorescence emission profile" .


###  http://purl.allotrope.org/ontologies/result#AFR_0002965
af-r:AFR_0002965 rdf:type owl:Class ;
                 rdfs:subClassOf af-r:AFR_0000992 ,
                                 <http://purl.org/linked-data/cube#DataSet> ,
                                 [ rdf:type owl:Restriction ;
                                   owl:onProperty [ owl:inverseOf af-x:AFX_0002737
                                                  ] ;
                                   owl:someValuesFrom af-r:AFR_0002964
                                 ] ;
                 skos:definition "A fluorescence emission profile data cube is a data cube that represents a fluorescence emission profile. [Allotrope]" ;
                 skos:prefLabel "fluorescence emission profile data cube" .


###  http://purl.allotrope.org/ontologies/result#AFR_0003209
af-r:AFR_0003209 rdf:type owl:Class ;
                 rdfs:subClassOf af-r:AFR_0000992 ,
                                 <http://purl.org/linked-data/cube#DataSet> ,
                                 [ rdf:type owl:Restriction ;
                                   owl:onProperty [ owl:inverseOf af-x:AFX_0002737
                                                  ] ;
                                   owl:someValuesFrom af-r:AFR_0003211
                                 ] ;
                 skos:definition "A fluorescence area scan data cube is a data cube that represents a fluorescence area scan. [Allotrope]" ;
                 skos:prefLabel "fluorescence area scan data cube" .


###  http://purl.allotrope.org/ontologies/result#AFR_0003211
af-r:AFR_0003211 rdf:type owl:Class ;
                 rdfs:subClassOf af-r:AFR_0002499 ;
                 af-x:AFX_0002798 "true"^^xsd:boolean ;
                 skos:definition "A fluorescence area scan is a data distribution function of the fluorescence of a material entity scanned over a predefined area. [Allotrope]" ;
                 skos:prefLabel "fluorescence area scan" .


###  http://purl.allotrope.org/ontologies/role#AFRL_0000526
af-rl:AFRL_0000526 rdf:type owl:Class .


###  http://purl.allotrope.org/ontologies/role#AFRL_0000573
af-rl:AFRL_0000573 rdf:type owl:Class ;
                   rdfs:subClassOf af-rl:AFRL_0000574 ,
                                   [ rdf:type owl:Restriction ;
                                     owl:onProperty ro:_0000081 ;
                                     owl:someValuesFrom chebi:_23367
                                   ] ;
                   skos:definition "A fluorescent tag role is the role of a molecular entity in a fluorescence experiment that is attached chemically to aid in the detection of a biomolecule. [Allotrope, Wikipedia]" ;
                   skos:prefLabel "fluorescent tag role" .


###  http://purl.allotrope.org/ontologies/role#AFRL_0000574
af-rl:AFRL_0000574 rdf:type owl:Class ;
                   owl:equivalentClass [ owl:intersectionOf ( bfo:_0000023
                                                              [ rdf:type owl:Restriction ;
                                                                owl:onProperty bfo:_0000054 ;
                                                                owl:someValuesFrom af-p:AFP_0002788
                                                              ]
                                                            ) ;
                                         rdf:type owl:Class
                                       ] ;
                   af-x:AFX_0002798 "true"^^xsd:boolean ;
                   skos:definition "A fluorimetry role is a role of a material entity realized in a fluorimetry process. [Allotrope]" ;
                   skos:prefLabel "fluorimetry role" .


#################################################################
#    Individuals
#################################################################

###  http://www.allotrope.org
<http://www.allotrope.org> rdf:type owl:NamedIndividual ,
                                    foaf:Organization ;
                           foaf:name "Allotrope Foundation" .


###  http://purl.allotrope.org/voc/attribution
<http://purl.allotrope.org/voc/attribution> rdf:type owl:NamedIndividual ,
                                                     dct:RightsStatement ;
                                            dct:description """
These taxonomies contain material or may constitute derivative works of material which may be subject to copyright by one of the following organizations.  By using these taxonomies, you agree to the following terms and conditions applicable to its contents:
******************************************************************************
Copyright Notice and Terms for IUPAC Gold Book
______________________________________________________________________________
Copyright © 1998, Regents of the University of California
All rights reserved.
Redistribution and use in source and binary forms, with or without modification, are permitted provided that the following conditions are met:
1. Redistributions of source code must retain the above copyright notice, this list of conditions and the following disclaimer.
2. Redistributions in binary form must reproduce the above copyright notice, this list of conditions and the following disclaimer in the documentation and/or other materials provided with the distribution.
THIS SOFTWARE IS PROVIDED BY THE COPYRIGHT HOLDERS AND CONTRIBUTORS \"AS IS\" AND ANY EXPRESS OR IMPLIED WARRANTIES, INCLUDING, BUT NOT LIMITED TO, THE IMPLIED WARRANTIES OF MERCHANTABILITY AND FITNESS FOR A PARTICULAR PURPOSE ARE DISCLAIMED. IN NO EVENT SHALL THE COPYRIGHT HOLDER OR CONTRIBUTORS BE LIABLE FOR ANY DIRECT, INDIRECT, INCIDENTAL, SPECIAL, EXEMPLARY, OR CONSEQUENTIAL DAMAGES (INCLUDING, BUT NOT LIMITED TO, PROCUREMENT OF SUBSTITUTE GOODS OR SERVICES; LOSS OF USE, DATA, OR PROFITS; OR BUSINESS INTERRUPTION) HOWEVER CAUSED AND ON ANY THEORY OF LIABILITY, WHETHER IN CONTRACT, STRICT LIABILITY, OR TORT (INCLUDING NEGLIGENCE OR OTHERWISE) ARISING IN ANY WAY OUT OF THE USE OF THIS SOFTWARE, EVEN IF ADVISED OF THE POSSIBILITY OF SUCH DAMAGE.
******************************************************************************
Copyright Notice and Terms for PSI-MS (Proteomics Standards Initiative - Mass Spectrometry) Mass spectrometer output files and spectra interpretation
_____________________________________________________________________________
Created by Matt Chambers, Andreas Bertsch, Marius Kallhardt, Eric Deutsch Fredrik Levander, Pierre-Alain Binz, and Gerhard Mayer. Publisher: HUPO Proteomics Standards Initiative Mass Spectrometry Standards Working Group and HUPO Proteomics Standards Initiative Proteomics Informatics Working Group. This work is used pursuant to a Creative Commons license available here: http://creativecommons.org/licenses/by/3.0/legalcode

******************************************************************************
Attribution Notice for National Center for Biomedical Ontology materials.

This work contains material from the Cell Ontology and Clinical Measurement Ontology, available here: http://bioportal.bioontology.org/.
******************************************************************************
Attribution Notice for ChEBI
This work contains material from the European Bioinformatics Institute’s ChEBI database.
******************************************************************************
Attribution Notice for Quantities Units Dimensions Data Types (http://www.qudt.org/)
This work contains content from www.qudt.org and is used pursuant to a Creative Commons License available here: http://creativecommons.org/licenses/by-sa/3.0/us/legalcode. The original work may have been modified.
******************************************************************************
Copyright and Attribution Notice for Dublin Core Metadata Initiative Document
This work contains material from the following DCMI document used pursuant to a creative commons license available here: https://creativecommons.org/licenses/by/4.0/legalcode. This material may have been modified or changed.
Timestamped URL:          http://dublincore.org/documents/2012/06/14/dcmi-terms/
Date Issued:                       2012-06-14
Document Status:            This is a DCMI Recommendation.
Copyright © 1995-2015 DCMI. All Rights Reserved. DCMI liability, trademark/service mark, document use and software licensing rules apply.
******************************************************************************

""" ;
                                            dct:title "Derivative works attribution" .


###  http://purl.allotrope.org/voc/copyright
<http://purl.allotrope.org/voc/copyright> rdf:type owl:NamedIndividual ,
                                                   dct:RightsStatement ;
                                          dct:description "Copyright © 2021 Allotrope Foundation" ;
                                          dct:rightsHolder <http://www.allotrope.org> ;
                                          dct:title "Copyright © 2021 Allotrope Foundation" .


###  http://purl.allotrope.org/voc/creative-commons-attribution-license
<http://purl.allotrope.org/voc/creative-commons-attribution-license> rdf:type owl:NamedIndividual ,
                                                                              dct:LicenseDocument ;
                                                                     dct:description """This work is licensed under a Creative Commons Attribution 4.0 International License http://creativecommons.org/licenses/by/4.0/.

THESE MATERIALS ARE PROVIDED \"AS IS\" AND ALLOTROPE EXPRESSLY DISCLAIMS ALL WARRANTIES, EXPRESS, IMPLIED OR STATUTORY, INCLUDING, WITHOUT LIMITATION, THE WARRANTIES OF NON-INFRINGEMENT, TITLE, MERCHANTABILITY AND FITNESS FOR A PARTICULAR PURPOSE.

Copyright © 2015-2025 Allotrope Foundation
""" ;
                                                                     dct:title "Creative Commons Attribution 4.0 International Public License" .


###  Generated by the OWL API (version 5.1.19) https://github.com/owlcs/owlapi/
