@prefix : <http://purl.allotrope.org/voc/afo/domain/REC/2025/06/foam-height#> .
@prefix cl: <http://purl.obolibrary.org/obo/CL> .
@prefix go: <http://purl.obolibrary.org/obo/GO> .
@prefix ro: <http://purl.obolibrary.org/obo/RO> .
@prefix bfo: <http://purl.obolibrary.org/obo/BFO> .
@prefix dct: <http://purl.org/dc/terms/> .
@prefix iao: <http://purl.obolibrary.org/obo/IAO> .
@prefix obi: <http://purl.obolibrary.org/obo/OBI> .
@prefix owl: <http://www.w3.org/2002/07/owl#> .
@prefix rdf: <http://www.w3.org/1999/02/22-rdf-syntax-ns#> .
@prefix xml: <http://www.w3.org/XML/1998/namespace> .
@prefix xsd: <http://www.w3.org/2001/XMLSchema#> .
@prefix af-c: <http://purl.allotrope.org/ontologies/common#> .
@prefix af-e: <http://purl.allotrope.org/ontologies/equipment#> .
@prefix af-m: <http://purl.allotrope.org/ontologies/material#> .
@prefix af-p: <http://purl.allotrope.org/ontologies/process#> .
@prefix af-q: <http://purl.allotrope.org/ontologies/quality#> .
@prefix af-r: <http://purl.allotrope.org/ontologies/result#> .
@prefix af-x: <http://purl.allotrope.org/ontologies/property#> .
@prefix chmo: <http://purl.obolibrary.org/obo/CHMO> .
@prefix foaf: <http://xmlns.com/foaf/0.1/> .
@prefix pato: <http://purl.obolibrary.org/obo/PATO> .
@prefix rdfs: <http://www.w3.org/2000/01/rdf-schema#> .
@prefix skos: <http://www.w3.org/2004/02/skos/core#> .
@prefix chebi: <http://purl.obolibrary.org/obo/CHEBI> .
@prefix af-cur: <http://purl.allotrope.org/ontologies/curation#> .
@base <http://purl.allotrope.org/voc/afo/domain/REC/2025/06/foam-height#> .

<http://purl.allotrope.org/voc/afo/domain/REC/2025/06/foam-height> rdf:type owl:Ontology ;
                                                                              owl:versionIRI <http://purl.allotrope.org/voc/afo/domain/REC/2025/06/foam-height> ;
                                                                              owl:imports <http://purl.allotrope.org/voc/afo/REC/2025/06/afo> ;
                                                                              dct:contributor <http://www.allotrope.org> ;
                                                                              dct:issued "2025-06-25T12:00:00Z"^^xsd:dateTime ;
                                                                              dct:license <http://purl.allotrope.org/voc/creative-commons-attribution-license> ;
                                                                              dct:modified "2025-04-04T12:00:00Z"^^xsd:dateTime ;
                                                                              dct:publisher <http://www.allotrope.org> ;
                                                                              dct:rights <http://purl.allotrope.org/voc/attribution> ,
                                                                                         <http://purl.allotrope.org/voc/copyright> ;
                                                                              dct:rightsHolder <http://www.allotrope.org> ;
                                                                              dct:title "AFO Foam Height Domain Ontology (REC/2025/06)" ;
                                                                              owl:versionInfo "REC/2025/06" .

#################################################################
#    Annotation properties
#################################################################

###  http://purl.allotrope.org/ontologies/property#AFX_0002796
af-x:AFX_0002796 rdf:type owl:AnnotationProperty .


###  http://purl.allotrope.org/ontologies/property#AFX_0002798
af-x:AFX_0002798 rdf:type owl:AnnotationProperty .


###  http://purl.allotrope.org/ontologies/property#AFX_0002809
af-x:AFX_0002809 rdf:type owl:AnnotationProperty .


###  http://purl.org/dc/terms/source
dct:source rdf:type owl:AnnotationProperty .


###  http://www.w3.org/2004/02/skos/core#altLabel
skos:altLabel rdf:type owl:AnnotationProperty .


###  http://www.w3.org/2004/02/skos/core#changeNote
skos:changeNote rdf:type owl:AnnotationProperty .


###  http://www.w3.org/2004/02/skos/core#definition
skos:definition rdf:type owl:AnnotationProperty .


###  http://www.w3.org/2004/02/skos/core#example
skos:example rdf:type owl:AnnotationProperty .


###  http://www.w3.org/2004/02/skos/core#note
skos:note rdf:type owl:AnnotationProperty .


###  http://www.w3.org/2004/02/skos/core#prefLabel
skos:prefLabel rdf:type owl:AnnotationProperty .


###  http://www.w3.org/2004/02/skos/core#scopeNote
skos:scopeNote rdf:type owl:AnnotationProperty .


#################################################################
#    Classes
#################################################################

###  http://purl.allotrope.org/ontologies/result#AFR_0002661
af-r:AFR_0002661 rdf:type owl:Class ;
                 rdfs:subClassOf af-r:AFR_0001243 ;
                 skos:definition "A maximum row setting is a control setting specifying a maximum row of pixels in a raster image. [Allotrope]" ;
                 skos:prefLabel "maximum row setting (foam height)" .


###  http://purl.allotrope.org/ontologies/result#AFR_0002662
af-r:AFR_0002662 rdf:type owl:Class ;
                 rdfs:subClassOf af-r:AFR_0001243 ;
                 skos:definition "A foam detection sensitivity setting is a control setting that specifies the sensitivity for detection of foam. [Allotrope]" ;
                 skos:prefLabel "foam detection sensitivity setting" .


###  http://purl.allotrope.org/ontologies/result#AFR_0002663
af-r:AFR_0002663 rdf:type owl:Class ;
                 rdfs:subClassOf af-r:AFR_0001243 ;
                 skos:definition "A smoothing window setting is a control setting that specifies the smoothing window for foam detection. [Allotrope]" ;
                 skos:prefLabel "smoothing window setting" .


###  http://purl.allotrope.org/ontologies/result#AFR_0002665
af-r:AFR_0002665 rdf:type owl:Class ;
                 rdfs:subClassOf af-r:AFR_0002473 ;
                 skos:definition "A liquid start row is the minimum row of pixels in a raster image where a liquid is detected. [Allotrope]" ;
                 skos:prefLabel "liquid start row" .


###  http://purl.allotrope.org/ontologies/result#AFR_0002666
af-r:AFR_0002666 rdf:type owl:Class ;
                 rdfs:subClassOf af-r:AFR_0002473 ;
                 skos:definition "A liquid end row is the maximum row of pixels in a raster image where a liquid is detected. [Allotrope]" ;
                 skos:prefLabel "liquid end row" .


###  http://purl.allotrope.org/ontologies/result#AFR_0002667
af-r:AFR_0002667 rdf:type owl:Class ;
                 rdfs:subClassOf af-r:AFR_0000207 ;
                 skos:definition "A foam detection result is an assay result that specifies whether foam was detected. [Allotrope]" ;
                 skos:prefLabel "foam detection result" .


###  http://purl.allotrope.org/ontologies/result#AFR_0002668
af-r:AFR_0002668 rdf:type owl:Class ;
                 rdfs:subClassOf af-r:AFR_0002473 ;
                 skos:definition "A foam start row is the minimum row of pixels in a raster image where a foam is detected. [Allotrope]" ;
                 skos:prefLabel "foam start row" .


###  http://purl.allotrope.org/ontologies/result#AFR_0002669
af-r:AFR_0002669 rdf:type owl:Class ;
                 rdfs:subClassOf af-r:AFR_0002473 ;
                 skos:definition "A foam end row is the maximum row of pixels in a raster image where a foam is detected. [Allotrope]" ;
                 skos:prefLabel "foam end row" .


###  http://purl.allotrope.org/ontologies/result#AFR_0002670
af-r:AFR_0002670 rdf:type owl:Class ;
                 rdfs:subClassOf af-r:AFR_0000984 ;
                 skos:definition "A liquid row count is a count of the number of rows of pixels in a raster image where liquid is detected. [Allotrope]" ;
                 skos:prefLabel "liquid row count" .


###  http://purl.allotrope.org/ontologies/result#AFR_0002671
af-r:AFR_0002671 rdf:type owl:Class ;
                 rdfs:subClassOf af-r:AFR_0000984 ;
                 skos:definition "A foam row count is a count of the number of rows of pixels in a raster image where foam is detected, including any air gap if present. [Allotrope]" ;
                 skos:prefLabel "foam row count" .


###  http://purl.allotrope.org/ontologies/result#AFR_0002672
af-r:AFR_0002672 rdf:type owl:Class ;
                 rdfs:subClassOf af-r:AFR_0000984 ;
                 skos:definition "A total row count is a count of the number of rows of pixels in a raster image where any liquid or foam is detected. [Allotrope]" ;
                 skos:prefLabel "total row count (foam height)" .


###  http://purl.allotrope.org/ontologies/result#AFR_0002673
af-r:AFR_0002673 rdf:type owl:Class ;
                 rdfs:subClassOf af-r:AFR_0002692 ,
                                 [ rdf:type owl:Restriction ;
                                   owl:onProperty af-x:AFX_0002816 ;
                                   owl:someValuesFrom [ rdf:type owl:Restriction ;
                                                        owl:onProperty ro:_0000080 ;
                                                        owl:someValuesFrom af-m:AFM_0000403
                                                      ]
                                 ] ;
                 skos:definition "A liquid height is a height of some liquid. [Allotrope]" ;
                 skos:prefLabel "liquid height" .


###  http://purl.allotrope.org/ontologies/result#AFR_0002674
af-r:AFR_0002674 rdf:type owl:Class ;
                 rdfs:subClassOf af-r:AFR_0002696 ;
                 skos:definition "A total foam height is a height of some foam, including any air gap if present. [Allotrope]" ;
                 skos:prefLabel "total foam height" .


###  http://purl.allotrope.org/ontologies/result#AFR_0002675
af-r:AFR_0002675 rdf:type owl:Class ;
                 rdfs:subClassOf af-r:AFR_0002692 ,
                                 [ rdf:type owl:Restriction ;
                                   owl:onProperty af-x:AFX_0002816 ;
                                   owl:someValuesFrom [ rdf:type owl:Restriction ;
                                                        owl:onProperty ro:_0000080 ;
                                                        owl:someValuesFrom chmo:_0000993
                                                      ]
                                 ] ;
                 skos:definition "A total material height is the summation of heights of some collection of materials. [Allotrope]" ;
                 skos:prefLabel "total material height" .


###  http://purl.allotrope.org/ontologies/result#AFR_0002676
af-r:AFR_0002676 rdf:type owl:Class ;
                 rdfs:subClassOf af-r:AFR_0000207 ;
                 skos:definition "An air gap detection result is an assay result that specifies whether an air gap was detected. [Allotrope]" ;
                 skos:prefLabel "air gap detection result" .


###  http://purl.allotrope.org/ontologies/result#AFR_0002677
af-r:AFR_0002677 rdf:type owl:Class ;
                 rdfs:subClassOf af-r:AFR_0000984 ;
                 skos:definition "A normalized foam row count is a count of the number of rows of pixels in a raster image where foam is detected, excluding any air gap if present. [Allotrope]" ;
                 skos:prefLabel "normalized foam row count" .


###  http://purl.allotrope.org/ontologies/result#AFR_0002678
af-r:AFR_0002678 rdf:type owl:Class ;
                 rdfs:subClassOf af-r:AFR_0002696 ;
                 skos:definition "A normalized foam height is a height of some foam, excluding any air gap if present. [Allotrope]" ;
                 skos:prefLabel "normalized foam height" .


###  http://purl.allotrope.org/ontologies/result#AFR_0002679
af-r:AFR_0002679 rdf:type owl:Class ;
                 rdfs:subClassOf af-r:AFR_0000984 ;
                 skos:definition "An above gap foam row count is a count of the number of rows of pixels in a raster image where foam is detected above an air gap. [Allotrope]" ;
                 skos:prefLabel "above gap foam row count" .


###  http://purl.allotrope.org/ontologies/result#AFR_0002680
af-r:AFR_0002680 rdf:type owl:Class ;
                 rdfs:subClassOf af-r:AFR_0000984 ;
                 skos:definition "A below gap foam row count is a count of the number of rows of pixels in a raster image where foam is detected below an air gap. [Allotrope]" ;
                 skos:prefLabel "below gap foam row count" .


###  http://purl.allotrope.org/ontologies/result#AFR_0002681
af-r:AFR_0002681 rdf:type owl:Class ;
                 rdfs:subClassOf af-r:AFR_0000922 ;
                 skos:definition "A liquid homogeneity gradient is a description describing the magnitude of the difference between the foam and liquid sides of an extrapolated boundary in a sample. [Allotrope]" ;
                 skos:prefLabel "liquid homogeneity gradient" .


###  http://purl.allotrope.org/ontologies/result#AFR_0002683
af-r:AFR_0002683 rdf:type owl:Class ;
                 rdfs:subClassOf af-c:AFC_0000160 ,
                                 iao:_0000310 ,
                                 [ rdf:type owl:Restriction ;
                                   owl:onProperty ro:_0002351 ;
                                   owl:someValuesFrom af-r:AFR_0002684
                                 ] ;
                 skos:definition "A bubble aggregate document is a document that aggregates bubble documents. [Allotrope]" ;
                 skos:prefLabel "bubble aggregate document" .


###  http://purl.allotrope.org/ontologies/result#AFR_0002684
af-r:AFR_0002684 rdf:type owl:Class ;
                 rdfs:subClassOf iao:_0000310 ,
                                 [ rdf:type owl:Restriction ;
                                   owl:onProperty iao:_0000136 ;
                                   owl:someValuesFrom af-m:AFM_0001125
                                 ] ;
                 skos:definition "A bubble document is a document that encompasses the information associated with a bubble. [Allotrope]" ;
                 skos:prefLabel "bubble document" .


###  http://purl.allotrope.org/ontologies/result#AFR_0002696
af-r:AFR_0002696 rdf:type owl:Class ;
                 rdfs:subClassOf af-r:AFR_0002692 ,
                                 [ rdf:type owl:Restriction ;
                                   owl:onProperty af-x:AFX_0002816 ;
                                   owl:someValuesFrom [ rdf:type owl:Restriction ;
                                                        owl:onProperty ro:_0000080 ;
                                                        owl:someValuesFrom af-m:AFM_0001032
                                                      ]
                                 ] ;
                 skos:definition "A foam height is a height of some foam. [Allotrope]" ;
                 skos:prefLabel "foam height" .


###  http://purl.allotrope.org/ontologies/result#AFR_0002847
af-r:AFR_0002847 rdf:type owl:Class ;
                 rdfs:subClassOf af-c:AFC_0000160 ,
                                 iao:_0000310 ,
                                 [ rdf:type owl:Restriction ;
                                   owl:onProperty ro:_0002351 ;
                                   owl:someValuesFrom af-r:AFR_0002848
                                 ] ;
                 skos:definition "A foam height aggregate document is a document that aggregates foam height documents. [Allotrope]" ;
                 skos:prefLabel "foam height aggregate document" .


###  http://purl.allotrope.org/ontologies/result#AFR_0002848
af-r:AFR_0002848 rdf:type owl:Class ;
                 rdfs:subClassOf iao:_0000310 ;
                 skos:definition "A foam height document is a document that encompasses the information associated with some foam height run. [Allotrope]" ;
                 skos:prefLabel "foam height document" .


#################################################################
#    Individuals
#################################################################

###  http://www.allotrope.org
<http://www.allotrope.org> rdf:type owl:NamedIndividual ,
                                    foaf:Organization ;
                           foaf:name "Allotrope Foundation" .


###  http://purl.allotrope.org/voc/attribution
<http://purl.allotrope.org/voc/attribution> rdf:type owl:NamedIndividual ,
                                                     dct:RightsStatement ;
                                            dct:description """
These taxonomies contain material or may constitute derivative works of material which may be subject to copyright by one of the following organizations.  By using these taxonomies, you agree to the following terms and conditions applicable to its contents:
******************************************************************************
Copyright Notice and Terms for IUPAC Gold Book
______________________________________________________________________________
Copyright © 1998, Regents of the University of California
All rights reserved.
Redistribution and use in source and binary forms, with or without modification, are permitted provided that the following conditions are met:
1. Redistributions of source code must retain the above copyright notice, this list of conditions and the following disclaimer.
2. Redistributions in binary form must reproduce the above copyright notice, this list of conditions and the following disclaimer in the documentation and/or other materials provided with the distribution.
THIS SOFTWARE IS PROVIDED BY THE COPYRIGHT HOLDERS AND CONTRIBUTORS \"AS IS\" AND ANY EXPRESS OR IMPLIED WARRANTIES, INCLUDING, BUT NOT LIMITED TO, THE IMPLIED WARRANTIES OF MERCHANTABILITY AND FITNESS FOR A PARTICULAR PURPOSE ARE DISCLAIMED. IN NO EVENT SHALL THE COPYRIGHT HOLDER OR CONTRIBUTORS BE LIABLE FOR ANY DIRECT, INDIRECT, INCIDENTAL, SPECIAL, EXEMPLARY, OR CONSEQUENTIAL DAMAGES (INCLUDING, BUT NOT LIMITED TO, PROCUREMENT OF SUBSTITUTE GOODS OR SERVICES; LOSS OF USE, DATA, OR PROFITS; OR BUSINESS INTERRUPTION) HOWEVER CAUSED AND ON ANY THEORY OF LIABILITY, WHETHER IN CONTRACT, STRICT LIABILITY, OR TORT (INCLUDING NEGLIGENCE OR OTHERWISE) ARISING IN ANY WAY OUT OF THE USE OF THIS SOFTWARE, EVEN IF ADVISED OF THE POSSIBILITY OF SUCH DAMAGE.
******************************************************************************
Copyright Notice and Terms for PSI-MS (Proteomics Standards Initiative - Mass Spectrometry) Mass spectrometer output files and spectra interpretation
_____________________________________________________________________________
Created by Matt Chambers, Andreas Bertsch, Marius Kallhardt, Eric Deutsch Fredrik Levander, Pierre-Alain Binz, and Gerhard Mayer. Publisher: HUPO Proteomics Standards Initiative Mass Spectrometry Standards Working Group and HUPO Proteomics Standards Initiative Proteomics Informatics Working Group. This work is used pursuant to a Creative Commons license available here: http://creativecommons.org/licenses/by/3.0/legalcode

******************************************************************************
Attribution Notice for National Center for Biomedical Ontology materials.

This work contains material from the Cell Ontology and Clinical Measurement Ontology, available here: http://bioportal.bioontology.org/.
******************************************************************************
Attribution Notice for ChEBI
This work contains material from the European Bioinformatics Institute’s ChEBI database.
******************************************************************************
Attribution Notice for Quantities Units Dimensions Data Types (http://www.qudt.org/)
This work contains content from www.qudt.org and is used pursuant to a Creative Commons License available here: http://creativecommons.org/licenses/by-sa/3.0/us/legalcode. The original work may have been modified.
******************************************************************************
Copyright and Attribution Notice for Dublin Core Metadata Initiative Document
This work contains material from the following DCMI document used pursuant to a creative commons license available here: https://creativecommons.org/licenses/by/4.0/legalcode. This material may have been modified or changed.
Timestamped URL:          http://dublincore.org/documents/2012/06/14/dcmi-terms/
Date Issued:                       2012-06-14
Document Status:            This is a DCMI Recommendation.
Copyright © 1995-2015 DCMI. All Rights Reserved. DCMI liability, trademark/service mark, document use and software licensing rules apply.
******************************************************************************

""" ;
                                            dct:title "Derivative works attribution" .


###  http://purl.allotrope.org/voc/copyright
<http://purl.allotrope.org/voc/copyright> rdf:type owl:NamedIndividual ,
                                                   dct:RightsStatement ;
                                          dct:description "Copyright © 2021 Allotrope Foundation" ;
                                          dct:rightsHolder <http://www.allotrope.org> ;
                                          dct:title "Copyright © 2021 Allotrope Foundation" .


###  http://purl.allotrope.org/voc/creative-commons-attribution-license
<http://purl.allotrope.org/voc/creative-commons-attribution-license> rdf:type owl:NamedIndividual ,
                                                                              dct:LicenseDocument ;
                                                                     dct:description """This work is licensed under a Creative Commons Attribution 4.0 International License http://creativecommons.org/licenses/by/4.0/.

THESE MATERIALS ARE PROVIDED \"AS IS\" AND ALLOTROPE EXPRESSLY DISCLAIMS ALL WARRANTIES, EXPRESS, IMPLIED OR STATUTORY, INCLUDING, WITHOUT LIMITATION, THE WARRANTIES OF NON-INFRINGEMENT, TITLE, MERCHANTABILITY AND FITNESS FOR A PARTICULAR PURPOSE.

Copyright © 2015-2025 Allotrope Foundation
""" ;
                                                                     dct:title "Creative Commons Attribution 4.0 International Public License" .


###  Generated by the OWL API (version 5.1.19) https://github.com/owlcs/owlapi/
