<?xml version="1.0"?>
<rdf:RDF xmlns="http://www.w3id.org/animl/ontology/"
     xml:base="http://www.w3id.org/animl/ontology/"
     xmlns:aml="http://www.w3id.org/animl/ontology/"
     xmlns:cc="http://creativecommons.org/ns#"
     xmlns:dc="http://purl.org/dc/elements/1.1/"
     xmlns:owl="http://www.w3.org/2002/07/owl#"
     xmlns:rdf="http://www.w3.org/1999/02/22-rdf-syntax-ns#"
     xmlns:xml="http://www.w3.org/XML/1998/namespace"
     xmlns:xsd="http://www.w3.org/2001/XMLSchema#"
     xmlns:rdfs="http://www.w3.org/2000/01/rdf-schema#"
     xmlns:vann="http://purl.org/vocab/vann/"
     xmlns:terms="http://purl.org/dc/terms/">
    <owl:Ontology rdf:about="http://www.w3id.org/animl/ontology/">
        <owl:versionIRI rdf:resource="http://www.w3id.org/animl/ontology/1.0.0/"/>

        <owl:imports rdf:resource="http://www.ontologydesignpatterns.org/cp/owl/collectionentity.owl"/>
        <owl:imports rdf:resource="http://www.ontologydesignpatterns.org/cp/owl/sequence.owl"/>
        <owl:imports rdf:resource="http://www.ontologydesignpatterns.org/cp/owl/bag.owl"/>

        <cc:license rdf:resource="https://creativecommons.org/licenses/by/4.0/"/>
        <dc:license rdf:resource="https://creativecommons.org/licenses/by/4.0/"/>
        <terms:license rdf:resource="https://creativecommons.org/licenses/by/4.0/"/>

        <dc:creator xml:lang="en">Wilf Morlidge</dc:creator>
        <dc:creator xml:lang="en">Jacopo de Berardinis</dc:creator>
        <dc:creator xml:lang="en">Elliott Watkiss-Leek</dc:creator>
        <dc:creator xml:lang="en">George Hannah</dc:creator>
        <dc:creator xml:lang="en">Valentina Tamma</dc:creator>
        <dc:creator xml:lang="en">Harry Rostron</dc:creator>
        <dc:creator xml:lang="en">Andrew Ng</dc:creator>
        <dc:creator xml:lang="en">Ewan Johnson</dc:creator>
        <dc:creator xml:lang="en">Andrew Mitchell</dc:creator>
        <dc:creator xml:lang="en">Terry R. Payne</dc:creator>

        <dc:title xml:lang="en">The AnIML Ontology</dc:title>
        <rdfs:label xml:lang="en">The AnIML Ontology</rdfs:label>

        <dc:description xml:lang="en">The AnIML Ontology is a OWL-based model that formalises the semantics of the Analytical Information Markup Language (AnIML) and aligns it with the Allotrope Data Format to support cross-system and cross-lab interoperability.</dc:description>
        <rdfs:comment xml:lang="en">The AnIML Ontology is a OWL-based model that formalises the semantics of the Analytical Information Markup Language (AnIML) and aligns it with the Allotrope Data Format to support cross-system and cross-lab interoperability.</rdfs:comment>

        <owl:versionInfo xml:lang="en">1.0.0</owl:versionInfo>
        <terms:issued>2025-02-01</terms:issued>
        <terms:modified>2025-02-27</terms:modified>
        <vann:preferredNamespacePrefix>aml</vann:preferredNamespacePrefix>
        <vann:preferredNamespaceUri>http://www.w3id.org/animl/ontology/</vann:preferredNamespaceUri>
    </owl:Ontology>


    <!--animl_core-->


    <!-- 
    ///////////////////////////////////////////////////////////////////////////////////////
    //
    // Object Properties
    //
    ///////////////////////////////////////////////////////////////////////////////////////
     -->


    <!-- this denotes the property of an object having a governing specification -->

    <owl:ObjectProperty rdf:about="http://www.w3id.org/animl/ontology/hasSpecification">
    <rdfs:comment xml:lang="en">This denotes the property of an object having a governing specification</rdfs:comment>
    <rdfs:domain>
        <owl:Class>
            <owl:unionOf rdf:parseType="Collection">
                <rdf:Description rdf:about="http://www.w3id.org/animl/ontology/Reference"/>
                <rdf:Description rdf:about="http://www.w3id.org/animl/ontology/UseCase"/>
                <rdf:Description rdf:about="http://www.w3id.org/animl/ontology/Category"/>
                <rdf:Description rdf:about="http://www.w3id.org/animl/ontology/Parameter"/>
                <rdf:Description rdf:about="http://www.w3id.org/animl/ontology/SeriesSet"/>
                <rdf:Description rdf:about="http://www.w3id.org/animl/ontology/ExperimentStep"/>
                <rdf:Description rdf:about="http://www.w3id.org/animl/ontology/Method"/>
                <rdf:Description rdf:about="http://www.w3id.org/animl/ontology/Result"/>
                <rdf:Description rdf:about="http://www.w3id.org/animl/ontology/Series"/>
                <rdf:Description rdf:about="http://www.w3id.org/animl/ontology/DataPoint"/>
                <rdf:Description rdf:about="http://www.w3id.org/animl/ontology/SeriesSpecification"/>
            </owl:unionOf>
        </owl:Class>
    </rdfs:domain>

    <rdfs:range>
        <owl:Class>
            <owl:unionOf rdf:parseType="Collection">
                <rdf:Description rdf:about="http://www.w3id.org/animl/ontology/ItemSpecification"/>
                <rdf:Description rdf:about="http://www.w3id.org/animl/ontology/ParameterSpecification"/>
                <rdf:Description rdf:about="http://www.w3id.org/animl/ontology/ReferenceSpecification"/>
                <rdf:Description rdf:about="http://www.w3id.org/animl/ontology/SeriesSpecification"/>
                <rdf:Description rdf:about="http://www.w3id.org/animl/ontology/DataPointSpecification"/>
            </owl:unionOf>
        </owl:Class>
    </rdfs:range>
    </owl:ObjectProperty>
    
    <!-- this is the inverse of the above property which denotes that a specification is used by an object -->

    <owl:ObjectProperty rdf:about="http://www.w3id.org/animl/ontology/usedBy">
        <rdfs:comment xml:lang="en">The inverse of the specification property which denotes that a specification is used by an object</rdfs:comment>
        <rdfs:domain>
            <owl:Class>
                <owl:unionOf rdf:parseType="Collection">
                    <rdf:Description rdf:about="http://www.w3id.org/animl/ontology/ItemSpecification"/>
                    <rdf:Description rdf:about="http://www.w3id.org/animl/ontology/ParameterSpecification"/>
                    <rdf:Description rdf:about="http://www.w3id.org/animl/ontology/ReferenceSpecification"/>
                    <rdf:Description rdf:about="http://www.w3id.org/animl/ontology/SeriesSpecification"/>
                    <rdf:Description rdf:about="http://www.w3id.org/animl/ontology/DataPointSpecification"/>
                </owl:unionOf>
            </owl:Class>
        </rdfs:domain>

        <rdfs:range>
            <owl:Class>
                <owl:unionOf rdf:parseType="Collection">
                    <rdf:Description rdf:about="http://www.w3id.org/animl/ontology/Reference"/>
                    <rdf:Description rdf:about="http://www.w3id.org/animl/ontology/Role"/>
                    <rdf:Description rdf:about="http://www.w3id.org/animl/ontology/Category"/>
                    <rdf:Description rdf:about="http://www.w3id.org/animl/ontology/Parameter"/>
                    <rdf:Description rdf:about="http://www.w3id.org/animl/ontology/SeriesSet"/>
                    <rdf:Description rdf:about="http://www.w3id.org/animl/ontology/ExperimentStep"/>
                    <rdf:Description rdf:about="http://www.w3id.org/animl/ontology/Method"/>
                    <rdf:Description rdf:about="http://www.w3id.org/animl/ontology/Result"/>
                    <rdf:Description rdf:about="http://www.w3id.org/animl/ontology/Series"/>
                    <rdf:Description rdf:about="http://www.w3id.org/animl/ontology/DataPoint"/>
                    <rdf:Description rdf:about="http://www.w3id.org/animl/ontology/SeriesSpecification"/>
                </owl:unionOf>
            </owl:Class>
        </rdfs:range>
    </owl:ObjectProperty>





    <!-- this is a reified data property denoting that the domain (which is conceptually a component of a series determined before the series
    is created) has a plotscale, which itself is a class of individuals equivalent to the possible settings of the reified data property -->
    <owl:ObjectProperty rdf:about="http://www.w3id.org/animl/ontology/hasPlotScale">
        <rdfs:comment xml:lang="en">A reified data property denoting that the domain (which is conceptually a component of a series determined before the series is created) has a plotscale, which itself is a class of individuals equivalent to the possible settings of the reified data property</rdfs:comment>
        <rdfs:domain rdf:resource="http://www.w3id.org/animl/ontology/SeriesSpecification"/>
        <rdfs:range rdf:resource="http://www.w3id.org/animl/ontology/PlotScale"/>
    </owl:ObjectProperty>

    <!-- this is a reified property for the concept of a role being fulfilled by an agent, in english the concept of a task / job being done by someone-->
    
    <owl:ObjectProperty rdf:about="http://www.ontologydesignpatterns.org/cp/owl/bag.owl#isRoleOf">
        <rdfs:comment xml:lang="en">A reified property for the concept of a role being fulfilled by an agent, in english the concept of a task / job being done by someone</rdfs:comment>
        <rdfs:domain rdf:resource="http://www.w3id.org/animl/ontology/Role"/>
        <rdfs:range rdf:resource="http://www.w3id.org/animl/ontology/Agent"/>
    </owl:ObjectProperty>

    <!-- this is almost the inverse of the above, however it carries the connotation that the agent becomes defined by their task
    this is in the same way that if a human practices medicine to fulfill a need for medical treatment, then that need becomes met,
    however it also makes the human a doctor.-->

    <owl:ObjectProperty rdf:about="http://www.w3id.org/animl/ontology/isClassifiedBy">
        <rdfs:comment xml:lang="en">This is the inverse of the bag association, however it carries the connotation that the agent becomes defined by their task. This is in the same way that if a human practices medicine to fulfill a need for medical treatment, then that need becomes met, however it also makes the human a doctor.</rdfs:comment>
        <rdfs:domain rdf:resource="http://www.w3id.org/animl/ontology/Agent"/>
        <rdfs:range rdf:resource="http://www.w3id.org/animl/ontology/Role"/>
    </owl:ObjectProperty>


    <!-- this is an implementation of the common 'hasPart' realtion to denote the special relation between series and datapoint specifications,
    wherein series specifications govern some of the attributes of their corresponding dataPointSpecifications-->
    
    <owl:ObjectProperty rdf:about="http://www.w3id.org/animl/ontology/hasPart">
        <rdfs:comment xml:lang="en">An implementation of the common 'hasPart' realtion to denote the special relation between series and datapoint specifications, wherein series specifications govern some of the attributes of their corresponding dataPointSpecifications</rdfs:comment>
        <rdfs:domain rdf:resource="http://www.w3id.org/animl/ontology/SeriesSpecification"/>
        <rdfs:range rdf:resource="http://www.w3id.org/animl/ontology/DataPointSpecification"/>
    </owl:ObjectProperty>

    <owl:ObjectProperty rdf:about="http://www.w3id.org/animl/ontology/isPartOf">
        <rdfs:domain rdf:resource="http://www.w3id.org/animl/ontology/DataPointSpecification"/>
        <rdfs:range rdf:resource="http://www.w3id.org/animl/ontology/SeriesSpecification"/>
    </owl:ObjectProperty>





    <!-- this relationship indicates the object, conceptually the area of the animl document describing that object, that a change has been made to -->

    <owl:ObjectProperty rdf:about="http://www.w3id.org/animl/ontology/affects">
        <rdfs:comment xml:lang="en">This relationship indicates the object, conceptually the area of the animl document describing that object, that a change has been made to</rdfs:comment>
        <rdfs:domain rdf:resource="http://www.w3id.org/animl/ontology/Change"/>
        <rdfs:range rdf:resource="http://www.w3.org/2002/07/owl#Thing"/>
    </owl:ObjectProperty>
    


    <!-- this relationship shows that an animl document contains all the information regarding (e.i denotes) a particular experiment -->

    <owl:ObjectProperty rdf:about="http://www.w3id.org/animl/ontology/denotes">
        <rdfs:comment xml:lang="en">This relationship shows that an animl document contains all the information regarding (e.i denotes) a particular experiment</rdfs:comment>
        <rdfs:domain rdf:resource="http://www.w3id.org/animl/ontology/Document"/>
        <rdfs:range rdf:resource="http://www.w3id.org/animl/ontology/Experiment"/>
    </owl:ObjectProperty>


    <!-- this is the inverse of the above relation  -->

    <owl:ObjectProperty rdf:about="http://www.w3id.org/animl/ontology/denotedBy">
        <rdfs:comment xml:lang="en">This is the inverse of the denotes relation</rdfs:comment>
        <rdfs:domain rdf:resource="http://www.w3id.org/animl/ontology/Experiment"/>
        <rdfs:range rdf:resource="http://www.w3id.org/animl/ontology/Document"/>
    </owl:ObjectProperty>
    

    <!-- this property denotes that an object of a class has a role associated with it, this generalises asociations to several classes
    of objects that are now generalised as role -->

    <owl:ObjectProperty rdf:about="http://www.w3id.org/animl/ontology/requiresRole">
        <rdfs:comment xml:lang="en">This property denotes that an object of a class has a role associated with it, this generalises asociations to several classes of objects that are now generalised as role</rdfs:comment>
        <rdfs:domain>
            <owl:Class>
                <owl:unionOf rdf:parseType="Collection">
                    <rdf:Description rdf:about="http://www.w3id.org/animl/ontology/Method"/>
                    <rdf:Description rdf:about="http://www.w3id.org/animl/ontology/AuditTrailEntry"/>
                </owl:unionOf>
            </owl:Class>
        </rdfs:domain>
        <rdfs:range rdf:resource="http://www.w3id.org/animl/ontology/Role"/>
    </owl:ObjectProperty>
    

    


    <!-- this denotes that a category includes a parameter -->

    <owl:ObjectProperty rdf:about="http://www.w3id.org/animl/ontology/hasParameter">
        <rdfs:comment xml:lang="en">This denotes that a category includes a parameter</rdfs:comment>
        <rdfs:domain rdf:resource="http://www.w3id.org/animl/ontology/Category"/>
        <rdfs:range rdf:resource="http://www.w3id.org/animl/ontology/Parameter"/>
    </owl:ObjectProperty>


    <!-- this denotes the relationship between a result and a category -->

    <owl:ObjectProperty rdf:about="http://www.w3id.org/animl/ontology/hasResultCategory">
        <rdfs:comment xml:lang="en">This denotes the relationship between a result and a category</rdfs:comment>
        <rdfs:domain rdf:resource="http://www.w3id.org/animl/ontology/Result"/>
        <rdfs:range rdf:resource="http://www.w3id.org/animl/ontology/Category"/>
    </owl:ObjectProperty>
    


    <!-- this denotes the relationship between a sample and a category -->

    <owl:ObjectProperty rdf:about="http://www.w3id.org/animl/ontology/hasSampleCategory">
        <rdfs:comment xml:lang="en">This denotes the relationship between a sample and a category</rdfs:comment>
        <rdfs:domain rdf:resource="http://www.w3id.org/animl/ontology/Sample"/>
        <rdfs:range rdf:resource="http://www.w3id.org/animl/ontology/Category"/>
    </owl:ObjectProperty>
    


    <!-- this denotes the inclusion of a set of samples in a document, they are attached to the doucment as samples exist outside of the  -->

    <owl:ObjectProperty rdf:about="http://www.w3id.org/animl/ontology/hasSampleSet">
        <rdfs:comment xml:lang="en">This denotes the inclusion of a set of samples in a document, they are attached to the doucment as samples exist outside of the</rdfs:comment>
        <rdfs:domain rdf:resource="http://www.w3id.org/animl/ontology/Document"/>
        <rdfs:range rdf:resource="http://www.w3id.org/animl/ontology/SampleSet"/>
    </owl:ObjectProperty>



    <!-- this denotes the relationship of a category object with another of the same class,
     where the information of one category may be a component of another broader one -->

    <owl:ObjectProperty rdf:about="http://www.w3id.org/animl/ontology/hasSubCategory">
        <rdfs:comment xml:lang="en">This denotes the relationship of a category object with another of the same class, where the information of one category may be a component of another broader one</rdfs:comment>
        <rdfs:domain rdf:resource="http://www.w3id.org/animl/ontology/Category"/>
        <rdfs:range rdf:resource="http://www.w3id.org/animl/ontology/Category"/>
    </owl:ObjectProperty>
    


    <!-- this denotes the property of have tags attached to you, as well as specifying the set of tags for which this is true -->

    <owl:ObjectProperty rdf:about="http://www.w3id.org/animl/ontology/hasTags">
        <rdfs:comment xml:lang="en">This denotes the property of have tags attached to you, as well as specifying the set of tags for which this is true</rdfs:comment>
        <rdfs:domain>
            <owl:Class>
                <owl:unionOf rdf:parseType="Collection">
                    <rdf:Description rdf:about="http://www.w3id.org/animl/ontology/Sample"/>
                    <rdf:Description rdf:about="http://www.w3id.org/animl/ontology/ExperimentStep"/>
                </owl:unionOf>
            </owl:Class>
        </rdfs:domain>
        <rdfs:range rdf:resource="http://www.w3id.org/animl/ontology/TagSet"/>
    </owl:ObjectProperty>
    


    <!-- this is distinct from the concept of data type
    
    where a classes equivalent in the animl xml was bound by an attribute to one of a set of enumerated types,
    we have reified that attribute and created type classes whose individuals are the possible settings of type for the relevant class.
    
    this relationship is the relation between a class and its type class -->

    <owl:ObjectProperty rdf:about="http://www.w3id.org/animl/ontology/hasType">
        <rdfs:comment xml:lang="en">This is distinct from the concept of data type where a classes equivalent in the animl xml was bound by an attribute to one of a set of enumerated types, we have reified that attribute and created type classes whose individuals are the possible settings of type for the relevant class. this relationship is the relation between a class and its type class</rdfs:comment>
        <rdfs:domain>
            <owl:Class>
                <owl:unionOf rdf:parseType="Collection">
                    <rdf:Description rdf:about="http://www.w3id.org/animl/ontology/Container"/>
                    <rdf:Description rdf:about="http://www.w3id.org/animl/ontology/Agent"/>
                    <rdf:Description rdf:about="http://www.w3id.org/animl/ontology/Change"/>
                    <rdf:Description rdf:about="http://www.w3id.org/animl/ontology/DataPoint"/>
                </owl:unionOf>
            </owl:Class>
        </rdfs:domain>
        <rdfs:range>
            <owl:Class>
                <owl:unionOf rdf:parseType="Collection">
                    <rdf:Description rdf:about="http://www.w3id.org/animl/ontology/ContainerType"/>
                    <rdf:Description rdf:about="http://www.w3id.org/animl/ontology/AgentType"/>
                    <rdf:Description rdf:about="http://www.w3id.org/animl/ontology/ChangeType"/>
                    <rdf:Description rdf:about="http://www.w3id.org/animl/ontology/DataPointType"/>
                </owl:unionOf>
            </owl:Class>
        </rdfs:range>
    </owl:ObjectProperty>
    


    <!-- this is the property linking a document to its version history -->

    <owl:ObjectProperty rdf:about="http://www.w3id.org/animl/ontology/hasAuditTrail">
        <rdfs:comment xml:lang="en">This is the property linking a document and agents to their version history</rdfs:comment>
        <rdfs:domain>
            <owl:Class>
                <owl:unionOf rdf:parseType="Collection">
                    <rdf:Description rdf:about="http://www.w3id.org/animl/ontology/Document"/>
                    <rdf:Description rdf:about="http://www.w3id.org/animl/ontology/Agent"/>
                </owl:unionOf>
            </owl:Class>
        </rdfs:domain>
        <rdfs:range rdf:resource="http://www.w3id.org/animl/ontology/AuditTrail"/>
    </owl:ObjectProperty>

    <owl:ObjectProperty rdf:about="http://www.w3id.org/animl/ontology/hasAuditTrailEntry">
        <rdfs:domain rdf:resource="http://www.w3id.org/animl/ontology/AuditTrail"/>
        <rdfs:range rdf:resource="http://www.w3id.org/animl/ontology/AuditTrailEntry"/>
    </owl:ObjectProperty>
    
    <!-- this property is designed to link an experiment step to is associated infrastructure -->

    <owl:ObjectProperty rdf:about="http://www.w3id.org/animl/ontology/includesInfrastructure">
        <rdfs:comment xml:lang="en">This property is designed to link an experiment step to is associated infrastructure</rdfs:comment>
        <rdfs:domain rdf:resource="http://www.w3id.org/animl/ontology/ExperimentStep"/>
        <rdfs:range rdf:resource="http://www.w3id.org/animl/ontology/Infrastructure"/>
    </owl:ObjectProperty>
    


    <!-- this property does not make complete sense at a human level
    it ties a sample into the sampleincontainer situation since a sample in that situation has the property of being contained
     -->

    <owl:ObjectProperty rdf:about="http://www.w3id.org/animl/ontology/isContained">
        <rdfs:comment xml:lang="en">This property does not make complete sense at a human level it ties a sample into the sampleincontainer situation since a sample in that situation has the property of being contained</rdfs:comment>
        <rdfs:domain rdf:resource="http://www.w3id.org/animl/ontology/Sample"/>
        <rdfs:range rdf:resource="http://www.w3id.org/animl/ontology/SampleInContainer"/>
    </owl:ObjectProperty>
    


    <!-- this is not the inverse of the above property, it links a sampleIncontainer situation to a container as the object
    doing the containing within the situation -->

    <owl:ObjectProperty rdf:about="http://www.w3id.org/animl/ontology/isContainedBy">
        <rdfs:comment xml:lang="en">This is not the inverse of the above property, it links a sampleIncontainer situation to a container as the object doing the containing within the situation</rdfs:comment>
        <rdfs:domain rdf:resource="http://www.w3id.org/animl/ontology/SampleInContainer"/>
        <rdfs:range rdf:resource="http://www.w3id.org/animl/ontology/Container"/>
    </owl:ObjectProperty>

    <!-- this relation indicates that it is at a particular version that a change is made -->

    <owl:ObjectProperty rdf:about="http://www.w3id.org/animl/ontology/makesChange">
        <rdfs:comment xml:lang="en">This relation indicates that it is at a particular version that a change is made</rdfs:comment>
        <rdfs:domain rdf:resource="http://www.w3id.org/animl/ontology/AuditTrailEntry"/>
        <rdfs:range rdf:resource="http://www.w3id.org/animl/ontology/Change"/>
    </owl:ObjectProperty>
    


    <!-- this relation is to link an experimentStep to its results, and also to indicate that said results are created in the step -->

    <owl:ObjectProperty rdf:about="http://www.w3id.org/animl/ontology/producesResult">
        <rdfs:comment xml:lang="en">This relation is to link an experimentStep to its results, and also to indicate that said results are created in the step</rdfs:comment>
        <rdfs:domain rdf:resource="http://www.w3id.org/animl/ontology/ExperimentStep"/>
        <rdfs:range rdf:resource="http://www.w3id.org/animl/ontology/Result"/>
    </owl:ObjectProperty>
    


    <!-- this relation links a signature to the signableitem, conceptually an area of the animl file (or one of the files it represents),
    it is attached it. it also indicates that the given signable item is watermarked by the signature-->

    <owl:ObjectProperty rdf:about="http://www.w3id.org/animl/ontology/marks">
        <rdfs:comment xml:lang="en">This relation links a signature to the signableitem, conceptually an area of the animl file (or one of the files it represents), it is attached it. it also indicates that the given signable item is watermarked by the signature</rdfs:comment>
        <rdfs:domain rdf:resource="http://www.w3id.org/animl/ontology/Signature"/>
        <rdfs:range rdf:resource="http://www.w3.org/2002/07/owl#Thing"/>
    </owl:ObjectProperty>
    


    <!-- this denotes the inclusion of a method in an experiment step, and also indicates that a method is something that is utilised
    in an exmperiment step rather than being part of it -->

    <owl:ObjectProperty rdf:about="http://www.w3id.org/animl/ontology/usesMethod">
        <rdfs:comment xml:lang="en">This denotes the inclusion of a method in an experiment step, and also indicates that a method is something that is utilised in an exmperiment step rather than being part of it</rdfs:comment>
        <rdfs:domain rdf:resource="http://www.w3id.org/animl/ontology/ExperimentStep"/>
        <rdfs:range rdf:resource="http://www.w3id.org/animl/ontology/Method"/>
    </owl:ObjectProperty>


    <!-- this denotes the inclusion of a technique in an experiment step, and also indicates that a technique is something that is utilised
    in an exmperiment step rather than being part of it -->

    <owl:ObjectProperty rdf:about="http://www.w3id.org/animl/ontology/usesTechnique">
        <rdfs:comment xml:lang="en">This denotes the inclusion of a technique in an experiment step, and also indicates that a technique is something that is utilised in an exmperiment step rather than being part of it</rdfs:comment>
        <rdfs:domain rdf:resource="http://www.w3id.org/animl/ontology/ExperimentStep"/>
        <rdfs:range rdf:resource="http://www.w3id.org/animl/ontology/Technique"/>
    </owl:ObjectProperty>

    <!-- this represents the idea of an object containing an object, without having neccessary parthood-->

    <owl:ObjectProperty rdf:about="http://www.w3id.org/animl/ontology/includes">
        <rdfs:comment xml:lang="en">This represents the idea of an object containing an object, without having neccessary parthood</rdfs:comment>
        <rdfs:domain>
            <owl:Class>
                <owl:unionOf rdf:parseType="Collection">
                    <rdf:Description rdf:about="http://www.w3id.org/animl/ontology/Infrastructure"/>
                    <rdf:Description rdf:about="http://www.w3id.org/animl/ontology/Result"/>
                </owl:unionOf>
            </owl:Class>
        </rdfs:domain>
        <rdfs:range rdf:resource="http://www.w3id.org/animl/ontology/ReferenceSet"/>
    </owl:ObjectProperty>
    
    <!-- 
    ///////////////////////////////////////////////////////////////////////////////////////
    //
    // Data properties
    //
    ///////////////////////////////////////////////////////////////////////////////////////
     -->



    <!-- this is used to indicate effects an attribute, or an entire element -->

    <owl:DatatypeProperty rdf:about="http://www.w3id.org/animl/ontology/scope">
        <rdfs:comment xml:lang="en">This is used to indicate effects an attribute, or an entire element</rdfs:comment>
        <rdfs:subPropertyOf rdf:resource="http://www.w3.org/2002/07/owl#topDataProperty"/>
        <rdfs:domain rdf:resource="http://www.w3id.org/animl/ontology/Change"/>
        <rdfs:range rdf:resource="http://www.w3.org/2001/XMLSchema#string"/>
    </owl:DatatypeProperty>
    


    <!-- this is used to indicate which version of the animl markup language was used to create the document -->

    <owl:DatatypeProperty rdf:about="http://www.w3id.org/animl/ontology/animlVersion">
        <rdfs:comment xml:lang="en">This is used to indicate which version of the animl markup language was used to create the document</rdfs:comment>
        <rdfs:subPropertyOf rdf:resource="http://www.w3.org/2002/07/owl#topDataProperty"/>
        <rdfs:domain rdf:resource="http://www.w3id.org/animl/ontology/Document"/>
        <rdfs:range rdf:resource="http://www.w3.org/2001/XMLSchema#string"/>
    </owl:DatatypeProperty>
    


    <!-- this is used to store the characters underlying the barcode for a sample -->

    <owl:DatatypeProperty rdf:about="http://www.w3id.org/animl/ontology/barcode">
        <rdfs:comment xml:lang="en">This is used to store the characters underlying the barcode for a sample</rdfs:comment>
        <rdfs:subPropertyOf rdf:resource="http://www.w3.org/2002/07/owl#topDataProperty"/>
        <rdfs:domain rdf:resource="http://www.w3id.org/animl/ontology/Sample"/>
        <rdfs:range rdf:resource="http://www.w3.org/2001/XMLSchema#string"/>
    </owl:DatatypeProperty>
    

 <!-- this exists to enable human readable comments to be attached to all objects in the ontology -->

    <owl:DatatypeProperty rdf:about="http://www.w3id.org/animl/ontology/comment">
        <rdfs:comment xml:lang="en">This exists to enable human readable comments to be attached to all objects in the ontology</rdfs:comment>
        <rdfs:subPropertyOf rdf:resource="http://www.w3.org/2002/07/owl#topDataProperty"/>
        <rdfs:domain rdf:resource="http://www.w3.org/2002/07/owl#Thing"/>
        <rdfs:range rdf:resource="http://www.w3.org/2001/XMLSchema#string"/>
    </owl:DatatypeProperty>
    


    <!-- this expresses the Id which a container is given to allow it be found in a group of containers -->

    <owl:DatatypeProperty rdf:about="http://www.w3id.org/animl/ontology/containerId">
        <rdfs:comment xml:lang="en">This expresses the Id which a container is given to allow it be found in a group of containers</rdfs:comment>
        <rdfs:subPropertyOf rdf:resource="http://www.w3.org/2002/07/owl#topDataProperty"/>
        <rdfs:domain rdf:resource="http://www.w3id.org/animl/ontology/Container"/>
        <rdfs:range rdf:resource="http://www.w3.org/2001/XMLSchema#string"/>
    </owl:DatatypeProperty>
    


    <!-- this represents the row position of a sample in a container, within the reified sampleInContainer situation -->

    <owl:DatatypeProperty rdf:about="http://www.w3id.org/animl/ontology/containerRow">
        <rdfs:comment xml:lang="en">This represents the row position of a sample in a container, within the reified sampleInContainer situation</rdfs:comment>
        <rdfs:subPropertyOf rdf:resource="http://www.w3.org/2002/07/owl#topDataProperty"/>
        <rdfs:domain rdf:resource="http://www.w3id.org/animl/ontology/SampleInContainer"/>
        <rdfs:range rdf:resource="http://www.w3.org/2001/XMLSchema#int"/>
    </owl:DatatypeProperty>
    


    <!-- this represents the column position of a sample in a container, within the reified sampleInContainer situation -->

    <owl:DatatypeProperty rdf:about="http://www.w3id.org/animl/ontology/containmentColumn">
        <rdfs:comment xml:lang="en">This represents the column position of a sample in a container, within the reified sampleInContainer situation</rdfs:comment>
        <rdfs:subPropertyOf rdf:resource="http://www.w3.org/2002/07/owl#topDataProperty"/>
        <rdfs:domain rdf:resource="http://www.w3id.org/animl/ontology/SampleInContainer"/>
        <rdfs:range rdf:resource="http://www.w3.org/2001/XMLSchema#int"/>
    </owl:DatatypeProperty>
    


    <!-- this represents the email address of an agent -->

    <owl:DatatypeProperty rdf:about="http://www.w3id.org/animl/ontology/email">
        <rdfs:comment xml:lang="en">This represents the email address of an agent</rdfs:comment>
        <rdfs:subPropertyOf rdf:resource="http://www.w3.org/2002/07/owl#topDataProperty"/>
        <rdfs:domain rdf:resource="http://www.w3id.org/animl/ontology/Agent"/>
        <rdfs:range rdf:resource="http://www.w3.org/2001/XMLSchema#string"/>
    </owl:DatatypeProperty>


    <!-- this is any machine readable code not assigned within the system, for example if an agent has an employee number -->

    <owl:DatatypeProperty rdf:about="http://www.w3id.org/animl/ontology/identifier">
        <rdfs:comment xml:lang="en">This is any machine readable code not assigned within the system, for example if an agent has an employee number</rdfs:comment>
        <rdfs:subPropertyOf rdf:resource="http://www.w3.org/2002/07/owl#topDataProperty"/>
        <rdfs:domain rdf:resource="http://www.w3id.org/animl/ontology/Agent"/>
        <rdfs:range rdf:resource="http://www.w3.org/2001/XMLSchema#string"/>
    </owl:DatatypeProperty>
    
    <!-- this represents a human readable physical location (typically an address, site number, or building space ref) for an agent -->

    <owl:DatatypeProperty rdf:about="http://www.w3id.org/animl/ontology/location">
        <rdfs:comment xml:lang="en">This represents a human readable physical location (typically an address, site number, or building space ref) for an agent</rdfs:comment>
        <rdfs:subPropertyOf rdf:resource="http://www.w3.org/2002/07/owl#topDataProperty"/>
        <rdfs:domain rdf:resource="http://www.w3id.org/animl/ontology/Agent"/>
        <rdfs:range rdf:resource="http://www.w3.org/2001/XMLSchema#string"/>
    </owl:DatatypeProperty>
    


    <!-- this is a generalisation of name,model, etc meaning the human understood identifier for something  -->

    <owl:DatatypeProperty rdf:about="http://www.w3id.org/animl/ontology/name">
        <rdfs:comment xml:lang="en">This is a generalisation of name,model, etc meaning the human understood identifier for something</rdfs:comment>
        <rdfs:subPropertyOf rdf:resource="http://www.w3.org/2002/07/owl#topDataProperty"/>
        <rdfs:domain>
            <owl:Class>
                <owl:unionOf rdf:parseType="Collection">
                    <rdf:Description rdf:about="http://www.w3id.org/animl/ontology/Agent"/>
                    <rdf:Description rdf:about="http://www.w3id.org/animl/ontology/ItemSpecification"/>
                    <rdf:Description rdf:about="http://www.w3id.org/animl/ontology/Tag"/>
                    <rdf:Description rdf:about="http://www.w3id.org/animl/ontology/Template"/>
                </owl:unionOf>
            </owl:Class>
        </rdfs:domain>
        <rdfs:range rdf:resource="http://www.w3.org/2001/XMLSchema#string"/>
    </owl:DatatypeProperty>
    


    <!-- this represents as a string literal the post change state of an item changed in a change -->

    <owl:DatatypeProperty rdf:about="http://www.w3id.org/animl/ontology/newValue">
        <rdfs:comment xml:lang="en">This represents as a string literal the post change state of an item changed in a change</rdfs:comment>
        <rdfs:subPropertyOf rdf:resource="http://www.w3.org/2002/07/owl#topDataProperty"/>
        <rdfs:domain rdf:resource="http://www.w3id.org/animl/ontology/Change"/>
        <rdfs:range rdf:resource="http://www.w3.org/2001/XMLSchema#string"/>
    </owl:DatatypeProperty>
    


    <!-- this represents as a string literal the per change state of an item changed in a change -->

    <owl:DatatypeProperty rdf:about="http://www.w3id.org/animl/ontology/oldValue">
        <rdfs:comment xml:lang="en">This represents as a string literal the per change state of an item changed in a change</rdfs:comment>
        <rdfs:subPropertyOf rdf:resource="http://www.w3.org/2002/07/owl#topDataProperty"/>
        <rdfs:domain rdf:resource="http://www.w3id.org/animl/ontology/Change"/>
        <rdfs:range rdf:resource="http://www.w3.org/2001/XMLSchema#string"/>
    </owl:DatatypeProperty>
    


    <!-- this is an optional property recording the operating system of an agent, where an agent is human, or
    a piece of mechanical hardware this value will be none. -->

    <owl:DatatypeProperty rdf:about="http://www.w3id.org/animl/ontology/operatingSystem">
        <rdfs:comment xml:lang="en">This is an optional property recording the operating system of an agent, where an agent is human, or a piece of mechanical hardware this value will be none.</rdfs:comment>
        <rdfs:subPropertyOf rdf:resource="http://www.w3.org/2002/07/owl#topDataProperty"/>
        <rdfs:domain rdf:resource="http://www.w3id.org/animl/ontology/Agent"/>
        <rdfs:range rdf:resource="http://www.w3.org/2001/XMLSchema#string"/>
    </owl:DatatypeProperty>
    


    <!-- this denotes the organisation to which an agent belongs, this can be the employer of a human agent
    , or the owner of a non human agent. -->

    <owl:DatatypeProperty rdf:about="http://www.w3id.org/animl/ontology/organisation">
        <rdfs:comment xml:lang="en">This denotes the organisation to which an agent belongs, this can be the employer of a human agent, or the owner of a non human agent.</rdfs:comment>
        <rdfs:subPropertyOf rdf:resource="http://www.w3.org/2002/07/owl#topDataProperty"/>
        <rdfs:domain rdf:resource="http://www.w3id.org/animl/ontology/Agent"/>
        <rdfs:range rdf:resource="http://www.w3.org/2001/XMLSchema#string"/>
    </owl:DatatypeProperty>
    


    <!-- this is an optional property denoting the phone number of an agent, where the agent is not human this will be none -->

    <owl:DatatypeProperty rdf:about="http://www.w3id.org/animl/ontology/phone">
        <rdfs:comment xml:lang="en">This is an optional property denoting the phone number of an agent, where the agent is not human this will be none</rdfs:comment>
        <rdfs:subPropertyOf rdf:resource="http://www.w3.org/2002/07/owl#topDataProperty"/>
        <rdfs:domain rdf:resource="http://www.w3id.org/animl/ontology/Agent"/>
        <rdfs:range rdf:resource="http://www.w3.org/2001/XMLSchema#string"/>
    </owl:DatatypeProperty>
    


    <!-- this property represents the actual data corresponding to a datapoint object of the individual sub class -->

    <owl:DatatypeProperty rdf:about="http://www.w3id.org/animl/ontology/pointValue">
        <rdfs:comment xml:lang="en">This property represents the actual data corresponding to a datapoint object of the individual sub class</rdfs:comment>
        <rdfs:domain>
            <owl:Class>
                <owl:unionOf rdf:parseType="Collection">
                    <rdf:Description rdf:about="http://www.w3id.org/animl/ontology/Parameter"/>
                    <rdf:Description rdf:about="http://www.w3id.org/animl/ontology/DataPoint"/>
                </owl:unionOf>
            </owl:Class>
        </rdfs:domain>
        <rdfs:subPropertyOf rdf:resource="http://www.w3.org/2002/07/owl#topDataProperty"/>
        <rdfs:domain>
            <owl:Class>
                <owl:unionOf rdf:parseType="Collection">
                    <rdf:Description rdf:about="http://www.w3id.org/animl/ontology/Parameter"/>
                    <rdf:Description rdf:about="http://www.w3id.org/animl/ontology/DataPoint"/>
                </owl:unionOf>
            </owl:Class>
        </rdfs:domain>
        <rdfs:range rdf:resource="http://www.w3.org/2001/XMLSchema#anysimpletype"/>
    </owl:DatatypeProperty>


    <!-- this is a natural language description justifying a change  -->

    <owl:DatatypeProperty rdf:about="http://www.w3id.org/animl/ontology/reason">
        <rdfs:comment xml:lang="en">This is a natural language description justifying a change</rdfs:comment>
        <rdfs:subPropertyOf rdf:resource="http://www.w3.org/2002/07/owl#topDataProperty"/>
        <rdfs:domain rdf:resource="http://www.w3id.org/animl/ontology/AuditTrail"/>
        <rdfs:range rdf:resource="http://www.w3.org/2001/XMLSchema#string"/>
    </owl:DatatypeProperty>
    
    
    <!-- this is an optional parameter which points outside of the file to the location of storage for the raw data that was later
    translated into a sample or experimentStep -->

    <owl:DatatypeProperty rdf:about="http://www.w3id.org/animl/ontology/sourceDataLocation">
        <rdfs:comment xml:lang="en">This is an optional parameter which points outside of the file to the location of storage for the raw data that was later translated into a sample or experimentStep</rdfs:comment>
        <rdfs:subPropertyOf rdf:resource="http://www.w3.org/2002/07/owl#topDataProperty"/>
        <rdfs:domain>
            <owl:Class>
                <owl:unionOf rdf:parseType="Collection">
                    <rdf:Description rdf:about="http://www.w3id.org/animl/ontology/Sample"/>
                    <rdf:Description rdf:about="http://www.w3id.org/animl/ontology/ExperimentStep"/>
                </owl:unionOf>
            </owl:Class>
        </rdfs:domain>
        <rdfs:range rdf:resource="http://www.w3.org/2001/XMLSchema#string"/>
    </owl:DatatypeProperty>
    
    <!-- this is a dataTime indicating the exact point in time at which an object was created -->

    <owl:DatatypeProperty rdf:about="http://www.w3id.org/animl/ontology/timeStamp">
        <rdfs:comment xml:lang="en">This is a dataTime indicating the exact point in time at which an object was created</rdfs:comment>
        <rdfs:subPropertyOf rdf:resource="http://www.w3.org/2002/07/owl#topDataProperty"/>
        <rdfs:domain>
            <owl:Class>
                <owl:unionOf rdf:parseType="Collection">
                    <rdf:Description rdf:about="http://www.w3id.org/animl/ontology/Infrastructure"/>
                    <rdf:Description rdf:about="http://www.w3id.org/animl/ontology/AuditTrail"/>
                </owl:unionOf>
            </owl:Class>
        </rdfs:domain>
        <rdfs:range rdf:resource="http://www.w3.org/2001/XMLSchema#dateTime"/>
    </owl:DatatypeProperty>
    


    <!-- this is an untyped string serving as a container for any data that may need to be included in a tag -->

    <owl:DatatypeProperty rdf:about="http://www.w3id.org/animl/ontology/value">
        <rdfs:comment xml:lang="en">This is an untyped string serving as a container for any data that may need to be included in a tag</rdfs:comment>
        <rdfs:subPropertyOf rdf:resource="http://www.w3.org/2002/07/owl#topDataProperty"/>
        <rdfs:domain rdf:resource="http://www.w3id.org/animl/ontology/Tag"/>
        <rdfs:range rdf:resource="http://www.w3.org/2001/XMLSchema#string"/>
    </owl:DatatypeProperty>
    



    <!-- this is a parameter indicating whether a series should be seen, it is intended as a flag for external systems that may be 
    used to display animl data -->

    <owl:DatatypeProperty rdf:about="http://www.w3id.org/animl/ontology/visability">
        <rdfs:comment xml:lang="en">This is a parameter indicating whether a series should be seen, it is intended as a flag for external systems that may be used to display animl data</rdfs:comment>
        <rdfs:domain rdf:resource="http://www.w3id.org/animl/ontology/Series"/>
        <rdfs:range rdf:resource="http://www.w3.org/2001/XMLSchema#boolean"/>
    </owl:DatatypeProperty>
    


    <!-- 
    ///////////////////////////////////////////////////////////////////////////////////////
    //
    // Classes
    //
    ///////////////////////////////////////////////////////////////////////////////////////
     -->



    


    <!-- a container for all the parameter and seriesSet data structures associated with something
    since it contains data structures, and thus is a data structure, a category may also contain another
    category as a sub-category -->

    <owl:Class rdf:about="http://www.w3id.org/animl/ontology/Category">
        <rdfs:comment xml:lang="en">A container for all the parameter and seriesSet data structures associated with something since it contains data structures, and thus is a data structure, a category may also contain another category as a sub-category</rdfs:comment>
        <rdfs:subClassOf>
            <owl:Restriction>
                <owl:onProperty rdf:resource="http://www.w3id.org/animl/ontology/hasSpecification"/>
                <owl:allValuesFrom rdf:resource="http://www.w3id.org/animl/ontology/ItemSpecification"/>
            </owl:Restriction>
        </rdfs:subClassOf>
        <rdfs:subClassOf>
            <owl:Restriction>
                <owl:onProperty rdf:resource="http://www.w3id.org/animl/ontology/hasParameter"/>
                <owl:allValuesFrom rdf:resource="http://www.w3id.org/animl/ontology/Parameter"/>
            </owl:Restriction>
        </rdfs:subClassOf>
        <rdfs:subClassOf>
            <owl:Restriction>
                <owl:onProperty rdf:resource="http://www.w3id.org/animl/ontology/hasSubCategory"/>
                <owl:allValuesFrom rdf:resource="http://www.w3id.org/animl/ontology/Category"/>
            </owl:Restriction>
        </rdfs:subClassOf>
    </owl:Class>
    


    <!-- this is an enumeration class, e.i a class that exists only to reify the enumeration of a property of another class,
    in this case the individuals for this class correspond to the possible types of a container object -->
    <owl:Class rdf:about="http://www.w3id.org/animl/ontology/ContainerType">
        <rdfs:comment xml:lang="en">This is an enumeration class, e.i a class that exists only to reify the enumeration of a property of another class, in this case the individuals for this class correspond to the possible types of a container object</rdfs:comment>
    </owl:Class>
    


    <!-- a container for a datapoint, despite transitively being a container for a single datapoint, this is not equivalent
    to a datapoint, as it is independent of an enclosing data structure -->

    <owl:Class rdf:about="http://www.w3id.org/animl/ontology/Parameter">
        <rdfs:comment xml:lang="en">A container for a datapoint, despite transitively being a container for a single datapoint, this is not equivalent to a datapoint, as it is independent of an enclosing data structure</rdfs:comment>
        <rdfs:subClassOf>
            <owl:Restriction>
                <owl:onProperty rdf:resource="http://www.w3id.org/animl/ontology/hasSpecification"/>
                <owl:allValuesFrom rdf:resource="http://www.w3id.org/animl/ontology/ParameterSpecification"/>
            </owl:Restriction>
        </rdfs:subClassOf>
    </owl:Class>
    


    <!--a sample is any item which is used, or that data regarding which is used, in an experiment in the document,
    they are often the subject of referencing to indicate that they are used in an experimentstep, however their
    set is attached to the document itself since they exist outside the context of the experiments described -->
    <owl:Class rdf:about="http://www.w3id.org/animl/ontology/Sample">
        <rdfs:comment xml:lang="en">A sample is any item which is used, or that data regarding which is used, in an experiment in the document, they are often the subject of referencing to indicate that they are used in an experimentstep, however their set is attached to the document itself since they exist outside the context of the experiments described</rdfs:comment>
        <rdfs:subClassOf>
            <owl:Restriction>
                <owl:onProperty rdf:resource="http://www.w3id.org/animl/ontology/hasSampleCategory"/>
                <owl:allValuesFrom rdf:resource="http://www.w3id.org/animl/ontology/Category"/>
            </owl:Restriction>
        </rdfs:subClassOf>
        <rdfs:subClassOf>
            <owl:Restriction>
                <owl:onProperty rdf:resource="http://www.w3id.org/animl/ontology/hasTags"/>
                <owl:allValuesFrom rdf:resource="http://www.w3id.org/animl/ontology/TagSet"/>
            </owl:Restriction>
        </rdfs:subClassOf>
        <rdfs:subClassOf>
            <owl:Restriction>
                <owl:onProperty rdf:resource="http://www.w3id.org/animl/ontology/isContained"/>
                <owl:allValuesFrom rdf:resource="http://www.w3id.org/animl/ontology/SampleInContainer"/>
            </owl:Restriction>
        </rdfs:subClassOf>
    </owl:Class>
    
    


    <!-- this is an ordered set of series data structures, series generally appear in sets
    when it is necessary to express multiple dimensions of data captured over the same interval
    or otherwise in the same context window -->
    <owl:Class rdf:about="http://www.w3id.org/animl/ontology/SeriesSet">
        <rdfs:comment xml:lang="en">This is an ordered set of series data structures, series generally appear in sets when it is necessary to express multiple dimensions of data captured over the same interval or otherwise in the same context window</rdfs:comment>
        <rdfs:subClassOf>
            <owl:Restriction>
                <owl:onProperty rdf:resource="http://www.w3id.org/animl/ontology/hasSpecification"/>
                <owl:allValuesFrom rdf:resource="http://www.w3id.org/animl/ontology/ItemSpecification"/>
            </owl:Restriction>
        </rdfs:subClassOf>
        <rdfs:subClassOf>
            <owl:Restriction>
                <owl:onProperty rdf:resource="http://www.ontologydesignpatterns.org/cp/owl/collectionentity.owl#hasMember"/>
                <owl:allValuesFrom rdf:resource="http://www.w3id.org/animl/ontology/Series"/>
            </owl:Restriction>
        </rdfs:subClassOf>
    </owl:Class>
    


    <!-- this is the set of tags which exist in the document -->
    <owl:Class rdf:about="http://www.w3id.org/animl/ontology/TagSet">
        <rdfs:comment xml:lang="en">This is the set of tags which exist in the document</rdfs:comment>
        <rdfs:subClassOf>
            <owl:Restriction>
                <owl:onProperty rdf:resource="http://www.ontologydesignpatterns.org/cp/owl/collectionentity.owl#hasMember"/>
                <owl:allValuesFrom rdf:resource="http://www.w3id.org/animl/ontology/Tag"/>
            </owl:Restriction>
        </rdfs:subClassOf>
    </owl:Class>
    


    <!-- an agent is a generalisation of several classes, author, software, device etc and may denote any external intentional object that acts on the system -->
    <owl:Class rdf:about="http://www.w3id.org/animl/ontology/Agent">
        <rdfs:comment xml:lang="en">An agent is a generalisation of several classes, author, software, device etc and may denote any external intentional object that acts on the system</rdfs:comment>
        <rdfs:subClassOf>
            <owl:Restriction>
                <owl:onProperty rdf:resource="http://www.w3id.org/animl/ontology/hasType"/>
                <owl:allValuesFrom rdf:resource="http://www.w3id.org/animl/ontology/AgentType"/>
            </owl:Restriction>
        </rdfs:subClassOf>
        <rdfs:subClassOf>      
            <owl:Restriction>
                <owl:onProperty rdf:resource="http://www.ontologydesignpatterns.org/cp/owl/bag.owl#isClassifiedBy"/>
                <owl:allValuesFrom rdf:resource="http://www.w3id.org/animl/ontology/Role"/>
            </owl:Restriction>
        </rdfs:subClassOf>
        <rdfs:subClassOf>  
            <owl:Restriction>
                <owl:onProperty rdf:resource="http://www.w3id.org/animl/ontology/hasAuditTrail"/>
                <owl:allValuesFrom rdf:resource="http://www.w3id.org/animl/ontology/AuditTrail"/>
            </owl:Restriction>
        </rdfs:subClassOf>
    </owl:Class>


    <!-- this is the concept of a role that an object in the system may need an agent to fulfil
    
                <owl:Restriction>
                <owl:onProperty rdf:resource="http://www.ontologydesignpatterns.org/cp/owl/bag.owl#isClassifiedBy"/>
                <owl:allValuesFrom rdf:resource="http://www.w3id.org/animl/ontology/Role"/>
            </owl:Restriction>-->
    <owl:Class rdf:about="http://www.w3id.org/animl/ontology/Role">
        <rdfs:comment xml:lang="en">This is the concept of a role that an object in the system may need an agent to fulfil</rdfs:comment>
        <rdfs:subClassOf>
            <owl:Restriction>
                <owl:onProperty rdf:resource="http://www.w3id.org/animl/ontology/isRoleOf"/>
                <owl:allValuesFrom rdf:resource="http://www.w3id.org/animl/ontology/Agent"/>
            </owl:Restriction>
        </rdfs:subClassOf>
    </owl:Class>
    


    <!-- this is an enumeration class, e.i a class that exists only to reify the enumeration of a property of another class,
    in this case the individuals for this class correspond to the possible types of intentional objects that could interact with the system -->
    <owl:Class rdf:about="http://www.w3id.org/animl/ontology/AgentType">
        <rdfs:comment xml:lang="en">This is an enumeration class, e.i a class that exists only to reify the enumeration of a property of another class, in this case the individuals for this class correspond to the possible types of intentional objects that could interact with the system</rdfs:comment>
    </owl:Class>

    <!-- enumeration class for encodings-->
    <owl:Class rdf:about="http://www.w3id.org/animl/ontology/DataPointType">
        <rdfs:comment xml:lang="en">Enumeration class for encodings</rdfs:comment>
    </owl:Class>
    


    <!-- this denotes the conceptual object of a change to the document, and is used to link to information regarding the context of a change
    as well as the state of the system before and after it -->
    <owl:Class rdf:about="http://www.w3id.org/animl/ontology/Change">
        <rdfs:comment xml:lang="en">This denotes the conceptual object of a change to the document, and is used to link to information regarding the context of a change as well as the state of the system before and after it</rdfs:comment>
        <rdfs:subClassOf>
            <owl:Restriction>
                <owl:onProperty rdf:resource="http://www.w3id.org/animl/ontology/affects"/>
                <owl:allValuesFrom rdf:resource="http://www.w3.org/2002/07/owl#Thing"/>
            </owl:Restriction>
        </rdfs:subClassOf>
        <rdfs:subClassOf>
            <owl:Restriction>
                <owl:onProperty rdf:resource="http://www.w3id.org/animl/ontology/hasType"/>
                <owl:allValuesFrom rdf:resource="http://www.w3id.org/animl/ontology/ChangeType"/>
            </owl:Restriction>
        </rdfs:subClassOf>
    </owl:Class>
    


    <!-- this is an enumeration class, e.i a class that exists only to reify the enumeration of a property of another class,
    in this case the individuals for this class correspond to the possible types of actions that could have been perfromed on
    an area of the document to consistute a change -->
    <owl:Class rdf:about="http://www.w3id.org/animl/ontology/ChangeType">
        <rdfs:comment xml:lang="en">This is an enumeration class, e.i a class that exists only to reify the enumeration of a property of another class, in this case the individuals for this class correspond to the possible types of actions that could have been perfromed on an area of the document to consistute a change</rdfs:comment>
    </owl:Class>
    

    <!-- this is a reification of the situation wherein a sample is present a container, used to allow information about the position of the sample in the container
    to be encoded-->
    <owl:Class rdf:about="http://www.w3id.org/animl/ontology/SampleInContainer">
        <rdfs:comment xml:lang="en">This is a reification of the situation wherein a sample is present a container, used to allow information about the position of the sample in the container to be encoded</rdfs:comment>
        <rdfs:subClassOf rdf:resource="http://www.w3.org/2002/07/owl#Thing"/>
        <rdfs:subClassOf>
            <owl:Restriction>
                <owl:onProperty rdf:resource="http://www.w3id.org/animl/ontology/isContainedBy"/>
                <owl:allValuesFrom rdf:resource="http://www.w3id.org/animl/ontology/Container"/>
            </owl:Restriction>
        </rdfs:subClassOf>
    </owl:Class>


    <!-- this is a subclass / special case of sample which is used to denote a sample which contains other samples,
    it is pointed to by the sampleincontinare situation to indicate the containing sample without allowing samples
    to directly contain themselves or force them to have a containerid when they may not always have one -->
    <owl:Class rdf:about="http://www.w3id.org/animl/ontology/Container">
        <rdfs:comment xml:lang="en">This is a subclass / special case of sample which is used to denote a sample which contains other samples, it is pointed to by the sampleincontinare situation to indicate the containing sample without allowing samples to directly contain themselves or force them to have a containerid when they may not always have one</rdfs:comment>
        <rdfs:subClassOf rdf:resource="http://www.w3id.org/animl/ontology/Sample"/>
        <rdfs:subClassOf>
            <owl:Restriction>
                <owl:onProperty rdf:resource="http://www.w3id.org/animl/ontology/hasType"/>
                <owl:someValuesFrom rdf:resource="http://www.w3id.org/animl/ontology/ContainerType"/>
            </owl:Restriction>
        </rdfs:subClassOf>
    </owl:Class>
    


    <!-- this is the root node of the document, and links into its major componentw -->
    <owl:Class rdf:about="http://www.w3id.org/animl/ontology/Document">
        <rdfs:comment xml:lang="en">This is the root node of the document, and links into its major componentw</rdfs:comment>
        <rdfs:subClassOf>
            <owl:Restriction>
                <owl:onProperty rdf:resource="http://www.w3id.org/animl/ontology/denotes"/>
                <owl:allValuesFrom rdf:resource="http://www.w3id.org/animl/ontology/Experiment"/>
            </owl:Restriction>
        </rdfs:subClassOf>
        <rdfs:subClassOf>
            <owl:Restriction>
                <owl:onProperty rdf:resource="http://www.w3id.org/animl/ontology/hasAuditTrail"/>
                <owl:allValuesFrom rdf:resource="http://www.w3id.org/animl/ontology/AuditTrail"/>
            </owl:Restriction>
        </rdfs:subClassOf>
        <rdfs:subClassOf>
            <owl:Restriction>
                <owl:onProperty rdf:resource="http://www.w3id.org/animl/ontology/hasSampleSet"/>
                <owl:allValuesFrom rdf:resource="http://www.w3id.org/animl/ontology/SampleSet"/>
            </owl:Restriction>
        </rdfs:subClassOf>
    </owl:Class>
    



    


    <!-- this is a conceptual representation of an experiment in which operations occur, and a container
    for the ordered set of experiment steps -->
    <owl:Class rdf:about="http://www.w3id.org/animl/ontology/Experiment">
        <rdfs:comment xml:lang="en">This is a conceptual representation of an experiment in which operations occur, and a container for the ordered set of experiment steps</rdfs:comment>
        <rdfs:subClassOf>
            <owl:Restriction>
                <owl:onProperty rdf:resource="http://www.w3id.org/animl/ontology/denotedBy"/>
                <owl:allValuesFrom rdf:resource="http://www.w3id.org/animl/ontology/Document"/>
            </owl:Restriction>
        </rdfs:subClassOf>
        <rdfs:subClassOf>
            <owl:Restriction>
                <owl:onProperty rdf:resource="http://www.ontologydesignpatterns.org/cp/owl/collectionentity.owl#hasMember"/>
                <owl:allValuesFrom rdf:resource="http://www.w3id.org/animl/ontology/ExperimentStep"/>
            </owl:Restriction>
        </rdfs:subClassOf>
    </owl:Class>
    


    <!-- this is the root for the largest subsections of the document, it is a representation
    of a single action undertaken during an experiment, and consists of several components, external
    supporting factors, and outputs -->
    <owl:Class rdf:about="http://www.w3id.org/animl/ontology/ExperimentStep">
        <rdfs:comment xml:lang="en">This is the root for the largest subsections of the document, it is a representation of a single action undertaken during an experiment, and consists of several components, external supporting factors, and outputs</rdfs:comment>
        <rdfs:subClassOf>
            <owl:Restriction>
                <owl:onProperty rdf:resource="http://www.w3id.org/animl/ontology/hasSpecification"/>
                <owl:allValuesFrom rdf:resource="http://www.w3id.org/animl/ontology/ItemSpecification"/>
            </owl:Restriction>
        </rdfs:subClassOf>
        <rdfs:subClassOf>
            <owl:Restriction>
                <owl:onProperty rdf:resource="http://www.ontologydesignpatterns.org/cp/owl/collectionentity.owl#isMemberOf"/>
                <owl:allValuesFrom rdf:resource="http://www.w3id.org/animl/ontology/Experiment"/>
            </owl:Restriction>
        </rdfs:subClassOf>
        <rdfs:subClassOf>
            <owl:Restriction>
                <owl:onProperty rdf:resource="http://www.ontologydesignpatterns.org/cp/owl/sequence.owl#directlyPrecedes"/>
                <owl:allValuesFrom rdf:resource="http://www.w3id.org/animl/ontology/ExperimentStep"/>
            </owl:Restriction>
        </rdfs:subClassOf>
        <rdfs:subClassOf>
            <owl:Restriction>
                <owl:onProperty rdf:resource="http://www.ontologydesignpatterns.org/cp/owl/sequence.owl#directlyFollows"/>
                <owl:allValuesFrom rdf:resource="http://www.w3id.org/animl/ontology/ExperimentStep"/>
            </owl:Restriction>
        </rdfs:subClassOf>
        <rdfs:subClassOf>
            <owl:Restriction>
                <owl:onProperty rdf:resource="http://www.ontologydesignpatterns.org/cp/owl/bag.owl#isItemOf"/>
                <owl:allValuesFrom rdf:resource="http://www.w3id.org/animl/ontology/Template"/>
            </owl:Restriction>
        </rdfs:subClassOf>
        <rdfs:subClassOf>
            <owl:Restriction>
                <owl:onProperty rdf:resource="http://www.w3id.org/animl/ontology/hasTags"/>
                <owl:allValuesFrom rdf:resource="http://www.w3id.org/animl/ontology/TagSet"/>
            </owl:Restriction>
        </rdfs:subClassOf>
        <rdfs:subClassOf>
            <owl:Restriction>
                <owl:onProperty rdf:resource="http://www.w3id.org/animl/ontology/includesInfrastructure"/>
                <owl:allValuesFrom rdf:resource="http://www.w3id.org/animl/ontology/Infrastructure"/>
            </owl:Restriction>
        </rdfs:subClassOf>
        <rdfs:subClassOf>
            <owl:Restriction>
                <owl:onProperty rdf:resource="http://www.w3id.org/animl/ontology/producesResult"/>
                <owl:allValuesFrom rdf:resource="http://www.w3id.org/animl/ontology/Result"/>
            </owl:Restriction>
        </rdfs:subClassOf>
        <rdfs:subClassOf>
            <owl:Restriction>
                <owl:onProperty rdf:resource="http://www.w3id.org/animl/ontology/usesMethod"/>
                <owl:allValuesFrom rdf:resource="http://www.w3id.org/animl/ontology/Method"/>
            </owl:Restriction>
        </rdfs:subClassOf>
        <rdfs:subClassOf>
            <owl:Restriction>
                <owl:onProperty rdf:resource="http://www.w3id.org/animl/ontology/usesTechnique"/>
                <owl:allValuesFrom rdf:resource="http://www.w3id.org/animl/ontology/Technique"/>
            </owl:Restriction>
        </rdfs:subClassOf>
    </owl:Class>
    


    <!--  a subclass of datapoint which contains a freely assignable value. -->
    <owl:Class rdf:about="http://www.w3id.org/animl/ontology/DataPoint">
        <rdfs:comment xml:lang="en">A subclass of datapoint which contains a freely assignable value.</rdfs:comment>
        <rdfs:subClassOf>
            <owl:Restriction>
                <owl:onProperty rdf:resource="http://www.ontologydesignpatterns.org/cp/owl/sequence.owl#directlyPrecedes"/>
                <owl:allValuesFrom rdf:resource="http://www.w3id.org/animl/ontology/DataPoint"/>
            </owl:Restriction>
        </rdfs:subClassOf>
        <rdfs:subClassOf>
            <owl:Restriction>
                <owl:onProperty rdf:resource="http://www.ontologydesignpatterns.org/cp/owl/sequence.owl#directlyFollows"/>
                <owl:allValuesFrom rdf:resource="http://www.w3id.org/animl/ontology/DataPoint"/>
            </owl:Restriction>
        </rdfs:subClassOf>
        <rdfs:subClassOf>
            <owl:Restriction>
                <owl:onProperty rdf:resource="http://www.w3id.org/animl/ontology/hasSpecification"/>
                <owl:allValuesFrom rdf:resource="http://www.w3id.org/animl/ontology/DataPointSpecification"/>
            </owl:Restriction>
        </rdfs:subClassOf>
        <rdfs:subClassOf>
            <owl:Restriction>
                <owl:onProperty rdf:resource="http://www.ontologydesignpatterns.org/cp/owl/collectionentity.owl#isMemberOf"/>
                <owl:allValuesFrom rdf:resource="http://www.w3id.org/animl/ontology/Series"/>
            </owl:Restriction>
        </rdfs:subClassOf>
    </owl:Class>
    


    <!-- this is a container for all the data needed to begin / which consitute, an experiment,
    this is expected to include a set of sample and can also include previous results, or any component
    of a previous experiment.
    
    this is deliberately vague so that whatever information is deemed relevant may be include,
    
    for example you may or may not wish to store the fact that a piece of machinary has finished 
    moving an is free to be acquired. -->
    <owl:Class rdf:about="http://www.w3id.org/animl/ontology/Infrastructure">
        <rdfs:comment xml:lang="en">This is a container for all the data needed to begin / which consitute, an experiment, this is expected to include a set of sample and can also include previous results, or any component of a previous experiment. this is deliberately vague so that whatever information is deemed relevant may be include, for example you may or may not wish to store the fact that a piece of machinary has finished moving an is free to be acquired.</rdfs:comment>
        <rdfs:subClassOf>
            <owl:Restriction>
                <owl:onProperty rdf:resource="http://www.w3id.org/animl/ontology/includes"/>
                <owl:allValuesFrom rdf:resource="http://www.w3id.org/animl/ontology/ReferenceSet"/>
            </owl:Restriction>
        </rdfs:subClassOf>
    </owl:Class>
    


    <!-- this broadly denotes the procedure employed to carry out the experiment, and typically
    consists of a set of parameters describing the steps involved.
    
    however since this component contains a category (a largely unrestricted data container)
    it may take a variety of forms -->
    <owl:Class rdf:about="http://www.w3id.org/animl/ontology/Method">
        <rdfs:comment xml:lang="en">This broadly denotes the procedure employed to carry out the experiment, and typically consists of a set of parameters describing the steps involved. however since this component contains a category (a largely unrestricted data container) it may take a variety of forms</rdfs:comment>
        <rdfs:subClassOf>
            <owl:Restriction>
                <owl:onProperty rdf:resource="http://www.w3id.org/animl/ontology/hasSpecification"/>
                <owl:allValuesFrom rdf:resource="http://www.w3id.org/animl/ontology/ItemSpecification"/>
            </owl:Restriction>
        </rdfs:subClassOf>
        <rdfs:subClassOf>
            <owl:Restriction>
                <owl:onProperty rdf:resource="http://www.w3id.org/animl/ontology/requiresRole"/>
                <owl:allValuesFrom rdf:resource="http://www.w3id.org/animl/ontology/Role"/>
            </owl:Restriction>
        </rdfs:subClassOf>
        <rdfs:subClassOf>
            <owl:Restriction>
                <owl:onProperty rdf:resource="http://www.w3id.org/animl/ontology/hasMethodCategory"/>
                <owl:allValuesFrom rdf:resource="http://www.w3id.org/animl/ontology/Category"/>
            </owl:Restriction>
        </rdfs:subClassOf>
    </owl:Class>
    

    


    <!-- this is a container for any subset of data that is output from an experimentstep,
    though conventionally the salient 'results'
    
    as with the other direct components of experimentstep its sturcutre allows for 
    freely assigned data to be introduced though sub elements, allowing this to take a
    variety of forms -->
    <owl:Class rdf:about="http://www.w3id.org/animl/ontology/Result">
        <rdfs:comment xml:lang="en">This is a container for any subset of data that is output from an experimentstep, though conventionally the salient 'results' as with the other direct components of experimentstep its sturcutre allows for freely assigned data to be introduced though sub elements, allowing this to take a variety of forms</rdfs:comment>
        <rdfs:subClassOf>
            <owl:Restriction>
                <owl:onProperty rdf:resource="http://www.w3id.org/animl/ontology/hasSpecification"/>
                <owl:allValuesFrom rdf:resource="http://www.w3id.org/animl/ontology/ItemSpecification"/>
            </owl:Restriction>
        </rdfs:subClassOf>
        <rdfs:subClassOf>
            <owl:Restriction>
                <owl:onProperty rdf:resource="http://www.w3id.org/animl/ontology/hasResultCategory"/>
                <owl:allValuesFrom rdf:resource="http://www.w3id.org/animl/ontology/Category"/>
            </owl:Restriction>
        </rdfs:subClassOf>
        <rdfs:subClassOf>
            <owl:Restriction>
                <owl:onProperty rdf:resource="http://www.w3id.org/animl/ontology/includes"/>
                <owl:allValuesFrom rdf:resource="http://www.w3id.org/animl/ontology/ReferenceSet"/>
            </owl:Restriction>
        </rdfs:subClassOf>
    </owl:Class>
    


    <!-- this is a container for the set of samples used in the experiment -->
    <owl:Class rdf:about="http://www.w3id.org/animl/ontology/SampleSet">
        <rdfs:comment xml:lang="en">This is a container for the set of samples used in the experiment</rdfs:comment>
        <rdfs:subClassOf>
            <owl:Restriction>
                <owl:onProperty rdf:resource="http://www.ontologydesignpatterns.org/cp/owl/collectionentity.owl#hasMember"/>
                <owl:allValuesFrom rdf:resource="http://www.w3id.org/animl/ontology/Sample"/>
            </owl:Restriction>
        </rdfs:subClassOf>
    </owl:Class>
    


    <!-- a series is a data sturcture containing ordered data points, a series may contain data points of any of the 
    three data point subclasses, but the subclass of all the datapoints in a series must be the same -->
    <owl:Class rdf:about="http://www.w3id.org/animl/ontology/Series">
        <rdfs:comment xml:lang="en">A series is a data sturcture containing ordered data points, a series may contain data points of any of the three data point subclasses, but the subclass of all the datapoints in a series must be the same</rdfs:comment>
        <rdfs:subClassOf>
            <owl:Restriction>
                <owl:onProperty rdf:resource="http://www.ontologydesignpatterns.org/cp/owl/collectionentity.owl#hasMember"/>
                <owl:allValuesFrom rdf:resource="http://www.w3id.org/animl/ontology/DataPoint"/>
            </owl:Restriction>
        </rdfs:subClassOf>
        <rdfs:subClassOf>
            <owl:Restriction>
                <owl:onProperty rdf:resource="http://www.w3id.org/animl/ontology/hasSpecification"/>
                <owl:allValuesFrom rdf:resource="http://www.w3id.org/animl/ontology/SeriesSpecification"/>
            </owl:Restriction>
        </rdfs:subClassOf>
        <rdfs:subClassOf>
            <owl:Restriction>
                <owl:onProperty rdf:resource="http://www.ontologydesignpatterns.org/cp/owl/collectionentity.owl#isMemberOf"/>
                <owl:allValuesFrom rdf:resource="http://www.w3id.org/animl/ontology/SeriesSet"/>
            </owl:Restriction>
        </rdfs:subClassOf>
    </owl:Class>
    


    <!-- this is the superclass for many of the most common classes in the document, largely the components of an experiment step
    it exists purely to indicate that all its subclasses can be marked by a signature -->




    <!-- this is a member of a set of signatures which, when linked to a signable item, causes it to be watermarked -->
    <owl:Class rdf:about="http://www.w3id.org/animl/ontology/Signature">
        <rdfs:comment xml:lang="en">This is a member of a set of signatures which, when linked to a signable item, causes it to be watermarked</rdfs:comment>
        <rdfs:subClassOf>
            <owl:Restriction>
                <owl:onProperty rdf:resource="http://www.ontologydesignpatterns.org/cp/owl/collectionentity.owl#isMemberOf"/>
                <owl:allValuesFrom rdf:resource="http://www.w3id.org/animl/ontology/SignatureSet"/>
            </owl:Restriction>
        </rdfs:subClassOf>
        <rdfs:subClassOf>
            <owl:Restriction>
                <owl:onProperty rdf:resource="http://www.w3id.org/animl/ontology/marks"/>
                <owl:allValuesFrom rdf:resource="http://www.w3.org/2002/07/owl#Thing"/>
            </owl:Restriction>
        </rdfs:subClassOf>
    </owl:Class>

    <!-- this is a container for the set of signatures present in the document -->
    <owl:Class rdf:about="http://www.w3id.org/animl/ontology/SignatureSet">
        <rdfs:comment xml:lang="en">This is a container for the set of signatures present in the document</rdfs:comment>
    </owl:Class>

    <!-- this is a loosely governed container which can be attached to an experiment step or sample to provide
    additional data about them, where said data is not otherwise expressable -->
    <owl:Class rdf:about="http://www.w3id.org/animl/ontology/Tag">
        <rdfs:comment xml:lang="en">This is a loosely governed container which can be attached to an experiment step or sample to provide additional data about them, where said data is not otherwise expressable</rdfs:comment>
    </owl:Class>
    
    <!-- this is a subclass of experimentstep used in place of its superclass when the author wishes to denote
    that the experiment is an example of / specification for a type of experimentstep -->
    <owl:Class rdf:about="http://www.w3id.org/animl/ontology/Template">
        <rdfs:comment xml:lang="en">This is a subclass of experimentstep used in place of its superclass when the author wishes to denote that the experiment is an example of / specification for a type of experimentstep</rdfs:comment>
        <rdfs:subClassOf>
            <owl:Restriction>
                <owl:onProperty rdf:resource="http://www.ontologydesignpatterns.org/cp/owl/bag.owl#hasItem"/>
                <owl:allValuesFrom rdf:resource="http://www.w3id.org/animl/ontology/ExperimentStep"/>
            </owl:Restriction>
        </rdfs:subClassOf>
    </owl:Class>
    
    <!-- this is a specific version, representing the state of the document at a particular moment in time,
    it links to an unordered collection of changes (denoting the difference between this and the previous version)
    , as well as indicating its own relative position by pointing to the previous and next version.
    
    it also has metadata attributes and links to the agents responsible for it -->
    <owl:Class rdf:about="http://www.w3id.org/animl/ontology/AuditTrailEntry">
        <rdfs:comment xml:lang="en">This is a specific version, representing the state of the document at a particular moment in time, it links to an unordered collection of changes (denoting the difference between this and the previous version), as well as indicating its own relative position by pointing to the previous and next version. it also has metadata attributes and links to the agents responsible for it</rdfs:comment>
        <rdfs:subClassOf>
            <owl:Restriction>
                <owl:onProperty rdf:resource="http://www.ontologydesignpatterns.org/cp/owl/sequence.owl#directlyPrecedes"/>
                <owl:allValuesFrom rdf:resource="http://www.w3id.org/animl/ontology/AuditTrailEntry"/>
            </owl:Restriction>
        </rdfs:subClassOf>
        <rdfs:subClassOf>
            <owl:Restriction>
                <owl:onProperty rdf:resource="http://www.ontologydesignpatterns.org/cp/owl/sequence.owl#directlyFollows"/>
                <owl:allValuesFrom rdf:resource="http://www.w3id.org/animl/ontology/AuditTrailEntry"/>
            </owl:Restriction>
        </rdfs:subClassOf>
        <rdfs:subClassOf>
            <owl:Restriction>
                <owl:onProperty rdf:resource="http://www.w3id.org/animl/ontology/requiresRole"/>
                <owl:allValuesFrom rdf:resource="http://www.w3id.org/animl/ontology/Role"/>
            </owl:Restriction>
        </rdfs:subClassOf>
        <rdfs:subClassOf>
            <owl:Restriction>
                <owl:onProperty rdf:resource="http://www.w3id.org/animl/ontology/makesChange"/>
                <owl:allValuesFrom rdf:resource="http://www.w3id.org/animl/ontology/Change"/>
            </owl:Restriction>
        </rdfs:subClassOf>
    </owl:Class>
    


    <!-- this is the set of versions of a document ,as well as the structure allowing navigation between them -->
    <owl:Class rdf:about="http://www.w3id.org/animl/ontology/AuditTrail">
        <rdfs:comment xml:lang="en">This is the set of versions of a document ,as well as the structure allowing navigation between them</rdfs:comment>
        <rdfs:subClassOf>
            <owl:Restriction>
                <owl:onProperty rdf:resource="http://www.w3id.org/animl/ontology/hasAuditTrailEntry"/>
                <owl:allValuesFrom rdf:resource="http://www.w3id.org/animl/ontology/AuditTrail"/>
            </owl:Restriction>
        </rdfs:subClassOf>
    </owl:Class>
    


    <!-- the fundamental root element for all ontologies -->

    <rdf:Description rdf:about="http://www.w3.org/2002/07/owl#Thing">
        <rdfs:comment xml:lang="en">The fundamental root element for all ontologies</rdfs:comment>
    </rdf:Description>
    


    <!-- 
    ///////////////////////////////////////////////////////////////////////////////////////
    //
    // Individuals
    //
    ///////////////////////////////////////////////////////////////////////////////////////
     -->

    <!-- a type of sample containing sample -->

    <owl:NamedIndividual rdf:about="http://www.w3id.org/animl/ontology/determinate">
        <rdfs:comment xml:lang="en">Determinate container type</rdfs:comment>
        <rdf:type rdf:resource="http://www.w3id.org/animl/ontology/ContainerType"/>
    </owl:NamedIndividual>
    
    <!-- a type of sample containing sample -->

    <owl:NamedIndividual rdf:about="http://www.w3id.org/animl/ontology/indeterminate">
        <rdfs:comment xml:lang="en">Indeterminate container type</rdfs:comment>
        <rdf:type rdf:resource="http://www.w3id.org/animl/ontology/ContainerType"/>
    </owl:NamedIndividual>
    
    <!-- a type of sample containing sample -->

    <owl:NamedIndividual rdf:about="http://www.w3id.org/animl/ontology/rectangular_Tray">
        <rdfs:comment xml:lang="en">Rectangular tray container type</rdfs:comment>
        <rdf:type rdf:resource="http://www.w3id.org/animl/ontology/ContainerType"/>
    </owl:NamedIndividual>
    

    <!-- a type of sample containing sample -->

    <owl:NamedIndividual rdf:about="http://www.w3id.org/animl/ontology/1536_Wells">
        <rdfs:comment xml:lang="en">1536 wells container type</rdfs:comment>
        <rdf:type rdf:resource="http://www.w3id.org/animl/ontology/ContainerType"/>
    </owl:NamedIndividual>
    


    <!-- a type of sample containing sample -->

    <owl:NamedIndividual rdf:about="http://www.w3id.org/animl/ontology/24_Wells">
        <rdfs:comment xml:lang="en">24 wells container type</rdfs:comment>
        <rdf:type rdf:resource="http://www.w3id.org/animl/ontology/ContainerType"/>
    </owl:NamedIndividual>
    


    <!-- a type of sample containing sample -->

    <owl:NamedIndividual rdf:about="http://www.w3id.org/animl/ontology/384_Wells">
        <rdfs:comment xml:lang="en">384 wells container type</rdfs:comment>
        <rdf:type rdf:resource="http://www.w3id.org/animl/ontology/ContainerType"/>
    </owl:NamedIndividual>
    


    <!-- a type of sample containing sample -->

    <owl:NamedIndividual rdf:about="http://www.w3id.org/animl/ontology/6_Wells">
        <rdfs:comment xml:lang="en">6 wells container type</rdfs:comment>
        <rdf:type rdf:resource="http://www.w3id.org/animl/ontology/ContainerType"/>
    </owl:NamedIndividual>
    


    <!-- a type of sample containing sample -->

    <owl:NamedIndividual rdf:about="http://www.w3id.org/animl/ontology/96_Wells">
        <rdfs:comment xml:lang="en">96 wells container type</rdfs:comment>
        <rdf:type rdf:resource="http://www.w3id.org/animl/ontology/ContainerType"/>
    </owl:NamedIndividual>
    


    <!-- a type of change to a an element of a document -->

    <owl:NamedIndividual rdf:about="http://www.w3id.org/animl/ontology/creation">
        <rdfs:comment xml:lang="en">A creation change type</rdfs:comment>
        <rdf:type rdf:resource="http://www.w3id.org/animl/ontology/ChangeType"/>
    </owl:NamedIndividual>
    


    <!-- a type of change to a an element of a document -->

    <owl:NamedIndividual rdf:about="http://www.w3id.org/animl/ontology/deletion">
        <rdfs:comment xml:lang="en">A deletion change type</rdfs:comment>
        <rdf:type rdf:resource="http://www.w3id.org/animl/ontology/ChangeType"/>
    </owl:NamedIndividual>
    


    <!-- a type of agent, and a subtype of creator agent -->

    <owl:NamedIndividual rdf:about="http://www.w3id.org/animl/ontology/HumanAgent">
        <rdfs:comment xml:lang="en">A person as a human agent type</rdfs:comment>
        <rdf:type rdf:resource="http://www.w3id.org/animl/ontology/AgentType"/>
    </owl:NamedIndividual>
    


    <!-- a type of change to a an element of a document -->

    <owl:NamedIndividual rdf:about="http://www.w3id.org/animl/ontology/modification">
        <rdfs:comment xml:lang="en">A modification change type</rdfs:comment>
        <rdf:type rdf:resource="http://www.w3id.org/animl/ontology/ChangeType"/>
    </owl:NamedIndividual>
    


    <!-- a type of agent -->

    <owl:NamedIndividual rdf:about="http://www.w3id.org/animl/ontology/softwareAgent">
        <rdfs:comment xml:lang="en">A software agent type</rdfs:comment>
        <rdf:type rdf:resource="http://www.w3id.org/animl/ontology/AgentType"/>
    </owl:NamedIndividual>
    


    <!-- a type of agent -->

    <owl:NamedIndividual rdf:about="http://www.w3id.org/animl/ontology/hardwareAgent">
        <rdfs:comment xml:lang="en">A hardware agent type</rdfs:comment>
        <rdf:type rdf:resource="http://www.w3id.org/animl/ontology/AgentType"/>
    </owl:NamedIndividual>

    <!-- a type of dataPoint-->
    <owl:NamedIndividual rdf:about="http://www.w3id.org/animl/ontology/binaryEncoding">
        <rdfs:comment xml:lang="en">A binary encoding data point type</rdfs:comment>
        <rdf:type rdf:resource="http://www.w3id.org/animl/ontology/DataPointType"/>
    </owl:NamedIndividual>

    <!-- a type of dataPoint-->
    <owl:NamedIndividual rdf:about="http://www.w3id.org/animl/ontology/autoIncrementedEncoding">
        <rdfs:comment xml:lang="en">An auto incremented encoding data point type</rdfs:comment>
        <rdf:type rdf:resource="http://www.w3id.org/animl/ontology/DataPointType"/>
    </owl:NamedIndividual>

    <!-- a type of dataPoint-->
    <owl:NamedIndividual rdf:about="http://www.w3id.org/animl/ontology/individualEncoding">
        <rdfs:comment xml:lang="en">An individual encoding data point type</rdfs:comment>
        <rdf:type rdf:resource="http://www.w3id.org/animl/ontology/DataPointType"/>
    </owl:NamedIndividual>
    



        <!-- 
    // ANIML_TECHNIQUE
    // ANIML_TECHNIQUE
    // ANIML_TECHNIQUE
    // ANIML_TECHNIQUE
    // ANIML_TECHNIQUE
    // ANIML_TECHNIQUE
    // ANIML_TECHNIQUE
     -->

    <!-- this component represents the animl technique schema, or arguably meta schema, which restricts the format of technique definition documents.
    
    the purpose of a technique definition government is conceptually to express the steps involved in a type of scientific operation, and practically
    to govern certain of the properties for elements involved in an experiment step
    
    the effect of an ATDD file on an animl knowledge base can be expressed as a set of object specifications, themsleves objects with ispart relations to 
    experiment step related objects. with these specification objects being the domain for the relationships and data (regarding the object specified) that are
    pre determined by the ATDD.
    
    since the technique file is itself a specification for ATDD files, it can be expressed as an ontology for the specification objects-->

        <!-- 
    ///////////////////////////////////////////////////////////////////////////////////////
    //
    // Object Properties
    //
    ///////////////////////////////////////////////////////////////////////////////////////
     -->

         <!-- denotes the relationship contained within the context of the specification for a referenced item,
    a relationship which indicates the requirement for the referenced item to have been consumed in a particular technique
    here technique may be viewed in its form as a specification for an experiment step -->

    <owl:ObjectProperty rdf:about="http://www.w3id.org/animl/ontology/consumedBy">
        <rdfs:comment xml:lang="en">Denotes the relationship contained within the context of the specification for a referenced item, a relationship which indicates the requirement for the referenced item to have been consumed in a particular technique here technique may be viewed in its form as a specification for an experiment step</rdfs:comment>
        <rdfs:domain rdf:resource="http://www.w3id.org/animl/ontology/ReferenceSpecification"/>
        <rdfs:range rdf:resource="http://www.w3id.org/animl/ontology/Technique"/>
    </owl:ObjectProperty>
    


    <!-- this is the inverse of the above relation, and denotes the requirement for a technique to consume the referenced item of a referenec
    in order for that item to be referenced
    this relationship is not entirely intuitive, but it is necessary to preserve expressivity found in the original xml -->

    <owl:ObjectProperty rdf:about="http://www.w3id.org/animl/ontology/consumes">
        <rdfs:comment xml:lang="en">Denotes the requirement for a technique to consume the referenced item of a referenec in order for that item to be referenced this relationship is not entirely intuitive, but it is necessary to preserve expressivity found in the original xml</rdfs:comment>
        <rdfs:domain rdf:resource="http://www.w3id.org/animl/ontology/Technique"/>
        <rdfs:range rdf:resource="http://www.w3id.org/animl/ontology/ReferenceSpecification"/>
    </owl:ObjectProperty>
    


    <!-- denotes the relationship contained within the context of the specification for a referenced item,
    a relationship which indicates the requirement for the referenced item to have been derived from a particular technique
    here technique may be viewed in its form as a specification for an experiment step  -->

    <owl:ObjectProperty rdf:about="http://www.w3id.org/animl/ontology/derivedFrom">
        <rdfs:comment xml:lang="en">Denotes the relationship contained within the context of the specification for a referenced item, a relationship which indicates the requirement for the referenced item to have been derived from a particular technique here technique may be viewed in its form as a specification for an experiment step</rdfs:comment>
        <rdfs:domain rdf:resource="http://www.w3id.org/animl/ontology/ReferenceSpecification"/>
        <rdfs:range rdf:resource="http://www.w3id.org/animl/ontology/Technique"/>
    </owl:ObjectProperty>
    


    <!-- this is the inverse of the above relation, and denotes the requirement for a technique to derive the referenced item of a referenec
    in order for that item to be referenced
    this relationship is not entirely intuitive, but it is necessary to preserve expressivity found in the original xml -->

    <owl:ObjectProperty rdf:about="http://www.w3id.org/animl/ontology/derives">
        <rdfs:comment xml:lang="en">Denotes the requirement for a technique to derive the referenced item of a referenec in order for that item to be referenced this relationship is not entirely intuitive, but it is necessary to preserve expressivity found in the original xml</rdfs:comment>
        <rdfs:domain rdf:resource="http://www.w3id.org/animl/ontology/Technique"/>
        <rdfs:range rdf:resource="http://www.w3id.org/animl/ontology/ReferenceSpecification"/>
    </owl:ObjectProperty>


        <!-- this relationship denotes that the 'extension' (itself a subclass of technique) exists to:
    extend the technqiue if you consider techniques as independent
    complete the specification for an experiment step, if you consider technqieus as specifications for experiment steps -->

    <owl:ObjectProperty rdf:about="http://www.w3id.org/animl/ontology/extends">
        <rdfs:comment xml:lang="en">Denotes that the 'extension' (itself a subclass of technique) exists to: extend the technqiue if you consider techniques as independent complete the specification for an experiment step, if you consider technqieus as specifications for experiment steps</rdfs:comment>
        <rdfs:domain rdf:resource="http://www.w3id.org/animl/ontology/Technique"/>
        <rdfs:range rdf:resource="http://www.w3id.org/animl/ontology/Technique"/>
    </owl:ObjectProperty>
    

    <!-- this is the inverse of the above relation, denoting that a technique is extended or completed by a particular extension -->



    <!-- denotes that a class is a container for data with corresponding units of measurement, a complex quantity may have multiple units
    e.i mph, or rpm -->

    <owl:ObjectProperty rdf:about="http://www.w3id.org/animl/ontology/hasUnits">
        <rdfs:comment xml:lang="en">Denotes that a class is a container for data with corresponding units of measurement, a complex quantity may have multiple units e.i mph, or rpm</rdfs:comment>
        <rdfs:domain rdf:resource="http://www.w3id.org/animl/ontology/ParameterSpecification"/>
        <rdfs:range rdf:resource="http://www.w3id.org/animl/ontology/Units"/>
    </owl:ObjectProperty>

        <!-- conceptually this relationship is the property of being bound to a specific data type, which forces classes representing data containers
    to have individuals that only contain data of specific types
    
    however it is attached to the specification for such containers, since the type of data a container may hold is governed by its specification -->

    <owl:ObjectProperty rdf:about="http://www.w3id.org/animl/ontology/hasDataType">
        <rdfs:comment xml:lang="en">Conceptually this relationship is the property of being bound to a specific data type, which forces classes representing data containers to have individuals that only contain data of specific types however it is attached to the specification for such containers, since the type of data a container may hold is governed by its specification</rdfs:comment>
        <rdfs:domain rdf:resource="http://www.w3id.org/animl/ontology/ParameterSpecification"/>
        <rdfs:range rdf:resource="http://www.w3id.org/animl/ontology/DataType"/>
    </owl:ObjectProperty>
    

            <!-- 
    ///////////////////////////////////////////////////////////////////////////////////////
    //
    // Data Properties
    //
    ///////////////////////////////////////////////////////////////////////////////////////
     -->

         <!-- a constant value added to the equation resulting from the combination of data with units -->

        <owl:DatatypeProperty rdf:about="http://www.w3id.org/animl/ontology/offset">
        <rdfs:comment xml:lang="en">A constant value added to the equation resulting from the combination of data with units</rdfs:comment>
            <rdfs:domain rdf:resource="http://www.w3id.org/animl/ontology/SIUnit"/>
            <rdfs:range rdf:resource="http://www.w3.org/2001/XMLSchema#double"/>
        </owl:DatatypeProperty>
    


        <!-- an english language description of type of objects or measurements to which units may be assigned -->

        <owl:DatatypeProperty rdf:about="http://www.w3id.org/animl/ontology/quantity">
        <rdfs:comment xml:lang="en">A description of type of objects or measurements to which units may be assigned</rdfs:comment>
            <rdfs:domain rdf:resource="http://www.w3id.org/animl/ontology/Units"/>
            <rdfs:range rdf:resource="http://www.w3.org/2001/XMLSchema#double"/>
        </owl:DatatypeProperty>

        <!-- a raised power, typically used to raise the dimensionality of spacial data -->

        <owl:DatatypeProperty rdf:about="http://www.w3id.org/animl/ontology/exponent">
            <rdfs:comment xml:lang="en">A raised power, typically used to raise the dimensionality of spacial data</rdfs:comment>
            <rdfs:domain rdf:resource="http://www.w3id.org/animl/ontology/SIUnit"/>
            <rdfs:range rdf:resource="http://www.w3.org/2001/XMLSchema#double"/>
        </owl:DatatypeProperty>
    
        <!-- a coefficient upon a set of units, typically an order of magnitude -->

        <owl:DatatypeProperty rdf:about="http://www.w3id.org/animl/ontology/factor">
            <rdfs:comment xml:lang="en">A coefficient upon a set of units, typically an order of magnitude</rdfs:comment>
            <rdfs:domain rdf:resource="http://www.w3id.org/animl/ontology/SIUnit"/>
            <rdfs:range rdf:resource="http://www.w3.org/2001/XMLSchema#double"/>
        </owl:DatatypeProperty>

        <!-- a string space for the bibliography related to an object -->

        <owl:DatatypeProperty rdf:about="http://www.w3id.org/animl/ontology/citations">
            <rdfs:comment xml:lang="en">A string space for the bibliography related to an object</rdfs:comment>
            <rdfs:domain>
                <owl:Class>
                    <owl:unionOf rdf:parseType="Collection">
                        <rdf:Description rdf:about="http://www.w3id.org/animl/ontology/Technique"/>
                        <rdf:Description rdf:about="http://www.w3id.org/animl/ontology/ItemSpecification"/>
                    </owl:unionOf>
                </owl:Class>
            </rdfs:domain>
            <rdfs:range rdf:resource="http://www.w3.org/2001/XMLSchema#string"/>
        </owl:DatatypeProperty>

        <!-- a string space for a software requirement enumeration for an object -->

        <owl:DatatypeProperty rdf:about="http://www.w3id.org/animl/ontology/dependency">
            <rdfs:comment xml:lang="en">A string space for a software requirement enumeration for an object</rdfs:comment>
            <rdfs:domain rdf:resource="http://www.w3id.org/animl/ontology/SeriesSpecification"/>
            <rdfs:range rdf:resource="http://www.w3.org/2001/XMLSchema#string"/>
        </owl:DatatypeProperty>

        <!-- the semantic web identifier for a the superclass of technique and extension, used as a path to import an ATDD to an animl file -->


        <!-- a boolean denoting whether or not a technique or extension will work without being extended -->

        <owl:DatatypeProperty rdf:about="http://www.w3id.org/animl/ontology/abstract">
            <rdfs:comment xml:lang="en">A boolean denoting whether or not a technique or extension will work without being extended</rdfs:comment>
            <rdfs:domain rdf:resource="http://www.w3id.org/animl/ontology/Technique"/>
            <rdfs:range rdf:resource="http://www.w3.org/2001/XMLSchema#boolean"/>
        </owl:DatatypeProperty>

        <!-- a unique token used to authenticate identity of an ATDD for security purposes -->

        <owl:DatatypeProperty rdf:about="http://www.w3id.org/animl/ontology/token">
            <rdfs:comment xml:lang="en">A unique token used to authenticate identity of an ATDD for security purposes</rdfs:comment>
            <rdfs:domain rdf:resource="http://www.w3id.org/animl/ontology/Technique"/>
            <rdfs:range rdf:resource="http://www.w3.org/2001/XMLSchema#token"/>
        </owl:DatatypeProperty>


            <!-- 
    ///////////////////////////////////////////////////////////////////////////////////////
    //
    // Classes
    //
    ///////////////////////////////////////////////////////////////////////////////////////
     -->

         <!-- this is the generic superclass for specifications, those objects which represent components of animl-core classes which
        are governed by the relevant ATDD file,each specification may be a part of exactly one other object -->
        <owl:Class rdf:about="http://www.w3id.org/animl/ontology/Specification">
            <rdfs:comment xml:lang="en">This is the generic superclass for specifications, those objects which represent components of animl-core classes which are governed by the relevant ATDD file,each specification may be a part of exactly one other object</rdfs:comment>
            <rdfs:subClassOf>
                <owl:Restriction>
                    <owl:onProperty rdf:resource="http://www.w3id.org/animl/ontology/usedBy"/>
                    <owl:minCardinality rdf:datatype="http://www.w3.org/2001/XMLSchema#nonNegativeInteger">1</owl:minCardinality>
                </owl:Restriction>
            </rdfs:subClassOf>
        </owl:Class>


         <!-- a simple class which exists only to be a component of those classes whose only governed components are those in specification
         these classes (A) cannot be directly part of specification, as then it would be possible for classes in A to have part to the more complex
         and specialised subclasses of specification   -->  
        <owl:Class rdf:about="http://www.w3id.org/animl/ontology/ItemSpecification">
            <rdfs:comment xml:lang="en">A simple class which exists only to be a component of those classes whose only governed components are those in specification these classes (A) cannot be directly part of specification, as then it would be possible for classes in A to have part to the more complex and specialised subclasses of specification</rdfs:comment>
            <rdfs:subClassOf rdf:resource="http://www.w3id.org/animl/ontology/Specification"/>

            <!-- AllValuesFrom constraint over a union of classes -->


            <rdfs:subClassOf>
                <owl:Restriction>
                    <owl:onProperty rdf:resource="http://www.w3id.org/animl/ontology/usedBy"/>
                    <owl:allValuesFrom>
                        <owl:Class>
                            <owl:unionOf rdf:parseType="Collection">
                                <rdf:Description rdf:about="http://www.w3id.org/animl/ontology/Role"/>
                                <rdf:Description rdf:about="http://www.w3id.org/animl/ontology/Category"/>
                                <rdf:Description rdf:about="http://www.w3id.org/animl/ontology/ExperimentStep"/>
                                <rdf:Description rdf:about="http://www.w3id.org/animl/ontology/Method"/>
                                <rdf:Description rdf:about="http://www.w3id.org/animl/ontology/Result"/>
                            </owl:unionOf>
                        </owl:Class>
                    </owl:allValuesFrom>
                </owl:Restriction>
            </rdfs:subClassOf>
        </owl:Class>



        <!-- this is the subclass of specification which applies to parameters, and includes additional attribute restrictions,
        as well as indicating that the data in a parameter must be linked to a certain set of units -->
        <owl:Class rdf:about="http://www.w3id.org/animl/ontology/ParameterSpecification">
            <rdfs:comment xml:lang="en">This is the subclass of specification which applies to parameters, and includes additional attribute restrictions, as well as indicating that the data in a parameter must be linked to a certain set of units</rdfs:comment>
            <rdfs:subClassOf rdf:resource="http://www.w3id.org/animl/ontology/Specification"/>
            <rdfs:subClassOf>
                <owl:Restriction>
                    <owl:onProperty rdf:resource="http://www.w3id.org/animl/ontology/hasDataType"/>
                    <owl:allValuesFrom rdf:resource="http://www.w3id.org/animl/ontology/DataType"/>
                </owl:Restriction>
            </rdfs:subClassOf>
            <rdfs:subClassOf>
                <owl:Restriction>
                    <owl:onProperty rdf:resource="http://www.w3id.org/animl/ontology/hasUnits"/>
                    <owl:allValuesFrom rdf:resource="http://www.w3id.org/animl/ontology/Units"/>
                </owl:Restriction>
            </rdfs:subClassOf>
            <rdfs:subClassOf>
                <owl:Restriction>
                    <owl:onProperty rdf:resource="http://www.w3id.org/animl/ontology/usedBy"/>
                    <owl:allValuesFrom rdf:resource="http://www.w3id.org/animl/ontology/Parameter"/>
                </owl:Restriction>
            </rdfs:subClassOf>
        </owl:Class>


        <!-- this is the subclass of specification which applies to series, and includes additional attribute restrictions,
        as well as indicating that the data points of a series must all have a common set of units -->
        <owl:Class rdf:about="http://www.w3id.org/animl/ontology/SeriesSpecification">
            <rdfs:comment xml:lang="en">This is the subclass of specification which applies to series, and includes additional attribute restrictions, as well as indicating that the data points of a series must all have a common set of units</rdfs:comment>
            <rdfs:subClassOf rdf:resource="http://www.w3id.org/animl/ontology/Specification"/>
            <rdfs:subClassOf>
                <owl:Restriction>
                    <owl:onProperty rdf:resource="http://www.w3id.org/animl/ontology/hasDataType"/>
                    <owl:allValuesFrom rdf:resource="http://www.w3id.org/animl/ontology/DataType"/>
                </owl:Restriction>
            </rdfs:subClassOf>
            <rdfs:subClassOf>
                <owl:Restriction>
                    <owl:onProperty rdf:resource="http://www.w3id.org/animl/ontology/hasPlotScale"/>
                    <owl:allValuesFrom rdf:resource="http://www.w3id.org/animl/ontology/PlotScale"/>
                </owl:Restriction>
            </rdfs:subClassOf>
            <rdfs:subClassOf>
                <owl:Restriction>
                    <owl:onProperty rdf:resource="http://www.w3id.org/animl/ontology/hasUnits"/>
                    <owl:allValuesFrom rdf:resource="http://www.w3id.org/animl/ontology/Units"/>
                </owl:Restriction>
            </rdfs:subClassOf>
            <rdfs:subClassOf>
                <owl:Restriction>
                    <owl:onProperty rdf:resource="http://www.w3id.org/animl/ontology/usedBy"/>
                    <owl:allValuesFrom rdf:resource="http://www.w3id.org/animl/ontology/Series"/>
                </owl:Restriction>
            </rdfs:subClassOf>
            <rdfs:subClassOf>
                <owl:Restriction>
                    <owl:onProperty rdf:resource="http://www.w3id.org/animl/ontology/hasPart"/>
                    <owl:qualifiedCardinality rdf:datatype="http://www.w3.org/2001/XMLSchema#nonNegativeInteger">1</owl:qualifiedCardinality>
                    <owl:onClass rdf:resource="http://www.w3id.org/animl/ontology/DataPointSpecification"/>
                </owl:Restriction>
            </rdfs:subClassOf>
        </owl:Class>

        <!-- data point specification-->
        <owl:Class rdf:about="http://www.w3id.org/animl/ontology/DataPointSpecification">
            <rdfs:comment xml:lang="en">Data point specification</rdfs:comment>
            <rdfs:subClassOf rdf:resource="http://www.w3id.org/animl/ontology/Specification"/>
            <rdfs:subClassOf>
                <owl:Restriction>
                    <owl:onProperty rdf:resource="http://www.w3id.org/animl/ontology/hasDataType"/>
                    <owl:allValuesFrom rdf:resource="http://www.w3id.org/animl/ontology/DataType"/>
                </owl:Restriction>
            </rdfs:subClassOf>
            <rdfs:subClassOf>
                <owl:Restriction>
                    <owl:onProperty rdf:resource="http://www.w3id.org/animl/ontology/hasType"/>
                    <owl:allValuesFrom rdf:resource="http://www.w3id.org/animl/ontology/DataPointType"/>
                </owl:Restriction>
            </rdfs:subClassOf>
            <rdfs:subClassOf>
                <owl:Restriction>
                    <owl:onProperty rdf:resource="http://www.w3id.org/animl/ontology/usedBy"/>
                    <owl:allValuesFrom>
                        <owl:Class>
                            <owl:unionOf rdf:parseType="Collection">
                                <rdf:Description rdf:about="http://www.w3id.org/animl/ontology/DataPoint"/>
                                <rdf:Description rdf:about="http://www.w3id.org/animl/ontology/SeriesSpecification"/>
                            </owl:unionOf>
                        </owl:Class>
                    </owl:allValuesFrom>
                </owl:Restriction>
            </rdfs:subClassOf>
            <rdfs:subClassOf>
                <owl:Restriction>
                    <owl:onProperty rdf:resource="http://www.w3id.org/animl/ontology/isPartOf"/>
                    <owl:qualifiedCardinality rdf:datatype="http://www.w3.org/2001/XMLSchema#nonNegativeInteger">1</owl:qualifiedCardinality>
                    <owl:onClass rdf:resource="http://www.w3id.org/animl/ontology/SeriesSpecification"/>
                </owl:Restriction>
            </rdfs:subClassOf>
        </owl:Class>

        <!-- this is the specification subclass for a reference, it may have either a consumedby or derived from relation to any 
        technique (and exactly one of each relation). this is because the technique of an experimentstep governs whether a
        sample is produced or consumed during it.
        
        this could be considered to be a property of a sample specification, except that samples are understood to exist outside
        of the context of the experiment (especially since some are neither consumed or produced in the experiment) and as such the ATDD
        can only govern the way in which they are linked into the experiment. -->

        <owl:AllDisjointProperties>
            <owl:members rdf:parseType="Collection">
                <rdf:Description rdf:about="http://www.w3id.org/animl/ontology/derivedFrom"/>
                <rdf:Description rdf:about="http://www.w3id.org/animl/ontology/consumedBy"/>
            </owl:members>
        </owl:AllDisjointProperties>
        <owl:Class rdf:about="http://www.w3id.org/animl/ontology/ReferenceSpecification">
            <rdfs:comment xml:lang="en">This is the specification subclass for a reference, it may have either a consumedby or derived from relation to any technique (and exactly one of each relation). this is because the technique of an experimentstep governs whether a sample is produced or consumed during it. this could be considered to be a property of a sample specification, except that samples are understood to exist outside of the context of the experiment (especially since some are neither consumed or produced in the experiment) and as such the ATDD can only govern the way in which they are linked into the experiment.</rdfs:comment>
            <rdfs:subClassOf rdf:resource="http://www.w3id.org/animl/ontology/Specification"/>
            <rdfs:subClassOf>
                <owl:Restriction>
                    <owl:onProperty rdf:resource="http://www.w3id.org/animl/ontology/consumedBy"/>
                    <owl:allValuesFrom rdf:resource="http://www.w3id.org/animl/ontology/Technique"/>
                </owl:Restriction>
            </rdfs:subClassOf>
            <rdfs:subClassOf>
                <owl:Restriction>
                    <owl:onProperty rdf:resource="http://www.w3id.org/animl/ontology/derivedFrom"/>
                    <owl:allValuesFrom rdf:resource="http://www.w3id.org/animl/ontology/Technique"/>
                </owl:Restriction>
            </rdfs:subClassOf>
            <rdfs:subClassOf>
                <owl:Restriction>
                    <owl:onProperty rdf:resource="http://www.w3id.org/animl/ontology/derivedFrom"/>
                    <owl:maxCardinality rdf:datatype="http://www.w3.org/2001/XMLSchema#nonNegativeInteger">1</owl:maxCardinality>
                </owl:Restriction>
            </rdfs:subClassOf>
            <rdfs:subClassOf>
                <owl:Restriction>
                    <owl:onProperty rdf:resource="http://www.w3id.org/animl/ontology/consumedBy"/>
                    <owl:maxCardinality rdf:datatype="http://www.w3.org/2001/XMLSchema#nonNegativeInteger">1</owl:maxCardinality>
                </owl:Restriction>
            </rdfs:subClassOf>
            <rdfs:subClassOf>
                <owl:Restriction>
                    <owl:onProperty rdf:resource="http://www.w3id.org/animl/ontology/usedBy"/>
                    <owl:allValuesFrom rdf:resource="http://www.w3id.org/animl/ontology/Reference"/>
                </owl:Restriction>
            </rdfs:subClassOf>
        </owl:Class>


        <!-- this is an enumeration class, e.i a class that exists only to reify the enumeration of a property of another class,
        in this case the individuals for this class correspond to the possible data types for a datapoint -->
        <owl:Class rdf:about="http://www.w3id.org/animl/ontology/DataType">
            <rdfs:comment xml:lang="en">This is an enumeration class, e.i a class that exists only to reify the enumeration of a property of another class, in this case the individuals for this class correspond to the possible data types for a datapoint</rdfs:comment>
        </owl:Class>


        <!-- this is an enumeration class, e.i a class that exists only to reify the enumeration of a property of another class,
        in this case the individuals for this class correspond to the possible kinds of scale a datapoint with units
        may be on. e.i it determines whether a datapoint is on a linear, logarithmic, or other kind of scale -->
        <owl:Class rdf:about="http://www.w3id.org/animl/ontology/PlotScale">
            <rdfs:comment xml:lang="en">This is an enumeration class, e.i a class that exists only to reify the enumeration of a property of another class, in this case the individuals for this class correspond to the possible kinds of scale a datapoint with units may be on. e.i it determines whether a datapoint is on a linear, logarithmic, or other kind of scale</rdfs:comment>
        </owl:Class>



        <!-- this is an ordered collection of Siunits which acts to create a compound unit -->
        <owl:Class rdf:about="http://www.w3id.org/animl/ontology/Units">
            <rdfs:comment xml:lang="en">This is an ordered collection of Siunits which acts to create a compound unit</rdfs:comment>
            <rdfs:subClassOf>
                <owl:Restriction>
                    <owl:onProperty rdf:resource="http://www.ontologydesignpatterns.org/cp/owl/collectionentity.owl#hasMember"/>
                    <owl:allValuesFrom rdf:resource="http://www.w3id.org/animl/ontology/SIUnit"/>
                </owl:Restriction>
            </rdfs:subClassOf>
        </owl:Class>

        <!-- this is unique in the document in that it is both an enumeration class, e.i a class that  reifies the enumeration of a property of another class,
        and links to members of its own class to indicate its position in an ordered set. this is because it is known that its individuals must correspond to one of the
        limited set of Siunits, but those units can still be combined in an intractable number of ways, making direct enumeration of options impossible. -->
        <owl:Class rdf:about="http://www.w3id.org/animl/ontology/SIUnit">
            <rdfs:comment xml:lang="en">This is unique in the document in that it is both an enumeration class, e.i a class that  reifies the enumeration of a property of another class, and links to members of its own class to indicate its position in an ordered set. this is because it is known that its individuals must correspond to one of the limited set of Siunits, but those units can still be combined in an intractable number of ways, making direct enumeration of options impossible.</rdfs:comment>
            <rdfs:subClassOf>
                <owl:Restriction>
                    <owl:onProperty rdf:resource="http://www.ontologydesignpatterns.org/cp/owl/sequence.owl#directlyPrecedes"/>
                    <owl:allValuesFrom rdf:resource="http://www.w3id.org/animl/ontology/Units"/>
                </owl:Restriction>
            </rdfs:subClassOf>
            <rdfs:subClassOf>
                <owl:Restriction>
                    <owl:onProperty rdf:resource="http://www.ontologydesignpatterns.org/cp/owl/sequence.owl#directlyFollows"/>
                    <owl:allValuesFrom rdf:resource="http://www.w3id.org/animl/ontology/Units"/>
                </owl:Restriction>
            </rdfs:subClassOf>
            <rdfs:subClassOf>
                <owl:Restriction>
                    <owl:onProperty rdf:resource="http://www.ontologydesignpatterns.org/cp/owl/collectionentity.owl#isMemberOf"/>
                    <owl:allValuesFrom rdf:resource="http://www.w3id.org/animl/ontology/Units"/>
                </owl:Restriction>
            </rdfs:subClassOf>
        </owl:Class>


        <!-- this is the superclass of technique and extension, which houses their common attributes and expresses
        the fact that the two classes are the same apart from extensions extending techniques -->


        <!-- this is a container for all the specification objects that exist in the ATDD governance component of a
        animl KB. conceptually it is 
        also the broader specification for an experiment step, it is identical to its superclass of definition
         except in that it can be extended by extensions,
        and can have derive and consume relations, which express the ability of an ATDD to govern when samples
        are created or destroyed during experiment steps.
        
        as with their inverses, a technique may not have a derive and consume relation to the same reference specification.
        however unlike a reference specification, it may have multiple derive and consume relations over all.  -->

        <owl:AllDisjointProperties>
            <owl:members rdf:parseType="Collection">
                <rdf:Description rdf:about="http://www.w3id.org/animl/ontology/derives"/>
                <rdf:Description rdf:about="http://www.w3id.org/animl/ontology/consumes"/>
            </owl:members>
        </owl:AllDisjointProperties>


        <owl:Class rdf:about="http://www.w3id.org/animl/ontology/Technique">
            <rdfs:comment xml:lang="en">This is a container for all the specification objects that exist in the ATDD governance component of a animl KB. conceptually it is also the broader specification for an experiment step, it is identical to its superclass of definition except in that it can be extended by extensions, and can have derive and consume relations, which express the ability of an ATDD to govern when samples are created or destroyed during experiment steps. as with their inverses, a technique may not have a derive and consume relation to the same reference specification. however unlike a reference specification, it may have multiple derive and consume relations over all.</rdfs:comment>
            <rdfs:subClassOf>
                <owl:Restriction>
                    <owl:onProperty rdf:resource="http://www.w3id.org/animl/ontology/consumes"/>
                    <owl:allValuesFrom rdf:resource="http://www.w3id.org/animl/ontology/ReferenceSpecification"/>
                </owl:Restriction>
            </rdfs:subClassOf>
            <rdfs:subClassOf>
                <owl:Restriction>
                    <owl:onProperty rdf:resource="http://www.w3id.org/animl/ontology/derives"/>
                    <owl:allValuesFrom rdf:resource="http://www.w3id.org/animl/ontology/ReferenceSpecification"/>
                </owl:Restriction>
            </rdfs:subClassOf>
            <rdfs:subClassOf>
                <owl:Restriction>
                    <owl:onProperty rdf:resource="http://www.w3id.org/animl/ontology/extends"/>
                    <owl:allValuesFrom rdf:resource="http://www.w3id.org/animl/ontology/Technique"/>
                </owl:Restriction>
            </rdfs:subClassOf>
        </owl:Class>

        <!-- this is a subclass of definition which is identical to it, with the exception
        that it can only be present in an ATDD when extending a technique, and cannot have
        derives or consumes relations -->



            <!-- 
    ///////////////////////////////////////////////////////////////////////////////////////
    //
    // individuals
    //
    ///////////////////////////////////////////////////////////////////////////////////////
     -->

         <!-- a fundamental scientific unit -->

        <owl:NamedIndividual rdf:about="http://www.w3id.org/animl/ontology/includes">
            <rdf:type rdf:resource="http://www.w3id.org/animl/ontology/SIUnit"/>
        </owl:NamedIndividual>
        


        <!-- a data type -->

        <owl:NamedIndividual rdf:about="http://www.w3id.org/animl/ontology/boolean">
            <rdf:type rdf:resource="http://www.w3id.org/animl/ontology/DataType"/>
        </owl:NamedIndividual>
        


        <!-- a data type -->

        <owl:NamedIndividual rdf:about="http://www.w3id.org/animl/ontology/dateTime">
            <rdf:type rdf:resource="http://www.w3id.org/animl/ontology/DataType"/>
        </owl:NamedIndividual>
        


        <!-- a data type -->

        <owl:NamedIndividual rdf:about="http://www.w3id.org/animl/ontology/embeddedXML">
            <rdf:type rdf:resource="http://www.w3id.org/animl/ontology/DataType"/>
        </owl:NamedIndividual>
        


        <!-- a data type -->

        <owl:NamedIndividual rdf:about="http://www.w3id.org/animl/ontology/float32">
            <rdf:type rdf:resource="http://www.w3id.org/animl/ontology/DataType"/>
        </owl:NamedIndividual>
        


        <!-- a data type -->

        <owl:NamedIndividual rdf:about="http://www.w3id.org/animl/ontology/int32">
            <rdf:type rdf:resource="http://www.w3id.org/animl/ontology/DataType"/>
        </owl:NamedIndividual>
        


        <!-- a data type -->

        <owl:NamedIndividual rdf:about="http://www.w3id.org/animl/ontology/int64">
            <rdf:type rdf:resource="http://www.w3id.org/animl/ontology/DataType"/>
        </owl:NamedIndividual>
        


        <!-- a fundamental scientific unit -->

        <owl:NamedIndividual rdf:about="http://www.w3id.org/animl/ontology/k">
            <rdf:type rdf:resource="http://www.w3id.org/animl/ontology/SIUnit"/>
        </owl:NamedIndividual>
        


        <!-- a data type -->

        <owl:NamedIndividual rdf:about="http://www.w3id.org/animl/ontology/pNG">
            <rdf:type rdf:resource="http://www.w3id.org/animl/ontology/DataType"/>
        </owl:NamedIndividual>
        


        <!-- a data type -->

        <owl:NamedIndividual rdf:about="http://www.w3id.org/animl/ontology/sVG">
            <rdf:type rdf:resource="http://www.w3id.org/animl/ontology/DataType"/>
        </owl:NamedIndividual>
        


        <!-- a data type -->

        <owl:NamedIndividual rdf:about="http://www.w3id.org/animl/ontology/string">
            <rdf:type rdf:resource="http://www.w3id.org/animl/ontology/DataType"/>
        </owl:NamedIndividual>
        


        <!-- a fundamental scientific unit -->

        <owl:NamedIndividual rdf:about="http://www.w3id.org/animl/ontology/cD">
            <rdf:type rdf:resource="http://www.w3id.org/animl/ontology/SIUnit"/>
        </owl:NamedIndividual>


        <!-- a data type -->

        <owl:NamedIndividual rdf:about="http://www.w3id.org/animl/ontology/float64">
            <rdf:type rdf:resource="http://www.w3id.org/animl/ontology/DataType"/>
        </owl:NamedIndividual>

        <!-- a fundamental scientific unit -->

        <owl:NamedIndividual rdf:about="http://www.w3id.org/animl/ontology/kG">
            <rdf:type rdf:resource="http://www.w3id.org/animl/ontology/SIUnit"/>
        </owl:NamedIndividual>
        


        <!-- a type of graphical scale -->

        <owl:NamedIndividual rdf:about="http://www.w3id.org/animl/ontology/linear">
            <rdf:type rdf:resource="http://www.w3id.org/animl/ontology/PlotScale"/>
        </owl:NamedIndividual>
        


        <!-- a type of graphical scale -->

        <owl:NamedIndividual rdf:about="http://www.w3id.org/animl/ontology/ln">
            <rdf:type rdf:resource="http://www.w3id.org/animl/ontology/PlotScale"/>
        </owl:NamedIndividual>
        


        <!-- a type of graphical scale -->

        <owl:NamedIndividual rdf:about="http://www.w3id.org/animl/ontology/log">
            <rdf:type rdf:resource="http://www.w3id.org/animl/ontology/PlotScale"/>
        </owl:NamedIndividual>
        


        <!-- a fundamental scientific unit -->

        <owl:NamedIndividual rdf:about="http://www.w3id.org/animl/ontology/m">
            <rdf:type rdf:resource="http://www.w3id.org/animl/ontology/SIUnit"/>
        </owl:NamedIndividual>
        


        <!-- a fundamental scientific unit -->

        <owl:NamedIndividual rdf:about="http://www.w3id.org/animl/ontology/mol">
            <rdf:type rdf:resource="http://www.w3id.org/animl/ontology/SIUnit"/>
        </owl:NamedIndividual>

            <!-- an indication that a data point has no units of measurement -->

        <owl:NamedIndividual rdf:about="http://www.w3id.org/animl/ontology/none">
            <rdf:type rdf:resource="http://www.w3id.org/animl/ontology/PlotScale"/>
        </owl:NamedIndividual>

            <!-- a fundamental scientific unit -->

        <owl:NamedIndividual rdf:about="http://www.w3id.org/animl/ontology/s">
            <rdf:type rdf:resource="http://www.w3id.org/animl/ontology/SIUnit"/>
        </owl:NamedIndividual>

            <!-- a fundamental scientific unit -->

        <owl:NamedIndividual rdf:about="http://www.w3id.org/animl/ontology/1">
            <rdf:type rdf:resource="http://www.w3id.org/animl/ontology/SIUnit"/>
        </owl:NamedIndividual>

    
            <!-- 
    // ANIML_REFERENCE_PATTERN
    // ANIML_REFERENCE_PATTERN
    // ANIML_REFERENCE_PATTERN
    // ANIML_REFERENCE_PATTERN
    // ANIML_REFERENCE_PATTERN
    

     -->


     <!-- this pattern is a generalisation of the behaviour (found at multiple points in the animl xml) of classes, typically
     classes representing activities or information supporting activities, to be related by a number of methods to other classes,
     typically representing persistent data within containers, which cannot be directly related to them since they are members of indexed
     data structures or containers
     
     the core of this pattern is the reference set, and the references it contains. the reference set corresponds to a data structure in which
     all the referenced data points reside, and each reference corresponds to each data point.
     
     certain information regarding the relationship of the referenced information to the object referencing it is also reified as object properties
     with domain in the reference class.
     
     a class which references other classes includes a reference set-->

        <!--object properties-->
            <!-- this relation denotes that the referenceset in the domain contains references to data within a data structure
            of the range class -->

            <owl:ObjectProperty rdf:about="http://www.w3id.org/animl/ontology/subject">
                <rdfs:comment xml:lang="en">This relation denotes that the referenceset in the domain contains references to data within a data structure of the range class</rdfs:comment>
                <rdfs:domain rdf:resource="http://www.w3id.org/animl/ontology/ReferenceSet"/>
                <rdfs:range>
                    <owl:Class>
                        <owl:unionOf rdf:parseType="Collection">
                            <rdf:Description rdf:about="http://www.w3id.org/animl/ontology/Experiment"/>
                            <rdf:Description rdf:about="http://www.w3id.org/animl/ontology/SampleSet"/>
                            <rdf:Description rdf:about="http://www.w3id.org/animl/ontology/Series"/>
                        </owl:unionOf>
                    </owl:Class>
                </rdfs:range>
            </owl:ObjectProperty>


            <!-- this indicates that the domain reference points to something of the range class -->

            <owl:ObjectProperty rdf:about="http://www.w3id.org/animl/ontology/pointsTo">
                <rdfs:comment xml:lang="en">This indicates that the domain reference points to something of the range class</rdfs:comment>
                <rdfs:domain rdf:resource="http://www.w3id.org/animl/ontology/Reference"/>
                <rdfs:range>
                    <owl:Class>
                        <owl:unionOf rdf:parseType="Collection">
                            <rdf:Description rdf:about="http://www.w3id.org/animl/ontology/DataPoint"/>
                            <rdf:Description rdf:about="http://www.w3id.org/animl/ontology/ExperimentStep"/>
                            <rdf:Description rdf:about="http://www.w3id.org/animl/ontology/Sample"/>
                        </owl:unionOf>
                    </owl:Class>
                </rdfs:range>
            </owl:ObjectProperty>


            <!-- this relation represents a reified data property, where a reference is related to the textual description of
            the role of the data it points to, this is an optional property distinct from function and the consumes/derives relationship,
            it is used when further infromation about the purpose of the data is necessary to store  -->

            <owl:ObjectProperty rdf:about="http://www.w3id.org/animl/ontology/hasUseCase">
                <rdfs:comment xml:lang="en">This relation represents a reified data property, where a reference is related to the textual description of the role of the data it points to, this is an optional property distinct from function and the consumes/derives relationship, it is used when further infromation about the purpose of the data is necessary to store</rdfs:comment>
                <rdfs:domain rdf:resource="http://www.w3id.org/animl/ontology/Reference"/>
                <rdfs:range rdf:resource="http://www.w3id.org/animl/ontology/UseCase"/>
            </owl:ObjectProperty>

            <!-- this relation represents a reified data property, where a reference is related to the textual description of
            the function of the data it points to -->

            <owl:ObjectProperty rdf:about="http://www.w3id.org/animl/ontology/hasFunction">
                <rdfs:comment xml:lang="en">This relation represents a reified data property, where a reference is related to the textual description of the function of the data it points to</rdfs:comment>
                <rdfs:domain rdf:resource="http://www.w3id.org/animl/ontology/Reference"/>
                <rdfs:range rdf:resource="http://www.w3id.org/animl/ontology/Function"/>
            </owl:ObjectProperty>

        <!--data properties-->

            <!-- this indicates the first position in an ordered set that a contained item
            will be pointed to by a reference in the domain reference set  -->

            <owl:DatatypeProperty rdf:about="http://www.w3id.org/animl/ontology/startValue">
                <rdfs:comment xml:lang="en">This indicates the first position in an ordered set that a contained item will be pointed to by a reference in the domain reference set</rdfs:comment>
                <rdfs:domain rdf:resource="http://www.w3id.org/animl/ontology/ReferenceSet"/>
                <rdfs:range rdf:resource="http://www.w3.org/2001/XMLSchema#nonNegativeInteger"/>
            </owl:DatatypeProperty>

            <!-- this indicates the last position in an ordered set that a contained item
            will be pointed to by a reference in the domain reference set -->

            <owl:DatatypeProperty rdf:about="http://www.w3id.org/animl/ontology/endValue">
                <rdfs:comment xml:lang="en">This indicates the last position in an ordered set that a contained item will be pointed to by a reference in the domain reference set</rdfs:comment>
                <rdfs:domain rdf:resource="http://www.w3id.org/animl/ontology/ReferenceSet"/>
                <rdfs:range rdf:resource="http://www.w3.org/2001/XMLSchema#nonNegativeInteger"/>
            </owl:DatatypeProperty>

        <!--objects-->

            <!-- this is a reference set as discussed in the header for this odp, note that it can only look
            within one data structure -->
            <owl:Class rdf:about="http://www.w3id.org/animl/ontology/ReferenceSet">
                <rdfs:comment xml:lang="en">This is a reference set as discussed in the header for this odp, note that it can only look within one data structure</rdfs:comment>
                <rdfs:subClassOf>
                    <owl:Restriction>
                        <owl:onProperty rdf:resource="http://www.w3id.org/animl/ontology/subject"/>
                        <owl:allValuesFrom>
                            <owl:Class>
                                <owl:unionOf rdf:parseType="Collection">
                                    <rdf:Description rdf:about="http://www.w3id.org/animl/ontology/Series"/>
                                    <rdf:Description rdf:about="http://www.w3id.org/animl/ontology/Experiment"/>
                                    <rdf:Description rdf:about="http://www.w3id.org/animl/ontology/SampleSet"/>
                                </owl:unionOf>
                            </owl:Class>
                        </owl:allValuesFrom>
                    </owl:Restriction>
                </rdfs:subClassOf>

            <!-- Max cardinality restriction -->
                <rdfs:subClassOf>
                    <owl:Restriction>
                        <owl:onProperty rdf:resource="http://www.w3id.org/animl/ontology/pointsTo"/>
                        <owl:maxCardinality rdf:datatype="http://www.w3.org/2001/XMLSchema#nonNegativeInteger">1</owl:maxCardinality>
                    </owl:Restriction>
                </rdfs:subClassOf>

                <rdfs:subClassOf>
                    <owl:Restriction>
                        <owl:onProperty rdf:resource="http://www.ontologydesignpatterns.org/cp/owl/collectionentity.owl#hasMember"/>
                        <owl:allValuesFrom rdf:resource="http://www.w3id.org/animl/ontology/Reference"/>
                    </owl:Restriction>
                </rdfs:subClassOf>
            </owl:Class>

            <!-- this is a referenec as discussed in the header for this odp, note that it can
            only point to one piece of data -->
            <owl:Class rdf:about="http://www.w3id.org/animl/ontology/Reference">
                <rdfs:comment xml:lang="en">This is a reference for the odp, note that it can only point to one piece of data</rdfs:comment>
                <rdfs:subClassOf>
                    <owl:Restriction>
                        <owl:onProperty rdf:resource="http://www.w3id.org/animl/ontology/hasFunction"/>
                        <owl:allValuesFrom rdf:resource="http://www.w3id.org/animl/ontology/Function"/>
                    </owl:Restriction>
                </rdfs:subClassOf>
                <rdfs:subClassOf>
                    <owl:Restriction>
                        <owl:onProperty rdf:resource="http://www.w3id.org/animl/ontology/hasSpecification"/>
                        <owl:allValuesFrom rdf:resource="http://www.w3id.org/animl/ontology/ReferenceSpecification"/>
                    </owl:Restriction>
                </rdfs:subClassOf>
                <rdfs:subClassOf>
                    <owl:Restriction>
                        <owl:onProperty rdf:resource="http://www.w3id.org/animl/ontology/hasUseCase"/>
                        <owl:allValuesFrom rdf:resource="http://www.w3id.org/animl/ontology/UseCase"/>
                    </owl:Restriction>
                </rdfs:subClassOf>

                <!-- Combined allValuesFrom restriction using owl:unionOf -->
                <rdfs:subClassOf>
                    <owl:Restriction>
                        <owl:onProperty rdf:resource="http://www.w3id.org/animl/ontology/pointsTo"/>
                        <owl:allValuesFrom>
                            <owl:Class>
                                <owl:unionOf rdf:parseType="Collection">
                                    <rdf:Description rdf:about="http://www.w3id.org/animl/ontology/DataPoint"/>
                                    <rdf:Description rdf:about="http://www.w3id.org/animl/ontology/ExperimentStep"/>
                                    <rdf:Description rdf:about="http://www.w3id.org/animl/ontology/Sample"/>
                                </owl:unionOf>
                            </owl:Class>
                        </owl:allValuesFrom>
                    </owl:Restriction>
                </rdfs:subClassOf>


                <!-- Max cardinality restriction -->
                <rdfs:subClassOf>
                    <owl:Restriction>
                        <owl:onProperty rdf:resource="http://www.w3id.org/animl/ontology/pointsTo"/>
                        <owl:maxCardinality rdf:datatype="http://www.w3.org/2001/XMLSchema#nonNegativeInteger">1</owl:maxCardinality>
                    </owl:Restriction>
                </rdfs:subClassOf>

                <rdfs:subClassOf>
                    <owl:Restriction>
                        <owl:onProperty rdf:resource="http://www.ontologydesignpatterns.org/cp/owl/collectionentity.owl#isMemberOf"/>
                        <owl:allValuesFrom rdf:resource="http://www.w3id.org/animl/ontology/ReferenceSet"/>
                    </owl:Restriction>
                </rdfs:subClassOf>
            </owl:Class>
            
            <!-- this is a reified natural language field for the use case of a set of referenced datapoints  -->
            <owl:Class rdf:about="http://www.w3id.org/animl/ontology/UseCase">
                <rdfs:comment xml:lang="en">This is a reified natural language field for the use case of a set of referenced datapoints</rdfs:comment>
            </owl:Class>


            <!-- this is a reified natural language field for the 'function' of data when being referenced
            this is optional and works to distinguish the general purpose of data from its immediate use
            
            this is an artefact from the construction of owl that has been left in to avoid damaging expressivity -->
            <owl:Class rdf:about="http://www.w3id.org/animl/ontology/Function">
                <rdfs:comment xml:lang="en">This is a reified natural language field for the 'function' of data when being referenced this is optional and works to distinguish the general purpose of data from its immediate use this is an artefact from the construction of owl that has been left in to avoid damaging expressivity</rdfs:comment>
            </owl:Class>
</rdf:RDF>
