@prefix : <http://purl.allotrope.org/voc/afo/domain/REC/2025/06/dynamic-vapor-sorption#> .
@prefix qb: <http://purl.org/linked-data/cube#> .
@prefix ro: <http://purl.obolibrary.org/obo/RO> .
@prefix bfo: <http://purl.obolibrary.org/obo/BFO> .
@prefix dct: <http://purl.org/dc/terms/> .
@prefix owl: <http://www.w3.org/2002/07/owl#> .
@prefix rdf: <http://www.w3.org/1999/02/22-rdf-syntax-ns#> .
@prefix xml: <http://www.w3.org/XML/1998/namespace> .
@prefix xsd: <http://www.w3.org/2001/XMLSchema#> .
@prefix af-c: <http://purl.allotrope.org/ontologies/common#> .
@prefix af-e: <http://purl.allotrope.org/ontologies/equipment#> .
@prefix af-m: <http://purl.allotrope.org/ontologies/material#> .
@prefix af-p: <http://purl.allotrope.org/ontologies/process#> .
@prefix af-q: <http://purl.allotrope.org/ontologies/quality#> .
@prefix af-r: <http://purl.allotrope.org/ontologies/result#> .
@prefix af-x: <http://purl.allotrope.org/ontologies/property#> .
@prefix foaf: <http://xmlns.com/foaf/0.1/> .
@prefix pato: <http://purl.obolibrary.org/obo/PATO> .
@prefix rdfs: <http://www.w3.org/2000/01/rdf-schema#> .
@prefix skos: <http://www.w3.org/2004/02/skos/core#> .
@prefix af-re: <http://purl.allotrope.org/ontologies/realizable#> .
@prefix af-rl: <http://purl.allotrope.org/ontologies/role#> .
@prefix af-cur: <http://purl.allotrope.org/ontologies/curation#> .
@base <http://purl.allotrope.org/voc/afo/domain/REC/2025/06/dynamic-vapor-sorption#> .

<http://purl.allotrope.org/voc/afo/domain/REC/2025/06/dynamic-vapor-sorption> rdf:type owl:Ontology ;
                                                                                         owl:versionIRI <http://purl.allotrope.org/voc/afo/domain/REC/2025/06/dynamic-vapor-sorption> ;
                                                                                         owl:imports <http://purl.allotrope.org/voc/afo/REC/2025/06/afo> ;
                                                                                         dct:contributor <http://www.allotrope.org> ;
                                                                                         dct:issued "2025-06-25T12:00:00Z"^^xsd:dateTime ;
                                                                                         dct:license <http://purl.allotrope.org/voc/creative-commons-attribution-license> ;
                                                                                         dct:modified "2025-04-04T12:00:00Z"^^xsd:dateTime ;
                                                                                         dct:publisher <http://www.allotrope.org> ;
                                                                                         dct:rights <http://purl.allotrope.org/voc/attribution> ,
                                                                                                    <http://purl.allotrope.org/voc/copyright> ;
                                                                                         dct:rightsHolder <http://www.allotrope.org> ;
                                                                                         dct:title "AFO Dynamic Vapor Sorption Domain Ontology (REC/2025/06)" ;
                                                                                         owl:priorVersion <http://purl.allotrope.org/voc/afo/domain/REC/2025/03/dynamic-vapor-sorption> ;
                                                                                         owl:versionInfo "REC/2025/06" .

#################################################################
#    Classes
#################################################################

###  http://purl.allotrope.org/ontologies/process#AFP_0003765
af-p:AFP_0003765 rdf:type owl:Class ;
                 rdfs:subClassOf af-p:AFP_0002294 ;
                 dct:source <https://en.wikipedia.org/wiki/Dynamic_vapor_sorption> ;
                 skos:altLabel "DVS" ;
                 skos:definition "Dynamic vapor sorption is a gravimetric technique that measures how quickly and how much of a solvent is absorbed by a sample. It does this by varying the vapor concentration surrounding the sample and measuring the change in mass which this produces. [Wikipedia]" ;
                 skos:prefLabel "dynamic vapor sorption" .


###  http://purl.allotrope.org/ontologies/realizable#AFRE_0000019
af-re:AFRE_0000019 rdf:type owl:Class ;
                   rdfs:subClassOf af-re:AFRE_0000004 ,
                                   [ rdf:type owl:Restriction ;
                                     owl:onProperty bfo:_0000054 ;
                                     owl:someValuesFrom bfo:_0000182
                                   ] ;
                   dct:source <https://en.wikipedia.org/wiki/Hysteresis> ;
                   skos:definition "Hysteresis is the time-based dependence of a system's output on present and past inputs. The dependence arises because the history affects the value of an internal state. To predict its future outputs, either its internal state or its history must be known. [Wikipedia]" ;
                   skos:prefLabel "hysteresis" .


###  http://purl.allotrope.org/ontologies/result#AFR_0002143
af-r:AFR_0002143 rdf:type owl:Class ;
                 rdfs:subClassOf af-r:AFR_0001277 ,
                                 [ rdf:type owl:Restriction ;
                                   owl:onProperty af-x:AFX_0002801 ;
                                   owl:someValuesFrom af-r:AFR_0002552
                                 ] ;
                 skos:altLabel "hygroscopicity per E.U" ;
                 skos:definition "A hygroscopicity type is a classification datum that classifies the hygroscopicity of a material due to moisture sorption at 25°C and 80% relative humidity. [Allotrope]" ;
                 skos:prefLabel "hygroscopicity type" .


###  http://purl.allotrope.org/ontologies/result#AFR_0002144
af-r:AFR_0002144 rdf:type owl:Class ;
                 rdfs:subClassOf af-r:AFR_0001836 ;
                 skos:definition "A hysteresis assessment is an assessment about the hysteresis observed in a cyclic experiment. [Allotrope]" ;
                 skos:prefLabel "hysteresis assessment" .


###  http://purl.allotrope.org/ontologies/result#AFR_0002145
af-r:AFR_0002145 rdf:type owl:Class ;
                 rdfs:subClassOf qb:DataSet ;
                 skos:definition "A vapor sorption data cube is a data cube that is a representation of a vapor sorption experimental result. [Allotrope]" ;
                 skos:prefLabel "vapor sorption data cube" .


###  http://purl.allotrope.org/ontologies/result#AFR_0002146
af-r:AFR_0002146 rdf:type owl:Class ;
                 rdfs:subClassOf af-r:AFR_0001505 ;
                 skos:definition "A target P/P0 setting is a setting to set the relative pressure of a vapor. [Allotrope]" ;
                 skos:prefLabel "target P/P0 setting" .


###  http://purl.allotrope.org/ontologies/result#AFR_0002147
af-r:AFR_0002147 rdf:type owl:Class ;
                 rdfs:subClassOf af-r:AFR_0001583 ;
                 skos:definition "An actual P/P0 result is a quality quantification facet that quantifies the relative pressure of the sample. [Allotrope]" ;
                 skos:prefLabel "actual P/P0 result" .


###  http://purl.allotrope.org/ontologies/result#AFR_0002152
af-r:AFR_0002152 rdf:type owl:Class ;
                 rdfs:subClassOf af-r:AFR_0001881 ,
                                 [ rdf:type owl:Restriction ;
                                   owl:onProperty af-x:AFX_0002816 ;
                                   owl:someValuesFrom [ owl:intersectionOf ( [ rdf:type owl:Restriction ;
                                                                               owl:onProperty af-x:AFX_0002730 ;
                                                                               owl:someValuesFrom af-rl:AFRL_0000250
                                                                             ]
                                                                             [ rdf:type owl:Restriction ;
                                                                               owl:onProperty af-x:AFX_0002803 ;
                                                                               owl:someValuesFrom [ owl:intersectionOf ( af-r:AFR_0002154
                                                                                                                         [ rdf:type owl:Restriction ;
                                                                                                                           owl:onProperty af-x:AFX_0002730 ;
                                                                                                                           owl:someValuesFrom af-rl:AFRL_0000478
                                                                                                                         ]
                                                                                                                       ) ;
                                                                                                    rdf:type owl:Class
                                                                                                  ]
                                                                             ]
                                                                             [ rdf:type owl:Restriction ;
                                                                               owl:onProperty af-x:AFX_0002803 ;
                                                                               owl:someValuesFrom [ owl:intersectionOf ( af-r:AFR_0002156
                                                                                                                         [ rdf:type owl:Restriction ;
                                                                                                                           owl:onProperty af-x:AFX_0002730 ;
                                                                                                                           owl:someValuesFrom af-rl:AFRL_0000478
                                                                                                                         ]
                                                                                                                       ) ;
                                                                                                    rdf:type owl:Class
                                                                                                  ]
                                                                             ]
                                                                           ) ;
                                                        rdf:type owl:Class
                                                      ]
                                 ] ;
                 skos:definition "A total gas flow rate is a flow rate that quantifies the motion of the sum of the dry and saturated gas over time. [Allotrope]" ;
                 skos:prefLabel "total gas flow rate" .


###  http://purl.allotrope.org/ontologies/result#AFR_0002153
af-r:AFR_0002153 rdf:type owl:Class ;
                 rdfs:subClassOf af-r:AFR_0001243 ,
                                 [ rdf:type owl:Restriction ;
                                   owl:onProperty af-x:AFX_0002704 ;
                                   owl:someValuesFrom [ rdf:type owl:Restriction ;
                                                        owl:onProperty ro:_0000087 ;
                                                        owl:someValuesFrom af-rl:AFRL_0000531
                                                      ]
                                 ] ;
                 skos:definition "A saturated gas flow rate setting is a setting that specifies the target saturated gas flow rate. [Allotrope]" ;
                 skos:prefLabel "saturated gas flow rate setting" .


###  http://purl.allotrope.org/ontologies/result#AFR_0002154
af-r:AFR_0002154 rdf:type owl:Class ;
                 rdfs:subClassOf af-r:AFR_0001881 ,
                                 [ rdf:type owl:Restriction ;
                                   owl:onProperty af-x:AFX_0002816 ;
                                   owl:someValuesFrom [ rdf:type owl:Restriction ;
                                                        owl:onProperty ro:_0000087 ;
                                                        owl:someValuesFrom af-rl:AFRL_0000531
                                                      ]
                                 ] ;
                 skos:definition "A saturated gas flow rate is a flow rate that quantifies the motion of the saturated gas over time. [Allotrope]" ;
                 skos:prefLabel "saturated gas flow rate" .


###  http://purl.allotrope.org/ontologies/result#AFR_0002155
af-r:AFR_0002155 rdf:type owl:Class ;
                 rdfs:subClassOf af-r:AFR_0001243 ,
                                 [ rdf:type owl:Restriction ;
                                   owl:onProperty af-x:AFX_0002704 ;
                                   owl:someValuesFrom [ rdf:type owl:Restriction ;
                                                        owl:onProperty ro:_0000087 ;
                                                        owl:someValuesFrom af-rl:AFRL_0000530
                                                      ]
                                 ] ;
                 skos:definition "A dry gas flow rate setting is a setting that specifies the target dry gas flow rate. [Allotrope]" ;
                 skos:prefLabel "dry gas flow rate setting" .


###  http://purl.allotrope.org/ontologies/result#AFR_0002156
af-r:AFR_0002156 rdf:type owl:Class ;
                 rdfs:subClassOf af-r:AFR_0001881 ,
                                 [ rdf:type owl:Restriction ;
                                   owl:onProperty af-x:AFX_0002816 ;
                                   owl:someValuesFrom [ rdf:type owl:Restriction ;
                                                        owl:onProperty ro:_0000087 ;
                                                        owl:someValuesFrom af-rl:AFRL_0000530
                                                      ]
                                 ] ;
                 skos:definition "A dry gas flow rate is a flow rate that quantifies the motion of the dry gas over time. [Allotrope]" ;
                 skos:prefLabel "dry gas flow rate" .


###  http://purl.allotrope.org/ontologies/result#AFR_0002158
af-r:AFR_0002158 rdf:type owl:Class ;
                 rdfs:subClassOf af-r:AFR_0001918 ,
                                 [ rdf:type owl:Restriction ;
                                   owl:onProperty af-x:AFX_0002816 ;
                                   owl:someValuesFrom [ rdf:type owl:Restriction ;
                                                        owl:onProperty ro:_0000087 ;
                                                        owl:someValuesFrom af-rl:AFRL_0000532
                                                      ]
                                 ] ;
                 skos:definition "An inlet gas pressure is a quality qualification facet that quantifies the pressure of the inlet gas. [Allotrope]" ;
                 skos:prefLabel "inlet gas pressure" .


###  http://purl.allotrope.org/ontologies/result#AFR_0002159
af-r:AFR_0002159 rdf:type owl:Class ;
                 rdfs:subClassOf af-r:AFR_0001881 ,
                                 [ rdf:type owl:Restriction ;
                                   owl:onProperty af-x:AFX_0002816 ;
                                   owl:someValuesFrom [ rdf:type owl:Restriction ;
                                                        owl:onProperty ro:_0000087 ;
                                                        owl:someValuesFrom af-rl:AFRL_0000529
                                                      ]
                                 ] ;
                 skos:definition "An exhaust gas flow rate is a flow rate that quantifies the flow rate of the exhaust gas. [Allotrope]" ;
                 skos:prefLabel "exhaust gas flow rate" .


###  http://purl.allotrope.org/ontologies/result#AFR_0002552
af-r:AFR_0002552 rdf:type owl:Class ;
                 rdfs:subClassOf af-c:AFC_0000050 ,
                                 [ rdf:type owl:Restriction ;
                                   owl:onProperty af-x:AFX_0002806 ;
                                   owl:someValuesFrom af-q:AFQ_0000279
                                 ] ;
                 skos:definition "A hygroscopicity code is a code that indicates a range of hygroscopicity. [Allotrope]" ;
                 skos:prefLabel "hygroscopicity code" .


###  http://purl.allotrope.org/ontologies/role#AFRL_0000528
af-rl:AFRL_0000528 rdf:type owl:Class ;
                   rdfs:subClassOf bfo:_0000023 ,
                                   [ rdf:type owl:Restriction ;
                                     owl:onProperty bfo:_0000054 ;
                                     owl:someValuesFrom af-p:AFP_0003765
                                   ] ;
                   skos:definition "A dynamic vapor sorption role is a role that is realized in some dynamic vapor sorption process. [Allotrope]" ;
                   skos:prefLabel "dynamic vapor sorption role" .


###  http://purl.allotrope.org/ontologies/role#AFRL_0000529
af-rl:AFRL_0000529 rdf:type owl:Class ;
                   rdfs:subClassOf af-rl:AFRL_0000528 ,
                                   [ rdf:type owl:Restriction ;
                                     owl:onProperty ro:_0000081 ;
                                     owl:someValuesFrom af-m:AFM_0000154
                                   ] ;
                   skos:altLabel "exhaust gas" ,
                                 "exhaust gas role" ;
                   skos:definition "An exhaust gas role is the role of the waste gas exhausted from the system in the dynamic vapor sorption process. [Allotrope]" ;
                   skos:prefLabel "exhaust gas role (DVS)" .


###  http://purl.allotrope.org/ontologies/role#AFRL_0000530
af-rl:AFRL_0000530 rdf:type owl:Class ;
                   rdfs:subClassOf af-rl:AFRL_0000528 ,
                                   [ rdf:type owl:Restriction ;
                                     owl:onProperty ro:_0000081 ;
                                     owl:someValuesFrom af-m:AFM_0000154
                                   ] ;
                   skos:altLabel "dry gas" ,
                                 "dry gas role" ;
                   skos:definition "A dry gas role is the role of the gas devoid of the vapor in the dynamic vapor sorption process. [Allotrope]" ;
                   skos:prefLabel "dry gas role (DVS)" .


###  http://purl.allotrope.org/ontologies/role#AFRL_0000531
af-rl:AFRL_0000531 rdf:type owl:Class ;
                   rdfs:subClassOf af-rl:AFRL_0000528 ,
                                   [ rdf:type owl:Restriction ;
                                     owl:onProperty ro:_0000081 ;
                                     owl:someValuesFrom af-m:AFM_0000154
                                   ] ;
                   skos:altLabel "saturated gas" ,
                                 "saturated gas role" ;
                   skos:definition "A saturated gas role is the role of the gas saturated with the vapor in a dynamic vapor sorption process. [Allotrope]" ;
                   skos:prefLabel "saturated gas role (DVS)" .


###  http://purl.allotrope.org/ontologies/role#AFRL_0000532
af-rl:AFRL_0000532 rdf:type owl:Class ;
                   rdfs:subClassOf af-rl:AFRL_0000528 ;
                   skos:altLabel "inlet gas" ,
                                 "inlet gas role" ;
                   skos:definition "An inlet gas role is the role of the gas led into the system in the dynamic vapor sorption process. [Allotrope]" ;
                   skos:prefLabel "inlet gas role (DVS)" .


###  http://purl.org/linked-data/cube#DataSet
qb:DataSet rdf:type owl:Class .


#################################################################
#    Individuals
#################################################################

###  http://www.allotrope.org
<http://www.allotrope.org> rdf:type owl:NamedIndividual ,
                                    foaf:Organization ;
                           foaf:name "Allotrope Foundation" .


###  http://purl.allotrope.org/ontologies/result#AFR_0002172
af-r:AFR_0002172 rdf:type owl:NamedIndividual ,
                          af-r:AFR_0002552 ;
                 skos:changeNote "2021-09-29 Moved under hygroscopicity code. [Allotrope]" ;
                 skos:definition "Hygroscopic is a hygroscopicity type that denotes the increase in mass as equal to or greater than 2% and less than 15%. [Allotrope]" ;
                 skos:prefLabel "hygroscopic" .


###  http://purl.allotrope.org/ontologies/result#AFR_0002173
af-r:AFR_0002173 rdf:type owl:NamedIndividual ,
                          af-r:AFR_0002552 ;
                 skos:changeNote "2021-09-29 Moved under hygroscopicity code. [Allotrope]" ;
                 skos:definition "Slightly hygroscopic is a hygroscopicity type that denotes the increase in mass as equal to or greater than 0.2% and less than 2%. [Allotrope]" ;
                 skos:prefLabel "slightly hygroscopic" .


###  http://purl.allotrope.org/ontologies/result#AFR_0002174
af-r:AFR_0002174 rdf:type owl:NamedIndividual ,
                          af-r:AFR_0002552 ;
                 skos:changeNote "2021-09-29 Moved under hygroscopicity code. [Allotrope]" ;
                 skos:definition "Non-hygroscopic is a hygroscopicity type that denotes the increase in mass as no greater than 0.2%. [Allotrope]" ;
                 skos:prefLabel "non-hygroscopic" .


###  http://purl.allotrope.org/ontologies/result#AFR_0002200
af-r:AFR_0002200 rdf:type owl:NamedIndividual ,
                          af-r:AFR_0002552 ;
                 skos:changeNote "2021-09-29 Moved under hygroscopicity code. [Allotrope]" ;
                 skos:definition "Deliquescent is a hygroscopicity type that denotes the substance as sufficiently absorbant to form a liquid. [Allotrope]" ;
                 skos:prefLabel "deliquescent" .


###  http://purl.allotrope.org/ontologies/result#AFR_0002201
af-r:AFR_0002201 rdf:type owl:NamedIndividual ,
                          af-r:AFR_0002552 ;
                 skos:changeNote "2021-09-29 Moved under hygroscopicity code. [Allotrope]" ;
                 skos:definition "Very hygroscopic is a hygroscopicity type that denotes the increase in mass as equal to or greater than 15%. [Allotrope]" ;
                 skos:prefLabel "very hygroscopic" .


###  http://purl.allotrope.org/voc/attribution
<http://purl.allotrope.org/voc/attribution> rdf:type owl:NamedIndividual ,
                                                     dct:RightsStatement ;
                                            dct:description """
These taxonomies contain material or may constitute derivative works of material which may be subject to copyright by one of the following organizations.  By using these taxonomies, you agree to the following terms and conditions applicable to its contents:
******************************************************************************
Copyright Notice and Terms for IUPAC Gold Book
______________________________________________________________________________
Copyright © 1998, Regents of the University of California
All rights reserved.
Redistribution and use in source and binary forms, with or without modification, are permitted provided that the following conditions are met:
1. Redistributions of source code must retain the above copyright notice, this list of conditions and the following disclaimer.
2. Redistributions in binary form must reproduce the above copyright notice, this list of conditions and the following disclaimer in the documentation and/or other materials provided with the distribution.
THIS SOFTWARE IS PROVIDED BY THE COPYRIGHT HOLDERS AND CONTRIBUTORS \"AS IS\" AND ANY EXPRESS OR IMPLIED WARRANTIES, INCLUDING, BUT NOT LIMITED TO, THE IMPLIED WARRANTIES OF MERCHANTABILITY AND FITNESS FOR A PARTICULAR PURPOSE ARE DISCLAIMED. IN NO EVENT SHALL THE COPYRIGHT HOLDER OR CONTRIBUTORS BE LIABLE FOR ANY DIRECT, INDIRECT, INCIDENTAL, SPECIAL, EXEMPLARY, OR CONSEQUENTIAL DAMAGES (INCLUDING, BUT NOT LIMITED TO, PROCUREMENT OF SUBSTITUTE GOODS OR SERVICES; LOSS OF USE, DATA, OR PROFITS; OR BUSINESS INTERRUPTION) HOWEVER CAUSED AND ON ANY THEORY OF LIABILITY, WHETHER IN CONTRACT, STRICT LIABILITY, OR TORT (INCLUDING NEGLIGENCE OR OTHERWISE) ARISING IN ANY WAY OUT OF THE USE OF THIS SOFTWARE, EVEN IF ADVISED OF THE POSSIBILITY OF SUCH DAMAGE.
******************************************************************************
Copyright Notice and Terms for PSI-MS (Proteomics Standards Initiative - Mass Spectrometry) Mass spectrometer output files and spectra interpretation
_____________________________________________________________________________
Created by Matt Chambers, Andreas Bertsch, Marius Kallhardt, Eric Deutsch Fredrik Levander, Pierre-Alain Binz, and Gerhard Mayer. Publisher: HUPO Proteomics Standards Initiative Mass Spectrometry Standards Working Group and HUPO Proteomics Standards Initiative Proteomics Informatics Working Group. This work is used pursuant to a Creative Commons license available here: http://creativecommons.org/licenses/by/3.0/legalcode

******************************************************************************
Attribution Notice for National Center for Biomedical Ontology materials.

This work contains material from the Cell Ontology and Clinical Measurement Ontology, available here: http://bioportal.bioontology.org/.
******************************************************************************
Attribution Notice for ChEBI
This work contains material from the European Bioinformatics Institute’s ChEBI database.
******************************************************************************
Attribution Notice for Quantities Units Dimensions Data Types (http://www.qudt.org/)
This work contains content from www.qudt.org and is used pursuant to a Creative Commons License available here: http://creativecommons.org/licenses/by-sa/3.0/us/legalcode. The original work may have been modified.
******************************************************************************
Copyright and Attribution Notice for Dublin Core Metadata Initiative Document
This work contains material from the following DCMI document used pursuant to a creative commons license available here: https://creativecommons.org/licenses/by/4.0/legalcode. This material may have been modified or changed.
Timestamped URL:          http://dublincore.org/documents/2012/06/14/dcmi-terms/
Date Issued:                       2012-06-14
Document Status:            This is a DCMI Recommendation.
Copyright © 1995-2015 DCMI. All Rights Reserved. DCMI liability, trademark/service mark, document use and software licensing rules apply.
******************************************************************************

""" ;
                                            dct:title "Derivative works attribution" .


###  http://purl.allotrope.org/voc/copyright
<http://purl.allotrope.org/voc/copyright> rdf:type owl:NamedIndividual ,
                                                   dct:RightsStatement ;
                                          dct:description "Copyright © 2015-2025 Allotrope Foundation" ;
                                          dct:rightsHolder <http://www.allotrope.org> ;
                                          dct:title "Copyright © 2015-2025 Allotrope Foundation" .


###  http://purl.allotrope.org/voc/creative-commons-attribution-license
<http://purl.allotrope.org/voc/creative-commons-attribution-license> rdf:type owl:NamedIndividual ,
                                                                              dct:LicenseDocument ;
                                                                     dct:description """This work is licensed under a Creative Commons Attribution 4.0 International License http://creativecommons.org/licenses/by/4.0/.

THESE MATERIALS ARE PROVIDED \"AS IS\" AND ALLOTROPE EXPRESSLY DISCLAIMS ALL WARRANTIES, EXPRESS, IMPLIED OR STATUTORY, INCLUDING, WITHOUT LIMITATION, THE WARRANTIES OF NON-INFRINGEMENT, TITLE, MERCHANTABILITY AND FITNESS FOR A PARTICULAR PURPOSE.

Copyright © 2015-2025 Allotrope Foundation
""" ;
                                                                     dct:rightsHolder <http://www.allotrope.org> ;
                                                                     dct:title "Creative Commons Attribution 4.0 International Public License" .


###  Generated by the OWL API (version 5.1.19) https://github.com/owlcs/owlapi/
