@prefix : <http://purl.allotrope.org/voc/afo/domain/REC/2025/06/ir#> .
@prefix dct: <http://purl.org/dc/terms/> .
@prefix owl: <http://www.w3.org/2002/07/owl#> .
@prefix rdf: <http://www.w3.org/1999/02/22-rdf-syntax-ns#> .
@prefix xml: <http://www.w3.org/XML/1998/namespace> .
@prefix xsd: <http://www.w3.org/2001/XMLSchema#> .
@prefix af-c: <http://purl.allotrope.org/ontologies/common#> .
@prefix af-e: <http://purl.allotrope.org/ontologies/equipment#> .
@prefix af-m: <http://purl.allotrope.org/ontologies/material#> .
@prefix af-p: <http://purl.allotrope.org/ontologies/process#> .
@prefix af-q: <http://purl.allotrope.org/ontologies/quality#> .
@prefix af-r: <http://purl.allotrope.org/ontologies/result#> .
@prefix af-x: <http://purl.allotrope.org/ontologies/property#> .
@prefix foaf: <http://xmlns.com/foaf/0.1/> .
@prefix rdfs: <http://www.w3.org/2000/01/rdf-schema#> .
@prefix skos: <http://www.w3.org/2004/02/skos/core#> .
@prefix af-cur: <http://purl.allotrope.org/ontologies/curation#> .
@base <http://purl.allotrope.org/voc/afo/domain/REC/2025/06/ir#> .

<http://purl.allotrope.org/voc/afo/domain/REC/2025/06/ir> rdf:type owl:Ontology ;
                                                                     owl:versionIRI <http://purl.allotrope.org/voc/afo/domain/REC/2025/06/ir> ;
                                                                     owl:imports <http://purl.allotrope.org/voc/afo/REC/2025/06/afo> ,
                                                                                 <http://purl.allotrope.org/voc/qb/REC/2018/10/cube> ;
                                                                     dct:contributor <http://www.allotrope.org> ;
                                                                     dct:issued "2025-06-25T12:00:00Z"^^xsd:dateTime ;
                                                                     dct:license <http://purl.allotrope.org/voc/creative-commons-attribution-license> ;
                                                                     dct:modified "2025-04-04T12:00:00Z"^^xsd:dateTime ;
                                                                     dct:publisher <http://www.allotrope.org> ;
                                                                     dct:rights <http://purl.allotrope.org/voc/attribution> ,
                                                                                <http://purl.allotrope.org/voc/copyright> ;
                                                                     dct:rightsHolder <http://www.allotrope.org> ;
                                                                     dct:title "AFO Infrared (IR) Domain Ontology (REC/2025/06)" ;
                                                                     owl:priorVersion <http://purl.allotrope.org/voc/afo/domain/REC/2025/03/ir> ;
                                                                     owl:versionInfo "REC/2025/06" .

#################################################################
#    Annotation properties
#################################################################

###  http://purl.allotrope.org/ontologies/property#AFX_0002796
af-x:AFX_0002796 rdf:type owl:AnnotationProperty .


###  http://purl.allotrope.org/ontologies/property#AFX_0002798
af-x:AFX_0002798 rdf:type owl:AnnotationProperty .


###  http://purl.allotrope.org/ontologies/property#AFX_0002809
af-x:AFX_0002809 rdf:type owl:AnnotationProperty .


###  http://purl.org/dc/terms/source
dct:source rdf:type owl:AnnotationProperty .


###  http://www.w3.org/2004/02/skos/core#altLabel
skos:altLabel rdf:type owl:AnnotationProperty .


###  http://www.w3.org/2004/02/skos/core#changeNote
skos:changeNote rdf:type owl:AnnotationProperty .


###  http://www.w3.org/2004/02/skos/core#definition
skos:definition rdf:type owl:AnnotationProperty .


###  http://www.w3.org/2004/02/skos/core#example
skos:example rdf:type owl:AnnotationProperty .


###  http://www.w3.org/2004/02/skos/core#note
skos:note rdf:type owl:AnnotationProperty .


###  http://www.w3.org/2004/02/skos/core#prefLabel
skos:prefLabel rdf:type owl:AnnotationProperty .


###  http://www.w3.org/2004/02/skos/core#scopeNote
skos:scopeNote rdf:type owl:AnnotationProperty .


#################################################################
#    Classes
#################################################################

###  http://purl.allotrope.org/ontologies/result#AFR_0002057
af-r:AFR_0002057 rdf:type owl:Class ;
                 rdfs:subClassOf af-r:AFR_0000992 ,
                                 af-r:AFR_0002105 ,
                                 <http://purl.org/linked-data/cube#DataSet> ,
                                 [ rdf:type owl:Restriction ;
                                   owl:onProperty [ owl:inverseOf af-x:AFX_0002737
                                                  ] ;
                                   owl:someValuesFrom af-r:AFR_0002103
                                 ] ;
                 skos:definition "An infrared interferogram data cube is a data cube that is a representation of an infrared interferogram. [Allotrope]" ;
                 skos:prefLabel "infrared interferogram data cube" .


###  http://purl.allotrope.org/ontologies/result#AFR_0002058
af-r:AFR_0002058 rdf:type owl:Class ;
                 rdfs:subClassOf af-r:AFR_0000992 ,
                                 af-r:AFR_0002105 ,
                                 <http://purl.org/linked-data/cube#DataSet> ,
                                 [ rdf:type owl:Restriction ;
                                   owl:onProperty [ owl:inverseOf af-x:AFX_0002737
                                                  ] ;
                                   owl:someValuesFrom af-r:AFR_0000251
                                 ] ;
                 skos:definition "An infrared spectrum data cube is a data cube that is a representation of an infrared spectrum. [Allotrope]" ;
                 skos:prefLabel "infrared spectrum data cube" .


###  http://purl.allotrope.org/ontologies/result#AFR_0002070
af-r:AFR_0002070 rdf:type owl:Class ;
                 rdfs:subClassOf <http://purl.obolibrary.org/obo/IAO_0000310> ,
                                 [ rdf:type owl:Restriction ;
                                   owl:onProperty <http://purl.obolibrary.org/obo/IAO_0000136> ;
                                   owl:someValuesFrom af-p:AFP_0001787
                                 ] ;
                 skos:altLabel "FTIR document" ,
                               "FTIR result" ,
                               "Fourier transform infrared result" ;
                 skos:definition "A FTIR document is a document that encompasses the information associated with a Fourier Transform Infrared Spectroscopic run. [Allotrope]" ;
                 skos:prefLabel "Fourier transform infrared document" .


###  http://purl.allotrope.org/ontologies/result#AFR_0002251
af-r:AFR_0002251 rdf:type owl:Class ;
                 rdfs:subClassOf af-r:AFR_0001505 ;
                 skos:definition "An optical velocity setting is a setting that specifies the velocity of the moving mirror during the run. [Allotrope]" ;
                 skos:prefLabel "optical velocity setting" .


###  http://purl.allotrope.org/ontologies/result#AFR_0002326
af-r:AFR_0002326 rdf:type owl:Class ;
                 rdfs:subClassOf <http://purl.obolibrary.org/obo/IAO_0000310> ,
                                 [ rdf:type owl:Restriction ;
                                   owl:onProperty <http://purl.obolibrary.org/obo/IAO_0000136> ;
                                   owl:someValuesFrom af-p:AFP_0001787
                                 ] ;
                 skos:altLabel "NIR document" ,
                               "near infra-red document" ,
                               "near-infrared document" ;
                 skos:definition "A near infrared document is a document that encompasses the information associated with a near-infrared spectroscopy process. [Allotrope]" ;
                 skos:prefLabel "near infrared document" .


###  http://purl.allotrope.org/ontologies/result#AFR_0002327
af-r:AFR_0002327 rdf:type owl:Class ;
                 rdfs:subClassOf af-r:AFR_0001060 ;
                 skos:altLabel "3-dimensional FTIR spectra" ,
                               "3-dimensional FTIR spectrum" ,
                               "3D FTIR spectra" ,
                               "3D FTIR spectrum" ,
                               "three dimensional FTIR spectra" ,
                               "three dimensional FTIR spectrum" ,
                               "three-dimensional FTIR spectra" ;
                 skos:definition "A three-dimensional FTIR spectrum is a data distribution function that is a plot of absorbance or transmittance versus wavelength and versus time obtained by measuring the amount of radiation absorbed by a sample as a function of the wavelength of incident radiation from the infrared region (2.5–25 μm) and as a function of time. [Allotrope]" ;
                 skos:prefLabel "three-dimensional FTIR spectrum" .


###  http://purl.allotrope.org/ontologies/result#AFR_0002329
af-r:AFR_0002329 rdf:type owl:Class ;
                 rdfs:subClassOf af-r:AFR_0001060 ;
                 skos:altLabel "3-dimensional NIR spectra" ,
                               "3-dimensional NIR spectrum" ,
                               "3-dimensional near infra-red spectra" ,
                               "3-dimensional near infra-red spectrum" ,
                               "3-dimensional near infrared (NIR) spectra" ,
                               "3-dimensional near infrared (NIR) spectrum" ,
                               "3-dimensional near infrared spectra" ,
                               "3D NIR spectra" ,
                               "3D NIR spectrum" ,
                               "3D near infra-red spectra" ,
                               "3D near infra-red spectrum" ,
                               "3D near infrared (NIR) spectra" ,
                               "3D near infrared (NIR) spectrum" ,
                               "3D near infrared spectra" ,
                               "three dimensional NIR spectra" ,
                               "three dimensional NIR spectrum" ,
                               "three dimensional near infra-red spectra" ,
                               "three dimensional near infra-red spectrum" ,
                               "three dimensional near infrared (NIR) spectra" ,
                               "three dimensional near infrared (NIR) spectrum" ,
                               "three dimensional near infrared spectra" ,
                               "three-dimensional NIR spectra" ,
                               "three-dimensional NIR spectrum" ,
                               "three-dimensional near infra-red spectra" ,
                               "three-dimensional near infra-red spectrum" ,
                               "three-dimensional near infrared (NIR) spectra" ,
                               "three-dimensional near infrared (NIR) spectrum" ,
                               "three-dimensional near infrared spectra" ;
                 skos:definition "A three-dimensional near infrared spectrum is a data distribution function that is a plot of absorbance or transmittance versus wavelength and versus time obtained by measuring the amount of radiation absorbed by a sample as a function of the wavelength of incident radiation from the near infrared region (0.8-2 µm) and as a function of time. [Allotrope]" ;
                 skos:prefLabel "three-dimensional near infrared spectrum" .


###  http://purl.allotrope.org/ontologies/result#AFR_0002357
af-r:AFR_0002357 rdf:type owl:Class ;
                 rdfs:subClassOf af-r:AFR_0000576 ;
                 af-x:AFX_0002798 "true"^^xsd:boolean ;
                 skos:altLabel "FTIR profile result" ;
                 skos:definition "An FTIR profile is a profile that quantifies the absorbance by or transmittance through a material entity over time and by frequency in the infrared range. [Allotrope]" ;
                 skos:prefLabel "FTIR profile" .


###  http://purl.allotrope.org/ontologies/result#AFR_0002360
af-r:AFR_0002360 rdf:type owl:Class ;
                 rdfs:subClassOf af-r:AFR_0000576 ;
                 af-x:AFX_0002798 "true"^^xsd:boolean ;
                 skos:altLabel "NIR profile" ,
                               "NIR profile result" ,
                               "near infra-red profile" ,
                               "near infra-red profile result" ,
                               "near infrared profile result" ,
                               "near-infrared profile" ,
                               "near-infrared profile result" ;
                 skos:definition "A near infrared profile is a profile that quantifies absorbed or transmitted radiation over time in the near infrared region (0.8-2 µm). [Allotrope]" ;
                 skos:prefLabel "near infrared profile" .


###  http://purl.allotrope.org/ontologies/result#AFR_0002390
af-r:AFR_0002390 rdf:type owl:Class ;
                 rdfs:subClassOf af-r:AFR_0002650 ;
                 af-x:AFX_0002798 "true"^^xsd:boolean ;
                 skos:altLabel "michelson interferometer acquisition mode setting" ;
                 skos:changeNote "2022-06-20 Subclassed under measurement mode setting and renamed to conform with parent. [Allotrope]" ;
                 skos:definition "A michelson interferometer measurement mode setting is a control setting that specifies whether the interferogram measurement is single or double-sided and whether one or both scan directions are used in the measurement. [Allotrope]" ;
                 skos:prefLabel "michelson interferometer measurement mode setting" .


#################################################################
#    Individuals
#################################################################

###  http://www.allotrope.org
<http://www.allotrope.org> rdf:type owl:NamedIndividual ,
                                    foaf:Organization ;
                           foaf:name "Allotrope Foundation" .


###  http://purl.allotrope.org/voc/attribution
<http://purl.allotrope.org/voc/attribution> rdf:type owl:NamedIndividual ,
                                                     dct:RightsStatement ;
                                            dct:description """
These taxonomies contain material or may constitute derivative works of material which may be subject to copyright by one of the following organizations.  By using these taxonomies, you agree to the following terms and conditions applicable to its contents:
******************************************************************************
Copyright Notice and Terms for IUPAC Gold Book
______________________________________________________________________________
Copyright © 1998, Regents of the University of California
All rights reserved.
Redistribution and use in source and binary forms, with or without modification, are permitted provided that the following conditions are met:
1. Redistributions of source code must retain the above copyright notice, this list of conditions and the following disclaimer.
2. Redistributions in binary form must reproduce the above copyright notice, this list of conditions and the following disclaimer in the documentation and/or other materials provided with the distribution.
THIS SOFTWARE IS PROVIDED BY THE COPYRIGHT HOLDERS AND CONTRIBUTORS \"AS IS\" AND ANY EXPRESS OR IMPLIED WARRANTIES, INCLUDING, BUT NOT LIMITED TO, THE IMPLIED WARRANTIES OF MERCHANTABILITY AND FITNESS FOR A PARTICULAR PURPOSE ARE DISCLAIMED. IN NO EVENT SHALL THE COPYRIGHT HOLDER OR CONTRIBUTORS BE LIABLE FOR ANY DIRECT, INDIRECT, INCIDENTAL, SPECIAL, EXEMPLARY, OR CONSEQUENTIAL DAMAGES (INCLUDING, BUT NOT LIMITED TO, PROCUREMENT OF SUBSTITUTE GOODS OR SERVICES; LOSS OF USE, DATA, OR PROFITS; OR BUSINESS INTERRUPTION) HOWEVER CAUSED AND ON ANY THEORY OF LIABILITY, WHETHER IN CONTRACT, STRICT LIABILITY, OR TORT (INCLUDING NEGLIGENCE OR OTHERWISE) ARISING IN ANY WAY OUT OF THE USE OF THIS SOFTWARE, EVEN IF ADVISED OF THE POSSIBILITY OF SUCH DAMAGE.
******************************************************************************
Copyright Notice and Terms for PSI-MS (Proteomics Standards Initiative - Mass Spectrometry) Mass spectrometer output files and spectra interpretation
_____________________________________________________________________________
Created by Matt Chambers, Andreas Bertsch, Marius Kallhardt, Eric Deutsch Fredrik Levander, Pierre-Alain Binz, and Gerhard Mayer. Publisher: HUPO Proteomics Standards Initiative Mass Spectrometry Standards Working Group and HUPO Proteomics Standards Initiative Proteomics Informatics Working Group. This work is used pursuant to a Creative Commons license available here: http://creativecommons.org/licenses/by/3.0/legalcode

******************************************************************************
Attribution Notice for National Center for Biomedical Ontology materials.

This work contains material from the Cell Ontology and Clinical Measurement Ontology, available here: http://bioportal.bioontology.org/.
******************************************************************************
Attribution Notice for ChEBI
This work contains material from the European Bioinformatics Institute’s ChEBI database.
******************************************************************************
Attribution Notice for Quantities Units Dimensions Data Types (http://www.qudt.org/)
This work contains content from www.qudt.org and is used pursuant to a Creative Commons License available here: http://creativecommons.org/licenses/by-sa/3.0/us/legalcode. The original work may have been modified.
******************************************************************************
Copyright and Attribution Notice for Dublin Core Metadata Initiative Document
This work contains material from the following DCMI document used pursuant to a creative commons license available here: https://creativecommons.org/licenses/by/4.0/legalcode. This material may have been modified or changed.
Timestamped URL:          http://dublincore.org/documents/2012/06/14/dcmi-terms/
Date Issued:                       2012-06-14
Document Status:            This is a DCMI Recommendation.
Copyright © 1995-2015 DCMI. All Rights Reserved. DCMI liability, trademark/service mark, document use and software licensing rules apply.
******************************************************************************

""" ;
                                            dct:title "Derivative works attribution" .


###  http://purl.allotrope.org/voc/copyright
<http://purl.allotrope.org/voc/copyright> rdf:type owl:NamedIndividual ,
                                                   dct:RightsStatement ;
                                          dct:description "Copyright © 2015-2025 Allotrope Foundation" ;
                                          dct:rightsHolder <http://www.allotrope.org> ;
                                          dct:title "Copyright © 2015-2025 Allotrope Foundation" .


###  http://purl.allotrope.org/voc/creative-commons-attribution-license
<http://purl.allotrope.org/voc/creative-commons-attribution-license> rdf:type owl:NamedIndividual ,
                                                                              dct:LicenseDocument ;
                                                                     dct:description """This work is licensed under a Creative Commons Attribution 4.0 International License http://creativecommons.org/licenses/by/4.0/.

THESE MATERIALS ARE PROVIDED \"AS IS\" AND ALLOTROPE EXPRESSLY DISCLAIMS ALL WARRANTIES, EXPRESS, IMPLIED OR STATUTORY, INCLUDING, WITHOUT LIMITATION, THE WARRANTIES OF NON-INFRINGEMENT, TITLE, MERCHANTABILITY AND FITNESS FOR A PARTICULAR PURPOSE.

Copyright © 2015-2025 Allotrope Foundation
""" ;
                                                                     dct:title "Creative Commons Attribution 4.0 International Public License" .


###  Generated by the OWL API (version 5.1.19) https://github.com/owlcs/owlapi/
