@prefix : <http://purl.allotrope.org/voc/afo/domain/WD/2025/06/atomic-spectroscopy#> .
@prefix cl: <http://purl.obolibrary.org/obo/CL> .
@prefix go: <http://purl.obolibrary.org/obo/GO> .
@prefix ro: <http://purl.obolibrary.org/obo/RO> .
@prefix bfo: <http://purl.obolibrary.org/obo/BFO> .
@prefix dct: <http://purl.org/dc/terms/> .
@prefix iao: <http://purl.obolibrary.org/obo/IAO> .
@prefix obi: <http://purl.obolibrary.org/obo/OBI> .
@prefix owl: <http://www.w3.org/2002/07/owl#> .
@prefix rdf: <http://www.w3.org/1999/02/22-rdf-syntax-ns#> .
@prefix xml: <http://www.w3.org/XML/1998/namespace> .
@prefix xsd: <http://www.w3.org/2001/XMLSchema#> .
@prefix af-c: <http://purl.allotrope.org/ontologies/common#> .
@prefix af-e: <http://purl.allotrope.org/ontologies/equipment#> .
@prefix af-m: <http://purl.allotrope.org/ontologies/material#> .
@prefix af-p: <http://purl.allotrope.org/ontologies/process#> .
@prefix af-q: <http://purl.allotrope.org/ontologies/quality#> .
@prefix af-r: <http://purl.allotrope.org/ontologies/result#> .
@prefix af-x: <http://purl.allotrope.org/ontologies/property#> .
@prefix rdfs: <http://www.w3.org/2000/01/rdf-schema#> .
@prefix skos: <http://www.w3.org/2004/02/skos/core#> .
@prefix af-cur: <http://purl.allotrope.org/ontologies/curation#> .
@base <http://purl.allotrope.org/voc/afo/domain/WD/2025/06/atomic-spectroscopy#> .

<http://purl.allotrope.org/voc/afo/domain/WD/2025/06/atomic-spectroscopy> rdf:type owl:Ontology ;
                                                                                     owl:versionIRI <http://purl.allotrope.org/voc/afo/domain/WD/2025/06/atomic-spectroscopy> ;
                                                                                     owl:imports <http://purl.allotrope.org/voc/afo/WD/2025/06/afo> ;
                                                                                     dct:issued "2025-06-25T12:00:00Z"^^xsd:dateTime ;
                                                                                     dct:license <http://purl.allotrope.org/voc/creative-commons-attribution-license> ;
                                                                                     dct:modified "2025-04-04T12:00:00Z"^^xsd:dateTime ;
                                                                                     dct:rights <http://purl.allotrope.org/voc/attribution> ,
                                                                                                <http://purl.allotrope.org/voc/copyright> ;
                                                                                     dct:rightsHolder <http://www.allotrope.org> ;
                                                                                     dct:title "AFO Atomic Spectroscopy Domain Ontology - (WD/2025/06)" ;
                                                                                     owl:priorVersion <http://purl.allotrope.org/voc/afo/domain/WD/WD/2018/04/atomic-spectroscopy> ;
                                                                                     owl:versionInfo "WD/2025/06" .

#################################################################
#    Annotation properties
#################################################################

###  http://purl.allotrope.org/ontologies/property#AFX_0002796
af-x:AFX_0002796 rdf:type owl:AnnotationProperty .


###  http://purl.allotrope.org/ontologies/property#AFX_0002798
af-x:AFX_0002798 rdf:type owl:AnnotationProperty .


###  http://purl.allotrope.org/ontologies/property#AFX_0002809
af-x:AFX_0002809 rdf:type owl:AnnotationProperty .


###  http://purl.org/dc/terms/source
dct:source rdf:type owl:AnnotationProperty .


###  http://www.w3.org/2004/02/skos/core#altLabel
skos:altLabel rdf:type owl:AnnotationProperty .


###  http://www.w3.org/2004/02/skos/core#changeNote
skos:changeNote rdf:type owl:AnnotationProperty .


###  http://www.w3.org/2004/02/skos/core#definition
skos:definition rdf:type owl:AnnotationProperty .


###  http://www.w3.org/2004/02/skos/core#example
skos:example rdf:type owl:AnnotationProperty .


###  http://www.w3.org/2004/02/skos/core#note
skos:note rdf:type owl:AnnotationProperty .


###  http://www.w3.org/2004/02/skos/core#prefLabel
skos:prefLabel rdf:type owl:AnnotationProperty .


###  http://www.w3.org/2004/02/skos/core#scopeNote
skos:scopeNote rdf:type owl:AnnotationProperty .


#################################################################
#    Classes
#################################################################

###  http://purl.allotrope.org/ontologies/process#AFP_0000041
af-p:AFP_0000041 rdf:type owl:Class ;
                 rdfs:subClassOf af-p:AFP_0001279 ;
                 skos:altLabel "F-AES" ,
                               "FAES" ,
                               "flame atomic emission spectroscopy" ,
                               "flame emission spectroscopy" ;
                 skos:definition "A type of atomic emission spectrometry where the sample is excited using an N2/oxide-acetylene flame. [CHMO]" ;
                 skos:prefLabel "flame atomic emission spectroscopy" .


###  http://purl.allotrope.org/ontologies/process#AFP_0000048
af-p:AFP_0000048 rdf:type owl:Class ;
                 rdfs:subClassOf af-p:AFP_0001279 ;
                 skos:altLabel "LIP AES" ,
                               "laser-induced atomic emission spectrometry" ;
                 skos:definition "A type of atomic emission spectrometry where a laser pulse is used as the excitation source. [CHMO]" ;
                 skos:prefLabel "laser-induced atomic emission spectroscopy" .


###  http://purl.allotrope.org/ontologies/process#AFP_0000085
af-p:AFP_0000085 rdf:type owl:Class ;
                 rdfs:subClassOf af-p:AFP_0000687 ;
                 skos:altLabel "QT-AAS" ,
                               "QTAAS" ,
                               "quartz tube atomic absorption spectrometry" ;
                 skos:definition "A type of atomic absorption spectrometry where a solid sample is atomised by placing it in a small quartz tube which is rapidly heated by passing a current through it. [CHMO]" ;
                 skos:prefLabel "quartz tube atomic absorption spectroscopy" .


###  http://purl.allotrope.org/ontologies/process#AFP_0000106
af-p:AFP_0000106 rdf:type owl:Class ;
                 rdfs:subClassOf af-p:AFP_0000572 ;
                 skos:altLabel "FI-FAAS" ,
                               "FIFAAS" ,
                               "flow injection flame atomic absorption spectrometry" ;
                 skos:definition "A type of atomic absorption spectrometry where flow injection is used to carry a gas phase sample to flame where it is atomised. [CHMO]" ;
                 skos:prefLabel "flow injection flame atomic absorption spectrometry" .


###  http://purl.allotrope.org/ontologies/process#AFP_0000128
af-p:AFP_0000128 rdf:type owl:Class ;
                 rdfs:subClassOf af-p:AFP_0000447 ;
                 skos:altLabel "HG-AAS" ,
                               "HGAAS" ,
                               "hydride generation atomic absorption spectrometry" ,
                               "hydride-generation atomic absorption spectrometry" ;
                 skos:definition "A type of atomic absorption spectrometry where metal samples such as As, Sb and Se are vaporised by converting them into volatile hydrides. [CHMO]" ;
                 skos:prefLabel "hydride generation atomic absorption spectroscopy" .


###  http://purl.allotrope.org/ontologies/process#AFP_0000159
af-p:AFP_0000159 rdf:type owl:Class ;
                 rdfs:subClassOf af-p:AFP_0000447 ;
                 skos:altLabel "cold vapour AAS"@en-gb ,
                               "CV-AAS" ,
                               "CVAAS" ,
                               "cold vapor AAS" ,
                               "cold vapor atomic absorption spectrometry" ;
                 skos:changeNote "2016-02-03 Switched labels [OSTHUS]" ,
                                 "2016-02-25 fix translations [OSTHUS]" ;
                 skos:definition "A type of atomic absorption spectrometry where no vaporization step is required because the sample is a volatile heavy metal such as mercury, which is a vapour at room temperature. [CHMO]" ;
                 skos:prefLabel "cold vapour atomic absorption spectrometry"@en-gb ,
                                "cold vapor atomic absorption spectroscopy" .


###  http://purl.allotrope.org/ontologies/process#AFP_0000163
af-p:AFP_0000163 rdf:type owl:Class ;
                 rdfs:subClassOf af-p:AFP_0002291 ;
                 skos:altLabel "plasma AFS" ,
                               "plasma atomic fluorescence spectrometry" ;
                 skos:definition "A type of atomic fluorescence spectroscopy where a plasma is used to excite the atoms in the sample. [CHMO]" ;
                 skos:prefLabel "plasma atomic fluorescence spectroscopy" .


###  http://purl.allotrope.org/ontologies/process#AFP_0000187
af-p:AFP_0000187 rdf:type owl:Class ;
                 rdfs:subClassOf af-p:AFP_0000558 ;
                 skos:altLabel "CCP AES" ,
                               "CCP-AES" ,
                               "capacitively coupled plasma atomic emission spectrometry" ;
                 skos:definition "A type of atomic emission spectrometry where a plasma generated by a potential difference between two electrodes, one of which is grounded and one of which is live. [CHMO]" ;
                 skos:prefLabel "capacitively coupled plasma atomic emission spectroscopy" .


###  http://purl.allotrope.org/ontologies/process#AFP_0000289
af-p:AFP_0000289 rdf:type owl:Class ;
                 rdfs:subClassOf af-p:AFP_0001391 ;
                 skos:altLabel "nanosecond LIBS" ,
                               "nanosecond laser induced breakdown spectrometry" ,
                               "ns-LIBS" ;
                 skos:definition "A type of atomic emission spectrometry where a high energy nanosecond laser pulse is used to generate a plasma which acts as the excitation source. [CHMO]" ;
                 skos:prefLabel "nanosecond laser-induced breakdown spectroscopy" .


###  http://purl.allotrope.org/ontologies/process#AFP_0000447
af-p:AFP_0000447 rdf:type owl:Class ;
                 rdfs:subClassOf af-p:AFP_0001727 ;
                 skos:altLabel "AAS" ,
                               "atomic absorption spectrometry" ;
                 skos:definition "A type of atomic spectroscopy where the sample is illuminated with ultraviolet or visible light which is absorbed by the non-excited atoms at characteristic wavelengths. [CHMO]" ;
                 skos:prefLabel "atomic absorption spectroscopy" .


###  http://purl.allotrope.org/ontologies/process#AFP_0000450
af-p:AFP_0000450 rdf:type owl:Class ;
                 rdfs:subClassOf af-p:AFP_0000678 ;
                 skos:altLabel "SPE-ICP-AES" ;
                 skos:definition "A type of atomic emission spectrometry where the sample mixture is first separated by solid phase extraction and then excited using a plasma generated by electromagnetic inductance. [CHMO]" ;
                 skos:prefLabel "solid phase extraction inductively coupled plasma atomic emission spectroscopy" .


###  http://purl.allotrope.org/ontologies/process#AFP_0000520
af-p:AFP_0000520 rdf:type owl:Class ;
                 rdfs:subClassOf af-p:AFP_0000773 ;
                 skos:altLabel "SS-GF-AAS" ,
                               "SS-GFAAS" ,
                               "direct solid samples graphite furnace atomic absorption spectrometry" ,
                               "direct solid samples graphite furnace atomic absorption spectroscopy" ,
                               "direct solid sampling graphite furnace atomic absorption spectrometry" ,
                               "direct solid sampling graphite furnace atomic absorption spectroscopy" ,
                               "solid samples graphite furnace atomic absorption spectrometry" ,
                               "solid samples graphite furnace atomic absorption spectroscopy" ,
                               "solid sampling graphite furnace atomic absorption spectrometry" ;
                 skos:definition "A type of atomic absorption spectrometry where a solid sample is atomised by placing it in a small graphite-coated tube which is rapidly heated by passing a current through it. [CHMO]" ;
                 skos:prefLabel "solid sampling graphite furnace atomic absorption spectrometry" .


###  http://purl.allotrope.org/ontologies/process#AFP_0000558
af-p:AFP_0000558 rdf:type owl:Class ;
                 rdfs:subClassOf af-p:AFP_0001279 ;
                 skos:altLabel "plasma AES" ;
                 skos:definition "Any type of atomic emission spectrometry where a plasma is used as the excitation source. [CHMO]" ;
                 skos:prefLabel "plasma atomic emission spectroscopy" .


###  http://purl.allotrope.org/ontologies/process#AFP_0000560
af-p:AFP_0000560 rdf:type owl:Class ;
                 rdfs:subClassOf af-p:AFP_0001279 ;
                 skos:altLabel "ETAES" ,
                               "electrothermal atomic emission spectrometry" ;
                 skos:definition "A type of atomic emission spectrometry where the sample is atomised using a probe which is rapidly heated by passing a current through it. [CHMO]" ;
                 skos:prefLabel "electrothermal atomic emission spectroscopy" .


###  http://purl.allotrope.org/ontologies/process#AFP_0000563
af-p:AFP_0000563 rdf:type owl:Class ;
                 rdfs:subClassOf af-p:AFP_0000447 ;
                 skos:altLabel "F-AAS" ,
                               "FAAS" ,
                               "flame atomic absorption spectroscopy" ;
                 skos:definition "A type of atomic absorption spectrometry where the sample is  aspirated, aerosolised, and mixed with combustible gases, such as acetylene and air or acetylene and nitrous oxide. The mixture is then ignited and atomised in a flame whose temperature ranges from 2100-2800 °C. During combustion, atoms of the element of interest in the sample absorb light at characteristic wavelengths. [CHMO]" ;
                 skos:prefLabel "flame atomic absorption spectrometry" .


###  http://purl.allotrope.org/ontologies/process#AFP_0000569
af-p:AFP_0000569 rdf:type owl:Class ;
                 rdfs:subClassOf af-p:AFP_0002230 ;
                 skos:altLabel "furnace ionisation non-thermal excitation spectrometry"@en-gb ,
                               "FINES" ,
                               "furnace ionization non-thermal excitation spectrometry" ;
                 skos:definition "A type of atomic emission spectrometry where the sample is atomised by placing it in a small graphite-coated tube which is rapidly heated by passing a current through it, then ionized and excited using a glow discharge (a potential difference applied across two electrodes immersed in the sample gas). [CHMO]" ;
                 skos:prefLabel "furnace ionisation nonthermal excitation spectrometry"@en-gb ,
                                "furnace ionization nonthermal excitation spectrometry" .


###  http://purl.allotrope.org/ontologies/process#AFP_0000572
af-p:AFP_0000572 rdf:type owl:Class ;
                 rdfs:subClassOf af-p:AFP_0000447 ;
                 skos:altLabel "FI-AAS" ,
                               "FIAAS" ,
                               "flow injection atomic absorption spectroscopy" ;
                 skos:definition "A type of atomic absorption spectrometry where flow injection is used to transfer a sample to the spectrometer. [CHMO]" ;
                 skos:prefLabel "flow injection atomic absorption spectrometry" .


###  http://purl.allotrope.org/ontologies/process#AFP_0000678
af-p:AFP_0000678 rdf:type owl:Class ;
                 rdfs:subClassOf af-p:AFP_0000558 ;
                 skos:altLabel "ICP AES" ,
                               "ICP OES" ,
                               "ICP-AES" ,
                               "ICP-OES" ,
                               "inductively coupled plasma atomic emission spectrometry" ,
                               "inductively coupled plasma atomic emission spectroscopy" ,
                               "inductively coupled plasma optical emission spectrometry" ,
                               "inductively coupled plasma optical emission spectroscopy" ,
                               "inductively coupled plasma-atomic emission spectrometry" ,
                               "inductively coupled plasma-atomic emission spectroscopy" ,
                               "inductively coupled plasma-optical emission spectrometry" ,
                               "inductively coupled plasma-optical emission spectroscopy" ;
                 skos:definition "A type of atomic emission spectrometry where a plasma generated by electromagnetic induction is used as the excitation source. [CHMO]" ;
                 skos:prefLabel "inductively-coupled plasma atomic emission spectroscopy" .


###  http://purl.allotrope.org/ontologies/process#AFP_0000687
af-p:AFP_0000687 rdf:type owl:Class ;
                 rdfs:subClassOf af-p:AFP_0000447 ;
                 skos:altLabel "ET-AAS" ,
                               "ETAAS" ,
                               "electrothermal atomic absorption spectroscopy" ;
                 skos:definition "A type of atomic absorption spectrometry where the sample is atomised using a probe which is rapidly heated by passing a current through it. [CHMO]" ;
                 skos:prefLabel "electrothermal atomic absorption spectrometry" .


###  http://purl.allotrope.org/ontologies/process#AFP_0000740
af-p:AFP_0000740 rdf:type owl:Class ;
                 rdfs:subClassOf af-p:AFP_0001279 ;
                 skos:altLabel "spark AES" ,
                               "spark OES" ,
                               "spark atomic emission spectroscopy" ,
                               "spark optical emission spectrometry" ,
                               "spark optical emission spectroscopy" ,
                               "spark-AES" ,
                               "spark-OES" ,
                               "spark-atomic emission spectrometry" ,
                               "spark-excitation atomic emission spectrometry" ,
                               "spark-excitation atomic emission spectroscopy" ,
                               "spark-optical emission spectrometry" ,
                               "spark-optical emission spectroscopy" ;
                 skos:definition "A type of atomic emission spectrometry where the sample is excited by an arc or spark between two electrodes. [CHMO]" ;
                 skos:prefLabel "spark atomic emission spectrometry" .


###  http://purl.allotrope.org/ontologies/process#AFP_0000770
af-p:AFP_0000770 rdf:type owl:Class ;
                 rdfs:subClassOf af-p:AFP_0001380 ;
                 skos:altLabel "HC-AES" ,
                               "HC-OES" ,
                               "HCGD-AES" ,
                               "HCGD-OES" ,
                               "hollow cathode glow discharge atomic emission spectrometry" ,
                               "hollow cathode glow discharge atomic emission spectroscopy" ,
                               "hollow cathode glow discharge optical emission spectrometry" ,
                               "hollow cathode optical emission spectrometry" ,
                               "hollow-cathode glow discharge atomic emission spectrometry" ,
                               "hollow-cathode glow discharge atomic emission spectroscopy" ,
                               "hollow-cathode glow discharge optical emission spectroscopy" ,
                               "hollow-cathode optical emission spectrometry" ;
                 skos:definition "A type of atomic emission spectrometry where a glow discharge (a potential difference applied across two electrodes immersed in the sample gas) is used to excite the sample. The plasma source contains a hollow cylindrical metal cathode containing the metal for excitation, and an anode. [CHMO]" ;
                 skos:prefLabel "hollow-cathode atomic emission spectroscopy" .


###  http://purl.allotrope.org/ontologies/process#AFP_0000773
af-p:AFP_0000773 rdf:type owl:Class ;
                 rdfs:subClassOf af-p:AFP_0000687 ;
                 skos:altLabel "GF-AAS" ,
                               "GFAAS" ,
                               "graphite furnace atomic absorption spectroscopy" ,
                               "graphite-furnace atomic-absorption spectroscopy" ;
                 skos:definition "A type of atomic absorption spectrometry where the sample is atomised by placing it in a small graphite-coated tube which is rapidly heated by passing a current through it. [CHMO]" ;
                 skos:prefLabel "graphite furnace atomic absorption spectrometry" .


###  http://purl.allotrope.org/ontologies/process#AFP_0000803
af-p:AFP_0000803 rdf:type owl:Class ;
                 rdfs:subClassOf af-p:AFP_0000678 ;
                 skos:altLabel "nebulisation inductively coupled plasma atomic emission spectrometry"@en-gb ,
                               "nebulization inductively coupled plasma atomic emission spectrometry" ;
                 skos:definition "A type of atomic emission spectrometry where the sample mixture is first passed through a nebulizer to form a mist of finely dispersed droplets (using compressed air) and then excited using a plasma generated by electromagnetic inductance. [CHMO]" ;
                 skos:prefLabel "nebulization inductively coupled plasma atomic emission spectroscopy"@en-gb ,
                                "nebulisation inductively-coupled plasma atomic emission spectroscopy" .


###  http://purl.allotrope.org/ontologies/process#AFP_0000841
af-p:AFP_0000841 rdf:type owl:Class ;
                 rdfs:subClassOf af-p:AFP_0000558 ;
                 skos:altLabel "MIP AES" ,
                               "MIP-AES" ,
                               "microwave-induced plasma atomic emission spectroscopy" ;
                 skos:definition "A type of atomic emission spectrometry where a plasma generated by microwave bombardment is used as the excitation source. [CHMO]" ;
                 skos:prefLabel "microwave induced plasma atomic emission spectrometry" .


###  http://purl.allotrope.org/ontologies/process#AFP_0000859
af-p:AFP_0000859 rdf:type owl:Class ;
                 rdfs:subClassOf af-p:AFP_0000558 ;
                 skos:altLabel "DCP-AES" ,
                               "DCPAES" ,
                               "d.c. AES" ,
                               "d.c. plasma atomic emission spectrometry" ,
                               "d.c. plasma atomic emission spectroscopy" ,
                               "direct current plasma atomic emission spectrometry" ;
                 skos:definition "A type of atomic emission spectrometry where a plasma generated by passing an electrical discharge between two electrodes is used as the excitation source. [CHMO]" ;
                 skos:prefLabel "direct current plasma atomic emission spectroscopy" .


###  http://purl.allotrope.org/ontologies/process#AFP_0000873
af-p:AFP_0000873 rdf:type owl:Class ;
                 rdfs:subClassOf af-p:AFP_0000558 ;
                 skos:altLabel "MTES" ,
                               "metastable transfer emission spectroscopy" ;
                 skos:definition "A type of atomic emission spectrometry where atoms are excited by energy transfer from metastable N2 species in a nitrogen plasma. [CHMO]" ;
                 skos:prefLabel "metastable transfer emission spectrometry" .


###  http://purl.allotrope.org/ontologies/process#AFP_0000930
af-p:AFP_0000930 rdf:type owl:Class ;
                 rdfs:subClassOf af-p:AFP_0000560 ;
                 skos:altLabel "GF-AES" ,
                               "GF-OES" ,
                               "GFAES" ,
                               "GFOES" ,
                               "graphite furnace atomic emission spectrometry" ,
                               "graphite furnace optical emission spectrometry" ,
                               "graphite furnace optical emission spectroscopy" ;
                 skos:definition "A type of atomic emission spectrometry where the sample is atomised by placing it in a small graphite-coated tube which is rapidly heated by passing a current through it. [CHMO]" ;
                 skos:prefLabel "graphite furnace atomic emission spectrometry" .


###  http://purl.allotrope.org/ontologies/process#AFP_0001199
af-p:AFP_0001199 rdf:type owl:Class ;
                 rdfs:subClassOf af-p:AFP_0000678 ;
                 skos:altLabel "HG-ICP-AES" ,
                               "HG-ICP-OES" ,
                               "hydride generation inductively coupled plasma atomic emission spectrometry" ,
                               "hydride generation inductively coupled plasma optical emission spectrometry" ,
                               "hydride generation inductively coupled plasma optical emission spectroscopy" ;
                 skos:definition "Atomic emission spectrometry of metal samples such as As, Sb and Se that are vaporised by converting them into volatile hydrides and excited using a plasma generated by electromagnetic induction. [CHMO]" ;
                 skos:prefLabel "hydride generation inductively coupled plasma atomic emission spectroscopy" .


###  http://purl.allotrope.org/ontologies/process#AFP_0001252
af-p:AFP_0001252 rdf:type owl:Class ;
                 rdfs:subClassOf af-p:AFP_0001391 ;
                 skos:altLabel "LISPS" ,
                               "double-pulse LIBS" ,
                               "double-pulse laser-induced breakdown spectrometry" ,
                               "double-pulse laser-induced breakdown spectroscopy" ,
                               "laser-induced shock wave spectrometry" ;
                 skos:definition "A type of atomic emission spectrometry where a high energy laser pulse is used to generate a plasma which acts as the excitation source. A second laser pulse then illuminates the sample resulting in a reheating of the laser plasma produced by the first pulse, leading to signal enhancement. [CHMO]" ;
                 skos:prefLabel "laser-induced shock wave plasma spectroscopy" .


###  http://purl.allotrope.org/ontologies/process#AFP_0001279
af-p:AFP_0001279 rdf:type owl:Class ;
                 rdfs:subClassOf af-p:AFP_0001727 ;
                 skos:altLabel "AES" ,
                               "OES" ,
                               "atomic emission spectrometry" ,
                               "optical emission spectrometry" ,
                               "optical emission spectroscopy" ;
                 skos:definition "A type of atomic spectroscopy where the atoms in the sample are excited and the emission of electromagnetic radiation at characteristic wavelengths is detected. [CHMO]" ;
                 skos:prefLabel "atomic emission spectroscopy" .


###  http://purl.allotrope.org/ontologies/process#AFP_0001344
af-p:AFP_0001344 rdf:type owl:Class ;
                 rdfs:subClassOf af-p:AFP_0002291 ;
                 skos:altLabel "HG-AFS" ,
                               "HGAFS" ,
                               "hydride generation atomic fluorescence spectrometry" ;
                 skos:definition "A type of atomic fluorescence spectroscopy of metal samples such as As, Sb and Se which are vaporised by converting them into volatile hydrides. [CHMO]" ;
                 skos:prefLabel "hydride generation atomic fluorescence spectroscopy" .


###  http://purl.allotrope.org/ontologies/process#AFP_0001372
af-p:AFP_0001372 rdf:type owl:Class ;
                 rdfs:subClassOf af-p:AFP_0000450 ;
                 skos:altLabel "FI-SPE-ICP-AES" ;
                 skos:definition "A type of atomic emission spectrometry where the sample mixture is first separated by solid phase extraction, carried to the spectrometer by flow injection and then excited using a plasma generated by electromagnetic inductance. [CHMO]" ;
                 skos:prefLabel "flow injection solid phase extraction inductively coupled plasma atomic emission spectroscopy" .


###  http://purl.allotrope.org/ontologies/process#AFP_0001380
af-p:AFP_0001380 rdf:type owl:Class ;
                 rdfs:subClassOf af-p:AFP_0001279 ;
                 skos:altLabel "GD-AES" ,
                               "GD-OES" ,
                               "glow discharge optical emission spectrometry" ,
                               "glow discharge optical emission spectroscopy" ;
                 skos:definition "A type of atomic emission spectrometry where a glow discharge (a potential difference applied across two electrodes immersed in the sample gas) is used to excite the sample. [CHMO]" ;
                 skos:prefLabel "glow discharge atomic emission spectroscopy" .


###  http://purl.allotrope.org/ontologies/process#AFP_0001391
af-p:AFP_0001391 rdf:type owl:Class ;
                 rdfs:subClassOf af-p:AFP_0000048 ;
                 skos:altLabel "LIBS" ,
                               "LIP AES" ,
                               "LIP-AES" ,
                               "LIPS" ,
                               "laser induced plasma spectrometry" ,
                               "laser induced plasma spectroscopy" ,
                               "laser-induced breakdown atomic emission spectrometry" ,
                               "laser-induced plasma atomic emission spectrometry" ,
                               "laser-induced plasma atomic emission spectroscopy" ,
                               "laser-induced plasma spectrometry" ,
                               "laser-induced plasma spectroscopy" ;
                 skos:definition "A type of atomic emission spectrometry where a high energy laser pulse is used to generate a plasma which acts as the excitation source. [CHMO]" ;
                 skos:prefLabel "laser-induced breakdown spectroscopy" .


###  http://purl.allotrope.org/ontologies/process#AFP_0001396
af-p:AFP_0001396 rdf:type owl:Class ;
                 rdfs:subClassOf af-p:AFP_0000447 ;
                 skos:altLabel "GD-AAS" ,
                               "GDAAS" ,
                               "atomic absorption glow-discharge spectrometry" ,
                               "glow discharge atomic absorption spectrometry" ,
                               "glow discharge atomic absorption spectroscopy" ;
                 skos:definition "A type of atomic absorption spectrometry where a glow discharge (a potential difference applied across two electrodes immersed in the sample gas) is used to atomise the sample before it absorbs ultra-violet or visible light atoms at characteristic wavelengths. [CHMO]" ;
                 skos:prefLabel "atomic absorption glow-discharge spectroscopy" .


###  http://purl.allotrope.org/ontologies/process#AFP_0001584
af-p:AFP_0001584 rdf:type owl:Class ;
                 rdfs:subClassOf af-p:AFP_0001995 ;
                 skos:altLabel "FI-TS-FF-AAS" ,
                               "flow injection thermospray flame furnace absorption spectrometry" ;
                 skos:definition "A type of atomic absorption spectrometry where the sample is carried to the spectrometer by flow injection and forced through a heated metal capillary tip before atomization in a flame furnace. [CHMO]" ;
                 skos:prefLabel "flow injection thermospray flame furnace absorption spectrometry" .


###  http://purl.allotrope.org/ontologies/process#AFP_0001692
af-p:AFP_0001692 rdf:type owl:Class ;
                 rdfs:subClassOf af-p:AFP_0000678 ;
                 skos:altLabel "LA ICP AES" ,
                               "LA ICP-AES" ,
                               "laser ablation ICP AES" ,
                               "laser ablation inductively coupled plasma atomic emission spectrometry" ;
                 skos:definition "A type of atomic emission spectrometry where the sample is vaporised by laser ablation and excited using a plasma generated by electromagnetic induction. [CHMO]" ;
                 skos:prefLabel "laser ablation inductively-coupled plasma atomic emission spectroscopy" .


###  http://purl.allotrope.org/ontologies/process#AFP_0001727
af-p:AFP_0001727 rdf:type owl:Class ;
                 rdfs:subClassOf af-p:AFP_0001655 ;
                 skos:altLabel "atomic spectrometry" ;
                 skos:definition "Any spectroscopic technique which is based upon the ability of atoms to absorb or emit electromagnetic radiation. In atomic spectroscopy the sample is vaporised and then atomised. [CHMO]" ;
                 skos:prefLabel "atomic spectroscopy" .


###  http://purl.allotrope.org/ontologies/process#AFP_0001734
af-p:AFP_0001734 rdf:type owl:Class ;
                 rdfs:subClassOf af-p:AFP_0002291 ;
                 skos:altLabel "ETAFS" ,
                               "electrothermal atomic fluorescence spectrometry" ;
                 skos:definition "A type of atomic fluorescence spectroscopy where the sample is atomised using a probe which is rapidly heated by passing a current through it. [CHMO]" ;
                 skos:prefLabel "electrothermal atomic fluorescence spectroscopy" .


###  http://purl.allotrope.org/ontologies/process#AFP_0001799
af-p:AFP_0001799 rdf:type owl:Class ;
                 rdfs:subClassOf af-p:AFP_0001692 ;
                 skos:altLabel "LM-ICP-AES" ,
                               "laser microprobe ICP-AES" ;
                 skos:definition "A type of atomic emission spectrometry where the sample is vaporised by laser ablation with a finely focused (<10 m diameter) laser and excited using a plasma generated by electromagnetic induction. [CHMO]" ;
                 skos:prefLabel "laser microprobe inductively coupled plasma atomic emission spectroscopy" .


###  http://purl.allotrope.org/ontologies/process#AFP_0001831
af-p:AFP_0001831 rdf:type owl:Class ;
                 rdfs:subClassOf af-p:AFP_0000163 ;
                 skos:altLabel "furnace atomisation plasma emission spectrometry"@en-gb ,
                               "FAPES" ,
                               "furnace atomization plasma emission spectrometry" ;
                 skos:definition "A type of atomic emission spectrometry where a furnace is used to atomize the sample and a plasma is used as the excitation source. [CHMO]" ;
                 skos:prefLabel "furnace atomisation plasma emission spectroscopy"@en-gb ,
                                "furnace atomization plasma emission spectrometry" .


###  http://purl.allotrope.org/ontologies/process#AFP_0001844
af-p:AFP_0001844 rdf:type owl:Class ;
                 rdfs:subClassOf af-p:AFP_0001391 ;
                 skos:altLabel "LIBS" ,
                               "micro LIBS" ;
                 skos:definition "A type of atomic emission spectrometry where a finely focused (<10 m diameter) high energy laser pulse is used to generate a plasma which acts as the excitation source. [CHMO]" ;
                 skos:prefLabel "micro laser-induced breakdown atomic emission spectroscopy" .


###  http://purl.allotrope.org/ontologies/process#AFP_0001972
af-p:AFP_0001972 rdf:type owl:Class ;
                 rdfs:subClassOf af-p:AFP_0002291 ;
                 skos:altLabel "FAFS" ,
                               "FFS" ,
                               "flame atomic fluorescence spectrometry" ,
                               "flame fluorescence spectrometry" ,
                               "flame fluorescence spectroscopy" ;
                 skos:definition "A type of atomic fluorescence spectroscopy where the sample is atomised using a flame. [CHMO]" ;
                 skos:prefLabel "flame atomic fluorescence spectroscopy" .


###  http://purl.allotrope.org/ontologies/process#AFP_0001995
af-p:AFP_0001995 rdf:type owl:Class ;
                 rdfs:subClassOf af-p:AFP_0000687 ;
                 skos:altLabel "(TS-FF)-AAS" ,
                               "TS-FF-AAS" ,
                               "thermospray flame furnace atomic absorption spectroscopy" ;
                 skos:definition "A type of atomic absorption spectrometry where sample is forced through a heated metal capillary tip before atomization in a flame. [CHMO]" ;
                 skos:prefLabel "thermospray flame furnace atomic absorption spectrometry" .


###  http://purl.allotrope.org/ontologies/process#AFP_0002136
af-p:AFP_0002136 rdf:type owl:Class ;
                 rdfs:subClassOf af-p:AFP_0000572 ;
                 skos:altLabel "FI-ETAAS" ,
                               "FIETAAS" ,
                               "flow injection electrothermal atomic absorption spectrometry" ,
                               "flow injection electrothermal atomisation atomic absorption spectrometry" ,
                               "flow injection electrothermal atomization atomic absorption spectrometry" ,
                               "flow injection electrothermal atomization atomic absorption spectroscopy" ;
                 skos:definition "A type of atomic absorption spectrometry where flow injection is used to carry a sample to an electrothermal atomiser where it is atomised using a probe which is rapidly heated by passing a current through it. [CHMO]" ;
                 skos:prefLabel "flow injection electrothermal atomic absorption spectrometry" .


###  http://purl.allotrope.org/ontologies/process#AFP_0002184
af-p:AFP_0002184 rdf:type owl:Class ;
                 rdfs:subClassOf af-p:AFP_0000447 ;
                 skos:altLabel "LS-AAS" ,
                               "LSAAS" ,
                               "line source atomic absorption spectrometry" ;
                 skos:definition "A type of atomic absorption spectrometry using a line source of radiation. [CHMO]" ;
                 skos:prefLabel "line-source atomic absorption spectroscopy" .


###  http://purl.allotrope.org/ontologies/process#AFP_0002230
af-p:AFP_0002230 rdf:type owl:Class ;
                 rdfs:subClassOf af-p:AFP_0000930 ;
                 skos:altLabel "FANES" ,
                               "furnace atomic non thermal excitation spectrometry" ,
                               "furnace atomic non-thermal excitation spectrometry" ,
                               "furnace atomic non-thermal excitation spectroscopy" ,
                               "furnace atomic nonthermal excitation spectroscopy" ;
                 skos:definition "A type of atomic emission spectrometry where the sample is atomised by placing it in a small graphite-coated tube which is rapidly heated by passing a current through it, then excited using a glow discharge (a potential difference applied across two electrodes immersed in the sample gas). [CHMO]" ;
                 skos:prefLabel "furnace atomic nonthermal excitation spectrometry" .


###  http://purl.allotrope.org/ontologies/process#AFP_0002245
af-p:AFP_0002245 rdf:type owl:Class ;
                 rdfs:subClassOf af-p:AFP_0000773 ;
                 skos:altLabel "slurry sampling graphite furnace atomic absorption spectroscopy" ;
                 skos:definition "A type of atomic absorption spectrometry where a solid sample is ground into a fine powder and suspensed in a diluent such as 0.1% HNO3 to form a 'slurry'. The sample is then atomised by placing it in a small graphite-coated tube which is rapidly heated by passing a current through it. [CHMO]" ;
                 skos:prefLabel "slurry sampling graphite furnace atomic absorption spectrometry" .


###  http://purl.allotrope.org/ontologies/process#AFP_0002286
af-p:AFP_0002286 rdf:type owl:Class ;
                 rdfs:subClassOf af-p:AFP_0001391 ;
                 skos:altLabel "fs-LIBS" ;
                 skos:definition "A type of atomic emission spectrometry where a high energy femtosecond laser pulse is used to generate a plasma which acts as the excitation source. [CHMO]" ;
                 skos:prefLabel "femtosecond laser-induced breakdown spectroscopy" .


###  http://purl.allotrope.org/ontologies/process#AFP_0002291
af-p:AFP_0002291 rdf:type owl:Class ;
                 rdfs:subClassOf af-p:AFP_0001727 ;
                 skos:altLabel "AFS" ,
                               "atomic fluorescence spectrometry" ;
                 skos:definition "Any type of atomic spectroscopy where an atom absorbs then spontaneously emits a photon. [CHMO]" ;
                 skos:prefLabel "atomic fluorescence spectroscopy" .


###  http://purl.allotrope.org/ontologies/process#AFP_0002340
af-p:AFP_0002340 rdf:type owl:Class ;
                 rdfs:subClassOf af-p:AFP_0000770 ;
                 skos:altLabel "PB/HC-AES" ,
                               "PB/HC-OES" ,
                               "PC-HC-AES" ,
                               "PC-HC-OES" ,
                               "particle beam/hollow cathode atomic emission spectroscopy" ,
                               "particle beam/hollow cathode optical emission spectroscopy" ,
                               "particle beam/hollow-cathode atomic emission spectroscopy" ,
                               "particle beam/hollow-cathode optical emission spectroscopy" ,
                               "particle-beam/hollow-cathode optical emission spectroscopy" ;
                 skos:definition "A type of atomic emission spectrometry where a glow discharge (a potential difference applied across two electrodes immersed in the sample gas) is used to excite the sample. A nebuliser is used to generate a finely dispersed aerosol containing the sample, which is desolvated, and a momentum separator is used to inject dry particles of the analyte (the 'particle beam') into the plasma source (which consists of a hollow cylindrical metal cathode containing the metal for excitation, and an anode). [CHMO]" ;
                 skos:prefLabel "particle-beam/hollow-cathode atomic emission spectroscopy" .


###  http://purl.allotrope.org/ontologies/process#AFP_0002344
af-p:AFP_0002344 rdf:type owl:Class ;
                 rdfs:subClassOf af-p:AFP_0002291 ;
                 skos:altLabel "LEAF" ,
                               "LEAFS" ,
                               "laser-enhanced atomic fluorescence spectrometry" ,
                               "laser-excited atomic fluorescence spectrometry" ,
                               "laser-excited atomic fluorescence spectroscopy" ;
                 skos:definition "A type of atomic fluorescence spectroscopy where a laser is used to excite the atoms in the sample. [CHMO]" ;
                 skos:prefLabel "laser-enhanced atomic fluorescence spectroscopy" .


###  http://purl.allotrope.org/ontologies/process#AFP_0002356
af-p:AFP_0002356 rdf:type owl:Class ;
                 rdfs:subClassOf af-p:AFP_0000803 ;
                 skos:altLabel "ultrasonic nebulisation inductively coupled plasma atomic emission spectrometry"@en-gb ,
                               "ultrasonic nebulisation inductively coupled plasma optical emission spectrometry"@en-gb ,
                               "ultrasonic nebulisation inductively coupled plasma optical emission spectroscopy"@en-gb ,
                               "USN-ICP-AES" ,
                               "USN-ICP-OES" ,
                               "ultrasonic nebulization inductively coupled plasma atomic emission spectrometry" ,
                               "ultrasonic nebulization inductively coupled plasma optical emission spectrometry" ,
                               "ultrasonic nebulization inductively coupled plasma optical emission spectroscopy" ;
                 skos:definition "A type of atomic emission spectrometry where the sample mixture is first passed through a nebulizer to form a mist of finely dispersed droplets (using high frequency vibrations) and then excited using a plasma generated by electromagnetic inductance. [CHMO]" ;
                 skos:prefLabel "ultrasonic nebulisation inductively coupled plasma atomic emission spectroscopy"@en-gb ,
                                "ultrasonic nebulization inductively coupled plasma atomic emission spectroscopy" .


###  http://purl.allotrope.org/ontologies/process#AFP_0002391
af-p:AFP_0002391 rdf:type owl:Class ;
                 rdfs:subClassOf af-p:AFP_0002291 ;
                 skos:altLabel "cold vapour AFS"@en-gb ,
                               "cold vapour atomic fluorescence spectrometry"@en-gb ,
                               "CV-AFS" ,
                               "CVAFS" ,
                               "cold vapor AFS" ,
                               "cold vapor atomic fluorescence spectrometry" ;
                 skos:changeNote "2016-02-03 Switched labels [OSTHUS]" ,
                                 "2016-02-25 fix translation [OSTHUS]" ;
                 skos:definition "A type of atomic fluorescence spectroscopy where no vaporization step is required because the sample is a volatile heavy metal such as mercury, which is a vapour at room temperature. [CHMO]" ;
                 skos:prefLabel "cold vapour atomic fluorescence spectroscopy"@en-gb ,
                                "cold vapor atomic fluorescence spectroscopy" .


#################################################################
#    Individuals
#################################################################

###  http://purl.allotrope.org/voc/attribution
<http://purl.allotrope.org/voc/attribution> rdf:type owl:NamedIndividual ,
                                                     dct:RightsStatement ;
                                            dct:description """
These taxonomies contain material or may constitute derivative works of material which may be subject to copyright by one of the following organizations.  By using these taxonomies, you agree to the following terms and conditions applicable to its contents:
******************************************************************************
Copyright Notice and Terms for IUPAC Gold Book
______________________________________________________________________________
Copyright © 1998, Regents of the University of California
All rights reserved.
Redistribution and use in source and binary forms, with or without modification, are permitted provided that the following conditions are met:
1. Redistributions of source code must retain the above copyright notice, this list of conditions and the following disclaimer.
2. Redistributions in binary form must reproduce the above copyright notice, this list of conditions and the following disclaimer in the documentation and/or other materials provided with the distribution.
THIS SOFTWARE IS PROVIDED BY THE COPYRIGHT HOLDERS AND CONTRIBUTORS \"AS IS\" AND ANY EXPRESS OR IMPLIED WARRANTIES, INCLUDING, BUT NOT LIMITED TO, THE IMPLIED WARRANTIES OF MERCHANTABILITY AND FITNESS FOR A PARTICULAR PURPOSE ARE DISCLAIMED. IN NO EVENT SHALL THE COPYRIGHT HOLDER OR CONTRIBUTORS BE LIABLE FOR ANY DIRECT, INDIRECT, INCIDENTAL, SPECIAL, EXEMPLARY, OR CONSEQUENTIAL DAMAGES (INCLUDING, BUT NOT LIMITED TO, PROCUREMENT OF SUBSTITUTE GOODS OR SERVICES; LOSS OF USE, DATA, OR PROFITS; OR BUSINESS INTERRUPTION) HOWEVER CAUSED AND ON ANY THEORY OF LIABILITY, WHETHER IN CONTRACT, STRICT LIABILITY, OR TORT (INCLUDING NEGLIGENCE OR OTHERWISE) ARISING IN ANY WAY OUT OF THE USE OF THIS SOFTWARE, EVEN IF ADVISED OF THE POSSIBILITY OF SUCH DAMAGE.
******************************************************************************
Copyright Notice and Terms for PSI-MS (Proteomics Standards Initiative - Mass Spectrometry) Mass spectrometer output files and spectra interpretation
_____________________________________________________________________________
Created by Matt Chambers, Andreas Bertsch, Marius Kallhardt, Eric Deutsch Fredrik Levander, Pierre-Alain Binz, and Gerhard Mayer. Publisher: HUPO Proteomics Standards Initiative Mass Spectrometry Standards Working Group and HUPO Proteomics Standards Initiative Proteomics Informatics Working Group. This work is used pursuant to a Creative Commons license available here: http://creativecommons.org/licenses/by/3.0/legalcode

******************************************************************************
Attribution Notice for National Center for Biomedical Ontology materials.

This work contains material from the Cell Ontology and Clinical Measurement Ontology, available here: http://bioportal.bioontology.org/.
******************************************************************************
Attribution Notice for ChEBI
This work contains material from the European Bioinformatics Institute’s ChEBI database.
******************************************************************************
Attribution Notice for Quantities Units Dimensions Data Types (http://www.qudt.org/)
This work contains content from www.qudt.org and is used pursuant to a Creative Commons License available here: http://creativecommons.org/licenses/by-sa/3.0/us/legalcode. The original work may have been modified.
******************************************************************************
Copyright and Attribution Notice for Dublin Core Metadata Initiative Document
This work contains material from the following DCMI document used pursuant to a creative commons license available here: https://creativecommons.org/licenses/by/4.0/legalcode. This material may have been modified or changed.
Timestamped URL:          http://dublincore.org/documents/2012/06/14/dcmi-terms/
Date Issued:                       2012-06-14
Document Status:            This is a DCMI Recommendation.
Copyright © 1995-2015 DCMI. All Rights Reserved. DCMI liability, trademark/service mark, document use and software licensing rules apply.
******************************************************************************

""" ;
                                            dct:title "Derivative works attribution" .


###  http://purl.allotrope.org/voc/copyright
<http://purl.allotrope.org/voc/copyright> rdf:type owl:NamedIndividual ,
                                                   dct:RightsStatement ;
                                          dct:description "(c) 2017 Allotrope Foundation" ;
                                          dct:title "(c) 2017 Allotrope Foundation" .


###  http://purl.allotrope.org/voc/creative-commons-attribution-license
<http://purl.allotrope.org/voc/creative-commons-attribution-license> rdf:type owl:NamedIndividual ,
                                                                              dct:LicenseDocument ;
                                                                     dct:description """This work is licensed under a Creative Commons Attribution 4.0 International License http://creativecommons.org/licenses/by/4.0/.

THESE MATERIALS ARE PROVIDED \"AS IS\" AND ALLOTROPE EXPRESSLY DISCLAIMS ALL WARRANTIES, EXPRESS, IMPLIED OR STATUTORY, INCLUDING, WITHOUT LIMITATION, THE WARRANTIES OF NON-INFRINGEMENT, TITLE, MERCHANTABILITY AND FITNESS FOR A PARTICULAR PURPOSE.

Copyright © 2015-2025 Allotrope Foundation
""" ;
                                                                     dct:title "Creative Commons Attribution 4.0 International Public License" .


###  http://purl.allotrope.org/voc/afo/domain/WD/2025/06/atomic-spectroscopy
<http://purl.allotrope.org/voc/afo/domain/WD/2025/06/atomic-spectroscopy> rdf:type owl:NamedIndividual .


###  Generated by the OWL API (version 5.1.19) https://github.com/owlcs/owlapi/
