@prefix : <http://purl.allotrope.org/voc/afo/domain/WD/2025/06/auger#> .
@prefix cl: <http://purl.obolibrary.org/obo/CL> .
@prefix go: <http://purl.obolibrary.org/obo/GO> .
@prefix ro: <http://purl.obolibrary.org/obo/RO> .
@prefix bfo: <http://purl.obolibrary.org/obo/BFO> .
@prefix dct: <http://purl.org/dc/terms/> .
@prefix iao: <http://purl.obolibrary.org/obo/IAO> .
@prefix obi: <http://purl.obolibrary.org/obo/OBI> .
@prefix owl: <http://www.w3.org/2002/07/owl#> .
@prefix rdf: <http://www.w3.org/1999/02/22-rdf-syntax-ns#> .
@prefix xml: <http://www.w3.org/XML/1998/namespace> .
@prefix xsd: <http://www.w3.org/2001/XMLSchema#> .
@prefix af-c: <http://purl.allotrope.org/ontologies/common#> .
@prefix af-e: <http://purl.allotrope.org/ontologies/equipment#> .
@prefix af-m: <http://purl.allotrope.org/ontologies/material#> .
@prefix af-p: <http://purl.allotrope.org/ontologies/process#> .
@prefix af-q: <http://purl.allotrope.org/ontologies/quality#> .
@prefix af-r: <http://purl.allotrope.org/ontologies/result#> .
@prefix af-x: <http://purl.allotrope.org/ontologies/property#> .
@prefix rdfs: <http://www.w3.org/2000/01/rdf-schema#> .
@prefix skos: <http://www.w3.org/2004/02/skos/core#> .
@prefix af-cur: <http://purl.allotrope.org/ontologies/curation#> .
@base <http://purl.allotrope.org/voc/afo/domain/WD/2025/06/auger#> .

<http://purl.allotrope.org/voc/afo/domain/WD/2025/06/auger> rdf:type owl:Ontology ;
                                                                       owl:versionIRI <http://purl.allotrope.org/voc/afo/domain/WD/2025/06/auger> ;
                                                                       owl:imports <http://purl.allotrope.org/voc/afo/WD/2025/06/afo> ;
                                                                       dct:issued "2025-06-25T12:00:00Z"^^xsd:dateTime ;
                                                                       dct:license <http://purl.allotrope.org/voc/creative-commons-attribution-license> ;
                                                                       dct:modified "2025-04-04T12:00:00Z"^^xsd:dateTime ;
                                                                       dct:rights <http://purl.allotrope.org/voc/attribution> ,
                                                                                  <http://purl.allotrope.org/voc/copyright> ;
                                                                       dct:rightsHolder <http://www.allotrope.org> ;
                                                                       dct:title "AFO Auger Domain Ontology (WD/2025/06)" ;
                                                                       owl:priorVersion <http://purl.allotrope.org/voc/afo/domain/WD/2018/04/auger> ;
                                                                       owl:versionInfo "WD/2025/06" .

#################################################################
#    Annotation properties
#################################################################

###  http://purl.allotrope.org/ontologies/property#AFX_0002796
af-x:AFX_0002796 rdf:type owl:AnnotationProperty .


###  http://purl.allotrope.org/ontologies/property#AFX_0002798
af-x:AFX_0002798 rdf:type owl:AnnotationProperty .


###  http://purl.allotrope.org/ontologies/property#AFX_0002809
af-x:AFX_0002809 rdf:type owl:AnnotationProperty .


###  http://purl.org/dc/terms/source
dct:source rdf:type owl:AnnotationProperty .


###  http://www.w3.org/2004/02/skos/core#altLabel
skos:altLabel rdf:type owl:AnnotationProperty .


###  http://www.w3.org/2004/02/skos/core#changeNote
skos:changeNote rdf:type owl:AnnotationProperty .


###  http://www.w3.org/2004/02/skos/core#definition
skos:definition rdf:type owl:AnnotationProperty .


###  http://www.w3.org/2004/02/skos/core#example
skos:example rdf:type owl:AnnotationProperty .


###  http://www.w3.org/2004/02/skos/core#note
skos:note rdf:type owl:AnnotationProperty .


###  http://www.w3.org/2004/02/skos/core#prefLabel
skos:prefLabel rdf:type owl:AnnotationProperty .


###  http://www.w3.org/2004/02/skos/core#scopeNote
skos:scopeNote rdf:type owl:AnnotationProperty .


#################################################################
#    Classes
#################################################################

###  http://purl.allotrope.org/ontologies/process#AFP_0000011
af-p:AFP_0000011 rdf:type owl:Class ;
                 rdfs:subClassOf af-p:AFP_0002325 ;
                 skos:altLabel "angle-resolved resonance Auger electron spectrometry" ,
                               "angle-resolved resonance Auger electron spectroscopy" ,
                               "angle-resolved resonant Auger electron spectrometry" ;
                 skos:definition "A type of spectroscopy where bombardment of a sample with high-energy photons results in the ionization of core electrons and the emission of so-called 'Auger' electrons. The wavelength of the incident photons is scanned over an absorption edge in the sample and the Auger electrons emitted are detected as a function of emission angle. [CHMO]" ;
                 skos:prefLabel "angle-resolved resonant Auger electron spectroscopy" .


###  http://purl.allotrope.org/ontologies/process#AFP_0000089
af-p:AFP_0000089 rdf:type owl:Class ;
                 rdfs:subClassOf af-p:AFP_0001526 ;
                 skos:altLabel "ion neutralisation spectrometry"@en-gb ,
                               "ion neutralisation spectroscopy"@en-gb ,
                               "IAES" ,
                               "IEAES" ,
                               "IES" ,
                               "IIAES" ,
                               "INS" ,
                               "ion neutralization spectrometry" ,
                               "ion neutralization spectroscopy" ,
                               "ion-electron spectroscopy" ,
                               "ion-excited Auger spectrometry" ,
                               "ion-induced Auger electron spectrometry" ,
                               "ion-induced Auger electron spectroscopy" ,
                               "ionelectron spectroscopy" ;
                 skos:definition "Any type of spectroscopy where ion bombardment of a sample results in the ionization of core electrons and the emission of so-called 'Auger' electrons, which are detected as a function of incident ion energy. [CHMO]" ;
                 skos:prefLabel "ion-excited Auger electron spectroscopy" .


###  http://purl.allotrope.org/ontologies/process#AFP_0000179
af-p:AFP_0000179 rdf:type owl:Class ;
                 rdfs:subClassOf af-p:AFP_0000089 ;
                 skos:altLabel "HAES" ,
                               "He+-excited Auger electron spectrometry" ;
                 skos:definition "A type of spectroscopy where the bombardment of a sample with He+ ions results in the ionization of core electrons and the emission of so-called 'Auger' electrons, which are detected as a function of incident He+ ion energy. [CHMO]" ;
                 skos:prefLabel "He+-excited Auger electron spectroscopy" .


###  http://purl.allotrope.org/ontologies/process#AFP_0000431
af-p:AFP_0000431 rdf:type owl:Class ;
                 rdfs:subClassOf af-p:AFP_0002460 ;
                 skos:altLabel "CX-AES" ,
                               "CXAES" ,
                               "bremsstrahlung Auger electron spectrometry" ,
                               "bremsstrahlung Auger electron spectroscopy" ,
                               "bremsstrahlung Auger spectrometry" ,
                               "bremsstrahlung Auger spectroscopy" ,
                               "continuous X-ray-induced Auger electron spectrometry" ,
                               "continuous X-ray-induced Auger spectrometry" ,
                               "continuous X-ray-induced Auger spectroscopy" ;
                 skos:definition "A type of spectroscopy where the bombardment of a sample with a continuous X-ray source (X-rays generated when electrons - or other high energy charged particles such as protons or alpha-particles - lose energy whilst passing through the Coulomb field of a nucleus) results in the ionization of core electrons and the emission of so-called 'Auger' electrons, which are detected. [CHMO]" ;
                 skos:prefLabel "continuous X-ray-induced Auger electron spectroscopy" .


###  http://purl.allotrope.org/ontologies/process#AFP_0000539
af-p:AFP_0000539 rdf:type owl:Class ;
                 rdfs:subClassOf af-p:AFP_0000089 ;
                 skos:altLabel "PAES" ,
                               "proton-induced Auger electron spectrometry" ;
                 skos:definition "A type of spectroscopy where the bombardment of a sample with protons results in the ionization of core electrons and the emission of so-called 'Auger' electrons, which are detected as a function of incident proton energy. [CHMO]" ;
                 skos:prefLabel "proton-induced Auger electron spectroscopy" .


###  http://purl.allotrope.org/ontologies/process#AFP_0000670
af-p:AFP_0000670 rdf:type owl:Class ;
                 rdfs:subClassOf af-p:AFP_0001526 ;
                 skos:altLabel "APYS" ,
                               "Auger electron partial yield spectrometry" ;
                 skos:definition "A type of spectroscopy where bombardment of a sample with high-energy photons results in the ionization of core electrons and the emission of so-called 'Auger' electrons. Only the Auger electrons emitted at a particular photon energy are detected. [CHMO]" ;
                 skos:prefLabel "Auger electron partial yield spectroscopy" .


###  http://purl.allotrope.org/ontologies/process#AFP_0000885
af-p:AFP_0000885 rdf:type owl:Class ;
                 rdfs:subClassOf af-p:AFP_0001526 ;
                 skos:altLabel "SPAES" ;
                 skos:definition "A type of spectroscopy where the bombardment of a sample with high-energy photons results in the ionization of core electrons and the emission of so-called 'Auger' electrons. The energies of these Auger electrons are detected as a function of incident photon energy and a magnet is used to align all electron spins parallel to the emitting surface. [CHMO]" ;
                 skos:prefLabel "spin-polarised Auger electron spectroscopy"@en-gb ,
                                "spin-polarized Auger electron spectrometry" .


###  http://purl.allotrope.org/ontologies/process#AFP_0000919
af-p:AFP_0000919 rdf:type owl:Class ;
                 rdfs:subClassOf af-p:AFP_0000089 ;
                 skos:altLabel "AIRES" ,
                               "angle-resolved ion-electron spectrometry" ,
                               "angle-resolved ion-electron spectroscopy" ;
                 skos:definition "Any type of spectroscopy where ion bombardment of a sample results in the ionization of core electrons and the emission of so-called 'Auger' electrons, which are detected as a function of emission angle. [CHMO]" ;
                 skos:prefLabel "angle-resolved ion-excited Auger electron spectroscopy" .


###  http://purl.allotrope.org/ontologies/process#AFP_0001059
af-p:AFP_0001059 rdf:type owl:Class ;
                 rdfs:subClassOf af-p:AFP_0001526 ;
                 skos:altLabel "ADAS" ,
                               "ARAES" ,
                               "angle-resolved Auger electron spectrometry" ,
                               "angle-resolved Auger electron spectroscopy" ,
                               "angular dependent Auger spectrometry" ;
                 skos:definition "A type of spectroscopy where bombardment of a sample with high-energy photons results in the ionization of core electrons and the emission of so-called 'Auger' electrons. The energies of these Auger electrons are detected as a function of emission angle. [CHMO]" ;
                 skos:prefLabel "angular dependent Auger electron spectroscopy" .


###  http://purl.allotrope.org/ontologies/process#AFP_0001249
af-p:AFP_0001249 rdf:type owl:Class ;
                 rdfs:subClassOf af-p:AFP_0001526 ;
                 skos:altLabel "EAES" ,
                               "EEAES" ,
                               "EIAES" ,
                               "electron-excited Auger electron spectrometry" ,
                               "electron-induced Auger electron spectrometry" ,
                               "electron-induced Auger electron spectroscopy " ;
                 skos:definition "A type of spectroscopy where electron bombardment of a sample results in the ionization of core electrons and the emission of so-called 'Auger' electron and the energies of these Auger electrons are detected as a function of incident electron energy. [CHMO]" ;
                 skos:prefLabel "electron-excited Auger electron spectroscopy" .


###  http://purl.allotrope.org/ontologies/process#AFP_0001490
af-p:AFP_0001490 rdf:type owl:Class ;
                 rdfs:subClassOf af-p:AFP_0000757 ;
                 skos:altLabel "polarised secondary electron spectrometry"@en-gb ,
                               "spin-polarised secondary electron spectrometry"@en-gb ,
                               "spin-polarised secondary electron spectroscopy"@en-gb ,
                               "polarized secondary electron spectrometry" ,
                               "polarized secondary electron spectroscopy" ,
                               "spin-polarized secondary electron spectrometry" ,
                               "spin-resolved secondary electron spectrometry" ,
                               "spin-resolved secondary electron spectroscopy" .


###  http://purl.allotrope.org/ontologies/process#AFP_0001539
af-p:AFP_0001539 rdf:type owl:Class ;
                 rdfs:subClassOf af-p:AFP_0001835 ;
                 skos:altLabel "EXFAS" ,
                               "SEELFS" ,
                               "extended fine Auger structures" .


###  http://purl.allotrope.org/ontologies/process#AFP_0001917
af-p:AFP_0001917 rdf:type owl:Class ;
                 rdfs:subClassOf af-p:AFP_0001249 ;
                 skos:altLabel "Auger electron microanalysis" ,
                               "EMAS" ,
                               "electron microprobe Auger electron spectrometry" ;
                 skos:definition "A type of spectroscopy where bombardment of a sample with a finely focused (<10 m diameter) beam of electrons results in the ionization of core electrons and the emission of so-called 'Auger' electrons. The energies of these Auger electrons are detected as a function of incident electron energy. [CHMO]" ;
                 skos:prefLabel "electron microprobe Auger spectroscopy" .


###  http://purl.allotrope.org/ontologies/process#AFP_0002036
af-p:AFP_0002036 rdf:type owl:Class ;
                 rdfs:subClassOf af-p:AFP_0000885 ;
                 skos:altLabel "SPARPES" ;
                 skos:definition "A type of spectroscopy where the bombardment of a sample with high-energy photons results in the ionization of core electrons and the emission of so-called 'Auger' electrons. The energies of these Auger electrons are detected as a function of emission angle and a magnet is used to align all electron spins parallel to the emitting surface. [CHMO]" ;
                 skos:prefLabel "spin-polarised angle-resolved Auger electron spectroscopy"@en-gb ,
                                "spin-polarized angle-resolved Auger electron spectometry" .


###  http://purl.allotrope.org/ontologies/process#AFP_0002266
af-p:AFP_0002266 rdf:type owl:Class ;
                 rdfs:subClassOf af-p:AFP_0001526 ;
                 skos:altLabel "SAES" ,
                               "scanning Auger electron spectrometry" ,
                               "scanning Auger spectrometry" ,
                               "scanning Auger spectroscopy" ;
                 skos:definition "A type of spectroscopy where a high-energy photon beam is scanned over the surface of a sample resulting in the ionization of core electrons and the emission of so-called 'Auger' electrons. The energies of these Auger electrons are detected as a function of incident photon energy. [CHMO]" ;
                 skos:prefLabel "scanning Auger electron spectroscopy" .


###  http://purl.allotrope.org/ontologies/process#AFP_0002325
af-p:AFP_0002325 rdf:type owl:Class ;
                 rdfs:subClassOf af-p:AFP_0001526 ;
                 skos:altLabel "RAES" ,
                               "resonance AES" ,
                               "resonance Auger electron spectrometry" ,
                               "resonance Auger electron spectroscopy" ,
                               "resonance Auger spectrometry" ,
                               "resonance Auger spectroscopy" ,
                               "resonant AES" ,
                               "resonant Auger electron spectrometry" ,
                               "resonant Auger spectrometry" ,
                               "resonant Auger spectroscopy" ;
                 skos:definition "A type of spectroscopy where bombardment of a sample with high-energy photons results in the ionization of core electrons and the emission of so-called 'Auger' electrons. The wavelength of the incident photons is scanned over an absorption edge in the sample and the Auger electrons emitted are detected as a function of energy. [CHMO]" ;
                 skos:prefLabel "resonant Auger electron spectroscopy" .


###  http://purl.allotrope.org/ontologies/process#AFP_0002380
af-p:AFP_0002380 rdf:type owl:Class ;
                 rdfs:subClassOf af-p:AFP_0002334 ;
                 skos:altLabel "AEAPS" ,
                               "Auger electron appearance potential spectrometry" ,
                               "EAAPS" ,
                               "IEMM" ,
                               "electron-excited Auger electron appearance potential spectrometry" ,
                               "electron-excited Auger electron appearance potential spectroscopy" ,
                               "incident energy modulation method spectrometry" ,
                               "incident energy modulation method spectroscopy" .


###  http://purl.allotrope.org/ontologies/process#AFP_0002460
af-p:AFP_0002460 rdf:type owl:Class ;
                 rdfs:subClassOf af-p:AFP_0001526 ;
                 skos:altLabel "X-ray excited Auger electron spectrometry" ,
                               "X-ray induced Auger electron spectrometry" ,
                               "X-ray induced Auger electron spectroscopy" ,
                               "XAES" ,
                               "XEAES" ,
                               "XIAES" ;
                 skos:definition "A type of spectroscopy where X-ray bombardment of a sample results in the ionization of core electrons and the emission of so-called 'Auger' electrons, which are detected as a function of incident X-ray energy. [CHMO]" ;
                 skos:prefLabel "X-ray excited Auger electron spectroscopy" .


#################################################################
#    Individuals
#################################################################

###  http://purl.allotrope.org/voc/attribution
<http://purl.allotrope.org/voc/attribution> rdf:type owl:NamedIndividual ,
                                                     dct:RightsStatement ;
                                            dct:description """
These taxonomies contain material or may constitute derivative works of material which may be subject to copyright by one of the following organizations.  By using these taxonomies, you agree to the following terms and conditions applicable to its contents:
******************************************************************************
Copyright Notice and Terms for IUPAC Gold Book
______________________________________________________________________________
Copyright © 1998, Regents of the University of California
All rights reserved.
Redistribution and use in source and binary forms, with or without modification, are permitted provided that the following conditions are met:
1. Redistributions of source code must retain the above copyright notice, this list of conditions and the following disclaimer.
2. Redistributions in binary form must reproduce the above copyright notice, this list of conditions and the following disclaimer in the documentation and/or other materials provided with the distribution.
THIS SOFTWARE IS PROVIDED BY THE COPYRIGHT HOLDERS AND CONTRIBUTORS \"AS IS\" AND ANY EXPRESS OR IMPLIED WARRANTIES, INCLUDING, BUT NOT LIMITED TO, THE IMPLIED WARRANTIES OF MERCHANTABILITY AND FITNESS FOR A PARTICULAR PURPOSE ARE DISCLAIMED. IN NO EVENT SHALL THE COPYRIGHT HOLDER OR CONTRIBUTORS BE LIABLE FOR ANY DIRECT, INDIRECT, INCIDENTAL, SPECIAL, EXEMPLARY, OR CONSEQUENTIAL DAMAGES (INCLUDING, BUT NOT LIMITED TO, PROCUREMENT OF SUBSTITUTE GOODS OR SERVICES; LOSS OF USE, DATA, OR PROFITS; OR BUSINESS INTERRUPTION) HOWEVER CAUSED AND ON ANY THEORY OF LIABILITY, WHETHER IN CONTRACT, STRICT LIABILITY, OR TORT (INCLUDING NEGLIGENCE OR OTHERWISE) ARISING IN ANY WAY OUT OF THE USE OF THIS SOFTWARE, EVEN IF ADVISED OF THE POSSIBILITY OF SUCH DAMAGE.
******************************************************************************
Copyright Notice and Terms for PSI-MS (Proteomics Standards Initiative - Mass Spectrometry) Mass spectrometer output files and spectra interpretation
_____________________________________________________________________________
Created by Matt Chambers, Andreas Bertsch, Marius Kallhardt, Eric Deutsch Fredrik Levander, Pierre-Alain Binz, and Gerhard Mayer. Publisher: HUPO Proteomics Standards Initiative Mass Spectrometry Standards Working Group and HUPO Proteomics Standards Initiative Proteomics Informatics Working Group. This work is used pursuant to a Creative Commons license available here: http://creativecommons.org/licenses/by/3.0/legalcode

******************************************************************************
Attribution Notice for National Center for Biomedical Ontology materials.

This work contains material from the Cell Ontology and Clinical Measurement Ontology, available here: http://bioportal.bioontology.org/.
******************************************************************************
Attribution Notice for ChEBI
This work contains material from the European Bioinformatics Institute’s ChEBI database.
******************************************************************************
Attribution Notice for Quantities Units Dimensions Data Types (http://www.qudt.org/)
This work contains content from www.qudt.org and is used pursuant to a Creative Commons License available here: http://creativecommons.org/licenses/by-sa/3.0/us/legalcode. The original work may have been modified.
******************************************************************************
Copyright and Attribution Notice for Dublin Core Metadata Initiative Document
This work contains material from the following DCMI document used pursuant to a creative commons license available here: https://creativecommons.org/licenses/by/4.0/legalcode. This material may have been modified or changed.
Timestamped URL:          http://dublincore.org/documents/2012/06/14/dcmi-terms/
Date Issued:                       2012-06-14
Document Status:            This is a DCMI Recommendation.
Copyright © 1995-2015 DCMI. All Rights Reserved. DCMI liability, trademark/service mark, document use and software licensing rules apply.
******************************************************************************

""" ;
                                            dct:title "Derivative works attribution" .


###  http://purl.allotrope.org/voc/copyright
<http://purl.allotrope.org/voc/copyright> rdf:type owl:NamedIndividual ,
                                                   dct:RightsStatement ;
                                          dct:description "(c) 2017 Allotrope Foundation" ;
                                          dct:title "(c) 2017 Allotrope Foundation" .


###  http://purl.allotrope.org/voc/creative-commons-attribution-license
<http://purl.allotrope.org/voc/creative-commons-attribution-license> rdf:type owl:NamedIndividual ,
                                                                              dct:LicenseDocument ;
                                                                     dct:description """This work is licensed under a Creative Commons Attribution 4.0 International License http://creativecommons.org/licenses/by/4.0/.

THESE MATERIALS ARE PROVIDED \"AS IS\" AND ALLOTROPE EXPRESSLY DISCLAIMS ALL WARRANTIES, EXPRESS, IMPLIED OR STATUTORY, INCLUDING, WITHOUT LIMITATION, THE WARRANTIES OF NON-INFRINGEMENT, TITLE, MERCHANTABILITY AND FITNESS FOR A PARTICULAR PURPOSE.

Copyright © 2015-2025 Allotrope Foundation
""" ;
                                                                     dct:title "Creative Commons Attribution 4.0 International Public License" .


###  http://purl.allotrope.org/voc/afo/domain/WD/2025/06/auger
<http://purl.allotrope.org/voc/afo/domain/WD/2025/06/auger> rdf:type owl:NamedIndividual .


###  Generated by the OWL API (version 5.1.19) https://github.com/owlcs/owlapi/
