@prefix : <http://purl.allotrope.org/voc/afo/domain/WD/2025/06/differential-scanning-calorimetry#> .
@prefix dct: <http://purl.org/dc/terms/> .
@prefix owl: <http://www.w3.org/2002/07/owl#> .
@prefix rdf: <http://www.w3.org/1999/02/22-rdf-syntax-ns#> .
@prefix xml: <http://www.w3.org/XML/1998/namespace> .
@prefix xsd: <http://www.w3.org/2001/XMLSchema#> .
@prefix af-c: <http://purl.allotrope.org/ontologies/common#> .
@prefix af-e: <http://purl.allotrope.org/ontologies/equipment#> .
@prefix af-m: <http://purl.allotrope.org/ontologies/material#> .
@prefix af-p: <http://purl.allotrope.org/ontologies/process#> .
@prefix af-q: <http://purl.allotrope.org/ontologies/quality#> .
@prefix af-r: <http://purl.allotrope.org/ontologies/result#> .
@prefix af-x: <http://purl.allotrope.org/ontologies/property#> .
@prefix rdfs: <http://www.w3.org/2000/01/rdf-schema#> .
@prefix skos: <http://www.w3.org/2004/02/skos/core#> .
@prefix af-cur: <http://purl.allotrope.org/ontologies/curation#> .
@base <http://purl.allotrope.org/voc/afo/domain/WD/2025/06/differential-scanning-calorimetry#> .

<http://purl.allotrope.org/voc/afo/domain/WD/2025/06/differential-scanning-calorimetry> rdf:type owl:Ontology ;
                                                                                                   owl:versionIRI <http://purl.allotrope.org/voc/afo/domain/WD/2025/06/differential-scanning-calorimetry> ;
                                                                                                   owl:imports <http://purl.allotrope.org/voc/afo/WD/2025/06/afo> ,
                                                                                                               <http://purl.allotrope.org/voc/afo/domain/REC/2025/06/differential-scanning-calorimetry> ;
                                                                                                   dct:issued "2025-06-25T12:00:00Z"^^xsd:dateTime ;
                                                                                                   dct:license <http://purl.allotrope.org/voc/creative-commons-attribution-license> ;
                                                                                                   dct:modified "2025-04-04T12:00:00Z"^^xsd:dateTime ;
                                                                                                   dct:rights <http://purl.allotrope.org/voc/attribution> ,
                                                                                                              <http://purl.allotrope.org/voc/copyright> ;
                                                                                                   dct:title "AFO Differential Scanning Calorimetry (DSC) Domain Ontology (WD/2025/06)" ;
                                                                                                   owl:priorVersion <http://purl.allotrope.org/voc/afo/domain/WD/2018/11/differential-scanning-calorimetry> ;
                                                                                                   owl:versionInfo "WD/2025/06" .

#################################################################
#    Annotation properties
#################################################################

###  http://purl.allotrope.org/ontologies/property#AFX_0002796
af-x:AFX_0002796 rdf:type owl:AnnotationProperty .


###  http://purl.allotrope.org/ontologies/property#AFX_0002798
af-x:AFX_0002798 rdf:type owl:AnnotationProperty .


###  http://purl.allotrope.org/ontologies/property#AFX_0002809
af-x:AFX_0002809 rdf:type owl:AnnotationProperty .


###  http://purl.org/dc/terms/source
dct:source rdf:type owl:AnnotationProperty .


###  http://www.w3.org/2004/02/skos/core#altLabel
skos:altLabel rdf:type owl:AnnotationProperty .


###  http://www.w3.org/2004/02/skos/core#changeNote
skos:changeNote rdf:type owl:AnnotationProperty .


###  http://www.w3.org/2004/02/skos/core#definition
skos:definition rdf:type owl:AnnotationProperty .


###  http://www.w3.org/2004/02/skos/core#example
skos:example rdf:type owl:AnnotationProperty .


###  http://www.w3.org/2004/02/skos/core#note
skos:note rdf:type owl:AnnotationProperty .


###  http://www.w3.org/2004/02/skos/core#prefLabel
skos:prefLabel rdf:type owl:AnnotationProperty .


###  http://www.w3.org/2004/02/skos/core#scopeNote
skos:scopeNote rdf:type owl:AnnotationProperty .


#################################################################
#    Object Properties
#################################################################

###  http://purl.allotrope.org/ontologies/property#AFX_0000425
af-x:AFX_0000425 rdf:type owl:ObjectProperty ;
                 rdfs:subPropertyOf af-x:AFX_0001159 ;
                 rdfs:range af-p:AFP_0002650 ;
                 skos:definition "The feedback mode code of the type of feedback between reference and sample heat cell during a differential scanning calorimetry measurement. [Allotrope]" ;
                 skos:prefLabel "feedback mode code" .


###  http://purl.allotrope.org/ontologies/property#AFX_0001159
af-x:AFX_0001159 rdf:type owl:ObjectProperty .


#################################################################
#    Classes
#################################################################

###  http://purl.allotrope.org/ontologies/process#AFP_0000427
af-p:AFP_0000427 rdf:type owl:Class ;
                 rdfs:subClassOf af-p:AFP_0002124 ;
                 skos:altLabel "power-compensation DSC" ;
                 skos:definition "The measurement of thermodynamic parameters (e.g. enthalpy) during a chemical or biochemical reaction of both a sample and a reference, by the known variation (step-wise or linear) of one variable, whilst a second is kept constant using a power compensation differential scanning calorimeter. [CHMO]" ;
                 skos:prefLabel "power-compensation differential scanning calorimetry" .


###  http://purl.allotrope.org/ontologies/process#AFP_0000595
af-p:AFP_0000595 rdf:type owl:Class ;
                 rdfs:subClassOf af-p:AFP_0002124 ;
                 skos:altLabel "TMDSC" ;
                 skos:definition "The measurement of thermodynamic parameters (e.g. enthalpy) during a chemical or biochemical reaction of both a sample and a reference, by the known variation (step-wise or linear) of temperature whilst a second variable is kept constant. [CHMO]" ;
                 skos:prefLabel "temperature-modulated differential scanning calorimetry" .


###  http://purl.allotrope.org/ontologies/process#AFP_0001402
af-p:AFP_0001402 rdf:type owl:Class ;
                 rdfs:subClassOf af-p:AFP_0000595 ;
                 skos:altLabel "DDSCle and a reference, by the known variation (step-wise or linear) of temperature whilst a second variable is kept constant. The power input is in the form of a saw-tooth wave. [CHMO]" ;
                 skos:prefLabel "dynamic differential scanning calorimetry" .


###  http://purl.allotrope.org/ontologies/process#AFP_0002132
af-p:AFP_0002132 rdf:type owl:Class ;
                 rdfs:subClassOf af-p:AFP_0000595 ;
                 skos:altLabel "MDSC" ;
                 skos:definition "The measurement of thermodynamic parameters (e.g. enthalpy) during a chemical or biochemical reaction of both a sample and a reference, by the known variation (step-wise or linear) of temperature whilst a second variable is kept constant. The power input is in the form of a sine wave. [CHMO]" ;
                 skos:prefLabel "modulated differential scanning calorimetry" .


###  http://purl.allotrope.org/ontologies/process#AFP_0002225
af-p:AFP_0002225 rdf:type owl:Class ;
                 rdfs:subClassOf af-p:AFP_0002124 ;
                 skos:altLabel "heat-flux DSC" ;
                 skos:definition "The measurement of thermodynamic parameters (e.g. enthalpy) during a chemical or biochemical reaction of both a sample and a reference, by the known variation (step-wise or linear) of one variable, whilst a second is kept constant using a heat-flux differential scanning calorimeter. [CHMO]" ;
                 skos:prefLabel "heat-flux differential scanning calorimetry" .


###  http://purl.allotrope.org/ontologies/process#AFP_0002650
af-p:AFP_0002650 rdf:type owl:Class ;
                 rdfs:subClassOf af-c:AFC_0000050 ;
                 skos:altLabel "FB mode code" ,
                               "feedback mode code" ;
                 skos:definition "The FB mode code is the code of the feedback mode used for a DSC measurement. [Allotrope]" ;
                 skos:prefLabel "differential scanning calorimetry feedback mode code" .


###  http://purl.allotrope.org/ontologies/process#AFP_0002694
af-p:AFP_0002694 rdf:type owl:Class ;
                 rdfs:subClassOf af-p:AFP_0002124 ;
                 skos:definition "Isothermal differential scanning calorimetry is a type of differential scanning calorimetry where the measurement takes place at constant temperature. [Allotrope]" ;
                 skos:prefLabel "isothermal differential scanning calorimetry" .


###  http://purl.allotrope.org/ontologies/process#AFP_0002697
af-p:AFP_0002697 rdf:type owl:Class ;
                 rdfs:subClassOf af-c:AFC_0000050 ;
                 skos:altLabel "DSC mode code" ;
                 skos:definition "The differential scanning calorimetry scan mode code encodes the mode of measurement of DSC. [Allotrope]" ;
                 skos:prefLabel "differential scanning calorimetry scan mode code" .


###  http://purl.allotrope.org/ontologies/result#AFR_0000238
af-r:AFR_0000238 rdf:type owl:Class ;
                 rdfs:subClassOf af-r:AFR_0000576 ;
                 skos:altLabel "heat release rate curve" ,
                               "heat-release rate curve" ,
                               "heat-release-rate curves" ;
                 skos:definition "A plot of heat release (W/m2) vs. time obtained during a calorimetry experiment. [CHMO]" ;
                 skos:prefLabel "heat-release-rate curve" .


#################################################################
#    Individuals
#################################################################

###  http://purl.allotrope.org/ontologies/process#AFP_0002696
af-p:AFP_0002696 rdf:type owl:NamedIndividual ,
                          af-p:AFP_0002697 ;
                 skos:definition "Upscan mode is a scan mode of differential scanning calorimetry that proceeds with increasing temperature. [Allotrope]" ;
                 skos:prefLabel "upscan" .


###  http://purl.allotrope.org/ontologies/process#AFP_0002703
af-p:AFP_0002703 rdf:type owl:NamedIndividual ,
                          af-p:AFP_0002697 ;
                 skos:definition "The code of isothermal DSC scan mode for scanning at a constant temperature. [Allotrope]" ;
                 skos:prefLabel "isothermal" .


###  http://purl.allotrope.org/ontologies/process#AFP_0002714
af-p:AFP_0002714 rdf:type owl:NamedIndividual ,
                          af-p:AFP_0002650 ;
                 skos:altLabel "medium feedback" ,
                               "mid FB" ,
                               "mid feedback" ;
                 skos:definition "The code of feedback mode of DSC measurements that have medium active compensation of differences of cell temperatures. [Allotrope]" ;
                 skos:prefLabel "mid" .


###  http://purl.allotrope.org/ontologies/process#AFP_0002743
af-p:AFP_0002743 rdf:type owl:NamedIndividual ,
                          af-p:AFP_0002650 ;
                 skos:altLabel "high FB" ,
                               "high feedback" ;
                 skos:definition "The code of feedback mode of DSC measurements that have high active compensation of differences of cell temperatures. [Allotrope]" ;
                 skos:prefLabel "high" .


###  http://purl.allotrope.org/ontologies/process#AFP_0002765
af-p:AFP_0002765 rdf:type owl:NamedIndividual ,
                          af-p:AFP_0002650 ;
                 skos:altLabel "no feedback" ,
                               "passive" ,
                               "passive feedback" ;
                 skos:definition "The code of feedback mode of DSC measurements that have no active compensation of differences of cell temperatures. [Allotrope]" ;
                 skos:prefLabel "none" .


###  http://purl.allotrope.org/ontologies/process#AFP_0002774
af-p:AFP_0002774 rdf:type owl:NamedIndividual ,
                          af-p:AFP_0002697 ;
                 skos:definition "The code of conventional DSC scan mode for scanning up/down at constant scan rate. [Allotrope]" ;
                 skos:prefLabel "conventional" .


###  http://purl.allotrope.org/ontologies/process#AFP_0002776
af-p:AFP_0002776 rdf:type owl:NamedIndividual ,
                          af-p:AFP_0002650 ;
                 skos:altLabel "low FB" ,
                               "low feedback" ;
                 skos:definition "The code of feedback mode of DSC measurements that have low active compensation of differences of cell temperatures. [Allotrope]" ;
                 skos:prefLabel "low" .


###  http://purl.allotrope.org/ontologies/process#AFP_0002804
af-p:AFP_0002804 rdf:type owl:NamedIndividual ,
                          af-p:AFP_0002697 ;
                 skos:definition "Downscan mode is a scan mode of differential scanning calorimetry that proceeds with decreasing temperature. [Allotrope]" ;
                 skos:prefLabel "downscan" .


###  http://purl.allotrope.org/ontologies/process#AFP_0002819
af-p:AFP_0002819 rdf:type owl:NamedIndividual ,
                          af-p:AFP_0002697 ;
                 skos:definition "The code of compressibility DSC scan mode for studying volumetric properties. [Allotrope]" ;
                 skos:prefLabel "compressibility" .


###  http://purl.allotrope.org/voc/attribution
<http://purl.allotrope.org/voc/attribution> rdf:type owl:NamedIndividual ,
                                                     dct:RightsStatement ;
                                            dct:description """
These taxonomies contain material or may constitute derivative works of material which may be subject to copyright by one of the following organizations.  By using these taxonomies, you agree to the following terms and conditions applicable to its contents:
******************************************************************************
Copyright Notice and Terms for IUPAC Gold Book
______________________________________________________________________________
Copyright © 1998, Regents of the University of California
All rights reserved.
Redistribution and use in source and binary forms, with or without modification, are permitted provided that the following conditions are met:
1. Redistributions of source code must retain the above copyright notice, this list of conditions and the following disclaimer.
2. Redistributions in binary form must reproduce the above copyright notice, this list of conditions and the following disclaimer in the documentation and/or other materials provided with the distribution.
THIS SOFTWARE IS PROVIDED BY THE COPYRIGHT HOLDERS AND CONTRIBUTORS \"AS IS\" AND ANY EXPRESS OR IMPLIED WARRANTIES, INCLUDING, BUT NOT LIMITED TO, THE IMPLIED WARRANTIES OF MERCHANTABILITY AND FITNESS FOR A PARTICULAR PURPOSE ARE DISCLAIMED. IN NO EVENT SHALL THE COPYRIGHT HOLDER OR CONTRIBUTORS BE LIABLE FOR ANY DIRECT, INDIRECT, INCIDENTAL, SPECIAL, EXEMPLARY, OR CONSEQUENTIAL DAMAGES (INCLUDING, BUT NOT LIMITED TO, PROCUREMENT OF SUBSTITUTE GOODS OR SERVICES; LOSS OF USE, DATA, OR PROFITS; OR BUSINESS INTERRUPTION) HOWEVER CAUSED AND ON ANY THEORY OF LIABILITY, WHETHER IN CONTRACT, STRICT LIABILITY, OR TORT (INCLUDING NEGLIGENCE OR OTHERWISE) ARISING IN ANY WAY OUT OF THE USE OF THIS SOFTWARE, EVEN IF ADVISED OF THE POSSIBILITY OF SUCH DAMAGE.
******************************************************************************
Copyright Notice and Terms for PSI-MS (Proteomics Standards Initiative - Mass Spectrometry) Mass spectrometer output files and spectra interpretation
_____________________________________________________________________________
Created by Matt Chambers, Andreas Bertsch, Marius Kallhardt, Eric Deutsch Fredrik Levander, Pierre-Alain Binz, and Gerhard Mayer. Publisher: HUPO Proteomics Standards Initiative Mass Spectrometry Standards Working Group and HUPO Proteomics Standards Initiative Proteomics Informatics Working Group. This work is used pursuant to a Creative Commons license available here: http://creativecommons.org/licenses/by/3.0/legalcode

******************************************************************************
Attribution Notice for National Center for Biomedical Ontology materials.

This work contains material from the Cell Ontology and Clinical Measurement Ontology, available here: http://bioportal.bioontology.org/.
******************************************************************************
Attribution Notice for ChEBI
This work contains material from the European Bioinformatics Institute’s ChEBI database.
******************************************************************************
Attribution Notice for Quantities Units Dimensions Data Types (http://www.qudt.org/)
This work contains content from www.qudt.org and is used pursuant to a Creative Commons License available here: http://creativecommons.org/licenses/by-sa/3.0/us/legalcode. The original work may have been modified.
******************************************************************************
Copyright and Attribution Notice for Dublin Core Metadata Initiative Document
This work contains material from the following DCMI document used pursuant to a creative commons license available here: https://creativecommons.org/licenses/by/4.0/legalcode. This material may have been modified or changed.
Timestamped URL:          http://dublincore.org/documents/2012/06/14/dcmi-terms/
Date Issued:                       2012-06-14
Document Status:            This is a DCMI Recommendation.
Copyright © 1995-2015 DCMI. All Rights Reserved. DCMI liability, trademark/service mark, document use and software licensing rules apply.
******************************************************************************

""" ;
                                            dct:title "Derivative works attribution" .


###  http://purl.allotrope.org/voc/copyright
<http://purl.allotrope.org/voc/copyright> rdf:type owl:NamedIndividual ,
                                                   dct:RightsStatement ;
                                          dct:description "Copyright © 2019 Allotrope Foundation" ;
                                          dct:rightsHolder <http://www.allotrope.org> ;
                                          dct:title "Copyright © 2019 Allotrope Foundation" .


###  http://purl.allotrope.org/voc/creative-commons-attribution-license
<http://purl.allotrope.org/voc/creative-commons-attribution-license> rdf:type owl:NamedIndividual ,
                                                                              dct:LicenseDocument ;
                                                                     dct:description """This work is licensed under a Creative Commons Attribution 4.0 International License http://creativecommons.org/licenses/by/4.0/.

THESE MATERIALS ARE PROVIDED \"AS IS\" AND ALLOTROPE EXPRESSLY DISCLAIMS ALL WARRANTIES, EXPRESS, IMPLIED OR STATUTORY, INCLUDING, WITHOUT LIMITATION, THE WARRANTIES OF NON-INFRINGEMENT, TITLE, MERCHANTABILITY AND FITNESS FOR A PARTICULAR PURPOSE.

Copyright © 2015-2025 Allotrope Foundation
""" ;
                                                                     dct:title "Creative Commons Attribution 4.0 International Public License" .


###  Generated by the OWL API (version 5.1.19) https://github.com/owlcs/owlapi/
