@prefix : <http://purl.allotrope.org/voc/afo/domain/WD/2025/06/electrophoresis#> .
@prefix cl: <http://purl.obolibrary.org/obo/CL> .
@prefix go: <http://purl.obolibrary.org/obo/GO> .
@prefix ro: <http://purl.obolibrary.org/obo/RO> .
@prefix bfo: <http://purl.obolibrary.org/obo/BFO> .
@prefix dct: <http://purl.org/dc/terms/> .
@prefix iao: <http://purl.obolibrary.org/obo/IAO> .
@prefix obi: <http://purl.obolibrary.org/obo/OBI> .
@prefix owl: <http://www.w3.org/2002/07/owl#> .
@prefix rdf: <http://www.w3.org/1999/02/22-rdf-syntax-ns#> .
@prefix xml: <http://www.w3.org/XML/1998/namespace> .
@prefix xsd: <http://www.w3.org/2001/XMLSchema#> .
@prefix af-c: <http://purl.allotrope.org/ontologies/common#> .
@prefix af-e: <http://purl.allotrope.org/ontologies/equipment#> .
@prefix af-m: <http://purl.allotrope.org/ontologies/material#> .
@prefix af-p: <http://purl.allotrope.org/ontologies/process#> .
@prefix af-q: <http://purl.allotrope.org/ontologies/quality#> .
@prefix af-r: <http://purl.allotrope.org/ontologies/result#> .
@prefix af-x: <http://purl.allotrope.org/ontologies/property#> .
@prefix rdfs: <http://www.w3.org/2000/01/rdf-schema#> .
@prefix skos: <http://www.w3.org/2004/02/skos/core#> .
@prefix af-cur: <http://purl.allotrope.org/ontologies/curation#> .
@base <http://purl.allotrope.org/voc/afo/domain/WD/2025/06/electrophoresis#> .

<http://purl.allotrope.org/voc/afo/domain/WD/2025/06/electrophoresis> rdf:type owl:Ontology ;
                                                                                 owl:versionIRI <http://purl.allotrope.org/voc/afo/domain/WD/2025/06/electrophoresis> ;
                                                                                 owl:imports <http://purl.allotrope.org/voc/afo/WD/2025/06/afo> ;
                                                                                 dct:issued "2025-06-25T12:00:00Z"^^xsd:dateTime ;
                                                                                 dct:license <http://purl.allotrope.org/voc/creative-commons-attribution-license> ;
                                                                                 dct:modified "2025-04-04T12:00:00Z"^^xsd:dateTime ;
                                                                                 dct:rights <http://purl.allotrope.org/voc/attribution> ,
                                                                                            <http://purl.allotrope.org/voc/copyright> ;
                                                                                 dct:title "AFO Electrophoresis Domain Ontology (WD/2025/06)" ;
                                                                                 owl:priorVersion <http://purl.allotrope.org/voc/afo/domain/WD/2018/11/electrophoresis> ;
                                                                                 owl:versionInfo "WD/2025/06" .

#################################################################
#    Annotation properties
#################################################################

###  http://purl.allotrope.org/ontologies/property#AFX_0002796
af-x:AFX_0002796 rdf:type owl:AnnotationProperty .


###  http://purl.allotrope.org/ontologies/property#AFX_0002798
af-x:AFX_0002798 rdf:type owl:AnnotationProperty .


###  http://purl.allotrope.org/ontologies/property#AFX_0002809
af-x:AFX_0002809 rdf:type owl:AnnotationProperty .


###  http://purl.org/dc/terms/source
dct:source rdf:type owl:AnnotationProperty .


###  http://www.w3.org/2004/02/skos/core#altLabel
skos:altLabel rdf:type owl:AnnotationProperty .


###  http://www.w3.org/2004/02/skos/core#changeNote
skos:changeNote rdf:type owl:AnnotationProperty .


###  http://www.w3.org/2004/02/skos/core#definition
skos:definition rdf:type owl:AnnotationProperty .


###  http://www.w3.org/2004/02/skos/core#example
skos:example rdf:type owl:AnnotationProperty .


###  http://www.w3.org/2004/02/skos/core#note
skos:note rdf:type owl:AnnotationProperty .


###  http://www.w3.org/2004/02/skos/core#prefLabel
skos:prefLabel rdf:type owl:AnnotationProperty .


###  http://www.w3.org/2004/02/skos/core#scopeNote
skos:scopeNote rdf:type owl:AnnotationProperty .


#################################################################
#    Classes
#################################################################

###  http://purl.allotrope.org/ontologies/material#AFM_0000235
af-m:AFM_0000235 rdf:type owl:Class ;
                 rdfs:subClassOf af-m:AFM_0000015 ;
                 skos:definition "A background electrolyte buffer is a buffer solution that contains a background electrolyte. [Allotrope]" ;
                 skos:prefLabel "background electrolyte buffer" .


###  http://purl.allotrope.org/ontologies/process#AFP_0000268
af-p:AFP_0000268 rdf:type owl:Class ;
                 rdfs:subClassOf af-p:AFP_0000669 ;
                 skos:definition "An electrophoresis method where the separation medium contains a reticulated system, for example an entangled polymer network, that further separates the analytes according to their size and shape. [CHMO]" ;
                 skos:prefLabel "sieving electrophoresis" .


###  http://purl.allotrope.org/ontologies/process#AFP_0000273
af-p:AFP_0000273 rdf:type owl:Class ;
                 rdfs:subClassOf af-p:AFP_0000312 ;
                 skos:altLabel "ESI-GEMMA" ;
                 skos:definition "A separation method where singly-charged complexes move at different speeds according to their electrophoretic mobilities in air under the influence of an electric field. The sample is ionized by forcing a solution (usually in an organic solvent) of the sample through a small heated capillary (at a flow rate of 1-10 L min-1) into an electric field to produce a very fine mist of charged droplets. [CHMO]" ;
                 skos:prefLabel "electrospray ionisation gas-phase electrophoretic mobility molecular analysis"@en-gb ,
                                "electrospray ionization gas-phase electrophoretic mobility molecular analysis" .


###  http://purl.allotrope.org/ontologies/process#AFP_0000300
af-p:AFP_0000300 rdf:type owl:Class ;
                 rdfs:subClassOf af-p:AFP_0001080 ,
                                 af-p:AFP_0001165 ;
                 skos:altLabel "CGE" ,
                               "gel CE" ;
                 skos:definition "A separation method that takes place in a capillary and where colloidal particles move at different speeds according to their electrophoretic mobilities in a separation medium consisting of gel, across which an electric field is applied. [CHMO]" ;
                 skos:prefLabel "capillary gel electrophoresis" .


###  http://purl.allotrope.org/ontologies/process#AFP_0000312
af-p:AFP_0000312 rdf:type owl:Class ;
                 rdfs:subClassOf af-p:AFP_0000669 ;
                 skos:altLabel "GEMMA" ;
                 skos:definition "A separation method where singly-charged complexes move at different speeds according to their electrophoretic mobilities in air under the influence of an electric field. [CHMO]" ;
                 skos:prefLabel "gas-phase electrophoretic mobility molecular analysis" .


###  http://purl.allotrope.org/ontologies/process#AFP_0000365
af-p:AFP_0000365 rdf:type owl:Class ;
                 rdfs:subClassOf af-p:AFP_0000669 ;
                 skos:altLabel "IEF" ,
                               "IEF focusing" ,
                               "IEF focussing" ,
                               "IEF separation" ,
                               "focusing" ,
                               "isoelectric focusing" ,
                               "isoelectric focussing" ;
                 skos:definition "An electrophoresis method for the separation of amphoteric analytes according to their isoelectric points by the application of an electric field along a pH gradient. [CHMO]" ;
                 skos:prefLabel "isoelectric focusing" .


###  http://purl.allotrope.org/ontologies/process#AFP_0000673
af-p:AFP_0000673 rdf:type owl:Class ;
                 rdfs:subClassOf af-p:AFP_0001179 ;
                 skos:definition "A multi-dimensional separation method where the separation processes are all electrophoresis. [CHMO]" ;
                 skos:prefLabel "multi-dimensional electrophoresis" .


###  http://purl.allotrope.org/ontologies/process#AFP_0001080
af-p:AFP_0001080 rdf:type owl:Class ;
                 rdfs:subClassOf af-p:AFP_0000268 ;
                 skos:definition "A separation method where colloidal particles move at different speeds according to their electrophoretic mobilities in a separation medium consisting of gel, across which an electric field is applied. [CHMO]" ;
                 skos:prefLabel "gel electrophoresis" .


###  http://purl.allotrope.org/ontologies/process#AFP_0001165
af-p:AFP_0001165 rdf:type owl:Class .


###  http://purl.allotrope.org/ontologies/process#AFP_0001468
af-p:AFP_0001468 rdf:type owl:Class ;
                 rdfs:subClassOf af-p:AFP_0001615 ;
                 skos:altLabel "DC dielectrophoresis" ,
                               "d.c. dielectrophoresis" ,
                               "dc dielectrophoresis" ,
                               "direct current dielectrophoresis" ,
                               "direct current dielectrophoretic analysis" ;
                 skos:definition "A separation method where colloidal particles move at different speeds according to their dielectrophoretic mobilities in a separation medium, across which a direct electric field is applied. [CHMO]" ;
                 skos:prefLabel "direct-current dielectrophoresis" .


###  http://purl.allotrope.org/ontologies/process#AFP_0001615
af-p:AFP_0001615 rdf:type owl:Class ;
                 rdfs:subClassOf af-p:AFP_0000422 ;
                 skos:altLabel "dielectrophoretic analysis" ;
                 skos:definition "A separation method where colloidal particles move at different speeds according to their dielectrophoretic mobilities in a separation medium, across which an electric field is applied. [CHMO]" ;
                 skos:prefLabel "dielectrophoresis" .


###  http://purl.allotrope.org/ontologies/process#AFP_0001644
af-p:AFP_0001644 rdf:type owl:Class ;
                 rdfs:subClassOf af-p:AFP_0000669 ;
                 skos:definition "An electrophoresis method in a discontinuous buffer system where the analytes migrate according to their electrophoretic mobilities, forming a chain of adjacent zones moving with equal velocity between two solutions, the leading and terminating electrolytes, bracketing the mobility range of the analytes. [CHMO]" ;
                 skos:prefLabel "isotachophoresis" .


###  http://purl.allotrope.org/ontologies/process#AFP_0001652
af-p:AFP_0001652 rdf:type owl:Class ;
                 rdfs:subClassOf af-p:AFP_0000669 ;
                 skos:altLabel "FFE" ;
                 skos:definition "An electrophoresis method where the sample is introduced continuously to the separation chamber and the electric field is applied perpendicular to the hydrodynamic flow resulting in two-dimensional separation of the analytes based on the flow rate and their electrophoretic mobilities. [CHMO]" ;
                 skos:prefLabel "free-flow electrophoresis" .


###  http://purl.allotrope.org/ontologies/process#AFP_0001850
af-p:AFP_0001850 rdf:type owl:Class ;
                 rdfs:subClassOf af-p:AFP_0001615 ;
                 skos:altLabel "AC dielectrophoresis" ,
                               "a.c. dielectrophoresis" ,
                               "ac dielectrophoresis" ,
                               "alternating current dielectrophoresis" ,
                               "alternating current dielectrophoretic analysis" ;
                 skos:definition "A separation method where colloidal particles move at different speeds according to their dielectrophoretic mobilities in a separation medium, across which an alternating electric field is applied. [CHMO]" ;
                 skos:prefLabel "alternating-current dielectrophoresis" .


###  http://purl.allotrope.org/ontologies/process#AFP_0001969
af-p:AFP_0001969 rdf:type owl:Class ;
                 rdfs:subClassOf af-p:AFP_0000673 ,
                                 af-p:AFP_0000768 ;
                 skos:altLabel "2-DE" ,
                               "2D electrophoresis" ,
                               "2DE" ;
                 skos:definition "A two-dimensional separation method where the separation processes are both electrophoresis. Separation occurs in one plane, that plane is rotated by 90 deg. and the next separation step is carried out. [CHMO]" ;
                 skos:prefLabel "two-dimensional electrophoresis" .


###  http://purl.allotrope.org/ontologies/process#AFP_0002297
af-p:AFP_0002297 rdf:type owl:Class ;
                 rdfs:subClassOf af-p:AFP_0000669 ;
                 skos:definition "A separation method where colloidal particles move at different speeds according to their electrophoretic mobilities in a separation medium, across which a pulsed electric field is applied (a field in which the voltage changes direction). [CHMO]" ;
                 skos:prefLabel "pulsed-field electrophoresis" .


###  http://purl.allotrope.org/ontologies/process#AFP_0002308
af-p:AFP_0002308 rdf:type owl:Class ;
                 rdfs:subClassOf af-p:AFP_0001644 ;
                 skos:altLabel "isotachophoretic focussing" ;
                 skos:definition "An electrophoresis method where colloidal particles move at different speeds in a separation medium that has an electrophoretic mobility gradient so that the analytes move and stack in the order of their electrophoretic mobilities. [CHMO]" ;
                 skos:prefLabel "isotachophoretic focusing" .


###  http://purl.allotrope.org/ontologies/process#AFP_0002364
af-p:AFP_0002364 rdf:type owl:Class ;
                 rdfs:subClassOf af-p:AFP_0000669 ;
                 skos:definition "An electrophoresis method where the separation medium has specific interactions with the analytes. [CHMO]" ;
                 skos:prefLabel "affinity electrophoresis" .


###  http://purl.allotrope.org/ontologies/process#AFP_0002426
af-p:AFP_0002426 rdf:type owl:Class ;
                 rdfs:subClassOf af-p:AFP_0000273 ;
                 skos:altLabel "nESI-GEMMA" ,
                               "nanoESI-GEMMA" ;
                 skos:definition "A separation method where singly-charged complexes move at different speeds according to their electrophoretic mobilities in air under the influence of an electric field. The sample is ionized by forcing a solution (usually in an organic solvent) of the sample through a small heated capillary (at a flow rate of nL min-1) into an electric field to produce a very fine mist of charged droplets. [CHMO]" ;
                 skos:prefLabel "nano electrospray ionisation gas-phase electrophoretic mobility molecular analysis"@en-gb ,
                                "nano electrospray ionization gas-phase electrophoretic mobility molecular analysis" .


#################################################################
#    Individuals
#################################################################

###  http://purl.allotrope.org/voc/attribution
<http://purl.allotrope.org/voc/attribution> rdf:type owl:NamedIndividual ,
                                                     dct:RightsStatement ;
                                            dct:description """
These taxonomies contain material or may constitute derivative works of material which may be subject to copyright by one of the following organizations.  By using these taxonomies, you agree to the following terms and conditions applicable to its contents:
******************************************************************************
Copyright Notice and Terms for IUPAC Gold Book
______________________________________________________________________________
Copyright © 1998, Regents of the University of California
All rights reserved.
Redistribution and use in source and binary forms, with or without modification, are permitted provided that the following conditions are met:
1. Redistributions of source code must retain the above copyright notice, this list of conditions and the following disclaimer.
2. Redistributions in binary form must reproduce the above copyright notice, this list of conditions and the following disclaimer in the documentation and/or other materials provided with the distribution.
THIS SOFTWARE IS PROVIDED BY THE COPYRIGHT HOLDERS AND CONTRIBUTORS \"AS IS\" AND ANY EXPRESS OR IMPLIED WARRANTIES, INCLUDING, BUT NOT LIMITED TO, THE IMPLIED WARRANTIES OF MERCHANTABILITY AND FITNESS FOR A PARTICULAR PURPOSE ARE DISCLAIMED. IN NO EVENT SHALL THE COPYRIGHT HOLDER OR CONTRIBUTORS BE LIABLE FOR ANY DIRECT, INDIRECT, INCIDENTAL, SPECIAL, EXEMPLARY, OR CONSEQUENTIAL DAMAGES (INCLUDING, BUT NOT LIMITED TO, PROCUREMENT OF SUBSTITUTE GOODS OR SERVICES; LOSS OF USE, DATA, OR PROFITS; OR BUSINESS INTERRUPTION) HOWEVER CAUSED AND ON ANY THEORY OF LIABILITY, WHETHER IN CONTRACT, STRICT LIABILITY, OR TORT (INCLUDING NEGLIGENCE OR OTHERWISE) ARISING IN ANY WAY OUT OF THE USE OF THIS SOFTWARE, EVEN IF ADVISED OF THE POSSIBILITY OF SUCH DAMAGE.
******************************************************************************
Copyright Notice and Terms for PSI-MS (Proteomics Standards Initiative - Mass Spectrometry) Mass spectrometer output files and spectra interpretation
_____________________________________________________________________________
Created by Matt Chambers, Andreas Bertsch, Marius Kallhardt, Eric Deutsch Fredrik Levander, Pierre-Alain Binz, and Gerhard Mayer. Publisher: HUPO Proteomics Standards Initiative Mass Spectrometry Standards Working Group and HUPO Proteomics Standards Initiative Proteomics Informatics Working Group. This work is used pursuant to a Creative Commons license available here: http://creativecommons.org/licenses/by/3.0/legalcode

******************************************************************************
Attribution Notice for National Center for Biomedical Ontology materials.

This work contains material from the Cell Ontology and Clinical Measurement Ontology, available here: http://bioportal.bioontology.org/.
******************************************************************************
Attribution Notice for ChEBI
This work contains material from the European Bioinformatics Institute’s ChEBI database.
******************************************************************************
Attribution Notice for Quantities Units Dimensions Data Types (http://www.qudt.org/)
This work contains content from www.qudt.org and is used pursuant to a Creative Commons License available here: http://creativecommons.org/licenses/by-sa/3.0/us/legalcode. The original work may have been modified.
******************************************************************************
Copyright and Attribution Notice for Dublin Core Metadata Initiative Document
This work contains material from the following DCMI document used pursuant to a creative commons license available here: https://creativecommons.org/licenses/by/4.0/legalcode. This material may have been modified or changed.
Timestamped URL:          http://dublincore.org/documents/2012/06/14/dcmi-terms/
Date Issued:                       2012-06-14
Document Status:            This is a DCMI Recommendation.
Copyright © 1995-2015 DCMI. All Rights Reserved. DCMI liability, trademark/service mark, document use and software licensing rules apply.
******************************************************************************

""" ;
                                            dct:title "Derivative works attribution" .


###  http://purl.allotrope.org/voc/copyright
<http://purl.allotrope.org/voc/copyright> rdf:type owl:NamedIndividual ,
                                                   dct:RightsStatement ;
                                          dct:description "Copyright © 2019 Allotrope Foundation" ;
                                          dct:rightsHolder <http://www.allotrope.org> ;
                                          dct:title "Copyright © 2019 Allotrope Foundation" .


###  http://purl.allotrope.org/voc/creative-commons-attribution-license
<http://purl.allotrope.org/voc/creative-commons-attribution-license> rdf:type owl:NamedIndividual ,
                                                                              dct:LicenseDocument ;
                                                                     dct:description """This work is licensed under a Creative Commons Attribution 4.0 International License http://creativecommons.org/licenses/by/4.0/.

THESE MATERIALS ARE PROVIDED \"AS IS\" AND ALLOTROPE EXPRESSLY DISCLAIMS ALL WARRANTIES, EXPRESS, IMPLIED OR STATUTORY, INCLUDING, WITHOUT LIMITATION, THE WARRANTIES OF NON-INFRINGEMENT, TITLE, MERCHANTABILITY AND FITNESS FOR A PARTICULAR PURPOSE.

Copyright © 2015-2025 Allotrope Foundation
""" ;
                                                                     dct:title "Creative Commons Attribution 4.0 International Public License" .


###  Generated by the OWL API (version 5.1.19) https://github.com/owlcs/owlapi/
