@prefix : <http://purl.allotrope.org/voc/afo/domain/WD/2025/06/electric-engineering#> .
@prefix dct: <http://purl.org/dc/terms/> .
@prefix owl: <http://www.w3.org/2002/07/owl#> .
@prefix rdf: <http://www.w3.org/1999/02/22-rdf-syntax-ns#> .
@prefix xml: <http://www.w3.org/XML/1998/namespace> .
@prefix xsd: <http://www.w3.org/2001/XMLSchema#> .
@prefix af-c: <http://purl.allotrope.org/ontologies/common#> .
@prefix af-e: <http://purl.allotrope.org/ontologies/equipment#> .
@prefix af-m: <http://purl.allotrope.org/ontologies/material#> .
@prefix af-p: <http://purl.allotrope.org/ontologies/process#> .
@prefix af-q: <http://purl.allotrope.org/ontologies/quality#> .
@prefix af-r: <http://purl.allotrope.org/ontologies/result#> .
@prefix af-x: <http://purl.allotrope.org/ontologies/property#> .
@prefix rdfs: <http://www.w3.org/2000/01/rdf-schema#> .
@prefix skos: <http://www.w3.org/2004/02/skos/core#> .
@prefix af-cur: <http://purl.allotrope.org/ontologies/curation#> .
@base <http://purl.allotrope.org/voc/afo/domain/WD/2025/06/electric-engineering#> .

<http://purl.allotrope.org/voc/afo/domain/WD/2025/06/electric-engineering> rdf:type owl:Ontology ;
                                                                                      owl:versionIRI <http://purl.allotrope.org/voc/afo/domain/WD/2025/06/electric-engineering> ;
                                                                                      owl:imports <http://purl.allotrope.org/voc/afo/WD/2025/06/afo> ,
                                                                                                  <http://purl.allotrope.org/voc/afo/domain/REC/2025/06/electric-engineering> ;
                                                                                      dct:issued "2025-06-25T12:00:00Z"^^xsd:dateTime ;
                                                                                      dct:license <http://purl.allotrope.org/voc/creative-commons-attribution-license> ;
                                                                                      dct:modified "2025-04-04T12:00:00Z"^^xsd:dateTime ;
                                                                                      dct:rights <http://purl.allotrope.org/voc/attribution> ,
                                                                                                 <http://purl.allotrope.org/voc/copyright> ;
                                                                                      dct:rightsHolder <http://www.allotrope.org> ;
                                                                                      dct:title "AFO Electric Engineering Domain Ontology (WD/2025/06)" ;
                                                                                      owl:priorVersion <http://purl.allotrope.org/voc/afo/domain/WD/2018/04/electric-engineering> ;
                                                                                      owl:versionInfo "WD/2025/06" .

#################################################################
#    Annotation properties
#################################################################

###  http://purl.allotrope.org/ontologies/property#AFX_0002796
af-x:AFX_0002796 rdf:type owl:AnnotationProperty .


###  http://purl.allotrope.org/ontologies/property#AFX_0002798
af-x:AFX_0002798 rdf:type owl:AnnotationProperty .


###  http://purl.allotrope.org/ontologies/property#AFX_0002809
af-x:AFX_0002809 rdf:type owl:AnnotationProperty .


###  http://purl.org/dc/terms/source
dct:source rdf:type owl:AnnotationProperty .


###  http://www.w3.org/2004/02/skos/core#altLabel
skos:altLabel rdf:type owl:AnnotationProperty .


###  http://www.w3.org/2004/02/skos/core#changeNote
skos:changeNote rdf:type owl:AnnotationProperty .


###  http://www.w3.org/2004/02/skos/core#definition
skos:definition rdf:type owl:AnnotationProperty .


###  http://www.w3.org/2004/02/skos/core#example
skos:example rdf:type owl:AnnotationProperty .


###  http://www.w3.org/2004/02/skos/core#note
skos:note rdf:type owl:AnnotationProperty .


###  http://www.w3.org/2004/02/skos/core#prefLabel
skos:prefLabel rdf:type owl:AnnotationProperty .


###  http://www.w3.org/2004/02/skos/core#scopeNote
skos:scopeNote rdf:type owl:AnnotationProperty .


#################################################################
#    Classes
#################################################################

###  http://purl.allotrope.org/ontologies/equipment#AFE_0000006
af-e:AFE_0000006 rdf:type owl:Class ;
                 rdfs:subClassOf af-e:AFE_0000172 ;
                 skos:definition "The BNC (Bayonet Neill–Concelman) connector is a miniature quick connect/disconnect radio frequency connector used for coaxial cable. It features two bayonet lugs on the female connector; mating is fully achieved with a quarter turn of the coupling nut. [Wikipedia]" ;
                 skos:prefLabel "BNC" .


###  http://purl.allotrope.org/ontologies/equipment#AFE_0000227
af-e:AFE_0000227 rdf:type owl:Class ;
                 rdfs:subClassOf af-e:AFE_0000172 ;
                 skos:altLabel "serial plug" ;
                 skos:definition "RS-232 is a standard for serial communication transmission of data. It formally defines the signals connecting between a computer terminal, and a data communication equipment, such as a modem. The RS-232 standard is commonly used in computer serial ports. [Wikipedia]" ;
                 skos:prefLabel "RS232" .


###  http://purl.allotrope.org/ontologies/equipment#AFE_0000233
af-e:AFE_0000233 rdf:type owl:Class ;
                 rdfs:subClassOf af-e:AFE_0000056 ;
                 skos:altLabel "patch clamp amplifier" ;
                 skos:definition "A piece of apparatus that is used to increase the amplitude of either the voltage or the current output from a patch-clamp (ion-channel measurement) experiment. [CHMO]" ;
                 skos:prefLabel "patch-clamp amplifier" .


###  http://purl.allotrope.org/ontologies/equipment#AFE_0000253
af-e:AFE_0000253 rdf:type owl:Class ;
                 rdfs:subClassOf af-e:AFE_0000068 ;
                 skos:definition "The UK 3-pin connector follows the british standard of BS 1363 which specifies the common single-phase AC power plugs and sockets that are used in the United Kingdom. [Allotrope]" ;
                 skos:prefLabel "UK 3-Pin connector" .


###  http://purl.allotrope.org/ontologies/equipment#AFE_0000338
af-e:AFE_0000338 rdf:type owl:Class ;
                 rdfs:subClassOf af-e:AFE_0000056 ;
                 dct:license <http://purl.allotrope.org/voc/iupac-license> ;
                 dct:rights <http://purl.allotrope.org/voc/iupac-copyright> ;
                 dct:source "IUPAC. Analytical Division. Compendium of Analytical Nomenclature (the Orange Book). Definitive Rules, 1979. Compiled by J. Inczédy, T. Lengyel, A. M. Ure. Blackwell Scientific Publications, Oxford (1997)." ;
                 skos:changeNote "2024-09-12 Changed [IUPAC Orange Book] attribution to [IUPAC] and added license, rights, and source fields." ;
                 skos:definition "A high gain DC voltage amplifier with high input impedance, low output impedance and the capability of producing a bipolar output from a bipolar input. [IUPAC]" ;
                 skos:prefLabel "operational amplifier" .


###  http://purl.allotrope.org/ontologies/equipment#AFE_0000379
af-e:AFE_0000379 rdf:type owl:Class ;
                 rdfs:subClassOf af-e:AFE_0000491 ;
                 skos:definition "A banana connector (commonly banana plug for the male, banana socket or banana jack for the female) is a single-wire (one conductor) electrical connector used for joining wires to equipment. [Wikipedia]" ;
                 skos:prefLabel "banana plug" .


###  http://purl.allotrope.org/ontologies/equipment#AFE_0000390
af-e:AFE_0000390 rdf:type owl:Class ;
                 rdfs:subClassOf af-e:AFE_0000172 ;
                 skos:altLabel "universal serial bus" ,
                               "usb" ;
                 skos:changeNote "2016-03-16 change pref label to uppercase, add alt labels" ;
                 skos:definition "Universal Serial Bus (USB) is an industry standard developed in the mid-1990s that defines the cables, connectors and communications protocols used in a bus for connection, communication, and power supply between computers and electronic devices. [Wikipedia]" ;
                 skos:prefLabel "USB" .


###  http://purl.allotrope.org/ontologies/equipment#AFE_0000432
af-e:AFE_0000432 rdf:type owl:Class ;
                 owl:equivalentClass [ owl:intersectionOf ( af-e:AFE_0000145
                                                            [ rdf:type owl:Restriction ;
                                                              owl:onProperty <http://purl.obolibrary.org/obo/BFO_0000050> ;
                                                              owl:someValuesFrom af-e:AFE_0000872
                                                            ]
                                                          ) ;
                                       rdf:type owl:Class
                                     ] ;
                 af-x:AFX_0002798 "true"^^xsd:boolean ;
                 skos:definition "An analog-to-digital converter channel is a special type of channel that belongs to an analog-to-digital converter. Usually there are several channels for one converter. [Allotrope]" ;
                 skos:prefLabel "analogue-to-digital converter channel"@en-gb ,
                                "analog-to-digital converter channel" .


###  http://purl.allotrope.org/ontologies/equipment#AFE_0000511
af-e:AFE_0000511 rdf:type owl:Class ;
                 rdfs:subClassOf af-e:AFE_0000172 ;
                 skos:definition "The F connector is a coaxial RF connector commonly used for over the air terrestrial television, cable television and universally for satellite television and cable modems, usually with RG-6/U cable or, in older installations, with RG-59/U cable. [Wikipedia]" ;
                 skos:prefLabel "F plug" .


###  http://purl.allotrope.org/ontologies/equipment#AFE_0000553
af-e:AFE_0000553 rdf:type owl:Class ;
                 rdfs:subClassOf af-e:AFE_0000172 ;
                 skos:altLabel "Metrohm connector" ;
                 skos:definition "LEMO is a push-pull connector made by the LEMO company. LEMO connectors are used in medical, industrial, audio/visual, telecommunications, military, scientific research and measurement applications. [Wikipedia]" ;
                 skos:prefLabel "LEMO connector" .


###  http://purl.allotrope.org/ontologies/equipment#AFE_0000714
af-e:AFE_0000714 rdf:type owl:Class ;
                 rdfs:subClassOf af-e:AFE_0000068 ;
                 skos:altLabel "euro 2-pin plug" ;
                 skos:definition "The Europlug (CEE 7/16) is a non-rewirable flat, two-pole domestic AC power plug that must be supplied attached to a power cord. [Wikipedia]" ;
                 skos:prefLabel "euro plug" .


###  http://purl.allotrope.org/ontologies/equipment#AFE_0000763
af-e:AFE_0000763 rdf:type owl:Class ;
                 rdfs:subClassOf af-e:AFE_0000172 ;
                 skos:altLabel "DIN-EL-0 S7" ;
                 skos:definition "The DIN-EL-S7 is an industry standard for electrodes. [Allotrope]" ;
                 skos:prefLabel "connector S7" .


###  http://purl.allotrope.org/ontologies/equipment#AFE_0000815
af-e:AFE_0000815 rdf:type owl:Class ;
                 rdfs:subClassOf af-e:AFE_0000056 ;
                 dct:source "https://en.wikipedia.org/wiki/Lock-in_amplifier" ;
                 skos:altLabel "lock in amplifier" ,
                               "phase-sensitive detector" ;
                 skos:changeNote "2024-09-12 Truncated definitions and replaced [PSI-MS] attribution with [Wikipedia] as this is the correct source." ;
                 skos:definition "A lock-in amplifier is a type of amplifier that can extract a signal with a known carrier wave from an extremely noisy environment. [Wikipedia]" ;
                 skos:prefLabel "lock-in amplifier" .


###  http://purl.allotrope.org/ontologies/equipment#AFE_0000840
af-e:AFE_0000840 rdf:type owl:Class ;
                 rdfs:subClassOf af-e:AFE_0000172 ;
                 skos:definition "The plug socket and plug shielded for pH electrodes as specified by DIN 19262. [Allotrope]" ;
                 skos:editorialNote "maybe moved into a pH domain ontology [OSTHUS]" ;
                 skos:prefLabel "DIN 19262 connector" .


###  http://purl.allotrope.org/ontologies/equipment#AFE_0001659
af-e:AFE_0001659 rdf:type owl:Class ;
                 rdfs:subClassOf af-e:AFE_0000145 ;
                 skos:altLabel "RF channel" ;
                 skos:changeNote "2015-11-25 add concept [Amgen]" ,
                                 "2016-02-02 add harmonized property restrictions [OSTHUS]" ;
                 skos:definition "A radio frequency channel is a channel for signals in the range of radio frequencies. [Allotrope]" ;
                 skos:example "RF channels of a ssNMR console" ;
                 skos:prefLabel "radio frequency channel" .


#################################################################
#    Individuals
#################################################################

###  http://purl.allotrope.org/voc/attribution
<http://purl.allotrope.org/voc/attribution> rdf:type owl:NamedIndividual ,
                                                     dct:RightsStatement ;
                                            dct:description """
These taxonomies contain material or may constitute derivative works of material which may be subject to copyright by one of the following organizations.  By using these taxonomies, you agree to the following terms and conditions applicable to its contents:
******************************************************************************
Copyright Notice and Terms for IUPAC Gold Book
______________________________________________________________________________
Copyright © 1998, Regents of the University of California
All rights reserved.
Redistribution and use in source and binary forms, with or without modification, are permitted provided that the following conditions are met:
1. Redistributions of source code must retain the above copyright notice, this list of conditions and the following disclaimer.
2. Redistributions in binary form must reproduce the above copyright notice, this list of conditions and the following disclaimer in the documentation and/or other materials provided with the distribution.
THIS SOFTWARE IS PROVIDED BY THE COPYRIGHT HOLDERS AND CONTRIBUTORS \"AS IS\" AND ANY EXPRESS OR IMPLIED WARRANTIES, INCLUDING, BUT NOT LIMITED TO, THE IMPLIED WARRANTIES OF MERCHANTABILITY AND FITNESS FOR A PARTICULAR PURPOSE ARE DISCLAIMED. IN NO EVENT SHALL THE COPYRIGHT HOLDER OR CONTRIBUTORS BE LIABLE FOR ANY DIRECT, INDIRECT, INCIDENTAL, SPECIAL, EXEMPLARY, OR CONSEQUENTIAL DAMAGES (INCLUDING, BUT NOT LIMITED TO, PROCUREMENT OF SUBSTITUTE GOODS OR SERVICES; LOSS OF USE, DATA, OR PROFITS; OR BUSINESS INTERRUPTION) HOWEVER CAUSED AND ON ANY THEORY OF LIABILITY, WHETHER IN CONTRACT, STRICT LIABILITY, OR TORT (INCLUDING NEGLIGENCE OR OTHERWISE) ARISING IN ANY WAY OUT OF THE USE OF THIS SOFTWARE, EVEN IF ADVISED OF THE POSSIBILITY OF SUCH DAMAGE.
******************************************************************************
Copyright Notice and Terms for PSI-MS (Proteomics Standards Initiative - Mass Spectrometry) Mass spectrometer output files and spectra interpretation
_____________________________________________________________________________
Created by Matt Chambers, Andreas Bertsch, Marius Kallhardt, Eric Deutsch Fredrik Levander, Pierre-Alain Binz, and Gerhard Mayer. Publisher: HUPO Proteomics Standards Initiative Mass Spectrometry Standards Working Group and HUPO Proteomics Standards Initiative Proteomics Informatics Working Group. This work is used pursuant to a Creative Commons license available here: http://creativecommons.org/licenses/by/3.0/legalcode

******************************************************************************
Attribution Notice for National Center for Biomedical Ontology materials.

This work contains material from the Cell Ontology and Clinical Measurement Ontology, available here: http://bioportal.bioontology.org/.
******************************************************************************
Attribution Notice for ChEBI
This work contains material from the European Bioinformatics Institute’s ChEBI database.
******************************************************************************
Attribution Notice for Quantities Units Dimensions Data Types (http://www.qudt.org/)
This work contains content from www.qudt.org and is used pursuant to a Creative Commons License available here: http://creativecommons.org/licenses/by-sa/3.0/us/legalcode. The original work may have been modified.
******************************************************************************
Copyright and Attribution Notice for Dublin Core Metadata Initiative Document
This work contains material from the following DCMI document used pursuant to a creative commons license available here: https://creativecommons.org/licenses/by/4.0/legalcode. This material may have been modified or changed.
Timestamped URL:          http://dublincore.org/documents/2012/06/14/dcmi-terms/
Date Issued:                       2012-06-14
Document Status:            This is a DCMI Recommendation.
Copyright © 1995-2015 DCMI. All Rights Reserved. DCMI liability, trademark/service mark, document use and software licensing rules apply.
******************************************************************************

""" ;
                                            dct:title "Derivative works attribution" .


###  http://purl.allotrope.org/voc/copyright
<http://purl.allotrope.org/voc/copyright> rdf:type owl:NamedIndividual ,
                                                   dct:RightsStatement ;
                                          dct:description "(c) 2017 Allotrope Foundation" ;
                                          dct:title "(c) 2017 Allotrope Foundation" .


###  http://purl.allotrope.org/voc/creative-commons-attribution-license
<http://purl.allotrope.org/voc/creative-commons-attribution-license> rdf:type owl:NamedIndividual ,
                                                                              dct:LicenseDocument ;
                                                                     dct:description """This work is licensed under a Creative Commons Attribution 4.0 International License http://creativecommons.org/licenses/by/4.0/.

THESE MATERIALS ARE PROVIDED \"AS IS\" AND ALLOTROPE EXPRESSLY DISCLAIMS ALL WARRANTIES, EXPRESS, IMPLIED OR STATUTORY, INCLUDING, WITHOUT LIMITATION, THE WARRANTIES OF NON-INFRINGEMENT, TITLE, MERCHANTABILITY AND FITNESS FOR A PARTICULAR PURPOSE.

Copyright © 2015-2025 Allotrope Foundation
""" ;
                                                                     dct:title "Creative Commons Attribution 4.0 International Public License" .


###  http://purl.allotrope.org/voc/afo/domain/WD/2025/06/electric-engineering
<http://purl.allotrope.org/voc/afo/domain/WD/2025/06/electric-engineering> rdf:type owl:NamedIndividual .


###  Generated by the OWL API (version 5.1.19) https://github.com/owlcs/owlapi/
