@prefix : <http://purl.allotrope.org/voc/afo/domain/WD/2025/06/granulation#> .
@prefix dct: <http://purl.org/dc/terms/> .
@prefix owl: <http://www.w3.org/2002/07/owl#> .
@prefix rdf: <http://www.w3.org/1999/02/22-rdf-syntax-ns#> .
@prefix xml: <http://www.w3.org/XML/1998/namespace> .
@prefix xsd: <http://www.w3.org/2001/XMLSchema#> .
@prefix af-c: <http://purl.allotrope.org/ontologies/common#> .
@prefix af-e: <http://purl.allotrope.org/ontologies/equipment#> .
@prefix af-m: <http://purl.allotrope.org/ontologies/material#> .
@prefix af-p: <http://purl.allotrope.org/ontologies/process#> .
@prefix af-q: <http://purl.allotrope.org/ontologies/quality#> .
@prefix af-r: <http://purl.allotrope.org/ontologies/result#> .
@prefix af-x: <http://purl.allotrope.org/ontologies/property#> .
@prefix rdfs: <http://www.w3.org/2000/01/rdf-schema#> .
@prefix skos: <http://www.w3.org/2004/02/skos/core#> .
@prefix af-cur: <http://purl.allotrope.org/ontologies/curation#> .
@base <http://purl.allotrope.org/voc/afo/domain/WD/2025/06/granulation#> .

<http://purl.allotrope.org/voc/afo/domain/WD/2025/06/granulation> rdf:type owl:Ontology ;
                                                                             owl:versionIRI <http://purl.allotrope.org/voc/afo/domain/WD/2025/06/granulation> ;
                                                                             owl:imports <http://purl.allotrope.org/voc/afo/WD/2025/06/afo> ;
                                                                             dct:issued "2025-06-25T12:00:00Z"^^xsd:dateTime ;
                                                                             dct:license <http://purl.allotrope.org/voc/creative-commons-attribution-license> ;
                                                                             dct:modified "2025-04-04T12:00:00Z"^^xsd:dateTime ;
                                                                             dct:rights <http://purl.allotrope.org/vocabulary/attribution> ,
                                                                                        <http://purl.allotrope.org/vocabulary/copyright> ;
                                                                             dct:title "AFO Granulation Domain Ontology (WD/2025/06)" ;
                                                                             owl:priorVersion <http://purl.allotrope.org/voc/afo/domain/WD/2018/04/granulation> ;
                                                                             owl:versionInfo "WD/2025/06" .

#################################################################
#    Annotation properties
#################################################################

###  http://purl.allotrope.org/ontologies/property#AFX_0002796
af-x:AFX_0002796 rdf:type owl:AnnotationProperty .


###  http://purl.allotrope.org/ontologies/property#AFX_0002798
af-x:AFX_0002798 rdf:type owl:AnnotationProperty .


###  http://purl.allotrope.org/ontologies/property#AFX_0002809
af-x:AFX_0002809 rdf:type owl:AnnotationProperty .


###  http://purl.org/dc/terms/source
dct:source rdf:type owl:AnnotationProperty .


###  http://www.w3.org/2004/02/skos/core#altLabel
skos:altLabel rdf:type owl:AnnotationProperty .


###  http://www.w3.org/2004/02/skos/core#changeNote
skos:changeNote rdf:type owl:AnnotationProperty .


###  http://www.w3.org/2004/02/skos/core#definition
skos:definition rdf:type owl:AnnotationProperty .


###  http://www.w3.org/2004/02/skos/core#example
skos:example rdf:type owl:AnnotationProperty .


###  http://www.w3.org/2004/02/skos/core#note
skos:note rdf:type owl:AnnotationProperty .


###  http://www.w3.org/2004/02/skos/core#prefLabel
skos:prefLabel rdf:type owl:AnnotationProperty .


###  http://www.w3.org/2004/02/skos/core#scopeNote
skos:scopeNote rdf:type owl:AnnotationProperty .


#################################################################
#    Classes
#################################################################

###  http://purl.allotrope.org/ontologies/equipment#AFE_0001719
af-e:AFE_0001719 rdf:type owl:Class ;
                 rdfs:subClassOf af-e:AFE_0001184 ;
                 skos:altLabel "feed material hopper" ;
                 skos:definition "A hopper is a storage container used to dispense materials into the feeding system of a given tablet press. [Allotrope]" ;
                 skos:prefLabel "hopper" .


###  http://purl.allotrope.org/ontologies/equipment#AFE_0001732
af-e:AFE_0001732 rdf:type owl:Class ;
                 rdfs:subClassOf af-e:AFE_0001733 ;
                 skos:definition "Knurled rollers are rollers with a rough product contact surface to allow more grip of the powder as it forces the material through the compression (nip) zone of compaction. [Allotrope]" ;
                 skos:prefLabel "knurled roller" .


###  http://purl.allotrope.org/ontologies/equipment#AFE_0001734
af-e:AFE_0001734 rdf:type owl:Class ;
                 rdfs:subClassOf af-e:AFE_0001733 ;
                 skos:definition "Rollers with a smooth product contact surface which can incur slip as material is passed through the compression (nip) zone of compaction. [Allotrope]" ;
                 skos:prefLabel "smooth roller" .


###  http://purl.allotrope.org/ontologies/equipment#AFE_0001735
af-e:AFE_0001735 rdf:type owl:Class ;
                 rdfs:subClassOf af-e:AFE_0001786 ;
                 skos:altLabel "metering screw" ;
                 skos:definition "A rotating helix that conveys powder blend from the hopper to the tamping screw. [Allotrope]" ;
                 skos:prefLabel "feed screw" .


###  http://purl.allotrope.org/ontologies/equipment#AFE_0001736
af-e:AFE_0001736 rdf:type owl:Class ;
                 rdfs:subClassOf af-e:AFE_0001786 ;
                 skos:definition "A screw that can vary speed to provide powder blend to the rollers at a constant rate, this screw also acts to consolidate the powder blend into the rollers. [Allotrope]" ;
                 skos:prefLabel "tamping screw" .


###  http://purl.allotrope.org/ontologies/equipment#AFE_0001737
af-e:AFE_0001737 rdf:type owl:Class ;
                 rdfs:subClassOf af-e:AFE_0000354 ;
                 skos:definition "The scrapers are positioned using fine gauges to ensure that compacted powder blend is scraped from the rollers to minimize accumulation of product. [Allotrope]" ;
                 skos:prefLabel "scraper assembly" .


###  http://purl.allotrope.org/ontologies/process#AFP_0000164
af-p:AFP_0000164 rdf:type owl:Class ;
                 rdfs:subClassOf af-p:AFP_0000797 ;
                 skos:altLabel "HEBM" ,
                               "high energy ball milling" ;
                 skos:definition "The mechanical reduction of the particle size of a solid sample by grinding with one or more inert balls (ceramic, flint or stainless steel, 2-8 mm diameter) rotating at high speed (up to 650 rpm) around a horizontal axis. A high-speed agitator is used to increase the speed of the balls which are held in vacuum or in an inert gas (e.g. Ar). [CHMO]" ;
                 skos:prefLabel "high-energy ball milling" .


###  http://purl.allotrope.org/ontologies/process#AFP_0000797
af-p:AFP_0000797 rdf:type owl:Class ;
                 rdfs:subClassOf af-p:AFP_0000911 ;
                 skos:definition "The mechanical reduction of the particle size of a solid sample by grinding with one or more inert balls (ceramic, flint, or stainless steel, 2-8 mm diameter) rotating around a horizontal axis. [CHMO]" ;
                 skos:prefLabel "ball milling" .


###  http://purl.allotrope.org/ontologies/process#AFP_0001351
af-p:AFP_0001351 rdf:type owl:Class ;
                 rdfs:subClassOf af-p:AFP_0000911 ;
                 skos:definition "The mechanical reduction of the particle size of a solid sample by attribution (friction), impact or cutting in the presence of a small amount of liquid (which is not a solvent for the solid). [CHMO]" ;
                 skos:prefLabel "wet grinding" .


###  http://purl.allotrope.org/ontologies/process#AFP_0001437
af-p:AFP_0001437 rdf:type owl:Class ;
                 rdfs:subClassOf af-p:AFP_0000911 ;
                 skos:altLabel "LAG" ,
                               "solvent-drop grinding" ;
                 skos:definition "The mechanical reduction of the particle size of a solid sample by attribution (friction), impact or cutting in the presence of a small amount of solvent. [CHMO]" ;
                 skos:prefLabel "liquid-assisted grinding" .


###  http://purl.allotrope.org/ontologies/process#AFP_0001554
af-p:AFP_0001554 rdf:type owl:Class ;
                 rdfs:subClassOf af-p:AFP_0000797 ;
                 skos:altLabel "HSBM" ,
                               "high speed ball milling" ;
                 skos:definition "The mechanical reduction of the particle size of a solid sample by grinding with one or more inert balls (ceramic, flint or stainless steel, 2-8 mm diameter) rotating at high speed around a horizontal axis. A high-speed agitator is used to increase the speed of the balls. [CHMO]" ;
                 skos:prefLabel "high-speed ball milling" .


#################################################################
#    Individuals
#################################################################

###  http://purl.allotrope.org/voc/creative-commons-attribution-license
<http://purl.allotrope.org/voc/creative-commons-attribution-license> rdf:type owl:NamedIndividual ,
                                                                              dct:LicenseDocument ;
                                                                     dct:description """This work is licensed under a Creative Commons Attribution 4.0 International License http://creativecommons.org/licenses/by/4.0/.

THESE MATERIALS ARE PROVIDED \"AS IS\" AND ALLOTROPE EXPRESSLY DISCLAIMS ALL WARRANTIES, EXPRESS, IMPLIED OR STATUTORY, INCLUDING, WITHOUT LIMITATION, THE WARRANTIES OF NON-INFRINGEMENT, TITLE, MERCHANTABILITY AND FITNESS FOR A PARTICULAR PURPOSE.

Copyright © 2015-2025 Allotrope Foundation
""" ;
                                                                     dct:title "Creative Commons Attribution 4.0 International Public License" .


###  http://purl.allotrope.org/vocabulary/attribution
<http://purl.allotrope.org/vocabulary/attribution> rdf:type owl:NamedIndividual ,
                                                            dct:RightsStatement ;
                                                   dct:description """
These taxonomies contain material or may constitute derivative works of material which may be subject to copyright by one of the following organizations.  By using these taxonomies, you agree to the following terms and conditions applicable to its contents:
******************************************************************************
Copyright Notice and Terms for IUPAC Gold Book
______________________________________________________________________________
Copyright © 1998, Regents of the University of California
All rights reserved.
Redistribution and use in source and binary forms, with or without modification, are permitted provided that the following conditions are met:
1. Redistributions of source code must retain the above copyright notice, this list of conditions and the following disclaimer.
2. Redistributions in binary form must reproduce the above copyright notice, this list of conditions and the following disclaimer in the documentation and/or other materials provided with the distribution.
THIS SOFTWARE IS PROVIDED BY THE COPYRIGHT HOLDERS AND CONTRIBUTORS \"AS IS\" AND ANY EXPRESS OR IMPLIED WARRANTIES, INCLUDING, BUT NOT LIMITED TO, THE IMPLIED WARRANTIES OF MERCHANTABILITY AND FITNESS FOR A PARTICULAR PURPOSE ARE DISCLAIMED. IN NO EVENT SHALL THE COPYRIGHT HOLDER OR CONTRIBUTORS BE LIABLE FOR ANY DIRECT, INDIRECT, INCIDENTAL, SPECIAL, EXEMPLARY, OR CONSEQUENTIAL DAMAGES (INCLUDING, BUT NOT LIMITED TO, PROCUREMENT OF SUBSTITUTE GOODS OR SERVICES; LOSS OF USE, DATA, OR PROFITS; OR BUSINESS INTERRUPTION) HOWEVER CAUSED AND ON ANY THEORY OF LIABILITY, WHETHER IN CONTRACT, STRICT LIABILITY, OR TORT (INCLUDING NEGLIGENCE OR OTHERWISE) ARISING IN ANY WAY OUT OF THE USE OF THIS SOFTWARE, EVEN IF ADVISED OF THE POSSIBILITY OF SUCH DAMAGE.
******************************************************************************
Copyright Notice and Terms for PSI-MS (Proteomics Standards Initiative - Mass Spectrometry) Mass spectrometer output files and spectra interpretation
_____________________________________________________________________________
Created by Matt Chambers, Andreas Bertsch, Marius Kallhardt, Eric Deutsch Fredrik Levander, Pierre-Alain Binz, and Gerhard Mayer. Publisher: HUPO Proteomics Standards Initiative Mass Spectrometry Standards Working Group and HUPO Proteomics Standards Initiative Proteomics Informatics Working Group. This work is used pursuant to a Creative Commons license available here: http://creativecommons.org/licenses/by/3.0/legalcode

******************************************************************************
Attribution Notice for National Center for Biomedical Ontology materials.

This work contains material from the Cell Ontology and Clinical Measurement Ontology, available here: http://bioportal.bioontology.org/.
******************************************************************************
Attribution Notice for ChEBI
This work contains material from the European Bioinformatics Institute’s ChEBI database.
******************************************************************************
Attribution Notice for Quantities Units Dimensions Data Types (http://www.qudt.org/)
This work contains content from www.qudt.org and is used pursuant to a Creative Commons License available here: http://creativecommons.org/licenses/by-sa/3.0/us/legalcode. The original work may have been modified.
******************************************************************************
Copyright and Attribution Notice for Dublin Core Metadata Initiative Document
This work contains material from the following DCMI document used pursuant to a creative commons license available here: https://creativecommons.org/licenses/by/4.0/legalcode. This material may have been modified or changed.
Timestamped URL:          http://dublincore.org/documents/2012/06/14/dcmi-terms/
Date Issued:                       2012-06-14
Document Status:            This is a DCMI Recommendation.
Copyright © 1995-2015 DCMI. All Rights Reserved. DCMI liability, trademark/service mark, document use and software licensing rules apply.
******************************************************************************

""" ;
                                                   dct:title "Derivative works attribution" .


###  http://purl.allotrope.org/vocabulary/copyright
<http://purl.allotrope.org/vocabulary/copyright> rdf:type owl:NamedIndividual ,
                                                          dct:RightsStatement ;
                                                 dct:description "Copyright © 2019 Allotrope Foundation" ;
                                                 dct:rightsHolder <http://www.allotrope.org> ;
                                                 dct:title "Copyright © 2019 Allotrope Foundation" .


###  Generated by the OWL API (version 5.1.19) https://github.com/owlcs/owlapi/
