@prefix : <http://purl.allotrope.org/voc/afo/domain/WD/2025/06/microscopy#> .
@prefix dct: <http://purl.org/dc/terms/> .
@prefix owl: <http://www.w3.org/2002/07/owl#> .
@prefix rdf: <http://www.w3.org/1999/02/22-rdf-syntax-ns#> .
@prefix xml: <http://www.w3.org/XML/1998/namespace> .
@prefix xsd: <http://www.w3.org/2001/XMLSchema#> .
@prefix af-c: <http://purl.allotrope.org/ontologies/common#> .
@prefix af-e: <http://purl.allotrope.org/ontologies/equipment#> .
@prefix af-m: <http://purl.allotrope.org/ontologies/material#> .
@prefix af-p: <http://purl.allotrope.org/ontologies/process#> .
@prefix af-q: <http://purl.allotrope.org/ontologies/quality#> .
@prefix af-r: <http://purl.allotrope.org/ontologies/result#> .
@prefix af-x: <http://purl.allotrope.org/ontologies/property#> .
@prefix rdfs: <http://www.w3.org/2000/01/rdf-schema#> .
@prefix skos: <http://www.w3.org/2004/02/skos/core#> .
@prefix af-cur: <http://purl.allotrope.org/ontologies/curation#> .
@base <http://purl.allotrope.org/voc/afo/domain/WD/2025/06/microscopy#> .

<http://purl.allotrope.org/voc/afo/domain/WD/2025/06/microscopy> rdf:type owl:Ontology ;
                                                                            owl:versionIRI <http://purl.allotrope.org/voc/afo/domain/WD/2025/06/microscopy> ;
                                                                            owl:imports <http://purl.allotrope.org/voc/afo/WD/2025/06/afo> ,
                                                                                        <http://purl.allotrope.org/voc/afo/domain/WD/2025/06/electron-microscopy> ,
                                                                                        <http://purl.allotrope.org/voc/afo/domain/WD/2025/06/ir-microscopy> ,
                                                                                        <http://purl.allotrope.org/voc/afo/domain/WD/2025/06/optical-microscopy> ,
                                                                                        <http://purl.allotrope.org/voc/afo/domain/WD/2025/06/raman-microscopy> ,
                                                                                        <http://purl.allotrope.org/voc/afo/domain/WD/2025/06/scanning-probe-microscopy> ;
                                                                            dct:issued "2025-06-25T12:00:00Z"^^xsd:dateTime ;
                                                                            dct:license <http://purl.allotrope.org/voc/creative-commons-attribution-license> ;
                                                                            dct:modified "2025-04-04T12:00:00Z"^^xsd:dateTime ;
                                                                            dct:rights <http://purl.allotrope.org/voc/attribution> ,
                                                                                       <http://purl.allotrope.org/voc/copyright> ;
                                                                            dct:title "AFO Microscopy Domain Ontology (WD/2025/06)" ;
                                                                            owl:priorVersion <http://purl.allotrope.org/voc/afo/domain/WD/2018/04/microscopy> ;
                                                                            owl:versionInfo "WD/2025/06" .

#################################################################
#    Annotation properties
#################################################################

###  http://purl.allotrope.org/ontologies/property#AFX_0002796
af-x:AFX_0002796 rdf:type owl:AnnotationProperty .


###  http://purl.allotrope.org/ontologies/property#AFX_0002798
af-x:AFX_0002798 rdf:type owl:AnnotationProperty .


###  http://purl.allotrope.org/ontologies/property#AFX_0002809
af-x:AFX_0002809 rdf:type owl:AnnotationProperty .


###  http://purl.org/dc/terms/source
dct:source rdf:type owl:AnnotationProperty .


###  http://www.w3.org/2004/02/skos/core#altLabel
skos:altLabel rdf:type owl:AnnotationProperty .


###  http://www.w3.org/2004/02/skos/core#changeNote
skos:changeNote rdf:type owl:AnnotationProperty .


###  http://www.w3.org/2004/02/skos/core#definition
skos:definition rdf:type owl:AnnotationProperty .


###  http://www.w3.org/2004/02/skos/core#example
skos:example rdf:type owl:AnnotationProperty .


###  http://www.w3.org/2004/02/skos/core#note
skos:note rdf:type owl:AnnotationProperty .


###  http://www.w3.org/2004/02/skos/core#prefLabel
skos:prefLabel rdf:type owl:AnnotationProperty .


###  http://www.w3.org/2004/02/skos/core#scopeNote
skos:scopeNote rdf:type owl:AnnotationProperty .


#################################################################
#    Classes
#################################################################

###  http://purl.allotrope.org/ontologies/process#AFP_0000124
af-p:AFP_0000124 rdf:type owl:Class ;
                 rdfs:subClassOf af-p:AFP_0001801 ;
                 skos:altLabel "EPR imaging" ,
                               "EPRI" ,
                               "ESR imaging" ,
                               "ESRI" ,
                               "electron paramagnetic imaging" .


###  http://purl.allotrope.org/ontologies/process#AFP_0000196
af-p:AFP_0000196 rdf:type owl:Class ;
                 rdfs:subClassOf af-p:AFP_0001864 ;
                 skos:altLabel "AP FIM" ,
                               "AP field ionization microscopy" ,
                               "AP field-ion microscopy" ,
                               "AP field-ionization microscopy" ,
                               "AP-FIM" ,
                               "AP/FIM" ,
                               "APFIM" ,
                               "atom probe field ionization microscopy" ,
                               "atom probe field-ion microscopy" ,
                               "atom probe field-ionization microscopy" ,
                               "atom-probe field-ion microscopy" ;
                 skos:definition "A type of microscopy where atoms in the vicinty of the specimen (which is in the form of a very sharp tip <10 m diameter) are ionized by the application of a strong electric field to the tip and an image is produced by the projection of the ions onto a fluorescent screen. The image consists of a pattern of spots of light which correspond to individual atoms on the specimen surface. When a sudden voltage pulse is applied to the tip, atoms from the surface of the specimen itself are be ejected and travel down a drift tube where their arrival time (a measure of the mass of the atom) can be determined. This allows the atomic composition of the specimen to be determined. [CHMO]" ;
                 skos:prefLabel "atom probe field ion microscopy" .


###  http://purl.allotrope.org/ontologies/process#AFP_0000206
af-p:AFP_0000206 rdf:type owl:Class ;
                 rdfs:subClassOf af-p:AFP_0000945 ;
                 skos:altLabel "SPCM" ;
                 skos:definition "A type of microscopy where a laser is scanned over the surface of the specimen and the photocurrent is recorded as a function of position. [CHMO]" ;
                 skos:prefLabel "scanning photocurrent microscopy" .


###  http://purl.allotrope.org/ontologies/process#AFP_0000218
af-p:AFP_0000218 rdf:type owl:Class ;
                 rdfs:subClassOf af-p:AFP_0002405 ;
                 skos:altLabel "PSTM" ,
                               "photon scanning tunneling microscopy" ,
                               "photon-scanning tunneling microscopy" ,
                               "photon-scanning tunnelling microscopy" ;
                 skos:definition "A type of microscopy where the specimen is illuminated with a near-field of photons. An image of the surface is obtained by mechanically moving an optical fibre probe in a raster scan over the specimen, line by line, and detecting any photons which tunnel from the specimen to the probe as a function of position. A feedback loop is used to maintain a fixed relationship between the optical fibre probe and surface during scanning. [CHMO]" ;
                 skos:prefLabel "photon scanning tunnelling microscopy" .


###  http://purl.allotrope.org/ontologies/process#AFP_0000221
af-p:AFP_0000221 rdf:type owl:Class ;
                 rdfs:subClassOf af-p:AFP_0002032 ;
                 skos:altLabel "STXM" ,
                               "STXRM" ,
                               "scanning TXM" ,
                               "scanning transmission XM" ;
                 skos:definition "An imaging technique where a finely focused (20-50 nm) beam of X-rays is scanned over the surface of the specimen, and the energies and intensities of the transmitted X-rays are measured as a function of position. [CHMO]" ;
                 skos:prefLabel "scanning transmission X-ray microscopy" .


###  http://purl.allotrope.org/ontologies/process#AFP_0000239
af-p:AFP_0000239 rdf:type owl:Class .


###  http://purl.allotrope.org/ontologies/process#AFP_0000339
af-p:AFP_0000339 rdf:type owl:Class ;
                 rdfs:subClassOf af-p:AFP_0002343 ;
                 skos:altLabel "NEXAFS microscopy" ,
                               "near edge X-ray absorption fine structure (NEXAFS) microscopy" ,
                               "near-edge X-ray absorption fine structure (NEXAFS) microscopy" ;
                 skos:definition "An imaging technique where soft X-rays (100-1000 eV) are directed at the specimen, and the difference in the X-ray absorption coefficient measured within 40 eV of the absorption edge by different elements (mainly O and C) produces an image. [CHMO]" ;
                 skos:prefLabel "near-edge X-ray absorption fine structure microscopy" .


###  http://purl.allotrope.org/ontologies/process#AFP_0000492
af-p:AFP_0000492 rdf:type owl:Class ;
                 rdfs:subClassOf af-p:AFP_0001216 ;
                 skos:altLabel "s-AFMIR" ,
                               "surface AFMIR" ,
                               "surface atomic force microscopy infrared microscopy" ;
                 skos:definition "The simultaneous collection of AFM topography data and spatially-resolved infrared spectra by measuring the infrared absorption via transient deformation of the AFM cantilever induced by an infrared pulsed laser (tuned to a wavelength that corresponds to a vibrational absorbing wavelength in the specimen) as a function of AFM tip position. Mid-IR radiation, generated using a periodically poled LiNbO3 crystal emitting tuneable laser is focussed directly on the specimen surface. [CHMO]" ;
                 skos:prefLabel "surface atomic force infrared microscopy" .


###  http://purl.allotrope.org/ontologies/process#AFP_0000635
af-p:AFP_0000635 rdf:type owl:Class ;
                 rdfs:subClassOf af-p:AFP_0000239 ;
                 skos:definition "A type of spectroscopy where the sample (in the form of a molecular beam) is vaporised by laser ablation before being irradiated with a single pulse of radiation in the microwave region (1-1000 mm) and the spectrum is subject to a Fourier transform. [CHMO]" ;
                 skos:prefLabel "laser ablation molecular beam Fourier transform microwave spectroscopy" .


###  http://purl.allotrope.org/ontologies/process#AFP_0000787
af-p:AFP_0000787 rdf:type owl:Class ;
                 rdfs:subClassOf af-p:AFP_0001216 ;
                 skos:altLabel "standard AFMIR" ,
                               "standard atomic force microscopy infrared microscopy" ;
                 skos:definition "The simultaneous collection of AFM topography data and spatially-resolved infrared spectra by measuring the infrared absorption via transient deformation of the AFM cantilever induced by an infrared pulsed laser (tuned to a wavelength that corresponds to a vibrational absorbing wavelength in the specimen) as a function of AFM tip position. The specimen is deposited on an ATR-compatible ZnSe prism and infrared light is introduced into the prism at an angle exceeding the critical angle for internal reflection. This produces an evanescent wave at the reflecting surface. [CHMO]" ;
                 skos:prefLabel "standard atomic force infrared microscopy" .


###  http://purl.allotrope.org/ontologies/process#AFP_0000850
af-p:AFP_0000850 rdf:type owl:Class ;
                 rdfs:subClassOf af-p:AFP_0000044 ;
                 skos:altLabel "IM" ;
                 skos:definition "A type of microscopy where ions are used to produce an image. [CHMO]" ;
                 skos:prefLabel "ion microscopy" .


###  http://purl.allotrope.org/ontologies/process#AFP_0000954
af-p:AFP_0000954 rdf:type owl:Class ;
                 rdfs:subClassOf af-p:AFP_0001412 ;
                 skos:altLabel "MRFM" ;
                 skos:definition "A type of microscopy which uses a cantilever tipped with a ferromagnetic (iron cobalt) particle to directly detect a modulated spin gradient force between sample spins and the tip to scan the surface of a magnetic specimen. As the ferromagnetic tip moves close to the sample, the nuclear spins become attracted to it and generate a small force on the cantilever. The spins are then repeatedly flipped, causing the cantilever to gently sway back and forth in a synchronous motion. That displacement is measured with an interferometer to create a series of 2D images of the sample. [CHMO]" ;
                 skos:prefLabel "magnetic resonance force microscopy" .


###  http://purl.allotrope.org/ontologies/process#AFP_0001097
af-p:AFP_0001097 rdf:type owl:Class ;
                 rdfs:subClassOf af-p:AFP_0002198 ;
                 skos:altLabel "SIMS imaging" ,
                               "SIMS microscopy" ,
                               "secondary ion mass spectroscopy imaging" ;
                 skos:definition "The collection of spatially resolved mass spectra of a sample during microscopy where the sample is bombarded with a stream of primary mass-selected particles and the secondary ions ejected from the sample are detected. The spectra are used to visualise the spatial distribution of compounds by their molecular masses. [CHMO]" ;
                 skos:prefLabel "secondary ion mass spectrometry imaging" .


###  http://purl.allotrope.org/ontologies/process#AFP_0001152
af-p:AFP_0001152 rdf:type owl:Class ;
                 rdfs:subClassOf af-p:AFP_0001339 ;
                 skos:altLabel "PEMS" ,
                               "PESM" ,
                               "photoelectron micro-spectrometry" ,
                               "photoelectron micro-spectroscopy" ,
                               "photoelectron microspectrometry" ;
                 skos:definition "A type of spectroscopy where the sample is illuminated with a finely focused (<10 m) photon beam causing ionization and the emission of photoelectrons, the energies of which are measured. [CHMO]" ;
                 skos:prefLabel "photoelectron microspectroscopy" .


###  http://purl.allotrope.org/ontologies/process#AFP_0001216
af-p:AFP_0001216 rdf:type owl:Class ;
                 rdfs:subClassOf af-p:AFP_0000782 ;
                 skos:altLabel "AFMIR" ,
                               "atomic force microscopy infrared microscopy" ;
                 skos:definition "The simultaneous collection of AFM topography data and spatially-resolved IR spectra by measuring the IR absorption via transient deformation of the AFM cantilever induced by an infrared pulsed laser (tuned to a wavelength that corresponds to a vibrational absorbing wavelength in the specimen) as a function of AFM tip position. [CHMO]" ;
                 skos:prefLabel "atomic force infrared microscopy" .


###  http://purl.allotrope.org/ontologies/process#AFP_0001301
af-p:AFP_0001301 rdf:type owl:Class ;
                 rdfs:subClassOf af-p:AFP_0001152 ;
                 skos:altLabel "EUV photoelectron micro-spectroscopy" ,
                               "EUV photoelectron microspectroscopy" ,
                               "extreme ultra-violet photoelectron microspectroscopy" ;
                 skos:definition "A type of spectroscopy where the sample is illuminated with a finely focused (<10 m) extreme ultraviolet (10-121 nm) photon beam causing ionization and the emission of photoelectrons, the energies of which are measured. [CHMO]" ;
                 skos:prefLabel "extreme ultraviolet photoelectron microspectroscopy" .


###  http://purl.allotrope.org/ontologies/process#AFP_0001322
af-p:AFP_0001322 rdf:type owl:Class ;
                 rdfs:subClassOf af-p:AFP_0002432 ;
                 skos:definition "A type of chemical imaging where an optical microscope is used to image the sample and locate a small area for fluorescence spectroscopy. [CHMO]" ;
                 skos:prefLabel "microspectrofluorometry" .


###  http://purl.allotrope.org/ontologies/process#AFP_0001452
af-p:AFP_0001452 rdf:type owl:Class ;
                 rdfs:subClassOf af-p:AFP_0002343 ;
                 skos:altLabel "X-ray fluorescence imaging" ,
                               "XFM" ,
                               "XRF imaging" ,
                               "x-ray fluorescence microprobe (XFM) analysis" ;
                 skos:definition "An imaging technique where a beam of X-rays is directed at the specimen and the intensities of the X-rays emitted due to core-to-core transitions (known as 'X-ray fluorescence') are detected as a function of wavelength and position. As these energies are element-specific, X-ray fluorescence microscopy can be used to determine spatially-resolved elemental composition. [CHMO]" ;
                 skos:prefLabel "X-ray fluorescence microscopy" .


###  http://purl.allotrope.org/ontologies/process#AFP_0001513
af-p:AFP_0001513 rdf:type owl:Class ;
                 rdfs:subClassOf af-p:AFP_0000418 ;
                 skos:altLabel "two photon excitation microscopy" ,
                               "two photon fluorescence imaging" ,
                               "two-photon excitation imaging" ,
                               "two-photon fluorescence imaging" ,
                               "two-photon fluorescence microscopy" ;
                 skos:definition "A type of microscopy where fluorophores in the specimen can be made to fluoresce (emit energy as visible light) by the near-simultaneous absorption of two photons. [CHMO]" ;
                 skos:prefLabel "two photon fluorescence microscopy" .


###  http://purl.allotrope.org/ontologies/process#AFP_0001555
af-p:AFP_0001555 rdf:type owl:Class ;
                 rdfs:subClassOf af-p:AFP_0001864 ;
                 skos:definition "A type of microscopy where atoms of He gas in the vicinty of the specimen are ionized and an image is produced by the projection of the ions onto a fluorescent screen. The image consists of a pattern of spots of light which correspond to individual atoms on the specimen surface. [CHMO]" ;
                 skos:prefLabel "helium-ion microscopy" .


###  http://purl.allotrope.org/ontologies/process#AFP_0001864
af-p:AFP_0001864 rdf:type owl:Class ;
                 rdfs:subClassOf af-p:AFP_0000850 ;
                 skos:altLabel "FIM" ,
                               "field ionization microscopy" ,
                               "field-ion microscopy" ,
                               "field-ionization microscopy" ;
                 skos:definition "A type of microscopy where atoms of an inert gas in the vicinty of the specimen (which is in the form of a very sharp tip <10 m diameter) are ionized by the application of a strong electric field to the tip and an image is produced by the projection of the ions onto a fluorescent screen. The image consists of a pattern of spots of light which correspond to individual atoms on the specimen surface. [CHMO]" ;
                 skos:prefLabel "field ion microscopy" .


###  http://purl.allotrope.org/ontologies/process#AFP_0001904
af-p:AFP_0001904 rdf:type owl:Class ;
                 rdfs:subClassOf af-p:AFP_0002427 ;
                 skos:altLabel "UV-TLM" ,
                               "ultra-violet thermal-lens microscopy" ,
                               "ultraviolet thermal lens microscopy" ,
                               "ultraviolet thermal-lens microscopy" ;
                 skos:definition "A type of microscopy where a probe laser and a pulsed ultra-violet excitation laser and are focused onto a specimen forming a refractive index distribution resulting in a concave excitation beam. The strength of this lens is proportional to the sample concentration and is detected by a change in transmittance in the probe beam. [CHMO]" ;
                 skos:prefLabel "ultra-violet thermal lens microscopy" .


###  http://purl.allotrope.org/ontologies/process#AFP_0002032
af-p:AFP_0002032 rdf:type owl:Class ;
                 rdfs:subClassOf af-p:AFP_0002343 ;
                 skos:altLabel "TXM" ,
                               "transmission XM" ;
                 skos:definition "An imaging technique where a finely focused beam of X-rays is directed at the specimen and the energies and intensities of the transmitted X-rays are measured as a function of position. [CHMO]" ;
                 skos:prefLabel "transmission X-ray microscopy" .


###  http://purl.allotrope.org/ontologies/process#AFP_0002131
af-p:AFP_0002131 rdf:type owl:Class ;
                 rdfs:subClassOf af-p:AFP_0000850 ;
                 skos:altLabel "SIM" ;
                 skos:definition "A type of microscopy where an ion beam is scanned over the specimen surface and the secondary electrons emitted are detected. [CHMO]" ;
                 skos:prefLabel "scanning ion microscopy" .


###  http://purl.allotrope.org/ontologies/process#AFP_0002198
af-p:AFP_0002198 rdf:type owl:Class .


###  http://purl.allotrope.org/ontologies/process#AFP_0002343
af-p:AFP_0002343 rdf:type owl:Class ;
                 rdfs:subClassOf af-p:AFP_0000044 ;
                 skos:altLabel "XM" ,
                               "XRM" ;
                 skos:definition "An imaging technique where soft X-rays (100-1000 eV) are directed at the specimen, and the difference in absorption of the X-rays by different elements (mainly O and C) produces an image. [CHMO]" ;
                 skos:prefLabel "X-ray microscopy" .


###  http://purl.allotrope.org/ontologies/process#AFP_0002399
af-p:AFP_0002399 rdf:type owl:Class ;
                 rdfs:subClassOf af-p:AFP_0002343 ;
                 skos:altLabel "SXM" ,
                               "SXRM" ,
                               "scanning XM" ,
                               "scanning XRM" ;
                 skos:definition "An imaging technique where soft X-rays (100-1000 eV) are scanned across a specimen, and the difference in absorption of the X-rays by different elements (mainly O and C) produces an image. [CHMO]" ;
                 skos:prefLabel "scanning X-ray microscopy" .


###  http://purl.allotrope.org/ontologies/process#AFP_0002427
af-p:AFP_0002427 rdf:type owl:Class ;
                 rdfs:subClassOf af-p:AFP_0000044 ;
                 skos:altLabel "TLM" ,
                               "thermal-lens microscopy" ;
                 skos:definition "A type of microscopy where and excitation laser and probe a laser are focused onto a specimen forming a refractive index distribution which results in a concave excitation beam. The strength of this lens is proportional to the sample concentration and is detected by a change in transmittance in the probe beam. [CHMO]" ;
                 skos:prefLabel "thermal lens microscopy" .


#################################################################
#    Individuals
#################################################################

###  http://purl.allotrope.org/voc/attribution
<http://purl.allotrope.org/voc/attribution> rdf:type owl:NamedIndividual ,
                                                     dct:RightsStatement ;
                                            dct:description """
These taxonomies contain material or may constitute derivative works of material which may be subject to copyright by one of the following organizations.  By using these taxonomies, you agree to the following terms and conditions applicable to its contents:
******************************************************************************
Copyright Notice and Terms for IUPAC Gold Book
______________________________________________________________________________
Copyright © 1998, Regents of the University of California
All rights reserved.
Redistribution and use in source and binary forms, with or without modification, are permitted provided that the following conditions are met:
1. Redistributions of source code must retain the above copyright notice, this list of conditions and the following disclaimer.
2. Redistributions in binary form must reproduce the above copyright notice, this list of conditions and the following disclaimer in the documentation and/or other materials provided with the distribution.
THIS SOFTWARE IS PROVIDED BY THE COPYRIGHT HOLDERS AND CONTRIBUTORS \"AS IS\" AND ANY EXPRESS OR IMPLIED WARRANTIES, INCLUDING, BUT NOT LIMITED TO, THE IMPLIED WARRANTIES OF MERCHANTABILITY AND FITNESS FOR A PARTICULAR PURPOSE ARE DISCLAIMED. IN NO EVENT SHALL THE COPYRIGHT HOLDER OR CONTRIBUTORS BE LIABLE FOR ANY DIRECT, INDIRECT, INCIDENTAL, SPECIAL, EXEMPLARY, OR CONSEQUENTIAL DAMAGES (INCLUDING, BUT NOT LIMITED TO, PROCUREMENT OF SUBSTITUTE GOODS OR SERVICES; LOSS OF USE, DATA, OR PROFITS; OR BUSINESS INTERRUPTION) HOWEVER CAUSED AND ON ANY THEORY OF LIABILITY, WHETHER IN CONTRACT, STRICT LIABILITY, OR TORT (INCLUDING NEGLIGENCE OR OTHERWISE) ARISING IN ANY WAY OUT OF THE USE OF THIS SOFTWARE, EVEN IF ADVISED OF THE POSSIBILITY OF SUCH DAMAGE.
******************************************************************************
Copyright Notice and Terms for PSI-MS (Proteomics Standards Initiative - Mass Spectrometry) Mass spectrometer output files and spectra interpretation
_____________________________________________________________________________
Created by Matt Chambers, Andreas Bertsch, Marius Kallhardt, Eric Deutsch Fredrik Levander, Pierre-Alain Binz, and Gerhard Mayer. Publisher: HUPO Proteomics Standards Initiative Mass Spectrometry Standards Working Group and HUPO Proteomics Standards Initiative Proteomics Informatics Working Group. This work is used pursuant to a Creative Commons license available here: http://creativecommons.org/licenses/by/3.0/legalcode

******************************************************************************
Attribution Notice for National Center for Biomedical Ontology materials.

This work contains material from the Cell Ontology and Clinical Measurement Ontology, available here: http://bioportal.bioontology.org/.
******************************************************************************
Attribution Notice for ChEBI
This work contains material from the European Bioinformatics Institute’s ChEBI database.
******************************************************************************
Attribution Notice for Quantities Units Dimensions Data Types (http://www.qudt.org/)
This work contains content from www.qudt.org and is used pursuant to a Creative Commons License available here: http://creativecommons.org/licenses/by-sa/3.0/us/legalcode. The original work may have been modified.
******************************************************************************
Copyright and Attribution Notice for Dublin Core Metadata Initiative Document
This work contains material from the following DCMI document used pursuant to a creative commons license available here: https://creativecommons.org/licenses/by/4.0/legalcode. This material may have been modified or changed.
Timestamped URL:          http://dublincore.org/documents/2012/06/14/dcmi-terms/
Date Issued:                       2012-06-14
Document Status:            This is a DCMI Recommendation.
Copyright © 1995-2015 DCMI. All Rights Reserved. DCMI liability, trademark/service mark, document use and software licensing rules apply.
******************************************************************************

""" ;
                                            dct:title "Derivative works attribution" .


###  http://purl.allotrope.org/voc/copyright
<http://purl.allotrope.org/voc/copyright> rdf:type owl:NamedIndividual ,
                                                   dct:RightsStatement ;
                                          dct:description "Copyright © 2021 Allotrope Foundation" ;
                                          dct:rightsHolder <http://www.allotrope.org> ;
                                          dct:title "Copyright © 2021 Allotrope Foundation" .


###  http://purl.allotrope.org/voc/creative-commons-attribution-license
<http://purl.allotrope.org/voc/creative-commons-attribution-license> rdf:type owl:NamedIndividual ,
                                                                              dct:LicenseDocument ;
                                                                     dct:description """This work is licensed under a Creative Commons Attribution 4.0 International License http://creativecommons.org/licenses/by/4.0/.

THESE MATERIALS ARE PROVIDED \"AS IS\" AND ALLOTROPE EXPRESSLY DISCLAIMS ALL WARRANTIES, EXPRESS, IMPLIED OR STATUTORY, INCLUDING, WITHOUT LIMITATION, THE WARRANTIES OF NON-INFRINGEMENT, TITLE, MERCHANTABILITY AND FITNESS FOR A PARTICULAR PURPOSE.

Copyright © 2015-2025 Allotrope Foundation
""" ;
                                                                     dct:title "Creative Commons Attribution 4.0 International Public License" .


###  Generated by the OWL API (version 5.1.19) https://github.com/owlcs/owlapi/
