@prefix : <http://purl.allotrope.org/voc/afo/domain/WD/2025/06/nmr#> .
@prefix cl: <http://purl.obolibrary.org/obo/CL> .
@prefix go: <http://purl.obolibrary.org/obo/GO> .
@prefix ro: <http://purl.obolibrary.org/obo/RO> .
@prefix bfo: <http://purl.obolibrary.org/obo/BFO> .
@prefix dct: <http://purl.org/dc/terms/> .
@prefix iao: <http://purl.obolibrary.org/obo/IAO> .
@prefix obi: <http://purl.obolibrary.org/obo/OBI> .
@prefix owl: <http://www.w3.org/2002/07/owl#> .
@prefix rdf: <http://www.w3.org/1999/02/22-rdf-syntax-ns#> .
@prefix xml: <http://www.w3.org/XML/1998/namespace> .
@prefix xsd: <http://www.w3.org/2001/XMLSchema#> .
@prefix af-c: <http://purl.allotrope.org/ontologies/common#> .
@prefix af-e: <http://purl.allotrope.org/ontologies/equipment#> .
@prefix af-m: <http://purl.allotrope.org/ontologies/material#> .
@prefix af-p: <http://purl.allotrope.org/ontologies/process#> .
@prefix af-q: <http://purl.allotrope.org/ontologies/quality#> .
@prefix af-r: <http://purl.allotrope.org/ontologies/result#> .
@prefix af-x: <http://purl.allotrope.org/ontologies/property#> .
@prefix rdfs: <http://www.w3.org/2000/01/rdf-schema#> .
@prefix skos: <http://www.w3.org/2004/02/skos/core#> .
@prefix af-cur: <http://purl.allotrope.org/ontologies/curation#> .
@base <http://purl.allotrope.org/voc/afo/domain/WD/2025/06/nmr#> .

<http://purl.allotrope.org/voc/afo/domain/WD/2025/06/nmr> rdf:type owl:Ontology ;
                                                                     owl:versionIRI <http://purl.allotrope.org/voc/afo/domain/WD/2025/06/nmr> ;
                                                                     owl:imports <http://purl.allotrope.org/voc/afo/WD/2025/06/afo> ,
                                                                                 <http://purl.allotrope.org/voc/afo/domain/REC/2025/06/nmr> ;
                                                                     dct:issued "2025-06-25T12:00:00Z"^^xsd:dateTime ;
                                                                     dct:license <http://purl.allotrope.org/voc/creative-commons-attribution-license> ;
                                                                     dct:modified "2025-04-04T12:00:00Z"^^xsd:dateTime ;
                                                                     dct:rights <http://purl.allotrope.org/voc/attribution> ,
                                                                                <http://purl.allotrope.org/voc/copyright> ;
                                                                     dct:title "AFO NMR Domain Ontology (WD/2025/06)" ;
                                                                     owl:priorVersion <http://purl.allotrope.org/voc/afo/domain/WD/2025/03/nmr> ;
                                                                     owl:versionInfo "WD/2025/06" .

#################################################################
#    Annotation properties
#################################################################

###  http://purl.allotrope.org/ontologies/property#AFX_0002796
af-x:AFX_0002796 rdf:type owl:AnnotationProperty .


###  http://purl.allotrope.org/ontologies/property#AFX_0002798
af-x:AFX_0002798 rdf:type owl:AnnotationProperty .


###  http://purl.allotrope.org/ontologies/property#AFX_0002809
af-x:AFX_0002809 rdf:type owl:AnnotationProperty .


###  http://purl.org/dc/terms/source
dct:source rdf:type owl:AnnotationProperty .


###  http://www.w3.org/2004/02/skos/core#altLabel
skos:altLabel rdf:type owl:AnnotationProperty .


###  http://www.w3.org/2004/02/skos/core#changeNote
skos:changeNote rdf:type owl:AnnotationProperty .


###  http://www.w3.org/2004/02/skos/core#definition
skos:definition rdf:type owl:AnnotationProperty .


###  http://www.w3.org/2004/02/skos/core#example
skos:example rdf:type owl:AnnotationProperty .


###  http://www.w3.org/2004/02/skos/core#note
skos:note rdf:type owl:AnnotationProperty .


###  http://www.w3.org/2004/02/skos/core#prefLabel
skos:prefLabel rdf:type owl:AnnotationProperty .


###  http://www.w3.org/2004/02/skos/core#scopeNote
skos:scopeNote rdf:type owl:AnnotationProperty .


#################################################################
#    Object Properties
#################################################################

###  http://purl.allotrope.org/ontologies/property#AFX_0000310
af-x:AFX_0000310 rdf:type owl:ObjectProperty ;
                 rdfs:range af-r:AFR_0000148 ;
                 skos:definition "The peak multiplicity observed for a coupled system in a chemical moeity. [Allotrope]" ;
                 skos:prefLabel "multiplicity" .


#################################################################
#    Classes
#################################################################

###  http://purl.allotrope.org/ontologies/equipment#AFE_0000011
af-e:AFE_0000011 rdf:type owl:Class ;
                 rdfs:subClassOf af-e:AFE_0000644 ;
                 skos:definition "A low frequency nuclear magnetic resonance spectrometer that is significantly more compact and portable than the conventional free standing equivalents. [Allotrope]" ;
                 skos:prefLabel "benchtop nuclear magnetic resonance spectrometer" .


###  http://purl.allotrope.org/ontologies/equipment#AFE_0000033
af-e:AFE_0000033 rdf:type owl:Class ;
                 rdfs:subClassOf af-e:AFE_0000736 ;
                 skos:definition "One of two small coiled electromagnets that perturbs the bulk magnetisation of a sample from equilibrium through a series of RF pulses and records the minute electrical signals as the bulk perturbed magnetisation relaxes back to its equilibrium state. The outer coil is the second RF coil of two wound on top of each other, the one furtherest away from the sample that is least tightly coupled to the sample under investigation. [Allotrope]" ;
                 skos:prefLabel "nuclear magnetic resonance probe outer RF coil" .


###  http://purl.allotrope.org/ontologies/equipment#AFE_0000096
af-e:AFE_0000096 rdf:type owl:Class ;
                 rdfs:subClassOf af-e:AFE_0000084 ;
                 skos:altLabel "dual broadband nuclear magnetic resonance probe" ;
                 skos:changeNote "2024-09-11 Changed [Amgen] attribution to [Allotrope] and fixed typo in prefLabel." ;
                 skos:definition "Tunable NMR spectrometer probe containing at least one channel with a broad tuning range. One RF channel is generally optimized for 1H observation and decoupling and not broadband, but can sometines be tuned to 19F. The second RF channel is generally used for the observation of nuclei other than 1H (eg. 13C, 15N). [Allotrope]" ;
                 skos:prefLabel "broadband nuclear magnetic resonance probe" .


###  http://purl.allotrope.org/ontologies/equipment#AFE_0000127
af-e:AFE_0000127 rdf:type owl:Class ;
                 rdfs:subClassOf af-e:AFE_0000718 ;
                 af-x:AFX_0002798 "true"^^xsd:boolean ;
                 af-x:AFX_0002809 obi:_0000578 ;
                 skos:altLabel "NMR tube" ;
                 skos:definition "The sample-tube holds the NMR sample and sits in the NMR probe. It is usually a fused quartz tube of 1.7 to 20 mm diameter. [Allotrope]" ;
                 skos:prefLabel "nuclear magnetic resonance tube" .


###  http://purl.allotrope.org/ontologies/equipment#AFE_0000258
af-e:AFE_0000258 rdf:type owl:Class ;
                 rdfs:subClassOf af-e:AFE_0000127 ;
                 af-x:AFX_0002798 "true"^^xsd:boolean ;
                 skos:altLabel "NMR shigemi tube" ;
                 skos:changeNote "2024-09-11 Changed [Amgen] attribution to [Allotrope]." ;
                 skos:definition "A Shigemi tube is a microscale NMR tube that uses susceptibility-matched glass to reduce the sample size within the RF coil region. Shigemi tubes may be appropriate for mass-limited sample. [Allotrope]" ;
                 skos:prefLabel "nuclear magnetic resonance shigemi tube" .


###  http://purl.allotrope.org/ontologies/equipment#AFE_0000261
af-e:AFE_0000261 rdf:type owl:Class ;
                 rdfs:subClassOf af-e:AFE_0000371 ;
                 af-x:AFX_0002798 "true"^^xsd:boolean ;
                 skos:altLabel "inner dewar" ;
                 skos:definition "The inner dewar of the NMR spectrometer containing the liquid helium. [Allotrope]" ;
                 skos:prefLabel "nuclear magnetic resonance spectrometer inner dewar" .


###  http://purl.allotrope.org/ontologies/equipment#AFE_0000269
af-e:AFE_0000269 rdf:type owl:Class ;
                 rdfs:subClassOf af-e:AFE_0000371 ;
                 af-x:AFX_0002798 "true"^^xsd:boolean ;
                 skos:altLabel "outer dewar" ;
                 skos:definition "A dewar in the NMR spectrometer that surrounds the inner dewar and contains liquid nitrogen. [Allotrope]" ;
                 skos:prefLabel "nuclear magnetic resonance outer dewar" .


###  http://purl.allotrope.org/ontologies/equipment#AFE_0000288
af-e:AFE_0000288 rdf:type owl:Class ;
                 rdfs:subClassOf af-e:AFE_0000084 ;
                 skos:definition "NMR spectrometer probe where the sample remains at ambient or regulated temperature, and  the probe RF coils and preamplifiers are typically cooled to around 10-15 K to aid in signal sensitivity and reducing the signal-to-noise (S/N) ratio. [Allotrope]" ;
                 skos:prefLabel "nuclear magnetic resonance cryoprobe" .


###  http://purl.allotrope.org/ontologies/equipment#AFE_0000371
af-e:AFE_0000371 rdf:type owl:Class ;
                 rdfs:subClassOf af-e:AFE_0000852 ,
                                 af-e:AFE_0001187 ;
                 af-x:AFX_0002798 "true"^^xsd:boolean ;
                 skos:definition "A tank inside the NMR spectrometer to support the cooling of some of the NMR probe electronics down to superconducting temperatures. [Allotrope]" ;
                 skos:prefLabel "nuclear magnetic resonance dewar" .


###  http://purl.allotrope.org/ontologies/equipment#AFE_0000503
af-e:AFE_0000503 rdf:type owl:Class ;
                 rdfs:subClassOf af-e:AFE_0000354 ;
                 skos:altLabel "NMR spinner" ;
                 skos:definition "A device that firmly holds the NMR tube in place to avoid the sample wobble and sample field inhomogeneity in the magnetic field. The spinner is spun by nitrogen or anhydrous aid at about 20Hz inside the NMR spectrometer. The spinner also serves as a loosly fitting piston head so that the sample can be slowly inserted into and slowly retrieved from inside the NMR spectrometer via gas flow/pressure. [Allotrope]" ;
                 skos:prefLabel "nuclear magnetic resonance spinner" .


###  http://purl.allotrope.org/ontologies/equipment#AFE_0000636
af-e:AFE_0000636 rdf:type owl:Class ;
                 rdfs:subClassOf af-e:AFE_0000736 ;
                 skos:definition "One of two small coiled electromagnets that perturbs the bulk magnetisation of a sample from equilibrium through a series of RF pulses and records the minute electrical signals as the bulk perturbed magnetisation relaxes back to its equilibrium state. The inner coil is the first RF coil of two wound on top of each other, that is closest to the sample, that gives best sensitivity as it is closest to and most tightly coupled to the sample under investigation. [Allotrope]" ;
                 skos:prefLabel "nuclear magnetic resonance probe inner RF coil" .


###  http://purl.allotrope.org/ontologies/equipment#AFE_0000736
af-e:AFE_0000736 rdf:type owl:Class ;
                 rdfs:subClassOf af-e:AFE_0000354 ;
                 skos:definition "The small coiled electromagnet that perturbs the bulk magnetisation of a sample from equilibrium through a series of RF pulses and records the minute electrical signals as the bulk perturbed magnetisation relaxes back to its equilibrium state. [Allotrope]" ;
                 skos:prefLabel "nuclear magnetic resonance probe RF coil" .


###  http://purl.allotrope.org/ontologies/equipment#AFE_0000780
af-e:AFE_0000780 rdf:type owl:Class ;
                 rdfs:subClassOf af-e:AFE_0000354 ;
                 skos:definition "A rod exposed on the NMR probe to manually tune a broad band probe to an X nucleus. [Allotrope]" ;
                 skos:prefLabel "nuclear magnetic resonance tuning rod" .


###  http://purl.allotrope.org/ontologies/equipment#AFE_0000880
af-e:AFE_0000880 rdf:type owl:Class ;
                 rdfs:subClassOf af-e:AFE_0000084 ;
                 skos:definition "Tunable NMR spectrometer probe that may be tuned to pulse up to four nuclei in a single NMR experiment. [Allotrope]" ;
                 skos:prefLabel "quadruple nuclear magnetic resonance probe" .


###  http://purl.allotrope.org/ontologies/equipment#AFE_0001642
af-e:AFE_0001642 rdf:type owl:Class ;
                 rdfs:subClassOf af-e:AFE_0000354 ;
                 skos:definition "The lock system is a device that locks the magnetic field strength of an NMR spectrometer at a desired, constant value. [Allotrope]" ;
                 skos:prefLabel "lock system" .


###  http://purl.allotrope.org/ontologies/equipment#AFE_0001643
af-e:AFE_0001643 rdf:type owl:Class ;
                 rdfs:subClassOf af-e:AFE_0000644 ;
                 skos:altLabel "solid state NMR spectrometer" ,
                               "ssNMR spectrometer" ;
                 skos:definition "A solid state NMR spectrometer is a type of nuclear magnetic resonance spectrometer that allows for measurement of solid samples. [Allotrope]" ;
                 skos:prefLabel "solid state nuclear magnetic resonance spectrometer" .


###  http://purl.allotrope.org/ontologies/equipment#AFE_0001644
af-e:AFE_0001644 rdf:type owl:Class ;
                 rdfs:subClassOf af-e:AFE_0000096 ;
                 skos:altLabel "HX" ,
                               "HX probe" ,
                               "HY" ,
                               "HY probe" ;
                 skos:definition "A double channel probe is a type of NMR tube that allows for measurements of two different nuclei at the same time. [Allotrope]" ;
                 skos:prefLabel "double channel probe" .


###  http://purl.allotrope.org/ontologies/equipment#AFE_0001645
af-e:AFE_0001645 rdf:type owl:Class ;
                 rdfs:subClassOf af-e:AFE_0000096 ;
                 skos:altLabel "HCN" ,
                               "HCN probe" ;
                 skos:definition "A triple channel probe is a type of NMR tube that allows for measurements of three different nuclei at the same time. [Allotrope]" ;
                 skos:prefLabel "triple channel probe" .


###  http://purl.allotrope.org/ontologies/equipment#AFE_0001646
af-e:AFE_0001646 rdf:type owl:Class ;
                 rdfs:subClassOf af-e:AFE_0000127 ;
                 af-x:AFX_0002798 "true"^^xsd:boolean ;
                 af-x:AFX_0002808 obi:_0000523 ;
                 skos:altLabel "ssNMR tube" ;
                 skos:definition "A rotor is a type of NMR tube usually made of Zirconia that allows for solid state NMR measurements. It can rotate at high frequencies. [Allotrope]" ;
                 skos:prefLabel "rotor" .


###  http://purl.allotrope.org/ontologies/equipment#AFE_0001647
af-e:AFE_0001647 rdf:type owl:Class ;
                 rdfs:subClassOf af-e:AFE_0001646 ;
                 af-x:AFX_0002798 "true"^^xsd:boolean ;
                 skos:definition "A thin wall rotor is a type of ssNMR tube with a thin wall diameter. [Allotrope]" ;
                 skos:prefLabel "thin wall rotor" .


###  http://purl.allotrope.org/ontologies/equipment#AFE_0001649
af-e:AFE_0001649 rdf:type owl:Class ;
                 rdfs:subClassOf af-e:AFE_0001648 ;
                 skos:definition "A rotor cap is a type of cap to seal ssNMR tubes. [Allotrope]" ;
                 skos:example "Vespel cap, Kel-F cap" ;
                 skos:prefLabel "rotor cap" .


###  http://purl.allotrope.org/ontologies/equipment#AFE_0001650
af-e:AFE_0001650 rdf:type owl:Class ;
                 rdfs:subClassOf af-e:AFE_0001646 ;
                 af-x:AFX_0002798 "true"^^xsd:boolean ;
                 skos:definition "A thick wall rotor is a type of ssNMR tube with a thick wall diameter. [Allotrope]" ;
                 skos:prefLabel "thick wall rotor" .


###  http://purl.allotrope.org/ontologies/equipment#AFE_0001652
af-e:AFE_0001652 rdf:type owl:Class ;
                 rdfs:subClassOf af-e:AFE_0000354 ;
                 skos:altLabel "radiofrequency transmitter" ,
                               "transmitter" ,
                               "waveform generator" ;
                 skos:definition "A pulse generator is a device that generates electromagnetic pulses with a certain waveform. [Allotrope]" ;
                 skos:example "pulse generator of an NMR spectrometer" ;
                 skos:prefLabel "pulse generator" .


###  http://purl.allotrope.org/ontologies/equipment#AFE_0001653
af-e:AFE_0001653 rdf:type owl:Class ;
                 rdfs:subClassOf af-e:AFE_0000354 ;
                 skos:definition "The magic angle spinning controller is a device that allows for setting up and controlling the properties of the magic angle spinning. [Allotrope]" ;
                 skos:prefLabel "magic angle spinning controller" .


###  http://purl.allotrope.org/ontologies/equipment#AFE_0001654
af-e:AFE_0001654 rdf:type owl:Class ;
                 rdfs:subClassOf af-e:AFE_0001646 ;
                 af-x:AFX_0002798 "true"^^xsd:boolean ;
                 skos:altLabel "MAS rotor" ,
                               "rotor" ;
                 skos:definition "A ceramic rotor is a type of ssNMR tube that consists of ceramic material. [Allotrope]" ;
                 skos:note "The size of the rotor is typically given by the outer diameter of the rotor, for example, 4.0 mm, 2.5 mm and 1.3 mm are standard rotor sizes." ;
                 skos:prefLabel "ceramic rotor" .


###  http://purl.allotrope.org/ontologies/equipment#AFE_0001656
af-e:AFE_0001656 rdf:type owl:Class ;
                 rdfs:subClassOf af-e:AFE_0000354 ;
                 skos:altLabel "shim system" ;
                 skos:definition "A shim is a device that allows for adjustment of the homogeneity of a magnetic field. [Allotrope]" ;
                 skos:prefLabel "shim" .


###  http://purl.allotrope.org/ontologies/equipment#AFE_0001657
af-e:AFE_0001657 rdf:type owl:Class ;
                 rdfs:subClassOf af-e:AFE_0000882 ;
                 af-x:AFX_0002798 "true"^^xsd:boolean ;
                 skos:altLabel "SB magnet" ;
                 skos:definition "A standard bore magnet is a superconducting magnet that has a standard bore. [Allotrope]" ;
                 skos:prefLabel "standard bore magnet" .


###  http://purl.allotrope.org/ontologies/equipment#AFE_0001658
af-e:AFE_0001658 rdf:type owl:Class ;
                 rdfs:subClassOf af-e:AFE_0000882 ;
                 af-x:AFX_0002798 "true"^^xsd:boolean ;
                 skos:altLabel "WB magnet" ;
                 skos:definition "A wide bore magnet is a superconducting magnet that has a wide bore. [Allotrope]" ;
                 skos:prefLabel "wide bore magnet" .


###  http://purl.allotrope.org/ontologies/process#AFP_0000001
af-p:AFP_0000001 rdf:type owl:Class ;
                 rdfs:subClassOf af-p:AFP_0000759 ;
                 skos:definition "A dimensionality reduction technique used in multidimensional NMR experiments. A nD NMR experiment is represented in n-1 dimensions by concerted, simultaneous interrogation of two spectral dimensions. [CHMO]" ;
                 skos:prefLabel "accordion spectroscopy" .


###  http://purl.allotrope.org/ontologies/process#AFP_0000024
af-p:AFP_0000024 rdf:type owl:Class ;
                 rdfs:subClassOf af-p:AFP_0002287 ;
                 skos:altLabel "selective INEPT" ;
                 skos:definition "A heteronuclear NMR experiment in which magnetization arising from 1H nuclei is transferred to covalently bound heteronuclei, thereby enhancing the NMR signal of the heteronuclei. Selective pulses, that only excite or 'select' some of the signals in the spectrum are used in this experiment. [CHMO]" ;
                 skos:prefLabel "selective insensitive nuclei enhancement by polarization transfer" .


###  http://purl.allotrope.org/ontologies/process#AFP_0000038
af-p:AFP_0000038 rdf:type owl:Class ;
                 rdfs:subClassOf af-p:AFP_0001702 ;
                 skos:altLabel "pulse ENDOR" ,
                               "pulse ENDOR spectroscopy" ,
                               "pulsed ENDOR" ,
                               "pulsed ENDOR spectroscopy" ;
                 skos:definition "A type of spectroscopy where a microwave frequency pulse is used to saturate the electron resonance transitions in a sample, and a radio frequency pulse is used excite a nuclear transition. [CHMO]" ;
                 skos:prefLabel "pulsed electron nuclear double resonance spectroscopy" .


###  http://purl.allotrope.org/ontologies/process#AFP_0000062
af-p:AFP_0000062 rdf:type owl:Class ;
                 rdfs:subClassOf af-p:AFP_0001230 ;
                 skos:altLabel "3D COSY-NOESY" ,
                               "3D-COSY-NOESY" ,
                               "COSY-NOESY" ;
                 skos:definition "A type of homonuclear three-dimensional NMR experiment in which a second frequency dimension is employed to disperse the signals and reveal correlations between nuclei which are J-coupled (usually <= 3 bonds apart). These signals are then correlated to nuclei that are spatially proximate within the molecule (<= 6 Angstrom apart). [CHMO]" ;
                 skos:prefLabel "correlation spectroscopy-nuclear Overhauser enhancement spectroscopy" .


###  http://purl.allotrope.org/ontologies/process#AFP_0000074
af-p:AFP_0000074 rdf:type owl:Class ;
                 rdfs:subClassOf af-p:AFP_0000681 ;
                 skos:definition "The nuclei being irradiated with an RF pulse is a different nuclei or the same nuclei and a different isotope that the nuclei being observed to relax back to equilibrium for generation of the NMR spectrum. [Allotrope]" ;
                 skos:prefLabel "heteronuclear decoupling" .


###  http://purl.allotrope.org/ontologies/process#AFP_0000086
af-p:AFP_0000086 rdf:type owl:Class ;
                 rdfs:subClassOf af-p:AFP_0001888 ;
                 skos:altLabel "BIRD" ,
                               "bilinear rotation decoupling" ;
                 skos:definition "A pulse cluster (a spin echo on 1H with inversion of 13C in the centre) used to achieve selective inversion of 12C-bound protons, thus achieving the removal of signals due to 12C-bound nuclei. For the pulse sequence see Chem. Phys. Lett., (1982), 93, pg 504. [CHMO]" ;
                 skos:prefLabel "bilinear rotation decoupling pulse sequence" .


###  http://purl.allotrope.org/ontologies/process#AFP_0000103
af-p:AFP_0000103 rdf:type owl:Class ;
                 rdfs:subClassOf af-p:AFP_0000906 ;
                 skos:altLabel "TPPM" ,
                               "TPPM pulse sequence" ,
                               "TPPM sequence" ,
                               "two pulse phase modulation" ,
                               "two-pulse phase modulation" ;
                 skos:definition "A continuous sequence of pulses used in magic angle spinning NMR to remove the effects of heteronuclear dipolar coupling. For the pulse sequence see J. Chem. Phys., (1996), 103, pg 6951. [CHMO]" ;
                 skos:prefLabel "two pulse phase modulation pulse sequence" .


###  http://purl.allotrope.org/ontologies/process#AFP_0000127
af-p:AFP_0000127 rdf:type owl:Class ;
                 rdfs:subClassOf af-p:AFP_0000305 ;
                 skos:altLabel "PFG-SE NMR" ,
                               "PFGSE" ,
                               "PFGSE-NMR" ,
                               "PGSE" ,
                               "pulsed field gradient (PFG) spin echo" ,
                               "pulsed field gradient spin-echo" ,
                               "pulsed field gradient-spin echo" ,
                               "pulsed field-gradient spin echo" ,
                               "pulsed-field-gradient spin-echo NMR spectroscopy" ;
                 skos:definition "An NMR experiment in which pulsed field gradients are applied to a spin echo sequence to cleanly and precisely excite particular resonances. Additionally, attenuation of signals occurs related to molecular diffusion allowing this technique to be used to determine self-diffusion coefficients. [CHMO]" ;
                 skos:prefLabel "pulsed field-gradient spin echo nuclear magnetic resonance spectroscopy" .


###  http://purl.allotrope.org/ontologies/process#AFP_0000144
af-p:AFP_0000144 rdf:type owl:Class ;
                 rdfs:subClassOf af-p:AFP_0001882 ;
                 skos:altLabel "GHMBC" ,
                               "gHMBC" ,
                               "gradient heteronuclear multiple bond coherence" ,
                               "gradient-selected HMBC" ;
                 skos:definition "A type of heteronuclear NMR spectroscopy where pulsed-field gradients are used and a second frequency dimension is employed to disperse the signals and reveal correlations between protons and nuclei which are 2-3 bonds removed. [CHMO]" ;
                 skos:prefLabel "gradient-selected heteronuclear multiple bond coherence" .


###  http://purl.allotrope.org/ontologies/process#AFP_0000199
af-p:AFP_0000199 rdf:type owl:Class ;
                 rdfs:subClassOf af-p:AFP_0000038 ;
                 skos:altLabel "95Mo ENDOR" ,
                               "95Mo ENDOR spectroscopy" ,
                               "molybdenum-95 ENDOR" ,
                               "molybdenum-95 ENDOR spectroscopy" ;
                 skos:definition "A type of spectroscopy where a microwave frequency pulse is used to saturate the electron resonance transitions in the 95Mo nuclei of a sample, and a radio frequency pulse is used excite a nuclear transition. [CHMO]" ;
                 skos:prefLabel "95Mo electron nuclear double resonance spectroscopy" .


###  http://purl.allotrope.org/ontologies/process#AFP_0000212
af-p:AFP_0000212 rdf:type owl:Class ;
                 rdfs:subClassOf af-p:AFP_0000318 ;
                 skos:altLabel "MAS QCPMG" ,
                               "MAS-QCPMG" ,
                               "QCPMG MAS" ,
                               "QCPMG-MAS" ;
                 skos:definition "An NMR experiment used to enhance the sensitivity of low gyromagnetic ratio nuclei by collapsing the intensity of the 'full' spectrum into discrete 'spikelets'/peaks. The intensities of the peaks vary according to the spin-spin relaxation rate (T2) and the envelope described by these peaks represents the full, static spectrum. The solid sample is spun rapidly at the magic angle (54.74 deg. with respect to the direction of the magnetic field) to reduce line broadening. [CHMO]" ;
                 skos:prefLabel "quadrupole Carr-Purcell-Meiboom-Gill using magic-angle spinning" .


###  http://purl.allotrope.org/ontologies/process#AFP_0000248
af-p:AFP_0000248 rdf:type owl:Class ;
                 rdfs:subClassOf af-p:AFP_0000759 ;
                 skos:altLabel " inversion recovery Fourier transform " ,
                               "IRFT" ,
                               "T1" ,
                               "relaxation time measurement" ;
                 skos:definition "An NMR experiment which measures spin-lattice (T1) relaxation rates by acquiring spectra at different delay times following inversion of the spin-state populations. [CHMO]" ;
                 skos:prefLabel "inversion recovery" .


###  http://purl.allotrope.org/ontologies/process#AFP_0000262
af-p:AFP_0000262 rdf:type owl:Class ;
                 rdfs:subClassOf af-p:AFP_0000759 ;
                 skos:altLabel "CSA experiment" ;
                 skos:definition "An NMR experiment in which differences in chemical shift are used to give information about the orientation of those spins with respect to the field and, thus, the orientation of the molecule. [CHMO]" ;
                 skos:prefLabel "chemical shift anisotropy experiment" .


###  http://purl.allotrope.org/ontologies/process#AFP_0000276
af-p:AFP_0000276 rdf:type owl:Class ;
                 rdfs:subClassOf af-p:AFP_0002063 ;
                 skos:altLabel "2D J-resolved spectroscopy " ,
                               "2D J-spectroscopy" ,
                               "2DJ spectroscopy" ,
                               "J-RES" ,
                               "J-resolved NMR" ,
                               "J-resolved NMR spectrometry" ,
                               "J-resolved NMR spectroscopy" ,
                               "J-resolved spectrometry" ,
                               "J-resolved spectroscopy" ,
                               "J-resolved spectroscopy NMR spectroscopy" ,
                               "J-spectrometry" ,
                               "JRES" ,
                               "JRES NMR" ,
                               "two-dimensional J-spectroscopy" ;
                 skos:definition "A type of homonuclear proton-proton NMR spectroscopy where chemical shift and J-coupling information are separated onto different frequency axes. [CHMO]" ;
                 skos:prefLabel "J-spectroscopy" .


###  http://purl.allotrope.org/ontologies/process#AFP_0000277
af-p:AFP_0000277 rdf:type owl:Class ;
                 rdfs:subClassOf af-p:AFP_0000906 ;
                 skos:altLabel "DUMBO" ,
                               "DUMBO pulse sequence" ,
                               "DUMBO sequence" ,
                               "decoupling using mind boggling optimization" ,
                               "decoupling using mind-boggling optimization" ;
                 skos:definition "A sequence of pulses used in magic angle spinning NMR to remove the effect of homonuclear dipolar couplings. For the pulse sequence see Chem. Phys. Lett., (2004), 398, pg 532. [CHMO]" ;
                 skos:prefLabel "decoupling using mind-boggling optimization pulse sequence" .


###  http://purl.allotrope.org/ontologies/process#AFP_0000278
af-p:AFP_0000278 rdf:type owl:Class ;
                 rdfs:subClassOf af-p:AFP_0002056 ;
                 skos:altLabel "EXORCYCLE" ;
                 skos:definition "A phase cycle technique used in FT NMR experiments whereby the sense of application (or phase) of the RF pulses is altered on repeating the experiment to eliminate spectral artefacts. Exorcyle takes its name from the fact that it is used to remove 'phantom' and 'ghost' peaks. For the technique see J. Magn. Reson., (1977), 27, pg 511. [CHMO]" ;
                 skos:prefLabel "exorcycle" .


###  http://purl.allotrope.org/ontologies/process#AFP_0000280
af-p:AFP_0000280 rdf:type owl:Class ;
                 rdfs:subClassOf af-p:AFP_0002044 ;
                 skos:altLabel "Hadamard NMR spectroscopy" ,
                               "Hadamard encoded NMR" ,
                               "Hadamard nuclear magnetic resonance spectroscopy" ,
                               "Hadamard-encoded NMR" ;
                 skos:definition "An NMR experiment in which multiple frequencies in an NMR spectrum are excited simultaneously over a broad frequency range using polychromatic pulses. [CHMO]" ;
                 skos:prefLabel "Hadamard-encoded nuclear magnetic resonance spectroscopy" .


###  http://purl.allotrope.org/ontologies/process#AFP_0000285
af-p:AFP_0000285 rdf:type owl:Class ;
                 rdfs:subClassOf af-p:AFP_0001927 ;
                 skos:altLabel "WURST" ,
                               "WURST pulse" ,
                               "wideband, uniform rate and smooth truncation" ;
                 skos:definition "An adiabatic shaped pulse incorporating a linear sweep through a frequency range used for selective inversion of spin state populations over wide ranges. For the pulse see J. Magn. Reson., Ser. A, (1995), 115, pg 273. [CHMO]" ;
                 skos:prefLabel "wideband, uniform rate and smooth truncation pulse" .


###  http://purl.allotrope.org/ontologies/process#AFP_0000288
af-p:AFP_0000288 rdf:type owl:Class ;
                 rdfs:subClassOf af-p:AFP_0000721 ;
                 skos:altLabel "GARP" ,
                               "GARP pulse sequence" ,
                               "GARP sequence" ,
                               "globally-optimized alternating phase rectangular pulse" ;
                 skos:definition "A sequence of composite pulses designed to remove signal splitting due to heteronuclear J-couplings in multinuclear liquid NMR experiments. For the pulse sequence see J. Magn. Reson., (1985), 64, pg 547. [CHMO]" ;
                 skos:prefLabel "globally optimized alternating phase rectangular pulse" .


###  http://purl.allotrope.org/ontologies/process#AFP_0000305
af-p:AFP_0000305 rdf:type owl:Class ;
                 rdfs:subClassOf af-p:AFP_0002044 ;
                 skos:altLabel "NMR diffusometry" ;
                 skos:definition "Any type of NMR spectroscopy used to measure diffusion coefficients. [CHMO]" ;
                 skos:prefLabel "nuclear magnetic resonance diffusometry" .


###  http://purl.allotrope.org/ontologies/process#AFP_0000308
af-p:AFP_0000308 rdf:type owl:Class ;
                 rdfs:subClassOf af-p:AFP_0002044 ;
                 skos:altLabel "3D NMR" ,
                               "3D NMR spectroscopy" ,
                               "3D-NMR" ,
                               "3D-NMR spectroscopy" ,
                               "three-dimensional (3D) NMR" ,
                               "three-dimensional NMR" ,
                               "three-dimensional NMR spectroscopy" ;
                 skos:definition "Any type of nuclear magnetic resonance spectroscopy in which three independent frequency dimensions are employed for the correlation and dispersal of signals (by employing two magnetization transfer steps). Each signal is described by three frequencies, thus effecting the distribution of signals within a cube. [CHMO]" ;
                 skos:prefLabel "three-dimensional nuclear magnetic resonance spectroscopy" .


###  http://purl.allotrope.org/ontologies/process#AFP_0000311
af-p:AFP_0000311 rdf:type owl:Class ;
                 rdfs:subClassOf af-p:AFP_0000721 ;
                 skos:altLabel "MLEV" ,
                               "MLEV pulse sequence" ,
                               "MLEV sequence" ;
                 skos:definition "A sequence of composite pulses designed to remove signal splitting due to heteronuclear J-couplings in multinuclear liquid NMR experiments. Also used to allow transfer of magnetization between nuclei (by making the spins precess with at the same chemical shift and thus enjoy strong coupling - isotropic mixing). For the pulse sequence see J. Magn. Reson., (1981), 43, pg 502. [CHMO]" ;
                 skos:prefLabel "Malcolm Levitt pulse sequence" .


###  http://purl.allotrope.org/ontologies/process#AFP_0000318
af-p:AFP_0000318 rdf:type owl:Class ;
                 rdfs:subClassOf af-p:AFP_0000759 ;
                 skos:altLabel "QCPMG experiment" ;
                 skos:definition "An NMR experiment used to measure spin-spin (T2) relaxation times of quadropolar nucei by acquiring multiple spin echos with the intensity decay of the echos proportional to T2. In the solid state, this is also used to enhance sensitivity of low gyromagnetic ratio nuclei by collapsing the intensity of the 'full' spectrum into discrete 'spikelets'/peaks. The intensities of the peaks vary according to T2 and the envelope described by these peaks represents the full, static spectrum. [CHMO]" ;
                 skos:prefLabel "quadrupole Carr-Purcell-Meiboom-Gill experiment" .


###  http://purl.allotrope.org/ontologies/process#AFP_0000325
af-p:AFP_0000325 rdf:type owl:Class ;
                 rdfs:subClassOf af-p:AFP_0002044 ;
                 skos:altLabel "backbone assignment experiment" ,
                               "triple resonance NMR" ,
                               "triple resonance NMR spectroscopy" ,
                               "triple resonance nuclear magnetic resonance spectroscopy" ,
                               "triple resonance nuclear magnetic spectroscopy" ,
                               "triple resonance spectroscopy" ,
                               "triple-resonance NMR" ,
                               "triple-resonance spectroscopy" ;
                 skos:definition "A type of NMR experiment in which excitation of the spin states of three different types of nuclei (1H, 13C and 15N) is employed. [CHMO]" ;
                 skos:prefLabel "triple-resonance spectroscopy" .


###  http://purl.allotrope.org/ontologies/process#AFP_0000335
af-p:AFP_0000335 rdf:type owl:Class ;
                 rdfs:subClassOf af-p:AFP_0001888 ;
                 skos:altLabel "HEHAHA" ,
                               "HEHAHA pulse sequence" ,
                               "HEHAHA sequence" ,
                               "heteronuclear Hartman-Hahn pulse sequence" ,
                               "heteronuclear Hartman-Hahn sequence" ,
                               "heteronuclear Hartmann Hahn" ;
                 skos:definition "An NMR pulse sequence used to transfer magnetization between protons and covalently bound (spin active) heteronuclei via isotropic mixing of their magnetization. Used to e.g. enhance the NMR signal of heteronuclei or to correlate chemical shifts of protons with heteronuclei. For the pulse sequence see J. Magn. Reson., (1991), 91, pg 444. [CHMO]" ;
                 skos:prefLabel "heteronuclear Hartmann Hahn pulse sequence" .


###  http://purl.allotrope.org/ontologies/process#AFP_0000338
af-p:AFP_0000338 rdf:type owl:Class ;
                 rdfs:subClassOf af-p:AFP_0000906 ;
                 skos:altLabel "BLEW" ,
                               "BLEW pulse sequence" ,
                               "BLEW sequence" ,
                               "Burum-Linder-Ernst windowless pulse sequence" ,
                               "Burum-Linder-Ernst windowless sequence" ;
                 skos:definition "A sequence of pulses used in magic angle spinning NMR to remove the effect of homonuclear dipolar couplings. A train/sequence of pulses is used to cyclically manipulate the signal whilst stroboscopic sampling ensures the effects of coupling are unobserved. For the pulse sequence see J. Magn. Reson., (1981), 44, pg 173. [CHMO]" ;
                 skos:prefLabel "Burum, Linder, Ernst windowless pulse sequence" .


###  http://purl.allotrope.org/ontologies/process#AFP_0000348
af-p:AFP_0000348 rdf:type owl:Class ;
                 rdfs:subClassOf af-p:AFP_0000759 ;
                 skos:altLabel "X half-filter" ;
                 skos:definition "A technique used in 2D NMR of isotopically enriched samples (usually 13C/15N) to remove signals of protons which are not bound to a particular isotope from one of the two domains of the experiment. For the technique see J. Magn. Reson., (1986), 70, pg 500. [CHMO]" ;
                 skos:prefLabel "X half filter" .


###  http://purl.allotrope.org/ontologies/process#AFP_0000349
af-p:AFP_0000349 rdf:type owl:Class ;
                 rdfs:subClassOf af-p:AFP_0000833 ;
                 skos:altLabel "WATERGATE" ,
                               "WATERGATE pulse sequence" ,
                               "WATERGATE sequence" ;
                 skos:definition "A pulse cluster used for solvent (water) suppression. The solvent resonances are selectively excited and pulsed field gradients used to destroy the signal. For the pulse sequence see J. Biomol. NMR, (1992), 2, pg 661. [CHMO]" ;
                 skos:prefLabel "water suppression through gradient tailored excitation" .


###  http://purl.allotrope.org/ontologies/process#AFP_0000363
af-p:AFP_0000363 rdf:type owl:Class ;
                 rdfs:subClassOf af-p:AFP_0000325 ;
                 skos:altLabel "HCANNH experiment" ;
                 skos:definition "A triple-resonance NMR experiment used to determine the chemical shifts of nuclei in a (isotopically enriched) protein. The chemical shift of the (backbone) amide proton is correlated with the chemical shift of the covalently bound nitrogen and with the alpha-carbon and proton of the same residue. The experiment name describes the path taken by the magnetization during the experiment. [CHMO]" ;
                 skos:prefLabel "HCANNH" .


###  http://purl.allotrope.org/ontologies/process#AFP_0000367
af-p:AFP_0000367 rdf:type owl:Class ;
                 rdfs:subClassOf af-p:AFP_0000326 ;
                 skos:altLabel "gas phase NMR" ,
                               "gas phase nuclear magnetic resonance spectroscopy" ,
                               "gas-phase nuclear magnetic resonance spectroscopy" ;
                 skos:definition "A type of spectroscopy in the gas phase where the energy states of spin-active nuclei placed in a static magnetic field are interrogated by inducing transitions between the states via radio frequency irradiation. [CHMO]" ;
                 skos:prefLabel "gas-phase nuclear magnetic resonance spectroscopy" .


###  http://purl.allotrope.org/ontologies/process#AFP_0000400
af-p:AFP_0000400 rdf:type owl:Class ;
                 rdfs:subClassOf af-p:AFP_0002044 ;
                 skos:altLabel "4D NMR" ,
                               "4D-NMR" ,
                               "four-dimensional NMR" ;
                 skos:definition "Any type of nuclear magnetic resonance spectroscopy in which four independent frequency dimensions are employed for the correlation and dispersal of signals (by employing three magnetization transfer steps). Each signal is described by four frequencies, thus effecting the distribution of signals within an axis of cubes. [CHMO]" ;
                 skos:prefLabel "four-dimensional nuclear magnetic resonance spectroscopy" .


###  http://purl.allotrope.org/ontologies/process#AFP_0000408
af-p:AFP_0000408 rdf:type owl:Class ;
                 rdfs:subClassOf af-p:AFP_0000759 ;
                 skos:altLabel "MQF" ;
                 skos:definition "An NMR technique used to edit the NMR response from a sample by selecting particular spin systems of interest according to the number of nuclei present within them. Usually achieved by appropriate cycling of the phase (direction of application) of the pulses in an experiment and of the receiver. [CHMO]" ;
                 skos:prefLabel "multiple quantum filter" .


###  http://purl.allotrope.org/ontologies/process#AFP_0000412
af-p:AFP_0000412 rdf:type owl:Class ;
                 rdfs:subClassOf af-p:AFP_0002041 ;
                 skos:altLabel "HR MAS" ,
                               "HR-MAS" ,
                               "HR-MAS NMR spectroscopy" ,
                               "HR/MAS" ,
                               "HRMAS" ,
                               "HRMAS NMR spectroscopy" ,
                               "high resolution magic-angle spinning" ;
                 skos:definition "A type of NMR spectroscopy using a solid sample and a high resolution magnetic susceptibility matching probe. Anisotropic interactions between nuclei, which are usually averaged by Brownian motion in liquid samples, cause significant line broadening in solid state NMR, but can be averaged to zero by spinning the sample very rapidly at the magic angle (54.74 deg. with respect to the direction of the magnetic field). [CHMO]" ;
                 skos:prefLabel "high-resolution magic angle spinning" .


###  http://purl.allotrope.org/ontologies/process#AFP_0000414
af-p:AFP_0000414 rdf:type owl:Class ;
                 rdfs:subClassOf af-p:AFP_0001874 ;
                 skos:altLabel "3D HSQC-TOCSY" ,
                               "3D TOCSY-HSQC" ,
                               "HSQC-TOCSY" ,
                               "TOCSY-HSQC" ;
                 skos:definition "A type of heteronuclear three-dimensional NMR experiment in which the proton signals of a 2D TOCSY spectrum are dispersed along a third frequency axis according to the chemical shift of their covalently bound heteronuclei. [CHMO]" ;
                 skos:prefLabel "heteronuclear single quantum coherence total correlation spectroscopy" .


###  http://purl.allotrope.org/ontologies/process#AFP_0000417
af-p:AFP_0000417 rdf:type owl:Class ;
                 rdfs:subClassOf af-p:AFP_0000325 ;
                 skos:altLabel "HNCAHA experiment" ;
                 skos:definition "A triple-resonance NMR experiment used to determine the chemical shifts of nuclei in a (isotopically enriched) protein. The chemical shift of the (backbone) amide proton is correlated with the chemical shift of the covalently bound nitrogen and the alpha-carbon and proton of the same residue. The experiment name describes the path taken by the magnetization during the experiment. [CHMO]" ;
                 skos:prefLabel "HNCAHA" .


###  http://purl.allotrope.org/ontologies/process#AFP_0000430
af-p:AFP_0000430 rdf:type owl:Class ;
                 rdfs:subClassOf af-p:AFP_0000943 ;
                 skos:altLabel "FSLG-CP" ,
                               "frequency switched Lee-Goldberg cross polarization" ;
                 skos:definition "A magic angle spinning NMR dipolar recoupling technique used to determine dipolar couplings between 1H and 13C nuclei. A FSLG sequence is used to remove homonuclear couplings (by spin-locking the 1H nuclei) and polarization transfer from the protons to the 13C via dipolar coupling manifests as a splitting of the detected 13C signal. [CHMO]" ;
                 skos:prefLabel "frequency-switched Lee-Goldberg cross polarization" .


###  http://purl.allotrope.org/ontologies/process#AFP_0000452
af-p:AFP_0000452 rdf:type owl:Class ;
                 rdfs:subClassOf af-p:AFP_0001888 ;
                 skos:definition "An NMR pulse sequence that decouples nuclei i.e. removes the effects of dipolar coupling or J-coupling from the spectrum. [CHMO]" ;
                 skos:prefLabel "decoupling pulse sequence" .


###  http://purl.allotrope.org/ontologies/process#AFP_0000465
af-p:AFP_0000465 rdf:type owl:Class ;
                 rdfs:subClassOf af-p:AFP_0000759 ;
                 skos:changeNote "2024-09-11 Replaced unlicensed definition with an Allotrope written one." ;
                 skos:definition "Water suppression is a nuclear magnetic resonance assay used to suppress the signal from water. [Allotrope]" ;
                 skos:prefLabel "water suppression" .


###  http://purl.allotrope.org/ontologies/process#AFP_0000467
af-p:AFP_0000467 rdf:type owl:Class ;
                 rdfs:subClassOf af-p:AFP_0002041 ;
                 skos:altLabel "STMAS" ,
                               "satellite-transition MAS" ,
                               "satellite-transition magic angle spinning" ,
                               "satellite-transition magic-angle spinning" ;
                 skos:definition "An NMR experiment where the selective excitation of central and satellite transitions during magic angle spinning is used for recording high-resolution NMR spectra of quadrupolar nuclei in solids. Central transitions are detected first, followed by satellite transitions. [CHMO]" ;
                 skos:prefLabel "satellite transition magic angle spinning" .


###  http://purl.allotrope.org/ontologies/process#AFP_0000473
af-p:AFP_0000473 rdf:type owl:Class ;
                 rdfs:subClassOf af-p:AFP_0002384 ;
                 skos:altLabel "3D COSY-DOSY" ,
                               "3D DOSY-COSY" ,
                               "COSY-DOSY" ,
                               "DOSY-COSY" ,
                               "correlation spectroscopy-diffusion-ordered spectroscopy" ;
                 skos:definition "A type of three-dimensional NMR experiment in which the signals of a 2D COSY spectrum are dispersed along a third frequency axis according to diffusion coefficient. [CHMO]" ;
                 skos:prefLabel "diffusion-ordered spectroscopy-correlation spectroscopy" .


###  http://purl.allotrope.org/ontologies/process#AFP_0000478
af-p:AFP_0000478 rdf:type owl:Class ;
                 rdfs:subClassOf af-p:AFP_0000906 ;
                 skos:altLabel "MREV" ,
                               "MREV pulse sequence" ,
                               "MREV sequence" ,
                               "Mansfield Rhim Elleman Vaughn sequence" ,
                               "Mansfield, Rhim, Elleman, Vaughn sequence" ,
                               "Mansfield-Rhim-Elleman-Vaughn pulse sequence" ,
                               "Mansfield-Rhim-Elleman-Vaughn sequence" ;
                 skos:definition "A pulse sequence used in magic angle spinning NMR to remove the effects of homonuclear dipolar coupling. For the pulse sequence see J. Chem. Phys., (1973), 59, pg 3740. [CHMO]" ;
                 skos:prefLabel "Mansfield, Rhim, Elleman, Vaughn pulse sequence" .


###  http://purl.allotrope.org/ontologies/process#AFP_0000495
af-p:AFP_0000495 rdf:type owl:Class ;
                 rdfs:subClassOf af-p:AFP_0001446 ;
                 skos:altLabel "OPSY-COSY" ;
                 skos:definition "A type of homonuclear NMR spectroscopy where a second frequency dimension is employed to disperse the signals and reveal correlations between nuclei which are J-coupled (usually <= 3 bonds apart). Thermal signals in the resulting spectra are then removed, whilst keeping the signals from para-hydrogen-derived protons intact. [CHMO]" ;
                 skos:prefLabel "only para-hydrogen spectroscopy correlation spectroscopy" .


###  http://purl.allotrope.org/ontologies/process#AFP_0000522
af-p:AFP_0000522 rdf:type owl:Class ;
                 rdfs:subClassOf af-p:AFP_0002044 ;
                 skos:altLabel "PFG-NMR" ;
                 skos:definition "A type of NMR spectroscopy where a spatially inhomogeneous magnetic field with a defined gradient is used, either to select a particular signal or to render unwanted signals undetectable. [CHMO]" ;
                 skos:prefLabel "pulsed-field gradient nuclear magnetic spectroscopy" .


###  http://purl.allotrope.org/ontologies/process#AFP_0000552
af-p:AFP_0000552 rdf:type owl:Class ;
                 rdfs:subClassOf af-p:AFP_0002044 ;
                 skos:altLabel "high field NMR" ,
                               "high-field NMR" ;
                 skos:definition "A type of spectroscopy where the energy states of spin-active nuclei placed in a static (>300 MHz) magnetic field are interrogated by inducing transitions between the states via radio frequency irradiation. Each experiment consists of a sequence of radio frequency pulses with delay periods in between them. [CHMO]" ;
                 skos:prefLabel "high-field nuclear magnetic resonance spectroscopy" .


###  http://purl.allotrope.org/ontologies/process#AFP_0000557
af-p:AFP_0000557 rdf:type owl:Class ;
                 rdfs:subClassOf af-p:AFP_0001230 ;
                 skos:altLabel "3D NOESY-COSY" ,
                               "3D-NOESY-COSY" ,
                               "NOESY-COSY" ;
                 skos:definition "A type of homonuclear three-dimensional NMR experiment in which correlations are seen between nuclei that are spatially proximate within a molecule (<= 6 Angstrom apart). These signals are then correlated with those protons to which they are J-coupled (usually <= 3 bonds apart). [CHMO]" ;
                 skos:prefLabel "nuclear Overhauser enhancement spectroscopy-correlation spectroscopy" .


###  http://purl.allotrope.org/ontologies/process#AFP_0000562
af-p:AFP_0000562 rdf:type owl:Class ;
                 rdfs:subClassOf af-p:AFP_0000743 ;
                 skos:definition "Truncation of the FID recorded either by insufficient acquisition time or by post acquisition processing. [Allotrope]" ;
                 skos:prefLabel "FID truncation" .


###  http://purl.allotrope.org/ontologies/process#AFP_0000576
af-p:AFP_0000576 rdf:type owl:Class ;
                 rdfs:subClassOf af-p:AFP_0002455 ;
                 skos:definition "The application of a Phase Correction algorithm to a Fourier transform NMR spectra such that it is optimised to accommodate for the frequency independent time delay between excitation (the RF pulse) and relaxation (acquiring the FID) to give maximum values of the FID Fourier Transform complex number set. [Allotrope]" ;
                 skos:prefLabel "first order phase correction" .


###  http://purl.allotrope.org/ontologies/process#AFP_0000581
af-p:AFP_0000581 rdf:type owl:Class ;
                 rdfs:subClassOf af-p:AFP_0001277 ;
                 skos:altLabel "DQF-COSY" ,
                               "double quantum filtered COSY" ,
                               "double quantum filtered correlation spectroscopy" ,
                               "double-quantum-filtered COSY" ;
                 skos:definition "A type of homonuclear NMR spectroscopy where a second frequency dimension is employed to disperse the signals and reveal correlations between nuclei which are J-coupled (usually <= 3 bonds apart). The response is edited by selecting only two-spin coupled systems, usually achieved by appropriate cycling of the phase (direction of application) of the pulses in the experiment. [CHMO]" ;
                 skos:prefLabel "double-quantum-filtered correlation spectroscopy" .


###  http://purl.allotrope.org/ontologies/process#AFP_0000584
af-p:AFP_0000584 rdf:type owl:Class ;
                 rdfs:subClassOf af-p:AFP_0002455 ;
                 skos:definition "The application of a mathematical operation to both the real and imaginary parts of the complex numbers represented by the FID recorded as the sample magnetisation vector relaxes from its excited state vector back to its equilibrium bulk magnetisation population as adjusted by the user set values. [Allotrope]" ;
                 skos:prefLabel "manual phase correction" .


###  http://purl.allotrope.org/ontologies/process#AFP_0000607
af-p:AFP_0000607 rdf:type owl:Class ;
                 rdfs:subClassOf af-p:AFP_0000325 ;
                 skos:altLabel "HNCO" ,
                               "HNCO experiment" ;
                 skos:definition "A triple-resonance NMR experiment used in to determine the chemical shifts of nuclei in a (isotopically enriched) protein. The chemical shift of the (backbone) amide proton is correlated with the chemical shift of the covalently bound nitrogen and the carbonyl carbon of the preceding residue. [CHMO]" ;
                 skos:prefLabel "HNCO" .


###  http://purl.allotrope.org/ontologies/process#AFP_0000628
af-p:AFP_0000628 rdf:type owl:Class ;
                 rdfs:subClassOf af-p:AFP_0001888 ;
                 skos:altLabel "DANTE" ,
                               "DANTE pulse sequence" ,
                               "DANTE sequence" ;
                 skos:changeNote "2024-09-11 Removed [Amgen] attribution as this is purely a [CHMO] term." ;
                 skos:definition "A pulse sequence used to selectively excite a frequency range by applying a series of very short pulses to manipulate, or nutate, the magnetization vectors of the desired spins, interspersed with delays which cause the off-resonance magnetisation not to be excited. For the pulse see J. Magn. Reson., (1978), 29, pg 433. [CHMO]" ;
                 skos:prefLabel "delays alternating with nutation for tailored excitation" .


###  http://purl.allotrope.org/ontologies/process#AFP_0000651
af-p:AFP_0000651 rdf:type owl:Class ;
                 rdfs:subClassOf af-p:AFP_0001332 ;
                 skos:altLabel "2D HSQC-NOESY" ,
                               "2D NOESY-HSQC" ,
                               "two-dimensional heteronuclear single quantum coherence nuclear Overhauser effect spectroscopy" ;
                 skos:definition "A 2D NMR experiment which correlates the chemical shifts of spatially proximate protons with the chemical shifts of all (of one type of) their covalently bound heteronuclei. [CHMO]" ;
                 skos:prefLabel "two-dimensional heteronuclear single quantum coherence-nuclear Overhauser effect spectroscopy" .


###  http://purl.allotrope.org/ontologies/process#AFP_0000656
af-p:AFP_0000656 rdf:type owl:Class ;
                 rdfs:subClassOf af-p:AFP_0000759 ;
                 skos:definition "An NMR experiment which measures the variation in amplitude of signals from dipolar-coupled nuclei over time, yielding information about the number of coupled nuclei in the system. [CHMO]" ;
                 skos:prefLabel "spin counting experiment" .


###  http://purl.allotrope.org/ontologies/process#AFP_0000657
af-p:AFP_0000657 rdf:type owl:Class ;
                 rdfs:subClassOf af-p:AFP_0001060 ;
                 skos:altLabel "2D NOESY" ,
                               "2D NOESY NMR" ,
                               "2D homonuclear NOESY " ,
                               "2D nOesy" ,
                               "2D nuclear Overhauser enhancement spectroscopy" ,
                               "2D-NOESY" ,
                               "2D-nOesy" ;
                 skos:definition "A type of homonuclear NMR spectroscopy where a second frequency dimension is employed, based on the nuclear Overhauser enhancement effect in which correlations are seen between nuclei that are spatially proximate within a molecule (<=6  Angstrom apart). [CHMO]" ;
                 skos:prefLabel "two-dimensional nuclear Overhauser enhancement spectroscopy" .


###  http://purl.allotrope.org/ontologies/process#AFP_0000681
af-p:AFP_0000681 rdf:type owl:Class ;
                 rdfs:subClassOf af-p:AFP_0000759 ;
                 dct:source "https://en.wikipedia.org/wiki/Nuclear_magnetic_resonance_decoupling" ;
                 skos:altLabel "NMR decoupling" ;
                 skos:changeNote "2024-09-11 Replaced [nmrML] attribution with [Wikipedia] as this is the correct source." ;
                 skos:definition "Nuclear magnetic resonance decoupling (NMR decoupling for short) is a special method used in nuclear magnetic resonance (NMR) spectroscopy where a sample to be analyzed is irradiated at a certain frequency or frequency range to eliminate fully or partially the effect of coupling between certain nuclei. NMR coupling refers to the effect of nuclei on each other in atoms within a couple of bonds distance of each other in molecules. This effect causes NMR signals in a spectrum to be split into multiple peaks which are up to several hertz (or tens or hundreds of hertz) frequency from each other. Decoupling fully or partially eliminates splitting of the signal between the nuclei irradiated and other nuclei such as the nuclei being analyzed in a certain spectrum. NMR spectroscopy and sometimes decoupling can help determine structures of chemical compounds. [Wikipedia]" ;
                 skos:prefLabel "nuclear magnetic resonance decoupling" .


###  http://purl.allotrope.org/ontologies/process#AFP_0000686
af-p:AFP_0000686 rdf:type owl:Class ;
                 rdfs:subClassOf af-p:AFP_0002044 ;
                 skos:altLabel "PHIP NMR" ,
                               "PHIP-NMR" ,
                               "PHIP-enhanced NMR" ,
                               "para-hydrogen induced polarization enhanced NMR spectroscopy" ;
                 skos:definition "A type of spectroscopy where the energy states of protons derived from para-hydrogen (dihydrogen with an antisymmetric nuclear spin arrangement) placed in a static magnetic field are interrogated by inducing transitions between the states via radio frequency irradiation. Each experiment consists of a sequence of radio frequency pulses with delay periods in between them. The non-Boltzmann spin population generated by para-hydrogen-derived protons gives rise to signal enhancement in the spectra, facilitating the detection of species present at low concentration. [CHMO]" ;
                 skos:prefLabel "para-hydrogen induced polarization enhanced nuclear magnetic resonance spectroscopy" .


###  http://purl.allotrope.org/ontologies/process#AFP_0000691
af-p:AFP_0000691 rdf:type owl:Class ;
                 rdfs:subClassOf af-p:AFP_0002041 ;
                 skos:altLabel "MQMAS" ,
                               "MQMAS NMR" ,
                               "multiple-quantum MAS" ,
                               "multiple-quantum excitation in combination with magic-angle spinning" ;
                 skos:definition "An NMR experiment used for half-integer quadrupolar nuclei, involving transitions between non-consecutive energy levels during the excitation of the spin system by multiple-quantum excitation pulses. [CHMO]" ;
                 skos:prefLabel "multiple-quantum excitation in combination with magic angle spinning" .


###  http://purl.allotrope.org/ontologies/process#AFP_0000694
af-p:AFP_0000694 rdf:type owl:Class ;
                 rdfs:subClassOf af-p:AFP_0002044 ;
                 skos:altLabel "DEPT" ,
                               "DEPT NMR" ,
                               "distortionless enhancement by polarization transfer" ;
                 skos:definition "A type of spectroscopy where the energy states of 13C nuclei placed in a static magnetic field are interrogated by inducing transitions between the states via radio frequency irradiation. Each experiment consists of a sequence of radio frequency pulses with delay periods in between them.The 13C NMR signals are enhanced by transferring 1H magnetization to 13C nuclei and the phase of the signals reflects the multiplicity i.e. CH, CH2 or CH3). Separate methyl, methylene and methine spectra may be obtained. [CHMO]" ;
                 skos:prefLabel "distortionless enhancement with polarization transfer" .


###  http://purl.allotrope.org/ontologies/process#AFP_0000715
af-p:AFP_0000715 rdf:type owl:Class ;
                 rdfs:subClassOf af-p:AFP_0001122 ;
                 skos:altLabel "2D Hadamard encoded TOCSY" ,
                               "Hadamard TOCSY" ,
                               "Hadamard-TOCSY" ;
                 skos:definition "A type of homonuclear NMR spectroscopy where a second frequency dimension is employed to disperse the signals and reveal correlations between all nuclei of a spin-system. All of the resonances in the spin system are excited by selecting only one line for excitation and the final spectrum consists of a series of 1D sub-spectra, each representing one spin system. [CHMO]" ;
                 skos:prefLabel "Hadamard-encoded total correlation spectroscopy" .


###  http://purl.allotrope.org/ontologies/process#AFP_0000719
af-p:AFP_0000719 rdf:type owl:Class ;
                 rdfs:subClassOf af-p:AFP_0000467 ;
                 skos:altLabel "I-STMAS" ,
                               "ISTMAS" ,
                               "inverse-STMAS" ;
                 skos:definition "An NMR experiment where the selective excitation of central and satellite transitions during magic angle spinning is used for recording high-resolution NMR spectra of quadrupolar nuclei in solids. Satellite transitions are detected first, followed by central transitions. [CHMO]" ;
                 skos:prefLabel "inverse satellite transition magic angle spinning" .


###  http://purl.allotrope.org/ontologies/process#AFP_0000721
af-p:AFP_0000721 rdf:type owl:Class ;
                 rdfs:subClassOf af-p:AFP_0000452 ;
                 skos:altLabel "CPD" ;
                 skos:definition "An NMR pulse sequence, employing composite pulses, which decouples nuclei i.e. removes the effects of (usually) J-coupling (line splitting) from the spectrum. [CHMO]" ;
                 skos:prefLabel "composite pulse decoupling sequence" .


###  http://purl.allotrope.org/ontologies/process#AFP_0000724
af-p:AFP_0000724 rdf:type owl:Class ;
                 rdfs:subClassOf af-p:AFP_0000759 ;
                 skos:altLabel "VAS" ,
                               "variable-angle spinning " ;
                 skos:definition "A technique used in solid-state NMR experiments to achieve the controlled reintroduction of dipolar couplings by varying the angle at which the sample is spun relative to the applied magnetic field. [CHMO]" ;
                 skos:prefLabel "variable angle spinning" .


###  http://purl.allotrope.org/ontologies/process#AFP_0000731
af-p:AFP_0000731 rdf:type owl:Class ;
                 rdfs:subClassOf af-p:AFP_0000408 ;
                 skos:altLabel "DQF" ;
                 skos:definition "An NMR technique used to edit the NMR response from a sample by selecting only two-spin coupled systems, usually achieved by appropriate cycling of the phase (direction of application) of the pulses in an experiment and of the receiver. [CHMO]" ;
                 skos:prefLabel "double quantum filter" .


###  http://purl.allotrope.org/ontologies/process#AFP_0000742
af-p:AFP_0000742 rdf:type owl:Class ;
                 rdfs:subClassOf af-p:AFP_0002063 ;
                 skos:altLabel "2D SLF" ,
                               "2D SLF NMR" ,
                               "2D separated local field NMR" ,
                               "2D-SLF" ,
                               "2D-SLF NMR" ,
                               "SLF NMR" ,
                               "SLF spectroscopy" ,
                               "separate local field NMR" ,
                               "separate-local-field NMR" ,
                               "separated local field (SLF) NMR" ,
                               "separated local field NMR" ,
                               "separated local field spectroscopy" ,
                               "separated-local field (SLF) NMR" ,
                               "separated-local field NMR" ,
                               "separated-local-field spectroscopy" ;
                 skos:definition "A two-dimensional NMR experiment which exploits the differential dipolar couplings which nuclei exhibit to their neighboring protons within local magnetic fields. The experiment consist of two time intervals: during the first time period the dipolar couplings are encoded in the NMR signal, while in the detection period the signals of different nuclei are separated on the basis of their differences in chemical shift. [CHMO]" ;
                 skos:prefLabel "separated-local-field nuclear magnetic resonance spectroscopy" .


###  http://purl.allotrope.org/ontologies/process#AFP_0000743
af-p:AFP_0000743 rdf:type owl:Class ;
                 rdfs:subClassOf af-p:AFP_0003598 ;
                 skos:definition "Data processing on nuclear magnetic resonance spectroscopy spectra or nuclear magnetic resonance spectroscopy FID. [Allotrope]" ;
                 skos:prefLabel "nuclear magnetic resonance spectroscopy data processing" .


###  http://purl.allotrope.org/ontologies/process#AFP_0000776
af-p:AFP_0000776 rdf:type owl:Class ;
                 rdfs:subClassOf af-p:AFP_0001230 ;
                 skos:altLabel "3D TOCSY-NOESY" ,
                               "3D-TOCSY-NOESY" ,
                               "TOCSY-NOESY" ;
                 skos:definition "A type of homonuclear three-dimensional NMR experiment spectroscopy which reveals correlations between all nuclei of a spin-system. These signals are then correlated to nuclei that are spatially proximate within the molecule (<= 6 Angstrom apart). [CHMO]" ;
                 skos:prefLabel "total correlation spectroscopy-nuclear Overhauser enhancement spectroscopy" .


###  http://purl.allotrope.org/ontologies/process#AFP_0000786
af-p:AFP_0000786 rdf:type owl:Class ;
                 rdfs:subClassOf af-p:AFP_0002056 ;
                 skos:altLabel "CYCLOPS" ;
                 skos:definition "A phase cycle technique used in FT NMR experiments whereby the sense of application (or phase) of the RF pulses is altered on repeating the experiment such that addition of the resulting signals results in increased intensity for the signals of interest and more effective noise reduction. For the technique see Progr. NMR Spectr., (1978), 12, pg 41. [CHMO]" ;
                 skos:prefLabel "cyclically ordered phase sequence" .


###  http://purl.allotrope.org/ontologies/process#AFP_0000788
af-p:AFP_0000788 rdf:type owl:Class ;
                 rdfs:subClassOf af-p:AFP_0002384 ;
                 skos:altLabel "3D DOSY-TOCSY" ,
                               "3D TOCSY-DOSY" ,
                               "DOSY-TOCSY" ,
                               "TOCSY-DOSY" ,
                               "total correlation spectroscopy-diffusion-ordered spectroscopy" ;
                 skos:definition "A type of three-dimensional NMR experiment in which the signals of a 2D TOCSY spectrum are dispersed along a third frequency axis according to diffusion coefficient. [CHMO]" ;
                 skos:prefLabel "diffusion-ordered spectroscopy-total correlation spectroscopy" .


###  http://purl.allotrope.org/ontologies/process#AFP_0000790
af-p:AFP_0000790 rdf:type owl:Class ;
                 rdfs:subClassOf af-p:AFP_0002044 ;
                 skos:altLabel "TROSY" ,
                               "TROSY NMR" ,
                               "transverse relaxation optimized spectroscopy " ;
                 skos:definition "A type of NMR experiment employed for protein samples in which relaxation mechanisms are optimised in order to suppress transverse relaxation times (T2) and deliver only the sharpest signal present in a multiplet. [CHMO]" ;
                 skos:prefLabel "transverse relaxation optimised spectroscopy" .


###  http://purl.allotrope.org/ontologies/process#AFP_0000826
af-p:AFP_0000826 rdf:type owl:Class ;
                 rdfs:subClassOf af-p:AFP_0001874 ;
                 skos:altLabel "3D HSQC-NOESY" ;
                 skos:definition "A 3D NMR experiment in which the chemical shifts of protons are correlated with the chemical shifts their covalently-bound heteronuclei and with the shifts of spatially proximate protons (<6 Angstrom). [CHMO]" ;
                 skos:prefLabel "heteronuclear single quantum coherence-nuclear Overhauser spectroscopy" .


###  http://purl.allotrope.org/ontologies/process#AFP_0000830
af-p:AFP_0000830 rdf:type owl:Class ;
                 rdfs:subClassOf af-p:AFP_0002044 ;
                 skos:altLabel "VT NMR" ,
                               "VT-NMR" ,
                               "variable temperature NMR" ,
                               "variable temperature nuclear magnetic resonance spectroscopy" ,
                               "variable-temperature NMR" ;
                 skos:definition "A type of spectroscopy where the response of a nucleus with non-zero spin to a perturbing magnetic field is detected at temperatures above or below the ambient probe temperature. Each experiment consists of a sequence of radio frequency pulses with delay periods in between them. [CHMO]" ;
                 skos:prefLabel "variable-temperature nuclear magnetic resonance spectroscopy" .


###  http://purl.allotrope.org/ontologies/process#AFP_0000833
af-p:AFP_0000833 rdf:type owl:Class ;
                 rdfs:subClassOf af-p:AFP_0001888 ;
                 skos:definition "An NMR pulse sequence that is used to suppress or remove the solvent signal. [CHMO]" ;
                 skos:prefLabel "solvent suppression pulse sequence" .


###  http://purl.allotrope.org/ontologies/process#AFP_0000865
af-p:AFP_0000865 rdf:type owl:Class ;
                 rdfs:subClassOf af-p:AFP_0000325 ;
                 skos:altLabel "4D HCCH-TOCSY" ;
                 skos:definition "A 4D triple-resonance NMR experiment used to determine the chemical shifts of nuclei in a (isotopically enriched) protein. The chemical shifts of the protons of a sidechain are correlated with their covalently bound 13C nuclei and with the other protons of the side-chain. [CHMO]" ;
                 skos:prefLabel "four-dimensional HCCH-total correlation spectroscopy" .


###  http://purl.allotrope.org/ontologies/process#AFP_0000875
af-p:AFP_0000875 rdf:type owl:Class ;
                 rdfs:subClassOf af-p:AFP_0001888 ;
                 skos:altLabel "CPMG" ,
                               "CPMG pulse sequence" ,
                               "CPMG sequence" ,
                               "Carr, Purcell,Meiboom,Gill pulse sequence" ,
                               "Carr-Purcell Meiboom-Gill pulse sequence" ,
                               "Carr-Purcell-Meiboom-Gill pulse sequence" ;
                 skos:definition "A pulse sequence which is applied during nuclear magnetic resonance spectroscopy to measure spin-spin (T2) relaxation times. For the pulse sequence see Rev. Sci. Inst., (1958), 29, pg 688. [CHMO]" ;
                 skos:prefLabel "Carr-Purcell-Meiboom-Gill pulse sequence" .


###  http://purl.allotrope.org/ontologies/process#AFP_0000879
af-p:AFP_0000879 rdf:type owl:Class ;
                 rdfs:subClassOf af-p:AFP_0000326 ;
                 skos:altLabel "NMR absorption spectroscopy" ,
                               "c.w. NMR" ,
                               "continuous wave nuclear magnetic resonance spectrometry" ,
                               "continuous wave nuclear magnetic resonance spectroscopy" ,
                               "cw-NMR" ;
                 skos:definition "A type of spectroscopy where the energy states of spin-active nuclei placed in a static magnetic field are interrogated by inducing transitions between the states via radio frequency irradiation. Spectra are obtained by scanning a range of radio frequencies. [CHMO]" ;
                 skos:prefLabel "continuous-wave nuclear magnetic resonance spectroscopy" .


###  http://purl.allotrope.org/ontologies/process#AFP_0000886
af-p:AFP_0000886 rdf:type owl:Class ;
                 rdfs:subClassOf af-p:AFP_0000691 ;
                 skos:altLabel "5QMAS" ,
                               "5QMAS NMR" ,
                               "five-quantum MAS" ,
                               "five-quantum excitation in combination with magic-angle spinning" ;
                 skos:definition "An NMR experiment used for 5/2-spin quadrupolar nuclei, involving transitions between non-consecutive energy levels during the excitation of the spin system by the first RF pulse. [CHMO]" ;
                 skos:prefLabel "five-quantum excitation in combination with magic angle spinning" .


###  http://purl.allotrope.org/ontologies/process#AFP_0000906
af-p:AFP_0000906 rdf:type owl:Class ;
                 rdfs:subClassOf af-p:AFP_0000452 ;
                 skos:definition "An NMR pulse sequence, used in magic angle spinning, that decouples nuclei i.e. removes the effects of (usually) J-coupling (line splitting) from the spectrum. [CHMO]" ;
                 skos:prefLabel "magic angle spinning decoupling pulse sequence" .


###  http://purl.allotrope.org/ontologies/process#AFP_0000910
af-p:AFP_0000910 rdf:type owl:Class ;
                 rdfs:subClassOf af-p:AFP_0001122 ;
                 skos:altLabel "IR-TOCSY" ,
                               "inversion recovery TOCSY" ,
                               "inversion-recovery TOCSY" ;
                 skos:definition "A two-dimensional NMR experiment which shows correlations between all the nuclei of a spin system and also allows determination of T1 relaxation rates. [CHMO]" ;
                 skos:prefLabel "inversion recovery total correlation spectroscopy" .


###  http://purl.allotrope.org/ontologies/process#AFP_0000926
af-p:AFP_0000926 rdf:type owl:Class ;
                 rdfs:subClassOf af-p:AFP_0000759 ;
                 skos:altLabel "PFG" ,
                               "ge-NMR" ,
                               "gradient NMR" ,
                               "gradient-enhanced NMR" ,
                               "gradient-selected NMR" ,
                               "gs-NMR" ,
                               "pulsed-field gradient" ;
                 skos:definition "A tool employed in NMR experiments; spatially inhomogeneous magnetic fields applied with a defined gradient. Used to either select a particular signal or to render unwanted signals undetectable. [CHMO]" ;
                 skos:prefLabel "pulsed field gradient" .


###  http://purl.allotrope.org/ontologies/process#AFP_0000943
af-p:AFP_0000943 rdf:type owl:Class ;
                 rdfs:subClassOf af-p:AFP_0002041 ;
                 skos:altLabel "PISEMA" ,
                               "dipolar recoupling distance experiment" ,
                               "dipolar recoupling experiment" ;
                 skos:definition "Magic angle spinning NMR experiments in which dipolar coupling is reintroduced to obtain information on the proximity of nuclei within the sample. [CHMO]" ;
                 skos:prefLabel "polarization inversion and spin exchange at the magic angle" .


###  http://purl.allotrope.org/ontologies/process#AFP_0000951
af-p:AFP_0000951 rdf:type owl:Class ;
                 rdfs:subClassOf af-p:AFP_0002041 ;
                 skos:altLabel "CP-MAS" ,
                               "CP-MAS NMR" ,
                               "CP/MAS" ,
                               "CP/MAS NMR" ,
                               "CPMAS" ,
                               "CPMAS NMR" ,
                               "cross polarization magic angle spinning" ,
                               "cross polarization magic angle spinning nuclear magnetic resonance spectroscopy" ,
                               "cross-polarization magic angle spinning nuclear magnetic resonance spectroscopy" ;
                 skos:definition "A type of NMR spectroscopy using a solid sample. Anisotropic interactions between nuclei, which are usually averaged by Brownian motion in liquid samples, cause significant line broadening in solid state NMR, but can be reduced to zero by spinning the sample very rapidly at the magic angle (54.74 deg. with respect to the direction of the magnetic field). Cross polarization is used to enhance the signal from weakly coupled nuclei. [CHMO]" ;
                 skos:prefLabel "cross-polarization magic angle spinning" .


###  http://purl.allotrope.org/ontologies/process#AFP_0000965
af-p:AFP_0000965 rdf:type owl:Class ;
                 rdfs:subClassOf af-p:AFP_0000691 ;
                 skos:altLabel "3QMAS" ,
                               "3QMAS NMR" ,
                               "TQMAS" ,
                               "TQMAS-NMR" ,
                               "triple-quantum MAS" ,
                               "triple-quantum excitation in combination with magic-angle spinning" ;
                 skos:definition "An NMR experiment used for 3/2-spin quadrupolar nuclei, involving transitions between non-consecutive energy levels during the excitation of the spin system by triple-quantum excitation pulses. [CHMO]" ;
                 skos:prefLabel "triple-quantum excitation in combination with magic angle spinning" .


###  http://purl.allotrope.org/ontologies/process#AFP_0000971
af-p:AFP_0000971 rdf:type owl:Class ;
                 rdfs:subClassOf af-p:AFP_0002063 ;
                 skos:altLabel "2D INADEQUATE" ,
                               "2D INADEQUATE NMR" ,
                               "INADEQUATE" ,
                               "INADEQUATE NMR" ;
                 skos:definition "A 2D NMR technique which correlates (commonly one-bond) J-coupled homonuclei. In one dimension, the signals appear at the chemical shift of a particular nucleus and in the other dimension, at a position which is the sum of the frequencies of that nucleus and its J-coupled partner. [CHMO]" ;
                 skos:prefLabel "incredible natural abundance double quantum transfer experiment" .


###  http://purl.allotrope.org/ontologies/process#AFP_0000981
af-p:AFP_0000981 rdf:type owl:Class ;
                 rdfs:subClassOf af-p:AFP_0000038 ;
                 skos:altLabel "57Fe ENDOR" ,
                               "57Fe ENDOR spectroscopy" ,
                               "iron-57 ENDOR" ,
                               "iron-57 ENDOR spectroscopy" ;
                 skos:definition "A type of spectroscopy where a microwave frequency pulse is used to saturate the electron resonance transitions in the 57Fe nuclei of a sample, and a radio frequency pulse is used excite a nuclear transition. [CHMO]" ;
                 skos:prefLabel "57Fe electron nuclear double resonance spectroscopy" .


###  http://purl.allotrope.org/ontologies/process#AFP_0000987
af-p:AFP_0000987 rdf:type owl:Class ;
                 rdfs:subClassOf af-p:AFP_0002408 ;
                 skos:altLabel "1D 1H NMR" ,
                               "1D proton NMR" ;
                 skos:changeNote "2024-09-11 Removed [Amgen] attribution as this is a [CHMO] term." ;
                 skos:definition "A type of spectroscopy where the energy states of 1H nuclei placed in a static magnetic field are interrogated by inducing transitions between the states via radio frequency irradiation. Each experiment consists of a sequence of radio frequency pulses with delay periods in between them, and the spectrum is obtained by plotting chemical shift vs. frequency. 1D 1H NMR usually uses one pulse (90 or 30 degree pulse) for excitation. [CHMO]" ;
                 skos:prefLabel "one-dimensional 1H nuclear magnetic resonance spectroscopy" .


###  http://purl.allotrope.org/ontologies/process#AFP_0000993
af-p:AFP_0000993 rdf:type owl:Class ;
                 rdfs:subClassOf af-p:AFP_0002044 ;
                 skos:altLabel "2H decoupled NMR" ,
                               "2H-decoupled NMR" ,
                               "deuterium-decoupled NMR" ,
                               "deuterium-decoupled NMR spectroscopy" ;
                 skos:definition "A type of NMR spectroscopy where (J/scalar) couplings to 2H nuclei are cancelled by applying radio frequency radiation to saturate or otherwise manipulate the 2H spins such that no evolution of the coupling occurs. [CHMO]" ;
                 skos:prefLabel "deuterium-decoupled nuclear magnetic resonance spectroscopy" .


###  http://purl.allotrope.org/ontologies/process#AFP_0001011
af-p:AFP_0001011 rdf:type owl:Class ;
                 rdfs:subClassOf af-p:AFP_0000325 ;
                 skos:altLabel "HCC(CO)NNH experiment" ;
                 skos:definition "A triple-resonance NMR experiment used to determine the chemical shifts of nuclei in a (isotopically enriched) protein. The chemical shift of the (backbone) amide proton is correlated with the chemical shift of the covalently bound nitrogen and with both the alpha- and beta-carbons and protons of the preceding residue. The experiment name describes the path taken by the magnetization during the experiment. [CHMO]" ;
                 skos:prefLabel "HCC(CO)NNH" .


###  http://purl.allotrope.org/ontologies/process#AFP_0001060
af-p:AFP_0001060 rdf:type owl:Class ;
                 rdfs:subClassOf af-p:AFP_0002044 ;
                 skos:altLabel "2D EXSY" ,
                               "2D exchange spectroscopy" ,
                               "EXSY" ,
                               "NOE experiments" ,
                               "NOESY" ,
                               "NOESY NMR" ,
                               "NOEsy" ,
                               "exchange spectrometry" ,
                               "exchange spectroscopy" ,
                               "nOesy" ,
                               "nuclear Overhauser effect spectrometry" ,
                               "nuclear Overhauser effect spectroscopy" ,
                               "nuclear Overhauser enhancement spectrometry" ;
                 skos:definition "A type of homonuclear NMR spectroscopy based on the nuclear Overhauser enhancement effect in which correlations are seen between nuclei that are spatially proximate within a molecule (<= 6 Angstrom apart). [CHMO]" ;
                 skos:prefLabel "nuclear Overhauser enhancement spectroscopy" .


###  http://purl.allotrope.org/ontologies/process#AFP_0001068
af-p:AFP_0001068 rdf:type owl:Class ;
                 rdfs:subClassOf af-p:AFP_0000759 ;
                 skos:altLabel "PRE" ,
                               "paramagnetic relaxation enhancements" ;
                 skos:definition "An NMR technique whereby paramagnetic ions are introduced to a sample which cause enhanced relaxation of the spins in proximity of the paramagnetic spin label, giving long-range (up to 24 Angstrom) structural information. Also used in binding studies, allowing identification of the atoms involved in binding. [CHMO]" ;
                 skos:prefLabel "paramagnetic relaxation enhancement" .


###  http://purl.allotrope.org/ontologies/process#AFP_0001102
af-p:AFP_0001102 rdf:type owl:Class ;
                 rdfs:subClassOf af-p:AFP_0001888 ;
                 skos:altLabel "DPFGSE" ,
                               "DPFGSE excitation" ,
                               "DPFGSE pulse sequence" ,
                               "DPFGSE sequence" ,
                               "double pulsed field gradient spin echo" ,
                               "double pulsed field gradient spin-echo" ,
                               "double pulsed field gradient spin-echo pulse sequence" ;
                 skos:definition "An NMR pulse sequence in which pulsed field gradients are applied to a doubled spin echo sequence to cleanly and precisely excite particular resonances. For the pulse sequence see J. Magn. Reson. A, (1995), 112, pg 275. [CHMO]" ;
                 skos:prefLabel "double pulsed field gradient spin echo pulse sequence" .


###  http://purl.allotrope.org/ontologies/process#AFP_0001122
af-p:AFP_0001122 rdf:type owl:Class ;
                 rdfs:subClassOf af-p:AFP_0002044 ;
                 skos:altLabel "HOHAHA spectrometry" ,
                               "HOHAHA spectroscopy" ,
                               "TOCSY" ,
                               "homonuclear Hartmann Hahn spectroscopy" ,
                               "homonuclear Hartmann,Hahn spectroscopy" ,
                               "homonuclear Hartmann-Hahn spectroscopy" ,
                               "total correlated spectroscopy" ,
                               "total correlation spectrometry" ;
                 skos:definition "A type of homonuclear NMR spectroscopy which reveal correlations between all nuclei of a spin-system. [CHMO]" ;
                 skos:prefLabel "total correlation spectroscopy" .


###  http://purl.allotrope.org/ontologies/process#AFP_0001148
af-p:AFP_0001148 rdf:type owl:Class ;
                 rdfs:subClassOf af-p:AFP_0000657 ;
                 skos:altLabel "fb-NOESY" ,
                               "fb-NOESY NMR" ,
                               "fb-nOesy" ,
                               "flip-back nuclear Overhauser effect spectrometry" ,
                               "flip-back nuclear Overhauser effect spectroscopy" ,
                               "flip-back nuclear Overhauser enhancement spectrometry" ;
                 skos:definition "A type of heteronuclear two-dimensional NMR spectroscopy incorporating a water flip-back sequence, based on the nuclear Overhauser enhancement effect in which correlations are seen between nuclei that are spatially proximate within a molecule (<= 6 Angstrom apart). [CHMO]" ;
                 skos:prefLabel "flip-back nuclear Overhauser enhancement spectroscopy" .


###  http://purl.allotrope.org/ontologies/process#AFP_0001222
af-p:AFP_0001222 rdf:type owl:Class ;
                 rdfs:subClassOf af-p:AFP_0001361 ,
                                 af-p:AFP_0002041 ;
                 skos:altLabel "PDLF with R-type recoupling" ,
                               "R-PDLF" ,
                               "R-type recoupling proton detected local field spectroscopy" ,
                               "proton-deteced separated local field spectroscopy with R-type recoupling" ;
                 skos:definition "A magic-angle spinning NMR experiment to measure dipolar couplings. Dipolar couplings are reintroduced by synchronising RF pulses with the rotation of the rotor. Spectral simplification occurs via the proton detected separated local field protocol where 1H-1H interactions are decoupled and proton magnetization is passed through 13C nuclei present at natural abundance. [CHMO]" ;
                 skos:prefLabel "R-type recoupling proton detected separated local field spectroscopy" .


###  http://purl.allotrope.org/ontologies/process#AFP_0001230
af-p:AFP_0001230 rdf:type owl:Class ;
                 rdfs:subClassOf af-p:AFP_0000308 ;
                 skos:altLabel "homonuclear 3D NMR" ;
                 skos:definition "Any type of nuclear magnetic resonance spectroscopy in which three independent frequency dimensions are employed for the correlation and dispersal of signals. Each signal is described by three frequencies, all arising from the same type of nucleus, thus effecting the distribution of signals within a cube. [CHMO]" ;
                 skos:prefLabel "homonuclear three-dimensional nuclear magnetic resonance spectroscopy" .


###  http://purl.allotrope.org/ontologies/process#AFP_0001233
af-p:AFP_0001233 rdf:type owl:Class ;
                 rdfs:subClassOf af-p:AFP_0001211 ;
                 skos:altLabel "PDMR" .


###  http://purl.allotrope.org/ontologies/process#AFP_0001264
af-p:AFP_0001264 rdf:type owl:Class ;
                 rdfs:subClassOf af-p:AFP_0000833 ;
                 skos:altLabel "WEFT" ,
                               "WEFT pulse sequence" ,
                               "WEFT sequence" ,
                               "water-elimination Fourier transform" ;
                 skos:definition "A pulse cluster used to suppress solvent (water) signals exploiting the differing relaxation properties of solvent and sample. Resonances are inverted and the subsequent recovery period is chosen such that the solvent signal is at a null point when the signal is detected. For the pulse sequence see J. Chem. Phys., (1972), 56, pg 3182. [CHMO]" ;
                 skos:prefLabel "water elimination Fourier transform" .


###  http://purl.allotrope.org/ontologies/process#AFP_0001277
af-p:AFP_0001277 rdf:type owl:Class ;
                 rdfs:subClassOf af-p:AFP_0002063 ;
                 skos:altLabel "COSY" ,
                               "correlated spectrometry" ,
                               "correlated spectroscopy" ,
                               "correlation spectrometry" ;
                 skos:definition "A type of homonuclear NMR spectroscopy where a second frequency dimension is employed to disperse the signals and reveal correlations between nuclei which are J-coupled (usually <= 3 bonds apart). [CHMO]" ;
                 skos:prefLabel "correlation spectroscopy" .


###  http://purl.allotrope.org/ontologies/process#AFP_0001297
af-p:AFP_0001297 rdf:type owl:Class ;
                 rdfs:subClassOf af-p:AFP_0000759 ;
                 skos:altLabel "states-TPPI" ,
                               "states-TPPI acquisition" ;
                 skos:definition "A technique used in multidimensional NMR experiments to achieve frequency discrimination of the signals in the additional dimensions. [CHMO]" ;
                 skos:prefLabel "states-time proportional phase incrementation" .


###  http://purl.allotrope.org/ontologies/process#AFP_0001307
af-p:AFP_0001307 rdf:type owl:Class ;
                 rdfs:subClassOf af-p:AFP_0001964 ;
                 skos:altLabel "band selective decoupling" ,
                               "narrow band decoupling" ,
                               "specific band decoupling" ,
                               "specific decoupling" ;
                 skos:definition "A specified narrow frequency band associated with a specific nuclei of a specified isotope is selectively irradiated with a weak RF pulse. [Allotrope]" ;
                 skos:prefLabel "specific proton decoupling" .


###  http://purl.allotrope.org/ontologies/process#AFP_0001315
af-p:AFP_0001315 rdf:type owl:Class ;
                 rdfs:subClassOf af-p:AFP_0001230 ;
                 skos:altLabel "3D NOESY-TOCSY" ,
                               "3D-NOESY-TOCSY" ,
                               "NOESY-TOCSY" ;
                 skos:definition "A type of homonuclear NMR spectroscopy which reveal correlations between all nuclei of a spin-system. These signals are then correlated to nuclei that are spatially proximate within the molecule (<= 6 Angstrom apart). [CHMO]" ;
                 skos:prefLabel "nuclear Overhauser enhancement spectroscopy-total correlation spectroscopy" .


###  http://purl.allotrope.org/ontologies/process#AFP_0001320
af-p:AFP_0001320 rdf:type owl:Class ;
                 rdfs:subClassOf af-p:AFP_0001060 ;
                 skos:altLabel "1D NOESY" ,
                               "1D nOesy" ,
                               "1D nuclear Overhauser enhancement spectroscopy" ,
                               "1D-NOESY" ,
                               "1D-nOesy" ,
                               "NOESY NMR" ;
                 skos:definition "A type of homonuclear NMR spectroscopy where only one frequency dimension is employed, based on the nuclear Overhauser enhancement effect in which correlations are seen between nuclei that are spatially proximate within a molecule (<=6  Angstrom apart). [CHMO]" ;
                 skos:prefLabel "one-dimensional nuclear Overhauser enhancement spectroscopy" .


###  http://purl.allotrope.org/ontologies/process#AFP_0001325
af-p:AFP_0001325 rdf:type owl:Class ;
                 rdfs:subClassOf af-p:AFP_0000759 ;
                 skos:altLabel "CT experiment" ,
                               "CT method" ,
                               "constant time experiment" ,
                               "constant time method" ;
                 skos:definition "A technique used in 2D NMR whereby the chemical shift frequency modulation of the FIDs necessary to interrogate the second dimension is achieved by moving the position of a RF pulse within a fixed time period on subsequent repeats of the experiment. [CHMO]" ;
                 skos:prefLabel "constant time method" .


###  http://purl.allotrope.org/ontologies/process#AFP_0001329
af-p:AFP_0001329 rdf:type owl:Class ;
                 rdfs:subClassOf af-p:AFP_0001332 ;
                 skos:altLabel "HSQC" ;
                 skos:definition "A type of heteronuclear NMR spectroscopy where a second frequency dimension is employed to disperse the signals and reveal correlations between protons and the nuclei to which they are covalently bound. [CHMO]" ;
                 skos:prefLabel "heteronuclear single quantum coherence" .


###  http://purl.allotrope.org/ontologies/process#AFP_0001332
af-p:AFP_0001332 rdf:type owl:Class ;
                 rdfs:subClassOf af-p:AFP_0002063 ;
                 skos:altLabel "heteronuclear 2D NMR" ;
                 skos:definition "Any type of heteronuclear NMR spectroscopy where a second frequency dimension is employed. [CHMO]" ;
                 skos:prefLabel "heteronuclear two-dimensional nuclear magnetic resonance spectroscopy" .


###  http://purl.allotrope.org/ontologies/process#AFP_0001349
af-p:AFP_0001349 rdf:type owl:Class ;
                 rdfs:subClassOf af-p:AFP_0001211 ;
                 skos:altLabel "FDMR" .


###  http://purl.allotrope.org/ontologies/process#AFP_0001356
af-p:AFP_0001356 rdf:type owl:Class ;
                 rdfs:subClassOf af-p:AFP_0000759 ;
                 skos:altLabel "TPPI" ;
                 skos:definition "A technique used in multidimensional NMR experiments to achieve frequency discrimination of the signals in the additional dimensions. [CHMO]" ;
                 skos:prefLabel "time proportional phase incrementation" .


###  http://purl.allotrope.org/ontologies/process#AFP_0001361
af-p:AFP_0001361 rdf:type owl:Class ;
                 rdfs:subClassOf af-p:AFP_0000742 ;
                 skos:altLabel "PDLF" ,
                               "proton detected local field spectroscopy" ,
                               "proton-detected SLF" ,
                               "proton-detected separated local field spectroscopy" ;
                 skos:definition "An NMR experiment for the measurement of heteronuclear dipolar couplings. 1H-1H interactions are decoupled and proton magnetization is passed through 13C nuclei present at natural abundance to simplify a dipolarly coupled spectrum. [CHMO]" ;
                 skos:prefLabel "proton detected separated local field spectroscopy" .


###  http://purl.allotrope.org/ontologies/process#AFP_0001365
af-p:AFP_0001365 rdf:type owl:Class ;
                 rdfs:subClassOf af-p:AFP_0000759 ;
                 skos:definition "An NMR technique whereby particular resonances are saturated (their spin-state populations are equalised). Commonly used to suppress solvent signals. [CHMO]" ;
                 skos:prefLabel "presaturation" .


###  http://purl.allotrope.org/ontologies/process#AFP_0001378
af-p:AFP_0001378 rdf:type owl:Class ;
                 rdfs:subClassOf af-p:AFP_0001927 ;
                 skos:altLabel "CHIRP" ,
                               "CHIRP pulse" ,
                               "chirp pulse" ;
                 skos:definition "An adiabatic shaped pulse. The resonance frequency is swept through a defined RF range during application of the pulse. Allows excitation of a broader range of frequencies than the size of the RF field. For the pulse see J. Magn. Reson., Ser. A, (1993), 102, pg 293. [CHMO]" ;
                 skos:prefLabel "chirped pulse" .


###  http://purl.allotrope.org/ontologies/process#AFP_0001393
af-p:AFP_0001393 rdf:type owl:Class ;
                 rdfs:subClassOf af-p:AFP_0002041 ;
                 skos:altLabel "REDOR" ,
                               "rotational echo double resonance spectroscopy" ,
                               "rotational echo double-resonance (REDOR) spectroscopy" ;
                 skos:definition "A magic angle spinning NMR experiment in which the evolution of dipolar couplings between nuclei is controlled by applying pulses at appropriate points in the rotational period, allowing the determination of the size of the coupling and, thus, yielding distance information. [CHMO]" ;
                 skos:prefLabel "rotational-echo double-resonance spectroscopy" .


###  http://purl.allotrope.org/ontologies/process#AFP_0001414
af-p:AFP_0001414 rdf:type owl:Class ;
                 rdfs:subClassOf af-p:AFP_0001888 ;
                 skos:altLabel "spin echo sequence" ,
                               "spin-echo pulse sequence" ,
                               "spin-echo sequence" ;
                 skos:definition "A pulse cluster used in NMR experiments which manipulates signals such that, at the end of the sequence, the effects of chemical shift differences have been compensated/removed. Used most simply to compensate for inhomogeneities in the magnetic field but delays in the sequence also permit various possible manipulations of the magnetization. For the pulse sequence see Phys. Rev., (1950), 80, pg 580. [CHMO]" ;
                 skos:prefLabel "spin echo pulse sequence" .


###  http://purl.allotrope.org/ontologies/process#AFP_0001432
af-p:AFP_0001432 rdf:type owl:Class ;
                 rdfs:subClassOf af-p:AFP_0000759 ;
                 skos:altLabel "PASE" ,
                               "PASE NMR" ,
                               "PAramagneticSignalsEnhancement" ,
                               "paramagnetic signals enhancement NMR " ,
                               "paramagneticsignalsenhancement" ;
                 skos:definition "A method for NMR spectra acquisition of paramagnetic proteins, based on the use of homonuclear broadband decoupling of the diamagnetic region. [CHMO]" ;
                 skos:prefLabel "paramagnetic signals enhancement" .


###  http://purl.allotrope.org/ontologies/process#AFP_0001443
af-p:AFP_0001443 rdf:type owl:Class ;
                 rdfs:subClassOf af-p:AFP_0000759 ;
                 skos:definition "An NMR experiment which exploits the increased efficiency of energy (magnetization) transfer between nuclei via dipolar coupling in rigid or semi-rigid samples. The rate at which polarization is transferred between spins is measured giving information on the proximity and orientation of the interacting spins within the sample. [CHMO]" ;
                 skos:prefLabel "spin diffusion experiment" .


###  http://purl.allotrope.org/ontologies/process#AFP_0001446
af-p:AFP_0001446 rdf:type owl:Class ;
                 rdfs:subClassOf af-p:AFP_0000522 ;
                 skos:altLabel "OPSY" ,
                               "OPSY NMR" ;
                 skos:definition "An NMR experiment where pulsed field gradients are used to filter thermal signals from NMR spectra whilst leaving those derived from para-hydrogen-derived protons intact. [CHMO]" ;
                 skos:prefLabel "only para-hydrogen spectroscopy" .


###  http://purl.allotrope.org/ontologies/process#AFP_0001454
af-p:AFP_0001454 rdf:type owl:Class ;
                 rdfs:subClassOf af-p:AFP_0000743 ;
                 skos:definition "Standardizing an NMR spectra setting the reference point to a known value. [Allotrope]" ;
                 skos:example "usually residual solvent protons in 1H NMR spectroscopy for example, or reference inserts e.g. TMS" ;
                 skos:prefLabel "spectral referencing" .


###  http://purl.allotrope.org/ontologies/process#AFP_0001456
af-p:AFP_0001456 rdf:type owl:Class ;
                 rdfs:subClassOf af-p:AFP_0000467 ;
                 skos:altLabel "SCAM-STMAS" ;
                 skos:definition "An NMR experiment where the selective excitation of satellite transitions during magic angle spinning is used for recording high-resolution NMR spectra of quadrupolar nuclei in solids. In conventional magic angle spinning the spinning angle must be very accurate, but this technique can self-compensate  magic-angle errors of up to (+/- 1.0 deg.). [CHMO]" ;
                 skos:prefLabel "satellite transition magic angle spinning with self-compensation for the magic angle misset" .


###  http://purl.allotrope.org/ontologies/process#AFP_0001469
af-p:AFP_0001469 rdf:type owl:Class ;
                 rdfs:subClassOf af-p:AFP_0001888 ;
                 skos:altLabel "TOSS" ,
                               "TOSS pulse sequence" ,
                               "TOSS sequence" ;
                 skos:definition "A pulse sequence used in magic angle spinning NMR experiments to remove additional signals resulting from spinning the sample too slowly to obtain a response composed solely of isotropic chemical shifts. [CHMO]" ;
                 skos:prefLabel "total suppression of sidebands pulse sequence" .


###  http://purl.allotrope.org/ontologies/process#AFP_0001498
af-p:AFP_0001498 rdf:type owl:Class ;
                 rdfs:subClassOf af-p:AFP_0001888 ;
                 skos:altLabel "DOUBTFUL" ,
                               "DOUBTFUL pulse sequence" ,
                               "DOUBTFUL sequence" ;
                 skos:definition "A pulse sequence used to selectively resolve the signals from two coupled nuclei, see J. Am. Chem. Soc., (1982), 104, pg 4286. [CHMO]" ;
                 skos:prefLabel "double quantum transitions for finding unresolved lines" .


###  http://purl.allotrope.org/ontologies/process#AFP_0001525
af-p:AFP_0001525 rdf:type owl:Class ;
                 rdfs:subClassOf af-p:AFP_0001060 ;
                 skos:altLabel "PASE NOESY" ,
                               "PASE-NOE" ,
                               "PASE-NOESY" ;
                 skos:definition "A type of homonuclear NMR spectroscopy based on the nuclear Overhauser enhancement effect in which correlations are seen between nuclei that are spatially proximate within a molecule (<= 6 Angstrom apart). Spectra recorded with suppression of the diamagnetic window by the PASE pulse sequence. [CHMO]" ;
                 skos:prefLabel "nuclear Overhauser enhancement spectroscopy with paramagnetic signals enhancement" .


###  http://purl.allotrope.org/ontologies/process#AFP_0001534
af-p:AFP_0001534 rdf:type owl:Class ;
                 rdfs:subClassOf af-p:AFP_0000127 ;
                 skos:altLabel "PGNE" ,
                               "PGNE NMR" ,
                               "PGNE-NMR" ,
                               "pulsed gradient non-linear echo" ,
                               "pulsed gradient nonlinear echo" ,
                               "pulsed gradient nonlinear spin echo" ;
                 skos:definition "An NMR experiment used to measure small diffusion coefficients via the attenuation of signals occurring due to molecular diffusion during the application of pulsed field gradients. [CHMO]" ;
                 skos:prefLabel "pulsed gradient non-linear spin echo nuclear magnetic resonance spectroscopy" .


###  http://purl.allotrope.org/ontologies/process#AFP_0001544
af-p:AFP_0001544 rdf:type owl:Class ;
                 rdfs:subClassOf af-p:AFP_0001332 ;
                 skos:altLabel "HMQC" ,
                               "HMQC NMR" ;
                 skos:definition "A type of heteronuclear NMR spectroscopy where a second frequency dimension is employed to disperse the signals and reveal correlations between protons and the nuclei to which they are covalently bound. [CHMO]" ;
                 skos:prefLabel "heteronuclear multiple quantum coherence" .


###  http://purl.allotrope.org/ontologies/process#AFP_0001552
af-p:AFP_0001552 rdf:type owl:Class ;
                 rdfs:subClassOf af-p:AFP_0000305 ;
                 skos:altLabel "DOSY" ,
                               "DOSY NMR" ,
                               "diffusion NMR" ,
                               "diffusion ordered NMR spectroscopy" ,
                               "diffusion ordered spectroscopy" ,
                               "diffusion-edited NMR spectroscopy" ,
                               "diffusion-edited spectroscopy" ,
                               "diffusion-ordered NMR spectroscopy" ,
                               "diffusion-ordered nuclear magnetic resonance spectroscopy" ;
                 skos:definition "A type of NMR spectroscopy using pulsed-field gradients where the rate of decay of NMR signals in each component of a sample mixture is measured across a series of experiments. The rate of signal decay is proportional to the diffusion coefficient for each component. [CHMO]" ;
                 skos:prefLabel "diffusion-ordered spectroscopy" .


###  http://purl.allotrope.org/ontologies/process#AFP_0001558
af-p:AFP_0001558 rdf:type owl:Class ;
                 rdfs:subClassOf af-p:AFP_0001888 ;
                 skos:definition "A set of finely tuned RF pulses that achieve the same result with greater precision and fewer imperfections as a result of field inhomogeneity and off-resonance effects than a single RF pulse. [Allotrope]" ;
                 skos:prefLabel "nuclear magnetic resonance composite pulse sequence" .


###  http://purl.allotrope.org/ontologies/process#AFP_0001575
af-p:AFP_0001575 rdf:type owl:Class ;
                 rdfs:subClassOf af-p:AFP_0000325 ;
                 skos:altLabel "HN(CO)CA" ,
                               "HN(CO)CA experiment" ,
                               "HNCOCA" ,
                               "HNCOCA experiment" ;
                 skos:definition "A triple-resonance NMR experiment used to determine the chemical shifts of nuclei in a (isotopically enriched) protein. The chemical shift of the (backbone) amide proton is correlated with the chemical shift of the covalently bound nitrogen and the alpha-carbon of the preceding residue. [CHMO]" ;
                 skos:prefLabel "HNCOCA" .


###  http://purl.allotrope.org/ontologies/process#AFP_0001578
af-p:AFP_0001578 rdf:type owl:Class ;
                 rdfs:subClassOf af-p:AFP_0001320 ;
                 skos:altLabel "1D NOE Difference" ,
                               "1D NOE difference spectroscopy" ,
                               "NOE DIFF" ,
                               "NOE Difference" ,
                               "NOE-DIFF" ,
                               "NOE-Difference" ,
                               "NOE-difference" ,
                               "NOEd" ;
                 skos:definition "A 1D NMR experiment in which a 1D spectrum is subtracted from a spectrum acquired under steady-state NOE conditions. [CHMO]" ;
                 skos:prefLabel "nuclear Overhauser effect difference spectroscopy" .


###  http://purl.allotrope.org/ontologies/process#AFP_0001580
af-p:AFP_0001580 rdf:type owl:Class ;
                 rdfs:subClassOf af-p:AFP_0000721 ;
                 skos:altLabel "WALTZ" ,
                               "WALTZ pulse sequence" ,
                               "WALTZ sequence" ;
                 skos:definition "A sequence of composite pulses designed to remove signal splitting due to heteronuclear J-couplings in multinuclear liquid NMR experiments. Also used to allow transfer of magnetization between nuclei (by making the spins precess with at the same chemical shift and thus enjoy strong coupling - isotropic mixing). J. Magn. Reson., (1983), 52, pg 335. [CHMO]" ;
                 skos:prefLabel "wideband alternating-phase low-power technique for zero residual splitting" .


###  http://purl.allotrope.org/ontologies/process#AFP_0001589
af-p:AFP_0001589 rdf:type owl:Class ;
                 rdfs:subClassOf af-p:AFP_0000721 ;
                 skos:altLabel "SUSAN" ,
                               "SUSAN pulse sequence" ,
                               "SUSAN sequence" ;
                 skos:definition "A sequence of composite pulses designed to remove signal splitting due to heteronuclear J-couplings in multinuclear liquid NMR experiments. For the pulse sequence see J. Magn. Reson. A, (1994), 106, pg 241. [CHMO]" ;
                 skos:prefLabel "spin decoupling employing ultra-broadband-inversion sequences generated via simulated annealing" .


###  http://purl.allotrope.org/ontologies/process#AFP_0001603
af-p:AFP_0001603 rdf:type owl:Class ;
                 rdfs:subClassOf af-p:AFP_0001211 ;
                 skos:altLabel "ZF-ODMR" ,
                               "ZFODMR" ,
                               "Zf-ODMR" ,
                               "zero-field (zf) ODMR" ,
                               "zero-field ODMR" ,
                               "zf-ODMR" ;
                 skos:definition "A double resonance technique in which transitions between spin sublevels at zero applied magnetic field are detected by optical means (i.e. the polarization or the intensity of light emitted or absorbed by the sample depends on the population distribution in the spin levels). Usually these are sublevels of a triplet and the transitions are induced by microwaves. [CHMO]" ;
                 skos:prefLabel "zero-field optically detected magnetic resonance" .


###  http://purl.allotrope.org/ontologies/process#AFP_0001612
af-p:AFP_0001612 rdf:type owl:Class ;
                 rdfs:subClassOf af-p:AFP_0000875 ;
                 skos:altLabel "QCPMG" ,
                               "QCPMG NMR" ,
                               "QCPMG pulse sequence" ,
                               "QCPMG sequence" ,
                               "quadrupolar Carr, Purcell,Meiboom, Gill pulse sequence" ,
                               "quadrupolar Carr-Purcell Meiboom-Gill pulse sequence" ;
                 skos:definition "A pulse sequence which is applied during nuclear magnetic resonance spectroscopy of quadrupolar nuclei, to measure spin-spin (T2) relaxation times. In the solid state, the sequence is used to achieve sensitivity enhancement for nuclei with low gyromagnetic ratios. For the pulse sequence see J. Phys. Chem. A, (1997), 101, pg 8597. [CHMO]" ;
                 skos:prefLabel "quadrupolar Carr-Purcell-Meiboom-Gill pulse sequence" .


###  http://purl.allotrope.org/ontologies/process#AFP_0001630
af-p:AFP_0001630 rdf:type owl:Class ;
                 rdfs:subClassOf af-p:AFP_0000657 ;
                 skos:altLabel "steady state NOESY" ,
                               "steady state nOesy" ,
                               "steady-state NOESY" ,
                               "steady-state nOesy" ,
                               "steady-state nuclear Overhauser enhancement spectrometry" ;
                 skos:changeNote "2024-09-11 Removed [Amgen] attribution as this is purely a [CHMO] term." ;
                 skos:definition "A type of homonuclear NMR spectroscopy where a second frequency dimension is employed, based on the nuclear Overhauser enhancement effect in which correlations are seen between nuclei that are spatially proximate within a molecule (<= 6 Angstrom apart). In this technique, the saturation of a particular proton resonance (signal) perturbs the intensities of signals from spatially proximate nuclei. [CHMO]" ;
                 skos:prefLabel "steady-state nuclear Overhauser enhancement spectroscopy" .


###  http://purl.allotrope.org/ontologies/process#AFP_0001637
af-p:AFP_0001637 rdf:type owl:Class ;
                 rdfs:subClassOf af-p:AFP_0002044 ;
                 skos:altLabel "solution NMR" ,
                               "solution-state NMR" ;
                 skos:definition "A type of spectroscopy where the response of nuclei with non-zero spin, in a sample dissolved in a deuterated solvent,  to a perturbing magnetic field is detected. Each experiment consists of a sequence of radio frequency pulses with delay periods in between them. [CHMO]" ;
                 skos:prefLabel "solution-state nuclear magnetic resonance spectroscopy" .


###  http://purl.allotrope.org/ontologies/process#AFP_0001653
af-p:AFP_0001653 rdf:type owl:Class ;
                 rdfs:subClassOf af-p:AFP_0000721 ;
                 skos:altLabel "DIPSI" ,
                               "DIPSI pulse sequence" ,
                               "DIPSI sequence" ;
                 skos:definition "A sequence of composite pulses designed to remove signal splitting due to heteronuclear J-couplings in multinuclear liquid NMR experiments. Also used to allow transfer of magnetization between nuclei (by making the spins precess with at the same chemical shift and thus enjoy strong coupling - isotropic mixing). For the pulse sequence see J. Magn. Reson., (1988), 77, pg 274. [CHMO]" ;
                 skos:prefLabel "decoupling in the presence of scalar interactions" .


###  http://purl.allotrope.org/ontologies/process#AFP_0001699
af-p:AFP_0001699 rdf:type owl:Class ;
                 rdfs:subClassOf af-p:AFP_0002455 ;
                 skos:definition "The application of a mathematical operation to both the real and imaginary parts of the complex numbers represented by the FID recorded as the sample magnetisation vector relaxes from its excited state vector back to its equilibrium bulk magnetisation population as adjusted by automated algorithms in the data acquisition or processing software. [Allotrope]" ;
                 skos:prefLabel "automatic phase correction" .


###  http://purl.allotrope.org/ontologies/process#AFP_0001702
af-p:AFP_0001702 rdf:type owl:Class ;
                 rdfs:subClassOf af-p:AFP_0002129 ;
                 skos:altLabel "ENDOR" ,
                               "ENDOR spectroscopy" ,
                               "EPR detected NMR" ;
                 skos:prefLabel "electron nuclear double resonance " .


###  http://purl.allotrope.org/ontologies/process#AFP_0001705
af-p:AFP_0001705 rdf:type owl:Class ;
                 rdfs:subClassOf af-p:AFP_0000408 ;
                 skos:altLabel "TQF" ;
                 skos:definition "An NMR technique used to edit the NMR response from a sample by selecting only three-spin coupled systems, usually achieved by appropriate cycling of the phase (direction of application) of the pulses in an experiment and of the receiver. [CHMO]" ;
                 skos:prefLabel "triple quantum filter" .


###  http://purl.allotrope.org/ontologies/process#AFP_0001720
af-p:AFP_0001720 rdf:type owl:Class ;
                 rdfs:subClassOf af-p:AFP_0001702 ;
                 skos:altLabel "c.w. ENDOR" ,
                               "continous wave ENDOR" ,
                               "continuous wave electron nuclear double resonance spectroscopy" ,
                               "cw ENDOR" ,
                               "cw-ENDOR" ;
                 skos:definition "A type of spectroscopy where a sample is irradiated by a microwave frequency which matches an electron resonance transition, whilst nuclei in the vicinty of the unpaired eletron are excited by a radio frequency sweep. [CHMO]" ;
                 skos:prefLabel "continuous-wave electron nuclear double resonance spectroscopy" .


###  http://purl.allotrope.org/ontologies/process#AFP_0001723
af-p:AFP_0001723 rdf:type owl:Class ;
                 rdfs:subClassOf af-p:AFP_0001332 ;
                 skos:altLabel "2D HSQC-TOCSY" ,
                               "two-dimensional heteronuclear single quantum coherence spectroscopy" ;
                 skos:definition "A 2D NMR experiment that correlates chemical shifts of a heteronucleus and proton via 1J(X-H) heteronuclear coupling showing two different spectra cross-peaks, one for direct 1H-heteronuclear connectivity (HSQC cross-peak) and the second relayed 1H-heteronucleus connectivities due to cumulative transfer. [Allotrope]" ;
                 skos:prefLabel "two-dimensional heteronuclear single quantum coherence-total correlation spectroscopy" .


###  http://purl.allotrope.org/ontologies/process#AFP_0001726
af-p:AFP_0001726 rdf:type owl:Class ;
                 rdfs:subClassOf af-p:AFP_0000833 ;
                 skos:altLabel "JR" ,
                               "JR pulse sequence" ,
                               "JR sequence" ,
                               "jump and return" ,
                               "jump-and-return" ,
                               "jump-and-return pulse sequence" ;
                 skos:definition "A pulse cluster used for solvent suppression consisting of two RF pulses separated by a delay with conditions set such that the solvent signal alone is rendered unobservable by the second pulse. For the pulse sequence see J. Am. Chem. Soc., (1982), 104, pg 7310. [CHMO]" ;
                 skos:prefLabel "jump and return pulse sequence" .


###  http://purl.allotrope.org/ontologies/process#AFP_0001729
af-p:AFP_0001729 rdf:type owl:Class ;
                 rdfs:subClassOf af-p:AFP_0001544 ;
                 skos:altLabel "gHMQC" ,
                               "gradient HMQC" ,
                               "gradient heteronuclear multiple quantum coherence" ,
                               "gradient-selected HMQC" ;
                 skos:definition "A type of heteronuclear NMR spectroscopy where a second frequency dimension is employed to disperse the signals and reveal correlations between protons and the nuclei to which they are covalently bound. A spatially inhomogeneous magnetic field is applied with a defined gradient and used to either select a particular signal or to render unwanted signals undetectable. [CHMO]" ;
                 skos:prefLabel "gradient-selected heteronuclear multiple quantum coherence" .


###  http://purl.allotrope.org/ontologies/process#AFP_0001742
af-p:AFP_0001742 rdf:type owl:Class ;
                 rdfs:subClassOf af-p:AFP_0000681 ;
                 skos:definition "Selected nuclei of a specified isotope are unselectively irradiated with a soft RF pulse. The frequency range for the nuclei being irradiated typically differs from the frequency range for the nuclei relaxing back to their bulk magnetisation relaxation state. [Allotrope]" ;
                 skos:prefLabel "off-resonance decoupling" .


###  http://purl.allotrope.org/ontologies/process#AFP_0001745
af-p:AFP_0001745 rdf:type owl:Class ;
                 rdfs:subClassOf af-p:AFP_0000879 ;
                 skos:altLabel "1H NMR absorption spectroscopy" ,
                               "1H c.w. NMR" ,
                               "1H continuous wave nuclear magnetic resonance spectroscopy" ,
                               "1H cw-NMR" ;
                 skos:definition "A type of spectroscopy where the energy states of 1H nuclei placed in a static magnetic field are interrogated by inducing transitions between the states via radio frequency irradiation. Spectra are obtained by scanning a range of radio frequencies. [CHMO]" ;
                 skos:prefLabel "1H continuous-wave nuclear magnetic resonance spectroscopy" .


###  http://purl.allotrope.org/ontologies/process#AFP_0001751
af-p:AFP_0001751 rdf:type owl:Class ;
                 rdfs:subClassOf af-p:AFP_0000325 ;
                 skos:altLabel "HNCA experiment " ;
                 skos:definition "A triple-resonance NMR experiment used in to determine the chemical shifts of nuclei in a (isotopically enriched) protein. The chemical shift of the (backbone) amide proton is correlated with the chemical shift of the covalently bound nitrogen and the alpha carbons of the same and preceding residues. [CHMO]" ;
                 skos:prefLabel "HNCA" .


###  http://purl.allotrope.org/ontologies/process#AFP_0001772
af-p:AFP_0001772 rdf:type owl:Class ;
                 rdfs:subClassOf af-p:AFP_0000038 ;
                 skos:altLabel "1H ENDOR" ,
                               "1H ENDOR spectroscopy" ,
                               "hydrogen-1 ENDOR" ,
                               "hydrogen-1 ENDOR spectroscopy" ,
                               "proton ENDOR" ,
                               "proton ENDOR spectroscopy" ;
                 skos:definition "A type of spectroscopy where a microwave frequency pulse is used to saturate the electron resonance transitions in the 1H nuclei of a sample, and a radio frequency pulse is used excite a nuclear transition. [CHMO]" ;
                 skos:prefLabel "1H electron nuclear double resonance spectroscopy" .


###  http://purl.allotrope.org/ontologies/process#AFP_0001804
af-p:AFP_0001804 rdf:type owl:Class ;
                 rdfs:subClassOf af-p:AFP_0002041 ;
                 skos:altLabel "CTMAS" ,
                               "CTMAS NMR" ,
                               "central-transition magic-angle spinning" ;
                 skos:definition "An NMR experiment where the selective excitation of central transitions during magic angle spinning is used for recording high-resolution NMR spectra of quadrupolar nuclei in solids. [CHMO]" ;
                 skos:prefLabel "central transition magic angle spinning" .


###  http://purl.allotrope.org/ontologies/process#AFP_0001852
af-p:AFP_0001852 rdf:type owl:Class ;
                 rdfs:subClassOf af-p:AFP_0000127 ;
                 skos:altLabel "MASSEY" ,
                               "MASSEY NMR" ;
                 skos:definition "An NMR experiment used to measure self-diffusion coefficients via signal attenuation which occurs due to diffusion during the application of pulsed field gradients. This experiment also corrects for the effects of imperfect pulsed field gradients. [CHMO]" ;
                 skos:prefLabel "modulus addition using spatially separated echo spectroscopy" .


###  http://purl.allotrope.org/ontologies/process#AFP_0001867
af-p:AFP_0001867 rdf:type owl:Class ;
                 rdfs:subClassOf af-p:AFP_0002044 ;
                 skos:altLabel "proton-decoupled NMR" ,
                               "proton-decoupled NMR spectroscopy" ;
                 skos:definition "A type of NMR spectroscopy where (J/scalar) couplings to 1H nuclei are cancelled by applying radio frequency radiation to saturate or otherwise manipulate the 1H spins such that no evolution of the coupling occurs. [CHMO]" ;
                 skos:prefLabel "proton-decoupled nuclear magnetic resonance spectroscopy" .


###  http://purl.allotrope.org/ontologies/process#AFP_0001874
af-p:AFP_0001874 rdf:type owl:Class ;
                 rdfs:subClassOf af-p:AFP_0000308 ;
                 skos:altLabel "heteronuclear 3D NMR" ;
                 skos:definition "Any type of nuclear magnetic resonance spectroscopy in which three independent frequency dimensions are employed for the correlation and dispersal of signals. Each signal is described by three frequencies, arising from a combination of protons and heteronuclei, thus effecting the distribution of signals within a cube. [CHMO]" ;
                 skos:prefLabel "heteronuclear three-dimensional nuclear magnetic resonance spectroscopy" .


###  http://purl.allotrope.org/ontologies/process#AFP_0001880
af-p:AFP_0001880 rdf:type owl:Class ;
                 rdfs:subClassOf af-p:AFP_0000408 ;
                 skos:altLabel "SQF" ;
                 skos:definition "An NMR technique used to edit the NMR response from a sample by selecting only uncoupled spins (singlets), usually achieved by appropriate cycling of the phase (direction of application) of the pulses in an experiment and of the receiver. [CHMO]" ;
                 skos:prefLabel "single quantum filter" .


###  http://purl.allotrope.org/ontologies/process#AFP_0001882
af-p:AFP_0001882 rdf:type owl:Class ;
                 rdfs:subClassOf af-p:AFP_0001332 ;
                 skos:altLabel "HMBC" ,
                               "HMBC NMR" ;
                 skos:definition "A type of heteronuclear NMR spectroscopy where a second frequency dimension is employed to disperse the signals and reveal correlations between protons and nuclei which are 2-3 bonds removed. [CHMO]" ;
                 skos:prefLabel "heteronuclear multiple bond coherence" .


###  http://purl.allotrope.org/ontologies/process#AFP_0001888
af-p:AFP_0001888 rdf:type owl:Class ;
                 rdfs:subClassOf af-p:AFP_0002536 ;
                 skos:altLabel "NMR pulse sequence" ,
                               "pulse sequence" ;
                 skos:definition "A series of short (microsecond) bursts (pulses) of RF radiation separated by delays (of defined duration) designed to interact with, and manipulate the magnetic moments of spin-active nuclei during NMR spectroscopy. [CHMO]" ;
                 skos:prefLabel "nuclear magnetic resonance pulse sequence" .


###  http://purl.allotrope.org/ontologies/process#AFP_0001892
af-p:AFP_0001892 rdf:type owl:Class ;
                 rdfs:subClassOf af-p:AFP_0000743 ;
                 skos:changeNote "2024-09-11 Replaced definition with an Allotrope written one." ;
                 skos:definition "Post-acquisition water suppression is a data processing used to suppress the signal from the water solvent after data acquisition. [Allotrope]" ;
                 skos:prefLabel "post-acquisition water suppression" .


###  http://purl.allotrope.org/ontologies/process#AFP_0001898
af-p:AFP_0001898 rdf:type owl:Class ;
                 rdfs:subClassOf af-p:AFP_0002041 ;
                 skos:altLabel "CRAMPS" ,
                               "combined rotation and multiple pulse spectrometry" ;
                 skos:definition "A type of NMR spectroscopy using a solid sample. Anisotropic interactions between nuclei, which are usually averaged by Brownian motion in liquid samples, cause significant line broadening in solid state NMR, but can be averaged to zero by spinning the sample very rapidly at the magic angle (54.74 deg. with respect to the direction of the magnetic field).The combination of multiple-pulse NMR experiments and magic angle spinning. Each experiment consists of a sequence of radio frequency pulses with delay periods in between them. [CHMO]" ;
                 skos:prefLabel "combined rotation and multiple pulse spectroscopy" .


###  http://purl.allotrope.org/ontologies/process#AFP_0001920
af-p:AFP_0001920 rdf:type owl:Class ;
                 rdfs:subClassOf af-p:AFP_0000943 ;
                 skos:altLabel "2D VACSY" ,
                               "2D VACSY NMR" ,
                               "VACSY" ,
                               "VACSY NMR" ,
                               "variable-angle correlation spectroscopy " ;
                 skos:definition "A two-dimensional solid-state NMR experiment which correlates the chemical shift anisotropy of a nucleus with its isotropic chemical shift by performing a series of experiments each at a different spinning angle relative to the magnetic field. [CHMO]" ;
                 skos:prefLabel "variable angle correlation spectroscopy" .


###  http://purl.allotrope.org/ontologies/process#AFP_0001944
af-p:AFP_0001944 rdf:type owl:Class ;
                 rdfs:subClassOf af-p:AFP_0000657 ;
                 skos:altLabel "CAMELPSIN" ,
                               "ROESY" ,
                               "ROESY NMR" ,
                               "cross-relaxation appropriate for minimolecules emulated by locked spins" ,
                               "rOesy" ,
                               "rotating frame Overhauser effect spectrometry" ,
                               "rotating frame Overhauser enhancement spectrometry" ,
                               "rotating frame Overhauser enhancement spectroscopy" ,
                               "rotational Overhauser effect spectroscopy" ;
                 skos:definition "A type of heteronuclear NMR spectroscopy where a second frequency dimension is employed, based on the nuclear Overhauser enhancement (NOE) effect in which correlations are seen between nuclei that are spatially proximate within a molecule (<= 6 Angstrom apart). Spin-locking is employed to ensure that correlation between spins, which are close in space but have zero NOE, are seen. This technique is used for molecules whose tumbling regime lies at the border of positive and negative NOE responses. [CHMO]" ;
                 skos:prefLabel "rotating frame Overhauser effect spectroscopy" .


###  http://purl.allotrope.org/ontologies/process#AFP_0001964
af-p:AFP_0001964 rdf:type owl:Class ;
                 rdfs:subClassOf af-p:AFP_0000681 ;
                 skos:definition "The nuclei being irradiated with an RF pulse is the same nuclei and isotope as the nuclei being observed to relax back to equilibrium for generation of the NMR spectrum. [Allotrope]" ;
                 skos:prefLabel "homonuclear decoupling" .


###  http://purl.allotrope.org/ontologies/process#AFP_0001973
af-p:AFP_0001973 rdf:type owl:Class ;
                 rdfs:subClassOf af-p:AFP_0002384 ;
                 skos:altLabel "2DJ-DOSY" ,
                               "3D 2DJ-DOSY" ,
                               "3D DOSY-2DJ" ,
                               "DOSY-2DJ" ,
                               "diffusion-ordered spectroscopy-two-dimensional J-spectroscopy" ;
                 skos:definition "A type of three-dimensional NMR experiment in which the signals of a 2D J-spectrum are dispersed along a third frequency axis according to diffusion coefficient. [CHMO]" ;
                 skos:prefLabel "two-dimensional J-spectroscopy-diffusion-ordered spectroscopy" .


###  http://purl.allotrope.org/ontologies/process#AFP_0001983
af-p:AFP_0001983 rdf:type owl:Class ;
                 rdfs:subClassOf af-p:AFP_0001888 ;
                 skos:altLabel "FLOPSY" ,
                               "flip-flop spectroscopy" ;
                 skos:definition "A sequence of composite pulses designed to allow isotropic mixing of magnetisation between nuclei. For the pulse sequence see J. Magn.Reson., (1988), 77, pg 274. [CHMO]" ;
                 skos:prefLabel "flip flop spectroscopy" .


###  http://purl.allotrope.org/ontologies/process#AFP_0001997
af-p:AFP_0001997 rdf:type owl:Class ;
                 rdfs:subClassOf af-p:AFP_0001084 ;
                 skos:definition "An RF pulse that unselectively excites a spin system over a given bandwidth. [Allotrope]" ;
                 skos:prefLabel "hard pulse" .


###  http://purl.allotrope.org/ontologies/process#AFP_0002012
af-p:AFP_0002012 rdf:type owl:Class ;
                 rdfs:subClassOf af-p:AFP_0001122 ;
                 skos:altLabel "STOCSY" ,
                               "STOCSY NMR" ,
                               "statistical COSY" ;
                 skos:definition "A type of homonuclear NMR spectroscopy which reveal correlations between all nuclei of a spin-system. This technique exploits the correlations seen between the intensities of spectral features of multiple spectra so as to obtain a statistically derived spectrum. This technique is of particular value for metabolic profiling. [CHMO]" ;
                 skos:prefLabel "statistical total correlation spectroscopy" .


###  http://purl.allotrope.org/ontologies/process#AFP_0002041
af-p:AFP_0002041 rdf:type owl:Class ;
                 rdfs:subClassOf af-p:AFP_0002261 ;
                 skos:altLabel "MAS NMR" ,
                               "MAS NMR spectroscopy" ,
                               "MAS-NMR" ,
                               "SS-MAS NMR" ,
                               "magic angle spinning nuclear magnetic resonance spectrometry" ,
                               "magic-angle spinning" ,
                               "solid-state magic-angle-spinning NMR" ,
                               "ss-MAS-NMR" ;
                 skos:definition "A type of NMR spectroscopy using a solid sample. Anisotropic interactions between nuclei, which are usually averaged by Brownian motion in liquid samples, cause significant line broadening in solid state NMR, but can be averaged to zero by spinning the sample very rapidly at the magic angle (54.74 deg. with respect to the direction of the magnetic field). [CHMO]" ;
                 skos:prefLabel "magic angle spinning" .


###  http://purl.allotrope.org/ontologies/process#AFP_0002044
af-p:AFP_0002044 rdf:type owl:Class ;
                 rdfs:subClassOf af-p:AFP_0000326 ;
                 skos:altLabel "NMR" ,
                               "NMR spectrometry" ,
                               "NMR spectroscopy" ,
                               "nuclear magnetic resonance spectrometry" ,
                               "nuclear magnetic resonance spectroscopy" ,
                               "pulsed nuclear magnetic resonance spectrometry" ;
                 skos:definition "A type of spectroscopy where the energy states of spin-active nuclei placed in a static magnetic field are interrogated by inducing transitions between the states via radio frequency irradiation. Each experiment consists of a sequence of radio frequency pulses with delay periods in between them. [CHMO]" ;
                 skos:prefLabel "pulsed nuclear magnetic resonance spectroscopy" .


###  http://purl.allotrope.org/ontologies/process#AFP_0002049
af-p:AFP_0002049 rdf:type owl:Class ;
                 rdfs:subClassOf af-p:AFP_0000906 ;
                 skos:altLabel "MSHOT3" ,
                               "MSHOT3 pulse sequence" ,
                               "MSHOT3 sequence" ,
                               "magic sandwich high order truncation" ,
                               "magic sandwich high-order truncation" ;
                 skos:definition "A sequence of pulses used in magic angle spinning NMR to remove the effect of homonuclear dipolar couplings. For the pulse sequence see J. Chem. Phys., (1997), 125, pg 291. [CHMO]" ;
                 skos:prefLabel "magic sandwich high-order truncation pulse sequence" .


###  http://purl.allotrope.org/ontologies/process#AFP_0002050
af-p:AFP_0002050 rdf:type owl:Class ;
                 rdfs:subClassOf af-p:AFP_0001277 ;
                 skos:altLabel "gCOSY" ,
                               "gradient-selected COSY" ;
                 skos:definition "A type of homonuclear NMR spectroscopy where a second frequency dimension is employed to disperse the signals and reveal correlations between nuclei that are J-coupled (usually <= 3 bonds apart). A spatially inhomogeneous magnetic field is applied with a defined gradient and used to either select a particular signal or to render unwanted signals undetectable. [CHMO]" ;
                 skos:prefLabel "gradient-selected correlation spectroscopy" .


###  http://purl.allotrope.org/ontologies/process#AFP_0002054
af-p:AFP_0002054 rdf:type owl:Class ;
                 rdfs:subClassOf af-p:AFP_0001122 ;
                 skos:altLabel "2D TOCSY" ,
                               "2D-TOCSY" ,
                               "two-dimensional TOCSY" ;
                 skos:definition "A type of homonuclear NMR spectroscopy where a second frequency dimension is employed to disperse the signals and which reveal correlations between all nuclei of a spin-system. [CHMO]" ;
                 skos:prefLabel "two-dimensional total correlation spectroscopy" .


###  http://purl.allotrope.org/ontologies/process#AFP_0002056
af-p:AFP_0002056 rdf:type owl:Class ;
                 rdfs:subClassOf af-p:AFP_0000759 ;
                 skos:altLabel "phase sequence" ;
                 skos:definition "A technique used in FT NMR experiments whereby the sense of application (or phase) of the RF pulses is altered on repeating the experiment such that addition of the resulting signals results in increased intensity for the signals of interest, elimination of artefacts and more effective noise reduction. [CHMO]" ;
                 skos:prefLabel "phase cycle" .


###  http://purl.allotrope.org/ontologies/process#AFP_0002057
af-p:AFP_0002057 rdf:type owl:Class ;
                 rdfs:subClassOf af-p:AFP_0000743 ;
                 skos:altLabel "z-filling" ;
                 skos:definition "A recorded RF signal in NMR spectroscopy observed as the perturbed sample magnetisation relaxes back to its bulk magnetisation population state that has been suffixed with a set of data points containing many zeros. [Allotrope]" ;
                 skos:prefLabel "FID zero filling" .


###  http://purl.allotrope.org/ontologies/process#AFP_0002063
af-p:AFP_0002063 rdf:type owl:Class ;
                 rdfs:subClassOf af-p:AFP_0002044 ;
                 skos:altLabel "2-D NMR" ,
                               "2D NMR" ,
                               "2D NMR spectrometry" ,
                               "2D NMR spectroscopy" ,
                               "2D nuclear magnetic resonance" ,
                               "2D nuclear magnetic resonance spectrometry" ,
                               "two-dimensional NMR" ,
                               "two-dimensional nuclear magnetic resonance spectrometry" ,
                               "two-dimensional nuclear magnetic resonance spectroscopy" ;
                 skos:definition "An NMR experiment in which a second frequency dimension is employed to disperse the signals and reveal correlations between interacting nuclei. [CHMO]" ;
                 skos:prefLabel "two-dimensional nuclear magnetic resonance spectroscopy" .


###  http://purl.allotrope.org/ontologies/process#AFP_0002072
af-p:AFP_0002072 rdf:type owl:Class ;
                 rdfs:subClassOf af-p:AFP_0000325 ;
                 skos:altLabel "HN(CO)CAHA experiment" ;
                 skos:definition "A triple-resonance NMR experiment used to determine the chemical shifts of nuclei in a (isotopically enriched) protein. The chemical shift of the (backbone) amide proton is correlated with the chemical shift of the covalently bound nitrogen and with the alpha-carbon and proton of the preceding residue. The experiment name describes the path taken by the magnetization during the experiment. [CHMO]" ;
                 skos:prefLabel "HN(CO)CAHA" .


###  http://purl.allotrope.org/ontologies/process#AFP_0002075
af-p:AFP_0002075 rdf:type owl:Class ;
                 rdfs:subClassOf af-p:AFP_0001888 ;
                 skos:changeNote "2024-09-11 Changed [Amgen] attribution to [Allotrope]." ;
                 skos:definition "Homospoil is an NMR pulse sequence that results in linear variation of the magnetic field in the z direction. After the homospoil pulse, transverse magnetization in the slices of sample will acquire additional phase, which will vary with height. Net x-y plane magnetization will be zero. [Allotrope]" ;
                 skos:prefLabel "homospoil pulse sequence" .


###  http://purl.allotrope.org/ontologies/process#AFP_0002100
af-p:AFP_0002100 rdf:type owl:Class ;
                 rdfs:subClassOf af-p:AFP_0000759 ;
                 skos:altLabel "ZZ filter" ;
                 skos:definition "A technique used in NMR experiments to remove unwanted signals from the spectrum by destroying the magnetization giving rise to these signals using a pulsed filed gradient whilst the magnetization of interest is maintained in a state which is unaffected by the pulsed field gradient (ZZ-state). [CHMO]" ;
                 skos:prefLabel "ZZ-filter" .


###  http://purl.allotrope.org/ontologies/process#AFP_0002134
af-p:AFP_0002134 rdf:type owl:Class ;
                 rdfs:subClassOf af-p:AFP_0000038 ;
                 skos:altLabel "17O ENDOR" ,
                               "17O ENDOR spectroscopy" ,
                               "oxygen-17 ENDOR" ,
                               "oxygen-17 ENDOR spectroscopy" ;
                 skos:definition "A type of spectroscopy where a microwave frequency pulse is used to saturate the electron resonance transitions in the 17O nuclei of a sample, and a radio frequency pulse is used excite a nuclear transition. [CHMO]" ;
                 skos:prefLabel "17O electron nuclear double resonance spectroscopy" .


###  http://purl.allotrope.org/ontologies/process#AFP_0002153
af-p:AFP_0002153 rdf:type owl:Class ;
                 rdfs:subClassOf af-p:AFP_0000721 ;
                 skos:altLabel "PAR" ,
                               "PAR pulse sequence" ,
                               "PAR sequence" ,
                               "phase-alternated rotation of magnetization" ;
                 skos:definition "A sequence of composite pulses designed to remove signal splitting due to heteronuclear J-couplings in multinuclear liquid NMR experiments. [CHMO]" ;
                 skos:prefLabel "phase alternated rotation of magnetization" .


###  http://purl.allotrope.org/ontologies/process#AFP_0002176
af-p:AFP_0002176 rdf:type owl:Class ;
                 rdfs:subClassOf af-p:AFP_0002455 ;
                 skos:definition "The application of a phase correction algorithm to a Fourier transform NMR spectra such that it is optimised to give maximum values for the frequency dependent real part of the frequency signal (and minimum values for the imaginary part) of the FID Fourier transform complex number set. [Allotrope]" ;
                 skos:prefLabel "zero order phase correction" .


###  http://purl.allotrope.org/ontologies/process#AFP_0002181
af-p:AFP_0002181 rdf:type owl:Class ;
                 rdfs:subClassOf af-p:AFP_0000906 ;
                 skos:altLabel "WAHUHA" ,
                               "WAHUHA pulse sequence" ,
                               "WAHUHA sequence" ,
                               "Waugh Huber Haeberlin sequence" ,
                               "Waugh, Huber, Haeberlin pulse sequence" ,
                               "Waugh-Huber-Haeberlin pulse sequence" ,
                               "Waugh-Huber-Haeberlin sequence" ;
                 skos:definition "A pulse sequence used in magic angle spinning NMR to remove the effects of homonuclear dipolar coupling. For the pulse sequence see Phys. Rev. Lett., (1968), 20, pg 180. [CHMO]" ;
                 skos:prefLabel "Waugh, Huber, Haeberlin pulse sequence" .


###  http://purl.allotrope.org/ontologies/process#AFP_0002202
af-p:AFP_0002202 rdf:type owl:Class ;
                 rdfs:subClassOf af-p:AFP_0001552 ;
                 skos:altLabel "HR-DOSY" ,
                               "high resolution DOSY" ,
                               "high resolution diffusion-ordered spectroscopy" ,
                               "high-resolution DOSY" ;
                 skos:definition "A type of NMR spectroscopy using pulsed-field gradients where the rate of decay of NMR signals in each component of a sample mixture is measured across a series of experiments. The rate of signal decay is proportional to the diffusion coefficient for each component. The diffusion coefficient for each peak is measured and this information is used to construct a 2D spectrum. [CHMO]" ;
                 skos:prefLabel "high-resolution diffusion-ordered spectroscopy" .


###  http://purl.allotrope.org/ontologies/process#AFP_0002249
af-p:AFP_0002249 rdf:type owl:Class ;
                 rdfs:subClassOf af-p:AFP_0002384 ;
                 skos:altLabel "3D DOSY-HMQC" ,
                               "3D HMQC-DOSY" ,
                               "DOSY-HMQC" ,
                               "HMQC-DOSY" ,
                               "diffusion-ordered spectroscopy-heteronuclear multiple quantum coherence" ;
                 skos:definition "A type of three-dimensional NMR experiment in which the signals of a 2D HMQC spectrum are dispersed along a third frequency axis according to diffusion coefficient. [CHMO]" ;
                 skos:prefLabel "heteronuclear multiple quantum coherence-diffusion-ordered spectroscopy" .


###  http://purl.allotrope.org/ontologies/process#AFP_0002261
af-p:AFP_0002261 rdf:type owl:Class ;
                 rdfs:subClassOf af-p:AFP_0002044 ;
                 skos:altLabel "SS-NMR" ,
                               "SSNMR" ,
                               "solid state NMR" ,
                               "solid state nuclear magnetic resonance spectrometry" ,
                               "solid-state NMR" ;
                 skos:definition "A type of spectroscopy where the response of nuclei with non-zero spin, in a solid sample, to a perturbing magnetic field is detected. Each experiment consists of a sequence of radio frequency pulses with delay periods in between them. [CHMO]" ;
                 skos:prefLabel "solid-state nuclear magnetic resonance spectroscopy" .


###  http://purl.allotrope.org/ontologies/process#AFP_0002263
af-p:AFP_0002263 rdf:type owl:Class ;
                 rdfs:subClassOf af-p:AFP_0001122 ;
                 skos:altLabel "1D TOCSY" ,
                               "1D-TOCSY" ,
                               "one-dimensional TOCSY" ;
                 skos:definition "A type of homonuclear NMR spectroscopy which reveal correlations between all nuclei of a spin-system.  An individual 1H resonance is selected and inverted to yield a spectrum of all hydrogens directly or indirectly scalar coupled to it. [CHMO]" ;
                 skos:prefLabel "one-dimensional total correlation spectroscopy" .


###  http://purl.allotrope.org/ontologies/process#AFP_0002273
af-p:AFP_0002273 rdf:type owl:Class ;
                 rdfs:subClassOf af-p:AFP_0000759 ;
                 skos:definition "A technique used in multidimensional NMR experiments to achieve frequency discrimination of the signals in the additional dimensions. [CHMO]" ;
                 skos:prefLabel "states acquisition" .


###  http://purl.allotrope.org/ontologies/process#AFP_0002287
af-p:AFP_0002287 rdf:type owl:Class ;
                 rdfs:subClassOf af-p:AFP_0000759 ;
                 skos:altLabel "INEPT" ,
                               "INEPT NMR" ;
                 skos:definition "A heteronuclear NMR experiment in which magnetization arising from 1H nuclei is transferred to covalently bound heteronuclei, thereby enhancing the NMR signal of the heteronuclei. [CHMO]" ;
                 skos:prefLabel "insensitive nuclei enhancement by polarization transfer" .


###  http://purl.allotrope.org/ontologies/process#AFP_0002290
af-p:AFP_0002290 rdf:type owl:Class ;
                 rdfs:subClassOf af-p:AFP_0002044 ;
                 skos:altLabel "ultra high field NMR" ,
                               "ultra high-field NMR" ,
                               "ultrahigh-field NMR" ;
                 skos:definition "A type of spectroscopy where the energy states of spin-active nuclei placed in a static (>900 MHz) magnetic field are interrogated by inducing transitions between the states via radio frequency irradiation. Each experiment consists of a sequence of radio frequency pulses with delay periods in between them. [CHMO]" ;
                 skos:prefLabel "ultra-high-field nuclear magnetic resonance spectroscopy" .


###  http://purl.allotrope.org/ontologies/process#AFP_0002300
af-p:AFP_0002300 rdf:type owl:Class ;
                 rdfs:subClassOf af-p:AFP_0000681 ;
                 skos:definition "All nuclei of a specified isotope are unselectively irradiated with an RF pulse. [Allotrope]" ;
                 skos:prefLabel "broadband decoupling" .


###  http://purl.allotrope.org/ontologies/process#AFP_0002350
af-p:AFP_0002350 rdf:type owl:Class ;
                 rdfs:subClassOf af-p:AFP_0001874 ;
                 skos:altLabel "3D NOESY-HSQC" ;
                 skos:definition "A 3D NMR experiment in which the chemical shifts of protons are correlated with the chemical shifts of spatially proximate protons (<6 Angstrom) and with the shifts of the heteronuclei bound to these proximate protons. [CHMO]" ;
                 skos:prefLabel "three-dimensional nuclear Overhauser spectroscopy-heteronuclear single quantum coherence" .


###  http://purl.allotrope.org/ontologies/process#AFP_0002368
af-p:AFP_0002368 rdf:type owl:Class ;
                 rdfs:subClassOf af-p:AFP_0002445 ;
                 skos:altLabel "STDD-NMR" ,
                               "saturation-transfer double-difference nuclear magnetic resonance spectroscopy" ;
                 skos:definition "A type of NMR spectroscopy where radio frequency pulses are used to induce an equal population of upper and lower spin states in ('saturate') certain selected protons, removing their signal from the NMR spectrum. The signal from two different samples is obtained simultaneously and common signals are cancelled automatically. Saturation-transfer double-difference NMR is used to detect the transient binding of small molecule ligands to macromolecular receptors. [CHMO]" ;
                 skos:prefLabel "saturation transfer double difference nuclear magnetic resonance spectroscopy" .


###  http://purl.allotrope.org/ontologies/process#AFP_0002375
af-p:AFP_0002375 rdf:type owl:Class ;
                 rdfs:subClassOf af-p:AFP_0000759 ;
                 skos:altLabel "heteronuclear nXQF element" ;
                 skos:definition "A technique used in NMR of isotopically enriched samples (usually 13C/15N) to select for, or to remove signals of protons bound to a particular isotope. [CHMO]" ;
                 skos:prefLabel "X-filter" .


###  http://purl.allotrope.org/ontologies/process#AFP_0002376
af-p:AFP_0002376 rdf:type owl:Class ;
                 rdfs:subClassOf af-p:AFP_0000326 ;
                 skos:altLabel "liquid phase NMR" ,
                               "liquid phase nuclear magnetic resonance spectroscopy" ,
                               "liquid-phase nuclear magnetic resonance spectroscopy" ;
                 skos:definition "A type of spectroscopy in the liquid phase where the energy states of spin-active nuclei placed in a static magnetic field are interrogated by inducing transitions between the states via radio frequency irradiation. [CHMO]" ;
                 skos:prefLabel "liquid-phase nuclear magnetic resonance spectroscopy" .


###  http://purl.allotrope.org/ontologies/process#AFP_0002384
af-p:AFP_0002384 rdf:type owl:Class ;
                 rdfs:subClassOf af-p:AFP_0000308 ;
                 skos:altLabel "3D DOSY" ,
                               "3D DOSY NMR" ,
                               "3D-DOSY" ;
                 skos:definition "A type of three-dimensional NMR experiment in which the signals of a 2D NMR experiment are dispersed along a third frequency axis according to diffusion coefficient. [CHMO]" ;
                 skos:prefLabel "three-dimensional diffusion-ordered spectroscopy" .


###  http://purl.allotrope.org/ontologies/process#AFP_0002393
af-p:AFP_0002393 rdf:type owl:Class ;
                 rdfs:subClassOf af-p:AFP_0000657 ;
                 skos:altLabel "HOESY" ,
                               "HOESY NMR" ,
                               "heteronuclear Overhauser effect spectrometry" ,
                               "heteronuclear Overhauser effect spectroscopy" ,
                               "heteronuclear Overhauser enhancement spectrometry" ;
                 skos:definition "A type of heteronuclear NMR spectroscopy where a second frequency dimension is employed, based on the nuclear Overhauser enhancement effect in which correlations are seen between nuclei that are spatially proximate within a molecule (<= 6 Angstrom apart). [CHMO]" ;
                 skos:prefLabel "heteronuclear Overhauser enhancement spectroscopy" .


###  http://purl.allotrope.org/ontologies/process#AFP_0002408
af-p:AFP_0002408 rdf:type owl:Class ;
                 rdfs:subClassOf af-p:AFP_0002044 ;
                 skos:altLabel "1-D NMR" ,
                               "1D NMR" ,
                               "1D NMR spectrometry" ,
                               "1D NMR spectroscopy" ,
                               "1D nuclear magnetic resonance spectrometry" ,
                               "1D nuclear magnetic resonance spectroscopy" ,
                               "one-dimensional nuclear magnetic resonance spectrometry" ,
                               "one-dimensional nuclear magnetic resonance spectroscopy" ;
                 skos:definition "A type of spectroscopy where the energy states of spin-active nuclei placed in a static magnetic field are interrogated by inducing transitions between the states via radio frequency irradiation. Each experiment consists of a sequence of radio frequency pulses with delay periods in between them, and the spectrum is obtained by plotting intensity vs. chemical shift or frequency. [CHMO]" ;
                 skos:prefLabel "one-dimensional nuclear magnetic resonance spectroscopy" .


###  http://purl.allotrope.org/ontologies/process#AFP_0002445
af-p:AFP_0002445 rdf:type owl:Class ;
                 rdfs:subClassOf af-p:AFP_0001060 ;
                 skos:altLabel "STD" ,
                               "STD-NMR " ,
                               "STD-NMR spectroscopy " ,
                               "nuclear magnetic resonance saturation transfer difference (STD) spectroscopy" ,
                               "nuclear magnetic resonance saturation transfer difference spectroscopy" ,
                               "saturation transfer difference (STD) nuclear magnetic resonance spectroscopy " ;
                 skos:definition "A type of NMR spectroscopy where radio frequency pulses are used to induce an equal population of upper and lower spin states in ('saturate') certain selected protons, removing their signal from the NMR spectrum. The resulting spectrum is then subtracted from a reference spectrum obtained without saturation. Saturation-transfer NMR is used to detect the transient binding of small molecule ligands to macromolecular receptors. [CHMO]" ;
                 skos:prefLabel "saturation transfer difference nuclear magnetic resonance spectroscopy" .


###  http://purl.allotrope.org/ontologies/process#AFP_0002454
af-p:AFP_0002454 rdf:type owl:Class ;
                 rdfs:subClassOf af-p:AFP_0001332 ;
                 skos:altLabel "2D heteronuclear correlation spectroscopy" ,
                               "HETCOR" ,
                               "HETCORR" ,
                               "HETCOSY" ,
                               "HETEROCOR" ,
                               "hetCOSY" ,
                               "heteronuclear COSY" ,
                               "two-dimensional heteronuclear correlation spectroscopy" ;
                 skos:definition "A type of NMR spectroscopy where a second frequency dimension is employed to disperse the signals and reveal correlations between protons and heteronuclei. [CHMO]" ;
                 skos:prefLabel "heteronuclear correlation spectroscopy" .


###  http://purl.allotrope.org/ontologies/process#AFP_0002455
af-p:AFP_0002455 rdf:type owl:Class ;
                 rdfs:subClassOf af-p:AFP_0000743 ;
                 skos:definition "Application of a trigonometric mathematical operation to both the real and imaginary parts of the complex numbers represented by the FID recorded as the sample magnetization vector relaxes from its excited state vector back to its equilibrium bulk magnetization population. [Allotrope]" ;
                 skos:prefLabel "phase correction" .


###  http://purl.allotrope.org/ontologies/process#AFP_0002485
af-p:AFP_0002485 rdf:type owl:Class ;
                 rdfs:subClassOf af-p:AFP_0000694 ;
                 skos:altLabel "DEPTQ" ,
                               "DEPTQ NMR" ;
                 skos:changeNote "2024-09-11 Changed [OSTHUS] attribution to [Allotrope]." ;
                 skos:definition "A type of spectroscopy where the energy states of 13C nuclei placed in a static magnetic field are interrogated by inducing transitions between the states via radio frequency irradiation. Each experiment consists of a sequence of radio frequency pulses with delay periods in between them.The 13C NMR signals are enhanced by transferring 1H magnetization to 13C nuclei and the phase of the signals reflects the multiplicity i.e. CH, CH2 or CH3). Separate methyl, methylene and methine spectra may be obtained. The quaternary carbon centres are also represented in the spectra, albeit with reduced intensities, and are rendered with similar 'signs' to methylene groups. [Allotrope]" ;
                 skos:prefLabel "distortionless enhancement with polarization transfer retention of quaternaries" .


###  http://purl.allotrope.org/ontologies/process#AFP_0002486
af-p:AFP_0002486 rdf:type owl:Class ;
                 rdfs:subClassOf af-p:AFP_0001060 ;
                 skos:altLabel "EXSY" ,
                               "exchange spectroscopy" ,
                               "nuclear Overhauser enhancement spectrometry including chemical and conformational change" ;
                 skos:definition "A type of homonuclear NMR spectroscopy based on the nuclear Overhauser enhancement effect in which through space spin-lattice correlations are made between nuclei that are spatially proximate within a molecule (<= 6 Angstrom apart) but not directly bonded. The technique differs from the traditional NoE experiment in that it is also used to detect chemical and conformational change within the chemical moiety being examined. [Allotrope]" ;
                 skos:prefLabel "nuclear Overhauser enhancement spectroscopy including chemical and conformational change" .


###  http://purl.allotrope.org/ontologies/process#AFP_0002686
af-p:AFP_0002686 rdf:type owl:Class ;
                 rdfs:subClassOf af-p:AFP_0000485 ,
                                 obi:_0000011 ;
                 skos:altLabel "matching" ;
                 skos:definition "Probe matching is a process of adjustment of an NMR probe that makes sure that only a minimal part of the power at the probe is wasted. [Allotrope]" ;
                 skos:prefLabel "probe matching" .


###  http://purl.allotrope.org/ontologies/process#AFP_0002735
af-p:AFP_0002735 rdf:type owl:Class ;
                 rdfs:subClassOf af-p:AFP_0003331 ,
                                 obi:_0000011 ;
                 skos:definition "Locking is the process of establishing a magnetic field with a constant strength during an NMR measurement. [Allotrope]" ;
                 skos:prefLabel "locking" .


###  http://purl.allotrope.org/ontologies/process#AFP_0002752
af-p:AFP_0002752 rdf:type owl:Class ;
                 rdfs:subClassOf af-p:AFP_0003485 ,
                                 obi:_0000011 ;
                 skos:definition "Shimming is the process of adjusting the signal of an NMR spectrometer by changing the uniformity of the magnetic field. [Allotrope]" ;
                 skos:prefLabel "shimming" .


###  http://purl.allotrope.org/ontologies/process#AFP_0002796
af-p:AFP_0002796 rdf:type owl:Class ;
                 rdfs:subClassOf af-r:AFR_0001501 ;
                 skos:definition "A pulse program is a programmatic plan that defines the pulse sequence that is applied to the excitation of a sample. [Allotrope]" ;
                 skos:example "pulse program of ssNMR" ;
                 skos:prefLabel "pulse program" .


###  http://purl.allotrope.org/ontologies/process#AFP_0002838
af-p:AFP_0002838 rdf:type owl:Class ;
                 rdfs:subClassOf af-p:AFP_0000759 ;
                 skos:definition "A saturation recovery experiment is used to measure T1, especially if the line has a very broad shape or if inversion is impossible. A pulse sequence is applied that keeps the magnetization in the x-y plane until saturation is reached and then magnetization recovers during T1. [Allotrope]" ;
                 skos:prefLabel "saturation recovery" .


###  http://purl.allotrope.org/ontologies/result#AFR_0000017
af-r:AFR_0000017 rdf:type owl:Class ;
                 rdfs:subClassOf af-r:AFR_0000239 ,
                                 af-r:AFR_0000442 ;
                 skos:altLabel "1-D 1H NMR spectra" ,
                               "1-D 1H NMR spectrum" ,
                               "1D 1H NMR spectrum" ,
                               "1D NMR 1H spectra" ;
                 skos:definition "A plot of chemical shift vs. intensity for hydrogen-1 nuclei obtained by measuring the effect of the absorption of radio frequency radiation on nuclear spin-state transitions in the presence of a magnetic field. [CHMO]" ;
                 skos:prefLabel "one-dimensional proton nuclear magnetic resonance spectrum" .


###  http://purl.allotrope.org/ontologies/result#AFR_0000028
af-r:AFR_0000028 rdf:type owl:Class ;
                 rdfs:subClassOf af-r:AFR_0000521 ;
                 skos:altLabel "CP-MAS NMR spectra" ,
                               "CP-MAS NMR spectrum" ,
                               "CP/MAS NMR spectra" ,
                               "CP/MAS NMR spectrum" ,
                               "CPMAS NMR spectra" ,
                               "CPMAS NMR spectrum" ,
                               "cross-polarization magic angle spinning nuclear magnetic resonance spectra" ;
                 skos:definition "A nuclear magnetic resonance spectrum in which line broadening has been reduced to zero by spinning the sample very rapidly at the magic angle (54.74 deg. with respect to the direction of the magnetic field) and cross polarisation has been used to enhance the signal from weakly coupled nuclei. [CHMO]" ;
                 skos:prefLabel "cross-polarization magic angle spinning nuclear magnetic resonance spectrum" .


###  http://purl.allotrope.org/ontologies/result#AFR_0000143
af-r:AFR_0000143 rdf:type owl:Class ;
                 rdfs:subClassOf af-r:AFR_0000263 ;
                 skos:changeNote "2024-09-11 Changed [Amgen] attribution to [Allotrope]." ;
                 skos:definition "A proton-decoupled nuclear magnetic resonance spectrum is an NMR spectrum where coupling between protons and heteronuclei has been removed in order to improve the resolution of the spectrum of the heteronuclei. [Allotrope]" ;
                 skos:prefLabel "proton-decoupled nuclear magnetic resonance spectrum" .


###  http://purl.allotrope.org/ontologies/result#AFR_0000148
af-r:AFR_0000148 rdf:type owl:Class ;
                 rdfs:subClassOf af-c:AFC_0000050 ;
                 skos:definition "Code for describing the multiplicity of NMR peaks. [Allotrope]" ;
                 skos:example "singlet, doublet, multiplet" ;
                 skos:prefLabel "multiplicity code" .


###  http://purl.allotrope.org/ontologies/result#AFR_0000168
af-r:AFR_0000168 rdf:type owl:Class ;
                 rdfs:subClassOf af-r:AFR_0000263 ;
                 skos:altLabel "3D NMR spectra" ,
                               "3D NMR spectrum" ,
                               "3D-NMR spectra" ,
                               "3D-NMR spectrum" ;
                 skos:definition "A three-dimensional plot of chemical shift vs. intensity for spin-active nuclei obtained by measuring the effect of the absorption of radio frequency radiation on nuclear spin-state transitions in the presence of a magnetic field. Signals are defined in terms of three frequencies; by the chemical shift of a particular nucleus in one dimension and, in the other two, by the chemical shifts of correlated nuclei. [CHMO]" ;
                 skos:prefLabel "three-dimensional nuclear magnetic resonance spectrum" .


###  http://purl.allotrope.org/ontologies/result#AFR_0000176
af-r:AFR_0000176 rdf:type owl:Class ;
                 rdfs:subClassOf af-r:AFR_0000263 ;
                 skos:altLabel "CPMG spectra" ,
                               "CPMG spectrum" ,
                               "CPMG spin-echo spectra" ,
                               "CPMG spin-echo spectrum" ;
                 skos:definition "A plot of the nuclear magnetic resonance frequency vs. intensity composed of a series of peaks (separated by the reciprocal of a user-defined time delay in a CPMG pulse sequence) which describe the envelope of the full, static spectrum. [CHMO]" ;
                 skos:prefLabel "Carr-Purcell-Meiboom-Gill spectrum" .


###  http://purl.allotrope.org/ontologies/result#AFR_0000182
af-r:AFR_0000182 rdf:type owl:Class ;
                 rdfs:subClassOf af-r:AFR_0000521 ;
                 skos:altLabel "HR-MAS-NMR spectrum" ,
                               "HRMAS spectra" ,
                               "HRMAS spectrum" ,
                               "HRMAS-NMR spectra" ,
                               "high resolution MAS spectra" ,
                               "high resolution MAS spectrum" ,
                               "high-resolution MAS spectra" ,
                               "high-resolution MAS spectrum" ;
                 skos:definition "A nuclear magnetic resonance spectrum in which line broadening has been averaged to zero by spinning the sample very rapidly at the magic angle (54.74 deg. with respect to the direction of the magnetic field) and using a high-resolution magnetic susceptibility matching probe. [CHMO]" ;
                 skos:prefLabel "high-resolution magic angle spinning nuclear magnetic resonance spectrum" .


###  http://purl.allotrope.org/ontologies/result#AFR_0000183
af-r:AFR_0000183 rdf:type owl:Class ;
                 rdfs:subClassOf af-r:AFR_0000218 ;
                 skos:altLabel "HMBC spectra" ,
                               "HMBC spectrum" ;
                 skos:definition "A heteronuclear NMR spectrum where a second frequency dimension is employed to disperse the signals and reveal correlations between nuclei which are 2-3 bonds removed. [CHMO]" ;
                 skos:prefLabel "heteronuclear multiple bond coherence spectrum" .


###  http://purl.allotrope.org/ontologies/result#AFR_0000189
af-r:AFR_0000189 rdf:type owl:Class ;
                 rdfs:subClassOf af-r:AFR_0000218 ;
                 skos:altLabel "2D J-resolved NMR spectra" ,
                               "2D J-resolved NMR spectrum" ,
                               "J spectra" ,
                               "J spectrum" ,
                               "J-resolved NMR spectra" ,
                               "J-resolved NMR spectrum" ,
                               "J-resolved spectra" ,
                               "J-resolved spectrum" ,
                               "J-spectra" ,
                               "NMR J-spectra" ,
                               "NMR J-spectrum" ;
                 skos:definition "A two-dimensional NMR spectrum where signals are defined in terms of two frequencies; by the chemical shift of a particular nucleus in one dimension and, in the other, by the J-multiplets of correlated nuclei. [CHMO]" ;
                 skos:prefLabel "J-spectrum" .


###  http://purl.allotrope.org/ontologies/result#AFR_0000195
af-r:AFR_0000195 rdf:type owl:Class ;
                 rdfs:subClassOf af-r:AFR_0000451 ;
                 skos:changeNote "2024-09-11 Changed [OSTHUS] attribution to [Allotrope]." ;
                 skos:definition "Peaks not found along the diagonal of a 2D NMR spectrum that give yield to information on spin-spin coupling or spatial proximity of the two nuclei being observed. [Allotrope]" ;
                 skos:prefLabel "cross peak" .


###  http://purl.allotrope.org/ontologies/result#AFR_0000208
af-r:AFR_0000208 rdf:type owl:Class ;
                 rdfs:subClassOf af-r:AFR_0000263 ;
                 skos:altLabel "NOESY contour plot" ,
                               "NOESY spectra" ,
                               "NOESY spectrum" ;
                 skos:definition "A spectrum that shows the response of spin-active nuclei to radio frequency radiation in an applied magnetic field. The resonance frequencies of nuclei approximately 6 \\AA apart which are correlated by the nuclear Overhauser enhancement effect are plotted with intensities proportional to the populations of nuclei. [CHMO]" ;
                 skos:prefLabel "nuclear Overhauser enhancement spectrum" .


###  http://purl.allotrope.org/ontologies/result#AFR_0000217
af-r:AFR_0000217 rdf:type owl:Class ;
                 rdfs:subClassOf af-r:AFR_0000263 ;
                 skos:altLabel "DOSY spectrum" ,
                               "diffusion-edited NMR spectra" ,
                               "diffusion-edited NMR spectrum" ,
                               "diffusion-edited spectra" ,
                               "diffusion-edited spectrum" ,
                               "diffusion-ordered spectrum" ;
                 skos:definition "A two- or three-dimensional plot of one- or two-dimensional NMR spectra vs. the diffusion coefficients of the species involved. [CHMO]" ;
                 skos:prefLabel "diffusion-ordered spectrum" .


###  http://purl.allotrope.org/ontologies/result#AFR_0000218
af-r:AFR_0000218 rdf:type owl:Class ;
                 rdfs:subClassOf af-r:AFR_0000263 ;
                 skos:altLabel "2D NMR spectra" ,
                               "2D NMR spectrum" ,
                               "2D-NMR spectra" ,
                               "2D-NMR spectrum" ;
                 skos:definition "A two-dimensional plot of chemical shift vs. intensity for spin-active nuclei obtained by measuring the effect of the absorption of radio frequency radiation on nuclear spin-state transitions in the presence of a magnetic field. Signals are defined in terms of two frequencies; by the chemical shift of a particular nucleus in one dimension and, in the other, by the chemical shift of a correlated nucleus. [CHMO]" ;
                 skos:prefLabel "two-dimensional nuclear magnetic resonance spectrum" .


###  http://purl.allotrope.org/ontologies/result#AFR_0000239
af-r:AFR_0000239 rdf:type owl:Class ;
                 rdfs:subClassOf af-r:AFR_0000263 ;
                 skos:altLabel "1D NMR spectra" ,
                               "1D NMR spectrum" ,
                               "1D-NMR spectra" ,
                               "1D-NMR spectrum" ;
                 skos:definition "A plot of chemical shift vs. intensity for spin-active nuclei obtained by measuring the effect of the absorption of radio frequency radiation on nuclear spin-state transitions in the presence of a magnetic field. [CHMO]" ;
                 skos:prefLabel "one-dimensional nuclear magnetic resonance spectrum" .


###  http://purl.allotrope.org/ontologies/result#AFR_0000249
af-r:AFR_0000249 rdf:type owl:Class ;
                 rdfs:subClassOf af-r:AFR_0000263 ;
                 skos:altLabel "HETCOR spectrum" ;
                 skos:definition "A spectrum obtained from a heteronuclear correlation experiment. [CHMO]" ;
                 skos:prefLabel "heteronuclear correlation spectrum" .


###  http://purl.allotrope.org/ontologies/result#AFR_0000255
af-r:AFR_0000255 rdf:type owl:Class ;
                 rdfs:subClassOf af-r:AFR_0000218 ;
                 skos:altLabel "COSY NMR spectra" ,
                               "COSY NMR spectrum" ,
                               "COSY spectra" ,
                               "COSY spectrum" ;
                 skos:definition "A two-dimensional spectrum in which the position of a peak, in one dimension, corresponds to the chemical shift of a particular nucleus and, in the other dimension, to the chemical shift of a nucleus which is J-coupled to the first. [CHMO]" ;
                 skos:prefLabel "correlation spectroscopy spectrum" .


###  http://purl.allotrope.org/ontologies/result#AFR_0000264
af-r:AFR_0000264 rdf:type owl:Class ;
                 rdfs:subClassOf af-r:AFR_0000024 ;
                 skos:altLabel "NMR spectrum peak assignment target" ;
                 skos:definition "The description of the specific part a chemical moeity that is assigned to a NMR peak. [Allotrope]" ;
                 skos:example "nucleus" ;
                 skos:prefLabel "nuclear magnetic resonance spectrum peak assignment target" .


###  http://purl.allotrope.org/ontologies/result#AFR_0000283
af-r:AFR_0000283 rdf:type owl:Class ;
                 rdfs:subClassOf af-r:AFR_0000263 ;
                 skos:altLabel "DEPT NMR spectrum" ,
                               "DEPT spectrum" ;
                 skos:definition "A nuclear magnetic resonance spectrum where the where the nuclei of interest are carbon-13 nuclei, the signals from which are enhanced by the transfer of magnetisation from 1H nuclei. [CHMO]" ;
                 skos:prefLabel "distortionless enhancement with polarization transfer spectrum" .


###  http://purl.allotrope.org/ontologies/result#AFR_0000298
af-r:AFR_0000298 rdf:type owl:Class ;
                 rdfs:subClassOf af-r:AFR_0000352 ;
                 skos:altLabel "MAS QCPMG spectra" ,
                               "MAS QCPMG spectum" ,
                               "MAS-QCPMG spectra" ,
                               "MAS-QCPMG spectrum" ,
                               "QCPMG MAS spectra" ,
                               "QCPMG MAS spectrum" ,
                               "QCPMG-MAS spectra" ,
                               "QCPMG-MAS spectrum" ;
                 skos:definition "A plot of the nuclear magnetic resonance frequency vs. intensity composed of a series of peaks (separated by the reciprocal of a user-defined time delay in a QCPMG pulse sequence) which describe the envelope of the full, static spectrum. Line broadening has been averaged to zero by spinning the solid sample very rapidly at the magic angle (54.74 deg. with respect to the direction of the magnetic field). [CHMO]" ;
                 skos:prefLabel "magic-angle spinning quadrupolar Carr-Purcell-Meiboom-Gill spectrum" .


###  http://purl.allotrope.org/ontologies/result#AFR_0000352
af-r:AFR_0000352 rdf:type owl:Class ;
                 rdfs:subClassOf af-r:AFR_0000375 ;
                 skos:altLabel "QCPMG spectra" ,
                               "QCPMG spectrum" ,
                               "solid-state QCPMG spectra" ,
                               "solid-state QCPMG spectum" ;
                 skos:definition "A plot of the nuclear magnetic resonance frequency vs. intensity composed of a series of peaks (separated by the reciprocal of a user-defined time delay in a QCPMG pulse sequence) which describe the envelope of the full, static spectrum. [CHMO]" ;
                 skos:prefLabel "solid-state quadrupolar Carr-Purcell-Meiboom-Gill spectrum" .


###  http://purl.allotrope.org/ontologies/result#AFR_0000375
af-r:AFR_0000375 rdf:type owl:Class ;
                 rdfs:subClassOf af-r:AFR_0000263 ;
                 skos:altLabel "solid-state NMR spectra" ,
                               "solid-state nuclear magnetic resonance spectra" ;
                 skos:definition "A plot of the resonance frequency of nuclei in the same magnetic environment on a scale relative to their resonance frequency and with intensities proportional to the populations of nuclei in those environments for solid samples. [CHMO]" ;
                 skos:prefLabel "solid-state nuclear magnetic resonance spectrum" .


###  http://purl.allotrope.org/ontologies/result#AFR_0000407
af-r:AFR_0000407 rdf:type owl:Class ;
                 rdfs:subClassOf af-r:AFR_0000068 ;
                 skos:altLabel "NMR absorption spectra" ,
                               "NMR absorption spectrum" ,
                               "c.w. NMR spectra" ,
                               "c.w. NMR spectrum" ,
                               "continuous wave nuclear magnetic resonance spectra" ,
                               "continuous wave nuclear magnetic resonance spectrum" ,
                               "continuous-wave nuclear magnetic resonance spectra" ,
                               "cw-NMR spectra" ,
                               "cw-NMR spectrum" ;
                 skos:definition "A plot of the absorption of radio frequency radiation vs. frequency for spin-active nuclei. [CHMO]" ;
                 skos:prefLabel "continuous-wave nuclear magnetic resonance spectrum" .


###  http://purl.allotrope.org/ontologies/result#AFR_0000433
af-r:AFR_0000433 rdf:type owl:Class ;
                 rdfs:subClassOf af-r:AFR_0000208 ,
                                 af-r:AFR_0000218 ;
                 skos:altLabel "2D NOESY spectra" ,
                               "2D NOESY spectrum" ,
                               "2D NOESY-NMR spectra" ,
                               "2D NOESY-NMR spectrum" ;
                 skos:definition "A two-dimensional spectrum which plots the resonance frequency of homonuclear nuclei approximately 6 \\AA apart which are correlated by the nuclear Overhauser enhancement effect. The resonance frequencies are plotted with intensities proportional to the populations of nuclei. [CHMO]" ;
                 skos:prefLabel "two-dimensional nuclear Overhauser enhancement spectrum" .


###  http://purl.allotrope.org/ontologies/result#AFR_0000440
af-r:AFR_0000440 rdf:type owl:Class ;
                 rdfs:subClassOf af-r:AFR_0000407 ;
                 skos:altLabel "1H NMR absorption spectra" ,
                               "1H NMR absorption spectrum" ,
                               "1H c.w. NMR spectra" ,
                               "1H c.w. NMR spectrum" ,
                               "1H cw-NMR spectra" ,
                               "1H cw-NMR spectrum" ;
                 skos:definition "A plot of the absorption of radio frequency radiation vs. frequency for hydrogen-1 nuclei. [CHMO]" ;
                 skos:prefLabel "1H continuous-wave nuclear magnetic resonance spectrum" .


###  http://purl.allotrope.org/ontologies/result#AFR_0000442
af-r:AFR_0000442 rdf:type owl:Class ;
                 rdfs:subClassOf af-r:AFR_0000263 ;
                 skos:altLabel "1H NMR spectra" ,
                               "1H NMR spectrum" ,
                               "1H spectrum" ,
                               "proton NMR spectra" ,
                               "proton NMR spectrum" ;
                 skos:definition "Measurement of the effect of the absorption of radio frequency on nuclear spin-state transitions of hydrogen-1 in the presence of a magnetic field. [CHMO]" ;
                 skos:prefLabel "proton nuclear magnetic resonance spectrum" .


###  http://purl.allotrope.org/ontologies/result#AFR_0000447
af-r:AFR_0000447 rdf:type owl:Class ;
                 rdfs:subClassOf af-r:AFR_0000451 ;
                 skos:definition "Peaks found along the diagonal of a 2D NMR spectrum. [Allotrope]" ;
                 skos:prefLabel "diagonal peak" .


###  http://purl.allotrope.org/ontologies/result#AFR_0000451
af-r:AFR_0000451 rdf:type owl:Class ;
                 rdfs:subClassOf af-r:AFR_0000413 ;
                 skos:altLabel "NMR peak" ;
                 skos:definition "Peak resulting from a NMR acquisition. [Allotrope]" ;
                 skos:prefLabel "nuclear magnetic resonance peak" .


###  http://purl.allotrope.org/ontologies/result#AFR_0000476
af-r:AFR_0000476 rdf:type owl:Class ;
                 rdfs:subClassOf af-r:AFR_0000068 ;
                 skos:altLabel "FID" ;
                 skos:definition "A recorded RF signal in NMR spectroscopy observed as the perturbed sample magnetisation relaxes back to its bulk magnetisation population state. [Allotrope]" ;
                 skos:prefLabel "free induction decay" .


###  http://purl.allotrope.org/ontologies/result#AFR_0000517
af-r:AFR_0000517 rdf:type owl:Class ;
                 rdfs:subClassOf af-r:AFR_0000407 ;
                 skos:altLabel "first derivative NMR spectra" ,
                               "first derivative NMR spectrum" ;
                 skos:definition "A plot of the change in intensity of absorption vs. the change in frequency as a function of the frequency of radiation applied, for spin-active nuclei. [CHMO]" ;
                 skos:prefLabel "first derivative nuclear magnetic resonance spectrum" .


###  http://purl.allotrope.org/ontologies/result#AFR_0000521
af-r:AFR_0000521 rdf:type owl:Class ;
                 rdfs:subClassOf af-r:AFR_0000375 ;
                 skos:altLabel "MAS NMR spectrum" ,
                               "MAS spectrum" ;
                 skos:definition "A nuclear magnetic resonance spectrum in which line broadening has been averaged to zero by spinning the solid sample very rapidly at the magic angle (54.74 deg. with respect to the direction of the magnetic field). [CHMO]" ;
                 skos:prefLabel "magic angle spinning nuclear magnetic resonance spectrum" .


###  http://purl.allotrope.org/ontologies/result#AFR_0000773
af-r:AFR_0000773 rdf:type owl:Class ;
                 rdfs:subClassOf af-r:AFR_0000239 ;
                 skos:definition "Fluorine-19 nuclear magnetic resonance is an analytical technique used to identify fluorine-containing compounds. 19F is one of the most important nuclei for NMR spectroscopy. [Wikipedia]" ;
                 skos:prefLabel "one-dimensional 19F nuclear magnetic resonance spectrum" .


###  http://purl.allotrope.org/ontologies/result#AFR_0000781
af-r:AFR_0000781 rdf:type owl:Class ;
                 rdfs:subClassOf af-r:AFR_0000239 ;
                 skos:definition "Carbon-13 nuclear magnetic resonance most commonly known as carbon-13 NMR or 13C NMR or sometimes simply referred to as carbon NMR is the application of nuclear magnetic resonance (NMR) spectroscopy to carbon. It is analogous to proton NMR (1H NMR) and allows the identification of carbon atoms in an organic molecule just as proton NMR identifies hydrogen atoms. As such 13C NMR is an important tool in chemical structure elucidation in organic chemistry. 13C NMR detects only the 13C isotope of carbon, whose natural abundance is only 1.1%, because the main carbon isotope, 12C, is not detectable by NMR since it has zero net spin. [Wikipedia]" ;
                 skos:prefLabel "one-dimensional carbon 13 nuclear magnetic resonance spectrum" .


#################################################################
#    Individuals
#################################################################

###  http://purl.allotrope.org/ontologies/result#AFR_0000019
af-r:AFR_0000019 rdf:type owl:NamedIndividual ,
                          af-r:AFR_0000148 ;
                 dct:source "NMR Guidelines for ACS Journals, ACS Publications, 2013" ;
                 skos:altLabel "br" ,
                               "broad signal" ;
                 skos:definition "A NMR peak observed that is broad, usually indicating long range coupling or of exchangeable nature. [Allotrope]" ;
                 skos:prefLabel "broad" .


###  http://purl.allotrope.org/ontologies/result#AFR_0000075
af-r:AFR_0000075 rdf:type owl:NamedIndividual ,
                          af-r:AFR_0000148 ;
                 dct:source "NMR Guidelines for ACS Journals, ACS Publications, 2013" ;
                 skos:altLabel "qn" ;
                 skos:definition "A NMR peak observed as a quintet in an NMR spectrum assignable to a set of magnetically equivalent nuclei in first-order systems having two relative peak area of 1 : 4 : 6 : 4 : 1. [Allotrope]" ;
                 skos:prefLabel "quintet" .


###  http://purl.allotrope.org/ontologies/result#AFR_0000098
af-r:AFR_0000098 rdf:type owl:NamedIndividual ,
                          af-r:AFR_0000148 ;
                 dct:source "NMR Guidelines for ACS Journals, ACS Publications, 2013" ;
                 skos:altLabel "dd" ;
                 skos:definition "A common NMR peak descriptor used to represent multiplicity of the peak observed as a doublet of doublets. [Allotrope]" ;
                 skos:prefLabel "doublet of doublets" .


###  http://purl.allotrope.org/ontologies/result#AFR_0000121
af-r:AFR_0000121 rdf:type owl:NamedIndividual ,
                          af-r:AFR_0000148 ;
                 dct:source "NMR Guidelines for ACS Journals, ACS Publications, 2013" ;
                 skos:altLabel "s" ;
                 skos:definition "A single discrete isolated peak assignable to a set of magnetically equivalent nuclei of a chemical moiety. [Allotrope]" ;
                 skos:prefLabel "singlet" .


###  http://purl.allotrope.org/ontologies/result#AFR_0000124
af-r:AFR_0000124 rdf:type owl:NamedIndividual ,
                          af-r:AFR_0000148 ;
                 skos:definition "A set of non discernable non-attributable overlapping methylene NMR peaks. [Allotrope]" ;
                 skos:prefLabel "methylene envelope" .


###  http://purl.allotrope.org/ontologies/result#AFR_0000135
af-r:AFR_0000135 rdf:type owl:NamedIndividual ,
                          af-r:AFR_0000148 ;
                 dct:source "NMR Guidelines for ACS Journals, ACS Publications, 2013" ;
                 skos:altLabel "dt" ;
                 skos:definition "A common NMR peak descriptor used to represent multiplicity of the peak observed as a doublet of triplets. [Allotrope]" ;
                 skos:prefLabel "doublet of triplets" .


###  http://purl.allotrope.org/ontologies/result#AFR_0000259
af-r:AFR_0000259 rdf:type owl:NamedIndividual ,
                          af-r:AFR_0000148 ;
                 skos:altLabel "ddd" ;
                 skos:definition "A common NMR peak descriptor used to represent multiplicity of the peak observed as a doublet of doublet of doublets. [Allotrope]" ;
                 skos:prefLabel "doublet of doublet of doublets" .


###  http://purl.allotrope.org/ontologies/result#AFR_0000277
af-r:AFR_0000277 rdf:type owl:NamedIndividual ,
                          af-r:AFR_0000148 ;
                 skos:altLabel "sept" ;
                 skos:definition "A NMR peak observed as a septet in an NMR spectrum assignable to a set of magnetically equivalent nuclei in first-order systems having two relative peak area of 1 : 6 : 15 : 20 : 15 : 6 : 1. [Allotrope]" ;
                 skos:prefLabel "septet" .


###  http://purl.allotrope.org/ontologies/result#AFR_0000302
af-r:AFR_0000302 rdf:type owl:NamedIndividual ,
                          af-r:AFR_0000148 ;
                 skos:altLabel "ddt" ;
                 skos:definition "A common NMR peak descriptor used to represent multiplicity of the peak observed as a doublet of doublet of triplets. [Allotrope]" ;
                 skos:prefLabel "doublet of doublet of triplets" .


###  http://purl.allotrope.org/ontologies/result#AFR_0000315
af-r:AFR_0000315 rdf:type owl:NamedIndividual ,
                          af-r:AFR_0000148 ;
                 skos:altLabel "sex" ;
                 skos:definition "A NMR peak observed as a sextet in an NMR spectrum assignable to a set of magnetically equivalent nuclei in first-order systems having two relative peak area of 1 : 5 : 10 : 10 : 5 : 1. [Allotrope]" ;
                 skos:prefLabel "sextet" .


###  http://purl.allotrope.org/ontologies/result#AFR_0000335
af-r:AFR_0000335 rdf:type owl:NamedIndividual ,
                          af-r:AFR_0000148 ;
                 dct:source "NMR Guidelines for ACS Journals, ACS Publications, 2013" ;
                 skos:altLabel "m" ,
                               "mult" ;
                 skos:definition "A non discernable peak or set of overlapping peaks observed in an NMR spectra. [Allotrope]" ;
                 skos:prefLabel "multiplet" .


###  http://purl.allotrope.org/ontologies/result#AFR_0000408
af-r:AFR_0000408 rdf:type owl:NamedIndividual ,
                          af-r:AFR_0000148 ;
                 skos:altLabel "oct" ;
                 skos:definition "A NMR peak observed as a octet in an NMR spectrum assignable to a set of magnetically equivalent nuclei in first-order systems having two relative peak area of 1 : 7 : 21 : 35 : 35 : 21 : 7 : 1. [Allotrope]" ;
                 skos:prefLabel "octet" .


###  http://purl.allotrope.org/ontologies/result#AFR_0000431
af-r:AFR_0000431 rdf:type owl:NamedIndividual ,
                          af-r:AFR_0000148 ;
                 dct:source "NMR Guidelines for ACS Journals, ACS Publications, 2013" ;
                 skos:altLabel "tt" ;
                 skos:definition "A common NMR peak descriptor used to represent multiplicity of the peak observed as a triplet of triplets. [Allotrope]" ;
                 skos:prefLabel "triplet of triplets" .


###  http://purl.allotrope.org/ontologies/result#AFR_0000460
af-r:AFR_0000460 rdf:type owl:NamedIndividual ,
                          af-r:AFR_0000148 ;
                 dct:source "NMR Guidelines for ACS Journals, ACS Publications, 2013" ;
                 skos:altLabel "d" ;
                 skos:definition "A NMR peak observed as a doublet in an NMR spectrum assignable to a set of magnetically equivalent nuclei in first-order systems having two relative peak area of 1 : 1. [Allotrope]" ;
                 skos:prefLabel "doublet" .


###  http://purl.allotrope.org/ontologies/result#AFR_0000503
af-r:AFR_0000503 rdf:type owl:NamedIndividual ,
                          af-r:AFR_0000148 ;
                 dct:source "NMR Guidelines for ACS Journals, ACS Publications, 2013" ;
                 skos:altLabel "q" ;
                 skos:definition "An NMR peak observed as a quartet in an NMR spectrum assignable to a set of magnetically equivalent nuclei in first-order systems having two relative peak area of 1 : 3 : 3 : 1. [Allotrope]" ;
                 skos:prefLabel "quartet" .


###  http://purl.allotrope.org/ontologies/result#AFR_0000505
af-r:AFR_0000505 rdf:type owl:NamedIndividual ,
                          af-r:AFR_0000148 ;
                 dct:source "NMR Guidelines for ACS Journals, ACS Publications, 2013" ;
                 skos:altLabel "t" ;
                 skos:definition "A NMR peak observed as a triplet in an NMR spectrum assignable to a set of magnetically equivalent nuclei in first-order systems having two relative peak area of 1 : 2 : 1. [Allotrope]" ;
                 skos:prefLabel "triplet" .


###  http://purl.allotrope.org/ontologies/result#AFR_0000511
af-r:AFR_0000511 rdf:type owl:NamedIndividual ,
                          af-r:AFR_0000148 ;
                 skos:altLabel "dddd" ;
                 skos:definition "A common NMR peak descriptor used to represent multiplicity of the peak observed as a doublet of doublet of doublet of doublets. [Allotrope]" ;
                 skos:prefLabel "doublet of doublet of doublet of doublets" .


###  http://purl.allotrope.org/ontologies/result#AFR_0000520
af-r:AFR_0000520 rdf:type owl:NamedIndividual ,
                          af-r:AFR_0000148 ;
                 skos:altLabel "non" ;
                 skos:definition "A NMR peak observed as a nonet in an NMR spectrum assignable to a set of magnetically equivalent nuclei in first-order systems having two relative peak area of 1 : 8 : 28 : 56 : 70 : 56 : 28 : 8 : 1. [Allotrope]" ;
                 skos:prefLabel "nonet" .


###  http://purl.allotrope.org/ontologies/result#AFR_0000786
af-r:AFR_0000786 rdf:type owl:NamedIndividual ,
                          af-r:AFR_0000148 ;
                 dct:source "NMR Guidelines for ACS Journals, ACS Publications, 2013" ;
                 skos:altLabel "td" ;
                 skos:definition "A common NMR peak descriptor used to represent multiplicity of the peak observed as a triplet of doublets. [Allotrope]" ;
                 skos:prefLabel "triplet of doublets" .


###  http://purl.allotrope.org/voc/attribution
<http://purl.allotrope.org/voc/attribution> rdf:type owl:NamedIndividual ,
                                                     dct:RightsStatement ;
                                            dct:description """
These taxonomies contain material or may constitute derivative works of material which may be subject to copyright by one of the following organizations.  By using these taxonomies, you agree to the following terms and conditions applicable to its contents:
******************************************************************************
Copyright Notice and Terms for IUPAC Gold Book
______________________________________________________________________________
Copyright  1998, Regents of the University of California
All rights reserved.
Redistribution and use in source and binary forms, with or without modification, are permitted provided that the following conditions are met:
1. Redistributions of source code must retain the above copyright notice, this list of conditions and the following disclaimer.
2. Redistributions in binary form must reproduce the above copyright notice, this list of conditions and the following disclaimer in the documentation and/or other materials provided with the distribution.
THIS SOFTWARE IS PROVIDED BY THE COPYRIGHT HOLDERS AND CONTRIBUTORS \"AS IS\" AND ANY EXPRESS OR IMPLIED WARRANTIES, INCLUDING, BUT NOT LIMITED TO, THE IMPLIED WARRANTIES OF MERCHANTABILITY AND FITNESS FOR A PARTICULAR PURPOSE ARE DISCLAIMED. IN NO EVENT SHALL THE COPYRIGHT HOLDER OR CONTRIBUTORS BE LIABLE FOR ANY DIRECT, INDIRECT, INCIDENTAL, SPECIAL, EXEMPLARY, OR CONSEQUENTIAL DAMAGES (INCLUDING, BUT NOT LIMITED TO, PROCUREMENT OF SUBSTITUTE GOODS OR SERVICES; LOSS OF USE, DATA, OR PROFITS; OR BUSINESS INTERRUPTION) HOWEVER CAUSED AND ON ANY THEORY OF LIABILITY, WHETHER IN CONTRACT, STRICT LIABILITY, OR TORT (INCLUDING NEGLIGENCE OR OTHERWISE) ARISING IN ANY WAY OUT OF THE USE OF THIS SOFTWARE, EVEN IF ADVISED OF THE POSSIBILITY OF SUCH DAMAGE.
******************************************************************************
Copyright Notice and Terms for PSI-MS (Proteomics Standards Initiative - Mass Spectrometry) Mass spectrometer output files and spectra interpretation
_____________________________________________________________________________
Created by Matt Chambers, Andreas Bertsch, Marius Kallhardt, Eric Deutsch Fredrik Levander, Pierre-Alain Binz, and Gerhard Mayer. Publisher: HUPO Proteomics Standards Initiative Mass Spectrometry Standards Working Group and HUPO Proteomics Standards Initiative Proteomics Informatics Working Group. This work is used pursuant to a Creative Commons license available here: http://creativecommons.org/licenses/by/3.0/legalcode

******************************************************************************
Attribution Notice for National Center for Biomedical Ontology materials.

This work contains material from the Cell Ontology and Clinical Measurement Ontology, available here: http://bioportal.bioontology.org/.
******************************************************************************
Attribution Notice for ChEBI
This work contains material from the European Bioinformatics Institutes ChEBI database.
******************************************************************************
Attribution Notice for Quantities Units Dimensions Data Types (http://www.qudt.org/)
This work contains content from www.qudt.org and is used pursuant to a Creative Commons License available here: http://creativecommons.org/licenses/by-sa/3.0/us/legalcode. The original work may have been modified.
******************************************************************************
Copyright and Attribution Notice for Dublin Core Metadata Initiative Document
This work contains material from the following DCMI document used pursuant to a creative commons license available here: https://creativecommons.org/licenses/by/4.0/legalcode. This material may have been modified or changed.
Timestamped URL:          http://dublincore.org/documents/2012/06/14/dcmi-terms/
Date Issued:                       2012-06-14
Document Status:            This is a DCMI Recommendation.
Copyright  1995-2015 DCMI. All Rights Reserved. DCMI liability, trademark/service mark, document use and software licensing rules apply.
******************************************************************************

""" ;
                                            dct:title "Derivative works attribution" .


###  http://purl.allotrope.org/voc/copyright
<http://purl.allotrope.org/voc/copyright> rdf:type owl:NamedIndividual ,
                                                   dct:RightsStatement ;
                                          dct:description " 2020 Allotrope Foundation" ;
                                          dct:title " 2020 Allotrope Foundation" .


###  http://purl.allotrope.org/voc/creative-commons-attribution-license
<http://purl.allotrope.org/voc/creative-commons-attribution-license> rdf:type owl:NamedIndividual ,
                                                                              dct:LicenseDocument ;
                                                                     dct:description """This work is licensed under a Creative Commons Attribution 4.0 International License http://creativecommons.org/licenses/by/4.0/.

THESE MATERIALS ARE PROVIDED \"AS IS\" AND ALLOTROPE EXPRESSLY DISCLAIMS ALL WARRANTIES, EXPRESS, IMPLIED OR STATUTORY, INCLUDING, WITHOUT LIMITATION, THE WARRANTIES OF NON-INFRINGEMENT, TITLE, MERCHANTABILITY AND FITNESS FOR A PARTICULAR PURPOSE.

Copyright  2015-2025 Allotrope Foundation
""" ;
                                                                     dct:rightsHolder <http://www.allotrope.org> ;
                                                                     dct:title "Creative Commons Attribution 4.0 International Public License" .


###  Generated by the OWL API (version 5.1.19) https://github.com/owlcs/owlapi/
