@prefix : <http://purl.allotrope.org/voc/afo/domain/WD/2025/06/ph#> .
@prefix dct: <http://purl.org/dc/terms/> .
@prefix owl: <http://www.w3.org/2002/07/owl#> .
@prefix rdf: <http://www.w3.org/1999/02/22-rdf-syntax-ns#> .
@prefix xml: <http://www.w3.org/XML/1998/namespace> .
@prefix xsd: <http://www.w3.org/2001/XMLSchema#> .
@prefix af-c: <http://purl.allotrope.org/ontologies/common#> .
@prefix af-e: <http://purl.allotrope.org/ontologies/equipment#> .
@prefix af-m: <http://purl.allotrope.org/ontologies/material#> .
@prefix af-p: <http://purl.allotrope.org/ontologies/process#> .
@prefix af-q: <http://purl.allotrope.org/ontologies/quality#> .
@prefix af-r: <http://purl.allotrope.org/ontologies/result#> .
@prefix af-x: <http://purl.allotrope.org/ontologies/property#> .
@prefix rdfs: <http://www.w3.org/2000/01/rdf-schema#> .
@prefix skos: <http://www.w3.org/2004/02/skos/core#> .
@prefix af-cur: <http://purl.allotrope.org/ontologies/curation#> .
@base <http://purl.allotrope.org/voc/afo/domain/WD/2025/06/ph#> .

<http://purl.allotrope.org/voc/afo/domain/WD/2025/06/ph> rdf:type owl:Ontology ;
                                                                    owl:versionIRI <http://purl.allotrope.org/voc/afo/domain/WD/2025/06/ph> ;
                                                                    owl:imports <http://purl.allotrope.org/voc/afo/WD/2025/06/afo> ,
                                                                                <http://purl.allotrope.org/voc/afo/domain/REC/2025/06/ph> ,
                                                                                <http://purl.allotrope.org/voc/afo/domain/WD/2025/06/electrochemistry> ,
                                                                                <http://purl.allotrope.org/voc/afo/domain/WD/2025/06/titration> ;
                                                                    dct:issued "2025-06-25T12:00:00Z"^^xsd:dateTime ;
                                                                    dct:license <http://purl.allotrope.org/voc/creative-commons-attribution-license> ;
                                                                    dct:modified "2025-04-04T12:00:00Z"^^xsd:dateTime ;
                                                                    dct:rights <http://purl.allotrope.org/voc/attribution> ,
                                                                               <http://purl.allotrope.org/voc/copyright> ;
                                                                    dct:title "AFO pH Domain Ontology (WD/2025/06)" ;
                                                                    owl:priorVersion <http://purl.allotrope.org/voc/afo/domain/WD/2018/11/ph> ;
                                                                    owl:versionInfo "WD/2025/06" .

#################################################################
#    Annotation properties
#################################################################

###  http://purl.allotrope.org/ontologies/property#AFX_0002796
af-x:AFX_0002796 rdf:type owl:AnnotationProperty .


###  http://purl.allotrope.org/ontologies/property#AFX_0002798
af-x:AFX_0002798 rdf:type owl:AnnotationProperty .


###  http://purl.allotrope.org/ontologies/property#AFX_0002809
af-x:AFX_0002809 rdf:type owl:AnnotationProperty .


###  http://purl.org/dc/terms/source
dct:source rdf:type owl:AnnotationProperty .


###  http://www.w3.org/2004/02/skos/core#altLabel
skos:altLabel rdf:type owl:AnnotationProperty .


###  http://www.w3.org/2004/02/skos/core#changeNote
skos:changeNote rdf:type owl:AnnotationProperty .


###  http://www.w3.org/2004/02/skos/core#definition
skos:definition rdf:type owl:AnnotationProperty .


###  http://www.w3.org/2004/02/skos/core#example
skos:example rdf:type owl:AnnotationProperty .


###  http://www.w3.org/2004/02/skos/core#note
skos:note rdf:type owl:AnnotationProperty .


###  http://www.w3.org/2004/02/skos/core#prefLabel
skos:prefLabel rdf:type owl:AnnotationProperty .


###  http://www.w3.org/2004/02/skos/core#scopeNote
skos:scopeNote rdf:type owl:AnnotationProperty .


#################################################################
#    Object Properties
#################################################################

###  http://purl.allotrope.org/ontologies/property#AFX_0000051
af-x:AFX_0000051 rdf:type owl:ObjectProperty ;
                 dct:license <http://purl.allotrope.org/voc/iupac-license> ;
                 dct:rights <http://purl.allotrope.org/voc/iupac-copyright> ;
                 dct:source "Green Book, 3rd ed.: IUPAC Quantities, Units and Symbols in Physical Chemistry. Third Edition, RSC Publishing, Cambridge 2007." ,
                            "PAC, 1996, 68, 957 (Glossary of terms in quantities and units in Clinical Chemistry (IUPAC-IFCC Recommendations 1996))" ,
                            "PAC, 1997, 69, 1007 (Reference value standards and primary standards for pH measurements in D2O and aqueousorganic solvent mixtures: New accessions and assessments (Technical Report))" ;
                 rdfs:seeAlso "PAC, 1984, 56, 567 (Physicochemical quantities and units in clinical chemistry with special emphasis on activities and activity coefficients (Recommendations 1983)" ,
                              "PAC, 1990, 62, 2167 (Glossary of atmospheric chemistry terms (Recommendations 1990))" ,
                              "PAC, 2002, 74, 2169 (Measurement of pH. Definition, standards, and procedures (IUPAC Recommendations 2002))" ;
                 skos:changeNote "2024-09-12 Changed [IUPAC Gold Book] attribution to [IUPAC] and added license and rights fields." ;
                 skos:definition "The quantity pH is defined in terms of the activity of hydrogen(1+) ions (hydrogen ions) in solution: pH = − lg[a(H+)] = − lg [m(H+) γ_m(H+) / m0], where a(H+) is the activity of hydrogen ion (hydrogen 1+) in aqueous solution, H+(aq), γ_m(H+) is the activity coefficient of H+(aq) (molality basis) at molality m(H+), and m0 = 1 mol kg −1 is the standard molality. [IUPAC]" ;
                 skos:prefLabel "pH" .


###  http://purl.allotrope.org/ontologies/property#AFX_0000052
af-x:AFX_0000052 rdf:type owl:ObjectProperty ;
                 rdfs:subPropertyOf af-x:AFX_0000051 ;
                 skos:altLabel "pH" ;
                 skos:definition "The pH value of a calibration point. [Allotrope]" ;
                 skos:prefLabel "pH of calibration point" .


###  http://purl.allotrope.org/ontologies/property#AFX_0000053
af-x:AFX_0000053 rdf:type owl:ObjectProperty ;
                 rdfs:subPropertyOf af-x:AFX_0000051 ;
                 skos:definition "The pH value at a given temperature. [Allotrope]" ;
                 skos:example "Nova Flex pH at temp" ;
                 skos:prefLabel "pH at temperature" .


###  http://purl.allotrope.org/ontologies/property#AFX_0000067
af-x:AFX_0000067 rdf:type owl:ObjectProperty ;
                 rdfs:subPropertyOf af-x:AFX_0000051 ;
                 skos:definition "The temperature compensated pH is the calculated pH accounting for error due to a sample's temperature. [Allotrope]" ;
                 skos:prefLabel "temperature compensated pH" .


#################################################################
#    Classes
#################################################################

###  http://purl.allotrope.org/ontologies/equipment#AFE_0000237
af-e:AFE_0000237 rdf:type owl:Class ;
                 rdfs:subClassOf af-e:AFE_0000351 ;
                 skos:altLabel "pH glass electrode" ;
                 skos:changeNote "2016-02-02 Add harmonized property restrictions [OSTHUS]" ,
                                 "2024-09-12 Remove [GENE] attribution as this is purely [CHMO]." ;
                 skos:definition "A hydrogen-ion-responsive electrode consisting of a piece, usually a bulb, of special glass attached to a stem of high-resistance glass complete with internal reference electrode and internal filling solution system. [CHMO]" ;
                 skos:prefLabel "glass electrode" .


###  http://purl.allotrope.org/ontologies/equipment#AFE_0000351
af-e:AFE_0000351 rdf:type owl:Class ;
                 rdfs:subClassOf af-e:AFE_0000422 ;
                 skos:altLabel "pH analyser"@en-gb ,
                               "pH analyzer" ,
                               "pH sensor" ;
                 skos:changeNote "2017-10-25 Changed pref label to reflect taxonomy better [OSTHUS]" ;
                 skos:definition "The pH sensor is able to detect the amount of free hydrogen ions in a sample. [Allotrope]" ;
                 skos:prefLabel "pH electrode" .


###  http://purl.allotrope.org/ontologies/equipment#AFE_0000414
af-e:AFE_0000414 rdf:type owl:Class ;
                 rdfs:subClassOf af-e:AFE_0000115 ;
                 skos:definition "An electrochemical cell which is used for practical pH measurements, consisting of a hydrogen ion-responsive electrode and a reference electrode immersed in the test solution. [CHMO]" ;
                 skos:prefLabel "operational pH cell" .


###  http://purl.allotrope.org/ontologies/equipment#AFE_0000869
af-e:AFE_0000869 rdf:type owl:Class ;
                 rdfs:subClassOf af-e:AFE_0000351 ;
                 skos:changeNote "2016-02-02 add harmonized property restrictions [OSTHUS]" ;
                 skos:definition "The quinhydrone electrode is a type of redox electrode which can be used to measure the hydrogen ion concentration (pH) of a solution in a chemical experiment. It provides an alternative to the commonly used glass electrode in a pH meter. [Wikipedia]" ;
                 skos:prefLabel "quinhydrone electrode" .


###  http://purl.allotrope.org/ontologies/material#AFM_0000084
af-m:AFM_0000084 rdf:type owl:Class ;
                 rdfs:subClassOf af-m:AFM_0000015 ,
                                 af-m:AFM_0000133 ;
                 af-x:AFX_0002796 af-r:AFR_0001223 ;
                 skos:altLabel "pH calibration solution" ;
                 skos:definition "A pH calibration buffer provides a calibration point for pH calibrations. [Allotrope]" ;
                 skos:example "The 7.382 and 6.838 buffers are buffered to those specific pH's at 37Â°C and are NIST traceable." ;
                 skos:prefLabel "pH calibration buffer" .


###  http://purl.allotrope.org/ontologies/material#AFM_0000278
af-m:AFM_0000278 rdf:type owl:Class ;
                 rdfs:subClassOf af-m:AFM_0000133 ;
                 af-x:AFX_0002796 af-r:AFR_0001223 ;
                 dct:license <http://purl.allotrope.org/voc/iupac-license> ;
                 dct:rights <http://purl.allotrope.org/voc/iupac-copyright> ;
                 dct:source "PAC, 1985, 57, 531. (Definition of pH scales, standard reference values, measurement of pH and related terminology (Recommendations 1984)) on page 541" ;
                 skos:changeNote "2024-09-12 Changed [IUPAC Recommendations 2002] attribution to [IUPAC] and added license, rights, and source fields." ;
                 skos:definition "Values that may be assigned to secondary standard pH solutions at each temperature with reference to pH values of a primary standard of the same nominal composition. [IUPAC]" ;
                 skos:prefLabel "secondary pH standard" .


###  http://purl.allotrope.org/ontologies/process#AFP_0000195
af-p:AFP_0000195 rdf:type owl:Class ;
                 rdfs:subClassOf af-p:AFP_0002389 ;
                 skos:changeNote "2016-02-02 Add harmonized property restrictions [OSTHUS]" ;
                 skos:definition "Calibration of a pH meter using special data point positions. [Allotrope]" ;
                 skos:prefLabel "pH meter calibration" .


###  http://purl.allotrope.org/ontologies/result#AFR_0000025
af-r:AFR_0000025 rdf:type owl:Class ;
                 rdfs:subClassOf af-r:AFR_0000207 ;
                 skos:changeNote "2016-02-02 Add harmonized property restrictions [OSTHUS]" ;
                 skos:definition "A pH measurement result is the outcome of a the process of pH measurement. [Allotrope]" ;
                 skos:prefLabel "pH measurement result" .


###  http://purl.allotrope.org/ontologies/result#AFR_0000101
af-r:AFR_0000101 rdf:type owl:Class ;
                 rdfs:subClassOf af-r:AFR_0000490 ;
                 skos:changeNote "2016-02-02 Add harmonized property restrictions [OSTHUS]" ;
                 skos:definition "The pH titration curve contains the volume of the titrant as the independent variable and the pH of the solution as the dependent variable (because it changes depending on the composition of the two solutions). [Wikipedia]" ;
                 skos:prefLabel "pH titration curve" .


###  http://purl.allotrope.org/ontologies/result#AFR_0002289
af-r:AFR_0002289 rdf:type owl:Class ;
                 rdfs:subClassOf af-r:AFR_0001217 ;
                 dct:replaces af-p:AFP_0002302 ;
                 skos:changeNote "2020-12-17 Replaces deprecated term af-p:AFP_0002302 [Allotrope]" ;
                 skos:definition "A calibration point in a pH meter calibration. [Allotrope]" ;
                 skos:prefLabel "pH meter calibration point" .


#################################################################
#    Individuals
#################################################################

###  http://purl.allotrope.org/voc/attribution
<http://purl.allotrope.org/voc/attribution> rdf:type owl:NamedIndividual ,
                                                     dct:RightsStatement ;
                                            dct:description """
These taxonomies contain material or may constitute derivative works of material which may be subject to copyright by one of the following organizations.  By using these taxonomies, you agree to the following terms and conditions applicable to its contents:
******************************************************************************
Copyright Notice and Terms for IUPAC Gold Book
______________________________________________________________________________
Copyright © 1998, Regents of the University of California
All rights reserved.
Redistribution and use in source and binary forms, with or without modification, are permitted provided that the following conditions are met:
1. Redistributions of source code must retain the above copyright notice, this list of conditions and the following disclaimer.
2. Redistributions in binary form must reproduce the above copyright notice, this list of conditions and the following disclaimer in the documentation and/or other materials provided with the distribution.
THIS SOFTWARE IS PROVIDED BY THE COPYRIGHT HOLDERS AND CONTRIBUTORS \"AS IS\" AND ANY EXPRESS OR IMPLIED WARRANTIES, INCLUDING, BUT NOT LIMITED TO, THE IMPLIED WARRANTIES OF MERCHANTABILITY AND FITNESS FOR A PARTICULAR PURPOSE ARE DISCLAIMED. IN NO EVENT SHALL THE COPYRIGHT HOLDER OR CONTRIBUTORS BE LIABLE FOR ANY DIRECT, INDIRECT, INCIDENTAL, SPECIAL, EXEMPLARY, OR CONSEQUENTIAL DAMAGES (INCLUDING, BUT NOT LIMITED TO, PROCUREMENT OF SUBSTITUTE GOODS OR SERVICES; LOSS OF USE, DATA, OR PROFITS; OR BUSINESS INTERRUPTION) HOWEVER CAUSED AND ON ANY THEORY OF LIABILITY, WHETHER IN CONTRACT, STRICT LIABILITY, OR TORT (INCLUDING NEGLIGENCE OR OTHERWISE) ARISING IN ANY WAY OUT OF THE USE OF THIS SOFTWARE, EVEN IF ADVISED OF THE POSSIBILITY OF SUCH DAMAGE.
******************************************************************************
Copyright Notice and Terms for PSI-MS (Proteomics Standards Initiative - Mass Spectrometry) Mass spectrometer output files and spectra interpretation
_____________________________________________________________________________
Created by Matt Chambers, Andreas Bertsch, Marius Kallhardt, Eric Deutsch Fredrik Levander, Pierre-Alain Binz, and Gerhard Mayer. Publisher: HUPO Proteomics Standards Initiative Mass Spectrometry Standards Working Group and HUPO Proteomics Standards Initiative Proteomics Informatics Working Group. This work is used pursuant to a Creative Commons license available here: http://creativecommons.org/licenses/by/3.0/legalcode

******************************************************************************
Attribution Notice for National Center for Biomedical Ontology materials.

This work contains material from the Cell Ontology and Clinical Measurement Ontology, available here: http://bioportal.bioontology.org/.
******************************************************************************
Attribution Notice for ChEBI
This work contains material from the European Bioinformatics Institute’s ChEBI database.
******************************************************************************
Attribution Notice for Quantities Units Dimensions Data Types (http://www.qudt.org/)
This work contains content from www.qudt.org and is used pursuant to a Creative Commons License available here: http://creativecommons.org/licenses/by-sa/3.0/us/legalcode. The original work may have been modified.
******************************************************************************
Copyright and Attribution Notice for Dublin Core Metadata Initiative Document
This work contains material from the following DCMI document used pursuant to a creative commons license available here: https://creativecommons.org/licenses/by/4.0/legalcode. This material may have been modified or changed.
Timestamped URL:          http://dublincore.org/documents/2012/06/14/dcmi-terms/
Date Issued:                       2012-06-14
Document Status:            This is a DCMI Recommendation.
Copyright © 1995-2015 DCMI. All Rights Reserved. DCMI liability, trademark/service mark, document use and software licensing rules apply.
******************************************************************************

""" ;
                                            dct:title "Derivative works attribution" .


###  http://purl.allotrope.org/voc/copyright
<http://purl.allotrope.org/voc/copyright> rdf:type owl:NamedIndividual ,
                                                   dct:RightsStatement ;
                                          dct:description "Copyright © 2019 Allotrope Foundation" ;
                                          dct:rightsHolder <http://www.allotrope.org> ;
                                          dct:title "Copyright © 2019 Allotrope Foundation" .


###  http://purl.allotrope.org/voc/creative-commons-attribution-license
<http://purl.allotrope.org/voc/creative-commons-attribution-license> rdf:type owl:NamedIndividual ,
                                                                              dct:LicenseDocument ;
                                                                     dct:description """This work is licensed under a Creative Commons Attribution 4.0 International License http://creativecommons.org/licenses/by/4.0/.

THESE MATERIALS ARE PROVIDED \"AS IS\" AND ALLOTROPE EXPRESSLY DISCLAIMS ALL WARRANTIES, EXPRESS, IMPLIED OR STATUTORY, INCLUDING, WITHOUT LIMITATION, THE WARRANTIES OF NON-INFRINGEMENT, TITLE, MERCHANTABILITY AND FITNESS FOR A PARTICULAR PURPOSE.

Copyright © 2015-2025 Allotrope Foundation
""" ;
                                                                     dct:title "Creative Commons Attribution 4.0 International Public License" .


###  Generated by the OWL API (version 5.1.19) https://github.com/owlcs/owlapi/
