@prefix : <http://purl.allotrope.org/voc/afo/domain/WD/2025/06/property-coordination#> .
@prefix cl: <http://purl.obolibrary.org/obo/CL> .
@prefix go: <http://purl.obolibrary.org/obo/GO> .
@prefix ro: <http://purl.obolibrary.org/obo/RO> .
@prefix bfo: <http://purl.obolibrary.org/obo/BFO> .
@prefix dct: <http://purl.org/dc/terms/> .
@prefix iao: <http://purl.obolibrary.org/obo/IAO> .
@prefix obi: <http://purl.obolibrary.org/obo/OBI> .
@prefix owl: <http://www.w3.org/2002/07/owl#> .
@prefix rdf: <http://www.w3.org/1999/02/22-rdf-syntax-ns#> .
@prefix xml: <http://www.w3.org/XML/1998/namespace> .
@prefix xsd: <http://www.w3.org/2001/XMLSchema#> .
@prefix af-c: <http://purl.allotrope.org/ontologies/common#> .
@prefix af-e: <http://purl.allotrope.org/ontologies/equipment#> .
@prefix af-m: <http://purl.allotrope.org/ontologies/material#> .
@prefix af-p: <http://purl.allotrope.org/ontologies/process#> .
@prefix af-q: <http://purl.allotrope.org/ontologies/quality#> .
@prefix af-r: <http://purl.allotrope.org/ontologies/result#> .
@prefix af-x: <http://purl.allotrope.org/ontologies/property#> .
@prefix chmo: <http://purl.obolibrary.org/obo/CHMO> .
@prefix rdfs: <http://www.w3.org/2000/01/rdf-schema#> .
@prefix skos: <http://www.w3.org/2004/02/skos/core#> .
@prefix af-cq: <http://purl.allotrope.org/ontologies/common/qualifier#> .
@prefix af-fn: <http://purl.allotrope.org/ontologies/function#> .
@prefix af-re: <http://purl.allotrope.org/ontologies/realizable#> .
@prefix af-rl: <http://purl.allotrope.org/ontologies/role#> .
@prefix af-cur: <http://purl.allotrope.org/ontologies/curation#> .
@base <http://purl.allotrope.org/voc/afo/domain/WD/2025/06/property-coordination#> .

<http://purl.allotrope.org/voc/afo/domain/WD/2025/06/property-coordination> rdf:type owl:Ontology ;
                                                                                       owl:versionIRI <http://purl.allotrope.org/voc/afo/domain/WD/2025/06/property-coordination> ;
                                                                                       owl:imports <http://purl.allotrope.org/voc/afo/WD/2025/06/afo> ;
                                                                                       dct:description "AFT 1.1.5 legacy, will be removed" ;
                                                                                       dct:issued "2025-06-25T12:00:00Z"^^xsd:dateTime ;
                                                                                       dct:license <http://purl.allotrope.org/voc/creative-commons-attribution-license> ;
                                                                                       dct:modified "2025-04-04T12:00:00Z"^^xsd:dateTime ;
                                                                                       dct:rights <http://purl.allotrope.org/voc/attribution> ,
                                                                                                  <http://purl.allotrope.org/voc/copyright> ;
                                                                                       dct:rightsHolder <http://www.allotrope.org> ;
                                                                                       dct:title "AFO Property Coordination Domain Ontology (WD/2025/06)" ;
                                                                                       owl:priorVersion <http://purl.allotrope.org/voc/afo/domain/WD/2025/03/property-coordination> ;
                                                                                       owl:versionInfo "WD/2025/06" .

#################################################################
#    Annotation properties
#################################################################

###  http://purl.allotrope.org/ontologies/property#AFX_0002796
af-x:AFX_0002796 rdf:type owl:AnnotationProperty .


###  http://purl.allotrope.org/ontologies/property#AFX_0002798
af-x:AFX_0002798 rdf:type owl:AnnotationProperty .


###  http://purl.allotrope.org/ontologies/property#AFX_0002809
af-x:AFX_0002809 rdf:type owl:AnnotationProperty .


###  http://purl.org/dc/terms/source
dct:source rdf:type owl:AnnotationProperty .


###  http://www.w3.org/2004/02/skos/core#altLabel
skos:altLabel rdf:type owl:AnnotationProperty .


###  http://www.w3.org/2004/02/skos/core#changeNote
skos:changeNote rdf:type owl:AnnotationProperty .


###  http://www.w3.org/2004/02/skos/core#definition
skos:definition rdf:type owl:AnnotationProperty .


###  http://www.w3.org/2004/02/skos/core#example
skos:example rdf:type owl:AnnotationProperty .


###  http://www.w3.org/2004/02/skos/core#note
skos:note rdf:type owl:AnnotationProperty .


###  http://www.w3.org/2004/02/skos/core#prefLabel
skos:prefLabel rdf:type owl:AnnotationProperty .


###  http://www.w3.org/2004/02/skos/core#scopeNote
skos:scopeNote rdf:type owl:AnnotationProperty .


#################################################################
#    Classes
#################################################################

###  http://purl.allotrope.org/ontologies/common#AFC_0000108
af-c:AFC_0000108 rdf:type owl:Class ;
                 rdfs:subClassOf af-r:AFR_0001277 ;
                 skos:definition "Property coordination is a coordination of a property term with one or more terms to narrow the meaning. [Allotrope]" ;
                 skos:prefLabel "property coordination" .


###  http://purl.allotrope.org/ontologies/common#AFC_0000109
af-c:AFC_0000109 rdf:type owl:Class ;
                 rdfs:subClassOf af-r:AFR_0001277 ;
                 skos:definition "A property qualifier is a term that narrows the meaning of a more general property term in a certain aspect or context. [Allotrope]" ;
                 skos:prefLabel "property qualifier" .


###  http://purl.allotrope.org/ontologies/common#AFC_0000111
af-c:AFC_0000111 rdf:type owl:Class ;
                 rdfs:subClassOf af-c:AFC_0000109 ;
                 skos:definition "The statistical qualifier in a property coordination indicates the way the value of the property is derived from statistics. [Allotrope]" ;
                 skos:prefLabel "statistical qualifier" .


###  http://purl.allotrope.org/ontologies/common#AFC_0000145
af-c:AFC_0000145 rdf:type owl:Class ;
                 rdfs:subClassOf af-c:AFC_0000109 ;
                 skos:definition "The measurement qualifier in a property coordination indicates the way the value of the property is acquired or derived. [Allotrope]" ;
                 skos:prefLabel "measurement qualifier" .


###  http://purl.allotrope.org/ontologies/common#AFC_0000147
af-c:AFC_0000147 rdf:type owl:Class ;
                 rdfs:subClassOf af-c:AFC_0000109 ;
                 skos:definition "A boundary qualifier in the property coordination indicates limits on the values of properties. [Allotrope]" ;
                 skos:prefLabel "boundary qualifier" .


###  http://purl.allotrope.org/ontologies/common#AFC_0000148
af-c:AFC_0000148 rdf:type owl:Class ;
                 rdfs:subClassOf af-c:AFC_0000109 ;
                 skos:definition "Temporal qualifiers indicate a point in time of some temporal context. [Allotrope]" ;
                 skos:prefLabel "temporal qualifier" .


###  http://purl.allotrope.org/ontologies/common#AFC_0000152
af-c:AFC_0000152 rdf:type owl:Class ;
                 rdfs:subClassOf af-c:AFC_0000109 ;
                 skos:definition "An intention qualifier indicates an intention or purpose of the property in the context of the property coordination. [Allotrope]" ;
                 skos:prefLabel "intention qualifier" .


###  http://purl.org/dc/terms/LicenseDocument
dct:LicenseDocument rdf:type owl:Class .


###  http://purl.org/dc/terms/RightsStatement
dct:RightsStatement rdf:type owl:Class .


#################################################################
#    Individuals
#################################################################

###  http://purl.allotrope.org/ontologies/common/qualifier
<http://purl.allotrope.org/ontologies/common/qualifier> rdf:type owl:NamedIndividual ,
                                                                 skos:ConceptScheme .


###  http://purl.allotrope.org/ontologies/common/qualifier#AFC_0000110
af-cq:AFC_0000110 rdf:type owl:NamedIndividual ,
                           af-c:AFC_0000147 ;
                  skos:inScheme <http://purl.allotrope.org/ontologies/common/qualifier> ;
                  skos:definition "The maximum limit qualifier on the property coordination indicates that the coordinated property value is a set upper boundary value. [Allotrope]" ;
                  skos:prefLabel "maximum limit" ;
                  skos:scopeNote "property coordination" .


###  http://purl.allotrope.org/ontologies/common/qualifier#AFC_0000112
af-cq:AFC_0000112 rdf:type owl:NamedIndividual ,
                           af-c:AFC_0000111 ;
                  skos:inScheme <http://purl.allotrope.org/ontologies/common/qualifier> ;
                  skos:definition "The minimum qualifier on the property coordination indicates that the coordinated property value represents a minimum of a series of values. [Allotrope]" ;
                  skos:prefLabel "minimum" ;
                  skos:scopeNote "property coordination" .


###  http://purl.allotrope.org/ontologies/common/qualifier#AFC_0000113
af-cq:AFC_0000113 rdf:type owl:NamedIndividual ,
                           af-c:AFC_0000111 ;
                  skos:inScheme <http://purl.allotrope.org/ontologies/common/qualifier> ;
                  skos:definition "The maximum qualifier on the property coordination indicates that the coordinated property value represents a maximum of a series of values. [Allotrope]" ;
                  skos:prefLabel "maximum" ;
                  skos:scopeNote "property coordination" .


###  http://purl.allotrope.org/ontologies/common/qualifier#AFC_0000114
af-cq:AFC_0000114 rdf:type owl:NamedIndividual ,
                           af-c:AFC_0000111 ;
                  skos:inScheme <http://purl.allotrope.org/ontologies/common/qualifier> ;
                  skos:altLabel "arithmetic mean" ,
                                "mean" ;
                  skos:definition "The average qualifier on the property coordination indicates that the coordinated property value represents the average (arithmetic mean) of a series of values. [Allotrope]" ;
                  skos:prefLabel "average" ;
                  skos:scopeNote "property coordination" .


###  http://purl.allotrope.org/ontologies/common/qualifier#AFC_0000115
af-cq:AFC_0000115 rdf:type owl:NamedIndividual ,
                           af-c:AFC_0000111 ;
                  skos:inScheme <http://purl.allotrope.org/ontologies/common/qualifier> ;
                  skos:definition "The geometric mean qualifier on the property coordination indicates that the coordinated property value represents the geometric mean of a series of values. [Allotrope]" ;
                  skos:prefLabel "geometric mean" ;
                  skos:scopeNote "property coordination" .


###  http://purl.allotrope.org/ontologies/common/qualifier#AFC_0000116
af-cq:AFC_0000116 rdf:type owl:NamedIndividual ,
                           af-c:AFC_0000111 ;
                  skos:inScheme <http://purl.allotrope.org/ontologies/common/qualifier> ;
                  skos:altLabel "total" ;
                  skos:definition "The sum qualifier on the property coordination indicates that the coordinated property value represents the sum or total of a series of values. [Allotrope]" ;
                  skos:prefLabel "sum" ;
                  skos:scopeNote "property coordination" .


###  http://purl.allotrope.org/ontologies/common/qualifier#AFC_0000117
af-cq:AFC_0000117 rdf:type owl:NamedIndividual ,
                           af-c:AFC_0000147 ;
                  skos:inScheme <http://purl.allotrope.org/ontologies/common/qualifier> ;
                  skos:definition "The minium limit qualifier in the property coordination indicates that the coordinated property value is a set lower boundary value. [Allotrope]" ;
                  skos:prefLabel "minimum limit" ;
                  skos:scopeNote "property coordination" .


###  http://purl.allotrope.org/ontologies/common/qualifier#AFC_0000118
af-cq:AFC_0000118 rdf:type owl:NamedIndividual ,
                           af-c:AFC_0000152 ;
                  skos:inScheme <http://purl.allotrope.org/ontologies/common/qualifier> ;
                  skos:definition "The target qualifier in the property coordination that the value of the coordinated property is a target value for the property that should be reached in some process. [Allotrope]" ;
                  skos:prefLabel "target" ;
                  skos:scopeNote "property coordination" .


###  http://purl.allotrope.org/ontologies/common/qualifier#AFC_0000133
af-cq:AFC_0000133 rdf:type owl:NamedIndividual ,
                           af-c:AFC_0000111 ;
                  skos:inScheme <http://purl.allotrope.org/ontologies/common/qualifier> ;
                  skos:definition "The variance qualifier on the property coordination indicates that the coordinated property value represents a the variance qualifier of a series of values. [Allotrope]" ;
                  skos:prefLabel "variance" ;
                  skos:scopeNote "property coordination" .


###  http://purl.allotrope.org/ontologies/common/qualifier#AFC_0000134
af-cq:AFC_0000134 rdf:type owl:NamedIndividual ,
                           af-c:AFC_0000111 ;
                  skos:inScheme <http://purl.allotrope.org/ontologies/common/qualifier> ;
                  skos:definition "The standard deviation qualifier on the property coordination indicates that the coordinated property value represents a the standard deviation qualifier of a series of values. [Allotrope]" ;
                  skos:prefLabel "standard deviation" ;
                  skos:scopeNote "property coordination" .


###  http://purl.allotrope.org/ontologies/common/qualifier#AFC_0000135
af-cq:AFC_0000135 rdf:type owl:NamedIndividual ,
                           af-c:AFC_0000111 ;
                  skos:inScheme <http://purl.allotrope.org/ontologies/common/qualifier> ;
                  skos:definition "The relative standard deviation qualifier on the property coordination indicates that the coordinated property value represents a the relative standard deviation qualifier of a series of values. [Allotrope]" ;
                  skos:prefLabel "relative standard deviation" ;
                  skos:scopeNote "property coordination" .


###  http://purl.allotrope.org/ontologies/common/qualifier#AFC_0000136
af-cq:AFC_0000136 rdf:type owl:NamedIndividual ,
                           af-c:AFC_0000111 ;
                  skos:inScheme <http://purl.allotrope.org/ontologies/common/qualifier> ;
                  skos:definition "The median qualifier on the property coordination indicates that the coordinated property value represents a the median of a series of values. [Allotrope]" ;
                  skos:prefLabel "median" ;
                  skos:scopeNote "property coordination" .


###  http://purl.allotrope.org/ontologies/common/qualifier#AFC_0000137
af-cq:AFC_0000137 rdf:type owl:NamedIndividual ,
                           af-c:AFC_0000111 ;
                  skos:inScheme <http://purl.allotrope.org/ontologies/common/qualifier> ;
                  skos:definition "The first qualifier on the property coordination indicates that the coordinated property value is the first of an ordered series of values. [Allotrope]" ;
                  skos:prefLabel "first" ;
                  skos:scopeNote "property coordination" .


###  http://purl.allotrope.org/ontologies/common/qualifier#AFC_0000138
af-cq:AFC_0000138 rdf:type owl:NamedIndividual ,
                           af-c:AFC_0000111 ;
                  skos:inScheme <http://purl.allotrope.org/ontologies/common/qualifier> ;
                  skos:definition "The last qualifier on the property coordination indicates that the value of the coordinated property is the last value of an ordered series of values. [Allotrope]" ;
                  skos:prefLabel "last" ;
                  skos:scopeNote "property coordination" .


###  http://purl.allotrope.org/ontologies/common/qualifier#AFC_0000139
af-cq:AFC_0000139 rdf:type owl:NamedIndividual ,
                           af-c:AFC_0000145 ;
                  skos:inScheme <http://purl.allotrope.org/ontologies/common/qualifier> ;
                  skos:altLabel "ratio" ;
                  skos:definition "The relative qualifier indicates that the coordinated property is a measurable value indicated as ratio to another value. [Allotrope]" ;
                  skos:example "relative temperature" ;
                  skos:note "The base property of the property coordination is the property that is put into relation. The super property of the coordinated property is usually not the base property." ;
                  skos:prefLabel "relative" ;
                  skos:scopeNote "property coordination" .


###  http://purl.allotrope.org/ontologies/common/qualifier#AFC_0000140
af-cq:AFC_0000140 rdf:type owl:NamedIndividual ,
                           af-c:AFC_0000147 ;
                  skos:inScheme <http://purl.allotrope.org/ontologies/common/qualifier> ;
                  skos:definition "The range qualifier indicates that the coordinated property is a property that defines a range limit on values. [Allotrope]" ;
                  skos:prefLabel "range" ;
                  skos:scopeNote "property coordination" .


###  http://purl.allotrope.org/ontologies/common/qualifier#AFC_0000141
af-cq:AFC_0000141 rdf:type owl:NamedIndividual ,
                           af-c:AFC_0000111 ;
                  skos:inScheme <http://purl.allotrope.org/ontologies/common/qualifier> ;
                  skos:definition "The harmonic mean qualifier on the property coordination indicates that the coordinated property value represents the harmonic mean of a series of values. [Allotrope]" ;
                  skos:prefLabel "harmonic mean" ;
                  skos:scopeNote "property coordination" .


###  http://purl.allotrope.org/ontologies/common/qualifier#AFC_0000142
af-cq:AFC_0000142 rdf:type owl:NamedIndividual ,
                           af-c:AFC_0000145 ;
                  skos:inScheme <http://purl.allotrope.org/ontologies/common/qualifier> ;
                  skos:altLabel "unprocessed" ;
                  skos:definition "The raw qualifier indicates in a property coordination that the value of the coordinated property is an unprocessed value. [Allotrope]" ;
                  skos:prefLabel "raw" ;
                  skos:scopeNote "property coordination" .


###  http://purl.allotrope.org/ontologies/common/qualifier#AFC_0000143
af-cq:AFC_0000143 rdf:type owl:NamedIndividual ,
                           af-c:AFC_0000145 ;
                  skos:inScheme <http://purl.allotrope.org/ontologies/common/qualifier> ;
                  skos:altLabel "computed" ;
                  skos:definition "The calculated qualifier indicates in a property coordination that the value of the coordinated property is produced by calculation instead of measurement. [Allotrope]" ;
                  skos:example "calculated net weight" ;
                  skos:prefLabel "calculated" ;
                  skos:scopeNote "property coordination" .


###  http://purl.allotrope.org/ontologies/common/qualifier#AFC_0000144
af-cq:AFC_0000144 rdf:type owl:NamedIndividual ,
                           af-c:AFC_0000145 ;
                  skos:inScheme <http://purl.allotrope.org/ontologies/common/qualifier> ;
                  skos:altLabel "actual" ;
                  skos:definition "The measured qualifier indicates in a property coordination that the value of the coordinated property is produced directly by  measurement. [Allotrope]" ;
                  skos:prefLabel "measured" ;
                  skos:scopeNote "property coordination" .


###  http://purl.allotrope.org/ontologies/common/qualifier#AFC_0000146
af-cq:AFC_0000146 rdf:type owl:NamedIndividual ,
                           af-c:AFC_0000152 ;
                  skos:inScheme <http://purl.allotrope.org/ontologies/common/qualifier> ;
                  skos:definition "The threshold qualifier indicates in the property coordination that the value of the coordinated property is the value that must be exceeded for a certain reaction, phenomenon, result, or condition to occur or be manifested. [Allotrope]" ;
                  skos:prefLabel "threshold" ;
                  skos:scopeNote "property coordination" .


###  http://purl.allotrope.org/ontologies/common/qualifier#AFC_0000149
af-cq:AFC_0000149 rdf:type owl:NamedIndividual ,
                           af-c:AFC_0000148 ;
                  skos:inScheme <http://purl.allotrope.org/ontologies/common/qualifier> ;
                  skos:definition "The start qualifier indicates in the property coordination that the property is associated with the start of some process. [Allotrope]" ;
                  skos:example "start temperature" ;
                  skos:prefLabel "start" ;
                  skos:scopeNote "property coordination" .


###  http://purl.allotrope.org/ontologies/common/qualifier#AFC_0000150
af-cq:AFC_0000150 rdf:type owl:NamedIndividual ,
                           af-c:AFC_0000148 ;
                  skos:inScheme <http://purl.allotrope.org/ontologies/common/qualifier> ;
                  skos:altLabel "actual" ;
                  skos:definition "The current qualifier indicates in the property coordination that the property is associated with the current state of some process. [Allotrope]" ;
                  skos:prefLabel "current" ;
                  skos:scopeNote "property coordination" .


###  http://purl.allotrope.org/ontologies/common/qualifier#AFC_0000151
af-cq:AFC_0000151 rdf:type owl:NamedIndividual ,
                           af-c:AFC_0000148 ;
                  skos:inScheme <http://purl.allotrope.org/ontologies/common/qualifier> ;
                  skos:definition "The end qualifier indicates in the property coordination that the property is associated with the end of some process. [Allotrope]" ;
                  skos:prefLabel "end" ;
                  skos:scopeNote "property coordination" .


###  http://purl.allotrope.org/ontologies/common/qualifier#AFC_0000153
af-cq:AFC_0000153 rdf:type owl:NamedIndividual ,
                           af-c:AFC_0000152 ;
                  skos:inScheme <http://purl.allotrope.org/ontologies/common/qualifier> ;
                  dct:source "https://en.wikipedia.org/wiki/Setpoint_%28control_system%29" ;
                  skos:altLabel "set-point" ;
                  skos:definition "The setpoint qualifier in a property coordination indicates that the value of the coordinated property is a value that is a standard value or a norm in a controlled system. [Allotrope]" ;
                  skos:prefLabel "setpoint" ;
                  skos:scopeNote "property coordination" .


###  http://purl.allotrope.org/ontologies/common/qualifier#AFC_0000154
af-cq:AFC_0000154 rdf:type owl:NamedIndividual ,
                           af-c:AFC_0000145 ;
                  skos:inScheme <http://purl.allotrope.org/ontologies/common/qualifier> ;
                  skos:altLabel "adjusted" ;
                  skos:definition "The corrected qualifier indicates in a property coordination that indicates that  the value of the coordinated property has been corrected or adjusted from an original value. [Allotrope]" ;
                  skos:example "baseline corrected" ;
                  skos:prefLabel "corrected" ;
                  skos:scopeNote "property coordination" .


###  http://purl.allotrope.org/ontologies/common/qualifier#AFC_0000155
af-cq:AFC_0000155 rdf:type owl:NamedIndividual ,
                           af-c:AFC_0000152 ;
                  skos:inScheme <http://purl.allotrope.org/ontologies/common/qualifier> ;
                  skos:definition "The default qualifier in a property coordination indicates that the value of the coordinated property is a preset setting when no choice is done. [Allotrope]" ;
                  skos:prefLabel "default" ;
                  skos:scopeNote "property coordination" .


###  http://purl.allotrope.org/ontologies/common/qualifier#AFC_0000156
af-cq:AFC_0000156 rdf:type owl:NamedIndividual ,
                           af-c:AFC_0000145 ;
                  skos:inScheme <http://purl.allotrope.org/ontologies/common/qualifier> ;
                  dct:source "https://en.wikipedia.org/wiki/Reference_range" ;
                  skos:changeNote "2024-09-12 Replaced [VIM, OSTHUS] attribution with [Allotrope] as the definition appears to be aligned with other Allotrope-derived definitions, rather than sourced from VIM." ;
                  skos:definition "The reference qualifier indicates in a property coordination that the value of the coordinated property is the value taken from some reference group or individual used as basis for comparison with values of the same kind. [Allotrope]" ;
                  skos:prefLabel "reference" ;
                  skos:scopeNote "property coordination" .


###  http://purl.allotrope.org/ontologies/common/qualifier#AFC_0000157
af-cq:AFC_0000157 rdf:type owl:NamedIndividual ,
                           af-c:AFC_0000152 ;
                  skos:inScheme <http://purl.allotrope.org/ontologies/common/qualifier> ;
                  skos:altLabel "test" ;
                  skos:definition "The check qualifier indicates the the value of the coordinated property is a value, that triggers a certain reaction, phenomenon, result, or condition to occur or be manifested. [Allotrope]" ;
                  skos:prefLabel "check" ;
                  skos:scopeNote "property coordination" .


###  http://purl.allotrope.org/ontologies/common/qualifier#AFC_0000158
af-cq:AFC_0000158 rdf:type owl:NamedIndividual ,
                           af-c:AFC_0000145 ;
                  skos:inScheme <http://purl.allotrope.org/ontologies/common/qualifier> ;
                  dct:source "https://en.wikipedia.org/wiki/Real_versus_nominal_value" ;
                  skos:definition "The nominal qualifier indicates in a property coordination that the value of the coordinated property is a value existing in name only. It is assigned as a convenient designation rather than calculated by data analysis or following usual rounding methods. The use of nominal values can be based on de facto standards or some technical standards. [Wikipedia]" ;
                  skos:prefLabel "nominal" ;
                  skos:scopeNote "property coordination" .


###  http://purl.allotrope.org/ontologies/common/qualifier#AFC_0000159
af-cq:AFC_0000159 rdf:type owl:NamedIndividual ,
                           af-c:AFC_0000145 ;
                  skos:inScheme <http://purl.allotrope.org/ontologies/common/qualifier> ;
                  skos:definition "The absolute qualifier indicates that the coordinated property is a measurable value irrespective of its relation to another value. [Allotrope]" ;
                  skos:prefLabel "absolute" ;
                  skos:scopeNote "property coordination" .


###  http://purl.allotrope.org/voc/attribution
<http://purl.allotrope.org/voc/attribution> rdf:type owl:NamedIndividual ,
                                                     dct:RightsStatement ;
                                            dct:description """
These taxonomies contain material or may constitute derivative works of material which may be subject to copyright by one of the following organizations.  By using these taxonomies, you agree to the following terms and conditions applicable to its contents:
******************************************************************************
Copyright Notice and Terms for IUPAC Gold Book
______________________________________________________________________________
Copyright © 1998, Regents of the University of California
All rights reserved.
Redistribution and use in source and binary forms, with or without modification, are permitted provided that the following conditions are met:
1. Redistributions of source code must retain the above copyright notice, this list of conditions and the following disclaimer.
2. Redistributions in binary form must reproduce the above copyright notice, this list of conditions and the following disclaimer in the documentation and/or other materials provided with the distribution.
THIS SOFTWARE IS PROVIDED BY THE COPYRIGHT HOLDERS AND CONTRIBUTORS \"AS IS\" AND ANY EXPRESS OR IMPLIED WARRANTIES, INCLUDING, BUT NOT LIMITED TO, THE IMPLIED WARRANTIES OF MERCHANTABILITY AND FITNESS FOR A PARTICULAR PURPOSE ARE DISCLAIMED. IN NO EVENT SHALL THE COPYRIGHT HOLDER OR CONTRIBUTORS BE LIABLE FOR ANY DIRECT, INDIRECT, INCIDENTAL, SPECIAL, EXEMPLARY, OR CONSEQUENTIAL DAMAGES (INCLUDING, BUT NOT LIMITED TO, PROCUREMENT OF SUBSTITUTE GOODS OR SERVICES; LOSS OF USE, DATA, OR PROFITS; OR BUSINESS INTERRUPTION) HOWEVER CAUSED AND ON ANY THEORY OF LIABILITY, WHETHER IN CONTRACT, STRICT LIABILITY, OR TORT (INCLUDING NEGLIGENCE OR OTHERWISE) ARISING IN ANY WAY OUT OF THE USE OF THIS SOFTWARE, EVEN IF ADVISED OF THE POSSIBILITY OF SUCH DAMAGE.
******************************************************************************
Copyright Notice and Terms for PSI-MS (Proteomics Standards Initiative - Mass Spectrometry) Mass spectrometer output files and spectra interpretation
_____________________________________________________________________________
Created by Matt Chambers, Andreas Bertsch, Marius Kallhardt, Eric Deutsch Fredrik Levander, Pierre-Alain Binz, and Gerhard Mayer. Publisher: HUPO Proteomics Standards Initiative Mass Spectrometry Standards Working Group and HUPO Proteomics Standards Initiative Proteomics Informatics Working Group. This work is used pursuant to a Creative Commons license available here: http://creativecommons.org/licenses/by/3.0/legalcode

******************************************************************************
Attribution Notice for National Center for Biomedical Ontology materials. 

This work contains material from the Cell Ontology and Clinical Measurement Ontology, available here: http://bioportal.bioontology.org/.
******************************************************************************
Attribution Notice for ChEBI
This work contains material from the European Bioinformatics Institute’s ChEBI database. 
******************************************************************************
Attribution Notice for Quantities Units Dimensions Data Types (http://www.qudt.org/)
This work contains content from www.qudt.org and is used pursuant to a Creative Commons License available here: http://creativecommons.org/licenses/by-sa/3.0/us/legalcode. The original work may have been modified. 
******************************************************************************
Copyright and Attribution Notice for Dublin Core Metadata Initiative Document
This work contains material from the following DCMI document used pursuant to a creative commons license available here: https://creativecommons.org/licenses/by/4.0/legalcode. This material may have been modified or changed.
Timestamped URL:          http://dublincore.org/documents/2012/06/14/dcmi-terms/ 
Date Issued:                       2012-06-14 
Document Status:            This is a DCMI Recommendation.
Copyright © 1995-2015 DCMI. All Rights Reserved. DCMI liability, trademark/service mark, document use and software licensing rules apply. 
******************************************************************************

""" ;
                                            dct:title "Derivative works attribution" .


###  http://purl.allotrope.org/voc/copyright
<http://purl.allotrope.org/voc/copyright> rdf:type owl:NamedIndividual ,
                                                   dct:RightsStatement ;
                                          dct:description "Copyright © 2015-2025 Allotrope Foundation" ;
                                          dct:rightsHolder <http://www.allotrope.org> ;
                                          dct:title "Copyright © 2015-2025 Allotrope Foundation" .


###  http://purl.allotrope.org/voc/creative-commons-attribution-license
<http://purl.allotrope.org/voc/creative-commons-attribution-license> rdf:type owl:NamedIndividual ,
                                                                              dct:LicenseDocument ;
                                                                     dct:description """This work is licensed under a Creative Commons Attribution 4.0 International License http://creativecommons.org/licenses/by/4.0/.

THESE MATERIALS ARE PROVIDED \"AS IS\" AND ALLOTROPE EXPRESSLY DISCLAIMS ALL WARRANTIES, EXPRESS, IMPLIED OR STATUTORY, INCLUDING, WITHOUT LIMITATION, THE WARRANTIES OF NON-INFRINGEMENT, TITLE, MERCHANTABILITY AND FITNESS FOR A PARTICULAR PURPOSE.

Copyright © 2015-2025 Allotrope Foundation
""" ;
                                                                     dct:title "Creative Commons Attribution 4.0 International Public License" .


#################################################################
#    General axioms
#################################################################

[ rdf:type owl:AllDifferent ;
  owl:distinctMembers ( af-cq:AFC_0000110
                        af-cq:AFC_0000117
                      )
] .


[ rdf:type owl:AllDifferent ;
  owl:distinctMembers ( af-cq:AFC_0000110
                        af-cq:AFC_0000140
                      )
] .


[ rdf:type owl:AllDifferent ;
  owl:distinctMembers ( af-cq:AFC_0000117
                        af-cq:AFC_0000140
                      )
] .


[ rdf:type owl:AllDifferent ;
  owl:distinctMembers ( af-cq:AFC_0000139
                        af-cq:AFC_0000159
                      )
] .


[ rdf:type owl:AllDifferent ;
  owl:distinctMembers ( af-cq:AFC_0000143
                        af-cq:AFC_0000144
                      )
] .


[ rdf:type owl:AllDifferent ;
  owl:distinctMembers ( af-cq:AFC_0000143
                        af-cq:AFC_0000158
                      )
] .


[ rdf:type owl:AllDifferent ;
  owl:distinctMembers ( af-cq:AFC_0000144
                        af-cq:AFC_0000158
                      )
] .


###  Generated by the OWL API (version 5.1.19) https://github.com/owlcs/owlapi/
