@prefix : <http://purl.allotrope.org/voc/afo/domain/WD/2025/06/pumping#> .
@prefix cl: <http://purl.obolibrary.org/obo/CL> .
@prefix go: <http://purl.obolibrary.org/obo/GO> .
@prefix ro: <http://purl.obolibrary.org/obo/RO> .
@prefix bfo: <http://purl.obolibrary.org/obo/BFO> .
@prefix dct: <http://purl.org/dc/terms/> .
@prefix iao: <http://purl.obolibrary.org/obo/IAO> .
@prefix obi: <http://purl.obolibrary.org/obo/OBI> .
@prefix owl: <http://www.w3.org/2002/07/owl#> .
@prefix rdf: <http://www.w3.org/1999/02/22-rdf-syntax-ns#> .
@prefix xml: <http://www.w3.org/XML/1998/namespace> .
@prefix xsd: <http://www.w3.org/2001/XMLSchema#> .
@prefix af-c: <http://purl.allotrope.org/ontologies/common#> .
@prefix af-e: <http://purl.allotrope.org/ontologies/equipment#> .
@prefix af-m: <http://purl.allotrope.org/ontologies/material#> .
@prefix af-p: <http://purl.allotrope.org/ontologies/process#> .
@prefix af-q: <http://purl.allotrope.org/ontologies/quality#> .
@prefix af-r: <http://purl.allotrope.org/ontologies/result#> .
@prefix af-x: <http://purl.allotrope.org/ontologies/property#> .
@prefix rdfs: <http://www.w3.org/2000/01/rdf-schema#> .
@prefix skos: <http://www.w3.org/2004/02/skos/core#> .
@prefix af-cur: <http://purl.allotrope.org/ontologies/curation#> .
@base <http://purl.allotrope.org/voc/afo/domain/WD/2025/06/pumping#> .

<http://purl.allotrope.org/voc/afo/domain/WD/2025/06/pumping> rdf:type owl:Ontology ;
                                                                         owl:versionIRI <http://purl.allotrope.org/voc/afo/domain/WD/2025/06/pumping> ;
                                                                         owl:imports <http://purl.allotrope.org/voc/afo/WD/2025/06/afo> ,
                                                                                     <http://purl.allotrope.org/voc/afo/domain/REC/2025/06/pumping> ;
                                                                         dct:issued "2025-06-25T12:00:00Z"^^xsd:dateTime ;
                                                                         dct:license <http://purl.allotrope.org/voc/creative-commons-attribution-license> ;
                                                                         dct:modified "2025-04-04T12:00:00Z"^^xsd:dateTime ;
                                                                         dct:rights <http://purl.allotrope.org/voc/copyright> ;
                                                                         dct:title "AFO Pumping Domain Ontology (WD/2025/06)" ;
                                                                         owl:priorVersion <http://purl.allotrope.org/voc/afo/domain/WD/2025/03/pumping> ;
                                                                         owl:versionInfo "WD/2025/06" .

#################################################################
#    Annotation properties
#################################################################

###  http://purl.allotrope.org/ontologies/property#AFX_0002796
af-x:AFX_0002796 rdf:type owl:AnnotationProperty .


###  http://purl.allotrope.org/ontologies/property#AFX_0002798
af-x:AFX_0002798 rdf:type owl:AnnotationProperty .


###  http://purl.allotrope.org/ontologies/property#AFX_0002809
af-x:AFX_0002809 rdf:type owl:AnnotationProperty .


###  http://purl.org/dc/terms/source
dct:source rdf:type owl:AnnotationProperty .


###  http://www.w3.org/2004/02/skos/core#altLabel
skos:altLabel rdf:type owl:AnnotationProperty .


###  http://www.w3.org/2004/02/skos/core#changeNote
skos:changeNote rdf:type owl:AnnotationProperty .


###  http://www.w3.org/2004/02/skos/core#definition
skos:definition rdf:type owl:AnnotationProperty .


###  http://www.w3.org/2004/02/skos/core#example
skos:example rdf:type owl:AnnotationProperty .


###  http://www.w3.org/2004/02/skos/core#note
skos:note rdf:type owl:AnnotationProperty .


###  http://www.w3.org/2004/02/skos/core#prefLabel
skos:prefLabel rdf:type owl:AnnotationProperty .


###  http://www.w3.org/2004/02/skos/core#scopeNote
skos:scopeNote rdf:type owl:AnnotationProperty .


#################################################################
#    Object Properties
#################################################################

###  http://purl.allotrope.org/ontologies/property#AFX_0000352
af-x:AFX_0000352 rdf:type owl:ObjectProperty .


#################################################################
#    Classes
#################################################################

###  http://purl.allotrope.org/ontologies/equipment#AFE_0000468
af-e:AFE_0000468 rdf:type owl:Class ;
                 rdfs:subClassOf af-e:AFE_0000499 ;
                 owl:disjointWith af-e:AFE_0000698 ;
                 af-x:AFX_0002798 "true"^^xsd:boolean ;
                 skos:changeNote "2024-09-12 Changed [OSTHUS] attribution to [Allotrope]." ;
                 skos:definition "A high pressure pump is a type of pump that can establish pressures above several hundreds of bar. [Allotrope]" ;
                 skos:prefLabel "high-pressure pump" .


###  http://purl.allotrope.org/ontologies/equipment#AFE_0000698
af-e:AFE_0000698 rdf:type owl:Class ;
                 rdfs:subClassOf af-e:AFE_0000499 ;
                 af-x:AFX_0002798 "true"^^xsd:boolean ;
                 skos:changeNote "2024-09-12 Changed [OSTHUS] attribution to [Allotrope]." ;
                 skos:definition "A low-pressure pump is a pump that works accurately at very low pressures. [Allotrope]" ;
                 skos:prefLabel "low-pressure pump" .


###  http://purl.allotrope.org/ontologies/equipment#AFE_0000701
af-e:AFE_0000701 rdf:type owl:Class ;
                 rdfs:subClassOf af-e:AFE_0000746 ,
                                 [ rdf:type owl:Restriction ;
                                   owl:onProperty ro:_0000085 ;
                                   owl:someValuesFrom <http://purl.allotrope.org/ontologies/function#AFFN_0000046>
                                 ] ;
                 skos:changeNote "2015-12-15 Improved definition [Amgen]" ;
                 skos:definition "A syringe which has the function of pumping material during an experiment. [CHMO]" ;
                 skos:prefLabel "syringe pump" .


###  http://purl.allotrope.org/ontologies/equipment#AFE_0000746
af-e:AFE_0000746 rdf:type owl:Class .


###  http://purl.allotrope.org/ontologies/equipment#AFE_0001131
af-e:AFE_0001131 rdf:type owl:Class ;
                 rdfs:subClassOf af-e:AFE_0000499 ;
                 dct:source "https://en.wikipedia.org/wiki/Circulating_pump" ,
                            "https://en.wikipedia.org/wiki/Circulator_pump" ;
                 skos:altLabel "circulating pump" ,
                               "circulator" ;
                 skos:changeNote "2015-11-03 Added concept [Amgen]" ;
                 skos:definition "A circulator pump is a specific type of pump used to circulate gases, liquids, or slurries in a closed circuit. They are commonly found circulating water in a hydronic heating or cooling system. Because they only circulate liquid within a closed circuit, they only need to overcome the friction of a piping system (as opposed to lifting a fluid from a point of lower potential energy to a point of higher potential energy). [Wikipedia]" ;
                 skos:prefLabel "circulator pump" .


###  http://purl.allotrope.org/ontologies/equipment#AFE_0001167
af-e:AFE_0001167 rdf:type owl:Class ;
                 rdfs:subClassOf af-e:AFE_0000499 ;
                 dct:source "https://en.wikipedia.org/wiki/Centrifugal_pump" ;
                 skos:changeNote "2015-11-03 Added concept [Amgen]" ;
                 skos:definition "Centrifugal pumps are a sub-class of dynamic axisymmetric work-absorbing turbomachinery. Centrifugal pumps are used to transport fluids by the conversion of rotational kinetic energy to the hydrodynamic energy of the fluid flow. The rotational energy typically comes from an engine or electric motor. The fluid enters the pump impeller along or near to the rotating axis and is accelerated by the impeller, flowing radially outward into a diffuser or volute chamber (casing), from where it exits. [Wikipedia]" ;
                 skos:prefLabel "centrifugal pump" .


###  http://purl.allotrope.org/ontologies/equipment#AFE_0001168
af-e:AFE_0001168 rdf:type owl:Class ;
                 rdfs:subClassOf af-e:AFE_0001169 ;
                 dct:source "https://en.wikipedia.org/wiki/Peristaltic_pump" ;
                 skos:changeNote "2015-11-03 Added concept [Amgen]" ;
                 skos:definition "A peristaltic pump is a type of positive displacement pump used for pumping a variety of fluids. The fluid is contained within a flexible tube fitted inside a circular pump casing (though linear peristaltic pumps have been made). A rotor with a number of \"rollers\", \"shoes\", \"wipers\", or \"lobes\" attached to the external circumference of the rotor compresses the flexible tube. As the rotor turns, the part of the tube under compression is pinched closed (or \"occludes\") thus forcing the fluid to be pumped to move through the tube. Additionally, as the tube opens to its natural state after the passing of the cam (\"restitution\" or \"resilience\") fluid flow is induced to the pump. [Wikipedia]" ;
                 skos:prefLabel "peristaltic pump" .


###  http://purl.allotrope.org/ontologies/equipment#AFE_0001169
af-e:AFE_0001169 rdf:type owl:Class ;
                 rdfs:subClassOf af-e:AFE_0000499 ;
                 dct:source "https://en.wikipedia.org/wiki/Pump#Positive_displacement_pump" ;
                 skos:changeNote "2015-11-03 Added concept [Amgen]" ;
                 skos:definition "A positive displacement pump makes a fluid move by trapping a fixed amount and forcing (displacing) that trapped volume into the discharge pipe. [Wikipedia]" ;
                 skos:prefLabel "positive displacement pump" .


###  http://purl.allotrope.org/ontologies/equipment#AFE_0001170
af-e:AFE_0001170 rdf:type owl:Class ;
                 rdfs:subClassOf af-e:AFE_0002182 ;
                 af-x:AFX_0002798 "true"^^xsd:boolean ;
                 dct:source "https://en.wikipedia.org/wiki/Vacuum_pump" ;
                 skos:changeNote "2015-11-03 Added concept [Amgen]" ,
                                 "2017-12-08 Moved under gas pump [OSTHUS]" ;
                 skos:definition "A vacuum pump is a device that removes gas molecules from a sealed volume in order to leave behind a partial vacuum. [Wikipedia]" ;
                 skos:prefLabel "vacuum pump" .


###  http://purl.allotrope.org/ontologies/equipment#AFE_0001171
af-e:AFE_0001171 rdf:type owl:Class ;
                 rdfs:subClassOf af-e:AFE_0001169 ;
                 skos:altLabel "membrane pump" ;
                 skos:changeNote "2015-11-03 add concept [Amgen]" ;
                 skos:definition "A diaphragm pump is a positive displacement pump that uses a combination of the reciprocating action of a rubber, thermoplastic or teflon diaphragm and suitable valves on either side of the diaphragm (check valve, butterfly valves, flap valves, or any other form of shut-off valves) to pump a fluid. [Wikipedia]" ;
                 skos:prefLabel "diaphragm pump" .


###  http://purl.allotrope.org/ontologies/equipment#AFE_0001174
af-e:AFE_0001174 rdf:type owl:Class ;
                 rdfs:subClassOf bfo:_0000029 ,
                                 [ rdf:type owl:Restriction ;
                                   owl:onProperty af-x:AFX_0000352 ;
                                   owl:someValuesFrom af-e:AFE_0000499
                                 ] ;
                 skos:changeNote "2015-11-03 Added concept [Amgen]" ;
                 skos:definition "The outlet location is said to be at the discharge side of the pump. [Wikipedia]" ;
                 skos:prefLabel "discharge side" .


###  http://purl.allotrope.org/ontologies/equipment#AFE_0001175
af-e:AFE_0001175 rdf:type owl:Class ;
                 rdfs:subClassOf bfo:_0000029 ,
                                 [ rdf:type owl:Restriction ;
                                   owl:onProperty af-x:AFX_0000352 ;
                                   owl:someValuesFrom af-e:AFE_0000499
                                 ] ;
                 rdfs:comment "2017-11-06 move under bfo:site [OSTHUS]" ;
                 skos:changeNote "2015-11-03 add concept [Amgen]" ;
                 skos:definition "The inlet location is said to be at the suction side of the pump. [Wikipedia]" ;
                 skos:prefLabel "suction side" .


###  http://purl.allotrope.org/ontologies/equipment#AFE_0001176
af-e:AFE_0001176 rdf:type owl:Class ;
                 rdfs:subClassOf af-e:AFE_0000499 ;
                 af-x:AFX_0002798 "true"^^xsd:boolean ;
                 skos:changeNote "2015-11-03 add concept [Amgen]" ;
                 skos:definition "A metering pump moves a precise volume of liquid in a specified time period providing an accurate flow rate. [Wikipedia]" ;
                 skos:prefLabel "metering pump" .


###  http://purl.allotrope.org/ontologies/equipment#AFE_0001177
af-e:AFE_0001177 rdf:type owl:Class ;
                 rdfs:subClassOf af-e:AFE_0001169 ;
                 skos:changeNote "2015-11-03 add concept [Amgen]" ;
                 skos:definition "A piston pump is a type of positive displacement pump where the high-pressure seal reciprocates with the piston. Piston pumps can be used to move liquids or compress gases. [Wikipedia]" ;
                 skos:prefLabel "piston pump" .


###  http://purl.allotrope.org/ontologies/equipment#AFE_0001178
af-e:AFE_0001178 rdf:type owl:Class ;
                 rdfs:subClassOf af-e:AFE_0001169 ;
                 skos:changeNote "2015-11-03 add concept [Amgen]" ;
                 skos:definition "A plunger pump is a type of positive displacement pump where the high-pressure seal is stationary and a smooth cylindrical plunger slides through the seal. [Wikipedia]" ;
                 skos:prefLabel "plunger pump" .


###  http://purl.allotrope.org/ontologies/equipment#AFE_0001181
af-e:AFE_0001181 rdf:type owl:Class ;
                 rdfs:subClassOf af-e:AFE_0001169 ;
                 skos:changeNote "2015-11-03 add concept [Amgen]" ,
                                 "2024-09-12 Changed [OSTHUS] attribution to [Allotrope]." ;
                 skos:definition "A bellows pump forces fluid from an inlet to a discharge area by bellows. [Allotrope]" ;
                 skos:prefLabel "bellows pump" .


###  http://purl.allotrope.org/ontologies/equipment#AFE_0001739
af-e:AFE_0001739 rdf:type owl:Class ;
                 rdfs:subClassOf af-e:AFE_0000499 ;
                 af-x:AFX_0002798 "true"^^xsd:boolean ;
                 skos:changeNote "2015-11-25 Added concept [Amgen]" ,
                                 "2015-12-15 Improved definition [Amgen]" ,
                                 "2024-09-12 Changed [Amgen] attribution to [Allotrope]." ;
                 skos:definition "A liquid pump is a device used to transfer liquids. [Allotrope]" ;
                 skos:prefLabel "liquid pump" .


###  http://purl.allotrope.org/ontologies/equipment#AFE_0002182
af-e:AFE_0002182 rdf:type owl:Class ;
                 rdfs:subClassOf af-e:AFE_0000499 ;
                 af-x:AFX_0002798 "true"^^xsd:boolean ;
                 skos:changeNote "2017-12-08 Added concept [OSTHUS]" ,
                                 "2024-09-12 Changed [Amgen] attribution to [Allotrope]." ;
                 skos:definition "A gas pump is a device used to transfer gases. [Allotrope]" ;
                 skos:prefLabel "gas pump" .


#################################################################
#    Individuals
#################################################################

###  http://purl.allotrope.org/voc/attribution
<http://purl.allotrope.org/voc/attribution> rdf:type owl:NamedIndividual ,
                                                     dct:RightsStatement ;
                                            dct:description """
These taxonomies contain material or may constitute derivative works of material which may be subject to copyright by one of the following organizations.  By using these taxonomies, you agree to the following terms and conditions applicable to its contents:
******************************************************************************
Copyright Notice and Terms for IUPAC Gold Book
______________________________________________________________________________
Copyright © 1998, Regents of the University of California
All rights reserved.
Redistribution and use in source and binary forms, with or without modification, are permitted provided that the following conditions are met:
1. Redistributions of source code must retain the above copyright notice, this list of conditions and the following disclaimer.
2. Redistributions in binary form must reproduce the above copyright notice, this list of conditions and the following disclaimer in the documentation and/or other materials provided with the distribution.
THIS SOFTWARE IS PROVIDED BY THE COPYRIGHT HOLDERS AND CONTRIBUTORS \"AS IS\" AND ANY EXPRESS OR IMPLIED WARRANTIES, INCLUDING, BUT NOT LIMITED TO, THE IMPLIED WARRANTIES OF MERCHANTABILITY AND FITNESS FOR A PARTICULAR PURPOSE ARE DISCLAIMED. IN NO EVENT SHALL THE COPYRIGHT HOLDER OR CONTRIBUTORS BE LIABLE FOR ANY DIRECT, INDIRECT, INCIDENTAL, SPECIAL, EXEMPLARY, OR CONSEQUENTIAL DAMAGES (INCLUDING, BUT NOT LIMITED TO, PROCUREMENT OF SUBSTITUTE GOODS OR SERVICES; LOSS OF USE, DATA, OR PROFITS; OR BUSINESS INTERRUPTION) HOWEVER CAUSED AND ON ANY THEORY OF LIABILITY, WHETHER IN CONTRACT, STRICT LIABILITY, OR TORT (INCLUDING NEGLIGENCE OR OTHERWISE) ARISING IN ANY WAY OUT OF THE USE OF THIS SOFTWARE, EVEN IF ADVISED OF THE POSSIBILITY OF SUCH DAMAGE.
******************************************************************************
Copyright Notice and Terms for PSI-MS (Proteomics Standards Initiative - Mass Spectrometry) Mass spectrometer output files and spectra interpretation
_____________________________________________________________________________
Created by Matt Chambers, Andreas Bertsch, Marius Kallhardt, Eric Deutsch Fredrik Levander, Pierre-Alain Binz, and Gerhard Mayer. Publisher: HUPO Proteomics Standards Initiative Mass Spectrometry Standards Working Group and HUPO Proteomics Standards Initiative Proteomics Informatics Working Group. This work is used pursuant to a Creative Commons license available here: http://creativecommons.org/licenses/by/3.0/legalcode

******************************************************************************
Attribution Notice for National Center for Biomedical Ontology materials.

This work contains material from the Cell Ontology and Clinical Measurement Ontology, available here: http://bioportal.bioontology.org/.
******************************************************************************
Attribution Notice for ChEBI
This work contains material from the European Bioinformatics Institute’s ChEBI database.
******************************************************************************
Attribution Notice for Quantities Units Dimensions Data Types (http://www.qudt.org/)
This work contains content from www.qudt.org and is used pursuant to a Creative Commons License available here: http://creativecommons.org/licenses/by-sa/3.0/us/legalcode. The original work may have been modified.
******************************************************************************
Copyright and Attribution Notice for Dublin Core Metadata Initiative Document
This work contains material from the following DCMI document used pursuant to a creative commons license available here: https://creativecommons.org/licenses/by/4.0/legalcode. This material may have been modified or changed.
Timestamped URL:          http://dublincore.org/documents/2012/06/14/dcmi-terms/
Date Issued:                       2012-06-14
Document Status:            This is a DCMI Recommendation.
Copyright © 1995-2015 DCMI. All Rights Reserved. DCMI liability, trademark/service mark, document use and software licensing rules apply.
******************************************************************************

""" ;
                                            dct:title "Derivative works attribution" .


###  http://purl.allotrope.org/voc/copyright
<http://purl.allotrope.org/voc/copyright> rdf:type owl:NamedIndividual ,
                                                   dct:RightsStatement ;
                                          dct:description "(c) 2018 Allotrope Foundation" ;
                                          dct:title "(c) 2018 Allotrope Foundation" .


###  http://purl.allotrope.org/voc/creative-commons-attribution-license
<http://purl.allotrope.org/voc/creative-commons-attribution-license> rdf:type owl:NamedIndividual ,
                                                                              dct:LicenseDocument ;
                                                                     dct:description """This work is licensed under a Creative Commons Attribution 4.0 International License http://creativecommons.org/licenses/by/4.0/.

THESE MATERIALS ARE PROVIDED \"AS IS\" AND ALLOTROPE EXPRESSLY DISCLAIMS ALL WARRANTIES, EXPRESS, IMPLIED OR STATUTORY, INCLUDING, WITHOUT LIMITATION, THE WARRANTIES OF NON-INFRINGEMENT, TITLE, MERCHANTABILITY AND FITNESS FOR A PARTICULAR PURPOSE.

Copyright © 2015-2025 Allotrope Foundation
""" ;
                                                                     dct:rightsHolder <http://www.allotrope.org> ;
                                                                     dct:title "Creative Commons Attribution 4.0 International Public License" .


###  Generated by the OWL API (version 5.1.19) https://github.com/owlcs/owlapi/
