@prefix : <http://purl.allotrope.org/voc/afo/domain/WD/2025/06/reflectometry#> .
@prefix cl: <http://purl.obolibrary.org/obo/CL> .
@prefix go: <http://purl.obolibrary.org/obo/GO> .
@prefix ro: <http://purl.obolibrary.org/obo/RO> .
@prefix bfo: <http://purl.obolibrary.org/obo/BFO> .
@prefix dct: <http://purl.org/dc/terms/> .
@prefix iao: <http://purl.obolibrary.org/obo/IAO> .
@prefix obi: <http://purl.obolibrary.org/obo/OBI> .
@prefix owl: <http://www.w3.org/2002/07/owl#> .
@prefix rdf: <http://www.w3.org/1999/02/22-rdf-syntax-ns#> .
@prefix xml: <http://www.w3.org/XML/1998/namespace> .
@prefix xsd: <http://www.w3.org/2001/XMLSchema#> .
@prefix af-c: <http://purl.allotrope.org/ontologies/common#> .
@prefix af-e: <http://purl.allotrope.org/ontologies/equipment#> .
@prefix af-m: <http://purl.allotrope.org/ontologies/material#> .
@prefix af-p: <http://purl.allotrope.org/ontologies/process#> .
@prefix af-q: <http://purl.allotrope.org/ontologies/quality#> .
@prefix af-r: <http://purl.allotrope.org/ontologies/result#> .
@prefix af-x: <http://purl.allotrope.org/ontologies/property#> .
@prefix rdfs: <http://www.w3.org/2000/01/rdf-schema#> .
@prefix skos: <http://www.w3.org/2004/02/skos/core#> .
@prefix af-cur: <http://purl.allotrope.org/ontologies/curation#> .
@base <http://purl.allotrope.org/voc/afo/domain/WD/2025/06/reflectometry#> .

<http://purl.allotrope.org/voc/afo/domain/WD/2025/06/reflectometry> rdf:type owl:Ontology ;
                                                                               owl:versionIRI <http://purl.allotrope.org/voc/afo/domain/WD/2025/06/reflectometry> ;
                                                                               owl:imports <http://purl.allotrope.org/voc/afo/WD/2025/06/afo> ;
                                                                               dct:issued "2025-06-25T12:00:00Z"^^xsd:dateTime ;
                                                                               dct:license <http://purl.allotrope.org/voc/creative-commons-attribution-license> ;
                                                                               dct:modified "2025-04-04T12:00:00Z"^^xsd:dateTime ;
                                                                               dct:rights <http://purl.allotrope.org/voc/attribution> ,
                                                                                          <http://purl.allotrope.org/voc/copyright> ;
                                                                               dct:title "AFO Reflectometry Domain Ontology - working draft" ;
                                                                               owl:priorVersion <http://purl.allotrope.org/voc/afo/domain/WD/2018/04/reflectometry> ;
                                                                               owl:versionInfo "WD/2025/06" .

#################################################################
#    Annotation properties
#################################################################

###  http://purl.allotrope.org/ontologies/property#AFX_0002796
af-x:AFX_0002796 rdf:type owl:AnnotationProperty .


###  http://purl.allotrope.org/ontologies/property#AFX_0002798
af-x:AFX_0002798 rdf:type owl:AnnotationProperty .


###  http://purl.allotrope.org/ontologies/property#AFX_0002809
af-x:AFX_0002809 rdf:type owl:AnnotationProperty .


###  http://purl.org/dc/terms/source
dct:source rdf:type owl:AnnotationProperty .


###  http://www.w3.org/2004/02/skos/core#altLabel
skos:altLabel rdf:type owl:AnnotationProperty .


###  http://www.w3.org/2004/02/skos/core#changeNote
skos:changeNote rdf:type owl:AnnotationProperty .


###  http://www.w3.org/2004/02/skos/core#definition
skos:definition rdf:type owl:AnnotationProperty .


###  http://www.w3.org/2004/02/skos/core#example
skos:example rdf:type owl:AnnotationProperty .


###  http://www.w3.org/2004/02/skos/core#note
skos:note rdf:type owl:AnnotationProperty .


###  http://www.w3.org/2004/02/skos/core#prefLabel
skos:prefLabel rdf:type owl:AnnotationProperty .


###  http://www.w3.org/2004/02/skos/core#scopeNote
skos:scopeNote rdf:type owl:AnnotationProperty .


#################################################################
#    Classes
#################################################################

###  http://purl.allotrope.org/ontologies/process#AFP_0000076
af-p:AFP_0000076 rdf:type owl:Class ;
                 rdfs:subClassOf af-p:AFP_0001673 ;
                 skos:altLabel "specular X-ray reflectivity" ,
                               "specular XRR" ;
                 skos:definition "A method for determining structure by directing a beam of X-rays at an extremely flat surface (at angle theta to the surface) and measuring the intensity of the X-rays which undergo specular reflection (and are emitted at angle theta from the surface). [CHMO]" ;
                 skos:prefLabel "specular X-ray reflectometry" .


###  http://purl.allotrope.org/ontologies/process#AFP_0000479
af-p:AFP_0000479 rdf:type owl:Class ;
                 rdfs:subClassOf af-p:AFP_0000229 ;
                 skos:altLabel "neutron reflection" ,
                               "neutron reflectivity" ,
                               "specular neutron reflectivity" ,
                               "specular neutron reflectrometry" ;
                 skos:definition "A method for determining structure by directing a beam of neutrons onto an extremely flat surface and measuring the intensity of the reflected neutrons as a function of angle and neutron wavelength. [CHMO]" ;
                 skos:prefLabel "neutron reflectometry" .


###  http://purl.allotrope.org/ontologies/process#AFP_0000608
af-p:AFP_0000608 rdf:type owl:Class ;
                 rdfs:subClassOf af-p:AFP_0001058 ;
                 skos:altLabel "OFDR" ,
                               "optical frequency domain reflectivity" ,
                               "optical frequency domain reflectometry" ,
                               "optical frequency-domain reflectivity" ;
                 skos:definition "A method for determining structure by illuminating an extremely flat surface with light from a pulsed laser and interfering the light reflected from the sample at the Brewster angle with light reflected from a reference mirror. Intereference only occurs when the difference in the optical path lengths between the two mirrors is within the coherence length of the optical source. The frequency of the laser pulse is proportional to the time delay between each of the signals returning. [CHMO]" ;
                 skos:prefLabel "optical frequency-domain reflectometry" .


###  http://purl.allotrope.org/ontologies/process#AFP_0000823
af-p:AFP_0000823 rdf:type owl:Class ;
                 rdfs:subClassOf af-p:AFP_0001673 ;
                 skos:altLabel "RSoXR" ,
                               "resonant soft X-ray reflectivity " ;
                 skos:definition "A method for determining structure by directing a beam of X-rays at a surface (e.g. a thin film) and measuring the complex index of refraction as a function of incident X-ray energy, near the absorption edge. [CHMO]" ;
                 skos:prefLabel "resonant soft X-ray reflectometry" .


###  http://purl.allotrope.org/ontologies/process#AFP_0000990
af-p:AFP_0000990 rdf:type owl:Class ;
                 rdfs:subClassOf af-p:AFP_0000997 ;
                 skos:altLabel "scanning angle reflectivity" ,
                               "scanning-angle reflectivity" ,
                               "scanning-angle reflectometry" ;
                 skos:definition "A method for determining structure by illuminating an extremely flat surface with visible light and measuring the intensity of light reflected at different angles around the Brewster angle. [CHMO]" ;
                 skos:prefLabel "scanning angle reflectometry" .


###  http://purl.allotrope.org/ontologies/process#AFP_0000997
af-p:AFP_0000997 rdf:type owl:Class ;
                 rdfs:subClassOf af-p:AFP_0000229 ;
                 skos:altLabel "OR" ,
                               "light laser reflectivity" ,
                               "light laser reflectometry" ,
                               "light reflectivity" ,
                               "light reflectometry" ,
                               "optical laser reflectivity" ,
                               "optical reflectivity" ;
                 skos:definition "A method for determining structure by illuminating an extremely flat surface with visible light and measuring the intensity of the reflected light as a function of angle. The reflected light has two polarised components, s (perpendicular) and p (parallel). The reflectivity of s-polarized light depends on the angle of incidence, but the reflectivity of p-polarized light vanishes at the Brewster angle. [CHMO]" ;
                 skos:prefLabel "optical reflectometry" .


###  http://purl.allotrope.org/ontologies/process#AFP_0001058
af-p:AFP_0001058 rdf:type owl:Class ;
                 rdfs:subClassOf af-p:AFP_0001153 ;
                 skos:altLabel "OCDR" ,
                               "OLCR" ,
                               "optical coherence-domain reflectivity" ,
                               "optical low-coherence domain reflectivity" ,
                               "optical low-coherence domain reflectometry" ;
                 skos:definition "A method for determining structure by illuminating an extremely flat surface with visible light and interfering the light reflected from the sample at the Brewster angle with light reflected from a reference mirror. Intereference only occurs when the difference in the optical path lengths between the two mirrors is within the coherence length of the optical source. [CHMO]" ;
                 skos:prefLabel "optical coherence-domain reflectometry" .


###  http://purl.allotrope.org/ontologies/process#AFP_0001076
af-p:AFP_0001076 rdf:type owl:Class ;
                 rdfs:subClassOf af-p:AFP_0001673 ;
                 skos:altLabel "GIXRR" ,
                               "glancing incidence X-ray reflectivity " ,
                               "glancing incidence X-ray reflectometry" ,
                               "glancing incidence XRR" ,
                               "glancing-incidence X-ray reflectivity" ,
                               "glancing-incidence XRR" ;
                 skos:definition "A method for determining structure by directing a beam of X-rays at a low angle (<5 deg) toward an extremely flat surface and measuring the intensity of the reflected X-rays as a function of angle. X-ray reflectometry is used to determine the structure of thin films. [CHMO]" ;
                 skos:prefLabel "glancing-incidence X-ray reflectometry" .


###  http://purl.allotrope.org/ontologies/process#AFP_0001153
af-p:AFP_0001153 rdf:type owl:Class ;
                 rdfs:subClassOf af-p:AFP_0000997 ;
                 skos:altLabel "fixed angle reflectivity" ,
                               "fixed-angle reflectivity" ,
                               "fixed-angle reflectometry" ,
                               "optical fixed angle reflectivity" ,
                               "optical fixed angle reflectometry" ,
                               "optical fixed-angle reflectivity" ,
                               "optical fixed-angle reflectometry" ;
                 skos:definition "A method for determining structure by illuminating an extremely flat surface with visible light and measuring the intensity of the light reflected at the Brewster angle. [CHMO]" ;
                 skos:prefLabel "fixed angle reflectometry" .


###  http://purl.allotrope.org/ontologies/process#AFP_0001167
af-p:AFP_0001167 rdf:type owl:Class ;
                 rdfs:subClassOf af-p:AFP_0000479 ;
                 skos:altLabel "polarised neutron reflection"@en-gb ,
                               "polarised neutron reflectivity"@en-gb ,
                               "spin polarised neutron reflectivity "@en-gb ,
                               "spin-polarised reflection measurements"@en-gb ,
                               "PNR" ,
                               "polarized neutron reflection" ,
                               "polarized neutron reflectivity" ,
                               "spin polarized neutron reflectivity " ,
                               "spin-polarized reflection measurements" ;
                 skos:definition "A method for determining structure by directing polarized neutrons onto an extremely flat surface and measuring the intensity of the reflected neutrons as a function of angle and neutron wavelength. [CHMO]" ;
                 skos:prefLabel "polarised neutron reflectometry"@en-gb ,
                                "polarized neutron reflectometry" .


###  http://purl.allotrope.org/ontologies/process#AFP_0001244
af-p:AFP_0001244 rdf:type owl:Class ;
                 rdfs:subClassOf af-p:AFP_0001673 ;
                 skos:altLabel "RXR" ,
                               "RXRR" ,
                               "relative X-ray reflectivity" ;
                 skos:definition "A method for determining structure by directing a beam of X-rays at an extremely flat surface (at a grazing angle) and measuring the intensity of the reflected X-rays as a function of angle. [CHMO]" ;
                 skos:prefLabel "relative X-ray reflectometry" .


###  http://purl.allotrope.org/ontologies/process#AFP_0001340
af-p:AFP_0001340 rdf:type owl:Class ;
                 rdfs:subClassOf af-p:AFP_0001673 ;
                 skos:altLabel "diffuse X-ray reflectance" ,
                               "diffuse XRR" ,
                               "off-specular X-ray reflectivity" ,
                               "off-specular X-ray reflectometry" ,
                               "off-specular XRR" ,
                               "specular XRR" ;
                 skos:definition "A method for determining structure by directing a beam of X-rays at an extremely flat surface (at angle theta minus omega to the surface) and measuring the intensity of the X-rays which undergo diffuse reflection (and are emitted at angle theta plus omega from the surface). [CHMO]" ;
                 skos:prefLabel "diffuse X-ray reflectometry" .


###  http://purl.allotrope.org/ontologies/process#AFP_0001488
af-p:AFP_0001488 rdf:type owl:Class ;
                 rdfs:subClassOf af-p:AFP_0001153 ;
                 skos:altLabel "SPAR" ,
                               "stagnation point adsorption reflectivity" ;
                 skos:definition "A method for determining structure by illuminating an extremely flat surface with visible light and monitoring the intensity of light reflected at the Brewster angle during the adsorption of particles on the surface. [CHMO]" ;
                 skos:prefLabel "stagnation point adsorption reflectometry" .


###  http://purl.allotrope.org/ontologies/process#AFP_0001665
af-p:AFP_0001665 rdf:type owl:Class ;
                 rdfs:subClassOf af-p:AFP_0001153 ;
                 skos:altLabel "OTDR" ,
                               "optical time domain reflectivity" ,
                               "optical time domain reflectometry" ,
                               "optical time-domain reflectivity" ,
                               "optical time-domain reflectometry" ;
                 skos:definition "A method for determining structure by directing an optical pulse through an optical fibre and measuring the intensity of light reflected at the Brewster angle as a function of time. [CHMO]" ;
                 skos:prefLabel "optical time-domain reflectometry" .


###  http://purl.allotrope.org/ontologies/process#AFP_0001673
af-p:AFP_0001673 rdf:type owl:Class ;
                 rdfs:subClassOf af-p:AFP_0000229 ;
                 skos:altLabel "X-ray reflectivity" ,
                               "XRR" ;
                 skos:definition "A method for determining structure by directing a beam of X-rays at an extremely flat surface and measuring the intensity of the reflected X-rays as a function of angle. X-ray reflectometry is used to determine the structure of thin films. [CHMO]" ;
                 skos:prefLabel "X-ray reflectometry" .


###  http://purl.allotrope.org/ontologies/process#AFP_0001713
af-p:AFP_0001713 rdf:type owl:Class ;
                 rdfs:subClassOf af-p:AFP_0001167 ;
                 skos:altLabel "MCNR" ,
                               "magnetic contrast neutron reflection" ,
                               "magnetic contrast neutron reflectivity" ,
                               "magnetic contrast reflection measurements" ,
                               "magnetic-contrast neutron reflection" ,
                               "magnetic-contrast neutron reflectometry" ,
                               "magnetic-contrast reflection measurements" ;
                 skos:definition "A method for determining structure by directing two beams of polarized neutrons (one spin 'up' and one spin 'down') onto the sample, which contains a ferromagnetic reference layer, and measuring the intensity of the reflected neutrons in the presence of an applied magnetic field. [CHMO]" ;
                 skos:prefLabel "magnetic contrast neutron reflectometry" .


###  http://purl.allotrope.org/ontologies/process#AFP_0002038
af-p:AFP_0002038 rdf:type owl:Class ;
                 rdfs:subClassOf af-p:AFP_0001665 ;
                 skos:altLabel "polarisation OTDR"@en-gb ,
                               "polarisation optical time domain reflectivity"@en-gb ,
                               "polarisation optical time-domain reflectivity"@en-gb ,
                               "polarisation optical time-domain reflectometry"@en-gb ,
                               "PODTR" ,
                               "polarization OTDR" ,
                               "polarization optical time domain reflectivity" ,
                               "polarization optical time-domain reflectivity" ,
                               "polarization optical time-domain reflectometry" ;
                 skos:definition "A method for determining structure by directing an optical pulse through an optical fibre and measuring the polarization state of light reflected at the Brewster angle as a function of time. [CHMO]" ;
                 skos:prefLabel "polarisation optical time domain reflectometry"@en-gb ,
                                "polarization optical time domain reflectometry" .


#################################################################
#    Individuals
#################################################################

###  http://purl.allotrope.org/voc/attribution
<http://purl.allotrope.org/voc/attribution> rdf:type owl:NamedIndividual ,
                                                     dct:RightsStatement ;
                                            dct:description """
These taxonomies contain material or may constitute derivative works of material which may be subject to copyright by one of the following organizations.  By using these taxonomies, you agree to the following terms and conditions applicable to its contents:
******************************************************************************
Copyright Notice and Terms for IUPAC Gold Book
______________________________________________________________________________
Copyright © 1998, Regents of the University of California
All rights reserved.
Redistribution and use in source and binary forms, with or without modification, are permitted provided that the following conditions are met:
1. Redistributions of source code must retain the above copyright notice, this list of conditions and the following disclaimer.
2. Redistributions in binary form must reproduce the above copyright notice, this list of conditions and the following disclaimer in the documentation and/or other materials provided with the distribution.
THIS SOFTWARE IS PROVIDED BY THE COPYRIGHT HOLDERS AND CONTRIBUTORS \"AS IS\" AND ANY EXPRESS OR IMPLIED WARRANTIES, INCLUDING, BUT NOT LIMITED TO, THE IMPLIED WARRANTIES OF MERCHANTABILITY AND FITNESS FOR A PARTICULAR PURPOSE ARE DISCLAIMED. IN NO EVENT SHALL THE COPYRIGHT HOLDER OR CONTRIBUTORS BE LIABLE FOR ANY DIRECT, INDIRECT, INCIDENTAL, SPECIAL, EXEMPLARY, OR CONSEQUENTIAL DAMAGES (INCLUDING, BUT NOT LIMITED TO, PROCUREMENT OF SUBSTITUTE GOODS OR SERVICES; LOSS OF USE, DATA, OR PROFITS; OR BUSINESS INTERRUPTION) HOWEVER CAUSED AND ON ANY THEORY OF LIABILITY, WHETHER IN CONTRACT, STRICT LIABILITY, OR TORT (INCLUDING NEGLIGENCE OR OTHERWISE) ARISING IN ANY WAY OUT OF THE USE OF THIS SOFTWARE, EVEN IF ADVISED OF THE POSSIBILITY OF SUCH DAMAGE.
******************************************************************************
Copyright Notice and Terms for PSI-MS (Proteomics Standards Initiative - Mass Spectrometry) Mass spectrometer output files and spectra interpretation
_____________________________________________________________________________
Created by Matt Chambers, Andreas Bertsch, Marius Kallhardt, Eric Deutsch Fredrik Levander, Pierre-Alain Binz, and Gerhard Mayer. Publisher: HUPO Proteomics Standards Initiative Mass Spectrometry Standards Working Group and HUPO Proteomics Standards Initiative Proteomics Informatics Working Group. This work is used pursuant to a Creative Commons license available here: http://creativecommons.org/licenses/by/3.0/legalcode

******************************************************************************
Attribution Notice for National Center for Biomedical Ontology materials.

This work contains material from the Cell Ontology and Clinical Measurement Ontology, available here: http://bioportal.bioontology.org/.
******************************************************************************
Attribution Notice for ChEBI
This work contains material from the European Bioinformatics Institute’s ChEBI database.
******************************************************************************
Attribution Notice for Quantities Units Dimensions Data Types (http://www.qudt.org/)
This work contains content from www.qudt.org and is used pursuant to a Creative Commons License available here: http://creativecommons.org/licenses/by-sa/3.0/us/legalcode. The original work may have been modified.
******************************************************************************
Copyright and Attribution Notice for Dublin Core Metadata Initiative Document
This work contains material from the following DCMI document used pursuant to a creative commons license available here: https://creativecommons.org/licenses/by/4.0/legalcode. This material may have been modified or changed.
Timestamped URL:          http://dublincore.org/documents/2012/06/14/dcmi-terms/
Date Issued:                       2012-06-14
Document Status:            This is a DCMI Recommendation.
Copyright © 1995-2015 DCMI. All Rights Reserved. DCMI liability, trademark/service mark, document use and software licensing rules apply.
******************************************************************************

""" ;
                                            dct:title "Derivative works attribution" .


###  http://purl.allotrope.org/voc/copyright
<http://purl.allotrope.org/voc/copyright> rdf:type owl:NamedIndividual ,
                                                   dct:RightsStatement ;
                                          dct:description "Copyright © 2019 Allotrope Foundation" ;
                                          dct:rightsHolder <http://www.allotrope.org> ;
                                          dct:title "Copyright © 2019 Allotrope Foundation" .


###  http://purl.allotrope.org/voc/creative-commons-attribution-license
<http://purl.allotrope.org/voc/creative-commons-attribution-license> rdf:type owl:NamedIndividual ,
                                                                              dct:LicenseDocument ;
                                                                     dct:description """This work is licensed under a Creative Commons Attribution 4.0 International License http://creativecommons.org/licenses/by/4.0/.

THESE MATERIALS ARE PROVIDED \"AS IS\" AND ALLOTROPE EXPRESSLY DISCLAIMS ALL WARRANTIES, EXPRESS, IMPLIED OR STATUTORY, INCLUDING, WITHOUT LIMITATION, THE WARRANTIES OF NON-INFRINGEMENT, TITLE, MERCHANTABILITY AND FITNESS FOR A PARTICULAR PURPOSE.

Copyright © 2015-2025 Allotrope Foundation
""" ;
                                                                     dct:title "Creative Commons Attribution 4.0 International Public License" .


###  Generated by the OWL API (version 5.1.19) https://github.com/owlcs/owlapi/
